<?xml version="1.0"?>
<rdf:RDF xmlns="http://standards.iso.org/iso/10303/tech/refdata/core"
     xml:base="http://standards.iso.org/iso/10303/tech/refdata/core"
     xmlns:dc="http://purl.org/dc/elements/1.1/"
     xmlns:owl="http://www.w3.org/2002/07/owl#"
     xmlns:rdf="http://www.w3.org/1999/02/22-rdf-syntax-ns#"
     xmlns:xml="http://www.w3.org/XML/1998/namespace"
     xmlns:xsd="http://www.w3.org/2001/XMLSchema#"
     xmlns:core="http://standards.iso.org/iso/10303/tech/refdata/core#"
     xmlns:rdfs="http://www.w3.org/2000/01/rdf-schema#"
     xmlns:skos="http://www.w3.org/2004/02/skos/core#"
     xmlns:terms="http://purl.org/dc/terms/">
    <owl:Ontology rdf:about="http://standards.iso.org/iso/10303/tech/refdata/core">
        <owl:versionIRI rdf:resource="http://standards.iso.org/iso/10303/tech/refdata/core_v3"/>
        <owl:imports rdf:resource="http://protege.stanford.edu/plugins/owl/dc/protege-dc.owl"/>
        <owl:imports rdf:resource="http://www.w3.org/2004/02/skos/core"/>
        <dc:coverage xml:lang="en">The classifiable objects from the Core_model.</dc:coverage>
        <dc:creator xml:lang="en">Jean Brangé, AFNeT Services</dc:creator>
        <dc:date>2023-10-04</dc:date>
        <dc:language>en</dc:language>
        <dc:source>ISO/TS 10303-4000</dc:source>
        <dc:type>TS</dc:type>
        <rdfs:comment xml:lang="en">This ontology is an OWL representation of the classes derived from ISO/TS 10303-4000 edition 3.</rdfs:comment>
        <rdfs:seeAlso rdf:resource="http://www.w3.org/TR/skos-reference/"/>
        <owl:priorVersion rdf:resource="http://standards.iso.org/iso/10303/tech/refdata/core_v2"/>
        <owl:versionInfo>3</owl:versionInfo>
        <skos:note>ISO/TC 184/SC 4/WG12 N11131</skos:note>
    </owl:Ontology>
    


    <!-- 
    ///////////////////////////////////////////////////////////////////////////////////////
    //
    // Annotation properties
    //
    ///////////////////////////////////////////////////////////////////////////////////////
     -->

    


    <!-- http://purl.org/dc/elements/1.1/contributor -->

    <owl:AnnotationProperty rdf:about="http://purl.org/dc/elements/1.1/contributor"/>
    


    <!-- http://purl.org/dc/elements/1.1/creator -->

    <owl:AnnotationProperty rdf:about="http://purl.org/dc/elements/1.1/creator"/>
    


    <!-- http://purl.org/dc/elements/1.1/date -->

    <owl:AnnotationProperty rdf:about="http://purl.org/dc/elements/1.1/date"/>
    


    <!-- http://purl.org/dc/elements/1.1/source -->

    <owl:AnnotationProperty rdf:about="http://purl.org/dc/elements/1.1/source"/>
    


    <!-- http://purl.org/dc/elements/1.1/type -->

    <owl:AnnotationProperty rdf:about="http://purl.org/dc/elements/1.1/type"/>
    


    <!-- 
    ///////////////////////////////////////////////////////////////////////////////////////
    //
    // Classes
    //
    ///////////////////////////////////////////////////////////////////////////////////////
     -->

    


    <!-- http://standards.iso.org/iso/10303/tech/refdata/core#STEPThing -->

    <owl:Class rdf:about="http://standards.iso.org/iso/10303/tech/refdata/core#STEPThing">
        <dc:creator>STEP Harmonization Team</dc:creator>
        <dc:date>2021-07-30</dc:date>
        <dc:source>ISO/TS 10303-4000</dc:source>
        <owl:versionInfo>1</owl:versionInfo>
    </owl:Class>
    


    <!-- http://standards.iso.org/iso/10303/tech/refdata/core#a014de90-130a-0135-b552-598f1b1392ae -->

    <owl:Class rdf:about="http://standards.iso.org/iso/10303/tech/refdata/core#a014de90-130a-0135-b552-598f1b1392ae">
        <rdfs:subClassOf rdf:resource="http://standards.iso.org/iso/10303/tech/refdata/core#c6260c30-130a-0135-b552-598f1b1392ae"/>
        <dc:contributor>STEP Harmonization Team</dc:contributor>
        <dc:creator>Phil Spiby, Eurostep</dc:creator>
        <dc:date>2022-09-01</dc:date>
        <dc:source>ISO/TS 10303-4000</dc:source>
        <dc:type>InWork</dc:type>
        <rdfs:comment xml:lang="en">A GeometricRepresentationRelationship is an abstract type of RepresentationRelationship that specifies a relationship between a ComposedGeometricModel and an item (specified by GeometricRepresentationSelect).</rdfs:comment>
        <owl:versionInfo>2</owl:versionInfo>
        <skos:changeNote>[2021-07-30] Initial definition.</skos:changeNote>
        <skos:changeNote>[2022-09-01] Phil Spiby, Eurostep: updated comment.</skos:changeNote>
        <skos:prefLabel xml:lang="en">geometric representation relationship</skos:prefLabel>
    </owl:Class>
    


    <!-- http://standards.iso.org/iso/10303/tech/refdata/core#a031dc70-130a-0135-b552-598f1b1392ae -->

    <owl:Class rdf:about="http://standards.iso.org/iso/10303/tech/refdata/core#a031dc70-130a-0135-b552-598f1b1392ae">
        <rdfs:subClassOf rdf:resource="http://standards.iso.org/iso/10303/tech/refdata/core#a014de90-130a-0135-b552-598f1b1392ae"/>
        <dc:contributor>STEP Harmonization Team</dc:contributor>
        <dc:creator>Phil Spiby, Eurostep</dc:creator>
        <dc:date>2022-09-01</dc:date>
        <dc:source>ISO/TS 10303-4000</dc:source>
        <dc:type>InWork</dc:type>
        <rdfs:comment xml:lang="en">A GeometricRepresentationRelationshipWithCartesianTransformation is a type of GeometricRepresentationRelationship that specifies a CartesianTransformation between the two GeometricCoordinateSpaces of the referenced GeometricModels.</rdfs:comment>
        <owl:versionInfo>1</owl:versionInfo>
        <skos:changeNote>[2021-07-30] Initial definition.</skos:changeNote>
        <skos:prefLabel xml:lang="en">geometric representation relationship with cartesian transformation</skos:prefLabel>
    </owl:Class>
    


    <!-- http://standards.iso.org/iso/10303/tech/refdata/core#a05da760-130a-0135-b552-598f1b1392ae -->

    <owl:Class rdf:about="http://standards.iso.org/iso/10303/tech/refdata/core#a05da760-130a-0135-b552-598f1b1392ae">
        <rdfs:subClassOf rdf:resource="http://standards.iso.org/iso/10303/tech/refdata/core#a014de90-130a-0135-b552-598f1b1392ae"/>
        <dc:contributor>STEP Harmonization Team</dc:contributor>
        <dc:creator>Phil Spiby, Eurostep</dc:creator>
        <dc:date>2022-09-01</dc:date>
        <dc:source>ISO/TS 10303-4000</dc:source>
        <dc:type>InWork</dc:type>
        <rdfs:comment xml:lang="en">A GeometricRepresentationRelationshipWithPlacementTransformation is a type of GeometricRepresentationRelationship that specifies a placement transformation by associating two AxisPlacements of the referenced GeometricModels onto each other.</rdfs:comment>
        <owl:versionInfo>1</owl:versionInfo>
        <skos:changeNote>[2021-07-30] Initial definition.</skos:changeNote>
        <skos:prefLabel xml:lang="en">geometric representation relationship with placement transformation</skos:prefLabel>
    </owl:Class>
    


    <!-- http://standards.iso.org/iso/10303/tech/refdata/core#a0791ea0-130a-0135-b552-598f1b1392ae -->

    <owl:Class rdf:about="http://standards.iso.org/iso/10303/tech/refdata/core#a0791ea0-130a-0135-b552-598f1b1392ae">
        <rdfs:subClassOf rdf:resource="http://standards.iso.org/iso/10303/tech/refdata/core#a014de90-130a-0135-b552-598f1b1392ae"/>
        <dc:contributor>STEP Harmonization Team</dc:contributor>
        <dc:creator>Phil Spiby, Eurostep</dc:creator>
        <dc:date>2022-09-01</dc:date>
        <dc:source>ISO/TS 10303-4000</dc:source>
        <dc:type>InWork</dc:type>
        <rdfs:comment xml:lang="en">A GeometricRepresentationRelationshipWithSameCoordinateSpace is a type of GeometricRepresentationRelationship without a geometry transformation between the Related and the Relating GeometricModels.</rdfs:comment>
        <owl:versionInfo>1</owl:versionInfo>
        <skos:changeNote>[2021-07-30] Initial definition.</skos:changeNote>
        <skos:prefLabel xml:lang="en">geometric representation relationship with same coordinate space</skos:prefLabel>
    </owl:Class>
    


    <!-- http://standards.iso.org/iso/10303/tech/refdata/core#a0a0cae0-130a-0135-b552-598f1b1392ae -->

    <owl:Class rdf:about="http://standards.iso.org/iso/10303/tech/refdata/core#a0a0cae0-130a-0135-b552-598f1b1392ae">
        <rdfs:subClassOf rdf:resource="http://standards.iso.org/iso/10303/tech/refdata/core#9e16c4a0-130a-0135-b552-598f1b1392ae"/>
        <dc:contributor>STEP Harmonization Team</dc:contributor>
        <dc:creator>Phil Spiby, Eurostep</dc:creator>
        <dc:date>2022-09-01</dc:date>
        <dc:source>ISO/TS 10303-4000</dc:source>
        <dc:type>InWork</dc:type>
        <rdfs:comment xml:lang="en">A Hardcopy is a type of File that is the actual physical object representing a DocumentVersion. It could be a stack of paper consisting of one or more sheets, on which some product data is written, printed or plotted.</rdfs:comment>
        <owl:versionInfo>1</owl:versionInfo>
        <skos:changeNote>[2021-07-30] Initial definition.</skos:changeNote>
        <skos:prefLabel xml:lang="en">hardcopy</skos:prefLabel>
    </owl:Class>
    


    <!-- http://standards.iso.org/iso/10303/tech/refdata/core#a0bf538a-5690-4511-a4e8-b1a1eb6375da -->

    <owl:Class rdf:about="http://standards.iso.org/iso/10303/tech/refdata/core#a0bf538a-5690-4511-a4e8-b1a1eb6375da">
        <rdfs:subClassOf rdf:resource="http://standards.iso.org/iso/10303/tech/refdata/core#STEPThing"/>
        <dc:contributor>STEP Harmonization Team</dc:contributor>
        <dc:creator>Phil Spiby, Eurostep</dc:creator>
        <dc:date>2022-09-01</dc:date>
        <dc:source>ISO/TS 10303-4000</dc:source>
        <dc:type>InWork</dc:type>
        <rdfs:comment xml:lang="en">A Location is a place where an activity or event can occur, or where a product or resource can exist.</rdfs:comment>
        <owl:versionInfo>1</owl:versionInfo>
        <skos:changeNote>[2021-07-30] Initial definition.</skos:changeNote>
        <skos:prefLabel xml:lang="en">location</skos:prefLabel>
    </owl:Class>
    


    <!-- http://standards.iso.org/iso/10303/tech/refdata/core#a187f29f-5cbd-4ff3-b1dc-bdd9f2ceb596 -->

    <owl:Class rdf:about="http://standards.iso.org/iso/10303/tech/refdata/core#a187f29f-5cbd-4ff3-b1dc-bdd9f2ceb596">
        <rdfs:subClassOf rdf:resource="http://standards.iso.org/iso/10303/tech/refdata/core#59b11220-3279-0135-b58f-598f1b1392ae"/>
        <dc:contributor>STEP Harmonization Team</dc:contributor>
        <dc:creator>Phil Spiby, Eurostep</dc:creator>
        <dc:date>2022-09-01</dc:date>
        <dc:source>ISO/TS 10303-4000</dc:source>
        <dc:type>InWork</dc:type>
        <rdfs:comment xml:lang="en">A JustificationRelationship is a relationship between two Justification objects.</rdfs:comment>
        <owl:versionInfo>2</owl:versionInfo>
        <skos:changeNote>[2021-07-30] Initial definition.</skos:changeNote>
        <skos:changeNote>[2022-09-01] Phil Spiby, Eurostep: updated comment.</skos:changeNote>
        <skos:prefLabel xml:lang="en">justification relationship</skos:prefLabel>
    </owl:Class>
    


    <!-- http://standards.iso.org/iso/10303/tech/refdata/core#a1967580-130a-0135-b552-598f1b1392ae -->

    <owl:Class rdf:about="http://standards.iso.org/iso/10303/tech/refdata/core#a1967580-130a-0135-b552-598f1b1392ae">
        <rdfs:subClassOf rdf:resource="http://standards.iso.org/iso/10303/tech/refdata/core#STEPThing"/>
        <dc:contributor>STEP Harmonization Team</dc:contributor>
        <dc:creator>Phil Spiby, Eurostep</dc:creator>
        <dc:date>2022-09-01</dc:date>
        <dc:source>ISO/TS 10303-4000</dc:source>
        <dc:type>InWork</dc:type>
        <rdfs:comment xml:lang="en">An Identifier is a mechanism to provide the identifying name or code for the activity or product data.</rdfs:comment>
        <owl:versionInfo>1</owl:versionInfo>
        <skos:changeNote>[2021-07-30] Initial definition.</skos:changeNote>
        <skos:prefLabel xml:lang="en">identifier</skos:prefLabel>
    </owl:Class>
    


    <!-- http://standards.iso.org/iso/10303/tech/refdata/core#a1e2c0c0-130a-0135-b552-598f1b1392ae -->

    <owl:Class rdf:about="http://standards.iso.org/iso/10303/tech/refdata/core#a1e2c0c0-130a-0135-b552-598f1b1392ae">
        <rdfs:subClassOf rdf:resource="http://standards.iso.org/iso/10303/tech/refdata/core#59b11220-3279-0135-b58f-598f1b1392ae"/>
        <dc:contributor>STEP Harmonization Team</dc:contributor>
        <dc:creator>Phil Spiby, Eurostep</dc:creator>
        <dc:date>2022-09-01</dc:date>
        <dc:source>ISO/TS 10303-4000</dc:source>
        <dc:type>InWork</dc:type>
        <rdfs:comment xml:lang="en">An IdentifierRelationship is a relationship between two Identifier objects.</rdfs:comment>
        <owl:versionInfo>1</owl:versionInfo>
        <skos:changeNote>[2021-07-30] Initial definition.</skos:changeNote>
        <skos:prefLabel xml:lang="en">identifier relationship</skos:prefLabel>
    </owl:Class>
    


    <!-- http://standards.iso.org/iso/10303/tech/refdata/core#a2321940-130a-0135-b552-598f1b1392ae -->

    <owl:Class rdf:about="http://standards.iso.org/iso/10303/tech/refdata/core#a2321940-130a-0135-b552-598f1b1392ae">
        <rdfs:subClassOf rdf:resource="http://standards.iso.org/iso/10303/tech/refdata/core#59b11220-3279-0135-b58f-598f1b1392ae"/>
        <dc:contributor>STEP Harmonization Team</dc:contributor>
        <dc:creator>Phil Spiby, Eurostep</dc:creator>
        <dc:date>2022-09-01</dc:date>
        <dc:source>ISO/TS 10303-4000</dc:source>
        <dc:type>InWork</dc:type>
        <rdfs:comment xml:lang="en">An IndividualAssemblyRelationship is either a relation between two IndividualPartView objects representing a view of the assembly (both related objects shall share at least one ViewContext) or a relation between an IndividualPartView and a PartView with an optional quantity.</rdfs:comment>
        <owl:versionInfo>2</owl:versionInfo>
        <skos:changeNote>[2021-07-30] Initial definition.</skos:changeNote>
        <skos:changeNote>[2022-09-01] Phil Spiby, Eurostep: updated comment updated example.</skos:changeNote>
        <skos:example xml:lang="en">An individual vehicle can be represented as being filled with fuel using a PartView for the grade or supplier part of fuel and a Quantity to specify how much fuel has been used.</skos:example>
        <skos:prefLabel xml:lang="en">individual assembly relationship</skos:prefLabel>
    </owl:Class>
    


    <!-- http://standards.iso.org/iso/10303/tech/refdata/core#a236446d-6e48-41ab-b5a3-dcce1a4ee3a1 -->

    <owl:Class rdf:about="http://standards.iso.org/iso/10303/tech/refdata/core#a236446d-6e48-41ab-b5a3-dcce1a4ee3a1">
        <rdfs:subClassOf rdf:resource="http://standards.iso.org/iso/10303/tech/refdata/core#1cfca290-3279-0135-b58f-598f1b1392ae"/>
        <dc:contributor>STEP Harmonization Team</dc:contributor>
        <dc:creator>Phil Spiby, Eurostep</dc:creator>
        <dc:date>2022-09-01</dc:date>
        <dc:source>ISO/TS 10303-4000</dc:source>
        <dc:type>InWork</dc:type>
        <rdfs:comment xml:lang="en">An AnalysisAssignment is an assignment of an Analysis to an item (specified by AnalysisAssignmentSelect) being analyzed.</rdfs:comment>
        <owl:versionInfo>1</owl:versionInfo>
        <skos:changeNote>[2021-07-30] Initial definition.</skos:changeNote>
        <skos:prefLabel xml:lang="en">analysis assignment</skos:prefLabel>
    </owl:Class>
    


    <!-- http://standards.iso.org/iso/10303/tech/refdata/core#a25ff3eb-4e00-4730-a576-3ed5f557a2a6 -->

    <owl:Class rdf:about="http://standards.iso.org/iso/10303/tech/refdata/core#a25ff3eb-4e00-4730-a576-3ed5f557a2a6">
        <rdfs:subClassOf rdf:resource="http://standards.iso.org/iso/10303/tech/refdata/core#68242b94-82e8-4841-8005-89981113e22f"/>
        <dc:contributor>STEP Harmonization Team</dc:contributor>
        <dc:creator>Phil Spiby, Eurostep</dc:creator>
        <dc:date>2022-09-01</dc:date>
        <dc:source>ISO/TS 10303-4000</dc:source>
        <dc:type>InWork</dc:type>
        <rdfs:comment xml:lang="en">A GlobalPositionLocation is a type of Locator specified through the identification of location on Earth using the geographical coordinates. These coordinates refer to a world geodesic system.</rdfs:comment>
        <owl:versionInfo>1</owl:versionInfo>
        <skos:changeNote>[2021-07-30] Initial definition.</skos:changeNote>
        <skos:prefLabel xml:lang="en">global position location</skos:prefLabel>
    </owl:Class>
    


    <!-- http://standards.iso.org/iso/10303/tech/refdata/core#a2719b60-dbf3-48e7-be31-ebb8c09491de -->

    <owl:Class rdf:about="http://standards.iso.org/iso/10303/tech/refdata/core#a2719b60-dbf3-48e7-be31-ebb8c09491de">
        <rdfs:subClassOf rdf:resource="http://standards.iso.org/iso/10303/tech/refdata/core#STEPThing"/>
        <dc:contributor>STEP Harmonization Team</dc:contributor>
        <dc:creator>Phil Spiby, Eurostep</dc:creator>
        <dc:date>2022-09-01</dc:date>
        <dc:source>ISO/TS 10303-4000</dc:source>
        <dc:type>InWork</dc:type>
        <rdfs:comment xml:lang="en">A ResourceEvent is an abstract generalization of instances that represents an event or action that affects the balance or availability of a managed resource. A ResourceEvent is the role of a resource event is determined by which is specified by the ClassifiedAs property.</rdfs:comment>
        <owl:versionInfo>2</owl:versionInfo>
        <skos:changeNote>[2021-07-30] Initial definition.</skos:changeNote>
        <skos:changeNote>[2022-09-01] Phil Spiby, Eurostep: updated comment updated example.</skos:changeNote>
        <skos:example xml:lang="en">A resource event can be classified as &quot;Planned&quot; or &quot;Actual&quot;.</skos:example>
        <skos:note xml:lang="en">Only non-abstract specializations of the ResourceEvent can be instantiated.</skos:note>
        <skos:prefLabel xml:lang="en">resource event</skos:prefLabel>
    </owl:Class>
    


    <!-- http://standards.iso.org/iso/10303/tech/refdata/core#a28912e0-130a-0135-b552-598f1b1392ae -->

    <owl:Class rdf:about="http://standards.iso.org/iso/10303/tech/refdata/core#a28912e0-130a-0135-b552-598f1b1392ae">
        <rdfs:subClassOf rdf:resource="http://standards.iso.org/iso/10303/tech/refdata/core#STEPThing"/>
        <dc:contributor>STEP Harmonization Team</dc:contributor>
        <dc:creator>Phil Spiby, Eurostep</dc:creator>
        <dc:date>2022-09-01</dc:date>
        <dc:source>ISO/TS 10303-4000</dc:source>
        <dc:type>InWork</dc:type>
        <rdfs:comment xml:lang="en">An IndividualPart is the identification of an individual artefact that has been made or is planned to be made. It is a collector of data common to all versions of the IndividualPart.</rdfs:comment>
        <owl:versionInfo>2</owl:versionInfo>
        <skos:changeNote>[2021-07-30] Initial definition.</skos:changeNote>
        <skos:changeNote>[2022-09-01] Phil Spiby, Eurostep: updated example updated note.</skos:changeNote>
        <skos:example xml:lang="en">The design of a personal computer is represented by a PartVersion.</skos:example>
        <skos:example xml:lang="en">The personal computer that has been ordered, allocated a serial number for manufacturing planning, but not yet manufactured, is represented by an IndividualPartVersion. An actual personal computer, also represented by an IndividualPartVersion, can be linked to the planed personal computer by an IndividualPartVersionRelationship object.</skos:example>
        <skos:example xml:lang="en">The personal computer with a serial number on a person&apos;s desk is represented by an IndividualPartVersion.</skos:example>
        <skos:note xml:lang="en">It is likely, but not essential, that the artefact was or will be made from a part design. The part design will be represented by a PartVersion which will be related to the IndividualPart by PartToIndividualPartAssociation.</skos:note>
        <skos:note xml:lang="en">Many physical parts can be produced from a given design. A single Part can lead to many IndividualPart objects.</skos:note>
        <skos:note xml:lang="en">Versions (IndividualPartVersion) of IndividualPart are used to represent whether an individual artefact is planned to be made or has already been made.</skos:note>
        <skos:note xml:lang="en">Where physical parts are being represented, an IndividualPart represents the planned or actual physical realization of a part.</skos:note>
        <skos:prefLabel xml:lang="en">individual part</skos:prefLabel>
    </owl:Class>
    


    <!-- http://standards.iso.org/iso/10303/tech/refdata/core#a289626f-a7fa-4a49-a802-bff9d5372f66 -->

    <owl:Class rdf:about="http://standards.iso.org/iso/10303/tech/refdata/core#a289626f-a7fa-4a49-a802-bff9d5372f66">
        <rdfs:subClassOf rdf:resource="http://standards.iso.org/iso/10303/tech/refdata/core#83b2a250-130a-0135-b552-598f1b1392ae"/>
        <dc:contributor>STEP Harmonization Team</dc:contributor>
        <dc:creator>Phil Spiby, Eurostep</dc:creator>
        <dc:date>2022-09-01</dc:date>
        <dc:source>ISO/TS 10303-4000</dc:source>
        <dc:type>InWork</dc:type>
        <rdfs:comment xml:lang="en">A SchemeVersionAssignment is an assignment of a SchemeVersion to an item (specified by SchemeVersionAssignmentSelect). The meaning of the assignment can be specified using the ClassifiedAs attribute inherited from the AssignmentObject.</rdfs:comment>
        <owl:versionInfo>1</owl:versionInfo>
        <skos:changeNote>[2022-09-01] Initial definition.</skos:changeNote>
        <skos:prefLabel xml:lang="en">scheme version assignment</skos:prefLabel>
    </owl:Class>
    


    <!-- http://standards.iso.org/iso/10303/tech/refdata/core#a2c4788d-72bb-4784-b74f-c8a344e9a39d -->

    <owl:Class rdf:about="http://standards.iso.org/iso/10303/tech/refdata/core#a2c4788d-72bb-4784-b74f-c8a344e9a39d">
        <rdfs:subClassOf rdf:resource="http://standards.iso.org/iso/10303/tech/refdata/core#59b11220-3279-0135-b58f-598f1b1392ae"/>
        <dc:contributor>STEP Harmonization Team</dc:contributor>
        <dc:creator>Phil Spiby, Eurostep</dc:creator>
        <dc:date>2022-09-01</dc:date>
        <dc:source>ISO/TS 10303-4000</dc:source>
        <dc:type>InWork</dc:type>
        <rdfs:comment xml:lang="en">A SystemViewRelationship is a relationship between two instances of SystemView. Unless specified in a specialization of this object, this relationship does not involve inheritance of data between the two related objects.</rdfs:comment>
        <owl:versionInfo>1</owl:versionInfo>
        <skos:changeNote>[2022-09-01] Initial definition.</skos:changeNote>
        <skos:prefLabel xml:lang="en">system view relationship</skos:prefLabel>
    </owl:Class>
    


    <!-- http://standards.iso.org/iso/10303/tech/refdata/core#a2f25c00-130a-0135-b552-598f1b1392ae -->

    <owl:Class rdf:about="http://standards.iso.org/iso/10303/tech/refdata/core#a2f25c00-130a-0135-b552-598f1b1392ae">
        <rdfs:subClassOf rdf:resource="http://standards.iso.org/iso/10303/tech/refdata/core#59b11220-3279-0135-b58f-598f1b1392ae"/>
        <dc:contributor>STEP Harmonization Team</dc:contributor>
        <dc:creator>Phil Spiby, Eurostep</dc:creator>
        <dc:date>2022-09-01</dc:date>
        <dc:source>ISO/TS 10303-4000</dc:source>
        <dc:type>InWork</dc:type>
        <rdfs:comment xml:lang="en">An IndividualPartRelationship is a relationship between two IndividualPart objects.</rdfs:comment>
        <owl:versionInfo>1</owl:versionInfo>
        <skos:changeNote>[2021-07-30] Initial definition.</skos:changeNote>
        <skos:prefLabel xml:lang="en">individual part relationship</skos:prefLabel>
    </owl:Class>
    


    <!-- http://standards.iso.org/iso/10303/tech/refdata/core#a3571140-130a-0135-b552-598f1b1392ae -->

    <owl:Class rdf:about="http://standards.iso.org/iso/10303/tech/refdata/core#a3571140-130a-0135-b552-598f1b1392ae">
        <rdfs:subClassOf rdf:resource="http://standards.iso.org/iso/10303/tech/refdata/core#STEPThing"/>
        <dc:contributor>STEP Harmonization Team</dc:contributor>
        <dc:creator>Phil Spiby, Eurostep</dc:creator>
        <dc:date>2022-09-01</dc:date>
        <dc:source>ISO/TS 10303-4000</dc:source>
        <dc:type>InWork</dc:type>
        <rdfs:comment xml:lang="en">An IndividualPartVersion is a version of an IndividualPart and acts as a collector of the views of this version.</rdfs:comment>
        <owl:versionInfo>2</owl:versionInfo>
        <skos:changeNote>[2021-07-30] Initial definition.</skos:changeNote>
        <skos:changeNote>[2022-09-01] Phil Spiby, Eurostep: updated example.</skos:changeNote>
        <skos:example xml:lang="en">The car on my drive is represented by an IndividualPart. The current configuration status of the car can be represented by an IndividualPartVersion related to that IndividualPart. If a safety modification is made to the car resulting in a new configuration status of the car, then this can be represented by a new IndividualPartVersion.</skos:example>
        <skos:prefLabel xml:lang="en">individual part version</skos:prefLabel>
    </owl:Class>
    


    <!-- http://standards.iso.org/iso/10303/tech/refdata/core#a39af5bb-97a7-4d7e-9dfb-5685e8570785 -->

    <owl:Class rdf:about="http://standards.iso.org/iso/10303/tech/refdata/core#a39af5bb-97a7-4d7e-9dfb-5685e8570785">
        <rdfs:subClassOf rdf:resource="http://standards.iso.org/iso/10303/tech/refdata/core#66348150-092a-4eb7-9561-0b83adfa15ff"/>
        <dc:contributor>STEP Harmonization Team</dc:contributor>
        <dc:creator>Jean Brangé, AFNeT Services</dc:creator>
        <dc:date>2023-10-04</dc:date>
        <dc:source>ISO/TS 10303-4000</dc:source>
        <dc:type>InWork</dc:type>
        <rdfs:comment xml:lang="en">A Datum is a type of ShapeElement from which dimensions and tolerances are referenced. This ShapeElement may, but need not, coincide with the boundary defining the product. A Datum is a datum as specified in ISO 5459. The application of Datum shall conform to the requirements of ISO 5459.</rdfs:comment>
        <owl:versionInfo>3</owl:versionInfo>
        <skos:changeNote>[2023-10-04] Jean Brangé, AFNeT Services: Initial definition.</skos:changeNote>
        <skos:note xml:lang="en">A Datum is a theoretically exact point, straight line, or plane used as a reference for locating and orienting tolerance zones.</skos:note>
        <skos:note xml:lang="en">The use and application of a group of features to establish a Datum is identified in ISO 5459. The group of features is established by using ShapeElementRelationship objects. The concept of a group of ShapeElements is defined in CompositeShapeElement.</skos:note>
        <skos:prefLabel xml:lang="en">datum</skos:prefLabel>
    </owl:Class>
    


    <!-- http://standards.iso.org/iso/10303/tech/refdata/core#a3c3b5c0-130a-0135-b552-598f1b1392ae -->

    <owl:Class rdf:about="http://standards.iso.org/iso/10303/tech/refdata/core#a3c3b5c0-130a-0135-b552-598f1b1392ae">
        <rdfs:subClassOf rdf:resource="http://standards.iso.org/iso/10303/tech/refdata/core#59b11220-3279-0135-b58f-598f1b1392ae"/>
        <dc:contributor>STEP Harmonization Team</dc:contributor>
        <dc:creator>Phil Spiby, Eurostep</dc:creator>
        <dc:date>2022-09-01</dc:date>
        <dc:source>ISO/TS 10303-4000</dc:source>
        <dc:type>InWork</dc:type>
        <rdfs:comment xml:lang="en">An IndividualPartVersionRelationship is a relationship between two IndividualPartVersion objects. Unless specified in a specialization of this object, this relationship does not involve inheritance of data between the two related objects.</rdfs:comment>
        <owl:versionInfo>2</owl:versionInfo>
        <skos:changeNote>[2021-07-30] Initial definition.</skos:changeNote>
        <skos:changeNote>[2022-09-01] Phil Spiby, Eurostep: updated comment.</skos:changeNote>
        <skos:prefLabel xml:lang="en">individual part version relationship</skos:prefLabel>
    </owl:Class>
    


    <!-- http://standards.iso.org/iso/10303/tech/refdata/core#a41f4340-130a-0135-b552-598f1b1392ae -->

    <owl:Class rdf:about="http://standards.iso.org/iso/10303/tech/refdata/core#a41f4340-130a-0135-b552-598f1b1392ae">
        <rdfs:subClassOf rdf:resource="http://standards.iso.org/iso/10303/tech/refdata/core#STEPThing"/>
        <dc:contributor>STEP Harmonization Team</dc:contributor>
        <dc:creator>Phil Spiby, Eurostep</dc:creator>
        <dc:date>2022-09-01</dc:date>
        <dc:source>ISO/TS 10303-4000</dc:source>
        <dc:type>InWork</dc:type>
        <rdfs:comment xml:lang="en">An IndividualPartView is a characterization view of a version of an IndividualPart.</rdfs:comment>
        <owl:versionInfo>1</owl:versionInfo>
        <skos:changeNote>[2021-07-30] Initial definition.</skos:changeNote>
        <skos:note xml:lang="en">The IndividualPartView supports the representation of different views of an IndividualPart for different purposes. Multiple views of the same IndividualPart are represented by different instances of IndividualPartView for the same IndividualPartVersion.</skos:note>
        <skos:prefLabel xml:lang="en">individual part view</skos:prefLabel>
    </owl:Class>
    


    <!-- http://standards.iso.org/iso/10303/tech/refdata/core#a4c532ef-e6ef-45eb-9fae-3e047c967cea -->

    <owl:Class rdf:about="http://standards.iso.org/iso/10303/tech/refdata/core#a4c532ef-e6ef-45eb-9fae-3e047c967cea">
        <rdfs:subClassOf rdf:resource="http://standards.iso.org/iso/10303/tech/refdata/core#ff04d2c5-cea4-41a6-be35-821c1495d8ba"/>
        <dc:contributor>STEP Harmonization Team</dc:contributor>
        <dc:creator>Phil Spiby, Eurostep</dc:creator>
        <dc:date>2022-09-01</dc:date>
        <dc:source>ISO/TS 10303-4000</dc:source>
        <dc:type>InWork</dc:type>
        <rdfs:comment xml:lang="en">A DecisionPoint is a type of StructuredTaskElement. It requires a decision that determines which further TaskElement is to be followed.</rdfs:comment>
        <owl:versionInfo>1</owl:versionInfo>
        <skos:changeNote>[2021-07-30] Initial definition.</skos:changeNote>
        <skos:note xml:lang="en">The condition on which the decision is based optionally allows a further TaskElement to be invoked to provide the basis for the decision.</skos:note>
        <skos:prefLabel xml:lang="en">decision point</skos:prefLabel>
    </owl:Class>
    


    <!-- http://standards.iso.org/iso/10303/tech/refdata/core#a4d96b80-130a-0135-b552-598f1b1392ae -->

    <owl:Class rdf:about="http://standards.iso.org/iso/10303/tech/refdata/core#a4d96b80-130a-0135-b552-598f1b1392ae">
        <rdfs:subClassOf rdf:resource="http://standards.iso.org/iso/10303/tech/refdata/core#59b11220-3279-0135-b58f-598f1b1392ae"/>
        <dc:contributor>STEP Harmonization Team</dc:contributor>
        <dc:creator>Phil Spiby, Eurostep</dc:creator>
        <dc:date>2022-09-01</dc:date>
        <dc:source>ISO/TS 10303-4000</dc:source>
        <dc:type>InWork</dc:type>
        <rdfs:comment xml:lang="en">An IndividualPartViewRelationship is a relation between two IndividualPartView objects.</rdfs:comment>
        <owl:versionInfo>2</owl:versionInfo>
        <skos:changeNote>[2021-07-30] Initial definition.</skos:changeNote>
        <skos:changeNote>[2022-09-01] Phil Spiby, Eurostep: updated comment.</skos:changeNote>
        <skos:prefLabel xml:lang="en">individual part view relationship</skos:prefLabel>
    </owl:Class>
    


    <!-- http://standards.iso.org/iso/10303/tech/refdata/core#a53fa760-130a-0135-b552-598f1b1392ae -->

    <owl:Class rdf:about="http://standards.iso.org/iso/10303/tech/refdata/core#a53fa760-130a-0135-b552-598f1b1392ae">
        <rdfs:subClassOf rdf:resource="http://standards.iso.org/iso/10303/tech/refdata/core#STEPThing"/>
        <dc:contributor>STEP Harmonization Team</dc:contributor>
        <dc:creator>Phil Spiby, Eurostep</dc:creator>
        <dc:date>2022-09-01</dc:date>
        <dc:source>ISO/TS 10303-4000</dc:source>
        <dc:type>InWork</dc:type>
        <rdfs:comment xml:lang="en">An InformationRight is a definition of what can or cannot be done with an item of information in the sense of legal rights and obligations.</rdfs:comment>
        <owl:versionInfo>2</owl:versionInfo>
        <skos:changeNote>[2021-07-30] Initial definition.</skos:changeNote>
        <skos:changeNote>[2022-09-01] Phil Spiby, Eurostep: updated comment updated example.</skos:changeNote>
        <skos:example xml:lang="en">Copyright is an InformationRight.</skos:example>
        <skos:example xml:lang="en">For the purposes of developing a new system, details of government furnished equipment can be made available to a specific project team. The team can copy and use the information internally, but cannot pass it on, either to a third part, or to another team, and has to destroy the information at the end of the contract.</skos:example>
        <skos:note xml:lang="en">The following additional data can be assigned to an InformationRight: InformationUsageRight.</skos:note>
        <skos:prefLabel xml:lang="en">information right</skos:prefLabel>
    </owl:Class>
    


    <!-- http://standards.iso.org/iso/10303/tech/refdata/core#a57f0907-bedc-466d-81b0-3a2da1066a52 -->

    <owl:Class rdf:about="http://standards.iso.org/iso/10303/tech/refdata/core#a57f0907-bedc-466d-81b0-3a2da1066a52">
        <rdfs:subClassOf rdf:resource="http://standards.iso.org/iso/10303/tech/refdata/core#95f1bde5-b263-4ca1-89df-33e1205800dd"/>
        <dc:contributor>STEP Harmonization Team</dc:contributor>
        <dc:creator>Phil Spiby, Eurostep</dc:creator>
        <dc:date>2022-09-01</dc:date>
        <dc:source>ISO/TS 10303-4000</dc:source>
        <dc:type>InWork</dc:type>
        <rdfs:comment xml:lang="en">A TaskInvocation is a type of TaskElement. It is an instruction to perform another task.</rdfs:comment>
        <owl:versionInfo>1</owl:versionInfo>
        <skos:changeNote>[2021-07-30] Initial definition.</skos:changeNote>
        <skos:example xml:lang="en">A TaskElement calls a predefined task to perform an instrument calibration.</skos:example>
        <skos:prefLabel xml:lang="en">task invocation</skos:prefLabel>
    </owl:Class>
    


    <!-- http://standards.iso.org/iso/10303/tech/refdata/core#a5890c70-130a-0135-b552-598f1b1392ae -->

    <owl:Class rdf:about="http://standards.iso.org/iso/10303/tech/refdata/core#a5890c70-130a-0135-b552-598f1b1392ae">
        <rdfs:subClassOf rdf:resource="http://standards.iso.org/iso/10303/tech/refdata/core#STEPThing"/>
        <dc:contributor>STEP Harmonization Team</dc:contributor>
        <dc:creator>Phil Spiby, Eurostep</dc:creator>
        <dc:date>2022-09-01</dc:date>
        <dc:source>ISO/TS 10303-4000</dc:source>
        <dc:type>InWork</dc:type>
        <rdfs:comment xml:lang="en">An InformationUsageRight is an application of an InformationRight to a specific usage context.</rdfs:comment>
        <owl:versionInfo>2</owl:versionInfo>
        <skos:changeNote>[2021-07-30] Initial definition.</skos:changeNote>
        <skos:changeNote>[2022-09-01] Phil Spiby, Eurostep: updated comment updated note.</skos:changeNote>
        <skos:note xml:lang="en">InformationUsageRight provides a mechanism for recording significant rights within a product database. The legal significance of the presence or absence of a right is outside the scope of this part of ISO 10303.</skos:note>
        <skos:note xml:lang="en">One view of the distinction between an InformationRight and an InformationUsageRight is that the InformationRight represents a standard clause in a contract, whereas an InformationUsageRight represents the fact that the clause is used in a specific contract.</skos:note>
        <skos:note xml:lang="en">The Approval of an InformationUsageRight carries the meaning that the right is granted to all information items in the relevant context, as opposed to the approval of an InformationUsageRightAssignment which is limited to specific items.</skos:note>
        <skos:note xml:lang="en">The context for the usage can be defined through the contract which defines the right, the organization that grants the right, the person or organization which is granted the right, and any dates such as the starting or ending dates for the right. The meaning of each association is identified through the roles of the assignments, and these are defined through reference data.</skos:note>
        <skos:note xml:lang="en">The following additional data can be assigned to an InformationUsageRight: Contract, DateTimeString, Document, DocumentVersion, DocumentDefinition, File, and InformationUsageRight.</skos:note>
        <skos:prefLabel xml:lang="en">information usage right</skos:prefLabel>
    </owl:Class>
    


    <!-- http://standards.iso.org/iso/10303/tech/refdata/core#a5bced84-19bd-411a-ab9e-5d1abc81a290 -->

    <owl:Class rdf:about="http://standards.iso.org/iso/10303/tech/refdata/core#a5bced84-19bd-411a-ab9e-5d1abc81a290">
        <rdfs:subClassOf rdf:resource="http://standards.iso.org/iso/10303/tech/refdata/core#1d59c650-3279-0135-b58f-598f1b1392ae"/>
        <dc:contributor>STEP Harmonization Team</dc:contributor>
        <dc:creator>Phil Spiby, Eurostep</dc:creator>
        <dc:date>2022-09-01</dc:date>
        <dc:source>ISO/TS 10303-4000</dc:source>
        <dc:type>InWork</dc:type>
        <rdfs:comment xml:lang="en">An InterfaceDefinitionFor is an association between an InterfaceSpecificationView and an item (specified by InterfaceDefinitionForSelect) that conforms to the specification.</rdfs:comment>
        <owl:versionInfo>2</owl:versionInfo>
        <skos:changeNote>[2021-07-30] Initial definition.</skos:changeNote>
        <skos:changeNote>[2022-09-01] Phil Spiby, Eurostep: updated comment updated example.</skos:changeNote>
        <skos:example xml:lang="en">The infrared transmitter in a television remote control conforms to the specification that has the identifier 2345/XYZ/001. An instance of the InterfaceDefinitionFor entity data type is necessary to identify this association.</skos:example>
        <skos:prefLabel xml:lang="en">interface definition for</skos:prefLabel>
    </owl:Class>
    


    <!-- http://standards.iso.org/iso/10303/tech/refdata/core#a5de7f70-130a-0135-b552-598f1b1392ae -->

    <owl:Class rdf:about="http://standards.iso.org/iso/10303/tech/refdata/core#a5de7f70-130a-0135-b552-598f1b1392ae">
        <rdfs:subClassOf rdf:resource="http://standards.iso.org/iso/10303/tech/refdata/core#1cfca290-3279-0135-b58f-598f1b1392ae"/>
        <dc:contributor>STEP Harmonization Team</dc:contributor>
        <dc:creator>Phil Spiby, Eurostep</dc:creator>
        <dc:date>2022-09-01</dc:date>
        <dc:source>ISO/TS 10303-4000</dc:source>
        <dc:type>InWork</dc:type>
        <rdfs:comment xml:lang="en">An InformationUsageRightAssignment is an assignment of a specific usage right to a set of items (specified by InformationUsageRightAssignmentSelect). The meaning of the assignment can be specified using the ClassifiedAs attribute inherited from the AssignmentObject.</rdfs:comment>
        <owl:versionInfo>2</owl:versionInfo>
        <skos:changeNote>[2021-07-30] Initial definition.</skos:changeNote>
        <skos:changeNote>[2022-09-01] Phil Spiby, Eurostep: updated comment.</skos:changeNote>
        <skos:note xml:lang="en">If an Approval is applied to this entity, it carries the meaning that the specific set of items is approved for the given usage. This approval generally indicates that the approval is exceptional and there is an implication that the set of entities should not be changed once the approval is given.</skos:note>
        <skos:prefLabel xml:lang="en">information usage right assignment</skos:prefLabel>
    </owl:Class>
    


    <!-- http://standards.iso.org/iso/10303/tech/refdata/core#a644bb50-130a-0135-b552-598f1b1392ae -->

    <owl:Class rdf:about="http://standards.iso.org/iso/10303/tech/refdata/core#a644bb50-130a-0135-b552-598f1b1392ae">
        <rdfs:subClassOf rdf:resource="http://standards.iso.org/iso/10303/tech/refdata/core#59b11220-3279-0135-b58f-598f1b1392ae"/>
        <dc:contributor>STEP Harmonization Team</dc:contributor>
        <dc:creator>Phil Spiby, Eurostep</dc:creator>
        <dc:date>2022-09-01</dc:date>
        <dc:source>ISO/TS 10303-4000</dc:source>
        <dc:type>InWork</dc:type>
        <rdfs:comment xml:lang="en">An InformationUsageRightRelationship is a relationship between two InformationUsageRight objects.</rdfs:comment>
        <owl:versionInfo>2</owl:versionInfo>
        <skos:changeNote>[2021-07-30] Initial definition.</skos:changeNote>
        <skos:changeNote>[2022-09-01] Phil Spiby, Eurostep: updated comment.</skos:changeNote>
        <skos:example xml:lang="en">Where one InformationUsageRight supersedes another, then the original right is pointed to by the relating attribute, its replacement by the related attribute, and the relationType attribute takes the value supersedes.</skos:example>
        <skos:note xml:lang="en">The following additional data can be assigned to an InformationUsageRightRelationship: Effectivity, and InformationUsageRight.</skos:note>
        <skos:prefLabel xml:lang="en">information usage right relationship</skos:prefLabel>
    </owl:Class>
    


    <!-- http://standards.iso.org/iso/10303/tech/refdata/core#a6adb047-6fbf-43c2-ae98-09bb0111b88c -->

    <owl:Class rdf:about="http://standards.iso.org/iso/10303/tech/refdata/core#a6adb047-6fbf-43c2-ae98-09bb0111b88c">
        <rdfs:subClassOf rdf:resource="http://standards.iso.org/iso/10303/tech/refdata/core#f8816baf-d66a-42f9-bdcc-38e946c9a2fa"/>
        <dc:contributor>STEP Harmonization Team</dc:contributor>
        <dc:creator>Jean Brangé, AFNeT Services</dc:creator>
        <dc:date>2023-10-04</dc:date>
        <dc:source>ISO/TS 10303-4000</dc:source>
        <dc:type>InWork</dc:type>
        <rdfs:comment xml:lang="en">An Extension is a type of DerivedShapeElement that corresponds to the extension of a curve or surface ShapeElement.</rdfs:comment>
        <owl:versionInfo>3</owl:versionInfo>
        <skos:changeNote>[2023-10-04] Jean Brangé, AFNeT Services: Initial definition.</skos:changeNote>
        <skos:prefLabel xml:lang="en">extension</skos:prefLabel>
    </owl:Class>
    


    <!-- http://standards.iso.org/iso/10303/tech/refdata/core#a6e36c50-130a-0135-b552-598f1b1392ae -->

    <owl:Class rdf:about="http://standards.iso.org/iso/10303/tech/refdata/core#a6e36c50-130a-0135-b552-598f1b1392ae">
        <rdfs:subClassOf rdf:resource="http://standards.iso.org/iso/10303/tech/refdata/core#1d59c650-3279-0135-b58f-598f1b1392ae"/>
        <dc:contributor>STEP Harmonization Team</dc:contributor>
        <dc:creator>Phil Spiby, Eurostep</dc:creator>
        <dc:date>2022-09-01</dc:date>
        <dc:source>ISO/TS 10303-4000</dc:source>
        <dc:type>InWork</dc:type>
        <rdfs:comment xml:lang="en">An InZone is an association between a BreakdownElementView that represents a zone and an item (specified by InZoneSelect) that exists within this zone.</rdfs:comment>
        <owl:versionInfo>2</owl:versionInfo>
        <skos:changeNote>[2021-07-30] Initial definition.</skos:changeNote>
        <skos:changeNote>[2022-09-01] Phil Spiby, Eurostep: updated comment.</skos:changeNote>
        <skos:prefLabel xml:lang="en">in zone</skos:prefLabel>
    </owl:Class>
    


    <!-- http://standards.iso.org/iso/10303/tech/refdata/core#a7123d6f-a605-4773-a311-5aa653b09aa3 -->

    <owl:Class rdf:about="http://standards.iso.org/iso/10303/tech/refdata/core#a7123d6f-a605-4773-a311-5aa653b09aa3">
        <rdfs:subClassOf rdf:resource="http://standards.iso.org/iso/10303/tech/refdata/core#af0b342e-b77d-4ac9-abdc-26d92ffb92a9"/>
        <dc:contributor>STEP Harmonization Team</dc:contributor>
        <dc:creator>Jean Brangé, AFNeT Services</dc:creator>
        <dc:date>2023-10-04</dc:date>
        <dc:source>ISO/TS 10303-4000</dc:source>
        <dc:type>InWork</dc:type>
        <rdfs:comment xml:lang="en">An EdgeOfUndefinedShapeSize is a type of GeometricDimension that represents an &quot;edge of undefined shape&quot; size as defined in ISO 13715.</rdfs:comment>
        <owl:versionInfo>3</owl:versionInfo>
        <skos:changeNote>[2023-10-04] Jean Brangé, AFNeT Services: Initial definition.</skos:changeNote>
        <skos:prefLabel xml:lang="en">edge of undefined shape size</skos:prefLabel>
    </owl:Class>
    


    <!-- http://standards.iso.org/iso/10303/tech/refdata/core#a8535000-130a-0135-b552-598f1b1392ae -->

    <owl:Class rdf:about="http://standards.iso.org/iso/10303/tech/refdata/core#a8535000-130a-0135-b552-598f1b1392ae">
        <rdfs:subClassOf rdf:resource="http://standards.iso.org/iso/10303/tech/refdata/core#STEPThing"/>
        <dc:contributor>STEP Harmonization Team</dc:contributor>
        <dc:creator>Phil Spiby, Eurostep</dc:creator>
        <dc:date>2022-09-01</dc:date>
        <dc:source>ISO/TS 10303-4000</dc:source>
        <dc:type>InWork</dc:type>
        <rdfs:comment xml:lang="en">A LifeCycleStage is a general stage in the product life cycle to which the concerned items belong.</rdfs:comment>
        <owl:versionInfo>1</owl:versionInfo>
        <skos:changeNote>[2021-07-30] Initial definition.</skos:changeNote>
        <skos:prefLabel xml:lang="en">life cycle stage</skos:prefLabel>
    </owl:Class>
    


    <!-- http://standards.iso.org/iso/10303/tech/refdata/core#a8a4d91a-ca00-4ae5-bc2f-4633cb44b5c3 -->

    <owl:Class rdf:about="http://standards.iso.org/iso/10303/tech/refdata/core#a8a4d91a-ca00-4ae5-bc2f-4633cb44b5c3">
        <rdfs:subClassOf rdf:resource="http://standards.iso.org/iso/10303/tech/refdata/core#59b11220-3279-0135-b58f-598f1b1392ae"/>
        <dc:contributor>STEP Harmonization Team</dc:contributor>
        <dc:creator>Jean Brangé, AFNeT Services</dc:creator>
        <dc:date>2023-10-04</dc:date>
        <dc:source>ISO/TS 10303-4000</dc:source>
        <dc:type>InWork</dc:type>
        <rdfs:comment xml:lang="en">A CalloutRelationship is a logical relationship between two annotation groups which appear on an annotated model.</rdfs:comment>
        <owl:versionInfo>3</owl:versionInfo>
        <skos:changeNote>[2023-10-04] Jean Brangé, AFNeT Services: Initial definition.</skos:changeNote>
        <skos:prefLabel xml:lang="en">callout relationship</skos:prefLabel>
    </owl:Class>
    


    <!-- http://standards.iso.org/iso/10303/tech/refdata/core#a8bfcb27-551c-459d-8286-eef3f247ce66 -->

    <owl:Class rdf:about="http://standards.iso.org/iso/10303/tech/refdata/core#a8bfcb27-551c-459d-8286-eef3f247ce66">
        <rdfs:subClassOf rdf:resource="http://standards.iso.org/iso/10303/tech/refdata/core#1cfca290-3279-0135-b58f-598f1b1392ae"/>
        <dc:contributor>STEP Harmonization Team</dc:contributor>
        <dc:creator>Jean Brangé, AFNeT Services</dc:creator>
        <dc:date>2023-10-04</dc:date>
        <dc:source>ISO/TS 10303-4000</dc:source>
        <dc:type>InWork</dc:type>
        <rdfs:comment xml:lang="en">A MaterialPropertyAssignment is an association of a material, that is, a MaterialIdentification object, with a material property, that is, a MaterialPropertyValue object. Many properties may be assigned to a single material by the instantiation of many MaterialPropertyAssignment objects.</rdfs:comment>
        <owl:versionInfo>3</owl:versionInfo>
        <skos:changeNote>[2023-10-04] Jean Brangé, AFNeT Services: Initial definition.</skos:changeNote>
        <skos:prefLabel xml:lang="en">material property assignment</skos:prefLabel>
    </owl:Class>
    


    <!-- http://standards.iso.org/iso/10303/tech/refdata/core#a9584843-0b56-4f53-a1d8-7fb598de7100 -->

    <owl:Class rdf:about="http://standards.iso.org/iso/10303/tech/refdata/core#a9584843-0b56-4f53-a1d8-7fb598de7100">
        <rdfs:subClassOf rdf:resource="http://standards.iso.org/iso/10303/tech/refdata/core#70fd2ab8-bdcb-481c-8096-ca0246ed15c5"/>
        <dc:contributor>STEP Harmonization Team</dc:contributor>
        <dc:creator>Phil Spiby, Eurostep</dc:creator>
        <dc:date>2022-09-01</dc:date>
        <dc:source>ISO/TS 10303-4000</dc:source>
        <dc:type>InWork</dc:type>
        <rdfs:comment xml:lang="en">A SlotAsRealized is a specialization of SlotVersion that identifies an individual that is a realized Slot.</rdfs:comment>
        <owl:versionInfo>1</owl:versionInfo>
        <skos:changeNote>[2022-09-01] Initial definition.</skos:changeNote>
        <skos:example xml:lang="en">FlyFasterWithUs Group operates an aircraft with serial number 1234 next year. The company records which individual engines power the aircraft at different times during the lifetime of the aircraft.</skos:example>
        <skos:prefLabel xml:lang="en">slot as realized</skos:prefLabel>
    </owl:Class>
    


    <!-- http://standards.iso.org/iso/10303/tech/refdata/core#a96471e0-130a-0135-b552-598f1b1392ae -->

    <owl:Class rdf:about="http://standards.iso.org/iso/10303/tech/refdata/core#a96471e0-130a-0135-b552-598f1b1392ae">
        <rdfs:subClassOf rdf:resource="http://standards.iso.org/iso/10303/tech/refdata/core#99130bd0-130a-0135-b552-598f1b1392ae"/>
        <dc:contributor>STEP Harmonization Team</dc:contributor>
        <dc:creator>Phil Spiby, Eurostep</dc:creator>
        <dc:date>2022-09-01</dc:date>
        <dc:source>ISO/TS 10303-4000</dc:source>
        <dc:type>InWork</dc:type>
        <rdfs:comment xml:lang="en">A LotEffectivity is a type of Effectivity for which the domain of applicability is defined as a given batch of items.</rdfs:comment>
        <owl:versionInfo>1</owl:versionInfo>
        <skos:changeNote>[2021-07-30] Initial definition.</skos:changeNote>
        <skos:prefLabel xml:lang="en">lot effectivity</skos:prefLabel>
    </owl:Class>
    


    <!-- http://standards.iso.org/iso/10303/tech/refdata/core#aaa1d3e0-130a-0135-b552-598f1b1392ae -->

    <owl:Class rdf:about="http://standards.iso.org/iso/10303/tech/refdata/core#aaa1d3e0-130a-0135-b552-598f1b1392ae">
        <rdfs:subClassOf rdf:resource="http://standards.iso.org/iso/10303/tech/refdata/core#STEPThing"/>
        <dc:contributor>STEP Harmonization Team</dc:contributor>
        <dc:creator>Phil Spiby, Eurostep</dc:creator>
        <dc:date>2022-09-01</dc:date>
        <dc:source>ISO/TS 10303-4000</dc:source>
        <dc:type>InWork</dc:type>
        <rdfs:comment xml:lang="en">A Market is a representation of a marketing segment for products.</rdfs:comment>
        <owl:versionInfo>1</owl:versionInfo>
        <skos:changeNote>[2021-07-30] Initial definition.</skos:changeNote>
        <skos:prefLabel xml:lang="en">market</skos:prefLabel>
    </owl:Class>
    


    <!-- http://standards.iso.org/iso/10303/tech/refdata/core#aaaee1e6-988a-43a6-baa7-68809c30a84d -->

    <owl:Class rdf:about="http://standards.iso.org/iso/10303/tech/refdata/core#aaaee1e6-988a-43a6-baa7-68809c30a84d">
        <rdfs:subClassOf rdf:resource="http://standards.iso.org/iso/10303/tech/refdata/core#STEPThing"/>
        <dc:contributor>STEP Harmonization Team</dc:contributor>
        <dc:creator>Phil Spiby, Eurostep</dc:creator>
        <dc:date>2022-09-01</dc:date>
        <dc:source>ISO/TS 10303-4000</dc:source>
        <dc:type>InWork</dc:type>
        <rdfs:comment xml:lang="en">A PositionGroup is a group for collecting people in their positions to cooperate in an assignment.</rdfs:comment>
        <owl:versionInfo>1</owl:versionInfo>
        <skos:changeNote>[2022-09-01] Initial definition.</skos:changeNote>
        <skos:example xml:lang="en">People representing utility companies who cooperate with each other to coordinate road works.</skos:example>
        <skos:prefLabel xml:lang="en">position group</skos:prefLabel>
    </owl:Class>
    


    <!-- http://standards.iso.org/iso/10303/tech/refdata/core#aacadd37-b6b6-4ecf-a3a8-589990ca860d -->

    <owl:Class rdf:about="http://standards.iso.org/iso/10303/tech/refdata/core#aacadd37-b6b6-4ecf-a3a8-589990ca860d">
        <rdfs:subClassOf rdf:resource="http://standards.iso.org/iso/10303/tech/refdata/core#59b11220-3279-0135-b58f-598f1b1392ae"/>
        <dc:contributor>STEP Harmonization Team</dc:contributor>
        <dc:creator>Phil Spiby, Eurostep</dc:creator>
        <dc:date>2022-09-01</dc:date>
        <dc:source>ISO/TS 10303-4000</dc:source>
        <dc:type>InWork</dc:type>
        <rdfs:comment xml:lang="en">A RelatedConsequence is a relationship that identifies an expected consequence of a specific perception of a risk.</rdfs:comment>
        <owl:versionInfo>1</owl:versionInfo>
        <skos:changeNote>[2022-09-01] Initial definition.</skos:changeNote>
        <skos:prefLabel xml:lang="en">related consequence</skos:prefLabel>
    </owl:Class>
    


    <!-- http://standards.iso.org/iso/10303/tech/refdata/core#aafe1ab1-3865-433a-b81d-475fefd1586f -->

    <owl:Class rdf:about="http://standards.iso.org/iso/10303/tech/refdata/core#aafe1ab1-3865-433a-b81d-475fefd1586f">
        <rdfs:subClassOf rdf:resource="http://standards.iso.org/iso/10303/tech/refdata/core#9f656069-ff2c-4f09-9091-f91388a14764"/>
        <dc:contributor>STEP Harmonization Team</dc:contributor>
        <dc:creator>Phil Spiby, Eurostep</dc:creator>
        <dc:date>2022-09-01</dc:date>
        <dc:source>ISO/TS 10303-4000</dc:source>
        <dc:type>InWork</dc:type>
        <rdfs:comment xml:lang="en">A StateTransition represents a transition between two State, identified respectively as a start and an end.</rdfs:comment>
        <owl:versionInfo>1</owl:versionInfo>
        <skos:changeNote>[2021-07-30] Initial definition.</skos:changeNote>
        <skos:prefLabel xml:lang="en">state transition</skos:prefLabel>
    </owl:Class>
    


    <!-- http://standards.iso.org/iso/10303/tech/refdata/core#ab417830-0eae-45bb-9b47-efb2d6d99faa -->

    <owl:Class rdf:about="http://standards.iso.org/iso/10303/tech/refdata/core#ab417830-0eae-45bb-9b47-efb2d6d99faa">
        <rdfs:subClassOf rdf:resource="http://standards.iso.org/iso/10303/tech/refdata/core#STEPThing"/>
        <dc:contributor>STEP Harmonization Team</dc:contributor>
        <dc:creator>Phil Spiby, Eurostep</dc:creator>
        <dc:date>2022-09-01</dc:date>
        <dc:source>ISO/TS 10303-4000</dc:source>
        <dc:type>InWork</dc:type>
        <rdfs:comment xml:lang="en">An Acknowledgement is a response requested for receipt of an Envelope.</rdfs:comment>
        <owl:versionInfo>2</owl:versionInfo>
        <skos:changeNote>[2021-07-30] Initial definition.</skos:changeNote>
        <skos:changeNote>[2022-09-01] Phil Spiby, Eurostep: updated comment.</skos:changeNote>
        <skos:prefLabel xml:lang="en">acknowledgement</skos:prefLabel>
    </owl:Class>
    


    <!-- http://standards.iso.org/iso/10303/tech/refdata/core#ac6001f4-ce24-4918-b379-cb4a37fc7621 -->

    <owl:Class rdf:about="http://standards.iso.org/iso/10303/tech/refdata/core#ac6001f4-ce24-4918-b379-cb4a37fc7621">
        <rdfs:subClassOf rdf:resource="http://standards.iso.org/iso/10303/tech/refdata/core#1d59c650-3279-0135-b58f-598f1b1392ae"/>
        <dc:contributor>STEP Harmonization Team</dc:contributor>
        <dc:creator>Phil Spiby, Eurostep</dc:creator>
        <dc:date>2022-09-01</dc:date>
        <dc:source>ISO/TS 10303-4000</dc:source>
        <dc:type>InWork</dc:type>
        <rdfs:comment xml:lang="en">A TaskElementStateAssociation is an association between a state (specified by StateOrStateDefinitionSelect) and a TaskElement.</rdfs:comment>
        <owl:versionInfo>2</owl:versionInfo>
        <skos:changeNote>[2021-07-30] Initial definition.</skos:changeNote>
        <skos:changeNote>[2022-09-01] Phil Spiby, Eurostep: updated name updated comment updated note.</skos:changeNote>
        <skos:prefLabel xml:lang="en">task element state association</skos:prefLabel>
    </owl:Class>
    


    <!-- http://standards.iso.org/iso/10303/tech/refdata/core#ac6d1e00-130a-0135-b552-598f1b1392ae -->

    <owl:Class rdf:about="http://standards.iso.org/iso/10303/tech/refdata/core#ac6d1e00-130a-0135-b552-598f1b1392ae">
        <rdfs:subClassOf rdf:resource="http://standards.iso.org/iso/10303/tech/refdata/core#STEPThing"/>
        <dc:contributor>STEP Harmonization Team</dc:contributor>
        <dc:creator>Phil Spiby, Eurostep</dc:creator>
        <dc:date>2022-09-01</dc:date>
        <dc:source>ISO/TS 10303-4000</dc:source>
        <dc:type>InWork</dc:type>
        <rdfs:comment xml:lang="en">A MeasureQualification is a means to provide information about measurements in which there is an associated uncertainty. The uncertainty can be specified as precision, qualitative uncertainty, or expanded uncertainty, and the type of the related datum shall be included. The uncertainty is defined in clause 2 of &apos;The Guide to the Expression of Uncertainty in Measurement&apos;.</rdfs:comment>
        <owl:versionInfo>2</owl:versionInfo>
        <skos:changeNote>[2021-07-30] Initial definition.</skos:changeNote>
        <skos:changeNote>[2022-09-01] Phil Spiby, Eurostep: updated comment.</skos:changeNote>
        <skos:prefLabel xml:lang="en">measure qualification</skos:prefLabel>
    </owl:Class>
    


    <!-- http://standards.iso.org/iso/10303/tech/refdata/core#ac90192f-e3d7-4341-9a82-0a72098388b9 -->

    <owl:Class rdf:about="http://standards.iso.org/iso/10303/tech/refdata/core#ac90192f-e3d7-4341-9a82-0a72098388b9">
        <rdfs:subClassOf rdf:resource="http://standards.iso.org/iso/10303/tech/refdata/core#1d59c650-3279-0135-b58f-598f1b1392ae"/>
        <dc:contributor>STEP Harmonization Team</dc:contributor>
        <dc:creator>Jean Brangé, AFNeT Services</dc:creator>
        <dc:date>2023-10-04</dc:date>
        <dc:source>ISO/TS 10303-4000</dc:source>
        <dc:type>InWork</dc:type>
        <rdfs:comment xml:lang="en">A KinematicLinkToOccurrenceAssociation is an association between a KinematicLink within a Mechanism and an Occurrence within an AssemblyDefinition.</rdfs:comment>
        <owl:versionInfo>3</owl:versionInfo>
        <skos:changeNote>[2023-10-04] Jean Brangé, AFNeT Services: Initial definition.</skos:changeNote>
        <skos:prefLabel xml:lang="en">kinematic link to occurrence association</skos:prefLabel>
    </owl:Class>
    


    <!-- http://standards.iso.org/iso/10303/tech/refdata/core#acb6e843-005f-4961-aabe-ef0e74ef9769 -->

    <owl:Class rdf:about="http://standards.iso.org/iso/10303/tech/refdata/core#acb6e843-005f-4961-aabe-ef0e74ef9769">
        <rdfs:subClassOf rdf:resource="http://standards.iso.org/iso/10303/tech/refdata/core#1d59c650-3279-0135-b58f-598f1b1392ae"/>
        <dc:contributor>STEP Harmonization Team</dc:contributor>
        <dc:creator>Phil Spiby, Eurostep</dc:creator>
        <dc:date>2022-09-01</dc:date>
        <dc:source>ISO/TS 10303-4000</dc:source>
        <dc:type>InWork</dc:type>
        <rdfs:comment xml:lang="en">A TaskMethodStateAssociation is an association between a state (specified by StateOrStateDefinitionSelect) and a TaskMethodVersion.</rdfs:comment>
        <owl:versionInfo>2</owl:versionInfo>
        <skos:changeNote>[2021-07-30] Initial definition.</skos:changeNote>
        <skos:changeNote>[2022-09-01] Phil Spiby, Eurostep: updated name updated comment updated note.</skos:changeNote>
        <skos:prefLabel xml:lang="en">task method state association</skos:prefLabel>
    </owl:Class>
    


    <!-- http://standards.iso.org/iso/10303/tech/refdata/core#acee6080-f1fa-4e40-94c5-75ba162fbf29 -->

    <owl:Class rdf:about="http://standards.iso.org/iso/10303/tech/refdata/core#acee6080-f1fa-4e40-94c5-75ba162fbf29">
        <rdfs:subClassOf rdf:resource="http://standards.iso.org/iso/10303/tech/refdata/core#59b11220-3279-0135-b58f-598f1b1392ae"/>
        <dc:contributor>STEP Harmonization Team</dc:contributor>
        <dc:creator>Phil Spiby, Eurostep</dc:creator>
        <dc:date>2022-09-01</dc:date>
        <dc:source>ISO/TS 10303-4000</dc:source>
        <dc:type>InWork</dc:type>
        <rdfs:comment xml:lang="en">An ExperienceTypeRelationship is a relationship between two ExperienceType objects.</rdfs:comment>
        <owl:versionInfo>1</owl:versionInfo>
        <skos:changeNote>[2022-09-01] Initial definition.</skos:changeNote>
        <skos:example xml:lang="en">Ten years programming experience made up of five years C++ programming experience and five years Java programming experience.</skos:example>
        <skos:prefLabel xml:lang="en">experience type relationship</skos:prefLabel>
    </owl:Class>
    


    <!-- http://standards.iso.org/iso/10303/tech/refdata/core#ad1ce100-5373-4e7c-b1eb-714bd099e6a1 -->

    <owl:Class rdf:about="http://standards.iso.org/iso/10303/tech/refdata/core#ad1ce100-5373-4e7c-b1eb-714bd099e6a1">
        <rdfs:subClassOf rdf:resource="http://standards.iso.org/iso/10303/tech/refdata/core#835280f0-130a-0135-b552-598f1b1392ae"/>
        <dc:contributor>STEP Harmonization Team</dc:contributor>
        <dc:creator>Phil Spiby, Eurostep</dc:creator>
        <dc:date>2022-09-01</dc:date>
        <dc:source>ISO/TS 10303-4000</dc:source>
        <dc:type>InWork</dc:type>
        <rdfs:comment xml:lang="en">A Scheme is a specialization of ActivityMethod. It provides the identification and description of an intended course of action to accomplish an objective. A Scheme allows for the ordering of entries. Dates and times can be specified for entries and time intervals between entries.</rdfs:comment>
        <owl:versionInfo>1</owl:versionInfo>
        <skos:changeNote>[2022-09-01] Initial definition.</skos:changeNote>
        <skos:example xml:lang="en">Acquisition plan, Maintenance plan, and Resource schedule are examples of schemes.</skos:example>
        <skos:note xml:lang="en">A Scheme can be classified as a Plan or a Schedule, and it can be further classified into specific types of Plans or Schedules.</skos:note>
        <skos:prefLabel xml:lang="en">scheme</skos:prefLabel>
    </owl:Class>
    


    <!-- http://standards.iso.org/iso/10303/tech/refdata/core#ad6d7700-130a-0135-b552-598f1b1392ae -->

    <owl:Class rdf:about="http://standards.iso.org/iso/10303/tech/refdata/core#ad6d7700-130a-0135-b552-598f1b1392ae">
        <rdfs:subClassOf rdf:resource="http://standards.iso.org/iso/10303/tech/refdata/core#cca6c810-130a-0135-b552-598f1b1392ae"/>
        <dc:contributor>STEP Harmonization Team</dc:contributor>
        <dc:creator>Jean Brangé, AFNeT Services</dc:creator>
        <dc:date>2023-10-04</dc:date>
        <dc:source>ISO/TS 10303-4000</dc:source>
        <dc:type>InWork</dc:type>
        <rdfs:comment xml:lang="en">A MomentsOfInertia is a type of ShapeDependentProperty that describes the matrix of inertia of a rigid body.</rdfs:comment>
        <owl:versionInfo>3</owl:versionInfo>
        <skos:changeNote>[2023-10-04] Jean Brangé, AFNeT Services: Initial definition.</skos:changeNote>
        <skos:prefLabel xml:lang="en">moments of inertia</skos:prefLabel>
    </owl:Class>
    


    <!-- http://standards.iso.org/iso/10303/tech/refdata/core#adbb48e0-130a-0135-b552-598f1b1392ae -->

    <owl:Class rdf:about="http://standards.iso.org/iso/10303/tech/refdata/core#adbb48e0-130a-0135-b552-598f1b1392ae">
        <rdfs:subClassOf rdf:resource="http://standards.iso.org/iso/10303/tech/refdata/core#87863f90-130a-0135-b552-598f1b1392ae"/>
        <dc:contributor>STEP Harmonization Team</dc:contributor>
        <dc:creator>Phil Spiby, Eurostep</dc:creator>
        <dc:date>2022-09-01</dc:date>
        <dc:source>ISO/TS 10303-4000</dc:source>
        <dc:type>InWork</dc:type>
        <rdfs:comment xml:lang="en">A NextAssemblyOccurrenceUsage is a type of AssemblyOccurrenceRelationship that is a relationship where the attribute Related specifies an occurrence of a constituent of an assembly and the attribute Relating specifies a view of the immediate parent assembly of the constituent.</rdfs:comment>
        <owl:versionInfo>2</owl:versionInfo>
        <skos:changeNote>[2021-07-30] Initial definition.</skos:changeNote>
        <skos:changeNote>[2022-09-01] Phil Spiby, Eurostep: updated example updated note.</skos:changeNote>
        <skos:example xml:lang="en">The assembly carburettor can be assembled from single parts. The power train assembly is assembled from other assemblies.</skos:example>
        <skos:note xml:lang="en">A constituent can be a single part or an assembly.</skos:note>
        <skos:prefLabel xml:lang="en">next assembly occurrence usage</skos:prefLabel>
    </owl:Class>
    


    <!-- http://standards.iso.org/iso/10303/tech/refdata/core#adc16360-130a-0135-b552-598f1b1392ae -->

    <owl:Class rdf:about="http://standards.iso.org/iso/10303/tech/refdata/core#adc16360-130a-0135-b552-598f1b1392ae">
        <rdfs:subClassOf rdf:resource="http://standards.iso.org/iso/10303/tech/refdata/core#88035ed0-130a-0135-b552-598f1b1392ae"/>
        <dc:contributor>STEP Harmonization Team</dc:contributor>
        <dc:creator>Phil Spiby, Eurostep</dc:creator>
        <dc:date>2022-09-01</dc:date>
        <dc:source>ISO/TS 10303-4000</dc:source>
        <dc:type>InWork</dc:type>
        <rdfs:comment xml:lang="en">A NextAssemblyViewUsage is a type of AssemblyViewRelationship that is a relationship where the attribute Related specifies a view of an assembly and the attribute Relating specifies a view of the immediate parent assembly of the constituent.</rdfs:comment>
        <owl:versionInfo>1</owl:versionInfo>
        <skos:changeNote>[2021-07-30] Initial definition.</skos:changeNote>
        <skos:prefLabel xml:lang="en">next assembly view usage</skos:prefLabel>
    </owl:Class>
    


    <!-- http://standards.iso.org/iso/10303/tech/refdata/core#add3b2e0-130a-0135-b552-598f1b1392ae -->

    <owl:Class rdf:about="http://standards.iso.org/iso/10303/tech/refdata/core#add3b2e0-130a-0135-b552-598f1b1392ae">
        <rdfs:subClassOf rdf:resource="http://standards.iso.org/iso/10303/tech/refdata/core#STEPThing"/>
        <dc:contributor>STEP Harmonization Team</dc:contributor>
        <dc:creator>Phil Spiby, Eurostep</dc:creator>
        <dc:date>2022-09-01</dc:date>
        <dc:source>ISO/TS 10303-4000</dc:source>
        <dc:type>InWork</dc:type>
        <rdfs:comment xml:lang="en">A NumericalContext is a context in which the number of significant digits and uncertainties can be defined. These number of significant digits and uncertainties apply to the NumericalValue objects that are used in that context.</rdfs:comment>
        <owl:versionInfo>2</owl:versionInfo>
        <skos:changeNote>[2021-07-30] Initial definition.</skos:changeNote>
        <skos:changeNote>[2022-09-01] Phil Spiby, Eurostep: updated comment.</skos:changeNote>
        <skos:prefLabel xml:lang="en">numerical context</skos:prefLabel>
    </owl:Class>
    


    <!-- http://standards.iso.org/iso/10303/tech/refdata/core#adf0ca52-98c1-4450-9a8b-67fe66e6adeb -->

    <owl:Class rdf:about="http://standards.iso.org/iso/10303/tech/refdata/core#adf0ca52-98c1-4450-9a8b-67fe66e6adeb">
        <rdfs:subClassOf rdf:resource="http://standards.iso.org/iso/10303/tech/refdata/core#1cfca290-3279-0135-b58f-598f1b1392ae"/>
        <dc:contributor>STEP Harmonization Team</dc:contributor>
        <dc:creator>Phil Spiby, Eurostep</dc:creator>
        <dc:date>2022-09-01</dc:date>
        <dc:source>ISO/TS 10303-4000</dc:source>
        <dc:type>InWork</dc:type>
        <rdfs:comment xml:lang="en">A StateDefinitionAssignment is an assignment of a StateDefinition to an item (specified by StateDefinitionAssignmentSelect). The meaning of the assignment can be specified using the ClassifiedAs attribute inherited from the AssignmentObject.</rdfs:comment>
        <owl:versionInfo>2</owl:versionInfo>
        <skos:changeNote>[2021-07-30] Initial definition.</skos:changeNote>
        <skos:changeNote>[2022-09-01] Phil Spiby, Eurostep: updated comment.</skos:changeNote>
        <skos:prefLabel xml:lang="en">state definition assignment</skos:prefLabel>
    </owl:Class>
    


    <!-- http://standards.iso.org/iso/10303/tech/refdata/core#adfff300-130a-0135-b552-598f1b1392ae -->

    <owl:Class rdf:about="http://standards.iso.org/iso/10303/tech/refdata/core#adfff300-130a-0135-b552-598f1b1392ae">
        <rdfs:subClassOf rdf:resource="http://standards.iso.org/iso/10303/tech/refdata/core#d75d6570-130a-0135-b552-598f1b1392ae"/>
        <dc:contributor>STEP Harmonization Team</dc:contributor>
        <dc:creator>Phil Spiby, Eurostep</dc:creator>
        <dc:date>2022-09-01</dc:date>
        <dc:source>ISO/TS 10303-4000</dc:source>
        <dc:type>InWork</dc:type>
        <rdfs:comment xml:lang="en">A NumericalValue is a type of ValueWithUnit representing a quantity expressed with a numerical value and a unit.</rdfs:comment>
        <owl:versionInfo>1</owl:versionInfo>
        <skos:changeNote>[2021-07-30] Initial definition.</skos:changeNote>
        <skos:prefLabel xml:lang="en">numerical value</skos:prefLabel>
    </owl:Class>
    


    <!-- http://standards.iso.org/iso/10303/tech/refdata/core#ae1e7780-130a-0135-b552-598f1b1392ae -->

    <owl:Class rdf:about="http://standards.iso.org/iso/10303/tech/refdata/core#ae1e7780-130a-0135-b552-598f1b1392ae">
        <rdfs:subClassOf rdf:resource="http://standards.iso.org/iso/10303/tech/refdata/core#STEPThing"/>
        <dc:contributor>STEP Harmonization Team</dc:contributor>
        <dc:creator>Phil Spiby, Eurostep</dc:creator>
        <dc:date>2022-09-01</dc:date>
        <dc:source>ISO/TS 10303-4000</dc:source>
        <dc:type>InWork</dc:type>
        <rdfs:comment xml:lang="en">An Occurrence is an occurrence of an object in a product structure that is defined by an item specified by OccurrenceOrOccurrenceDefinitionSelect.</rdfs:comment>
        <owl:versionInfo>2</owl:versionInfo>
        <skos:changeNote>[2021-07-30] Initial definition.</skos:changeNote>
        <skos:changeNote>[2022-09-01] Phil Spiby, Eurostep: updated comment updated example.</skos:changeNote>
        <skos:example xml:lang="en">In the case of a car, the Item &apos;wheel&apos; is defined once. Its PartVersion carries all the information necessary to define the wheel (such as its shape) independent of its usage. Additionally, there are 5 Occurrence objects for this wheel since there are 5 equal wheels used in this car: front-left, front-right, rear-left, rear-right, and spare wheel. Each of these instances can carry additional information such as placement or function. Each Occurrence is a DefinitionBasedOccurrence, or a SpecifiedOccurrence.</skos:example>
        <skos:prefLabel xml:lang="en">occurrence</skos:prefLabel>
    </owl:Class>
    


    <!-- http://standards.iso.org/iso/10303/tech/refdata/core#aeba1b40-130a-0135-b552-598f1b1392ae -->

    <owl:Class rdf:about="http://standards.iso.org/iso/10303/tech/refdata/core#aeba1b40-130a-0135-b552-598f1b1392ae">
        <rdfs:subClassOf rdf:resource="http://standards.iso.org/iso/10303/tech/refdata/core#59b11220-3279-0135-b58f-598f1b1392ae"/>
        <dc:contributor>STEP Harmonization Team</dc:contributor>
        <dc:creator>Phil Spiby, Eurostep</dc:creator>
        <dc:date>2022-09-01</dc:date>
        <dc:source>ISO/TS 10303-4000</dc:source>
        <dc:type>InWork</dc:type>
        <rdfs:comment xml:lang="en">An OccurrenceRelationship is a relationship between two Occurrence objects.</rdfs:comment>
        <owl:versionInfo>2</owl:versionInfo>
        <skos:changeNote>[2021-07-30] Initial definition.</skos:changeNote>
        <skos:changeNote>[2022-09-01] Phil Spiby, Eurostep: updated comment.</skos:changeNote>
        <skos:prefLabel xml:lang="en">occurrence relationship</skos:prefLabel>
    </owl:Class>
    


    <!-- http://standards.iso.org/iso/10303/tech/refdata/core#af0b342e-b77d-4ac9-abdc-26d92ffb92a9 -->

    <owl:Class rdf:about="http://standards.iso.org/iso/10303/tech/refdata/core#af0b342e-b77d-4ac9-abdc-26d92ffb92a9">
        <rdfs:subClassOf rdf:resource="http://standards.iso.org/iso/10303/tech/refdata/core#c050712f-0dca-495e-aa7d-2b2e21af712b"/>
        <dc:contributor>STEP Harmonization Team</dc:contributor>
        <dc:creator>Jean Brangé, AFNeT Services</dc:creator>
        <dc:date>2023-10-04</dc:date>
        <dc:source>ISO/TS 10303-4000</dc:source>
        <dc:type>InWork</dc:type>
        <rdfs:comment xml:lang="en">A DimensionalSize is a type of GeometricDimension. A DimensionalSize is a spatial characteristic of a ShapeElement that is represented by a measure. This magnitude is independent of the location of the ShapeElement on or within the product. A DimensionalSize is either an AngularSize or a CurvedSize, or a DiameterSize, or a MachiningFeatureSize, or a RadialSize, or a ThicknessSize</rdfs:comment>
        <owl:versionInfo>3</owl:versionInfo>
        <skos:changeNote>[2023-10-04] Jean Brangé, AFNeT Services: Initial definition.</skos:changeNote>
        <skos:example xml:lang="en">The diameter of a hole is 2 centimetres.</skos:example>
        <skos:note xml:lang="en">DimensionalSize as defined in this part of ISO 10303 describe an intrinsic length or angle characteristic of part shape. This includes characteristics of what are traditionally called &quot;features-of-size&quot;, but they are not limited to that usage alone. For example, the RadialSize and CurvedSize application objects describe characteristics which may not be applied to &quot;features-of-size&quot;.</skos:note>
        <skos:prefLabel xml:lang="en">dimensional size</skos:prefLabel>
    </owl:Class>
    


    <!-- http://standards.iso.org/iso/10303/tech/refdata/core#af34f679-506c-49c6-b5a6-e256865f1f28 -->

    <owl:Class rdf:about="http://standards.iso.org/iso/10303/tech/refdata/core#af34f679-506c-49c6-b5a6-e256865f1f28">
        <rdfs:subClassOf rdf:resource="http://standards.iso.org/iso/10303/tech/refdata/core#99130bd0-130a-0135-b552-598f1b1392ae"/>
        <dc:contributor>STEP Harmonization Team</dc:contributor>
        <dc:creator>Jean Brangé, AFNeT Services</dc:creator>
        <dc:date>2023-10-04</dc:date>
        <dc:source>ISO/TS 10303-4000</dc:source>
        <dc:type>InWork</dc:type>
        <rdfs:comment xml:lang="en">A VersionGraphEffectivity is a type of Effectivity for which the domain of applicability is defined as a possibly open-ended interval of versions. A &apos;start&apos; value shall always be specified with StartVersion, an &apos;end&apos; value may be specified.</rdfs:comment>
        <owl:versionInfo>3</owl:versionInfo>
        <skos:changeNote>[2023-10-04] Jean Brangé, AFNeT Services: Initial definition.</skos:changeNote>
        <skos:prefLabel xml:lang="en">version graph effectivity</skos:prefLabel>
    </owl:Class>
    


    <!-- http://standards.iso.org/iso/10303/tech/refdata/core#af699520-130a-0135-b552-598f1b1392ae -->

    <owl:Class rdf:about="http://standards.iso.org/iso/10303/tech/refdata/core#af699520-130a-0135-b552-598f1b1392ae">
        <rdfs:subClassOf rdf:resource="http://standards.iso.org/iso/10303/tech/refdata/core#STEPThing"/>
        <dc:contributor>STEP Harmonization Team</dc:contributor>
        <dc:creator>Phil Spiby, Eurostep</dc:creator>
        <dc:date>2022-09-01</dc:date>
        <dc:source>ISO/TS 10303-4000</dc:source>
        <dc:type>InWork</dc:type>
        <rdfs:comment xml:lang="en">An Organization is an administrative structure in which persons are active.</rdfs:comment>
        <owl:versionInfo>1</owl:versionInfo>
        <skos:changeNote>[2021-07-30] Initial definition.</skos:changeNote>
        <skos:prefLabel xml:lang="en">organization</skos:prefLabel>
    </owl:Class>
    


    <!-- http://standards.iso.org/iso/10303/tech/refdata/core#b000ef1d-5fe6-42d7-b10d-89463049fc43 -->

    <owl:Class rdf:about="http://standards.iso.org/iso/10303/tech/refdata/core#b000ef1d-5fe6-42d7-b10d-89463049fc43">
        <rdfs:subClassOf rdf:resource="http://standards.iso.org/iso/10303/tech/refdata/core#c6260c30-130a-0135-b552-598f1b1392ae"/>
        <dc:contributor>STEP Harmonization Team</dc:contributor>
        <dc:creator>Jean Brangé, AFNeT Services</dc:creator>
        <dc:date>2023-10-04</dc:date>
        <dc:source>ISO/TS 10303-4000</dc:source>
        <dc:type>InWork</dc:type>
        <rdfs:comment xml:lang="en">A TopologyToGeometryModelAssociation is a type of RepresentationRelationship that defines a set of binary associations between a topological origin item and a geometric target item. This association is not definitional and therefore will not bring the definition of the source into the target model. This set of binary associations is realized by a list of origin items and a list of target items that are coordinated so that the first origin item corresponds to the first target item, the second to the second and so on. The number of items on the origin and target sides shall be the same.</rdfs:comment>
        <owl:versionInfo>3</owl:versionInfo>
        <skos:changeNote>[2023-10-04] Jean Brangé, AFNeT Services: Initial definition.</skos:changeNote>
        <skos:note xml:lang="en">For users and implementers, note that the structure is not intended for Geometric Modeling. It is intended for traceability and verification purposes of the structure of the electrical wiring harness. To support wiring harness design requirements, the entities GeometryToTopologyModelAssociation and TopologyToGeometryModelAssociation, which are subtypes of RepresentationRelationship, are based on WiringHarnessAssemblyDesign, which is a subtype of AssemblyDefinition. GeometryToTopologyModelAssociation and TopologyToGeometryModelAssociation are referenced by an AssemblyOccurrenceRelationship. The design intent of the information model is to create one or more pairwise allocation associations between geometric elements and topological elements specific to electrical wire harness design. This specific usage of AssemblyOccurrenceRelationship is restricted to WiringHarnessAssemblyDesign.</skos:note>
        <skos:prefLabel xml:lang="en">topology to geometry model association</skos:prefLabel>
    </owl:Class>
    


    <!-- http://standards.iso.org/iso/10303/tech/refdata/core#b0178860-130a-0135-b552-598f1b1392ae -->

    <owl:Class rdf:about="http://standards.iso.org/iso/10303/tech/refdata/core#b0178860-130a-0135-b552-598f1b1392ae">
        <rdfs:subClassOf rdf:resource="http://standards.iso.org/iso/10303/tech/refdata/core#1cfca290-3279-0135-b58f-598f1b1392ae"/>
        <dc:contributor>STEP Harmonization Team</dc:contributor>
        <dc:creator>Phil Spiby, Eurostep</dc:creator>
        <dc:date>2022-09-01</dc:date>
        <dc:source>ISO/TS 10303-4000</dc:source>
        <dc:type>InWork</dc:type>
        <rdfs:comment xml:lang="en">A PersonOrganizationAssignment is an assignment of an organization or a person (specified by PersonOrganizationSelect) to an item (specified by PersonOrganizationAssignmentSelect). The meaning of the assignment can be specified using the ClassifiedAs attribute inherited from the AssignmentObject.</rdfs:comment>
        <owl:versionInfo>2</owl:versionInfo>
        <skos:changeNote>[2021-07-30] Initial definition.</skos:changeNote>
        <skos:changeNote>[2022-09-01] Phil Spiby, Eurostep: updated comment.</skos:changeNote>
        <skos:prefLabel xml:lang="en">person organization assignment</skos:prefLabel>
    </owl:Class>
    


    <!-- http://standards.iso.org/iso/10303/tech/refdata/core#b031a2d6-ce42-4d88-8f64-76049a4097f6 -->

    <owl:Class rdf:about="http://standards.iso.org/iso/10303/tech/refdata/core#b031a2d6-ce42-4d88-8f64-76049a4097f6">
        <rdfs:subClassOf rdf:resource="http://standards.iso.org/iso/10303/tech/refdata/core#1d59c650-3279-0135-b58f-598f1b1392ae"/>
        <dc:contributor>STEP Harmonization Team</dc:contributor>
        <dc:creator>Phil Spiby, Eurostep</dc:creator>
        <dc:date>2022-09-01</dc:date>
        <dc:source>ISO/TS 10303-4000</dc:source>
        <dc:type>InWork</dc:type>
        <rdfs:comment xml:lang="en">A TypeOfPersonDefinitionRequiredAttributesAssociation is an association between a TypeOfPersonDefinition and the attributes required to define that type of person.</rdfs:comment>
        <owl:versionInfo>1</owl:versionInfo>
        <skos:changeNote>[2022-09-01] Initial definition.</skos:changeNote>
        <skos:example xml:lang="en">The type of person &quot;van driver&quot; is required to possess the qualification named &quot;commercial driving license&quot; or the experience level &quot;3 years of driving more than 10,000 miles per year&quot;.</skos:example>
        <skos:prefLabel xml:lang="en">type of person definition required attributes association</skos:prefLabel>
    </owl:Class>
    


    <!-- http://standards.iso.org/iso/10303/tech/refdata/core#b080d180-130a-0135-b552-598f1b1392ae -->

    <owl:Class rdf:about="http://standards.iso.org/iso/10303/tech/refdata/core#b080d180-130a-0135-b552-598f1b1392ae">
        <rdfs:subClassOf rdf:resource="http://standards.iso.org/iso/10303/tech/refdata/core#59b11220-3279-0135-b58f-598f1b1392ae"/>
        <dc:contributor>STEP Harmonization Team</dc:contributor>
        <dc:creator>Phil Spiby, Eurostep</dc:creator>
        <dc:date>2022-09-01</dc:date>
        <dc:source>ISO/TS 10303-4000</dc:source>
        <dc:type>InWork</dc:type>
        <rdfs:comment xml:lang="en">An OrganizationRelationship is a relationship between two Organization objects.</rdfs:comment>
        <owl:versionInfo>2</owl:versionInfo>
        <skos:changeNote>[2021-07-30] Initial definition.</skos:changeNote>
        <skos:changeNote>[2022-09-01] Phil Spiby, Eurostep: updated comment updated example.</skos:changeNote>
        <skos:example xml:lang="en">A team belongs to a department which itself belongs to a company. Such an organizational structure can be described using instances of OrganizationRelationship.</skos:example>
        <skos:prefLabel xml:lang="en">organization relationship</skos:prefLabel>
    </owl:Class>
    


    <!-- http://standards.iso.org/iso/10303/tech/refdata/core#b0dad860-130a-0135-b552-598f1b1392ae -->

    <owl:Class rdf:about="http://standards.iso.org/iso/10303/tech/refdata/core#b0dad860-130a-0135-b552-598f1b1392ae">
        <rdfs:subClassOf rdf:resource="http://standards.iso.org/iso/10303/tech/refdata/core#STEPThing"/>
        <dc:contributor>STEP Harmonization Team</dc:contributor>
        <dc:creator>Phil Spiby, Eurostep</dc:creator>
        <dc:date>2022-09-01</dc:date>
        <dc:source>ISO/TS 10303-4000</dc:source>
        <dc:type>InWork</dc:type>
        <rdfs:comment xml:lang="en">A Part is an identification of definition of a part. It collects the definitional information of the versions of a part. A Part shall always be categorized as &apos;piece part&apos;, &apos;product&apos;, &apos;software&apos;, &apos;tool&apos;, or &apos;raw material&apos; using a ClassSelect.</rdfs:comment>
        <owl:versionInfo>2</owl:versionInfo>
        <skos:changeNote>[2021-07-30] Initial definition.</skos:changeNote>
        <skos:changeNote>[2022-09-01] Phil Spiby, Eurostep: updated comment updated example updated note.</skos:changeNote>
        <skos:example xml:lang="en">In the context of aeroplanes, a Part can be the airplane as a whole, the assembly of the engine, the body of the airplane, a fender, the side window glass, grease, or a stamping die.</skos:example>
        <skos:example xml:lang="en">In the context of cars, a Part can be the car as a whole, the assembly of the engine, the car body, a fender, the side window glass, grease, or a stamping die.</skos:example>
        <skos:note xml:lang="en">A Part can be either a single piece part, an assembly of arbitrary complexity, a raw material, or a tool.</skos:note>
        <skos:note xml:lang="en">A Part does not represent an actual physical object of the real world.</skos:note>
        <skos:note xml:lang="en">A Part is identified by an organization. The definition of the domain of uniqueness and the mechanism for guaranteeing the uniqueness of Part id are outside the scope of this capability.</skos:note>
        <skos:prefLabel xml:lang="en">part</skos:prefLabel>
    </owl:Class>
    


    <!-- http://standards.iso.org/iso/10303/tech/refdata/core#b1611f60-130a-0135-b552-598f1b1392ae -->

    <owl:Class rdf:about="http://standards.iso.org/iso/10303/tech/refdata/core#b1611f60-130a-0135-b552-598f1b1392ae">
        <rdfs:subClassOf rdf:resource="http://standards.iso.org/iso/10303/tech/refdata/core#59b11220-3279-0135-b58f-598f1b1392ae"/>
        <dc:contributor>STEP Harmonization Team</dc:contributor>
        <dc:creator>Phil Spiby, Eurostep</dc:creator>
        <dc:date>2022-09-01</dc:date>
        <dc:source>ISO/TS 10303-4000</dc:source>
        <dc:type>InWork</dc:type>
        <rdfs:comment xml:lang="en">A PartRelationship is a relationship between two Part objects.</rdfs:comment>
        <owl:versionInfo>1</owl:versionInfo>
        <skos:changeNote>[2021-07-30] Initial definition.</skos:changeNote>
        <skos:prefLabel xml:lang="en">part relationship</skos:prefLabel>
    </owl:Class>
    


    <!-- http://standards.iso.org/iso/10303/tech/refdata/core#b18ea11e-3f47-4345-af66-4ee67c77bc43 -->

    <owl:Class rdf:about="http://standards.iso.org/iso/10303/tech/refdata/core#b18ea11e-3f47-4345-af66-4ee67c77bc43">
        <rdfs:subClassOf rdf:resource="http://standards.iso.org/iso/10303/tech/refdata/core#83b2a250-130a-0135-b552-598f1b1392ae"/>
        <dc:contributor>STEP Harmonization Team</dc:contributor>
        <dc:creator>Phil Spiby, Eurostep</dc:creator>
        <dc:date>2022-09-01</dc:date>
        <dc:source>ISO/TS 10303-4000</dc:source>
        <dc:type>InWork</dc:type>
        <rdfs:comment xml:lang="en">A SchemeSubjectAssignment is an assignment of a Scheme to an item (specified by SchemeSubjectAssignment). The meaning of the assignment can be specified using the ClassifiedAs attribute inherited from the AssignmentObject.</rdfs:comment>
        <owl:versionInfo>1</owl:versionInfo>
        <skos:changeNote>[2022-09-01] Initial definition.</skos:changeNote>
        <skos:example xml:lang="en">The maintenance plan for an individual vehicle, where the subject attribute points to an entity instance representing that vehicle.</skos:example>
        <skos:note xml:lang="en">The SchemeSubjectAssignment links the Plans and Schedules with their associated subjects or targets. This can indicate the intent of the scheme.</skos:note>
        <skos:prefLabel xml:lang="en">scheme subject assignment</skos:prefLabel>
    </owl:Class>
    


    <!-- http://standards.iso.org/iso/10303/tech/refdata/core#b1ef00ee-9800-4df4-af83-f1cbb97213df -->

    <owl:Class rdf:about="http://standards.iso.org/iso/10303/tech/refdata/core#b1ef00ee-9800-4df4-af83-f1cbb97213df">
        <rdfs:subClassOf rdf:resource="http://standards.iso.org/iso/10303/tech/refdata/core#09cd1ad9-ed18-4c44-a399-eb27b8148d42"/>
        <dc:contributor>STEP Harmonization Team</dc:contributor>
        <dc:creator>Jean Brangé, AFNeT Services</dc:creator>
        <dc:date>2023-10-04</dc:date>
        <dc:source>ISO/TS 10303-4000</dc:source>
        <dc:type>InWork</dc:type>
        <rdfs:comment xml:lang="en">A CableOccurrenceTerminal is a type of OccurrenceTerminal for the identification of a terminal on a CableOccurrence. The terminal may be located at one of the ends or somewhere in the middle of a wire in the cable.</rdfs:comment>
        <owl:versionInfo>3</owl:versionInfo>
        <skos:changeNote>[2023-10-04] Jean Brangé, AFNeT Services: Initial definition.</skos:changeNote>
        <skos:prefLabel xml:lang="en">cable occurrence terminal</skos:prefLabel>
    </owl:Class>
    


    <!-- http://standards.iso.org/iso/10303/tech/refdata/core#b1fe8c11-8479-4e7c-9862-abc974661cd5 -->

    <owl:Class rdf:about="http://standards.iso.org/iso/10303/tech/refdata/core#b1fe8c11-8479-4e7c-9862-abc974661cd5">
        <rdfs:subClassOf rdf:resource="http://standards.iso.org/iso/10303/tech/refdata/core#1cfca290-3279-0135-b58f-598f1b1392ae"/>
        <dc:contributor>STEP Harmonization Team</dc:contributor>
        <dc:creator>Jean Brangé, AFNeT Services</dc:creator>
        <dc:date>2023-10-04</dc:date>
        <dc:source>ISO/TS 10303-4000</dc:source>
        <dc:type>InWork</dc:type>
        <rdfs:comment xml:lang="en">A ModelPropertyAssignment is an assignment of a ModelProperty to objects.</rdfs:comment>
        <owl:versionInfo>3</owl:versionInfo>
        <skos:changeNote>[2023-10-04] Jean Brangé, AFNeT Services: Initial definition.</skos:changeNote>
        <skos:example xml:lang="en">In the case of a welding operation, the welding points as a part of a wireframe model can be associated with a process operation to describe the locations where the robot has to weld for a welding process operation.</skos:example>
        <skos:prefLabel xml:lang="en">model property assignment</skos:prefLabel>
    </owl:Class>
    


    <!-- http://standards.iso.org/iso/10303/tech/refdata/core#b2046440-130a-0135-b552-598f1b1392ae -->

    <owl:Class rdf:about="http://standards.iso.org/iso/10303/tech/refdata/core#b2046440-130a-0135-b552-598f1b1392ae">
        <rdfs:subClassOf rdf:resource="http://standards.iso.org/iso/10303/tech/refdata/core#1d59c650-3279-0135-b58f-598f1b1392ae"/>
        <dc:contributor>STEP Harmonization Team</dc:contributor>
        <dc:creator>Phil Spiby, Eurostep</dc:creator>
        <dc:date>2022-09-01</dc:date>
        <dc:source>ISO/TS 10303-4000</dc:source>
        <dc:type>InWork</dc:type>
        <rdfs:comment xml:lang="en">A PartToIndividualPartAssociation is an association between a design, represented by Part, and the part that is planned to be made or has been made from the design, represented by IndividualPart.</rdfs:comment>
        <owl:versionInfo>1</owl:versionInfo>
        <skos:changeNote>[2021-07-30] Initial definition.</skos:changeNote>
        <skos:prefLabel xml:lang="en">part to individual part association</skos:prefLabel>
    </owl:Class>
    


    <!-- http://standards.iso.org/iso/10303/tech/refdata/core#b24a9500-130a-0135-b552-598f1b1392ae -->

    <owl:Class rdf:about="http://standards.iso.org/iso/10303/tech/refdata/core#b24a9500-130a-0135-b552-598f1b1392ae">
        <rdfs:subClassOf rdf:resource="http://standards.iso.org/iso/10303/tech/refdata/core#STEPThing"/>
        <dc:contributor>STEP Harmonization Team</dc:contributor>
        <dc:creator>Phil Spiby, Eurostep</dc:creator>
        <dc:date>2022-09-01</dc:date>
        <dc:source>ISO/TS 10303-4000</dc:source>
        <dc:type>InWork</dc:type>
        <rdfs:comment xml:lang="en">A PartVersion is an identification of a version of a part. It serves as the collector of the data characterizing a realizable object in various application contexts.</rdfs:comment>
        <owl:versionInfo>2</owl:versionInfo>
        <skos:changeNote>[2021-07-30] Initial definition.</skos:changeNote>
        <skos:changeNote>[2022-09-01] Phil Spiby, Eurostep: updated note.</skos:changeNote>
        <skos:note xml:lang="en">A PartVersion does not have to be referenced by any PartView.</skos:note>
        <skos:note xml:lang="en">A PartVersion is a part that can be produced, consumed, used to produce other PartVersion objects, or offered to the market.</skos:note>
        <skos:note xml:lang="en">The collection of defining information can be incomplete, in this case not all of the PartView objects needed to define a PartVersion are associated with the PartVersion.</skos:note>
        <skos:note xml:lang="en">The set of all PartVersion objects of a Part represents the history of the Part within a specific life-cycle stage or over its complete life cycle.</skos:note>
        <skos:prefLabel xml:lang="en">part version</skos:prefLabel>
    </owl:Class>
    


    <!-- http://standards.iso.org/iso/10303/tech/refdata/core#b28a5c59-702a-4368-8eac-fa5dde6a1fbd -->

    <owl:Class rdf:about="http://standards.iso.org/iso/10303/tech/refdata/core#b28a5c59-702a-4368-8eac-fa5dde6a1fbd">
        <rdfs:subClassOf rdf:resource="http://standards.iso.org/iso/10303/tech/refdata/core#STEPThing"/>
        <dc:contributor>STEP Harmonization Team</dc:contributor>
        <dc:creator>Phil Spiby, Eurostep</dc:creator>
        <dc:date>2022-09-01</dc:date>
        <dc:source>ISO/TS 10303-4000</dc:source>
        <dc:type>InWork</dc:type>
        <rdfs:comment xml:lang="en">A CollectionVersion is a revision of a Collection.</rdfs:comment>
        <owl:versionInfo>1</owl:versionInfo>
        <skos:changeNote>[2021-07-30] Initial definition.</skos:changeNote>
        <skos:prefLabel xml:lang="en">collection version</skos:prefLabel>
    </owl:Class>
    


    <!-- http://standards.iso.org/iso/10303/tech/refdata/core#b2a318e9-3343-471c-baf7-6517a3c5702f -->

    <owl:Class rdf:about="http://standards.iso.org/iso/10303/tech/refdata/core#b2a318e9-3343-471c-baf7-6517a3c5702f">
        <rdfs:subClassOf rdf:resource="http://standards.iso.org/iso/10303/tech/refdata/core#59b11220-3279-0135-b58f-598f1b1392ae"/>
        <dc:contributor>STEP Harmonization Team</dc:contributor>
        <dc:creator>Phil Spiby, Eurostep</dc:creator>
        <dc:date>2022-09-01</dc:date>
        <dc:source>ISO/TS 10303-4000</dc:source>
        <dc:type>InWork</dc:type>
        <rdfs:comment xml:lang="en">A SlotPlannedToRealized is a relationship between a realized individual of a slot and a corresponding planned individual.</rdfs:comment>
        <owl:versionInfo>1</owl:versionInfo>
        <skos:changeNote>[2022-09-01] Initial definition.</skos:changeNote>
        <skos:example xml:lang="en">WeMakeBigPlanes Limited builds aircraft serial number 2468 with a starboard engine attachment slot that was previously planned.</skos:example>
        <skos:prefLabel xml:lang="en">slot planned to realized</skos:prefLabel>
    </owl:Class>
    


    <!-- http://standards.iso.org/iso/10303/tech/refdata/core#b2dce9f0-130a-0135-b552-598f1b1392ae -->

    <owl:Class rdf:about="http://standards.iso.org/iso/10303/tech/refdata/core#b2dce9f0-130a-0135-b552-598f1b1392ae">
        <rdfs:subClassOf rdf:resource="http://standards.iso.org/iso/10303/tech/refdata/core#59b11220-3279-0135-b58f-598f1b1392ae"/>
        <dc:contributor>STEP Harmonization Team</dc:contributor>
        <dc:creator>Phil Spiby, Eurostep</dc:creator>
        <dc:date>2022-09-01</dc:date>
        <dc:source>ISO/TS 10303-4000</dc:source>
        <dc:type>InWork</dc:type>
        <rdfs:comment xml:lang="en">A PartVersionRelationship is a relationship between two PartVersion objects. Unless specified in a specialization of this object, this relationship does not involve inheritance of data between the two related objects.</rdfs:comment>
        <owl:versionInfo>2</owl:versionInfo>
        <skos:changeNote>[2021-07-30] Initial definition.</skos:changeNote>
        <skos:changeNote>[2022-09-01] Phil Spiby, Eurostep: updated comment.</skos:changeNote>
        <skos:prefLabel xml:lang="en">part version relationship</skos:prefLabel>
    </owl:Class>
    


    <!-- http://standards.iso.org/iso/10303/tech/refdata/core#b2e7bb78-e7e8-4c36-8f9d-2dc6845e626e -->

    <owl:Class rdf:about="http://standards.iso.org/iso/10303/tech/refdata/core#b2e7bb78-e7e8-4c36-8f9d-2dc6845e626e">
        <rdfs:subClassOf rdf:resource="http://standards.iso.org/iso/10303/tech/refdata/core#89f36b81-3d5e-48dd-90fc-80eaf4d96f3e"/>
        <dc:contributor>STEP Harmonization Team</dc:contributor>
        <dc:creator>Phil Spiby, Eurostep</dc:creator>
        <dc:date>2022-09-01</dc:date>
        <dc:source>ISO/TS 10303-4000</dc:source>
        <dc:type>InWork</dc:type>
        <rdfs:comment xml:lang="en">An AnalysisModel is used to support the description of Analysis concepts.</rdfs:comment>
        <owl:versionInfo>1</owl:versionInfo>
        <skos:changeNote>[2021-07-30] Initial definition.</skos:changeNote>
        <skos:prefLabel xml:lang="en">analysis model</skos:prefLabel>
    </owl:Class>
    


    <!-- http://standards.iso.org/iso/10303/tech/refdata/core#b332c8dc-450f-47e2-aa79-ac74fb43d7b3 -->

    <owl:Class rdf:about="http://standards.iso.org/iso/10303/tech/refdata/core#b332c8dc-450f-47e2-aa79-ac74fb43d7b3">
        <rdfs:subClassOf rdf:resource="http://standards.iso.org/iso/10303/tech/refdata/core#83b2a250-130a-0135-b552-598f1b1392ae"/>
        <dc:contributor>STEP Harmonization Team</dc:contributor>
        <dc:creator>Phil Spiby, Eurostep</dc:creator>
        <dc:date>2022-09-01</dc:date>
        <dc:source>ISO/TS 10303-4000</dc:source>
        <dc:type>InWork</dc:type>
        <rdfs:comment xml:lang="en">A TaskMethodVersionAssignment is an assignment of a TaskMethodVersion to an item (specified by TaskAssignmentSelect). The meaning of the assignment can be specified using the ClassifiedAs attribute inherited from the AssignmentObject.</rdfs:comment>
        <owl:versionInfo>2</owl:versionInfo>
        <skos:changeNote>[2021-07-30] Initial definition.</skos:changeNote>
        <skos:changeNote>[2022-09-01] Phil Spiby, Eurostep: updated comment updated note.</skos:changeNote>
        <skos:prefLabel xml:lang="en">task method version assignment</skos:prefLabel>
    </owl:Class>
    


    <!-- http://standards.iso.org/iso/10303/tech/refdata/core#b339f638-2dc5-41d4-8b5b-4da57eb5ad71 -->

    <owl:Class rdf:about="http://standards.iso.org/iso/10303/tech/refdata/core#b339f638-2dc5-41d4-8b5b-4da57eb5ad71">
        <rdfs:subClassOf rdf:resource="http://standards.iso.org/iso/10303/tech/refdata/core#44078e31-a1cb-4d89-b8d6-ab60b9140b06"/>
        <dc:contributor>STEP Harmonization Team</dc:contributor>
        <dc:creator>Jean Brangé, AFNeT Services</dc:creator>
        <dc:date>2023-10-04</dc:date>
        <dc:source>ISO/TS 10303-4000</dc:source>
        <dc:type>InWork</dc:type>
        <rdfs:comment xml:lang="en">A TargetCircularCurve is a type of PlacedTarget that specifies a DatumTarget that is defined by an implicit circular curve. The centre of the circle is specified by the placing AxisPlacement. The orientation of the TargetCircle is the x-y-plane of the AxisPlacement.</rdfs:comment>
        <owl:versionInfo>3</owl:versionInfo>
        <skos:changeNote>[2023-10-04] Jean Brangé, AFNeT Services: Initial definition.</skos:changeNote>
        <skos:prefLabel xml:lang="en">target circular curve</skos:prefLabel>
    </owl:Class>
    


    <!-- http://standards.iso.org/iso/10303/tech/refdata/core#b347e0c0-130a-0135-b552-598f1b1392ae -->

    <owl:Class rdf:about="http://standards.iso.org/iso/10303/tech/refdata/core#b347e0c0-130a-0135-b552-598f1b1392ae">
        <rdfs:subClassOf rdf:resource="http://standards.iso.org/iso/10303/tech/refdata/core#1d59c650-3279-0135-b58f-598f1b1392ae"/>
        <dc:contributor>STEP Harmonization Team</dc:contributor>
        <dc:creator>Phil Spiby, Eurostep</dc:creator>
        <dc:date>2022-09-01</dc:date>
        <dc:source>ISO/TS 10303-4000</dc:source>
        <dc:type>InWork</dc:type>
        <rdfs:comment xml:lang="en">A PartVersionToIndividualPartVersionAssociation is an association between a version of a design (specified by PartVersionOrProductConfigurationSelect), and the part version that is planned to be made or has been made from the design (via IndividualPartVersion).</rdfs:comment>
        <owl:versionInfo>2</owl:versionInfo>
        <skos:changeNote>[2021-07-30] Initial definition.</skos:changeNote>
        <skos:changeNote>[2022-09-01] Phil Spiby, Eurostep: updated comment.</skos:changeNote>
        <skos:prefLabel xml:lang="en">part version to individual part version association</skos:prefLabel>
    </owl:Class>
    


    <!-- http://standards.iso.org/iso/10303/tech/refdata/core#b35626d3-b304-473d-9394-3e453c8d8bb7 -->

    <owl:Class rdf:about="http://standards.iso.org/iso/10303/tech/refdata/core#b35626d3-b304-473d-9394-3e453c8d8bb7">
        <rdfs:subClassOf rdf:resource="http://standards.iso.org/iso/10303/tech/refdata/core#STEPThing"/>
        <dc:contributor>STEP Harmonization Team</dc:contributor>
        <dc:creator>Phil Spiby, Eurostep</dc:creator>
        <dc:date>2022-09-01</dc:date>
        <dc:source>ISO/TS 10303-4000</dc:source>
        <dc:type>InWork</dc:type>
        <rdfs:comment xml:lang="en">A ConditionEvaluationParameter is an identification of an item (specified by ConditionEvaluationParameterSelect) used in a ConditionEvaluation.</rdfs:comment>
        <owl:versionInfo>1</owl:versionInfo>
        <skos:changeNote>[2021-07-30] Initial definition.</skos:changeNote>
        <skos:example xml:lang="en">The measured value of oil pressure from gauge 3 on car with VIN 12345678 (value = 1.9 bar).</skos:example>
        <skos:prefLabel xml:lang="en">condition evaluation parameter</skos:prefLabel>
    </owl:Class>
    


    <!-- http://standards.iso.org/iso/10303/tech/refdata/core#b3585f65-ea84-436d-9c61-15f59910294b -->

    <owl:Class rdf:about="http://standards.iso.org/iso/10303/tech/refdata/core#b3585f65-ea84-436d-9c61-15f59910294b">
        <rdfs:subClassOf rdf:resource="http://standards.iso.org/iso/10303/tech/refdata/core#1f09cf40-e045-476a-b811-eb6e56de0ced"/>
        <dc:contributor>STEP Harmonization Team</dc:contributor>
        <dc:creator>Jean Brangé, AFNeT Services</dc:creator>
        <dc:date>2023-10-04</dc:date>
        <dc:source>ISO/TS 10303-4000</dc:source>
        <dc:type>InWork</dc:type>
        <rdfs:comment xml:lang="en">A CurvedDistance is a type of DimensionalLocation that represents the arc length along a curve.</rdfs:comment>
        <owl:versionInfo>3</owl:versionInfo>
        <skos:changeNote>[2023-10-04] Jean Brangé, AFNeT Services: Initial definition.</skos:changeNote>
        <skos:prefLabel xml:lang="en">curved distance</skos:prefLabel>
    </owl:Class>
    


    <!-- http://standards.iso.org/iso/10303/tech/refdata/core#b358c76a-a60a-41b0-9a38-76bf0afd568c -->

    <owl:Class rdf:about="http://standards.iso.org/iso/10303/tech/refdata/core#b358c76a-a60a-41b0-9a38-76bf0afd568c">
        <rdfs:subClassOf rdf:resource="http://standards.iso.org/iso/10303/tech/refdata/core#STEPThing"/>
        <dc:contributor>STEP Harmonization Team</dc:contributor>
        <dc:creator>Phil Spiby, Eurostep</dc:creator>
        <dc:date>2022-09-01</dc:date>
        <dc:source>ISO/TS 10303-4000</dc:source>
        <dc:type>InWork</dc:type>
        <rdfs:comment xml:lang="en">An Observation is an historical record of something that has occurred during the life of a product or its support environment. Its use is restricted to observations not directly represented in the data model, and should not be used where some other reporting data structure is defined.</rdfs:comment>
        <owl:versionInfo>1</owl:versionInfo>
        <skos:changeNote>[2022-09-01] Initial definition.</skos:changeNote>
        <skos:prefLabel xml:lang="en">observation</skos:prefLabel>
    </owl:Class>
    


    <!-- http://standards.iso.org/iso/10303/tech/refdata/core#b37d68d8-df6e-4ed0-a748-89f3942af44f -->

    <owl:Class rdf:about="http://standards.iso.org/iso/10303/tech/refdata/core#b37d68d8-df6e-4ed0-a748-89f3942af44f">
        <rdfs:subClassOf rdf:resource="http://standards.iso.org/iso/10303/tech/refdata/core#55105ef0-713f-409a-8306-fd8708d4ee3f"/>
        <dc:contributor>STEP Harmonization Team</dc:contributor>
        <dc:creator>Jean Brangé, AFNeT Services</dc:creator>
        <dc:date>2023-10-04</dc:date>
        <dc:source>ISO/TS 10303-4000</dc:source>
        <dc:type>InWork</dc:type>
        <rdfs:comment xml:lang="en">A StraightnessTolerance is a type of GeometricTolerance that specifies a tolerance zone within which the considered element of a feature or a derived median line must lie. Unless otherwise specified, the rules governing straightness tolerance defined in ISO 1101 shall apply. The toleranced shape element is a surface or a straight line. Refer to the definition of straightness tolerance in ISO 1101 for a description of the different tolerance zones. In the case of intersection curves, the ideal features corresponding to the intersection curves shall be linear and there shall be another ShapeElement, which is related to the toleranced shape element by a ShapeElementRelationship.</rdfs:comment>
        <owl:versionInfo>3</owl:versionInfo>
        <skos:changeNote>[2023-10-04] Jean Brangé, AFNeT Services: Initial definition.</skos:changeNote>
        <skos:note xml:lang="en">Alternatively straightness tolerance can be used according to the specifications given in ASME Y14.5-2009.</skos:note>
        <skos:prefLabel xml:lang="en">straightness tolerance</skos:prefLabel>
    </owl:Class>
    


    <!-- http://standards.iso.org/iso/10303/tech/refdata/core#b3911ec0-130a-0135-b552-598f1b1392ae -->

    <owl:Class rdf:about="http://standards.iso.org/iso/10303/tech/refdata/core#b3911ec0-130a-0135-b552-598f1b1392ae">
        <rdfs:subClassOf rdf:resource="http://standards.iso.org/iso/10303/tech/refdata/core#STEPThing"/>
        <dc:contributor>STEP Harmonization Team</dc:contributor>
        <dc:creator>Phil Spiby, Eurostep</dc:creator>
        <dc:date>2022-09-01</dc:date>
        <dc:source>ISO/TS 10303-4000</dc:source>
        <dc:type>InWork</dc:type>
        <rdfs:comment xml:lang="en">A PartView is a view of a Part with respect to specific criteria.</rdfs:comment>
        <owl:versionInfo>1</owl:versionInfo>
        <skos:changeNote>[2021-07-30] Initial definition.</skos:changeNote>
        <skos:prefLabel xml:lang="en">part view</skos:prefLabel>
    </owl:Class>
    


    <!-- http://standards.iso.org/iso/10303/tech/refdata/core#b3a9b996-c18c-4464-b398-d16e36d6711a -->

    <owl:Class rdf:about="http://standards.iso.org/iso/10303/tech/refdata/core#b3a9b996-c18c-4464-b398-d16e36d6711a">
        <rdfs:subClassOf rdf:resource="http://standards.iso.org/iso/10303/tech/refdata/core#9fee6ad0-130a-0135-b552-598f1b1392ae"/>
        <dc:contributor>STEP Harmonization Team</dc:contributor>
        <dc:creator>Jean Brangé, AFNeT Services</dc:creator>
        <dc:date>2023-10-04</dc:date>
        <dc:source>ISO/TS 10303-4000</dc:source>
        <dc:type>InWork</dc:type>
        <rdfs:comment xml:lang="en">A ConstituentShapeRepresentation is a type of GeometricRepresentation. It is the shape representation of composite part constituents. A ConstituentShapeRepresentation is one of the following: ThreeDGeometrySet, BeveledSheetRepresentation. CompositeSheetRepresentation.</rdfs:comment>
        <owl:versionInfo>3</owl:versionInfo>
        <skos:changeNote>[2023-10-04] Jean Brangé, AFNeT Services: Initial definition.</skos:changeNote>
        <skos:prefLabel xml:lang="en">constituent shape representation</skos:prefLabel>
    </owl:Class>
    


    <!-- http://standards.iso.org/iso/10303/tech/refdata/core#b44098a0-130a-0135-b552-598f1b1392ae -->

    <owl:Class rdf:about="http://standards.iso.org/iso/10303/tech/refdata/core#b44098a0-130a-0135-b552-598f1b1392ae">
        <rdfs:subClassOf rdf:resource="http://standards.iso.org/iso/10303/tech/refdata/core#59b11220-3279-0135-b58f-598f1b1392ae"/>
        <dc:contributor>STEP Harmonization Team</dc:contributor>
        <dc:creator>Phil Spiby, Eurostep</dc:creator>
        <dc:date>2022-09-01</dc:date>
        <dc:source>ISO/TS 10303-4000</dc:source>
        <dc:type>InWork</dc:type>
        <rdfs:comment xml:lang="en">A PartViewRelationship is a relationship between two PartView objects.</rdfs:comment>
        <owl:versionInfo>2</owl:versionInfo>
        <skos:changeNote>[2021-07-30] Initial definition.</skos:changeNote>
        <skos:changeNote>[2022-09-01] Phil Spiby, Eurostep: updated comment.</skos:changeNote>
        <skos:prefLabel xml:lang="en">part view relationship</skos:prefLabel>
    </owl:Class>
    


    <!-- http://standards.iso.org/iso/10303/tech/refdata/core#b4baaaa0-130a-0135-b552-598f1b1392ae -->

    <owl:Class rdf:about="http://standards.iso.org/iso/10303/tech/refdata/core#b4baaaa0-130a-0135-b552-598f1b1392ae">
        <rdfs:subClassOf rdf:resource="http://standards.iso.org/iso/10303/tech/refdata/core#1d59c650-3279-0135-b58f-598f1b1392ae"/>
        <dc:contributor>STEP Harmonization Team</dc:contributor>
        <dc:creator>Phil Spiby, Eurostep</dc:creator>
        <dc:date>2022-09-01</dc:date>
        <dc:source>ISO/TS 10303-4000</dc:source>
        <dc:type>InWork</dc:type>
        <rdfs:comment xml:lang="en">A PartViewToIndividualPartViewAssociation is an association between a design (specified by PartViewOrProductConfigurationSelect) and a view of the part that is planned to be made or has been made from the design, represented by IndividualPartView.</rdfs:comment>
        <owl:versionInfo>2</owl:versionInfo>
        <skos:changeNote>[2021-07-30] Initial definition.</skos:changeNote>
        <skos:changeNote>[2022-09-01] Phil Spiby, Eurostep: updated comment.</skos:changeNote>
        <skos:prefLabel xml:lang="en">part view to individual part view association</skos:prefLabel>
    </owl:Class>
    


    <!-- http://standards.iso.org/iso/10303/tech/refdata/core#b5a11300-130a-0135-b552-598f1b1392ae -->

    <owl:Class rdf:about="http://standards.iso.org/iso/10303/tech/refdata/core#b5a11300-130a-0135-b552-598f1b1392ae">
        <rdfs:subClassOf rdf:resource="http://standards.iso.org/iso/10303/tech/refdata/core#STEPThing"/>
        <dc:contributor>STEP Harmonization Team</dc:contributor>
        <dc:creator>Phil Spiby, Eurostep</dc:creator>
        <dc:date>2022-09-01</dc:date>
        <dc:source>ISO/TS 10303-4000</dc:source>
        <dc:type>InWork</dc:type>
        <rdfs:comment xml:lang="en">A Person is an individual human being.</rdfs:comment>
        <owl:versionInfo>1</owl:versionInfo>
        <skos:changeNote>[2021-07-30] Initial definition.</skos:changeNote>
        <skos:prefLabel xml:lang="en">person</skos:prefLabel>
    </owl:Class>
    


    <!-- http://standards.iso.org/iso/10303/tech/refdata/core#b608a929-7fa0-4643-8237-59c6cf4d0dbc -->

    <owl:Class rdf:about="http://standards.iso.org/iso/10303/tech/refdata/core#b608a929-7fa0-4643-8237-59c6cf4d0dbc">
        <rdfs:subClassOf rdf:resource="http://standards.iso.org/iso/10303/tech/refdata/core#5de267f0-5f95-4318-ab51-e6552200a8d7"/>
        <dc:contributor>STEP Harmonization Team</dc:contributor>
        <dc:creator>Jean Brangé, AFNeT Services</dc:creator>
        <dc:date>2023-10-04</dc:date>
        <dc:source>ISO/TS 10303-4000</dc:source>
        <dc:type>InWork</dc:type>
        <rdfs:comment xml:lang="en">An OccurrenceShapeFeature is a type of OccurrenceShapeElement that is a definitional part of the shape of an Occurrence or of another OccurrenceShapeFeature.</rdfs:comment>
        <owl:versionInfo>3</owl:versionInfo>
        <skos:changeNote>[2023-10-04] Jean Brangé, AFNeT Services: Initial definition.</skos:changeNote>
        <skos:prefLabel xml:lang="en">occurrence shape feature</skos:prefLabel>
    </owl:Class>
    


    <!-- http://standards.iso.org/iso/10303/tech/refdata/core#b62a6740-130a-0135-b552-598f1b1392ae -->

    <owl:Class rdf:about="http://standards.iso.org/iso/10303/tech/refdata/core#b62a6740-130a-0135-b552-598f1b1392ae">
        <rdfs:subClassOf rdf:resource="http://standards.iso.org/iso/10303/tech/refdata/core#STEPThing"/>
        <dc:contributor>STEP Harmonization Team</dc:contributor>
        <dc:creator>Phil Spiby, Eurostep</dc:creator>
        <dc:date>2022-09-01</dc:date>
        <dc:source>ISO/TS 10303-4000</dc:source>
        <dc:type>InWork</dc:type>
        <rdfs:comment xml:lang="en">A PersonInOrganization is the specification of a Person in the context of an Organization.</rdfs:comment>
        <owl:versionInfo>1</owl:versionInfo>
        <skos:changeNote>[2021-07-30] Initial definition.</skos:changeNote>
        <skos:prefLabel xml:lang="en">person in organization</skos:prefLabel>
    </owl:Class>
    


    <!-- http://standards.iso.org/iso/10303/tech/refdata/core#b636774a-e24a-444c-a45f-aa0fd1928b85 -->

    <owl:Class rdf:about="http://standards.iso.org/iso/10303/tech/refdata/core#b636774a-e24a-444c-a45f-aa0fd1928b85">
        <rdfs:subClassOf rdf:resource="http://standards.iso.org/iso/10303/tech/refdata/core#19573db2-1baa-4bad-acc6-010eef852d49"/>
        <dc:contributor>STEP Harmonization Team</dc:contributor>
        <dc:creator>Phil Spiby, Eurostep</dc:creator>
        <dc:date>2022-09-01</dc:date>
        <dc:source>ISO/TS 10303-4000</dc:source>
        <dc:type>InWork</dc:type>
        <rdfs:comment xml:lang="en">A StateObserved is a type of State. It represents a state that something has been observed to be in. This can be confirmed by measurement, or simply hypothesized.</rdfs:comment>
        <owl:versionInfo>2</owl:versionInfo>
        <skos:changeNote>[2021-07-30] Initial definition.</skos:changeNote>
        <skos:changeNote>[2022-09-01] Phil Spiby, Eurostep: updated comment.</skos:changeNote>
        <skos:prefLabel xml:lang="en">state observed</skos:prefLabel>
    </owl:Class>
    


    <!-- http://standards.iso.org/iso/10303/tech/refdata/core#b6b3bb80-130a-0135-b552-598f1b1392ae -->

    <owl:Class rdf:about="http://standards.iso.org/iso/10303/tech/refdata/core#b6b3bb80-130a-0135-b552-598f1b1392ae">
        <rdfs:subClassOf rdf:resource="http://standards.iso.org/iso/10303/tech/refdata/core#59b11220-3279-0135-b58f-598f1b1392ae"/>
        <dc:contributor>STEP Harmonization Team</dc:contributor>
        <dc:creator>Phil Spiby, Eurostep</dc:creator>
        <dc:date>2022-09-01</dc:date>
        <dc:source>ISO/TS 10303-4000</dc:source>
        <dc:type>InWork</dc:type>
        <rdfs:comment xml:lang="en">A PersonInOrganizationRelationship is a relationship between two PersonInOrganization objects.</rdfs:comment>
        <owl:versionInfo>2</owl:versionInfo>
        <skos:changeNote>[2021-07-30] Initial definition.</skos:changeNote>
        <skos:changeNote>[2022-09-01] Phil Spiby, Eurostep: updated comment updated example.</skos:changeNote>
        <skos:example xml:lang="en">The owner of important product data leaves a company and therefore has a successor. This relationship can be built up using the PersonInOrganizationRelationship.</skos:example>
        <skos:prefLabel xml:lang="en">person in organization relationship</skos:prefLabel>
    </owl:Class>
    


    <!-- http://standards.iso.org/iso/10303/tech/refdata/core#b6cd9d2d-5c0e-4bc7-8d49-1087c6b0b727 -->

    <owl:Class rdf:about="http://standards.iso.org/iso/10303/tech/refdata/core#b6cd9d2d-5c0e-4bc7-8d49-1087c6b0b727">
        <rdfs:subClassOf rdf:resource="http://standards.iso.org/iso/10303/tech/refdata/core#STEPThing"/>
        <dc:contributor>STEP Harmonization Team</dc:contributor>
        <dc:creator>Phil Spiby, Eurostep</dc:creator>
        <dc:date>2022-09-01</dc:date>
        <dc:source>ISO/TS 10303-4000</dc:source>
        <dc:type>InWork</dc:type>
        <rdfs:comment xml:lang="en">A Slot represents the position in which a part is or can be attached.</rdfs:comment>
        <owl:versionInfo>1</owl:versionInfo>
        <skos:changeNote>[2022-09-01] Initial definition.</skos:changeNote>
        <skos:example xml:lang="en">A fast jet aircraft has two engines. These engines are removable and interchangeable between individual aircraft. An attachment slot represents each installation position for an engine so as to ensure that an accurate record is maintained of which engines fly in which pairing on which aircraft for how many hours. A rack has several shelfs, where PCB-cards can be installed. Each position/shelf is considered a slot. The PCB-cards are in this case considered as parts.</skos:example>
        <skos:prefLabel xml:lang="en">slot</skos:prefLabel>
    </owl:Class>
    


    <!-- http://standards.iso.org/iso/10303/tech/refdata/core#b70ab520-130a-0135-b552-598f1b1392ae -->

    <owl:Class rdf:about="http://standards.iso.org/iso/10303/tech/refdata/core#b70ab520-130a-0135-b552-598f1b1392ae">
        <rdfs:subClassOf rdf:resource="http://standards.iso.org/iso/10303/tech/refdata/core#96c60e90-130a-0135-b552-598f1b1392ae"/>
        <dc:contributor>STEP Harmonization Team</dc:contributor>
        <dc:creator>Phil Spiby, Eurostep</dc:creator>
        <dc:date>2022-09-01</dc:date>
        <dc:source>ISO/TS 10303-4000</dc:source>
        <dc:type>InWork</dc:type>
        <rdfs:comment xml:lang="en">A PhysicalDocumentDefinition is a type of DocumentDefinition describing a piece of product data that is archived in a non-digital form.</rdfs:comment>
        <owl:versionInfo>1</owl:versionInfo>
        <skos:changeNote>[2021-07-30] Initial definition.</skos:changeNote>
        <skos:example xml:lang="en">Paper plots of technical drawings, micro fiche, or paper documents such as calculations or test reports are examples for a PhysicalDocumentDefinition.</skos:example>
        <skos:prefLabel xml:lang="en">physical document definition</skos:prefLabel>
    </owl:Class>
    


    <!-- http://standards.iso.org/iso/10303/tech/refdata/core#b72f5420-130a-0135-b552-598f1b1392ae -->

    <owl:Class rdf:about="http://standards.iso.org/iso/10303/tech/refdata/core#b72f5420-130a-0135-b552-598f1b1392ae">
        <rdfs:subClassOf rdf:resource="http://standards.iso.org/iso/10303/tech/refdata/core#8276c6f0-130a-0135-b552-598f1b1392ae"/>
        <dc:contributor>STEP Harmonization Team</dc:contributor>
        <dc:creator>Phil Spiby, Eurostep</dc:creator>
        <dc:date>2022-09-01</dc:date>
        <dc:source>ISO/TS 10303-4000</dc:source>
        <dc:type>InWork</dc:type>
        <rdfs:comment xml:lang="en">A PlannedActivity is a type of Activity that identifies a predicted Activity that is expected to take place in the future.</rdfs:comment>
        <owl:versionInfo>1</owl:versionInfo>
        <skos:changeNote>[2021-07-30] Initial definition.</skos:changeNote>
        <skos:prefLabel xml:lang="en">planned activity</skos:prefLabel>
    </owl:Class>
    


    <!-- http://standards.iso.org/iso/10303/tech/refdata/core#b77b9f60-130a-0135-b552-598f1b1392ae -->

    <owl:Class rdf:about="http://standards.iso.org/iso/10303/tech/refdata/core#b77b9f60-130a-0135-b552-598f1b1392ae">
        <rdfs:subClassOf rdf:resource="http://standards.iso.org/iso/10303/tech/refdata/core#a3571140-130a-0135-b552-598f1b1392ae"/>
        <dc:contributor>STEP Harmonization Team</dc:contributor>
        <dc:creator>Phil Spiby, Eurostep</dc:creator>
        <dc:date>2022-09-01</dc:date>
        <dc:source>ISO/TS 10303-4000</dc:source>
        <dc:type>InWork</dc:type>
        <rdfs:comment xml:lang="en">A PlannedIndividualPart is a type of IndividualPartVersion that represents a version of a planned artefact.</rdfs:comment>
        <owl:versionInfo>2</owl:versionInfo>
        <skos:changeNote>[2021-07-30] Initial definition.</skos:changeNote>
        <skos:changeNote>[2022-09-01] Phil Spiby, Eurostep: updated note.</skos:changeNote>
        <skos:note xml:lang="en">If the planned artefact (PlannedIndividualPart) is subsequently made into an actual artefact (RealizedIndividualPart) then they are related by the ProductPlannedToRealized relationship.</skos:note>
        <skos:note xml:lang="en">It can be planned to make the artefact from of a version of a part design (PartVersion). If this is the case, then the relationship between the artefact (PlannedIndividualPart) and the design (PartVersion) is represented by PartVersionToIndividualPartVersionAssociation.</skos:note>
        <skos:prefLabel xml:lang="en">planned individual part</skos:prefLabel>
    </owl:Class>
    


    <!-- http://standards.iso.org/iso/10303/tech/refdata/core#b7a6ee4f-98ab-43c4-aa58-afccd17c8302 -->

    <owl:Class rdf:about="http://standards.iso.org/iso/10303/tech/refdata/core#b7a6ee4f-98ab-43c4-aa58-afccd17c8302">
        <rdfs:subClassOf rdf:resource="http://standards.iso.org/iso/10303/tech/refdata/core#STEPThing"/>
        <dc:contributor>STEP Harmonization Team</dc:contributor>
        <dc:creator>Phil Spiby, Eurostep</dc:creator>
        <dc:date>2022-09-01</dc:date>
        <dc:source>ISO/TS 10303-4000</dc:source>
        <dc:type>InWork</dc:type>
        <rdfs:comment xml:lang="en">A SystemView provides a view of a system version relevant for one or more application domains.</rdfs:comment>
        <owl:versionInfo>1</owl:versionInfo>
        <skos:changeNote>[2022-09-01] Initial definition.</skos:changeNote>
        <skos:prefLabel xml:lang="en">system view</skos:prefLabel>
    </owl:Class>
    


    <!-- http://standards.iso.org/iso/10303/tech/refdata/core#b8746602-4164-4a98-8c82-340343f8170f -->

    <owl:Class rdf:about="http://standards.iso.org/iso/10303/tech/refdata/core#b8746602-4164-4a98-8c82-340343f8170f">
        <rdfs:subClassOf rdf:resource="http://standards.iso.org/iso/10303/tech/refdata/core#1cfca290-3279-0135-b58f-598f1b1392ae"/>
        <dc:contributor>STEP Harmonization Team</dc:contributor>
        <dc:creator>Jean Brangé, AFNeT Services</dc:creator>
        <dc:date>2023-10-04</dc:date>
        <dc:source>ISO/TS 10303-4000</dc:source>
        <dc:type>InWork</dc:type>
        <rdfs:comment xml:lang="en">A FrozenAssignment is a collection of objects that shall not be changed in any way.</rdfs:comment>
        <owl:versionInfo>3</owl:versionInfo>
        <skos:changeNote>[2023-10-04] Jean Brangé, AFNeT Services: Initial definition.</skos:changeNote>
        <skos:prefLabel xml:lang="en">frozen assignment</skos:prefLabel>
    </owl:Class>
    


    <!-- http://standards.iso.org/iso/10303/tech/refdata/core#b8f60a60-130a-0135-b552-598f1b1392ae -->

    <owl:Class rdf:about="http://standards.iso.org/iso/10303/tech/refdata/core#b8f60a60-130a-0135-b552-598f1b1392ae">
        <rdfs:subClassOf rdf:resource="http://standards.iso.org/iso/10303/tech/refdata/core#STEPThing"/>
        <dc:contributor>STEP Harmonization Team</dc:contributor>
        <dc:creator>Phil Spiby, Eurostep</dc:creator>
        <dc:date>2022-09-01</dc:date>
        <dc:source>ISO/TS 10303-4000</dc:source>
        <dc:type>InWork</dc:type>
        <rdfs:comment xml:lang="en">A PrecisionQualifier is a specification of the number of significant digits in the representation of a value.</rdfs:comment>
        <owl:versionInfo>1</owl:versionInfo>
        <skos:changeNote>[2021-07-30] Initial definition.</skos:changeNote>
        <skos:prefLabel xml:lang="en">precision qualifier</skos:prefLabel>
    </owl:Class>
    


    <!-- http://standards.iso.org/iso/10303/tech/refdata/core#b9130840-130a-0135-b552-598f1b1392ae -->

    <owl:Class rdf:about="http://standards.iso.org/iso/10303/tech/refdata/core#b9130840-130a-0135-b552-598f1b1392ae">
        <rdfs:subClassOf rdf:resource="http://standards.iso.org/iso/10303/tech/refdata/core#STEPThing"/>
        <dc:contributor>STEP Harmonization Team</dc:contributor>
        <dc:creator>Phil Spiby, Eurostep</dc:creator>
        <dc:date>2022-09-01</dc:date>
        <dc:source>ISO/TS 10303-4000</dc:source>
        <dc:type>InWork</dc:type>
        <rdfs:comment xml:lang="en">A TypeQualifier is the specification of a type of a datum.</rdfs:comment>
        <owl:versionInfo>1</owl:versionInfo>
        <skos:changeNote>[2021-07-30] Initial definition.</skos:changeNote>
        <skos:prefLabel xml:lang="en">type qualifier</skos:prefLabel>
    </owl:Class>
    


    <!-- http://standards.iso.org/iso/10303/tech/refdata/core#ba4a7e0b-c3bd-4ca5-b54a-478af53097a9 -->

    <owl:Class rdf:about="http://standards.iso.org/iso/10303/tech/refdata/core#ba4a7e0b-c3bd-4ca5-b54a-478af53097a9">
        <rdfs:subClassOf rdf:resource="http://standards.iso.org/iso/10303/tech/refdata/core#7c082e33-57b4-465b-aaad-04c8977d2353"/>
        <dc:contributor>STEP Harmonization Team</dc:contributor>
        <dc:creator>Phil Spiby, Eurostep</dc:creator>
        <dc:date>2022-09-01</dc:date>
        <dc:source>ISO/TS 10303-4000</dc:source>
        <dc:type>InWork</dc:type>
        <rdfs:comment xml:lang="en">A SimultaneousElements is a specialization of ConcurrentElements that represents two or more actions to be performed together.</rdfs:comment>
        <owl:versionInfo>1</owl:versionInfo>
        <skos:changeNote>[2021-07-30] Initial definition.</skos:changeNote>
        <skos:prefLabel xml:lang="en">simultaneous elements</skos:prefLabel>
    </owl:Class>
    


    <!-- http://standards.iso.org/iso/10303/tech/refdata/core#ba5f1f7a-ded3-4e1b-b44a-409d1bd51e28 -->

    <owl:Class rdf:about="http://standards.iso.org/iso/10303/tech/refdata/core#ba5f1f7a-ded3-4e1b-b44a-409d1bd51e28">
        <rdfs:subClassOf rdf:resource="http://standards.iso.org/iso/10303/tech/refdata/core#0cc8b831-37f7-4cd5-984f-dbb5588fbc1d"/>
        <dc:contributor>STEP Harmonization Team</dc:contributor>
        <dc:creator>Jean Brangé, AFNeT Services</dc:creator>
        <dc:date>2023-10-04</dc:date>
        <dc:source>ISO/TS 10303-4000</dc:source>
        <dc:type>InWork</dc:type>
        <rdfs:comment xml:lang="en">A HarnessNode is a type of PartShapeElement that represents a Vertex from a ConnectedEdgeWithLengthSetRepresentation for a WiringHarnessAssemblyDesign.</rdfs:comment>
        <owl:versionInfo>3</owl:versionInfo>
        <skos:changeNote>[2023-10-04] Jean Brangé, AFNeT Services: Initial definition.</skos:changeNote>
        <skos:prefLabel xml:lang="en">harness node</skos:prefLabel>
    </owl:Class>
    


    <!-- http://standards.iso.org/iso/10303/tech/refdata/core#bad0ff99-711e-4a97-ba64-261162d6e8e3 -->

    <owl:Class rdf:about="http://standards.iso.org/iso/10303/tech/refdata/core#bad0ff99-711e-4a97-ba64-261162d6e8e3">
        <rdfs:subClassOf rdf:resource="http://standards.iso.org/iso/10303/tech/refdata/core#1cfca290-3279-0135-b58f-598f1b1392ae"/>
        <dc:contributor>STEP Harmonization Team</dc:contributor>
        <dc:creator>Phil Spiby, Eurostep</dc:creator>
        <dc:date>2022-09-01</dc:date>
        <dc:source>ISO/TS 10303-4000</dc:source>
        <dc:type>InWork</dc:type>
        <rdfs:comment xml:lang="en">A TypeOfPersonAssignment is the assignment of a TypeOfPerson in a role to an item (specified by TypeOfPersonAssignmentSelect). The meaning of the assignment can be specified using the ClassifiedAs attribute inherited from the AssignmentObject.</rdfs:comment>
        <owl:versionInfo>1</owl:versionInfo>
        <skos:changeNote>[2022-09-01] Initial definition.</skos:changeNote>
        <skos:prefLabel xml:lang="en">type of person assignment</skos:prefLabel>
    </owl:Class>
    


    <!-- http://standards.iso.org/iso/10303/tech/refdata/core#bbe404df-38a1-41f5-877e-616a4ccb873c -->

    <owl:Class rdf:about="http://standards.iso.org/iso/10303/tech/refdata/core#bbe404df-38a1-41f5-877e-616a4ccb873c">
        <rdfs:subClassOf rdf:resource="http://standards.iso.org/iso/10303/tech/refdata/core#6d4d4ccd-20d2-4209-9fe6-17da7b3cb1a1"/>
        <dc:contributor>STEP Harmonization Team</dc:contributor>
        <dc:creator>Jean Brangé, AFNeT Services</dc:creator>
        <dc:date>2023-10-04</dc:date>
        <dc:source>ISO/TS 10303-4000</dc:source>
        <dc:type>InWork</dc:type>
        <rdfs:comment xml:lang="en">A PlyLaminateTable is a type of LaminateTable that provides an ordered list of Ply objects. The ordered list provides basic placement position within the laminate (see following figure). PlyLaminateTable.pngPly laminate table</rdfs:comment>
        <owl:versionInfo>3</owl:versionInfo>
        <skos:changeNote>[2023-10-04] Jean Brangé, AFNeT Services: Initial definition.</skos:changeNote>
        <skos:note xml:lang="en">The PlyLaminateTable is only valid to describe a LaminateTable.</skos:note>
        <skos:note xml:lang="en">The valid components of a PlyLaminateTable are plies only.</skos:note>
        <skos:prefLabel xml:lang="en">ply laminate table</skos:prefLabel>
    </owl:Class>
    


    <!-- http://standards.iso.org/iso/10303/tech/refdata/core#bc514af6-504d-408c-aa54-be5472451718 -->

    <owl:Class rdf:about="http://standards.iso.org/iso/10303/tech/refdata/core#bc514af6-504d-408c-aa54-be5472451718">
        <rdfs:subClassOf rdf:resource="http://standards.iso.org/iso/10303/tech/refdata/core#8b5ba2e8-9590-4ef0-be41-93e469bea12d"/>
        <dc:contributor>STEP Harmonization Team</dc:contributor>
        <dc:creator>Jean Brangé, AFNeT Services</dc:creator>
        <dc:date>2023-10-04</dc:date>
        <dc:source>ISO/TS 10303-4000</dc:source>
        <dc:type>InWork</dc:type>
        <rdfs:comment xml:lang="en">A ToleranceZoneWithDatum is a type of DirectedOrOrientedToleranceZone that includes direction or orientation classification with respect to referenced features.</rdfs:comment>
        <owl:versionInfo>3</owl:versionInfo>
        <skos:changeNote>[2023-10-04] Jean Brangé, AFNeT Services: Initial definition.</skos:changeNote>
        <skos:note xml:lang="en">Typically only a primary datum is used.</skos:note>
        <skos:prefLabel xml:lang="en">tolerance zone with datum</skos:prefLabel>
    </owl:Class>
    


    <!-- http://standards.iso.org/iso/10303/tech/refdata/core#bc81f040-130a-0135-b552-598f1b1392ae -->

    <owl:Class rdf:about="http://standards.iso.org/iso/10303/tech/refdata/core#bc81f040-130a-0135-b552-598f1b1392ae">
        <rdfs:subClassOf rdf:resource="http://standards.iso.org/iso/10303/tech/refdata/core#bd177980-130a-0135-b552-598f1b1392ae"/>
        <dc:contributor>STEP Harmonization Team</dc:contributor>
        <dc:creator>Phil Spiby, Eurostep</dc:creator>
        <dc:date>2022-09-01</dc:date>
        <dc:source>ISO/TS 10303-4000</dc:source>
        <dc:type>InWork</dc:type>
        <rdfs:comment xml:lang="en">A ProductClass is a type of ProductConcept that represents a set of similar products to be offered to the market. ProductClass objects that are related to each other by a ProductClassRelationship do not inherit any characteristics from each other. example_product_class_hierarchy.gif Example structure from the automotive domain of ProductClass objects in a hierarchy</rdfs:comment>
        <owl:versionInfo>2</owl:versionInfo>
        <skos:changeNote>[2021-07-30] Initial definition.</skos:changeNote>
        <skos:changeNote>[2022-09-01] Phil Spiby, Eurostep: updated note.</skos:changeNote>
        <skos:example xml:lang="en">In an organization which manufactures cars and engines for cars, the car models will be represented by ProductClass objects.</skos:example>
        <skos:example xml:lang="en">The following figure depicts a detail of an example of a structure that is built up by ProductClass and ProductClassRelationship objects.</skos:example>
        <skos:note xml:lang="en">A ProductClass can be characterized by a set of features or specifications identified by the customers or derived from customers&apos; needs.</skos:note>
        <skos:note xml:lang="en">A ProductClass enables to represent customer-oriented identification of products that are to be delivered to customers, while a Part enables to identify and to track the history of items that are designed and manufactured, as a tangible solution, or component of the solution, for a ProductClass.</skos:note>
        <skos:note xml:lang="en">Depending on the kind of industry and products, a ProductClass might be offered to the customers in one single or in many different configurations.</skos:note>
        <skos:note xml:lang="en">The definition of product classes is driven by market and customer requirements and forecasting. A ProductClass often corresponds to the highest-level item(s) manufactured by an organization for customers.</skos:note>
        <skos:prefLabel xml:lang="en">product class</skos:prefLabel>
    </owl:Class>
    


    <!-- http://standards.iso.org/iso/10303/tech/refdata/core#bcccb4e0-130a-0135-b552-598f1b1392ae -->

    <owl:Class rdf:about="http://standards.iso.org/iso/10303/tech/refdata/core#bcccb4e0-130a-0135-b552-598f1b1392ae">
        <rdfs:subClassOf rdf:resource="http://standards.iso.org/iso/10303/tech/refdata/core#59b11220-3279-0135-b58f-598f1b1392ae"/>
        <dc:contributor>STEP Harmonization Team</dc:contributor>
        <dc:creator>Phil Spiby, Eurostep</dc:creator>
        <dc:date>2022-09-01</dc:date>
        <dc:source>ISO/TS 10303-4000</dc:source>
        <dc:type>InWork</dc:type>
        <rdfs:comment xml:lang="en">A ProductClassRelationship is a relationship between two ProductClass objects.</rdfs:comment>
        <owl:versionInfo>2</owl:versionInfo>
        <skos:changeNote>[2021-07-30] Initial definition.</skos:changeNote>
        <skos:changeNote>[2022-09-01] Phil Spiby, Eurostep: updated comment.</skos:changeNote>
        <skos:prefLabel xml:lang="en">product class relationship</skos:prefLabel>
    </owl:Class>
    


    <!-- http://standards.iso.org/iso/10303/tech/refdata/core#bd177980-130a-0135-b552-598f1b1392ae -->

    <owl:Class rdf:about="http://standards.iso.org/iso/10303/tech/refdata/core#bd177980-130a-0135-b552-598f1b1392ae">
        <rdfs:subClassOf rdf:resource="http://standards.iso.org/iso/10303/tech/refdata/core#STEPThing"/>
        <dc:contributor>STEP Harmonization Team</dc:contributor>
        <dc:creator>Phil Spiby, Eurostep</dc:creator>
        <dc:date>2022-09-01</dc:date>
        <dc:source>ISO/TS 10303-4000</dc:source>
        <dc:type>InWork</dc:type>
        <rdfs:comment xml:lang="en">A ProductConcept is a representation of a set of similar products that were, are or will be proposed to customers.</rdfs:comment>
        <owl:versionInfo>1</owl:versionInfo>
        <skos:changeNote>[2021-07-30] Initial definition.</skos:changeNote>
        <skos:prefLabel xml:lang="en">product concept</skos:prefLabel>
    </owl:Class>
    


    <!-- http://standards.iso.org/iso/10303/tech/refdata/core#bd56a13d-7fc8-4c6a-89ed-77099b7cf230 -->

    <owl:Class rdf:about="http://standards.iso.org/iso/10303/tech/refdata/core#bd56a13d-7fc8-4c6a-89ed-77099b7cf230">
        <rdfs:subClassOf rdf:resource="http://standards.iso.org/iso/10303/tech/refdata/core#55105ef0-713f-409a-8306-fd8708d4ee3f"/>
        <dc:contributor>STEP Harmonization Team</dc:contributor>
        <dc:creator>Jean Brangé, AFNeT Services</dc:creator>
        <dc:date>2023-10-04</dc:date>
        <dc:source>ISO/TS 10303-4000</dc:source>
        <dc:type>InWork</dc:type>
        <rdfs:comment xml:lang="en">A CylindricityTolerance is a type of GeometricTolerance. It constrains the form of a cylindrical feature. Unless otherwise specified, the rules governing cylindricity tolerance defined in ISO 1101 shall apply.</rdfs:comment>
        <owl:versionInfo>3</owl:versionInfo>
        <skos:changeNote>[2023-10-04] Jean Brangé, AFNeT Services: Initial definition.</skos:changeNote>
        <skos:note xml:lang="en">Alternatively cylindricity tolerance can be used according to the specifications given in ASME Y14.5</skos:note>
        <skos:prefLabel xml:lang="en">cylindricity tolerance</skos:prefLabel>
    </owl:Class>
    


    <!-- http://standards.iso.org/iso/10303/tech/refdata/core#bd66597f-8a9d-4f1f-bc6f-12e46aeb0931 -->

    <owl:Class rdf:about="http://standards.iso.org/iso/10303/tech/refdata/core#bd66597f-8a9d-4f1f-bc6f-12e46aeb0931">
        <rdfs:subClassOf rdf:resource="http://standards.iso.org/iso/10303/tech/refdata/core#f8816baf-d66a-42f9-bdcc-38e946c9a2fa"/>
        <dc:contributor>STEP Harmonization Team</dc:contributor>
        <dc:creator>Jean Brangé, AFNeT Services</dc:creator>
        <dc:date>2023-10-04</dc:date>
        <dc:source>ISO/TS 10303-4000</dc:source>
        <dc:type>InWork</dc:type>
        <rdfs:comment xml:lang="en">A GeometricContact is a type of DerivedShapeElement that represents the common contact region between two ShapeElements. The involved ShapeElements shall not intersect with each other.</rdfs:comment>
        <owl:versionInfo>3</owl:versionInfo>
        <skos:changeNote>[2023-10-04] Jean Brangé, AFNeT Services: Initial definition.</skos:changeNote>
        <skos:prefLabel xml:lang="en">geometric contact</skos:prefLabel>
    </owl:Class>
    


    <!-- http://standards.iso.org/iso/10303/tech/refdata/core#bd748da0-130a-0135-b552-598f1b1392ae -->

    <owl:Class rdf:about="http://standards.iso.org/iso/10303/tech/refdata/core#bd748da0-130a-0135-b552-598f1b1392ae">
        <rdfs:subClassOf rdf:resource="http://standards.iso.org/iso/10303/tech/refdata/core#STEPThing"/>
        <dc:contributor>STEP Harmonization Team</dc:contributor>
        <dc:creator>Phil Spiby, Eurostep</dc:creator>
        <dc:date>2022-09-01</dc:date>
        <dc:source>ISO/TS 10303-4000</dc:source>
        <dc:type>InWork</dc:type>
        <rdfs:comment xml:lang="en">A ProductConfiguration is a manufacturable object or expected as so. A ProductConfiguration is defined with respect to the ProductClass from which it is a member. For a ProductConfiguration one or more additional Specification objects can be specified. In this case they enhance the characterization provided for the associated ProductClass.</rdfs:comment>
        <owl:versionInfo>2</owl:versionInfo>
        <skos:changeNote>[2021-07-30] Initial definition.</skos:changeNote>
        <skos:changeNote>[2022-09-01] Phil Spiby, Eurostep: updated comment updated example updated note.</skos:changeNote>
        <skos:example xml:lang="en">A ProductConfiguration can represent a component of a contracted product, onto which severe safety rules apply and for which configuration management is therefore rigorously applied.</skos:example>
        <skos:example xml:lang="en">A ProductConfiguration that is associated with a ProductClass that identifies a family of diesel engines is intended to lead to the manufacture of a specific case of diesel engine, and the ProductConfiguration that is associated with a ProductClass that identifies a car family will lead to the manufacture of a car.</skos:example>
        <skos:example xml:lang="en">If the colour is not specified for a given car family, the vehicle resulting from the realization of a ProductConfiguration associated to the ProductClass representing the car family can be without paint or painted in any available colour.</skos:example>
        <skos:note xml:lang="en">A ProductConfiguration can be established prior to the existence of a corresponding product.</skos:note>
        <skos:note xml:lang="en">A ProductConfiguration can identify a variation of a ProductClass, an entire ProductClass, or some portion thereof.</skos:note>
        <skos:note xml:lang="en">The actual set of Specification objects for a ProductConfiguration are obtained by the union of DefiningSpecifications and of the Specification objects related to the ./4_info_reqs_ProductSpecificationAndConfiguration.htm#SpecificationAssignment.AssignedTo AssignedTo through a SpecificationAssignment or a SpecificationConditionAssignment with AssociationType &apos;identification&apos; or &apos;non-replaceable standard&apos;.</skos:note>
        <skos:note xml:lang="en">The entity ProductConfiguration corresponds to the concept of configuration item defined, in some configuration management standards, as an item subject to configuration management.</skos:note>
        <skos:note xml:lang="en">The intent of ProductConfiguration is the identification of one manufacturable object whereas the intent of ProductClass is the gathering of products with similar characteristics.</skos:note>
        <skos:note xml:lang="en">The kind of product that is to be manufactured from the data of the ProductConfiguration, is defined by the ProductConcept to which the ProductConfiguration belongs.</skos:note>
        <skos:note xml:lang="en">The specification of a ProductConfiguration can be incomplete: there cannot be in DefiningSpecifications any instance of Specification for some SpecificationCategory declared as mandatory for the ./4_info_reqs_ProductSpecificationAndConfiguration.htm#SpecificationAssignment.AssignedTo AssignedTo. For these SpecificationCategory objects any Specification available in the context of the ./4_info_reqs_ProductSpecificationAndConfiguration.htm#SpecificationAssignment.AssignedTo AssignedTo is considered as valid for the manufacturing of the product characterized by the considered SpecificationAssignment.</skos:note>
        <skos:prefLabel xml:lang="en">product configuration</skos:prefLabel>
    </owl:Class>
    


    <!-- http://standards.iso.org/iso/10303/tech/refdata/core#be3b3900-130a-0135-b552-598f1b1392ae -->

    <owl:Class rdf:about="http://standards.iso.org/iso/10303/tech/refdata/core#be3b3900-130a-0135-b552-598f1b1392ae">
        <rdfs:subClassOf rdf:resource="http://standards.iso.org/iso/10303/tech/refdata/core#59b11220-3279-0135-b58f-598f1b1392ae"/>
        <dc:contributor>STEP Harmonization Team</dc:contributor>
        <dc:creator>Phil Spiby, Eurostep</dc:creator>
        <dc:date>2022-09-01</dc:date>
        <dc:source>ISO/TS 10303-4000</dc:source>
        <dc:type>InWork</dc:type>
        <rdfs:comment xml:lang="en">A ProductConfigurationRelationship is a relationship between two ProductConfiguration objects.</rdfs:comment>
        <owl:versionInfo>2</owl:versionInfo>
        <skos:changeNote>[2021-07-30] Initial definition.</skos:changeNote>
        <skos:changeNote>[2022-09-01] Phil Spiby, Eurostep: updated comment.</skos:changeNote>
        <skos:prefLabel xml:lang="en">product configuration relationship</skos:prefLabel>
    </owl:Class>
    


    <!-- http://standards.iso.org/iso/10303/tech/refdata/core#be51da23-f07f-49d2-91e7-ce97d34d9fb6 -->

    <owl:Class rdf:about="http://standards.iso.org/iso/10303/tech/refdata/core#be51da23-f07f-49d2-91e7-ce97d34d9fb6">
        <rdfs:subClassOf rdf:resource="http://standards.iso.org/iso/10303/tech/refdata/core#STEPThing"/>
        <dc:contributor>STEP Harmonization Team</dc:contributor>
        <dc:creator>Phil Spiby, Eurostep</dc:creator>
        <dc:date>2022-09-01</dc:date>
        <dc:source>ISO/TS 10303-4000</dc:source>
        <dc:type>InWork</dc:type>
        <rdfs:comment xml:lang="en">A Justification is the identification and description of the reasons for something. Justification entities can be associated with the data to which they apply.</rdfs:comment>
        <owl:versionInfo>2</owl:versionInfo>
        <skos:changeNote>[2021-07-30] Initial definition.</skos:changeNote>
        <skos:changeNote>[2022-09-01] Phil Spiby, Eurostep: updated comment updated example.</skos:changeNote>
        <skos:example xml:lang="en">A justification can be provided for a product design. Similarly, a justification can be provided for why an activity is needed or was undertaken.</skos:example>
        <skos:prefLabel xml:lang="en">justification</skos:prefLabel>
    </owl:Class>
    


    <!-- http://standards.iso.org/iso/10303/tech/refdata/core#be8d9ec0-130a-0135-b552-598f1b1392ae -->

    <owl:Class rdf:about="http://standards.iso.org/iso/10303/tech/refdata/core#be8d9ec0-130a-0135-b552-598f1b1392ae">
        <rdfs:subClassOf rdf:resource="http://standards.iso.org/iso/10303/tech/refdata/core#1d59c650-3279-0135-b58f-598f1b1392ae"/>
        <dc:contributor>STEP Harmonization Team</dc:contributor>
        <dc:creator>Phil Spiby, Eurostep</dc:creator>
        <dc:date>2022-09-01</dc:date>
        <dc:source>ISO/TS 10303-4000</dc:source>
        <dc:type>InWork</dc:type>
        <rdfs:comment xml:lang="en">A ProductDesignAssociation is a mechanism to associate a PartVersion with its corresponding ProductConfiguration. It specifies the explicit design that corresponds to the ProductConfiguration. The ProductDesignAssociation represents the statement that, in all definition contexts, the PartVersion is a valid way to implement the ProductConfiguration.</rdfs:comment>
        <owl:versionInfo>1</owl:versionInfo>
        <skos:changeNote>[2021-07-30] Initial definition.</skos:changeNote>
        <skos:note xml:lang="en">The ProductDesignAssociation might not be valid for other PartVersion objects.</skos:note>
        <skos:prefLabel xml:lang="en">product design association</skos:prefLabel>
    </owl:Class>
    


    <!-- http://standards.iso.org/iso/10303/tech/refdata/core#be9b4170-6aa7-44f1-87b9-8d618d4f8fb9 -->

    <owl:Class rdf:about="http://standards.iso.org/iso/10303/tech/refdata/core#be9b4170-6aa7-44f1-87b9-8d618d4f8fb9">
        <rdfs:subClassOf rdf:resource="http://standards.iso.org/iso/10303/tech/refdata/core#8b8e0c30-130a-0135-b552-598f1b1392ae"/>
        <dc:contributor>STEP Harmonization Team</dc:contributor>
        <dc:creator>Phil Spiby, Eurostep</dc:creator>
        <dc:date>2022-09-01</dc:date>
        <dc:source>ISO/TS 10303-4000</dc:source>
        <dc:type>InWork</dc:type>
        <rdfs:comment xml:lang="en">A BreakdownElementHierarchy defines a relationship between a Relating parent BreakdownElement and a Related child BreakdownElement.</rdfs:comment>
        <owl:versionInfo>2</owl:versionInfo>
        <skos:changeNote>[2021-07-30] Initial definition.</skos:changeNote>
        <skos:changeNote>[2022-09-01] Phil Spiby, Eurostep: updated comment.</skos:changeNote>
        <skos:prefLabel xml:lang="en">breakdown element hierarchy</skos:prefLabel>
    </owl:Class>
    


    <!-- http://standards.iso.org/iso/10303/tech/refdata/core#bec18000-130a-0135-b552-598f1b1392ae -->

    <owl:Class rdf:about="http://standards.iso.org/iso/10303/tech/refdata/core#bec18000-130a-0135-b552-598f1b1392ae">
        <rdfs:subClassOf rdf:resource="http://standards.iso.org/iso/10303/tech/refdata/core#a3c3b5c0-130a-0135-b552-598f1b1392ae"/>
        <dc:contributor>STEP Harmonization Team</dc:contributor>
        <dc:creator>Phil Spiby, Eurostep</dc:creator>
        <dc:date>2022-09-01</dc:date>
        <dc:source>ISO/TS 10303-4000</dc:source>
        <dc:type>InWork</dc:type>
        <rdfs:comment xml:lang="en">A ProductPlannedToRealized is a type of IndividualPartVersionRelationship that establishes that an actual artefact, represented by RealizedIndividualPart, has been realized as a version of a planned artefact, represented by PlannedIndividualPart.</rdfs:comment>
        <owl:versionInfo>2</owl:versionInfo>
        <skos:changeNote>[2021-07-30] Initial definition.</skos:changeNote>
        <skos:changeNote>[2022-09-01] Phil Spiby, Eurostep: updated comment.</skos:changeNote>
        <skos:prefLabel xml:lang="en">product planned to realized</skos:prefLabel>
    </owl:Class>
    


    <!-- http://standards.iso.org/iso/10303/tech/refdata/core#bf3a0b60-130a-0135-b552-598f1b1392ae -->

    <owl:Class rdf:about="http://standards.iso.org/iso/10303/tech/refdata/core#bf3a0b60-130a-0135-b552-598f1b1392ae">
        <rdfs:subClassOf rdf:resource="http://standards.iso.org/iso/10303/tech/refdata/core#STEPThing"/>
        <dc:contributor>STEP Harmonization Team</dc:contributor>
        <dc:creator>Phil Spiby, Eurostep</dc:creator>
        <dc:date>2022-09-01</dc:date>
        <dc:source>ISO/TS 10303-4000</dc:source>
        <dc:type>InWork</dc:type>
        <rdfs:comment xml:lang="en">A Project is an identified programme of work. It is a set of activities to create a product or service in accordance with specified resources and requirements.</rdfs:comment>
        <owl:versionInfo>2</owl:versionInfo>
        <skos:changeNote>[2021-07-30] Initial definition.</skos:changeNote>
        <skos:changeNote>[2022-09-01] Phil Spiby, Eurostep: updated note.</skos:changeNote>
        <skos:example xml:lang="en">For the development of a new car, a project is set up that is responsible for the development decisions, as well as for the accounting of the costs.</skos:example>
        <skos:note xml:lang="en">A Project can be further characterized with planned or actual dates, allowed budget, activities or resources by attribute values of this business object or by assignments to other business objects.</skos:note>
        <skos:prefLabel xml:lang="en">project</skos:prefLabel>
    </owl:Class>
    


    <!-- http://standards.iso.org/iso/10303/tech/refdata/core#bfcafbb6-c6ed-49fa-8dec-b307eb7619e5 -->

    <owl:Class rdf:about="http://standards.iso.org/iso/10303/tech/refdata/core#bfcafbb6-c6ed-49fa-8dec-b307eb7619e5">
        <rdfs:subClassOf rdf:resource="http://standards.iso.org/iso/10303/tech/refdata/core#STEPThing"/>
        <dc:contributor>STEP Harmonization Team</dc:contributor>
        <dc:creator>Phil Spiby, Eurostep</dc:creator>
        <dc:date>2022-09-01</dc:date>
        <dc:source>ISO/TS 10303-4000</dc:source>
        <dc:type>InWork</dc:type>
        <rdfs:comment xml:lang="en">A PersonName is a structured combination of name components that can represent Person names in accordance with different name pattern originating from different naming conventions and cultures. A PersonName consists of a non-empty set of PersonNameComponents.</rdfs:comment>
        <owl:versionInfo>1</owl:versionInfo>
        <skos:changeNote>[2021-07-30] Initial definition.</skos:changeNote>
        <skos:prefLabel xml:lang="en">person name</skos:prefLabel>
    </owl:Class>
    


    <!-- http://standards.iso.org/iso/10303/tech/refdata/core#bfec9280-130a-0135-b552-598f1b1392ae -->

    <owl:Class rdf:about="http://standards.iso.org/iso/10303/tech/refdata/core#bfec9280-130a-0135-b552-598f1b1392ae">
        <rdfs:subClassOf rdf:resource="http://standards.iso.org/iso/10303/tech/refdata/core#1cfca290-3279-0135-b58f-598f1b1392ae"/>
        <dc:contributor>STEP Harmonization Team</dc:contributor>
        <dc:creator>Phil Spiby, Eurostep</dc:creator>
        <dc:date>2022-09-01</dc:date>
        <dc:source>ISO/TS 10303-4000</dc:source>
        <dc:type>InWork</dc:type>
        <rdfs:comment xml:lang="en">A ProjectAssignment is an assignment of a Project to an item (specified by ProjectAssignmentSelect).</rdfs:comment>
        <owl:versionInfo>1</owl:versionInfo>
        <skos:changeNote>[2021-07-30] Initial definition.</skos:changeNote>
        <skos:prefLabel xml:lang="en">project assignment</skos:prefLabel>
    </owl:Class>
    


    <!-- http://standards.iso.org/iso/10303/tech/refdata/core#c0354eeb-a709-44fa-842f-16c012e80f48 -->

    <owl:Class rdf:about="http://standards.iso.org/iso/10303/tech/refdata/core#c0354eeb-a709-44fa-842f-16c012e80f48">
        <rdfs:subClassOf rdf:resource="http://standards.iso.org/iso/10303/tech/refdata/core#1d59c650-3279-0135-b58f-598f1b1392ae"/>
        <dc:contributor>STEP Harmonization Team</dc:contributor>
        <dc:creator>Phil Spiby, Eurostep</dc:creator>
        <dc:date>2022-09-01</dc:date>
        <dc:source>ISO/TS 10303-4000</dc:source>
        <dc:type>InWork</dc:type>
        <rdfs:comment xml:lang="en">An ObservedEnvironmentToDefinition is an association between a record of a set of observations about an environment, represented by an ObservedEnvironment, and a typical environment, represented by an EnvironmentDefinition. The typical environment is the expected environment about which observations have been made.</rdfs:comment>
        <owl:versionInfo>2</owl:versionInfo>
        <skos:changeNote>[2021-07-30] Initial definition.</skos:changeNote>
        <skos:changeNote>[2022-09-01] Phil Spiby, Eurostep: updated comment.</skos:changeNote>
        <skos:prefLabel xml:lang="en">observed environment to definition</skos:prefLabel>
    </owl:Class>
    


    <!-- http://standards.iso.org/iso/10303/tech/refdata/core#c050712f-0dca-495e-aa7d-2b2e21af712b -->

    <owl:Class rdf:about="http://standards.iso.org/iso/10303/tech/refdata/core#c050712f-0dca-495e-aa7d-2b2e21af712b">
        <rdfs:subClassOf rdf:resource="http://standards.iso.org/iso/10303/tech/refdata/core#STEPThing"/>
        <dc:contributor>STEP Harmonization Team</dc:contributor>
        <dc:creator>Jean Brangé, AFNeT Services</dc:creator>
        <dc:date>2023-10-04</dc:date>
        <dc:source>ISO/TS 10303-4000</dc:source>
        <dc:type>InWork</dc:type>
        <rdfs:comment xml:lang="en">A GeometricDimension is the specification of size of an element of a shape, or a displacement of one shape element relative to another shape element. A GeometricDimension is either a DimensionalLocation or a DimensionalSize.</rdfs:comment>
        <owl:versionInfo>3</owl:versionInfo>
        <skos:changeNote>[2023-10-04] Jean Brangé, AFNeT Services: Initial definition.</skos:changeNote>
        <skos:prefLabel xml:lang="en">geometric dimension</skos:prefLabel>
    </owl:Class>
    


    <!-- http://standards.iso.org/iso/10303/tech/refdata/core#c05ac994-a7cc-4f68-9f21-f87029262b02 -->

    <owl:Class rdf:about="http://standards.iso.org/iso/10303/tech/refdata/core#c05ac994-a7cc-4f68-9f21-f87029262b02">
        <rdfs:subClassOf rdf:resource="http://standards.iso.org/iso/10303/tech/refdata/core#59b11220-3279-0135-b58f-598f1b1392ae"/>
        <dc:contributor>STEP Harmonization Team</dc:contributor>
        <dc:creator>Jean Brangé, AFNeT Services</dc:creator>
        <dc:date>2023-10-04</dc:date>
        <dc:source>ISO/TS 10303-4000</dc:source>
        <dc:type>InWork</dc:type>
        <rdfs:comment xml:lang="en">A ProcessOperationDefinitionRelationship is an association between two ProcessOperationDefinition objects.</rdfs:comment>
        <owl:versionInfo>3</owl:versionInfo>
        <skos:changeNote>[2023-10-04] Jean Brangé, AFNeT Services: Initial definition.</skos:changeNote>
        <skos:prefLabel xml:lang="en">process operation definition relationship</skos:prefLabel>
    </owl:Class>
    


    <!-- http://standards.iso.org/iso/10303/tech/refdata/core#c05d7cc0-130a-0135-b552-598f1b1392ae -->

    <owl:Class rdf:about="http://standards.iso.org/iso/10303/tech/refdata/core#c05d7cc0-130a-0135-b552-598f1b1392ae">
        <rdfs:subClassOf rdf:resource="http://standards.iso.org/iso/10303/tech/refdata/core#59b11220-3279-0135-b58f-598f1b1392ae"/>
        <dc:contributor>STEP Harmonization Team</dc:contributor>
        <dc:creator>Phil Spiby, Eurostep</dc:creator>
        <dc:date>2022-09-01</dc:date>
        <dc:source>ISO/TS 10303-4000</dc:source>
        <dc:type>InWork</dc:type>
        <rdfs:comment xml:lang="en">A ProjectRelationship is a relationship between two Project objects.</rdfs:comment>
        <owl:versionInfo>2</owl:versionInfo>
        <skos:changeNote>[2021-07-30] Initial definition.</skos:changeNote>
        <skos:changeNote>[2022-09-01] Phil Spiby, Eurostep: updated comment.</skos:changeNote>
        <skos:prefLabel xml:lang="en">project relationship</skos:prefLabel>
    </owl:Class>
    


    <!-- http://standards.iso.org/iso/10303/tech/refdata/core#c0b90a40-130a-0135-b552-598f1b1392ae -->

    <owl:Class rdf:about="http://standards.iso.org/iso/10303/tech/refdata/core#c0b90a40-130a-0135-b552-598f1b1392ae">
        <rdfs:subClassOf rdf:resource="http://standards.iso.org/iso/10303/tech/refdata/core#87863f90-130a-0135-b552-598f1b1392ae"/>
        <dc:contributor>STEP Harmonization Team</dc:contributor>
        <dc:creator>Phil Spiby, Eurostep</dc:creator>
        <dc:date>2022-09-01</dc:date>
        <dc:source>ISO/TS 10303-4000</dc:source>
        <dc:type>InWork</dc:type>
        <rdfs:comment xml:lang="en">A PromissoryAssemblyOccurrenceUsage is a type of AssemblyOccurrenceRelationship. A PromissoryAssemblyOccurrenceUsage is a relationship between the occurrence of a constituent of an assembly and a view of the assembly itself. The relationship describes the intention to use the occurrence of a constituent of an assembly in an assembly. The constituent or the assembly that is associated by a PromissoryAssemblyOccurrenceUsage can have no geometric information.</rdfs:comment>
        <owl:versionInfo>2</owl:versionInfo>
        <skos:changeNote>[2021-07-30] Initial definition.</skos:changeNote>
        <skos:changeNote>[2022-09-01] Phil Spiby, Eurostep: updated comment updated example.</skos:changeNote>
        <skos:example xml:lang="en">In early design stages, the PromissoryAssemblyOccurrenceUsage can be used to create preliminary BOMs for prototyping.</skos:example>
        <skos:prefLabel xml:lang="en">promissory assembly occurrence usage</skos:prefLabel>
    </owl:Class>
    


    <!-- http://standards.iso.org/iso/10303/tech/refdata/core#c0bf24c0-130a-0135-b552-598f1b1392ae -->

    <owl:Class rdf:about="http://standards.iso.org/iso/10303/tech/refdata/core#c0bf24c0-130a-0135-b552-598f1b1392ae">
        <rdfs:subClassOf rdf:resource="http://standards.iso.org/iso/10303/tech/refdata/core#88035ed0-130a-0135-b552-598f1b1392ae"/>
        <dc:contributor>STEP Harmonization Team</dc:contributor>
        <dc:creator>Phil Spiby, Eurostep</dc:creator>
        <dc:date>2022-09-01</dc:date>
        <dc:source>ISO/TS 10303-4000</dc:source>
        <dc:type>InWork</dc:type>
        <rdfs:comment xml:lang="en">A PromissoryAssemblyViewUsage is a type of AssemblyViewRelationship. A PromissoryAssemblyViewUsage is a relationship between a Related view of an assembly constituent and a Relating view of the assembly itself. The relationship describes the intention to use the view of an assembly constituent in an assembly. The constituent or the assembly that is associated by a PromissoryAssemblyViewUsage can have no geometric information.</rdfs:comment>
        <owl:versionInfo>2</owl:versionInfo>
        <skos:changeNote>[2021-07-30] Initial definition.</skos:changeNote>
        <skos:changeNote>[2022-09-01] Phil Spiby, Eurostep: updated comment.</skos:changeNote>
        <skos:prefLabel xml:lang="en">promissory assembly view usage</skos:prefLabel>
    </owl:Class>
    


    <!-- http://standards.iso.org/iso/10303/tech/refdata/core#c0c6c5e0-130a-0135-b552-598f1b1392ae -->

    <owl:Class rdf:about="http://standards.iso.org/iso/10303/tech/refdata/core#c0c6c5e0-130a-0135-b552-598f1b1392ae">
        <rdfs:subClassOf rdf:resource="http://standards.iso.org/iso/10303/tech/refdata/core#STEPThing"/>
        <dc:contributor>STEP Harmonization Team</dc:contributor>
        <dc:creator>Phil Spiby, Eurostep</dc:creator>
        <dc:date>2022-09-01</dc:date>
        <dc:source>ISO/TS 10303-4000</dc:source>
        <dc:type>InWork</dc:type>
        <rdfs:comment xml:lang="en">A PropertyDefinition is the definition of a specific quality.</rdfs:comment>
        <owl:versionInfo>2</owl:versionInfo>
        <skos:changeNote>[2021-07-30] Initial definition.</skos:changeNote>
        <skos:changeNote>[2022-09-01] Phil Spiby, Eurostep: updated example.</skos:changeNote>
        <skos:example xml:lang="en">A PropertyDefinition can reflect physics or arbitrary user defined measurements.</skos:example>
        <skos:prefLabel xml:lang="en">property definition</skos:prefLabel>
    </owl:Class>
    


    <!-- http://standards.iso.org/iso/10303/tech/refdata/core#c0d8f11c-88c6-4f14-9592-511a58493e5f -->

    <owl:Class rdf:about="http://standards.iso.org/iso/10303/tech/refdata/core#c0d8f11c-88c6-4f14-9592-511a58493e5f">
        <rdfs:subClassOf rdf:resource="http://standards.iso.org/iso/10303/tech/refdata/core#STEPThing"/>
        <dc:contributor>STEP Harmonization Team</dc:contributor>
        <dc:creator>Phil Spiby, Eurostep</dc:creator>
        <dc:date>2022-09-01</dc:date>
        <dc:source>ISO/TS 10303-4000</dc:source>
        <dc:type>InWork</dc:type>
        <rdfs:comment xml:lang="en">A Collection identifies a set of data.</rdfs:comment>
        <owl:versionInfo>1</owl:versionInfo>
        <skos:changeNote>[2021-07-30] Initial definition.</skos:changeNote>
        <skos:prefLabel xml:lang="en">collection</skos:prefLabel>
    </owl:Class>
    


    <!-- http://standards.iso.org/iso/10303/tech/refdata/core#c1247222-6528-4897-a401-5a61bdfd511c -->

    <owl:Class rdf:about="http://standards.iso.org/iso/10303/tech/refdata/core#c1247222-6528-4897-a401-5a61bdfd511c">
        <rdfs:subClassOf rdf:resource="http://standards.iso.org/iso/10303/tech/refdata/core#ff04d2c5-cea4-41a6-be35-821c1495d8ba"/>
        <dc:contributor>STEP Harmonization Team</dc:contributor>
        <dc:creator>Phil Spiby, Eurostep</dc:creator>
        <dc:date>2022-09-01</dc:date>
        <dc:source>ISO/TS 10303-4000</dc:source>
        <dc:type>InWork</dc:type>
        <rdfs:comment xml:lang="en">A LoopingElement is a specialization of TaskElement. It invokes a specified number of repetitions of a further TaskElement.</rdfs:comment>
        <owl:versionInfo>1</owl:versionInfo>
        <skos:changeNote>[2021-07-30] Initial definition.</skos:changeNote>
        <skos:prefLabel xml:lang="en">looping element</skos:prefLabel>
    </owl:Class>
    


    <!-- http://standards.iso.org/iso/10303/tech/refdata/core#c126ace8-0b51-44f4-83a6-6aa3116f9ced -->

    <owl:Class rdf:about="http://standards.iso.org/iso/10303/tech/refdata/core#c126ace8-0b51-44f4-83a6-6aa3116f9ced">
        <rdfs:subClassOf rdf:resource="http://standards.iso.org/iso/10303/tech/refdata/core#59b11220-3279-0135-b58f-598f1b1392ae"/>
        <dc:contributor>STEP Harmonization Team</dc:contributor>
        <dc:creator>Phil Spiby, Eurostep</dc:creator>
        <dc:date>2022-09-01</dc:date>
        <dc:source>ISO/TS 10303-4000</dc:source>
        <dc:type>InWork</dc:type>
        <rdfs:comment xml:lang="en">An InterfaceSpecificationVersionRelationship is a relationship between two InterfaceSpecificationVersion objects.</rdfs:comment>
        <owl:versionInfo>2</owl:versionInfo>
        <skos:changeNote>[2021-07-30] Initial definition.</skos:changeNote>
        <skos:changeNote>[2022-09-01] Phil Spiby, Eurostep: updated comment.</skos:changeNote>
        <skos:prefLabel xml:lang="en">interface specification version relationship</skos:prefLabel>
    </owl:Class>
    


    <!-- http://standards.iso.org/iso/10303/tech/refdata/core#c12d01c0-130a-0135-b552-598f1b1392ae -->

    <owl:Class rdf:about="http://standards.iso.org/iso/10303/tech/refdata/core#c12d01c0-130a-0135-b552-598f1b1392ae">
        <rdfs:subClassOf rdf:resource="http://standards.iso.org/iso/10303/tech/refdata/core#1cfca290-3279-0135-b58f-598f1b1392ae"/>
        <dc:contributor>STEP Harmonization Team</dc:contributor>
        <dc:creator>Phil Spiby, Eurostep</dc:creator>
        <dc:date>2022-09-01</dc:date>
        <dc:source>ISO/TS 10303-4000</dc:source>
        <dc:type>InWork</dc:type>
        <rdfs:comment xml:lang="en">A PropertyDefinitionAssignment is an assignment of a PropertyDefinition to an item (specified by PropertyAssignmentSelect). The meaning of the assignment can be specified using the ClassifiedAs attribute inherited from the AssignmentObject.</rdfs:comment>
        <owl:versionInfo>2</owl:versionInfo>
        <skos:changeNote>[2021-07-30] Initial definition.</skos:changeNote>
        <skos:changeNote>[2022-09-01] Phil Spiby, Eurostep: updated comment updated example.</skos:changeNote>
        <skos:example xml:lang="en">A property &apos;mass&apos; defined in &apos;kg&apos; can be assigned to a Part.</skos:example>
        <skos:prefLabel xml:lang="en">property definition assignment</skos:prefLabel>
    </owl:Class>
    


    <!-- http://standards.iso.org/iso/10303/tech/refdata/core#c169dcd4-00dc-4db4-938c-f1c6d4608ef1 -->

    <owl:Class rdf:about="http://standards.iso.org/iso/10303/tech/refdata/core#c169dcd4-00dc-4db4-938c-f1c6d4608ef1">
        <rdfs:subClassOf rdf:resource="http://standards.iso.org/iso/10303/tech/refdata/core#835280f0-130a-0135-b552-598f1b1392ae"/>
        <dc:contributor>STEP Harmonization Team</dc:contributor>
        <dc:creator>Phil Spiby, Eurostep</dc:creator>
        <dc:date>2022-09-01</dc:date>
        <dc:source>ISO/TS 10303-4000</dc:source>
        <dc:type>InWork</dc:type>
        <rdfs:comment xml:lang="en">A SchemeVersion is a specialization of ActivityMethod. It allows for the version control of Scheme objects.</rdfs:comment>
        <owl:versionInfo>1</owl:versionInfo>
        <skos:changeNote>[2022-09-01] Initial definition.</skos:changeNote>
        <skos:prefLabel xml:lang="en">scheme version</skos:prefLabel>
    </owl:Class>
    


    <!-- http://standards.iso.org/iso/10303/tech/refdata/core#c1b96340-130a-0135-b552-598f1b1392ae -->

    <owl:Class rdf:about="http://standards.iso.org/iso/10303/tech/refdata/core#c1b96340-130a-0135-b552-598f1b1392ae">
        <rdfs:subClassOf rdf:resource="http://standards.iso.org/iso/10303/tech/refdata/core#59b11220-3279-0135-b58f-598f1b1392ae"/>
        <dc:contributor>STEP Harmonization Team</dc:contributor>
        <dc:creator>Phil Spiby, Eurostep</dc:creator>
        <dc:date>2022-09-01</dc:date>
        <dc:source>ISO/TS 10303-4000</dc:source>
        <dc:type>InWork</dc:type>
        <rdfs:comment xml:lang="en">A PropertyDefinitionAssignmentRelationship is a relationship between two PropertyDefinitionAssignment objects.</rdfs:comment>
        <owl:versionInfo>1</owl:versionInfo>
        <skos:changeNote>[2021-07-30] Initial definition.</skos:changeNote>
        <skos:prefLabel xml:lang="en">property definition assignment relationship</skos:prefLabel>
    </owl:Class>
    


    <!-- http://standards.iso.org/iso/10303/tech/refdata/core#c208bbc0-130a-0135-b552-598f1b1392ae -->

    <owl:Class rdf:about="http://standards.iso.org/iso/10303/tech/refdata/core#c208bbc0-130a-0135-b552-598f1b1392ae">
        <rdfs:subClassOf rdf:resource="http://standards.iso.org/iso/10303/tech/refdata/core#59b11220-3279-0135-b58f-598f1b1392ae"/>
        <dc:contributor>STEP Harmonization Team</dc:contributor>
        <dc:creator>Phil Spiby, Eurostep</dc:creator>
        <dc:date>2022-09-01</dc:date>
        <dc:source>ISO/TS 10303-4000</dc:source>
        <dc:type>InWork</dc:type>
        <rdfs:comment xml:lang="en">A PropertyDefinitionRelationship is a relationship between two PropertyDefinition objects.</rdfs:comment>
        <owl:versionInfo>2</owl:versionInfo>
        <skos:changeNote>[2021-07-30] Initial definition.</skos:changeNote>
        <skos:changeNote>[2022-09-01] Phil Spiby, Eurostep: updated example.</skos:changeNote>
        <skos:example xml:lang="en">A PropertyDefinitionRelationship can be used to indicate that the value of one PropertyDefinition can be derived from the value of another PropertyDefinition.</skos:example>
        <skos:prefLabel xml:lang="en">property definition relationship</skos:prefLabel>
    </owl:Class>
    


    <!-- http://standards.iso.org/iso/10303/tech/refdata/core#c2163417-6187-42ca-ac6b-3ff7f551d1a5 -->

    <owl:Class rdf:about="http://standards.iso.org/iso/10303/tech/refdata/core#c2163417-6187-42ca-ac6b-3ff7f551d1a5">
        <rdfs:subClassOf rdf:resource="http://standards.iso.org/iso/10303/tech/refdata/core#b3a9b996-c18c-4464-b398-d16e36d6711a"/>
        <dc:contributor>STEP Harmonization Team</dc:contributor>
        <dc:creator>Jean Brangé, AFNeT Services</dc:creator>
        <dc:date>2023-10-04</dc:date>
        <dc:source>ISO/TS 10303-4000</dc:source>
        <dc:type>InWork</dc:type>
        <rdfs:comment xml:lang="en">A ThreeDGeometrySet is a type of ConstituentShapeRepresentation that defines 3D boundary curve and surface geometry without topology. The surfaces used in the representation have a defined model surface context.</rdfs:comment>
        <owl:versionInfo>3</owl:versionInfo>
        <skos:changeNote>[2023-10-04] Jean Brangé, AFNeT Services: Initial definition.</skos:changeNote>
        <skos:prefLabel xml:lang="en">three dgeometry set</skos:prefLabel>
    </owl:Class>
    


    <!-- http://standards.iso.org/iso/10303/tech/refdata/core#c2556d12-6d7c-4af8-8251-7ccb3889a773 -->

    <owl:Class rdf:about="http://standards.iso.org/iso/10303/tech/refdata/core#c2556d12-6d7c-4af8-8251-7ccb3889a773">
        <rdfs:subClassOf rdf:resource="http://standards.iso.org/iso/10303/tech/refdata/core#c1247222-6528-4897-a401-5a61bdfd511c"/>
        <dc:contributor>STEP Harmonization Team</dc:contributor>
        <dc:creator>Phil Spiby, Eurostep</dc:creator>
        <dc:date>2022-09-01</dc:date>
        <dc:source>ISO/TS 10303-4000</dc:source>
        <dc:type>InWork</dc:type>
        <rdfs:comment xml:lang="en">A RepeatCount is a type of LoopingElement. It invokes a specified number of repetitions of the RepeatedElement inherited from LoopingElement.</rdfs:comment>
        <owl:versionInfo>2</owl:versionInfo>
        <skos:changeNote>[2021-07-30] Initial definition.</skos:changeNote>
        <skos:changeNote>[2022-09-01] Phil Spiby, Eurostep: updated comment.</skos:changeNote>
        <skos:prefLabel xml:lang="en">repeat count</skos:prefLabel>
    </owl:Class>
    


    <!-- http://standards.iso.org/iso/10303/tech/refdata/core#c27698c0-130a-0135-b552-598f1b1392ae -->

    <owl:Class rdf:about="http://standards.iso.org/iso/10303/tech/refdata/core#c27698c0-130a-0135-b552-598f1b1392ae">
        <rdfs:subClassOf rdf:resource="http://standards.iso.org/iso/10303/tech/refdata/core#STEPThing"/>
        <dc:contributor>STEP Harmonization Team</dc:contributor>
        <dc:creator>Phil Spiby, Eurostep</dc:creator>
        <dc:date>2022-09-01</dc:date>
        <dc:source>ISO/TS 10303-4000</dc:source>
        <dc:type>InWork</dc:type>
        <rdfs:comment xml:lang="en">A PropertyValue is the representation of PropertyDefinition by a numerical or textual value.</rdfs:comment>
        <owl:versionInfo>1</owl:versionInfo>
        <skos:changeNote>[2021-07-30] Initial definition.</skos:changeNote>
        <skos:prefLabel xml:lang="en">property value</skos:prefLabel>
    </owl:Class>
    


    <!-- http://standards.iso.org/iso/10303/tech/refdata/core#c2d3ace0-130a-0135-b552-598f1b1392ae -->

    <owl:Class rdf:about="http://standards.iso.org/iso/10303/tech/refdata/core#c2d3ace0-130a-0135-b552-598f1b1392ae">
        <rdfs:subClassOf rdf:resource="http://standards.iso.org/iso/10303/tech/refdata/core#1cfca290-3279-0135-b58f-598f1b1392ae"/>
        <dc:contributor>STEP Harmonization Team</dc:contributor>
        <dc:creator>Phil Spiby, Eurostep</dc:creator>
        <dc:date>2022-09-01</dc:date>
        <dc:source>ISO/TS 10303-4000</dc:source>
        <dc:type>InWork</dc:type>
        <rdfs:comment xml:lang="en">A PropertyValueAssignment is an assignment of a PropertyValue to an item (specified by PropertyAssignmentSelect). The meaning of the assignment can be specified using the ClassifiedAs attribute inherited from the AssignmentObject.</rdfs:comment>
        <owl:versionInfo>2</owl:versionInfo>
        <skos:changeNote>[2021-07-30] Initial definition.</skos:changeNote>
        <skos:changeNote>[2022-09-01] Phil Spiby, Eurostep: updated comment.</skos:changeNote>
        <skos:prefLabel xml:lang="en">property value assignment</skos:prefLabel>
    </owl:Class>
    


    <!-- http://standards.iso.org/iso/10303/tech/refdata/core#c359f3e0-130a-0135-b552-598f1b1392ae -->

    <owl:Class rdf:about="http://standards.iso.org/iso/10303/tech/refdata/core#c359f3e0-130a-0135-b552-598f1b1392ae">
        <rdfs:subClassOf rdf:resource="http://standards.iso.org/iso/10303/tech/refdata/core#59b11220-3279-0135-b58f-598f1b1392ae"/>
        <dc:contributor>STEP Harmonization Team</dc:contributor>
        <dc:creator>Phil Spiby, Eurostep</dc:creator>
        <dc:date>2022-09-01</dc:date>
        <dc:source>ISO/TS 10303-4000</dc:source>
        <dc:type>InWork</dc:type>
        <rdfs:comment xml:lang="en">A PropertyValueAssignmentRelationship is a relation between two PropertyValueAssignment objects.</rdfs:comment>
        <owl:versionInfo>2</owl:versionInfo>
        <skos:changeNote>[2021-07-30] Initial definition.</skos:changeNote>
        <skos:changeNote>[2022-09-01] Phil Spiby, Eurostep: updated comment.</skos:changeNote>
        <skos:prefLabel xml:lang="en">property value assignment relationship</skos:prefLabel>
    </owl:Class>
    


    <!-- http://standards.iso.org/iso/10303/tech/refdata/core#c3aad300-130a-0135-b552-598f1b1392ae -->

    <owl:Class rdf:about="http://standards.iso.org/iso/10303/tech/refdata/core#c3aad300-130a-0135-b552-598f1b1392ae">
        <rdfs:subClassOf rdf:resource="http://standards.iso.org/iso/10303/tech/refdata/core#59b11220-3279-0135-b58f-598f1b1392ae"/>
        <dc:contributor>STEP Harmonization Team</dc:contributor>
        <dc:creator>Phil Spiby, Eurostep</dc:creator>
        <dc:date>2022-09-01</dc:date>
        <dc:source>ISO/TS 10303-4000</dc:source>
        <dc:type>InWork</dc:type>
        <rdfs:comment xml:lang="en">A PropertyValueRelationship is a relation between two PropertyValue objects.</rdfs:comment>
        <owl:versionInfo>2</owl:versionInfo>
        <skos:changeNote>[2021-07-30] Initial definition.</skos:changeNote>
        <skos:changeNote>[2022-09-01] Phil Spiby, Eurostep: updated comment.</skos:changeNote>
        <skos:prefLabel xml:lang="en">property value relationship</skos:prefLabel>
    </owl:Class>
    


    <!-- http://standards.iso.org/iso/10303/tech/refdata/core#c4425810-130a-0135-b552-598f1b1392ae -->

    <owl:Class rdf:about="http://standards.iso.org/iso/10303/tech/refdata/core#c4425810-130a-0135-b552-598f1b1392ae">
        <rdfs:subClassOf rdf:resource="http://standards.iso.org/iso/10303/tech/refdata/core#59b11220-3279-0135-b58f-598f1b1392ae"/>
        <dc:contributor>STEP Harmonization Team</dc:contributor>
        <dc:creator>Phil Spiby, Eurostep</dc:creator>
        <dc:date>2022-09-01</dc:date>
        <dc:source>ISO/TS 10303-4000</dc:source>
        <dc:type>InWork</dc:type>
        <rdfs:comment xml:lang="en">A ProxyRelationship is a relationship between two Proxy objects.</rdfs:comment>
        <owl:versionInfo>2</owl:versionInfo>
        <skos:changeNote>[2021-07-30] Initial definition.</skos:changeNote>
        <skos:changeNote>[2022-09-01] Phil Spiby, Eurostep: updated comment.</skos:changeNote>
        <skos:prefLabel xml:lang="en">proxy relationship</skos:prefLabel>
    </owl:Class>
    


    <!-- http://standards.iso.org/iso/10303/tech/refdata/core#c454cd88-1e0a-4f7f-abb6-66636ec084dc -->

    <owl:Class rdf:about="http://standards.iso.org/iso/10303/tech/refdata/core#c454cd88-1e0a-4f7f-abb6-66636ec084dc">
        <rdfs:subClassOf rdf:resource="http://standards.iso.org/iso/10303/tech/refdata/core#78133794-f9d2-4e22-aaa0-49690cc93a39"/>
        <dc:contributor>STEP Harmonization Team</dc:contributor>
        <dc:creator>Jean Brangé, AFNeT Services</dc:creator>
        <dc:date>2023-10-04</dc:date>
        <dc:source>ISO/TS 10303-4000</dc:source>
        <dc:type>InWork</dc:type>
        <rdfs:comment xml:lang="en">A CrossSectionalGroupShapeElementWithLacing is a type of CrossSectionalGroupShapeElement where the group is established by lacing.</rdfs:comment>
        <owl:versionInfo>3</owl:versionInfo>
        <skos:changeNote>[2023-10-04] Jean Brangé, AFNeT Services: Initial definition.</skos:changeNote>
        <skos:prefLabel xml:lang="en">cross sectional group shape element with lacing</skos:prefLabel>
    </owl:Class>
    


    <!-- http://standards.iso.org/iso/10303/tech/refdata/core#c49029f0-130a-0135-b552-598f1b1392ae -->

    <owl:Class rdf:about="http://standards.iso.org/iso/10303/tech/refdata/core#c49029f0-130a-0135-b552-598f1b1392ae">
        <rdfs:subClassOf rdf:resource="http://standards.iso.org/iso/10303/tech/refdata/core#d66b1630-130a-0135-b552-598f1b1392ae"/>
        <dc:contributor>STEP Harmonization Team</dc:contributor>
        <dc:creator>Phil Spiby, Eurostep</dc:creator>
        <dc:date>2022-09-01</dc:date>
        <dc:source>ISO/TS 10303-4000</dc:source>
        <dc:type>InWork</dc:type>
        <rdfs:comment xml:lang="en">A QualitativeUncertainty is a type of UncertaintyQualifier. The uncertainty is defined in clause 2 of &apos;The Guide to the Expression of Uncertainty in Measurement&apos;.</rdfs:comment>
        <owl:versionInfo>2</owl:versionInfo>
        <skos:changeNote>[2021-07-30] Initial definition.</skos:changeNote>
        <skos:changeNote>[2022-09-01] Phil Spiby, Eurostep: updated comment.</skos:changeNote>
        <skos:prefLabel xml:lang="en">qualitative uncertainty</skos:prefLabel>
    </owl:Class>
    


    <!-- http://standards.iso.org/iso/10303/tech/refdata/core#c4a27970-130a-0135-b552-598f1b1392ae -->

    <owl:Class rdf:about="http://standards.iso.org/iso/10303/tech/refdata/core#c4a27970-130a-0135-b552-598f1b1392ae">
        <rdfs:subClassOf rdf:resource="http://standards.iso.org/iso/10303/tech/refdata/core#94453010-130a-0135-b552-598f1b1392ae"/>
        <dc:contributor>STEP Harmonization Team</dc:contributor>
        <dc:creator>Phil Spiby, Eurostep</dc:creator>
        <dc:date>2022-09-01</dc:date>
        <dc:source>ISO/TS 10303-4000</dc:source>
        <dc:type>InWork</dc:type>
        <rdfs:comment xml:lang="en">A QuantifiedOccurrence is a type of DefinitionBasedOccurrence which is quantified, or whose quantity depends on certain constraints.</rdfs:comment>
        <owl:versionInfo>2</owl:versionInfo>
        <skos:changeNote>[2021-07-30] Initial definition.</skos:changeNote>
        <skos:changeNote>[2022-09-01] Phil Spiby, Eurostep: updated example.</skos:changeNote>
        <skos:example xml:lang="en">In a BOM where the exact amount of grease or glue can usually not be specified as a quantity, the specification of this grease or glue are examples for giving just a selection criterion instead of an exact quantity.</skos:example>
        <skos:example xml:lang="en">In a TechnicalSolution for the front left brake a certain screw is used four times.</skos:example>
        <skos:example xml:lang="en">Radiator liquid or engine oil are examples for QuantifiedOccurrence objects.</skos:example>
        <skos:example xml:lang="en">To minimize the concentricity error of a wheel, weights are attached to the rim; this set of weights is a QuantifiedOccurrence whose quantity is defined by a criterion. The quantity as well as the position of these weights depends on the concentricity behaviour of each specific wheel as manufactured and tested.</skos:example>
        <skos:prefLabel xml:lang="en">quantified occurrence</skos:prefLabel>
    </owl:Class>
    


    <!-- http://standards.iso.org/iso/10303/tech/refdata/core#c4c19a30-130a-0135-b552-598f1b1392ae -->

    <owl:Class rdf:about="http://standards.iso.org/iso/10303/tech/refdata/core#c4c19a30-130a-0135-b552-598f1b1392ae">
        <rdfs:subClassOf rdf:resource="http://standards.iso.org/iso/10303/tech/refdata/core#a3571140-130a-0135-b552-598f1b1392ae"/>
        <dc:contributor>STEP Harmonization Team</dc:contributor>
        <dc:creator>Phil Spiby, Eurostep</dc:creator>
        <dc:date>2022-09-01</dc:date>
        <dc:source>ISO/TS 10303-4000</dc:source>
        <dc:type>InWork</dc:type>
        <rdfs:comment xml:lang="en">A RealizedIndividualPart is a type of IndividualPartVersion that represents a version of a realized artefact.</rdfs:comment>
        <owl:versionInfo>2</owl:versionInfo>
        <skos:changeNote>[2021-07-30] Initial definition.</skos:changeNote>
        <skos:changeNote>[2022-09-01] Phil Spiby, Eurostep: updated note.</skos:changeNote>
        <skos:note xml:lang="en">The artefact can have been made from a version of a part design (PartVersion). If this is the case, then the relationship between the artefact (RealizedIndividualPart) and the design (PartVersion) is represented by PartVersionToIndividualPartVersionAssociation.</skos:note>
        <skos:note xml:lang="en">The artefact can have been planned and represented by PlannedIndividualPart. In which case, the actual artefact (RealizedIndividualPart) is related to the planned artefact (PlannedIndividualPart) by the ProductPlannedToRealized relationship.</skos:note>
        <skos:note xml:lang="en">Where physical parts are being represented, the RealizedIndividualPart represents the physical part - something one can touch.</skos:note>
        <skos:prefLabel xml:lang="en">realized individual part</skos:prefLabel>
    </owl:Class>
    


    <!-- http://standards.iso.org/iso/10303/tech/refdata/core#c53987ca-d3b6-49ea-9dae-bd3865e2bb27 -->

    <owl:Class rdf:about="http://standards.iso.org/iso/10303/tech/refdata/core#c53987ca-d3b6-49ea-9dae-bd3865e2bb27">
        <rdfs:subClassOf rdf:resource="http://standards.iso.org/iso/10303/tech/refdata/core#f8816baf-d66a-42f9-bdcc-38e946c9a2fa"/>
        <dc:contributor>STEP Harmonization Team</dc:contributor>
        <dc:creator>Jean Brangé, AFNeT Services</dc:creator>
        <dc:date>2023-10-04</dc:date>
        <dc:source>ISO/TS 10303-4000</dc:source>
        <dc:type>InWork</dc:type>
        <rdfs:comment xml:lang="en">A GeometricAlignment is a type of DerivedShapeElement that defines a planar or linear feature that requires two or more features lying in the same plane or along the same line.</rdfs:comment>
        <owl:versionInfo>3</owl:versionInfo>
        <skos:changeNote>[2023-10-04] Jean Brangé, AFNeT Services: Initial definition.</skos:changeNote>
        <skos:prefLabel xml:lang="en">geometric alignment</skos:prefLabel>
    </owl:Class>
    


    <!-- http://standards.iso.org/iso/10303/tech/refdata/core#c54437b0-130a-0135-b552-598f1b1392ae -->

    <owl:Class rdf:about="http://standards.iso.org/iso/10303/tech/refdata/core#c54437b0-130a-0135-b552-598f1b1392ae">
        <rdfs:subClassOf rdf:resource="http://standards.iso.org/iso/10303/tech/refdata/core#b44098a0-130a-0135-b552-598f1b1392ae"/>
        <dc:contributor>STEP Harmonization Team</dc:contributor>
        <dc:creator>Phil Spiby, Eurostep</dc:creator>
        <dc:date>2022-09-01</dc:date>
        <dc:source>ISO/TS 10303-4000</dc:source>
        <dc:type>InWork</dc:type>
        <rdfs:comment xml:lang="en">A ReplacedPartViewRelationship is a type of PartViewRelationship where the Relating PartView is replaced by the Related PartView. Each ReplacedPartViewRelationship shall be referenced by an Effectivity that defines the start of the validity of the replacement.</rdfs:comment>
        <owl:versionInfo>2</owl:versionInfo>
        <skos:changeNote>[2021-07-30] Initial definition.</skos:changeNote>
        <skos:changeNote>[2022-09-01] Phil Spiby, Eurostep: updated note.</skos:changeNote>
        <skos:note xml:lang="en">A ReplacedPartViewRelationship can be used to build up version sequences of PartView objects.</skos:note>
        <skos:prefLabel xml:lang="en">replaced part view relationship</skos:prefLabel>
    </owl:Class>
    


    <!-- http://standards.iso.org/iso/10303/tech/refdata/core#c54bc6fa-f6d8-4943-85de-6439071c5325 -->

    <owl:Class rdf:about="http://standards.iso.org/iso/10303/tech/refdata/core#c54bc6fa-f6d8-4943-85de-6439071c5325">
        <rdfs:subClassOf rdf:resource="http://standards.iso.org/iso/10303/tech/refdata/core#0cc8b831-37f7-4cd5-984f-dbb5588fbc1d"/>
        <dc:contributor>STEP Harmonization Team</dc:contributor>
        <dc:creator>Jean Brangé, AFNeT Services</dc:creator>
        <dc:date>2023-10-04</dc:date>
        <dc:source>ISO/TS 10303-4000</dc:source>
        <dc:type>InWork</dc:type>
        <rdfs:comment xml:lang="en">A CrossSectionalPartShapeElement is a type of PartShapeElement that defines the cross-sectional shape of an extruded object perpendicular to the local centre line. The shape of the cross section is perpendicular to the local centre line in the geometric representation.</rdfs:comment>
        <owl:versionInfo>3</owl:versionInfo>
        <skos:changeNote>[2023-10-04] Jean Brangé, AFNeT Services: Initial definition.</skos:changeNote>
        <skos:prefLabel xml:lang="en">cross sectional part shape element</skos:prefLabel>
    </owl:Class>
    


    <!-- http://standards.iso.org/iso/10303/tech/refdata/core#c54ee610-130a-0135-b552-598f1b1392ae -->

    <owl:Class rdf:about="http://standards.iso.org/iso/10303/tech/refdata/core#c54ee610-130a-0135-b552-598f1b1392ae">
        <rdfs:subClassOf rdf:resource="http://standards.iso.org/iso/10303/tech/refdata/core#aeba1b40-130a-0135-b552-598f1b1392ae"/>
        <dc:contributor>STEP Harmonization Team</dc:contributor>
        <dc:creator>Phil Spiby, Eurostep</dc:creator>
        <dc:date>2022-09-01</dc:date>
        <dc:source>ISO/TS 10303-4000</dc:source>
        <dc:type>InWork</dc:type>
        <rdfs:comment xml:lang="en">A ReplacedUsageRelationship is a type of OccurrenceRelationship that is a relationship between two Occurrence objects where the relating Occurrence is replaced by the related Occurrence.</rdfs:comment>
        <owl:versionInfo>2</owl:versionInfo>
        <skos:changeNote>[2021-07-30] Initial definition.</skos:changeNote>
        <skos:changeNote>[2022-09-01] Phil Spiby, Eurostep: updated comment.</skos:changeNote>
        <skos:prefLabel xml:lang="en">replaced usage relationship</skos:prefLabel>
    </owl:Class>
    


    <!-- http://standards.iso.org/iso/10303/tech/refdata/core#c565c970-130a-0135-b552-598f1b1392ae -->

    <owl:Class rdf:about="http://standards.iso.org/iso/10303/tech/refdata/core#c565c970-130a-0135-b552-598f1b1392ae">
        <rdfs:subClassOf rdf:resource="http://standards.iso.org/iso/10303/tech/refdata/core#STEPThing"/>
        <dc:contributor>STEP Harmonization Team</dc:contributor>
        <dc:creator>Phil Spiby, Eurostep</dc:creator>
        <dc:date>2022-09-01</dc:date>
        <dc:source>ISO/TS 10303-4000</dc:source>
        <dc:type>InWork</dc:type>
        <rdfs:comment xml:lang="en">A Representation is a collection of one or more instances of RepresentationItem that are related in the specified RepresentationContext.</rdfs:comment>
        <owl:versionInfo>1</owl:versionInfo>
        <skos:changeNote>[2021-07-30] Initial definition.</skos:changeNote>
        <skos:prefLabel xml:lang="en">representation</skos:prefLabel>
    </owl:Class>
    


    <!-- http://standards.iso.org/iso/10303/tech/refdata/core#c6005999-ccf2-4503-bc60-2c802fda2358 -->

    <owl:Class rdf:about="http://standards.iso.org/iso/10303/tech/refdata/core#c6005999-ccf2-4503-bc60-2c802fda2358">
        <rdfs:subClassOf rdf:resource="http://standards.iso.org/iso/10303/tech/refdata/core#528ada01-3556-4da5-ab84-ee62c9d68215"/>
        <dc:contributor>STEP Harmonization Team</dc:contributor>
        <dc:creator>Jean Brangé, AFNeT Services</dc:creator>
        <dc:date>2023-10-04</dc:date>
        <dc:source>ISO/TS 10303-4000</dc:source>
        <dc:type>InWork</dc:type>
        <rdfs:comment xml:lang="en">An AllAroundShapeElementAlongCollectionPlane is a type of AllAroundShapeElement that represents the &quot;all around&quot; along a specified &quot;collection plane&quot; as defined in ISO 1101.</rdfs:comment>
        <owl:versionInfo>3</owl:versionInfo>
        <skos:changeNote>[2023-10-04] Jean Brangé, AFNeT Services: Initial definition.</skos:changeNote>
        <skos:prefLabel xml:lang="en">all around shape element along collection plane</skos:prefLabel>
    </owl:Class>
    


    <!-- http://standards.iso.org/iso/10303/tech/refdata/core#c618afb7-ee33-4147-b72f-634b9afff19f -->

    <owl:Class rdf:about="http://standards.iso.org/iso/10303/tech/refdata/core#c618afb7-ee33-4147-b72f-634b9afff19f">
        <rdfs:subClassOf rdf:resource="http://standards.iso.org/iso/10303/tech/refdata/core#59b11220-3279-0135-b58f-598f1b1392ae"/>
        <dc:contributor>STEP Harmonization Team</dc:contributor>
        <dc:creator>Phil Spiby, Eurostep</dc:creator>
        <dc:date>2022-09-01</dc:date>
        <dc:source>ISO/TS 10303-4000</dc:source>
        <dc:type>InWork</dc:type>
        <rdfs:comment xml:lang="en">A ProductGroupRelationship is a relationship between two ProductGroup objects.</rdfs:comment>
        <owl:versionInfo>1</owl:versionInfo>
        <skos:changeNote>[2022-09-01] Initial definition.</skos:changeNote>
        <skos:note xml:lang="en">A subset is a common type of relationship. It indicates that one ProductGroup is a subset of another.</skos:note>
        <skos:prefLabel xml:lang="en">product group relationship</skos:prefLabel>
    </owl:Class>
    


    <!-- http://standards.iso.org/iso/10303/tech/refdata/core#c6260c30-130a-0135-b552-598f1b1392ae -->

    <owl:Class rdf:about="http://standards.iso.org/iso/10303/tech/refdata/core#c6260c30-130a-0135-b552-598f1b1392ae">
        <rdfs:subClassOf rdf:resource="http://standards.iso.org/iso/10303/tech/refdata/core#59b11220-3279-0135-b58f-598f1b1392ae"/>
        <dc:contributor>STEP Harmonization Team</dc:contributor>
        <dc:creator>Phil Spiby, Eurostep</dc:creator>
        <dc:date>2022-09-01</dc:date>
        <dc:source>ISO/TS 10303-4000</dc:source>
        <dc:type>InWork</dc:type>
        <rdfs:comment xml:lang="en">A RepresentationRelationship is a relationship between two Representation objects.</rdfs:comment>
        <owl:versionInfo>2</owl:versionInfo>
        <skos:changeNote>[2021-07-30] Initial definition.</skos:changeNote>
        <skos:changeNote>[2022-09-01] Phil Spiby, Eurostep: updated comment.</skos:changeNote>
        <skos:prefLabel xml:lang="en">representation relationship</skos:prefLabel>
    </owl:Class>
    


    <!-- http://standards.iso.org/iso/10303/tech/refdata/core#c678796f-6801-40d9-9d18-f4d8c2e438b5 -->

    <owl:Class rdf:about="http://standards.iso.org/iso/10303/tech/refdata/core#c678796f-6801-40d9-9d18-f4d8c2e438b5">
        <rdfs:subClassOf rdf:resource="http://standards.iso.org/iso/10303/tech/refdata/core#55105ef0-713f-409a-8306-fd8708d4ee3f"/>
        <dc:contributor>STEP Harmonization Team</dc:contributor>
        <dc:creator>Jean Brangé, AFNeT Services</dc:creator>
        <dc:date>2023-10-04</dc:date>
        <dc:source>ISO/TS 10303-4000</dc:source>
        <dc:type>InWork</dc:type>
        <rdfs:comment xml:lang="en">An AngularityTolerance is a type of GeometricTolerance that is a constraint on the location of a surface, of a centre plane, of an edge, or of an axis that lies theoretically at a specified angle (other than 90 degrees) from a datum plane or from a datum axis. Unless otherwise specified the rules governing angularity tolerance defined in ISO 1101 shall apply. The specified angle shall not be a multiple of 90 degrees. In the case of 0 or 180 degrees, a ParallelismTolerance shall be used. In the case of 90 or 270 degrees, a PerpendicularityTolerance shall be used. The specified angle shall be defined using an instance of AngularLocation. The toleranced element is either a plane or a straight line. An AngularityTolerance specifies one of the following: a tolerance zone defined by two parallel planes at the specified basic angle from one or more datum planes or a datum axis within which surface, centre plane or axis of the considered feature must lie; a tolerance zone defined by a cylinder at the specified basic angle from one or more datum planes or a datum axis within which the considered feature must lie; a tolerance zone defined by two parallel lines at the specified basic angle from a datum plane or axis within which the considered element of the feature must lie.</rdfs:comment>
        <owl:versionInfo>3</owl:versionInfo>
        <skos:changeNote>[2023-10-04] Jean Brangé, AFNeT Services: Initial definition.</skos:changeNote>
        <skos:note xml:lang="en">Alternatively angularity tolerance can be used according to the specifications given in ASME Y14.5-2009.</skos:note>
        <skos:prefLabel xml:lang="en">angularity tolerance</skos:prefLabel>
    </owl:Class>
    


    <!-- http://standards.iso.org/iso/10303/tech/refdata/core#c67b5206-e769-4ee8-ae35-1f65831a5658 -->

    <owl:Class rdf:about="http://standards.iso.org/iso/10303/tech/refdata/core#c67b5206-e769-4ee8-ae35-1f65831a5658">
        <rdfs:subClassOf rdf:resource="http://standards.iso.org/iso/10303/tech/refdata/core#9c98fe40-130a-0135-b552-598f1b1392ae"/>
        <dc:contributor>STEP Harmonization Team</dc:contributor>
        <dc:creator>Jean Brangé, AFNeT Services</dc:creator>
        <dc:date>2023-10-04</dc:date>
        <dc:source>ISO/TS 10303-4000</dc:source>
        <dc:type>InWork</dc:type>
        <rdfs:comment xml:lang="en">An ExternalGeometricallyBoundedSurfaceShapeRepresentation is a type of ExternalGeometricModel that references an instance of type ../../../resources/aic_geometrically_bounded_surface/aic_geometrically_bounded_surface.htm#aic_geometrically_bounded_surface.geometrically_bounded_surface_shape_representation geometrically_bounded_surface_shape_representation (ISO 10303-507).</rdfs:comment>
        <owl:versionInfo>3</owl:versionInfo>
        <skos:changeNote>[2023-10-04] Jean Brangé, AFNeT Services: Initial definition.</skos:changeNote>
        <skos:prefLabel xml:lang="en">external geometrically bounded surface shape representation</skos:prefLabel>
    </owl:Class>
    


    <!-- http://standards.iso.org/iso/10303/tech/refdata/core#c6926290-130a-0135-b552-598f1b1392ae -->

    <owl:Class rdf:about="http://standards.iso.org/iso/10303/tech/refdata/core#c6926290-130a-0135-b552-598f1b1392ae">
        <rdfs:subClassOf rdf:resource="http://standards.iso.org/iso/10303/tech/refdata/core#STEPThing"/>
        <dc:contributor>STEP Harmonization Team</dc:contributor>
        <dc:creator>Phil Spiby, Eurostep</dc:creator>
        <dc:date>2022-09-01</dc:date>
        <dc:source>ISO/TS 10303-4000</dc:source>
        <dc:type>InWork</dc:type>
        <rdfs:comment xml:lang="en">A Requirement is an essential characteristic, condition, or capability that shall be met or exceeded by a system or a component to satisfy a contract, standard, specification, or other formally imposed document.</rdfs:comment>
        <owl:versionInfo>2</owl:versionInfo>
        <skos:changeNote>[2021-07-30] Initial definition.</skos:changeNote>
        <skos:changeNote>[2022-09-01] Phil Spiby, Eurostep: updated example updated note.</skos:changeNote>
        <skos:example xml:lang="en">A requirement can be identified as &apos;NOx emissions requirement&apos;, and uniquely identified as &apos;Req2&apos;.</skos:example>
        <skos:note xml:lang="en">Systems engineering tools and organizations can use differing identification mechanisms. Multiple identifiers can be managed in Requirement using the id attribute.</skos:note>
        <skos:note xml:lang="en">The term &apos;requirement&apos; is used here in the sense that term is used in systems engineering and similar industrial domains.</skos:note>
        <skos:note xml:lang="en">There can be many versions of a Requirement through RequirementVersion. There can also be more than one domain-specific view of a given RequirementVersion (using the RequirementView entity). The Requirement entity is simply a placeholder for holding a unique requirement. Most associations and properties could be defined at the Requirement, RequirementVersion or RequirementView level - that is in the context of a domain.</skos:note>
        <skos:prefLabel xml:lang="en">requirement</skos:prefLabel>
    </owl:Class>
    


    <!-- http://standards.iso.org/iso/10303/tech/refdata/core#c6f4a478-1902-4b34-a326-e487ef9007fa -->

    <owl:Class rdf:about="http://standards.iso.org/iso/10303/tech/refdata/core#c6f4a478-1902-4b34-a326-e487ef9007fa">
        <rdfs:subClassOf rdf:resource="http://standards.iso.org/iso/10303/tech/refdata/core#84099bf0-130a-0135-b552-598f1b1392ae"/>
        <dc:contributor>STEP Harmonization Team</dc:contributor>
        <dc:creator>Phil Spiby, Eurostep</dc:creator>
        <dc:date>2022-09-01</dc:date>
        <dc:source>ISO/TS 10303-4000</dc:source>
        <dc:type>InWork</dc:type>
        <rdfs:comment xml:lang="en">A TaskMethodVersionRelationship is a specialization of ActivityMethodRelationship that is a relationship between two TaskMethodVersion objects.</rdfs:comment>
        <owl:versionInfo>2</owl:versionInfo>
        <skos:changeNote>[2021-07-30] Initial definition.</skos:changeNote>
        <skos:changeNote>[2022-09-01] Phil Spiby, Eurostep: updated comment.</skos:changeNote>
        <skos:prefLabel xml:lang="en">task method version relationship</skos:prefLabel>
    </owl:Class>
    


    <!-- http://standards.iso.org/iso/10303/tech/refdata/core#c71722f0-130a-0135-b552-598f1b1392ae -->

    <owl:Class rdf:about="http://standards.iso.org/iso/10303/tech/refdata/core#c71722f0-130a-0135-b552-598f1b1392ae">
        <rdfs:subClassOf rdf:resource="http://standards.iso.org/iso/10303/tech/refdata/core#1cfca290-3279-0135-b58f-598f1b1392ae"/>
        <dc:contributor>STEP Harmonization Team</dc:contributor>
        <dc:creator>Phil Spiby, Eurostep</dc:creator>
        <dc:date>2022-09-01</dc:date>
        <dc:source>ISO/TS 10303-4000</dc:source>
        <dc:type>InWork</dc:type>
        <rdfs:comment xml:lang="en">A RequirementAssignment is an assignment of a Requirement (via a RequirementView) to an item (specified by RequirementAssignmentSelect) which is affected by the requirement. The meaning of the assignment can be specified using the ClassifiedAs attribute inherited from the AssignmentObject.</rdfs:comment>
        <owl:versionInfo>2</owl:versionInfo>
        <skos:changeNote>[2021-07-30] Initial definition.</skos:changeNote>
        <skos:changeNote>[2022-09-01] Phil Spiby, Eurostep: updated comment updated example.</skos:changeNote>
        <skos:example xml:lang="en">A requirement &apos;the vehicle shall have a maximum power output of at least 150BHP&apos; could be assigned to the item which represents the vehicle&apos;s engine.</skos:example>
        <skos:prefLabel xml:lang="en">requirement assignment</skos:prefLabel>
    </owl:Class>
    


    <!-- http://standards.iso.org/iso/10303/tech/refdata/core#c78b1a70-130a-0135-b552-598f1b1392ae -->

    <owl:Class rdf:about="http://standards.iso.org/iso/10303/tech/refdata/core#c78b1a70-130a-0135-b552-598f1b1392ae">
        <rdfs:subClassOf rdf:resource="http://standards.iso.org/iso/10303/tech/refdata/core#ca82fdb0-130a-0135-b552-598f1b1392ae"/>
        <dc:contributor>STEP Harmonization Team</dc:contributor>
        <dc:creator>Phil Spiby, Eurostep</dc:creator>
        <dc:date>2022-09-01</dc:date>
        <dc:source>ISO/TS 10303-4000</dc:source>
        <dc:type>InWork</dc:type>
        <rdfs:comment xml:lang="en">A RequirementCollectionRelationship is a type of RequirementViewRelationship. It identifies a collection relationship that is used to relate a parent (collection) requirement to its member requirements. This provides a method for collecting together a set of requirements and treating them as a single requirement, whilst still being able to refer to individual requirements.</rdfs:comment>
        <owl:versionInfo>1</owl:versionInfo>
        <skos:changeNote>[2021-07-30] Initial definition.</skos:changeNote>
        <skos:prefLabel xml:lang="en">requirement collection relationship</skos:prefLabel>
    </owl:Class>
    


    <!-- http://standards.iso.org/iso/10303/tech/refdata/core#c7974f70-130a-0135-b552-598f1b1392ae -->

    <owl:Class rdf:about="http://standards.iso.org/iso/10303/tech/refdata/core#c7974f70-130a-0135-b552-598f1b1392ae">
        <rdfs:subClassOf rdf:resource="http://standards.iso.org/iso/10303/tech/refdata/core#ca82fdb0-130a-0135-b552-598f1b1392ae"/>
        <dc:contributor>STEP Harmonization Team</dc:contributor>
        <dc:creator>Phil Spiby, Eurostep</dc:creator>
        <dc:date>2022-09-01</dc:date>
        <dc:source>ISO/TS 10303-4000</dc:source>
        <dc:type>InWork</dc:type>
        <rdfs:comment xml:lang="en">A RequirementDecompositionRelationship is a type of RequirementViewRelationship that identifies a decomposition relationship. This provides a method to represent that a Related RequirementView is a decomposition of a Relating RequirementView.</rdfs:comment>
        <owl:versionInfo>2</owl:versionInfo>
        <skos:changeNote>[2021-07-30] Initial definition.</skos:changeNote>
        <skos:changeNote>[2022-09-01] Phil Spiby, Eurostep: updated comment.</skos:changeNote>
        <skos:prefLabel xml:lang="en">requirement decomposition relationship</skos:prefLabel>
    </owl:Class>
    


    <!-- http://standards.iso.org/iso/10303/tech/refdata/core#c79d69f0-130a-0135-b552-598f1b1392ae -->

    <owl:Class rdf:about="http://standards.iso.org/iso/10303/tech/refdata/core#c79d69f0-130a-0135-b552-598f1b1392ae">
        <rdfs:subClassOf rdf:resource="http://standards.iso.org/iso/10303/tech/refdata/core#59b11220-3279-0135-b58f-598f1b1392ae"/>
        <dc:contributor>STEP Harmonization Team</dc:contributor>
        <dc:creator>Phil Spiby, Eurostep</dc:creator>
        <dc:date>2022-09-01</dc:date>
        <dc:source>ISO/TS 10303-4000</dc:source>
        <dc:type>InWork</dc:type>
        <rdfs:comment xml:lang="en">A RequirementRelationship is a relationship between two Requirement objects.</rdfs:comment>
        <owl:versionInfo>2</owl:versionInfo>
        <skos:changeNote>[2021-07-30] Initial definition.</skos:changeNote>
        <skos:changeNote>[2022-09-01] Phil Spiby, Eurostep: updated comment.</skos:changeNote>
        <skos:prefLabel xml:lang="en">requirement relationship</skos:prefLabel>
    </owl:Class>
    


    <!-- http://standards.iso.org/iso/10303/tech/refdata/core#c7f15650-130a-0135-b552-598f1b1392ae -->

    <owl:Class rdf:about="http://standards.iso.org/iso/10303/tech/refdata/core#c7f15650-130a-0135-b552-598f1b1392ae">
        <rdfs:subClassOf rdf:resource="http://standards.iso.org/iso/10303/tech/refdata/core#STEPThing"/>
        <dc:contributor>STEP Harmonization Team</dc:contributor>
        <dc:creator>Phil Spiby, Eurostep</dc:creator>
        <dc:date>2022-09-01</dc:date>
        <dc:source>ISO/TS 10303-4000</dc:source>
        <dc:type>InWork</dc:type>
        <rdfs:comment xml:lang="en">A RequirementSatisfactionAssertion is a relationship between an item (specified in RequirementAssignmentSelect) and a Requirement (via the RequirementView), asserting that the item satisfies the identified requirement.</rdfs:comment>
        <owl:versionInfo>2</owl:versionInfo>
        <skos:changeNote>[2021-07-30] Initial definition.</skos:changeNote>
        <skos:changeNote>[2022-09-01] Phil Spiby, Eurostep: updated example.</skos:changeNote>
        <skos:example xml:lang="en">A data type used to represent a vehicle&apos;s engine with a power output of 160BHP could be asserted to satisfy a requirement &apos;the vehicle shall have a maximum power output of at least 150BHP&apos;.</skos:example>
        <skos:prefLabel xml:lang="en">requirement satisfaction assertion</skos:prefLabel>
    </owl:Class>
    


    <!-- http://standards.iso.org/iso/10303/tech/refdata/core#c80bddee-4665-47e8-af7e-3033f14e7f65 -->

    <owl:Class rdf:about="http://standards.iso.org/iso/10303/tech/refdata/core#c80bddee-4665-47e8-af7e-3033f14e7f65">
        <rdfs:subClassOf rdf:resource="http://standards.iso.org/iso/10303/tech/refdata/core#66348150-092a-4eb7-9561-0b83adfa15ff"/>
        <dc:contributor>STEP Harmonization Team</dc:contributor>
        <dc:creator>Jean Brangé, AFNeT Services</dc:creator>
        <dc:date>2023-10-04</dc:date>
        <dc:source>ISO/TS 10303-4000</dc:source>
        <dc:type>InWork</dc:type>
        <rdfs:comment xml:lang="en">A PlaneShapeElement is a type of ShapeElement that is associated with a Plane.</rdfs:comment>
        <owl:versionInfo>3</owl:versionInfo>
        <skos:changeNote>[2023-10-04] Jean Brangé, AFNeT Services: Initial definition.</skos:changeNote>
        <skos:prefLabel xml:lang="en">plane shape element</skos:prefLabel>
    </owl:Class>
    


    <!-- http://standards.iso.org/iso/10303/tech/refdata/core#c85484f0-130a-0135-b552-598f1b1392ae -->

    <owl:Class rdf:about="http://standards.iso.org/iso/10303/tech/refdata/core#c85484f0-130a-0135-b552-598f1b1392ae">
        <rdfs:subClassOf rdf:resource="http://standards.iso.org/iso/10303/tech/refdata/core#STEPThing"/>
        <dc:contributor>STEP Harmonization Team</dc:contributor>
        <dc:creator>Phil Spiby, Eurostep</dc:creator>
        <dc:date>2022-09-01</dc:date>
        <dc:source>ISO/TS 10303-4000</dc:source>
        <dc:type>InWork</dc:type>
        <rdfs:comment xml:lang="en">A RequirementSource is a relationship between a requirement (via the RequirementView) and an item representing the source (specified in RequirementSourceSelect) of the requirement.</rdfs:comment>
        <owl:versionInfo>1</owl:versionInfo>
        <skos:changeNote>[2021-07-30] Initial definition.</skos:changeNote>
        <skos:prefLabel xml:lang="en">requirement source</skos:prefLabel>
    </owl:Class>
    


    <!-- http://standards.iso.org/iso/10303/tech/refdata/core#c8bc4770-130a-0135-b552-598f1b1392ae -->

    <owl:Class rdf:about="http://standards.iso.org/iso/10303/tech/refdata/core#c8bc4770-130a-0135-b552-598f1b1392ae">
        <rdfs:subClassOf rdf:resource="http://standards.iso.org/iso/10303/tech/refdata/core#ca82fdb0-130a-0135-b552-598f1b1392ae"/>
        <dc:contributor>STEP Harmonization Team</dc:contributor>
        <dc:creator>Phil Spiby, Eurostep</dc:creator>
        <dc:date>2022-09-01</dc:date>
        <dc:source>ISO/TS 10303-4000</dc:source>
        <dc:type>InWork</dc:type>
        <rdfs:comment xml:lang="en">A RequirementTracingRelationship is a type of RequirementViewRelationship. It identifies a tracing relationship.</rdfs:comment>
        <owl:versionInfo>2</owl:versionInfo>
        <skos:changeNote>[2021-07-30] Initial definition.</skos:changeNote>
        <skos:changeNote>[2022-09-01] Phil Spiby, Eurostep: updated example.</skos:changeNote>
        <skos:example xml:lang="en">A requirement on the performance of a catalytic converter in a car can be traced from a more general emissions requirement. A requirement can trace to many other requirements and vice versa - this is achieved by creating multiple instances of the tracing relationship entity.</skos:example>
        <skos:prefLabel xml:lang="en">requirement tracing relationship</skos:prefLabel>
    </owl:Class>
    


    <!-- http://standards.iso.org/iso/10303/tech/refdata/core#c8c3e890-130a-0135-b552-598f1b1392ae -->

    <owl:Class rdf:about="http://standards.iso.org/iso/10303/tech/refdata/core#c8c3e890-130a-0135-b552-598f1b1392ae">
        <rdfs:subClassOf rdf:resource="http://standards.iso.org/iso/10303/tech/refdata/core#STEPThing"/>
        <dc:contributor>STEP Harmonization Team</dc:contributor>
        <dc:creator>Phil Spiby, Eurostep</dc:creator>
        <dc:date>2022-09-01</dc:date>
        <dc:source>ISO/TS 10303-4000</dc:source>
        <dc:type>InWork</dc:type>
        <rdfs:comment xml:lang="en">A RequirementVersion is the identification of a specific version of a requirement.</rdfs:comment>
        <owl:versionInfo>2</owl:versionInfo>
        <skos:changeNote>[2021-07-30] Initial definition.</skos:changeNote>
        <skos:changeNote>[2022-09-01] Phil Spiby, Eurostep: updated note.</skos:changeNote>
        <skos:example xml:lang="en">A given requirement might have versions 1.0, 1.1, 1.2 and 2.0.</skos:example>
        <skos:note xml:lang="en">This entity is used to record different versions of a requirement. In this case, the word &apos;version&apos; implies &apos;revision&apos; - that is a specific release of a requirement.</skos:note>
        <skos:prefLabel xml:lang="en">requirement version</skos:prefLabel>
    </owl:Class>
    


    <!-- http://standards.iso.org/iso/10303/tech/refdata/core#c9504a10-130a-0135-b552-598f1b1392ae -->

    <owl:Class rdf:about="http://standards.iso.org/iso/10303/tech/refdata/core#c9504a10-130a-0135-b552-598f1b1392ae">
        <rdfs:subClassOf rdf:resource="http://standards.iso.org/iso/10303/tech/refdata/core#59b11220-3279-0135-b58f-598f1b1392ae"/>
        <dc:contributor>STEP Harmonization Team</dc:contributor>
        <dc:creator>Phil Spiby, Eurostep</dc:creator>
        <dc:date>2022-09-01</dc:date>
        <dc:source>ISO/TS 10303-4000</dc:source>
        <dc:type>InWork</dc:type>
        <rdfs:comment xml:lang="en">A RequirementVersionRelationship is a relationship between two RequirementVersion objects.</rdfs:comment>
        <owl:versionInfo>2</owl:versionInfo>
        <skos:changeNote>[2021-07-30] Initial definition.</skos:changeNote>
        <skos:changeNote>[2022-09-01] Phil Spiby, Eurostep: updated comment.</skos:changeNote>
        <skos:prefLabel xml:lang="en">requirement version relationship</skos:prefLabel>
    </owl:Class>
    


    <!-- http://standards.iso.org/iso/10303/tech/refdata/core#c9cbe2b0-130a-0135-b552-598f1b1392ae -->

    <owl:Class rdf:about="http://standards.iso.org/iso/10303/tech/refdata/core#c9cbe2b0-130a-0135-b552-598f1b1392ae">
        <rdfs:subClassOf rdf:resource="http://standards.iso.org/iso/10303/tech/refdata/core#STEPThing"/>
        <dc:contributor>STEP Harmonization Team</dc:contributor>
        <dc:creator>Phil Spiby, Eurostep</dc:creator>
        <dc:date>2022-09-01</dc:date>
        <dc:source>ISO/TS 10303-4000</dc:source>
        <dc:type>InWork</dc:type>
        <rdfs:comment xml:lang="en">A RequirementView is a view of a requirement version relevant for one or more application domains. This view collects requirement data for specific engineering purposes. Some requirements in a RequirementView might impact on different disciplines. Multiple RequirementView instances can be used to present different views of a given requirement for each discipline. The definition of the requirement is represented by a set of definitional properties referenced from RequirementView.definitionalRepresentations. If more than one definitional property is provided each property shall be equivalent. Any other property that is associated with the RequirementView is assumed to be a non-defining property, such as an annotation etc.</rdfs:comment>
        <owl:versionInfo>2</owl:versionInfo>
        <skos:changeNote>[2021-07-30] Initial definition.</skos:changeNote>
        <skos:changeNote>[2022-09-01] Phil Spiby, Eurostep: updated comment updated example.</skos:changeNote>
        <skos:example xml:lang="en">An engineer can have responsibility for collecting all requirements associated with the cooling of an engine - covering engine block, tubing, water pump, electric fan.</skos:example>
        <skos:example xml:lang="en">The requirement that the weight should be less than 4 Kg can be represented by a string representation &apos;weight shall be 4 Kg&apos; and a numeric representation &apos;4 Kg&apos; specified as a value with units.</skos:example>
        <skos:prefLabel xml:lang="en">requirement view</skos:prefLabel>
    </owl:Class>
    


    <!-- http://standards.iso.org/iso/10303/tech/refdata/core#ca82fdb0-130a-0135-b552-598f1b1392ae -->

    <owl:Class rdf:about="http://standards.iso.org/iso/10303/tech/refdata/core#ca82fdb0-130a-0135-b552-598f1b1392ae">
        <rdfs:subClassOf rdf:resource="http://standards.iso.org/iso/10303/tech/refdata/core#59b11220-3279-0135-b58f-598f1b1392ae"/>
        <dc:contributor>STEP Harmonization Team</dc:contributor>
        <dc:creator>Phil Spiby, Eurostep</dc:creator>
        <dc:date>2022-09-01</dc:date>
        <dc:source>ISO/TS 10303-4000</dc:source>
        <dc:type>InWork</dc:type>
        <rdfs:comment xml:lang="en">A RequirementViewRelationship is a relationship between two RequirementView objects.</rdfs:comment>
        <owl:versionInfo>2</owl:versionInfo>
        <skos:changeNote>[2021-07-30] Initial definition.</skos:changeNote>
        <skos:changeNote>[2022-09-01] Phil Spiby, Eurostep: updated comment.</skos:changeNote>
        <skos:prefLabel xml:lang="en">requirement view relationship</skos:prefLabel>
    </owl:Class>
    


    <!-- http://standards.iso.org/iso/10303/tech/refdata/core#caf921d7-c92e-43bf-988c-f606357d6089 -->

    <owl:Class rdf:about="http://standards.iso.org/iso/10303/tech/refdata/core#caf921d7-c92e-43bf-988c-f606357d6089">
        <rdfs:subClassOf rdf:resource="http://standards.iso.org/iso/10303/tech/refdata/core#1d59c650-3279-0135-b58f-598f1b1392ae"/>
        <dc:contributor>STEP Harmonization Team</dc:contributor>
        <dc:creator>Phil Spiby, Eurostep</dc:creator>
        <dc:date>2022-09-01</dc:date>
        <dc:source>ISO/TS 10303-4000</dc:source>
        <dc:type>InWork</dc:type>
        <rdfs:comment xml:lang="en">An ActivityMethodRealization is a specialization of an AssociationObject. It is a further specification of how an activity method is to be performed with the ActivityMethod.</rdfs:comment>
        <owl:versionInfo>2</owl:versionInfo>
        <skos:changeNote>[2021-07-30] Initial definition.</skos:changeNote>
        <skos:changeNote>[2022-09-01] Phil Spiby, Eurostep: updated example.</skos:changeNote>
        <skos:example xml:lang="en">For a given planned activity there can be a task specification, a statement of how task performance is to be logged and a schedule that all apply.</skos:example>
        <skos:note xml:lang="en">More than one specification can be associated with the same ActivityMethod.</skos:note>
        <skos:prefLabel xml:lang="en">activity method realization</skos:prefLabel>
    </owl:Class>
    


    <!-- http://standards.iso.org/iso/10303/tech/refdata/core#cb07be10-130a-0135-b552-598f1b1392ae -->

    <owl:Class rdf:about="http://standards.iso.org/iso/10303/tech/refdata/core#cb07be10-130a-0135-b552-598f1b1392ae">
        <rdfs:subClassOf rdf:resource="http://standards.iso.org/iso/10303/tech/refdata/core#STEPThing"/>
        <dc:contributor>STEP Harmonization Team</dc:contributor>
        <dc:creator>Phil Spiby, Eurostep</dc:creator>
        <dc:date>2022-09-01</dc:date>
        <dc:source>ISO/TS 10303-4000</dc:source>
        <dc:type>InWork</dc:type>
        <rdfs:comment xml:lang="en">A RetentionPeriod is the definition of a period of time that product data needs to be maintained due to organizational policy or legal requirements.</rdfs:comment>
        <owl:versionInfo>1</owl:versionInfo>
        <skos:changeNote>[2021-07-30] Initial definition.</skos:changeNote>
        <skos:prefLabel xml:lang="en">retention period</skos:prefLabel>
    </owl:Class>
    


    <!-- http://standards.iso.org/iso/10303/tech/refdata/core#cb75029e-938c-44ba-ba59-d96f4ebd1a0a -->

    <owl:Class rdf:about="http://standards.iso.org/iso/10303/tech/refdata/core#cb75029e-938c-44ba-ba59-d96f4ebd1a0a">
        <rdfs:subClassOf rdf:resource="http://standards.iso.org/iso/10303/tech/refdata/core#9d7f5922-5a61-4d2b-a73f-e4a27e70b2ce"/>
        <dc:contributor>STEP Harmonization Team</dc:contributor>
        <dc:creator>Phil Spiby, Eurostep</dc:creator>
        <dc:date>2022-09-01</dc:date>
        <dc:source>ISO/TS 10303-4000</dc:source>
        <dc:type>InWork</dc:type>
        <rdfs:comment xml:lang="en">A SequencingRelationship is a specialization of SchemeEntryRelationship. It defines a specific type of sequencing and relative timing for two SchemeEntry objects.</rdfs:comment>
        <owl:versionInfo>1</owl:versionInfo>
        <skos:changeNote>[2022-09-01] Initial definition.</skos:changeNote>
        <skos:example xml:lang="en">Specific types of sequencing could include start-start or finish-start.</skos:example>
        <skos:prefLabel xml:lang="en">sequencing relationship</skos:prefLabel>
    </owl:Class>
    


    <!-- http://standards.iso.org/iso/10303/tech/refdata/core#cb9ecdf0-130a-0135-b552-598f1b1392ae -->

    <owl:Class rdf:about="http://standards.iso.org/iso/10303/tech/refdata/core#cb9ecdf0-130a-0135-b552-598f1b1392ae">
        <rdfs:subClassOf rdf:resource="http://standards.iso.org/iso/10303/tech/refdata/core#STEPThing"/>
        <dc:contributor>STEP Harmonization Team</dc:contributor>
        <dc:creator>Phil Spiby, Eurostep</dc:creator>
        <dc:date>2022-09-01</dc:date>
        <dc:source>ISO/TS 10303-4000</dc:source>
        <dc:type>InWork</dc:type>
        <rdfs:comment xml:lang="en">A SecurityClassification is the level of confidentiality that is required in order to protect product data against unauthorized usage.</rdfs:comment>
        <owl:versionInfo>1</owl:versionInfo>
        <skos:changeNote>[2021-07-30] Initial definition.</skos:changeNote>
        <skos:prefLabel xml:lang="en">security classification</skos:prefLabel>
    </owl:Class>
    


    <!-- http://standards.iso.org/iso/10303/tech/refdata/core#cbb3ea8a-dd04-4e2b-b66e-1e1ddc87f69b -->

    <owl:Class rdf:about="http://standards.iso.org/iso/10303/tech/refdata/core#cbb3ea8a-dd04-4e2b-b66e-1e1ddc87f69b">
        <rdfs:subClassOf rdf:resource="http://standards.iso.org/iso/10303/tech/refdata/core#STEPThing"/>
        <dc:contributor>STEP Harmonization Team</dc:contributor>
        <dc:creator>Phil Spiby, Eurostep</dc:creator>
        <dc:date>2022-09-01</dc:date>
        <dc:source>ISO/TS 10303-4000</dc:source>
        <dc:type>InWork</dc:type>
        <rdfs:comment xml:lang="en">An InterfaceConnectorView identifies a view of an InterfaceConnectorVersion.</rdfs:comment>
        <owl:versionInfo>1</owl:versionInfo>
        <skos:changeNote>[2021-07-30] Initial definition.</skos:changeNote>
        <skos:example xml:lang="en">A reliability engineer assesses the likely failure modes of design version 3.8 for the connector between a brake unit and the hydraulic control system. The engineer generates a set of data that is a specific view of the connector. An instance of the InterfaceConnectorView entity data type collects these data together.</skos:example>
        <skos:prefLabel xml:lang="en">interface connector view</skos:prefLabel>
    </owl:Class>
    


    <!-- http://standards.iso.org/iso/10303/tech/refdata/core#cbe99290-130a-0135-b552-598f1b1392ae -->

    <owl:Class rdf:about="http://standards.iso.org/iso/10303/tech/refdata/core#cbe99290-130a-0135-b552-598f1b1392ae">
        <rdfs:subClassOf rdf:resource="http://standards.iso.org/iso/10303/tech/refdata/core#1cfca290-3279-0135-b58f-598f1b1392ae"/>
        <dc:contributor>STEP Harmonization Team</dc:contributor>
        <dc:creator>Phil Spiby, Eurostep</dc:creator>
        <dc:date>2022-09-01</dc:date>
        <dc:source>ISO/TS 10303-4000</dc:source>
        <dc:type>InWork</dc:type>
        <rdfs:comment xml:lang="en">A SecurityClassificationAssignment is an assignment of a SecurityClassification to an item (specified by SecurityClassificationAssignmentSelect). The meaning of the assignment can be specified using the ClassifiedAs attribute inherited from the AssignmentObject.</rdfs:comment>
        <owl:versionInfo>2</owl:versionInfo>
        <skos:changeNote>[2021-07-30] Initial definition.</skos:changeNote>
        <skos:changeNote>[2022-09-01] Phil Spiby, Eurostep: updated comment.</skos:changeNote>
        <skos:prefLabel xml:lang="en">security classification assignment</skos:prefLabel>
    </owl:Class>
    


    <!-- http://standards.iso.org/iso/10303/tech/refdata/core#cbed6b1b-7237-4766-8d68-8fad206bf336 -->

    <owl:Class rdf:about="http://standards.iso.org/iso/10303/tech/refdata/core#cbed6b1b-7237-4766-8d68-8fad206bf336">
        <rdfs:subClassOf rdf:resource="http://standards.iso.org/iso/10303/tech/refdata/core#f8816baf-d66a-42f9-bdcc-38e946c9a2fa"/>
        <dc:contributor>STEP Harmonization Team</dc:contributor>
        <dc:creator>Jean Brangé, AFNeT Services</dc:creator>
        <dc:date>2023-10-04</dc:date>
        <dc:source>ISO/TS 10303-4000</dc:source>
        <dc:type>InWork</dc:type>
        <rdfs:comment xml:lang="en">A ParallelOffset is a type of DerivedShapeElement that is located at a constant distance from a related element. If the basis is two dimensional, then all associated ShapeElements (the parallel offset and the basis shape aspect) lie in some common plane. If the basis is a surface, then all ShapeElements are embedded in three-dimensional space. The ParallelOffset is formed by the offset of each point of the basis, in a direction perpendicular to the basis by the offset distance.</rdfs:comment>
        <owl:versionInfo>3</owl:versionInfo>
        <skos:changeNote>[2023-10-04] Jean Brangé, AFNeT Services: Initial definition.</skos:changeNote>
        <skos:prefLabel xml:lang="en">parallel offset</skos:prefLabel>
    </owl:Class>
    


    <!-- http://standards.iso.org/iso/10303/tech/refdata/core#cc683870-130a-0135-b552-598f1b1392ae -->

    <owl:Class rdf:about="http://standards.iso.org/iso/10303/tech/refdata/core#cc683870-130a-0135-b552-598f1b1392ae">
        <rdfs:subClassOf rdf:resource="http://standards.iso.org/iso/10303/tech/refdata/core#99130bd0-130a-0135-b552-598f1b1392ae"/>
        <dc:contributor>STEP Harmonization Team</dc:contributor>
        <dc:creator>Phil Spiby, Eurostep</dc:creator>
        <dc:date>2022-09-01</dc:date>
        <dc:source>ISO/TS 10303-4000</dc:source>
        <dc:type>InWork</dc:type>
        <rdfs:comment xml:lang="en">A SerialEffectivity is a type of Effectivity for which the domain of applicability is defined as a possibly open-ended interval of serial numbers. A &apos;start&apos; value shall always be specified for SerialEffectivity, an &apos;end&apos; value can be specified.</rdfs:comment>
        <owl:versionInfo>2</owl:versionInfo>
        <skos:changeNote>[2021-07-30] Initial definition.</skos:changeNote>
        <skos:changeNote>[2022-09-01] Phil Spiby, Eurostep: updated comment.</skos:changeNote>
        <skos:prefLabel xml:lang="en">serial effectivity</skos:prefLabel>
    </owl:Class>
    


    <!-- http://standards.iso.org/iso/10303/tech/refdata/core#cc884390-130a-0135-b552-598f1b1392ae -->

    <owl:Class rdf:about="http://standards.iso.org/iso/10303/tech/refdata/core#cc884390-130a-0135-b552-598f1b1392ae">
        <rdfs:subClassOf rdf:resource="http://standards.iso.org/iso/10303/tech/refdata/core#STEPThing"/>
        <dc:contributor>STEP Harmonization Team</dc:contributor>
        <dc:creator>Phil Spiby, Eurostep</dc:creator>
        <dc:date>2022-09-01</dc:date>
        <dc:source>ISO/TS 10303-4000</dc:source>
        <dc:type>InWork</dc:type>
        <rdfs:comment xml:lang="en">A SetMembership is a relationship that is between a set and an item that indicates the item is a member of the set.</rdfs:comment>
        <owl:versionInfo>2</owl:versionInfo>
        <skos:changeNote>[2021-07-30] Initial definition.</skos:changeNote>
        <skos:changeNote>[2022-09-01] Phil Spiby, Eurostep: updated comment.</skos:changeNote>
        <skos:prefLabel xml:lang="en">set membership</skos:prefLabel>
    </owl:Class>
    


    <!-- http://standards.iso.org/iso/10303/tech/refdata/core#cca6c810-130a-0135-b552-598f1b1392ae -->

    <owl:Class rdf:about="http://standards.iso.org/iso/10303/tech/refdata/core#cca6c810-130a-0135-b552-598f1b1392ae">
        <rdfs:subClassOf rdf:resource="http://standards.iso.org/iso/10303/tech/refdata/core#STEPThing"/>
        <dc:contributor>STEP Harmonization Team</dc:contributor>
        <dc:creator>Jean Brangé, AFNeT Services</dc:creator>
        <dc:date>2023-10-04</dc:date>
        <dc:source>ISO/TS 10303-4000</dc:source>
        <dc:type>InWork</dc:type>
        <rdfs:comment xml:lang="en">A ShapeDependentProperty is a characteristic of the shape, or of a portion of the shape of an object. This object is either a Part, an occurrence of a Part in the product structure or the physical realization of a Part.</rdfs:comment>
        <owl:versionInfo>3</owl:versionInfo>
        <skos:changeNote>[2023-10-04] Jean Brangé, AFNeT Services: Initial definition.</skos:changeNote>
        <skos:note xml:lang="en">A ShapeDependentProperty is independent of the representations of the shape.</skos:note>
        <skos:prefLabel xml:lang="en">shape dependent property</skos:prefLabel>
    </owl:Class>
    


    <!-- http://standards.iso.org/iso/10303/tech/refdata/core#ce9ec1d2-b535-4a49-bd93-67a52b8d5dc4 -->

    <owl:Class rdf:about="http://standards.iso.org/iso/10303/tech/refdata/core#ce9ec1d2-b535-4a49-bd93-67a52b8d5dc4">
        <rdfs:subClassOf rdf:resource="http://standards.iso.org/iso/10303/tech/refdata/core#STEPThing"/>
        <dc:contributor>STEP Harmonization Team</dc:contributor>
        <dc:creator>Phil Spiby, Eurostep</dc:creator>
        <dc:date>2022-09-01</dc:date>
        <dc:source>ISO/TS 10303-4000</dc:source>
        <dc:type>InWork</dc:type>
        <rdfs:comment xml:lang="en">A Risk is the potential for realization of unwanted negative consequences of an event.</rdfs:comment>
        <owl:versionInfo>1</owl:versionInfo>
        <skos:changeNote>[2022-09-01] Initial definition.</skos:changeNote>
        <skos:example xml:lang="en">&apos;Line shutdown&apos; is an example of Risk in the context of a manufacturing system&apos;s reliability.</skos:example>
        <skos:example xml:lang="en">&apos;Privacy risk&apos; and &apos;security risk&apos; are examples of Risk for the telecommunications industry.</skos:example>
        <skos:example xml:lang="en">&apos;Transportation jam-up&apos;, &apos;customer anger&apos;, &apos;collateral damage&apos;, and &apos;greater susceptibility to interruption of supply during crises&apos; are all examples of Risk.</skos:example>
        <skos:example xml:lang="en">Timing such as &apos;premature rejection&apos; and &apos;premature commitment&apos; are other examples of Risk.</skos:example>
        <skos:note xml:lang="en">A risk can also have a possible positive outcome. In such cases it is often referred to as an opportunity or reward.</skos:note>
        <skos:note xml:lang="en">ISO Guide 73:2009 defines &quot;risk&quot; as the effect of uncertainty on objectives.</skos:note>
        <skos:note xml:lang="en">ISO/IEC Guide 51:2014 defines risk as the combination of the probability of occurrence of harm and the severity of that harm.</skos:note>
        <skos:note xml:lang="en">In the safety field, risk management is focused on prevention and mitigation of harm.</skos:note>
        <skos:prefLabel xml:lang="en">risk</skos:prefLabel>
    </owl:Class>
    


    <!-- http://standards.iso.org/iso/10303/tech/refdata/core#cea900b0-130a-0135-b552-598f1b1392ae -->

    <owl:Class rdf:about="http://standards.iso.org/iso/10303/tech/refdata/core#cea900b0-130a-0135-b552-598f1b1392ae">
        <rdfs:subClassOf rdf:resource="http://standards.iso.org/iso/10303/tech/refdata/core#94453010-130a-0135-b552-598f1b1392ae"/>
        <dc:contributor>STEP Harmonization Team</dc:contributor>
        <dc:creator>Phil Spiby, Eurostep</dc:creator>
        <dc:date>2022-09-01</dc:date>
        <dc:source>ISO/TS 10303-4000</dc:source>
        <dc:type>InWork</dc:type>
        <rdfs:comment xml:lang="en">A SingleOccurrence is a subtype of DefinitionBasedOccurrence. It is one specific occurrence of an object that uses an item (specified by OccurrenceDefinitionSelect) as its definition. A SingleOccurrence is a type of Occurrence.</rdfs:comment>
        <owl:versionInfo>2</owl:versionInfo>
        <skos:changeNote>[2021-07-30] Initial definition.</skos:changeNote>
        <skos:changeNote>[2022-09-01] Phil Spiby, Eurostep: updated comment updated example updated note.</skos:changeNote>
        <skos:example xml:lang="en">In a TechnicalSolution for the &apos;front left brake&apos;, a &apos;brake disk&apos; is used and its position is specified by a geometric Transformation.</skos:example>
        <skos:note xml:lang="en">A SingleOccurrence can or cannot be associated with placement information using an OccurrencePlacement.</skos:note>
        <skos:prefLabel xml:lang="en">single occurrence</skos:prefLabel>
    </owl:Class>
    


    <!-- http://standards.iso.org/iso/10303/tech/refdata/core#ceb138fc-fefc-4b1c-adcc-a7b54167744c -->

    <owl:Class rdf:about="http://standards.iso.org/iso/10303/tech/refdata/core#ceb138fc-fefc-4b1c-adcc-a7b54167744c">
        <rdfs:subClassOf rdf:resource="http://standards.iso.org/iso/10303/tech/refdata/core#STEPThing"/>
        <dc:contributor>STEP Harmonization Team</dc:contributor>
        <dc:creator>Phil Spiby, Eurostep</dc:creator>
        <dc:date>2022-09-01</dc:date>
        <dc:source>ISO/TS 10303-4000</dc:source>
        <dc:type>InWork</dc:type>
        <rdfs:comment xml:lang="en">An Environment is an abstract object where specialization allow to identify the definition of typical environment or to represents a record of observations about the environment.</rdfs:comment>
        <owl:versionInfo>1</owl:versionInfo>
        <skos:changeNote>[2021-07-30] Initial definition.</skos:changeNote>
        <skos:prefLabel xml:lang="en">environment</skos:prefLabel>
    </owl:Class>
    


    <!-- http://standards.iso.org/iso/10303/tech/refdata/core#ceec2430-130a-0135-b552-598f1b1392ae -->

    <owl:Class rdf:about="http://standards.iso.org/iso/10303/tech/refdata/core#ceec2430-130a-0135-b552-598f1b1392ae">
        <rdfs:subClassOf rdf:resource="http://standards.iso.org/iso/10303/tech/refdata/core#STEPThing"/>
        <dc:contributor>STEP Harmonization Team</dc:contributor>
        <dc:creator>Phil Spiby, Eurostep</dc:creator>
        <dc:date>2022-09-01</dc:date>
        <dc:source>ISO/TS 10303-4000</dc:source>
        <dc:type>InWork</dc:type>
        <rdfs:comment xml:lang="en">A Specification is a characteristic of a product. A Specification discriminates one product from other members of the same ProductClass. A Specification refers to a SpecificationCategory that completes the semantics of the Specification.</rdfs:comment>
        <owl:versionInfo>2</owl:versionInfo>
        <skos:changeNote>[2021-07-30] Initial definition.</skos:changeNote>
        <skos:changeNote>[2022-09-01] Phil Spiby, Eurostep: updated example updated note.</skos:changeNote>
        <skos:example xml:lang="en">&apos;coupe&apos;, &apos;hatch back&apos;, or &apos;sedan&apos; are examples for specifications belonging to the SpecificationCategory of type &apos;car body&apos;. &apos;radio 1 with CD player&apos; and &apos;radio 2 without CD player&apos; are examples for specifications belonging to the SpecificationCategory of type &apos;radio equipment&apos;. &apos;disk brake&apos; and &apos;drum brake&apos; are examples for specifications belonging to the SpecificationCategory of type &apos;braking system&apos;.</skos:example>
        <skos:note xml:lang="en">A Specification can be a characteristic of the members of more than one ProductClass using BreakdownVersionAssignment objects.</skos:note>
        <skos:note xml:lang="en">A Specification in combination with a ConditionalConfiguration can be used to define under which conditions a Part is used in combination with a ProductClass.</skos:note>
        <skos:prefLabel xml:lang="en">specification</skos:prefLabel>
    </owl:Class>
    


    <!-- http://standards.iso.org/iso/10303/tech/refdata/core#cf495d85-c86b-4f98-8e2d-0ac6039aecc4 -->

    <owl:Class rdf:about="http://standards.iso.org/iso/10303/tech/refdata/core#cf495d85-c86b-4f98-8e2d-0ac6039aecc4">
        <rdfs:subClassOf rdf:resource="http://standards.iso.org/iso/10303/tech/refdata/core#b44098a0-130a-0135-b552-598f1b1392ae"/>
        <dc:contributor>STEP Harmonization Team</dc:contributor>
        <dc:creator>Jean Brangé, AFNeT Services</dc:creator>
        <dc:date>2023-10-04</dc:date>
        <dc:source>ISO/TS 10303-4000</dc:source>
        <dc:type>InWork</dc:type>
        <rdfs:comment xml:lang="en">A ToolPartRelationship is a type of PartViewRelationship that is a relationship between two PartView objects. It establishes a relationship between a part (Related) and a tool (Relating) that is used to produce the part.</rdfs:comment>
        <owl:versionInfo>3</owl:versionInfo>
        <skos:changeNote>[2023-10-04] Jean Brangé, AFNeT Services: Initial definition.</skos:changeNote>
        <skos:example xml:lang="en">This relationship is, by default, valid only in the application contexts that are relevant for both related PartView objects.</skos:example>
        <skos:prefLabel xml:lang="en">tool part relationship</skos:prefLabel>
    </owl:Class>
    


    <!-- http://standards.iso.org/iso/10303/tech/refdata/core#cf6f5df0-130a-0135-b552-598f1b1392ae -->

    <owl:Class rdf:about="http://standards.iso.org/iso/10303/tech/refdata/core#cf6f5df0-130a-0135-b552-598f1b1392ae">
        <rdfs:subClassOf rdf:resource="http://standards.iso.org/iso/10303/tech/refdata/core#1cfca290-3279-0135-b58f-598f1b1392ae"/>
        <dc:contributor>STEP Harmonization Team</dc:contributor>
        <dc:creator>Phil Spiby, Eurostep</dc:creator>
        <dc:date>2022-09-01</dc:date>
        <dc:source>ISO/TS 10303-4000</dc:source>
        <dc:type>InWork</dc:type>
        <rdfs:comment xml:lang="en">A SpecificationAssignment is an assignment of a Specification to a ProductClass. The meaning of this association is specified further by the attribute AssociationType.</rdfs:comment>
        <owl:versionInfo>1</owl:versionInfo>
        <skos:changeNote>[2021-07-30] Initial definition.</skos:changeNote>
        <skos:prefLabel xml:lang="en">specification assignment</skos:prefLabel>
    </owl:Class>
    


    <!-- http://standards.iso.org/iso/10303/tech/refdata/core#cf85b47a-9e1e-45d7-b1ec-b209c2019468 -->

    <owl:Class rdf:about="http://standards.iso.org/iso/10303/tech/refdata/core#cf85b47a-9e1e-45d7-b1ec-b209c2019468">
        <rdfs:subClassOf rdf:resource="http://standards.iso.org/iso/10303/tech/refdata/core#83b2a250-130a-0135-b552-598f1b1392ae"/>
        <dc:contributor>STEP Harmonization Team</dc:contributor>
        <dc:creator>Phil Spiby, Eurostep</dc:creator>
        <dc:date>2022-09-01</dc:date>
        <dc:source>ISO/TS 10303-4000</dc:source>
        <dc:type>InWork</dc:type>
        <rdfs:comment xml:lang="en">A TaskMethodAssignment is a specialization of an AssignmentObject that represents an assignment of a TaskMethod to an item (specified by TaskAssignmentSelect). The meaning of the assignment can be specified using the ClassifiedAs attribute inherited from the AssignmentObject.</rdfs:comment>
        <owl:versionInfo>2</owl:versionInfo>
        <skos:changeNote>[2021-07-30] Initial definition.</skos:changeNote>
        <skos:changeNote>[2022-09-01] Phil Spiby, Eurostep: updated comment updated note.</skos:changeNote>
        <skos:prefLabel xml:lang="en">task method assignment</skos:prefLabel>
    </owl:Class>
    


    <!-- http://standards.iso.org/iso/10303/tech/refdata/core#cf96c7f3-c3f6-4f8f-a640-eb05f182e1d6 -->

    <owl:Class rdf:about="http://standards.iso.org/iso/10303/tech/refdata/core#cf96c7f3-c3f6-4f8f-a640-eb05f182e1d6">
        <rdfs:subClassOf rdf:resource="http://standards.iso.org/iso/10303/tech/refdata/core#95f1bde5-b263-4ca1-89df-33e1205800dd"/>
        <dc:contributor>STEP Harmonization Team</dc:contributor>
        <dc:creator>Phil Spiby, Eurostep</dc:creator>
        <dc:date>2022-09-01</dc:date>
        <dc:source>ISO/TS 10303-4000</dc:source>
        <dc:type>InWork</dc:type>
        <rdfs:comment xml:lang="en">A TaskStep is a specialization of TaskElement that is not further sub-divided.</rdfs:comment>
        <owl:versionInfo>1</owl:versionInfo>
        <skos:changeNote>[2021-07-30] Initial definition.</skos:changeNote>
        <skos:prefLabel xml:lang="en">task step</skos:prefLabel>
    </owl:Class>
    


    <!-- http://standards.iso.org/iso/10303/tech/refdata/core#cfa9fe8e-2654-4165-b9a0-f85fa5aeb597 -->

    <owl:Class rdf:about="http://standards.iso.org/iso/10303/tech/refdata/core#cfa9fe8e-2654-4165-b9a0-f85fa5aeb597">
        <rdfs:subClassOf rdf:resource="http://standards.iso.org/iso/10303/tech/refdata/core#ceb138fc-fefc-4b1c-adcc-a7b54167744c"/>
        <dc:contributor>STEP Harmonization Team</dc:contributor>
        <dc:creator>Phil Spiby, Eurostep</dc:creator>
        <dc:date>2022-09-01</dc:date>
        <dc:source>ISO/TS 10303-4000</dc:source>
        <dc:type>InWork</dc:type>
        <rdfs:comment xml:lang="en">An EnvironmentDefinition is a specialization of Environment that is used to identify the definition of typical environment in which a product is to be, has been or is planned to be deployed in, operated in, or supported in.</rdfs:comment>
        <owl:versionInfo>1</owl:versionInfo>
        <skos:changeNote>[2021-07-30] Initial definition.</skos:changeNote>
        <skos:prefLabel xml:lang="en">environment definition</skos:prefLabel>
    </owl:Class>
    


    <!-- http://standards.iso.org/iso/10303/tech/refdata/core#cfe04830-130a-0135-b552-598f1b1392ae -->

    <owl:Class rdf:about="http://standards.iso.org/iso/10303/tech/refdata/core#cfe04830-130a-0135-b552-598f1b1392ae">
        <rdfs:subClassOf rdf:resource="http://standards.iso.org/iso/10303/tech/refdata/core#STEPThing"/>
        <dc:contributor>STEP Harmonization Team</dc:contributor>
        <dc:creator>Phil Spiby, Eurostep</dc:creator>
        <dc:date>2022-09-01</dc:date>
        <dc:source>ISO/TS 10303-4000</dc:source>
        <dc:type>InWork</dc:type>
        <rdfs:comment xml:lang="en">A SpecificationCategory is a definition of a set of Specification objects serving the same purpose.</rdfs:comment>
        <owl:versionInfo>2</owl:versionInfo>
        <skos:changeNote>[2021-07-30] Initial definition.</skos:changeNote>
        <skos:changeNote>[2022-09-01] Phil Spiby, Eurostep: updated example.</skos:changeNote>
        <skos:example xml:lang="en">The category &apos;kind of drive&apos; for the Specification objects &apos;front wheel drive&apos; and &apos;rear wheel drive&apos; or the category &apos;level of equipment&apos; for the Specification objects &apos;standard&apos;, &apos;comfortable&apos;, and &apos;luxurious&apos; are examples for SpecificationCategory objects.</skos:example>
        <skos:prefLabel xml:lang="en">specification category</skos:prefLabel>
    </owl:Class>
    


    <!-- http://standards.iso.org/iso/10303/tech/refdata/core#d038c870-130a-0135-b552-598f1b1392ae -->

    <owl:Class rdf:about="http://standards.iso.org/iso/10303/tech/refdata/core#d038c870-130a-0135-b552-598f1b1392ae">
        <rdfs:subClassOf rdf:resource="http://standards.iso.org/iso/10303/tech/refdata/core#1cfca290-3279-0135-b58f-598f1b1392ae"/>
        <dc:contributor>STEP Harmonization Team</dc:contributor>
        <dc:creator>Phil Spiby, Eurostep</dc:creator>
        <dc:date>2022-09-01</dc:date>
        <dc:source>ISO/TS 10303-4000</dc:source>
        <dc:type>InWork</dc:type>
        <rdfs:comment xml:lang="en">A SpecificationCategoryAssignment is an assignment of a SpecificationCategory to a ProductClass. Additionally, this assignment specifies if the usage of one or more Specification objects belonging to this SpecificationCategory, is mandatory or optional for all products of that ProductClass. The meaning of the assignment can be specified using the ClassifiedAs attribute inherited from the AssignmentObject.</rdfs:comment>
        <owl:versionInfo>2</owl:versionInfo>
        <skos:changeNote>[2021-07-30] Initial definition.</skos:changeNote>
        <skos:changeNote>[2022-09-01] Phil Spiby, Eurostep: updated comment.</skos:changeNote>
        <skos:note xml:lang="en">The assignment of a SpecificationCategory to a ProductClass does not replace the association of single members of the SpecificationCategory to the ProductClass.</skos:note>
        <skos:prefLabel xml:lang="en">specification category assignment</skos:prefLabel>
    </owl:Class>
    


    <!-- http://standards.iso.org/iso/10303/tech/refdata/core#d0937706-0e0f-432f-a27f-95014e660652 -->

    <owl:Class rdf:about="http://standards.iso.org/iso/10303/tech/refdata/core#d0937706-0e0f-432f-a27f-95014e660652">
        <rdfs:subClassOf rdf:resource="http://standards.iso.org/iso/10303/tech/refdata/core#5952bf98-2ea0-46c9-8915-249fe039b206"/>
        <dc:contributor>STEP Harmonization Team</dc:contributor>
        <dc:creator>Phil Spiby, Eurostep</dc:creator>
        <dc:date>2022-09-01</dc:date>
        <dc:source>ISO/TS 10303-4000</dc:source>
        <dc:type>InWork</dc:type>
        <rdfs:comment xml:lang="en">A RiskPerception is a specialization of RiskView that defines values or concerns (a risk level) with which a stakeholder views a particular Risk. The risk level is represented by a set of property values referenced from RiskLevel. If more than one property value is provided each property value shall be equivalent.</rdfs:comment>
        <owl:versionInfo>1</owl:versionInfo>
        <skos:changeNote>[2022-09-01] Initial definition.</skos:changeNote>
        <skos:example xml:lang="en">One riskLevelRepresentation could be 4 (from a maximum of 5) and a second could be&quot;high&quot;.</skos:example>
        <skos:example xml:lang="en">The definition attribute of the RiskLevel could refer to a PropertyDefinition with a PropertyType attribute set to the RD individual &quot;risk level&quot;.</skos:example>
        <skos:note xml:lang="en">Risk will be perceived differently in different contexts, such as in the context of human safety, mission success, project time schedule, performance or economy.</skos:note>
        <skos:note xml:lang="en">RiskPerception can be used qualitatively or quantitatively to form a risk matrix.</skos:note>
        <skos:note xml:lang="en">RiskPerception can differ from objective data.</skos:note>
        <skos:note xml:lang="en">RiskPerception depends on the stake holder&apos;s expressed needs, issues, and knowledge.</skos:note>
        <skos:prefLabel xml:lang="en">risk perception</skos:prefLabel>
    </owl:Class>
    


    <!-- http://standards.iso.org/iso/10303/tech/refdata/core#d0a51ed0-130a-0135-b552-598f1b1392ae -->

    <owl:Class rdf:about="http://standards.iso.org/iso/10303/tech/refdata/core#d0a51ed0-130a-0135-b552-598f1b1392ae">
        <rdfs:subClassOf rdf:resource="http://standards.iso.org/iso/10303/tech/refdata/core#STEPThing"/>
        <dc:contributor>STEP Harmonization Team</dc:contributor>
        <dc:creator>Phil Spiby, Eurostep</dc:creator>
        <dc:date>2022-09-01</dc:date>
        <dc:source>ISO/TS 10303-4000</dc:source>
        <dc:type>InWork</dc:type>
        <rdfs:comment xml:lang="en">A SpecificationCategoryHierarchy is used to build up hierarchical structures of SpecificationCategory objects.</rdfs:comment>
        <owl:versionInfo>1</owl:versionInfo>
        <skos:changeNote>[2021-07-30] Initial definition.</skos:changeNote>
        <skos:prefLabel xml:lang="en">specification category hierarchy</skos:prefLabel>
    </owl:Class>
    


    <!-- http://standards.iso.org/iso/10303/tech/refdata/core#d0cd8f0f-07c9-4a4d-9aec-bc0ccc1d901d -->

    <owl:Class rdf:about="http://standards.iso.org/iso/10303/tech/refdata/core#d0cd8f0f-07c9-4a4d-9aec-bc0ccc1d901d">
        <rdfs:subClassOf rdf:resource="http://standards.iso.org/iso/10303/tech/refdata/core#02761765-5f96-4ed2-a51c-38aaa796367d"/>
        <dc:contributor>STEP Harmonization Team</dc:contributor>
        <dc:creator>Jean Brangé, AFNeT Services</dc:creator>
        <dc:date>2023-10-04</dc:date>
        <dc:source>ISO/TS 10303-4000</dc:source>
        <dc:type>InWork</dc:type>
        <rdfs:comment xml:lang="en">A ContinuousShapeElement is a type of CompositeShapeElement where the geometric elements associated with the underlying ShapeElement members are touching and thus establish a continuous region.</rdfs:comment>
        <owl:versionInfo>3</owl:versionInfo>
        <skos:changeNote>[2023-10-04] Jean Brangé, AFNeT Services: Initial definition.</skos:changeNote>
        <skos:prefLabel xml:lang="en">continuous shape element</skos:prefLabel>
    </owl:Class>
    


    <!-- http://standards.iso.org/iso/10303/tech/refdata/core#d0da86b0-130a-0135-b552-598f1b1392ae -->

    <owl:Class rdf:about="http://standards.iso.org/iso/10303/tech/refdata/core#d0da86b0-130a-0135-b552-598f1b1392ae">
        <rdfs:subClassOf rdf:resource="http://standards.iso.org/iso/10303/tech/refdata/core#1cfca290-3279-0135-b58f-598f1b1392ae"/>
        <dc:contributor>STEP Harmonization Team</dc:contributor>
        <dc:creator>Phil Spiby, Eurostep</dc:creator>
        <dc:date>2022-09-01</dc:date>
        <dc:source>ISO/TS 10303-4000</dc:source>
        <dc:type>InWork</dc:type>
        <rdfs:comment xml:lang="en">A SpecificationConditionAssignment is an assignment of a Condition to a ProductClass. The meaning of this association is specified further by the attribute ConditionType.</rdfs:comment>
        <owl:versionInfo>1</owl:versionInfo>
        <skos:changeNote>[2021-07-30] Initial definition.</skos:changeNote>
        <skos:prefLabel xml:lang="en">specification condition assignment</skos:prefLabel>
    </owl:Class>
    


    <!-- http://standards.iso.org/iso/10303/tech/refdata/core#d14e7e30-130a-0135-b552-598f1b1392ae -->

    <owl:Class rdf:about="http://standards.iso.org/iso/10303/tech/refdata/core#d14e7e30-130a-0135-b552-598f1b1392ae">
        <rdfs:subClassOf rdf:resource="http://standards.iso.org/iso/10303/tech/refdata/core#STEPThing"/>
        <dc:contributor>STEP Harmonization Team</dc:contributor>
        <dc:creator>Phil Spiby, Eurostep</dc:creator>
        <dc:date>2022-09-01</dc:date>
        <dc:source>ISO/TS 10303-4000</dc:source>
        <dc:type>InWork</dc:type>
        <rdfs:comment xml:lang="en">A SpecificationInclusion is a representation of the statement that specifies that the conformance to an item (IfCondition, specified by ConditionParameterSelect) implies the conformance to an additional item (IncludedSpecification, specified by ConditionParameterSelect).</rdfs:comment>
        <owl:versionInfo>2</owl:versionInfo>
        <skos:changeNote>[2021-07-30] Initial definition.</skos:changeNote>
        <skos:changeNote>[2022-09-01] Phil Spiby, Eurostep: updated comment updated example updated note.</skos:changeNote>
        <skos:example xml:lang="en">The source of such a completion can be a customer order.</skos:example>
        <skos:prefLabel xml:lang="en">specification inclusion</skos:prefLabel>
    </owl:Class>
    


    <!-- http://standards.iso.org/iso/10303/tech/refdata/core#d1796b3a-5ade-4d7a-b9e0-4af28a9cfddb -->

    <owl:Class rdf:about="http://standards.iso.org/iso/10303/tech/refdata/core#d1796b3a-5ade-4d7a-b9e0-4af28a9cfddb">
        <rdfs:subClassOf rdf:resource="http://standards.iso.org/iso/10303/tech/refdata/core#59b11220-3279-0135-b58f-598f1b1392ae"/>
        <dc:contributor>STEP Harmonization Team</dc:contributor>
        <dc:creator>Jean Brangé, AFNeT Services</dc:creator>
        <dc:date>2023-10-04</dc:date>
        <dc:source>ISO/TS 10303-4000</dc:source>
        <dc:type>InWork</dc:type>
        <rdfs:comment xml:lang="en">A ShapeElementRelationship is an association between two ShapeElement objects.</rdfs:comment>
        <owl:versionInfo>3</owl:versionInfo>
        <skos:changeNote>[2023-10-04] Jean Brangé, AFNeT Services: Initial definition.</skos:changeNote>
        <skos:prefLabel xml:lang="en">shape element relationship</skos:prefLabel>
    </owl:Class>
    


    <!-- http://standards.iso.org/iso/10303/tech/refdata/core#d1ad18f0-130a-0135-b552-598f1b1392ae -->

    <owl:Class rdf:about="http://standards.iso.org/iso/10303/tech/refdata/core#d1ad18f0-130a-0135-b552-598f1b1392ae">
        <rdfs:subClassOf rdf:resource="http://standards.iso.org/iso/10303/tech/refdata/core#1cfca290-3279-0135-b58f-598f1b1392ae"/>
        <dc:contributor>STEP Harmonization Team</dc:contributor>
        <dc:creator>Phil Spiby, Eurostep</dc:creator>
        <dc:date>2022-09-01</dc:date>
        <dc:source>ISO/TS 10303-4000</dc:source>
        <dc:type>InWork</dc:type>
        <rdfs:comment xml:lang="en">A SpecificationInclusionAssignment is an assignment of a SpecificationInclusion to a ProductClass. This assignment contains the information that a specific SpecificationInclusion applies for all products of that ProductClass. The meaning of the assignment can be specified using the ClassifiedAs attribute inherited from the AssignmentObject.</rdfs:comment>
        <owl:versionInfo>2</owl:versionInfo>
        <skos:changeNote>[2021-07-30] Initial definition.</skos:changeNote>
        <skos:changeNote>[2022-09-01] Phil Spiby, Eurostep: updated comment.</skos:changeNote>
        <skos:prefLabel xml:lang="en">specification inclusion assignment</skos:prefLabel>
    </owl:Class>
    


    <!-- http://standards.iso.org/iso/10303/tech/refdata/core#d214db70-130a-0135-b552-598f1b1392ae -->

    <owl:Class rdf:about="http://standards.iso.org/iso/10303/tech/refdata/core#d214db70-130a-0135-b552-598f1b1392ae">
        <rdfs:subClassOf rdf:resource="http://standards.iso.org/iso/10303/tech/refdata/core#ae1e7780-130a-0135-b552-598f1b1392ae"/>
        <dc:contributor>STEP Harmonization Team</dc:contributor>
        <dc:creator>Phil Spiby, Eurostep</dc:creator>
        <dc:date>2022-09-01</dc:date>
        <dc:source>ISO/TS 10303-4000</dc:source>
        <dc:type>InWork</dc:type>
        <rdfs:comment xml:lang="en">A SpecifiedOccurrence is a mechanism to identify a certain Occurrence in a multi-level assembly structure that reuses partial decompositions. A SpecifiedOccurrence is a type of Occurrence.</rdfs:comment>
        <owl:versionInfo>2</owl:versionInfo>
        <skos:changeNote>[2021-07-30] Initial definition.</skos:changeNote>
        <skos:changeNote>[2022-09-01] Phil Spiby, Eurostep: updated example.</skos:changeNote>
        <skos:example xml:lang="en">A &apos;chassis&apos; consists among others of the sub-assemblies &apos;front axle&apos; and &apos;rear axle&apos;. Both axle assemblies consist, among others, of the &apos;left wheel&apos; and the &apos;right wheel&apos;. In order to identify the &apos;left wheel&apos; of the &apos;rear axle&apos;, the SpecifiedOccurrence object references &apos;left wheel&apos; as definition, and &apos;rear axle&apos; as upperUsage.</skos:example>
        <skos:prefLabel xml:lang="en">specified occurrence</skos:prefLabel>
    </owl:Class>
    


    <!-- http://standards.iso.org/iso/10303/tech/refdata/core#d237f3d0-130a-0135-b552-598f1b1392ae -->

    <owl:Class rdf:about="http://standards.iso.org/iso/10303/tech/refdata/core#d237f3d0-130a-0135-b552-598f1b1392ae">
        <rdfs:subClassOf rdf:resource="http://standards.iso.org/iso/10303/tech/refdata/core#d66b1630-130a-0135-b552-598f1b1392ae"/>
        <dc:contributor>STEP Harmonization Team</dc:contributor>
        <dc:creator>Phil Spiby, Eurostep</dc:creator>
        <dc:date>2022-09-01</dc:date>
        <dc:source>ISO/TS 10303-4000</dc:source>
        <dc:type>InWork</dc:type>
        <rdfs:comment xml:lang="en">A StandardUncertainty is a type of UncertaintyQualifier. A StandardUncertainty can be an ExpandedUncertainty. The uncertainty is defined in ISO/IEC Guide 98-3.</rdfs:comment>
        <owl:versionInfo>2</owl:versionInfo>
        <skos:changeNote>[2021-07-30] Initial definition.</skos:changeNote>
        <skos:changeNote>[2022-09-01] Phil Spiby, Eurostep: updated comment.</skos:changeNote>
        <skos:prefLabel xml:lang="en">standard uncertainty</skos:prefLabel>
    </owl:Class>
    


    <!-- http://standards.iso.org/iso/10303/tech/refdata/core#d2a75770-130a-0135-b552-598f1b1392ae -->

    <owl:Class rdf:about="http://standards.iso.org/iso/10303/tech/refdata/core#d2a75770-130a-0135-b552-598f1b1392ae">
        <rdfs:subClassOf rdf:resource="http://standards.iso.org/iso/10303/tech/refdata/core#c27698c0-130a-0135-b552-598f1b1392ae"/>
        <dc:contributor>STEP Harmonization Team</dc:contributor>
        <dc:creator>Phil Spiby, Eurostep</dc:creator>
        <dc:date>2022-09-01</dc:date>
        <dc:source>ISO/TS 10303-4000</dc:source>
        <dc:type>InWork</dc:type>
        <rdfs:comment xml:lang="en">A StringValue is a type of PropertyValue that represents a sequence of one or more alphanumeric characters.</rdfs:comment>
        <owl:versionInfo>1</owl:versionInfo>
        <skos:changeNote>[2021-07-30] Initial definition.</skos:changeNote>
        <skos:prefLabel xml:lang="en">string value</skos:prefLabel>
    </owl:Class>
    


    <!-- http://standards.iso.org/iso/10303/tech/refdata/core#d2bb2d90-130a-0135-b552-598f1b1392ae -->

    <owl:Class rdf:about="http://standards.iso.org/iso/10303/tech/refdata/core#d2bb2d90-130a-0135-b552-598f1b1392ae">
        <rdfs:subClassOf rdf:resource="http://standards.iso.org/iso/10303/tech/refdata/core#9fee6ad0-130a-0135-b552-598f1b1392ae"/>
        <dc:contributor>STEP Harmonization Team</dc:contributor>
        <dc:creator>Phil Spiby, Eurostep</dc:creator>
        <dc:date>2022-09-01</dc:date>
        <dc:source>ISO/TS 10303-4000</dc:source>
        <dc:type>InWork</dc:type>
        <rdfs:comment xml:lang="en">A StyledModel is a type of GeometricRepresentation that defines the stub for a set of styling or annotation elements for which visual characteristics are specified. The geometric or annotation elements are defined in a DigitalFile.</rdfs:comment>
        <owl:versionInfo>1</owl:versionInfo>
        <skos:changeNote>[2021-07-30] Initial definition.</skos:changeNote>
        <skos:prefLabel xml:lang="en">styled model</skos:prefLabel>
    </owl:Class>
    


    <!-- http://standards.iso.org/iso/10303/tech/refdata/core#d2e76db0-130a-0135-b552-598f1b1392ae -->

    <owl:Class rdf:about="http://standards.iso.org/iso/10303/tech/refdata/core#d2e76db0-130a-0135-b552-598f1b1392ae">
        <rdfs:subClassOf rdf:resource="http://standards.iso.org/iso/10303/tech/refdata/core#STEPThing"/>
        <dc:contributor>STEP Harmonization Team</dc:contributor>
        <dc:creator>Phil Spiby, Eurostep</dc:creator>
        <dc:date>2022-09-01</dc:date>
        <dc:source>ISO/TS 10303-4000</dc:source>
        <dc:type>InWork</dc:type>
        <rdfs:comment xml:lang="en">A SubsetMember is a relationship that is between set A and set B that indicates: each member of set A is also a member of set B.</rdfs:comment>
        <owl:versionInfo>2</owl:versionInfo>
        <skos:changeNote>[2021-07-30] Initial definition.</skos:changeNote>
        <skos:changeNote>[2022-09-01] Phil Spiby, Eurostep: updated comment updated note.</skos:changeNote>
        <skos:note xml:lang="en">Set A can be equal to set B.</skos:note>
        <skos:prefLabel xml:lang="en">subset member</skos:prefLabel>
    </owl:Class>
    


    <!-- http://standards.iso.org/iso/10303/tech/refdata/core#d2eb1f4f-b98f-4393-a7ed-24dc41900bd2 -->

    <owl:Class rdf:about="http://standards.iso.org/iso/10303/tech/refdata/core#d2eb1f4f-b98f-4393-a7ed-24dc41900bd2">
        <rdfs:subClassOf rdf:resource="http://standards.iso.org/iso/10303/tech/refdata/core#66348150-092a-4eb7-9561-0b83adfa15ff"/>
        <dc:contributor>STEP Harmonization Team</dc:contributor>
        <dc:creator>Jean Brangé, AFNeT Services</dc:creator>
        <dc:date>2023-10-04</dc:date>
        <dc:source>ISO/TS 10303-4000</dc:source>
        <dc:type>InWork</dc:type>
        <rdfs:comment xml:lang="en">A DatumTarget is a type of ShapeElement. A DatumTarget is a datum target as specified in ISO 5459. The application of DatumTarget shall conform to the requirements of ISO 5459. Each DatumTarget is a PlacedTarget, a TargetArea, or a TargetCurve.</rdfs:comment>
        <owl:versionInfo>3</owl:versionInfo>
        <skos:changeNote>[2023-10-04] Jean Brangé, AFNeT Services: Initial definition.</skos:changeNote>
        <skos:example xml:lang="en">A cylindrical part is stabilized for measurement by resting it in a V block, thereby establishing a Datum from two instances of DatumTarget, which are straight lines.</skos:example>
        <skos:note xml:lang="en">A DatumTarget is the identification of a portion of a feature, which is used in the construction of a Datum when it is not desired to use an entire feature nor a substantial region.</skos:note>
        <skos:prefLabel xml:lang="en">datum target</skos:prefLabel>
    </owl:Class>
    


    <!-- http://standards.iso.org/iso/10303/tech/refdata/core#d30778d0-130a-0135-b552-598f1b1392ae -->

    <owl:Class rdf:about="http://standards.iso.org/iso/10303/tech/refdata/core#d30778d0-130a-0135-b552-598f1b1392ae">
        <rdfs:subClassOf rdf:resource="http://standards.iso.org/iso/10303/tech/refdata/core#59b11220-3279-0135-b58f-598f1b1392ae"/>
        <dc:contributor>STEP Harmonization Team</dc:contributor>
        <dc:creator>Phil Spiby, Eurostep</dc:creator>
        <dc:date>2022-09-01</dc:date>
        <dc:source>ISO/TS 10303-4000</dc:source>
        <dc:type>InWork</dc:type>
        <rdfs:comment xml:lang="en">A SuppliedObjectRelationship is a relationship between two objects of the SuppliedObjectSelect list representing the same object in different organizational contexts. The concept of multi-identification can also be used to distinguish objects in different organizational contexts. However, SuppliedObjectRelationship shall be used if the related object corresponds to an object at the supplier&apos;s site and if a distinction of additional information management is required.</rdfs:comment>
        <owl:versionInfo>2</owl:versionInfo>
        <skos:changeNote>[2021-07-30] Initial definition.</skos:changeNote>
        <skos:changeNote>[2022-09-01] Phil Spiby, Eurostep: updated comment updated example updated note.</skos:changeNote>
        <skos:example xml:lang="en">Usually, PartVersions that are provided by suppliers have at the supplier&apos;s site an id different from the one at the contractor&apos;s site: a PartVersion that is identified in a company by the identifier &apos;C425&apos; and the version id &apos;V2.0&apos; can correspond to the PartVersion that the supplier identifies as &apos;2X45&apos; with the version id &apos;V3.2&apos;.</skos:example>
        <skos:note xml:lang="en">The different organizational contexts can be represented by different OrganizationOrPersonInOrganizationAssignments.</skos:note>
        <skos:prefLabel xml:lang="en">supplied object relationship</skos:prefLabel>
    </owl:Class>
    


    <!-- http://standards.iso.org/iso/10303/tech/refdata/core#d30f001f-3b63-462c-9744-eb492b19bc60 -->

    <owl:Class rdf:about="http://standards.iso.org/iso/10303/tech/refdata/core#d30f001f-3b63-462c-9744-eb492b19bc60">
        <rdfs:subClassOf rdf:resource="http://standards.iso.org/iso/10303/tech/refdata/core#STEPThing"/>
        <dc:contributor>STEP Harmonization Team</dc:contributor>
        <dc:creator>Phil Spiby, Eurostep</dc:creator>
        <dc:date>2022-09-01</dc:date>
        <dc:source>ISO/TS 10303-4000</dc:source>
        <dc:type>InWork</dc:type>
        <rdfs:comment xml:lang="en">An ExperienceType is a category or class of experience.</rdfs:comment>
        <owl:versionInfo>1</owl:versionInfo>
        <skos:changeNote>[2022-09-01] Initial definition.</skos:changeNote>
        <skos:example xml:lang="en">flying</skos:example>
        <skos:example xml:lang="en">mechanical design</skos:example>
        <skos:example xml:lang="en">welding</skos:example>
        <skos:prefLabel xml:lang="en">experience type</skos:prefLabel>
    </owl:Class>
    


    <!-- http://standards.iso.org/iso/10303/tech/refdata/core#d36456e7-f236-4965-a037-486dd8ab90b9 -->

    <owl:Class rdf:about="http://standards.iso.org/iso/10303/tech/refdata/core#d36456e7-f236-4965-a037-486dd8ab90b9">
        <rdfs:subClassOf rdf:resource="http://standards.iso.org/iso/10303/tech/refdata/core#d75d6570-130a-0135-b552-598f1b1392ae"/>
        <dc:contributor>STEP Harmonization Team</dc:contributor>
        <dc:creator>Phil Spiby, Eurostep</dc:creator>
        <dc:date>2022-09-01</dc:date>
        <dc:source>ISO/TS 10303-4000</dc:source>
        <dc:type>InWork</dc:type>
        <rdfs:comment xml:lang="en">A ProbabilityDistribution is a specialization of ValueWithUnit that represents an assignment of probabilities (or probability densities in the case of continuous random variables) to all possible outcomes of a random variable.</rdfs:comment>
        <owl:versionInfo>1</owl:versionInfo>
        <skos:changeNote>[2022-09-01] Initial definition.</skos:changeNote>
        <skos:prefLabel xml:lang="en">probability distribution</skos:prefLabel>
    </owl:Class>
    


    <!-- http://standards.iso.org/iso/10303/tech/refdata/core#d397a83b-ddfa-46be-933c-547c6b4f2f12 -->

    <owl:Class rdf:about="http://standards.iso.org/iso/10303/tech/refdata/core#d397a83b-ddfa-46be-933c-547c6b4f2f12">
        <rdfs:subClassOf rdf:resource="http://standards.iso.org/iso/10303/tech/refdata/core#STEPThing"/>
        <dc:contributor>STEP Harmonization Team</dc:contributor>
        <dc:creator>Phil Spiby, Eurostep</dc:creator>
        <dc:date>2022-09-01</dc:date>
        <dc:source>ISO/TS 10303-4000</dc:source>
        <dc:type>InWork</dc:type>
        <rdfs:comment xml:lang="en">An InterfaceConnector identifies a part of a product with which one or more other products or the environment interacts.</rdfs:comment>
        <owl:versionInfo>2</owl:versionInfo>
        <skos:changeNote>[2021-07-30] Initial definition.</skos:changeNote>
        <skos:changeNote>[2022-09-01] Phil Spiby, Eurostep: updated note.</skos:changeNote>
        <skos:example xml:lang="en">A computer has a socket to which to connect a network cable. An instance of the InterfaceConnector entity data type identifies the role of the socket in the interface and is the subject of a specification that defines the necessary geometrical and electrical attributes to ensure a functioning interface between the computer and network hardware.</skos:example>
        <skos:note xml:lang="en">This is sometimes referred to as a &apos;port&apos;.</skos:note>
        <skos:prefLabel xml:lang="en">interface connector</skos:prefLabel>
    </owl:Class>
    


    <!-- http://standards.iso.org/iso/10303/tech/refdata/core#d3a17e30-1291-41ef-b222-b93ce73ab27a -->

    <owl:Class rdf:about="http://standards.iso.org/iso/10303/tech/refdata/core#d3a17e30-1291-41ef-b222-b93ce73ab27a">
        <rdfs:subClassOf rdf:resource="http://standards.iso.org/iso/10303/tech/refdata/core#9c98fe40-130a-0135-b552-598f1b1392ae"/>
        <dc:contributor>STEP Harmonization Team</dc:contributor>
        <dc:creator>Jean Brangé, AFNeT Services</dc:creator>
        <dc:date>2023-10-04</dc:date>
        <dc:source>ISO/TS 10303-4000</dc:source>
        <dc:type>InWork</dc:type>
        <rdfs:comment xml:lang="en">An ExternalCsgShapeRepresentation is a type of ExternalGeometricModel that references an instance of type ../../../resources/aic_csg/aic_csg.htm#aic_csg.csg_shape_representationcsg_shape_representation (ISO 10303-515).</rdfs:comment>
        <owl:versionInfo>3</owl:versionInfo>
        <skos:changeNote>[2023-10-04] Jean Brangé, AFNeT Services: Initial definition.</skos:changeNote>
        <skos:prefLabel xml:lang="en">external csg shape representation</skos:prefLabel>
    </owl:Class>
    


    <!-- http://standards.iso.org/iso/10303/tech/refdata/core#d3f940f6-b225-4934-ad98-ff71f3f3b727 -->

    <owl:Class rdf:about="http://standards.iso.org/iso/10303/tech/refdata/core#d3f940f6-b225-4934-ad98-ff71f3f3b727">
        <rdfs:subClassOf rdf:resource="http://standards.iso.org/iso/10303/tech/refdata/core#1d59c650-3279-0135-b58f-598f1b1392ae"/>
        <dc:contributor>STEP Harmonization Team</dc:contributor>
        <dc:creator>Phil Spiby, Eurostep</dc:creator>
        <dc:date>2022-09-01</dc:date>
        <dc:source>ISO/TS 10303-4000</dc:source>
        <dc:type>InWork</dc:type>
        <rdfs:comment xml:lang="en">A ResourceEventCorrespondenceAssociation is an association between a resource event and a corresponding statement of RequiredResource.</rdfs:comment>
        <owl:versionInfo>2</owl:versionInfo>
        <skos:changeNote>[2021-07-30] Initial definition.</skos:changeNote>
        <skos:changeNote>[2022-09-01] Phil Spiby, Eurostep: updated name updated comment updated example.</skos:changeNote>
        <skos:example xml:lang="en">A resource event correspondence association can be classified as &quot;Designated for&quot;.</skos:example>
        <skos:note xml:lang="en">A resource event can be planned or recorded without having a corresponding resource requirement statement.</skos:note>
        <skos:prefLabel xml:lang="en">resource event correspondence association</skos:prefLabel>
    </owl:Class>
    


    <!-- http://standards.iso.org/iso/10303/tech/refdata/core#d480b59d-3fd2-4915-a4c2-f30cb4b115aa -->

    <owl:Class rdf:about="http://standards.iso.org/iso/10303/tech/refdata/core#d480b59d-3fd2-4915-a4c2-f30cb4b115aa">
        <rdfs:subClassOf rdf:resource="http://standards.iso.org/iso/10303/tech/refdata/core#59b11220-3279-0135-b58f-598f1b1392ae"/>
        <dc:contributor>STEP Harmonization Team</dc:contributor>
        <dc:creator>Phil Spiby, Eurostep</dc:creator>
        <dc:date>2022-09-01</dc:date>
        <dc:source>ISO/TS 10303-4000</dc:source>
        <dc:type>InWork</dc:type>
        <rdfs:comment xml:lang="en">A PositionRelationship is a relationship between two Position objects.</rdfs:comment>
        <owl:versionInfo>1</owl:versionInfo>
        <skos:changeNote>[2022-09-01] Initial definition.</skos:changeNote>
        <skos:prefLabel xml:lang="en">position relationship</skos:prefLabel>
    </owl:Class>
    


    <!-- http://standards.iso.org/iso/10303/tech/refdata/core#d4836a70-130a-0135-b552-598f1b1392ae -->

    <owl:Class rdf:about="http://standards.iso.org/iso/10303/tech/refdata/core#d4836a70-130a-0135-b552-598f1b1392ae">
        <rdfs:subClassOf rdf:resource="http://standards.iso.org/iso/10303/tech/refdata/core#STEPThing"/>
        <dc:contributor>STEP Harmonization Team</dc:contributor>
        <dc:creator>Phil Spiby, Eurostep</dc:creator>
        <dc:date>2022-09-01</dc:date>
        <dc:source>ISO/TS 10303-4000</dc:source>
        <dc:type>InWork</dc:type>
        <rdfs:comment xml:lang="en">A TimeInterval is the specification of a unit of time.</rdfs:comment>
        <owl:versionInfo>1</owl:versionInfo>
        <skos:changeNote>[2021-07-30] Initial definition.</skos:changeNote>
        <skos:prefLabel xml:lang="en">time interval</skos:prefLabel>
    </owl:Class>
    


    <!-- http://standards.iso.org/iso/10303/tech/refdata/core#d4b13130-130a-0135-b552-598f1b1392ae -->

    <owl:Class rdf:about="http://standards.iso.org/iso/10303/tech/refdata/core#d4b13130-130a-0135-b552-598f1b1392ae">
        <rdfs:subClassOf rdf:resource="http://standards.iso.org/iso/10303/tech/refdata/core#1cfca290-3279-0135-b58f-598f1b1392ae"/>
        <dc:contributor>STEP Harmonization Team</dc:contributor>
        <dc:creator>Phil Spiby, Eurostep</dc:creator>
        <dc:date>2022-09-01</dc:date>
        <dc:source>ISO/TS 10303-4000</dc:source>
        <dc:type>InWork</dc:type>
        <rdfs:comment xml:lang="en">A TimeIntervalAssignment is an assignment of a TimeInterval to an item (specified by TimeIntervalAssignmentSelect). The TimeIntervalAssignment shall neither be used to convey effectivity information, such as information concerning valid use of product data, nor to convey retention information, nor duration information.</rdfs:comment>
        <owl:versionInfo>1</owl:versionInfo>
        <skos:changeNote>[2021-07-30] Initial definition.</skos:changeNote>
        <skos:note xml:lang="en">Such information is conveyed using Effectivity, RetentionPeriod, and Duration respectively.</skos:note>
        <skos:prefLabel xml:lang="en">time interval assignment</skos:prefLabel>
    </owl:Class>
    


    <!-- http://standards.iso.org/iso/10303/tech/refdata/core#d524c328-0343-4776-a43a-9df8c74acc5a -->

    <owl:Class rdf:about="http://standards.iso.org/iso/10303/tech/refdata/core#d524c328-0343-4776-a43a-9df8c74acc5a">
        <rdfs:subClassOf rdf:resource="http://standards.iso.org/iso/10303/tech/refdata/core#68242b94-82e8-4841-8005-89981113e22f"/>
        <dc:contributor>STEP Harmonization Team</dc:contributor>
        <dc:creator>Phil Spiby, Eurostep</dc:creator>
        <dc:date>2022-09-01</dc:date>
        <dc:source>ISO/TS 10303-4000</dc:source>
        <dc:type>InWork</dc:type>
        <rdfs:comment xml:lang="en">A GeographicalArea is a type of Locator specified through a geographical, physical or political region.</rdfs:comment>
        <owl:versionInfo>1</owl:versionInfo>
        <skos:changeNote>[2021-07-30] Initial definition.</skos:changeNote>
        <skos:example xml:lang="en">Europe, North America, Berlin and Indian Ocean.</skos:example>
        <skos:prefLabel xml:lang="en">geographical area</skos:prefLabel>
    </owl:Class>
    


    <!-- http://standards.iso.org/iso/10303/tech/refdata/core#d53f1950-130a-0135-b552-598f1b1392ae -->

    <owl:Class rdf:about="http://standards.iso.org/iso/10303/tech/refdata/core#d53f1950-130a-0135-b552-598f1b1392ae">
        <rdfs:subClassOf rdf:resource="http://standards.iso.org/iso/10303/tech/refdata/core#9384ed50-130a-0135-b552-598f1b1392ae"/>
        <dc:contributor>STEP Harmonization Team</dc:contributor>
        <dc:creator>Phil Spiby, Eurostep</dc:creator>
        <dc:date>2022-09-01</dc:date>
        <dc:source>ISO/TS 10303-4000</dc:source>
        <dc:type>InWork</dc:type>
        <rdfs:comment xml:lang="en">A TimeIntervalEffectivity is a type of Effectivity for which the domain of applicability is defined as a Duration. Depending on which of the StartDefinition and EndDefinition inherited attributes are specified, the actual domain of time defined by a TimeIntervalEffectivity is: the time interval that starts at the start date or event; the time interval that ends at the end date or event.</rdfs:comment>
        <owl:versionInfo>1</owl:versionInfo>
        <skos:changeNote>[2021-07-30] Initial definition.</skos:changeNote>
        <skos:prefLabel xml:lang="en">time interval effectivity</skos:prefLabel>
    </owl:Class>
    


    <!-- http://standards.iso.org/iso/10303/tech/refdata/core#d552ef70-130a-0135-b552-598f1b1392ae -->

    <owl:Class rdf:about="http://standards.iso.org/iso/10303/tech/refdata/core#d552ef70-130a-0135-b552-598f1b1392ae">
        <rdfs:subClassOf rdf:resource="http://standards.iso.org/iso/10303/tech/refdata/core#59b11220-3279-0135-b58f-598f1b1392ae"/>
        <dc:contributor>STEP Harmonization Team</dc:contributor>
        <dc:creator>Phil Spiby, Eurostep</dc:creator>
        <dc:date>2022-09-01</dc:date>
        <dc:source>ISO/TS 10303-4000</dc:source>
        <dc:type>InWork</dc:type>
        <rdfs:comment xml:lang="en">A TimeIntervalRelationship is a relationship between two TimeInterval objects.</rdfs:comment>
        <owl:versionInfo>2</owl:versionInfo>
        <skos:changeNote>[2021-07-30] Initial definition.</skos:changeNote>
        <skos:changeNote>[2022-09-01] Phil Spiby, Eurostep: updated comment updated note.</skos:changeNote>
        <skos:prefLabel xml:lang="en">time interval relationship</skos:prefLabel>
    </owl:Class>
    


    <!-- http://standards.iso.org/iso/10303/tech/refdata/core#d5ab2f97-854e-4272-bef6-f565c4a838f6 -->

    <owl:Class rdf:about="http://standards.iso.org/iso/10303/tech/refdata/core#d5ab2f97-854e-4272-bef6-f565c4a838f6">
        <rdfs:subClassOf rdf:resource="http://standards.iso.org/iso/10303/tech/refdata/core#STEPThing"/>
        <dc:contributor>STEP Harmonization Team</dc:contributor>
        <dc:creator>Phil Spiby, Eurostep</dc:creator>
        <dc:date>2022-09-01</dc:date>
        <dc:source>ISO/TS 10303-4000</dc:source>
        <dc:type>InWork</dc:type>
        <rdfs:comment xml:lang="en">A CollectionView represents a characterization of a CollectionVersion relevant in one or more application domains and for one or more life-cycle stages.</rdfs:comment>
        <owl:versionInfo>2</owl:versionInfo>
        <skos:changeNote>[2021-07-30] Initial definition.</skos:changeNote>
        <skos:changeNote>[2022-09-01] Phil Spiby, Eurostep: updated example.</skos:changeNote>
        <skos:example xml:lang="en">A set of data relevant to the design of the SS Titanic and a set of data relevant to the as-built description of the SS Titanic might be represented as two instances of CollectionView.</skos:example>
        <skos:prefLabel xml:lang="en">collection view</skos:prefLabel>
    </owl:Class>
    


    <!-- http://standards.iso.org/iso/10303/tech/refdata/core#d5ab6fb0-130a-0135-b552-598f1b1392ae -->

    <owl:Class rdf:about="http://standards.iso.org/iso/10303/tech/refdata/core#d5ab6fb0-130a-0135-b552-598f1b1392ae">
        <rdfs:subClassOf rdf:resource="http://standards.iso.org/iso/10303/tech/refdata/core#d4836a70-130a-0135-b552-598f1b1392ae"/>
        <dc:contributor>STEP Harmonization Team</dc:contributor>
        <dc:creator>Phil Spiby, Eurostep</dc:creator>
        <dc:date>2022-09-01</dc:date>
        <dc:source>ISO/TS 10303-4000</dc:source>
        <dc:type>InWork</dc:type>
        <rdfs:comment xml:lang="en">A TimeIntervalWithBounds is a type of TimeInterval. A TimeIntervalWithBounds is bounded either on one side or both sides.</rdfs:comment>
        <owl:versionInfo>1</owl:versionInfo>
        <skos:changeNote>[2021-07-30] Initial definition.</skos:changeNote>
        <skos:note xml:lang="en">If neither SecondaryBound nor Duration are specified, the time interval begins at the point in time identified by PrimaryBound and has no specified end point.</skos:note>
        <skos:prefLabel xml:lang="en">time interval with bounds</skos:prefLabel>
    </owl:Class>
    


    <!-- http://standards.iso.org/iso/10303/tech/refdata/core#d60ebc2c-d801-4620-9ea7-a84bfd9f5bbf -->

    <owl:Class rdf:about="http://standards.iso.org/iso/10303/tech/refdata/core#d60ebc2c-d801-4620-9ea7-a84bfd9f5bbf">
        <rdfs:subClassOf rdf:resource="http://standards.iso.org/iso/10303/tech/refdata/core#1d59c650-3279-0135-b58f-598f1b1392ae"/>
        <dc:contributor>STEP Harmonization Team</dc:contributor>
        <dc:creator>Jean Brangé, AFNeT Services</dc:creator>
        <dc:date>2023-10-04</dc:date>
        <dc:source>ISO/TS 10303-4000</dc:source>
        <dc:type>InWork</dc:type>
        <rdfs:comment xml:lang="en">A ProductStructureLinkMotionAssociation is an association between a LinkMotionRelationship and an Occurrence within an AssemblyDefinition.</rdfs:comment>
        <owl:versionInfo>3</owl:versionInfo>
        <skos:changeNote>[2023-10-04] Jean Brangé, AFNeT Services: Initial definition.</skos:changeNote>
        <skos:prefLabel xml:lang="en">product structure link motion association</skos:prefLabel>
    </owl:Class>
    


    <!-- http://standards.iso.org/iso/10303/tech/refdata/core#d61c59f0-130a-0135-b552-598f1b1392ae -->

    <owl:Class rdf:about="http://standards.iso.org/iso/10303/tech/refdata/core#d61c59f0-130a-0135-b552-598f1b1392ae">
        <rdfs:subClassOf rdf:resource="http://standards.iso.org/iso/10303/tech/refdata/core#9fddc900-130a-0135-b552-598f1b1392ae"/>
        <dc:contributor>STEP Harmonization Team</dc:contributor>
        <dc:creator>Phil Spiby, Eurostep</dc:creator>
        <dc:date>2022-09-01</dc:date>
        <dc:source>ISO/TS 10303-4000</dc:source>
        <dc:type>InWork</dc:type>
        <rdfs:comment xml:lang="en">A TransformedGeometricModel is a type of GeometricModel that is the transformation result of another GeometricModel.</rdfs:comment>
        <owl:versionInfo>1</owl:versionInfo>
        <skos:changeNote>[2021-07-30] Initial definition.</skos:changeNote>
        <skos:prefLabel xml:lang="en">transformed geometric model</skos:prefLabel>
    </owl:Class>
    


    <!-- http://standards.iso.org/iso/10303/tech/refdata/core#d66b1630-130a-0135-b552-598f1b1392ae -->

    <owl:Class rdf:about="http://standards.iso.org/iso/10303/tech/refdata/core#d66b1630-130a-0135-b552-598f1b1392ae">
        <rdfs:subClassOf rdf:resource="http://standards.iso.org/iso/10303/tech/refdata/core#STEPThing"/>
        <dc:contributor>STEP Harmonization Team</dc:contributor>
        <dc:creator>Phil Spiby, Eurostep</dc:creator>
        <dc:date>2022-09-01</dc:date>
        <dc:source>ISO/TS 10303-4000</dc:source>
        <dc:type>InWork</dc:type>
        <rdfs:comment xml:lang="en">An UncertaintyQualifier is a qualifier that specifies an uncertainty as defined in ISO/IEC Guide 98-3.</rdfs:comment>
        <owl:versionInfo>2</owl:versionInfo>
        <skos:changeNote>[2021-07-30] Initial definition.</skos:changeNote>
        <skos:changeNote>[2022-09-01] Phil Spiby, Eurostep: updated comment.</skos:changeNote>
        <skos:prefLabel xml:lang="en">uncertainty qualifier</skos:prefLabel>
    </owl:Class>
    


    <!-- http://standards.iso.org/iso/10303/tech/refdata/core#d698dcf0-130a-0135-b552-598f1b1392ae -->

    <owl:Class rdf:about="http://standards.iso.org/iso/10303/tech/refdata/core#d698dcf0-130a-0135-b552-598f1b1392ae">
        <rdfs:subClassOf rdf:resource="http://standards.iso.org/iso/10303/tech/refdata/core#STEPThing"/>
        <dc:contributor>STEP Harmonization Team</dc:contributor>
        <dc:creator>Phil Spiby, Eurostep</dc:creator>
        <dc:date>2022-09-01</dc:date>
        <dc:source>ISO/TS 10303-4000</dc:source>
        <dc:type>InWork</dc:type>
        <rdfs:comment xml:lang="en">A Unit is a quantity chosen as a standard in terms of which other quantities can be expressed. The types of units supported by this standard are SI units as well as derived or conversion-based units as defined in ISO 10303-41.</rdfs:comment>
        <owl:versionInfo>2</owl:versionInfo>
        <skos:changeNote>[2021-07-30] Initial definition.</skos:changeNote>
        <skos:changeNote>[2022-09-01] Phil Spiby, Eurostep: updated comment.</skos:changeNote>
        <skos:prefLabel xml:lang="en">unit</skos:prefLabel>
    </owl:Class>
    


    <!-- http://standards.iso.org/iso/10303/tech/refdata/core#d6d15210-130a-0135-b552-598f1b1392ae -->

    <owl:Class rdf:about="http://standards.iso.org/iso/10303/tech/refdata/core#d6d15210-130a-0135-b552-598f1b1392ae">
        <rdfs:subClassOf rdf:resource="http://standards.iso.org/iso/10303/tech/refdata/core#adfff300-130a-0135-b552-598f1b1392ae"/>
        <dc:contributor>STEP Harmonization Team</dc:contributor>
        <dc:creator>Phil Spiby, Eurostep</dc:creator>
        <dc:date>2022-09-01</dc:date>
        <dc:source>ISO/TS 10303-4000</dc:source>
        <dc:type>InWork</dc:type>
        <rdfs:comment xml:lang="en">A ValueLimit is a type of NumericalValue with a qualified numerical value representing either the lower limit or the upper limit of a specific physical characteristic.</rdfs:comment>
        <owl:versionInfo>2</owl:versionInfo>
        <skos:changeNote>[2021-07-30] Initial definition.</skos:changeNote>
        <skos:changeNote>[2022-09-01] Phil Spiby, Eurostep: updated example.</skos:changeNote>
        <skos:example xml:lang="en">&apos;30.5 max&apos; and &apos;5 min&apos; are examples for a ValueLimit.</skos:example>
        <skos:prefLabel xml:lang="en">value limit</skos:prefLabel>
    </owl:Class>
    


    <!-- http://standards.iso.org/iso/10303/tech/refdata/core#d6e38a84-a8b6-42d5-ab22-37fc10cde834 -->

    <owl:Class rdf:about="http://standards.iso.org/iso/10303/tech/refdata/core#d6e38a84-a8b6-42d5-ab22-37fc10cde834">
        <rdfs:subClassOf rdf:resource="http://standards.iso.org/iso/10303/tech/refdata/core#55105ef0-713f-409a-8306-fd8708d4ee3f"/>
        <dc:contributor>STEP Harmonization Team</dc:contributor>
        <dc:creator>Jean Brangé, AFNeT Services</dc:creator>
        <dc:date>2023-10-04</dc:date>
        <dc:source>ISO/TS 10303-4000</dc:source>
        <dc:type>InWork</dc:type>
        <rdfs:comment xml:lang="en">A RoundnessTolerance is a type of GeometricTolerance that specifies a tolerance zone bounded by two concentric circles within which each circular element of a surface must lie. For a sphere, a circular element is all points of the surface intersected by any plane passing through a common centre. For other surfaces, a circular element is all points of the surface intersected by any plane perpendicular to an axis. The RoundnessTolerance condition applies independently at any plane. Unless otherwise specified, the rules governing roundness tolerance defined in ISO 1101 shall apply.</rdfs:comment>
        <owl:versionInfo>3</owl:versionInfo>
        <skos:changeNote>[2023-10-04] Jean Brangé, AFNeT Services: Initial definition.</skos:changeNote>
        <skos:note xml:lang="en">Alternatively roundness tolerance can be used according to the specifications given in ASME Y14.5-2009.</skos:note>
        <skos:prefLabel xml:lang="en">roundness tolerance</skos:prefLabel>
    </owl:Class>
    


    <!-- http://standards.iso.org/iso/10303/tech/refdata/core#d6e52830-130a-0135-b552-598f1b1392ae -->

    <owl:Class rdf:about="http://standards.iso.org/iso/10303/tech/refdata/core#d6e52830-130a-0135-b552-598f1b1392ae">
        <rdfs:subClassOf rdf:resource="http://standards.iso.org/iso/10303/tech/refdata/core#c27698c0-130a-0135-b552-598f1b1392ae"/>
        <dc:contributor>STEP Harmonization Team</dc:contributor>
        <dc:creator>Phil Spiby, Eurostep</dc:creator>
        <dc:date>2022-09-01</dc:date>
        <dc:source>ISO/TS 10303-4000</dc:source>
        <dc:type>InWork</dc:type>
        <rdfs:comment xml:lang="en">A ValueList is a type of PropertyValue with an ordered collection of PropertyValue objects.</rdfs:comment>
        <owl:versionInfo>2</owl:versionInfo>
        <skos:changeNote>[2021-07-30] Initial definition.</skos:changeNote>
        <skos:changeNote>[2022-09-01] Phil Spiby, Eurostep: updated example.</skos:changeNote>
        <skos:example xml:lang="en">A PropertyDefinition can be composed of different property values such as &apos;mass&apos;, &apos;speed&apos;, and &apos;age&apos; which are altogether necessary in a given context. The ValueList collects all of them in a given order, such that each is identifiable by its index in the list.</skos:example>
        <skos:prefLabel xml:lang="en">value list</skos:prefLabel>
    </owl:Class>
    


    <!-- http://standards.iso.org/iso/10303/tech/refdata/core#d6f48728-6e63-4166-adeb-c6beb07e5f2d -->

    <owl:Class rdf:about="http://standards.iso.org/iso/10303/tech/refdata/core#d6f48728-6e63-4166-adeb-c6beb07e5f2d">
        <rdfs:subClassOf rdf:resource="http://standards.iso.org/iso/10303/tech/refdata/core#d2bb2d90-130a-0135-b552-598f1b1392ae"/>
        <dc:contributor>STEP Harmonization Team</dc:contributor>
        <dc:creator>Jean Brangé, AFNeT Services</dc:creator>
        <dc:date>2023-10-04</dc:date>
        <dc:source>ISO/TS 10303-4000</dc:source>
        <dc:type>InWork</dc:type>
        <rdfs:comment xml:lang="en">An ExternalStyledModel is a type of StyledModel that defines the stub for a set of geometric or annotation elements for which visual characteristics are specified. The geometric or annotation elements are defined in a DigitalFile.</rdfs:comment>
        <owl:versionInfo>3</owl:versionInfo>
        <skos:changeNote>[2023-10-04] Jean Brangé, AFNeT Services: Initial definition.</skos:changeNote>
        <skos:prefLabel xml:lang="en">external styled model</skos:prefLabel>
    </owl:Class>
    


    <!-- http://standards.iso.org/iso/10303/tech/refdata/core#d6f8fe50-130a-0135-b552-598f1b1392ae -->

    <owl:Class rdf:about="http://standards.iso.org/iso/10303/tech/refdata/core#d6f8fe50-130a-0135-b552-598f1b1392ae">
        <rdfs:subClassOf rdf:resource="http://standards.iso.org/iso/10303/tech/refdata/core#d75d6570-130a-0135-b552-598f1b1392ae"/>
        <dc:contributor>STEP Harmonization Team</dc:contributor>
        <dc:creator>Phil Spiby, Eurostep</dc:creator>
        <dc:date>2022-09-01</dc:date>
        <dc:source>ISO/TS 10303-4000</dc:source>
        <dc:type>InWork</dc:type>
        <rdfs:comment xml:lang="en">A ValueRange is a type of ValueWithUnit with a pair of numerical values representing the range in which the value shall lie.</rdfs:comment>
        <owl:versionInfo>1</owl:versionInfo>
        <skos:changeNote>[2021-07-30] Initial definition.</skos:changeNote>
        <skos:prefLabel xml:lang="en">value range</skos:prefLabel>
    </owl:Class>
    


    <!-- http://standards.iso.org/iso/10303/tech/refdata/core#d71a9010-130a-0135-b552-598f1b1392ae -->

    <owl:Class rdf:about="http://standards.iso.org/iso/10303/tech/refdata/core#d71a9010-130a-0135-b552-598f1b1392ae">
        <rdfs:subClassOf rdf:resource="http://standards.iso.org/iso/10303/tech/refdata/core#c27698c0-130a-0135-b552-598f1b1392ae"/>
        <dc:contributor>STEP Harmonization Team</dc:contributor>
        <dc:creator>Phil Spiby, Eurostep</dc:creator>
        <dc:date>2022-09-01</dc:date>
        <dc:source>ISO/TS 10303-4000</dc:source>
        <dc:type>InWork</dc:type>
        <rdfs:comment xml:lang="en">A ValueSet is a type of PropertyValue with an unordered collection of PropertyValue objects.</rdfs:comment>
        <owl:versionInfo>1</owl:versionInfo>
        <skos:changeNote>[2021-07-30] Initial definition.</skos:changeNote>
        <skos:prefLabel xml:lang="en">value set</skos:prefLabel>
    </owl:Class>
    


    <!-- http://standards.iso.org/iso/10303/tech/refdata/core#d723e1aa-0001-421b-b6a2-34253ee40ef7 -->

    <owl:Class rdf:about="http://standards.iso.org/iso/10303/tech/refdata/core#d723e1aa-0001-421b-b6a2-34253ee40ef7">
        <rdfs:subClassOf rdf:resource="http://standards.iso.org/iso/10303/tech/refdata/core#59b11220-3279-0135-b58f-598f1b1392ae"/>
        <dc:contributor>STEP Harmonization Team</dc:contributor>
        <dc:creator>Phil Spiby, Eurostep</dc:creator>
        <dc:date>2022-09-01</dc:date>
        <dc:source>ISO/TS 10303-4000</dc:source>
        <dc:type>InWork</dc:type>
        <rdfs:comment xml:lang="en">An AnalysisVersionRelationship is a relationship between two AnalysisVersion objects.</rdfs:comment>
        <owl:versionInfo>2</owl:versionInfo>
        <skos:changeNote>[2021-07-30] Initial definition.</skos:changeNote>
        <skos:changeNote>[2022-09-01] Phil Spiby, Eurostep: updated comment.</skos:changeNote>
        <skos:prefLabel xml:lang="en">analysis version relationship</skos:prefLabel>
    </owl:Class>
    


    <!-- http://standards.iso.org/iso/10303/tech/refdata/core#d72e1810-130a-0135-b552-598f1b1392ae -->

    <owl:Class rdf:about="http://standards.iso.org/iso/10303/tech/refdata/core#d72e1810-130a-0135-b552-598f1b1392ae">
        <rdfs:subClassOf rdf:resource="http://standards.iso.org/iso/10303/tech/refdata/core#d75d6570-130a-0135-b552-598f1b1392ae"/>
        <dc:contributor>STEP Harmonization Team</dc:contributor>
        <dc:creator>Phil Spiby, Eurostep</dc:creator>
        <dc:date>2022-09-01</dc:date>
        <dc:source>ISO/TS 10303-4000</dc:source>
        <dc:type>InWork</dc:type>
        <rdfs:comment xml:lang="en">A ValueWithTolerances is a type of ValueWithUnit that specifies a range of values by specifying a single nominal value and two tolerances that are offsets from the single value. The range is defined to be the closed interval [tolerancedValue + lowerLimit, tolerancedValue + upperLimit].</rdfs:comment>
        <owl:versionInfo>1</owl:versionInfo>
        <skos:changeNote>[2021-07-30] Initial definition.</skos:changeNote>
        <skos:prefLabel xml:lang="en">value with tolerances</skos:prefLabel>
    </owl:Class>
    


    <!-- http://standards.iso.org/iso/10303/tech/refdata/core#d72eb4d6-771e-448f-9d46-3b5fcb2982a1 -->

    <owl:Class rdf:about="http://standards.iso.org/iso/10303/tech/refdata/core#d72eb4d6-771e-448f-9d46-3b5fcb2982a1">
        <rdfs:subClassOf rdf:resource="http://standards.iso.org/iso/10303/tech/refdata/core#5a6c8b1f-63af-4307-9faf-9fdd6da5572c"/>
        <dc:contributor>STEP Harmonization Team</dc:contributor>
        <dc:creator>Jean Brangé, AFNeT Services</dc:creator>
        <dc:date>2023-10-04</dc:date>
        <dc:source>ISO/TS 10303-4000</dc:source>
        <dc:type>InWork</dc:type>
        <rdfs:comment xml:lang="en">A PlyLaminate is a type of ConstituentPart that is formed by two or more Ply objects that mate with each other. The plies have unique orientation and shape within the PlyLaminate. PlyLaminate.pngPly laminate</rdfs:comment>
        <owl:versionInfo>3</owl:versionInfo>
        <skos:changeNote>[2023-10-04] Jean Brangé, AFNeT Services: Initial definition.</skos:changeNote>
        <skos:note xml:lang="en">Examples of PlyLaminate shape include angle, cap, flat, general contour, simple contour, complex contour, channel, etc. (see following figure).</skos:note>
        <skos:prefLabel xml:lang="en">ply laminate</skos:prefLabel>
    </owl:Class>
    


    <!-- http://standards.iso.org/iso/10303/tech/refdata/core#d75d6570-130a-0135-b552-598f1b1392ae -->

    <owl:Class rdf:about="http://standards.iso.org/iso/10303/tech/refdata/core#d75d6570-130a-0135-b552-598f1b1392ae">
        <rdfs:subClassOf rdf:resource="http://standards.iso.org/iso/10303/tech/refdata/core#c27698c0-130a-0135-b552-598f1b1392ae"/>
        <dc:contributor>STEP Harmonization Team</dc:contributor>
        <dc:creator>Phil Spiby, Eurostep</dc:creator>
        <dc:date>2022-09-01</dc:date>
        <dc:source>ISO/TS 10303-4000</dc:source>
        <dc:type>InWork</dc:type>
        <rdfs:comment xml:lang="en">A ValueWithUnit is a type of PropertyValue with either a single numerical measure, or a range of numerical measures with upper, lower, or upper and lower bounds.</rdfs:comment>
        <owl:versionInfo>1</owl:versionInfo>
        <skos:changeNote>[2021-07-30] Initial definition.</skos:changeNote>
        <skos:prefLabel xml:lang="en">value with unit</skos:prefLabel>
    </owl:Class>
    


    <!-- http://standards.iso.org/iso/10303/tech/refdata/core#d80a2030-130a-0135-b552-598f1b1392ae -->

    <owl:Class rdf:about="http://standards.iso.org/iso/10303/tech/refdata/core#d80a2030-130a-0135-b552-598f1b1392ae">
        <rdfs:subClassOf rdf:resource="http://standards.iso.org/iso/10303/tech/refdata/core#59b11220-3279-0135-b58f-598f1b1392ae"/>
        <dc:contributor>STEP Harmonization Team</dc:contributor>
        <dc:creator>Phil Spiby, Eurostep</dc:creator>
        <dc:date>2022-09-01</dc:date>
        <dc:source>ISO/TS 10303-4000</dc:source>
        <dc:type>InWork</dc:type>
        <rdfs:comment xml:lang="en">A ViewOccurrenceRelationship is a relationship between a PartView and a DefinitionBasedOccurrence.</rdfs:comment>
        <owl:versionInfo>2</owl:versionInfo>
        <skos:changeNote>[2021-07-30] Initial definition.</skos:changeNote>
        <skos:changeNote>[2022-09-01] Phil Spiby, Eurostep: updated comment.</skos:changeNote>
        <skos:prefLabel xml:lang="en">view occurrence relationship</skos:prefLabel>
    </owl:Class>
    


    <!-- http://standards.iso.org/iso/10303/tech/refdata/core#d835b5be-6caa-4b7d-afc9-104e9985ade7 -->

    <owl:Class rdf:about="http://standards.iso.org/iso/10303/tech/refdata/core#d835b5be-6caa-4b7d-afc9-104e9985ade7">
        <rdfs:subClassOf rdf:resource="http://standards.iso.org/iso/10303/tech/refdata/core#66348150-092a-4eb7-9561-0b83adfa15ff"/>
        <dc:contributor>STEP Harmonization Team</dc:contributor>
        <dc:creator>Jean Brangé, AFNeT Services</dc:creator>
        <dc:date>2023-10-04</dc:date>
        <dc:source>ISO/TS 10303-4000</dc:source>
        <dc:type>InWork</dc:type>
        <rdfs:comment xml:lang="en">A DatumFeature is a type of ShapeElement on the boundary of the shape of a product. Unless otherwise specified, the rules governing datum feature defined in ISO 5459 shall apply.</rdfs:comment>
        <owl:versionInfo>3</owl:versionInfo>
        <skos:changeNote>[2023-10-04] Jean Brangé, AFNeT Services: Initial definition.</skos:changeNote>
        <skos:note xml:lang="en">Alternatively datum feature can be used according to the specifications given in ASME Y14.5</skos:note>
        <skos:prefLabel xml:lang="en">datum feature</skos:prefLabel>
    </owl:Class>
    


    <!-- http://standards.iso.org/iso/10303/tech/refdata/core#d8381cb4-ef44-45bb-ba54-3476e2f5f45e -->

    <owl:Class rdf:about="http://standards.iso.org/iso/10303/tech/refdata/core#d8381cb4-ef44-45bb-ba54-3476e2f5f45e">
        <rdfs:subClassOf rdf:resource="http://standards.iso.org/iso/10303/tech/refdata/core#0cc8b831-37f7-4cd5-984f-dbb5588fbc1d"/>
        <dc:contributor>STEP Harmonization Team</dc:contributor>
        <dc:creator>Jean Brangé, AFNeT Services</dc:creator>
        <dc:date>2023-10-04</dc:date>
        <dc:source>ISO/TS 10303-4000</dc:source>
        <dc:type>InWork</dc:type>
        <rdfs:comment xml:lang="en">A PartFeature is a type of PartShapeElement that represents an external shape feature of a PartView.</rdfs:comment>
        <owl:versionInfo>3</owl:versionInfo>
        <skos:changeNote>[2023-10-04] Jean Brangé, AFNeT Services: Initial definition.</skos:changeNote>
        <skos:prefLabel xml:lang="en">part feature</skos:prefLabel>
    </owl:Class>
    


    <!-- http://standards.iso.org/iso/10303/tech/refdata/core#d86da277-f8ae-488b-8ab6-37ab005b6109 -->

    <owl:Class rdf:about="http://standards.iso.org/iso/10303/tech/refdata/core#d86da277-f8ae-488b-8ab6-37ab005b6109">
        <rdfs:subClassOf rdf:resource="http://standards.iso.org/iso/10303/tech/refdata/core#STEPThing"/>
        <dc:contributor>STEP Harmonization Team</dc:contributor>
        <dc:creator>Phil Spiby, Eurostep</dc:creator>
        <dc:date>2022-09-01</dc:date>
        <dc:source>ISO/TS 10303-4000</dc:source>
        <dc:type>InWork</dc:type>
        <rdfs:comment xml:lang="en">An InterfaceConnectorOccurrence is an occurrence of an InterfaceConnectorView. The InterfaceConnectorOccurrence represents the place where a product used in an assembly can interact with other products in the assembly. The interaction is represented by an InterfaceConnection.</rdfs:comment>
        <owl:versionInfo>2</owl:versionInfo>
        <skos:changeNote>[2021-07-30] Initial definition.</skos:changeNote>
        <skos:changeNote>[2022-09-01] Phil Spiby, Eurostep: updated comment.</skos:changeNote>
        <skos:prefLabel xml:lang="en">interface connector occurrence</skos:prefLabel>
    </owl:Class>
    


    <!-- http://standards.iso.org/iso/10303/tech/refdata/core#d8e90e80-130a-0135-b552-598f1b1392ae -->

    <owl:Class rdf:about="http://standards.iso.org/iso/10303/tech/refdata/core#d8e90e80-130a-0135-b552-598f1b1392ae">
        <rdfs:subClassOf rdf:resource="http://standards.iso.org/iso/10303/tech/refdata/core#STEPThing"/>
        <dc:contributor>STEP Harmonization Team</dc:contributor>
        <dc:creator>Phil Spiby, Eurostep</dc:creator>
        <dc:date>2022-09-01</dc:date>
        <dc:source>ISO/TS 10303-4000</dc:source>
        <dc:type>InWork</dc:type>
        <rdfs:comment xml:lang="en">A WorkOrder is an authorization for one or more Activity objects to be performed.</rdfs:comment>
        <owl:versionInfo>2</owl:versionInfo>
        <skos:changeNote>[2021-07-30] Initial definition.</skos:changeNote>
        <skos:changeNote>[2022-09-01] Phil Spiby, Eurostep: updated note.</skos:changeNote>
        <skos:note xml:lang="en">One or more means that it is controlling the main activity and any sub-activity related to the activity by ActivityRelationship with RelationType of &apos;decomposition&apos;.</skos:note>
        <skos:prefLabel xml:lang="en">work order</skos:prefLabel>
    </owl:Class>
    


    <!-- http://standards.iso.org/iso/10303/tech/refdata/core#d93b072c-2d83-416e-b892-5964e964d01e -->

    <owl:Class rdf:about="http://standards.iso.org/iso/10303/tech/refdata/core#d93b072c-2d83-416e-b892-5964e964d01e">
        <rdfs:subClassOf rdf:resource="http://standards.iso.org/iso/10303/tech/refdata/core#59b11220-3279-0135-b58f-598f1b1392ae"/>
        <dc:contributor>STEP Harmonization Team</dc:contributor>
        <dc:creator>Jean Brangé, AFNeT Services</dc:creator>
        <dc:date>2023-10-04</dc:date>
        <dc:source>ISO/TS 10303-4000</dc:source>
        <dc:type>InWork</dc:type>
        <rdfs:comment xml:lang="en">A GeometricToleranceRelationship is a relationship between two instances of GeometricTolerance. The meaning of the relationship is specified within the attribute RelationType.</rdfs:comment>
        <owl:versionInfo>3</owl:versionInfo>
        <skos:changeNote>[2023-10-04] Jean Brangé, AFNeT Services: Initial definition.</skos:changeNote>
        <skos:prefLabel xml:lang="en">geometric tolerance relationship</skos:prefLabel>
    </owl:Class>
    


    <!-- http://standards.iso.org/iso/10303/tech/refdata/core#d964d356-facb-4d51-8bcb-615c00129619 -->

    <owl:Class rdf:about="http://standards.iso.org/iso/10303/tech/refdata/core#d964d356-facb-4d51-8bcb-615c00129619">
        <rdfs:subClassOf rdf:resource="http://standards.iso.org/iso/10303/tech/refdata/core#f8816baf-d66a-42f9-bdcc-38e946c9a2fa"/>
        <dc:contributor>STEP Harmonization Team</dc:contributor>
        <dc:creator>Jean Brangé, AFNeT Services</dc:creator>
        <dc:date>2023-10-04</dc:date>
        <dc:source>ISO/TS 10303-4000</dc:source>
        <dc:type>InWork</dc:type>
        <rdfs:comment xml:lang="en">A PerpendicularTo is a type of DerivedShapeElement that is oriented orthogonally to another ShapeElement.</rdfs:comment>
        <owl:versionInfo>3</owl:versionInfo>
        <skos:changeNote>[2023-10-04] Jean Brangé, AFNeT Services: Initial definition.</skos:changeNote>
        <skos:prefLabel xml:lang="en">perpendicular to</skos:prefLabel>
    </owl:Class>
    


    <!-- http://standards.iso.org/iso/10303/tech/refdata/core#d96c4840-130a-0135-b552-598f1b1392ae -->

    <owl:Class rdf:about="http://standards.iso.org/iso/10303/tech/refdata/core#d96c4840-130a-0135-b552-598f1b1392ae">
        <rdfs:subClassOf rdf:resource="http://standards.iso.org/iso/10303/tech/refdata/core#1cfca290-3279-0135-b58f-598f1b1392ae"/>
        <dc:contributor>STEP Harmonization Team</dc:contributor>
        <dc:creator>Phil Spiby, Eurostep</dc:creator>
        <dc:date>2022-09-01</dc:date>
        <dc:source>ISO/TS 10303-4000</dc:source>
        <dc:type>InWork</dc:type>
        <rdfs:comment xml:lang="en">A WorkOrderAssignment is an assignment of a WorkOrder an item (specified by WorkOrderAssignmentSelect) that is subject of this WorkOrder.</rdfs:comment>
        <owl:versionInfo>1</owl:versionInfo>
        <skos:changeNote>[2021-07-30] Initial definition.</skos:changeNote>
        <skos:prefLabel xml:lang="en">work order assignment</skos:prefLabel>
    </owl:Class>
    


    <!-- http://standards.iso.org/iso/10303/tech/refdata/core#d989099d-69b8-4d7b-95a7-0eb3b8a2586f -->

    <owl:Class rdf:about="http://standards.iso.org/iso/10303/tech/refdata/core#d989099d-69b8-4d7b-95a7-0eb3b8a2586f">
        <rdfs:subClassOf rdf:resource="http://standards.iso.org/iso/10303/tech/refdata/core#c565c970-130a-0135-b552-598f1b1392ae"/>
        <dc:contributor>STEP Harmonization Team</dc:contributor>
        <dc:creator>Jean Brangé, AFNeT Services</dc:creator>
        <dc:date>2023-10-04</dc:date>
        <dc:source>ISO/TS 10303-4000</dc:source>
        <dc:type>InWork</dc:type>
        <rdfs:comment xml:lang="en">A ReinforcementOrientationBasis is the definition of direction defined in terms of a PlyLaminate or CompositeAssembly. It is the basis for interpretation of the fiber orientation within a ply and is commonly known as a rosette.</rdfs:comment>
        <owl:versionInfo>3</owl:versionInfo>
        <skos:changeNote>[2023-10-04] Jean Brangé, AFNeT Services: Initial definition.</skos:changeNote>
        <skos:prefLabel xml:lang="en">reinforcement orientation basis</skos:prefLabel>
    </owl:Class>
    


    <!-- http://standards.iso.org/iso/10303/tech/refdata/core#d9d899e3-5c83-4be3-9738-ae144bc143f8 -->

    <owl:Class rdf:about="http://standards.iso.org/iso/10303/tech/refdata/core#d9d899e3-5c83-4be3-9738-ae144bc143f8">
        <rdfs:subClassOf rdf:resource="http://standards.iso.org/iso/10303/tech/refdata/core#d36456e7-f236-4965-a037-486dd8ab90b9"/>
        <dc:contributor>STEP Harmonization Team</dc:contributor>
        <dc:creator>Phil Spiby, Eurostep</dc:creator>
        <dc:date>2022-09-01</dc:date>
        <dc:source>ISO/TS 10303-4000</dc:source>
        <dc:type>InWork</dc:type>
        <rdfs:comment xml:lang="en">A DistributionByValue is a specialization of ProbabilityDistribution that explicitly lists pairs of random variable values and function values.</rdfs:comment>
        <owl:versionInfo>1</owl:versionInfo>
        <skos:changeNote>[2022-09-01] Initial definition.</skos:changeNote>
        <skos:note xml:lang="en">DistributionByValue is used where there is no named distribution which can be used to identify the distribution. This is the case when the distribution is derived from observation.</skos:note>
        <skos:prefLabel xml:lang="en">distribution by value</skos:prefLabel>
    </owl:Class>
    


    <!-- http://standards.iso.org/iso/10303/tech/refdata/core#d9e7cc39-134a-430a-92d9-bba8e9b73ca1 -->

    <owl:Class rdf:about="http://standards.iso.org/iso/10303/tech/refdata/core#d9e7cc39-134a-430a-92d9-bba8e9b73ca1">
        <rdfs:subClassOf rdf:resource="http://standards.iso.org/iso/10303/tech/refdata/core#STEPThing"/>
        <dc:contributor>STEP Harmonization Team</dc:contributor>
        <dc:creator>Phil Spiby, Eurostep</dc:creator>
        <dc:date>2022-09-01</dc:date>
        <dc:source>ISO/TS 10303-4000</dc:source>
        <dc:type>InWork</dc:type>
        <rdfs:comment xml:lang="en">A ConditionEvaluation is a record of the evaluation of a Condition and the subsequent result.</rdfs:comment>
        <owl:versionInfo>2</owl:versionInfo>
        <skos:changeNote>[2021-07-30] Initial definition.</skos:changeNote>
        <skos:changeNote>[2022-09-01] Phil Spiby, Eurostep: updated example.</skos:changeNote>
        <skos:example xml:lang="en">A Condition is defined as &quot;If the measured value of oil pressure from gauge 3 on a car is less than 2 bar then check the oil level&quot;. When the condition is evaluated it is recorded by an instance of ConditionEvaluation. The measured value of oil pressure from gauge 3 on car with VIN 12345678 is 1.9 bar. Therefore the result of the evaluated condition is true.</skos:example>
        <skos:prefLabel xml:lang="en">condition evaluation</skos:prefLabel>
    </owl:Class>
    


    <!-- http://standards.iso.org/iso/10303/tech/refdata/core#d9ef8200-130a-0135-b552-598f1b1392ae -->

    <owl:Class rdf:about="http://standards.iso.org/iso/10303/tech/refdata/core#d9ef8200-130a-0135-b552-598f1b1392ae">
        <rdfs:subClassOf rdf:resource="http://standards.iso.org/iso/10303/tech/refdata/core#59b11220-3279-0135-b58f-598f1b1392ae"/>
        <dc:contributor>STEP Harmonization Team</dc:contributor>
        <dc:creator>Phil Spiby, Eurostep</dc:creator>
        <dc:date>2022-09-01</dc:date>
        <dc:source>ISO/TS 10303-4000</dc:source>
        <dc:type>InWork</dc:type>
        <rdfs:comment xml:lang="en">A WorkOrderRelationship is a relationship between two WorkOrder objects.</rdfs:comment>
        <owl:versionInfo>1</owl:versionInfo>
        <skos:changeNote>[2021-07-30] Initial definition.</skos:changeNote>
        <skos:prefLabel xml:lang="en">work order relationship</skos:prefLabel>
    </owl:Class>
    


    <!-- http://standards.iso.org/iso/10303/tech/refdata/core#da480240-130a-0135-b552-598f1b1392ae -->

    <owl:Class rdf:about="http://standards.iso.org/iso/10303/tech/refdata/core#da480240-130a-0135-b552-598f1b1392ae">
        <rdfs:subClassOf rdf:resource="http://standards.iso.org/iso/10303/tech/refdata/core#STEPThing"/>
        <dc:contributor>STEP Harmonization Team</dc:contributor>
        <dc:creator>Phil Spiby, Eurostep</dc:creator>
        <dc:date>2022-09-01</dc:date>
        <dc:source>ISO/TS 10303-4000</dc:source>
        <dc:type>InWork</dc:type>
        <rdfs:comment xml:lang="en">A WorkRequest is a solicitation for some work to be done.</rdfs:comment>
        <owl:versionInfo>2</owl:versionInfo>
        <skos:changeNote>[2021-07-30] Initial definition.</skos:changeNote>
        <skos:changeNote>[2022-09-01] Phil Spiby, Eurostep: updated note.</skos:changeNote>
        <skos:note xml:lang="en">These requests cannot be acted upon depending on the authorization granted to the request or its associated WorkOrder.</skos:note>
        <skos:prefLabel xml:lang="en">work request</skos:prefLabel>
    </owl:Class>
    


    <!-- http://standards.iso.org/iso/10303/tech/refdata/core#dacdfd29-a895-4c18-82dd-a61924aeca84 -->

    <owl:Class rdf:about="http://standards.iso.org/iso/10303/tech/refdata/core#dacdfd29-a895-4c18-82dd-a61924aeca84">
        <rdfs:subClassOf rdf:resource="http://standards.iso.org/iso/10303/tech/refdata/core#1d59c650-3279-0135-b58f-598f1b1392ae"/>
        <dc:contributor>STEP Harmonization Team</dc:contributor>
        <dc:creator>Phil Spiby, Eurostep</dc:creator>
        <dc:date>2022-09-01</dc:date>
        <dc:source>ISO/TS 10303-4000</dc:source>
        <dc:type>InWork</dc:type>
        <rdfs:comment xml:lang="en">A TaskObjectiveStateAssociation is an association between a state (specified by StateOrStateDefinitionSelect) and a TaskObjective.</rdfs:comment>
        <owl:versionInfo>2</owl:versionInfo>
        <skos:changeNote>[2021-07-30] Initial definition.</skos:changeNote>
        <skos:changeNote>[2022-09-01] Phil Spiby, Eurostep: updated name updated comment updated note.</skos:changeNote>
        <skos:prefLabel xml:lang="en">task objective state association</skos:prefLabel>
    </owl:Class>
    


    <!-- http://standards.iso.org/iso/10303/tech/refdata/core#daf902c0-130a-0135-b552-598f1b1392ae -->

    <owl:Class rdf:about="http://standards.iso.org/iso/10303/tech/refdata/core#daf902c0-130a-0135-b552-598f1b1392ae">
        <rdfs:subClassOf rdf:resource="http://standards.iso.org/iso/10303/tech/refdata/core#1cfca290-3279-0135-b58f-598f1b1392ae"/>
        <dc:contributor>STEP Harmonization Team</dc:contributor>
        <dc:creator>Phil Spiby, Eurostep</dc:creator>
        <dc:date>2022-09-01</dc:date>
        <dc:source>ISO/TS 10303-4000</dc:source>
        <dc:type>InWork</dc:type>
        <rdfs:comment xml:lang="en">A WorkRequestAssignment is an assignment of a WorkRequest to an item (specified by WorkRequestAssignmentSelect) that is subject of this WorkRequest.</rdfs:comment>
        <owl:versionInfo>1</owl:versionInfo>
        <skos:changeNote>[2021-07-30] Initial definition.</skos:changeNote>
        <skos:prefLabel xml:lang="en">work request assignment</skos:prefLabel>
    </owl:Class>
    


    <!-- http://standards.iso.org/iso/10303/tech/refdata/core#db792f40-130a-0135-b552-598f1b1392ae -->

    <owl:Class rdf:about="http://standards.iso.org/iso/10303/tech/refdata/core#db792f40-130a-0135-b552-598f1b1392ae">
        <rdfs:subClassOf rdf:resource="http://standards.iso.org/iso/10303/tech/refdata/core#59b11220-3279-0135-b58f-598f1b1392ae"/>
        <dc:contributor>STEP Harmonization Team</dc:contributor>
        <dc:creator>Phil Spiby, Eurostep</dc:creator>
        <dc:date>2022-09-01</dc:date>
        <dc:source>ISO/TS 10303-4000</dc:source>
        <dc:type>InWork</dc:type>
        <rdfs:comment xml:lang="en">A WorkRequestRelationship is a relationship between two WorkRequest objects.</rdfs:comment>
        <owl:versionInfo>1</owl:versionInfo>
        <skos:changeNote>[2021-07-30] Initial definition.</skos:changeNote>
        <skos:prefLabel xml:lang="en">work request relationship</skos:prefLabel>
    </owl:Class>
    


    <!-- http://standards.iso.org/iso/10303/tech/refdata/core#ddc63614-f58c-4077-b81f-911e9040131b -->

    <owl:Class rdf:about="http://standards.iso.org/iso/10303/tech/refdata/core#ddc63614-f58c-4077-b81f-911e9040131b">
        <rdfs:subClassOf rdf:resource="http://standards.iso.org/iso/10303/tech/refdata/core#STEPThing"/>
        <dc:contributor>STEP Harmonization Team</dc:contributor>
        <dc:creator>Jean Brangé, AFNeT Services</dc:creator>
        <dc:date>2023-10-04</dc:date>
        <dc:source>ISO/TS 10303-4000</dc:source>
        <dc:type>InWork</dc:type>
        <rdfs:comment xml:lang="en">A MeasuredCharacteristic contains the result of measurement activity that is a set of properties resulting from an inspection of product data.</rdfs:comment>
        <owl:versionInfo>3</owl:versionInfo>
        <skos:changeNote>[2023-10-04] Jean Brangé, AFNeT Services: Initial definition.</skos:changeNote>
        <skos:note xml:lang="en">For consistency purpose between PropertyValues, the related PropertyDefinitions that are used in MeasuredCharacteristic may be the same as the ones used in PlannedCharacteristic.</skos:note>
        <skos:prefLabel xml:lang="en">measured characteristic</skos:prefLabel>
    </owl:Class>
    


    <!-- http://standards.iso.org/iso/10303/tech/refdata/core#de420483-9e8a-41af-9000-69c124abb275 -->

    <owl:Class rdf:about="http://standards.iso.org/iso/10303/tech/refdata/core#de420483-9e8a-41af-9000-69c124abb275">
        <rdfs:subClassOf rdf:resource="http://standards.iso.org/iso/10303/tech/refdata/core#STEPThing"/>
        <dc:contributor>STEP Harmonization Team</dc:contributor>
        <dc:creator>Phil Spiby, Eurostep</dc:creator>
        <dc:date>2022-09-01</dc:date>
        <dc:source>ISO/TS 10303-4000</dc:source>
        <dc:type>InWork</dc:type>
        <rdfs:comment xml:lang="en">A SecurityClassificationLevel is the definition of the level of confidentiality that is required in order to protect product data against unauthorized usage.</rdfs:comment>
        <owl:versionInfo>1</owl:versionInfo>
        <skos:changeNote>[2021-07-30] Initial definition.</skos:changeNote>
        <skos:prefLabel xml:lang="en">security classification level</skos:prefLabel>
    </owl:Class>
    


    <!-- http://standards.iso.org/iso/10303/tech/refdata/core#de7982a9-8b27-474c-8d27-21e22e629ae5 -->

    <owl:Class rdf:about="http://standards.iso.org/iso/10303/tech/refdata/core#de7982a9-8b27-474c-8d27-21e22e629ae5">
        <rdfs:subClassOf rdf:resource="http://standards.iso.org/iso/10303/tech/refdata/core#bc514af6-504d-408c-aa54-be5472451718"/>
        <dc:contributor>STEP Harmonization Team</dc:contributor>
        <dc:creator>Jean Brangé, AFNeT Services</dc:creator>
        <dc:date>2023-10-04</dc:date>
        <dc:source>ISO/TS 10303-4000</dc:source>
        <dc:type>InWork</dc:type>
        <rdfs:comment xml:lang="en">A DirectedToleranceZone is a type of ToleranceZoneWithDatum that represents an &quot;intersection plane&quot; for a geometric tolerance as defined in ISO 1101.</rdfs:comment>
        <owl:versionInfo>3</owl:versionInfo>
        <skos:changeNote>[2023-10-04] Jean Brangé, AFNeT Services: Initial definition.</skos:changeNote>
        <skos:prefLabel xml:lang="en">directed tolerance zone</skos:prefLabel>
    </owl:Class>
    


    <!-- http://standards.iso.org/iso/10303/tech/refdata/core#df8e5cf3-a71e-4765-8c69-da6a6c5aa3d4 -->

    <owl:Class rdf:about="http://standards.iso.org/iso/10303/tech/refdata/core#df8e5cf3-a71e-4765-8c69-da6a6c5aa3d4">
        <rdfs:subClassOf rdf:resource="http://standards.iso.org/iso/10303/tech/refdata/core#b608a929-7fa0-4643-8237-59c6cf4d0dbc"/>
        <dc:contributor>STEP Harmonization Team</dc:contributor>
        <dc:creator>Jean Brangé, AFNeT Services</dc:creator>
        <dc:date>2023-10-04</dc:date>
        <dc:source>ISO/TS 10303-4000</dc:source>
        <dc:type>InWork</dc:type>
        <rdfs:comment xml:lang="en">A CrossSectionalOccurrenceShapeElement is a type of OccurrenceShapeFeature that is an occurrence of a CrossSectionalPartShapeElement or of another CrossSectionalOccurrenceShapeElement.</rdfs:comment>
        <owl:versionInfo>3</owl:versionInfo>
        <skos:changeNote>[2023-10-04] Jean Brangé, AFNeT Services: Initial definition.</skos:changeNote>
        <skos:prefLabel xml:lang="en">cross sectional occurrence shape element</skos:prefLabel>
    </owl:Class>
    


    <!-- http://standards.iso.org/iso/10303/tech/refdata/core#e015fbfc-69b1-4e5a-b029-2c10d08ef7d3 -->

    <owl:Class rdf:about="http://standards.iso.org/iso/10303/tech/refdata/core#e015fbfc-69b1-4e5a-b029-2c10d08ef7d3">
        <rdfs:subClassOf rdf:resource="http://standards.iso.org/iso/10303/tech/refdata/core#1d59c650-3279-0135-b58f-598f1b1392ae"/>
        <dc:contributor>STEP Harmonization Team</dc:contributor>
        <dc:creator>Phil Spiby, Eurostep</dc:creator>
        <dc:date>2022-09-01</dc:date>
        <dc:source>ISO/TS 10303-4000</dc:source>
        <dc:type>InWork</dc:type>
        <rdfs:comment xml:lang="en">A ResourceAsRealizedAssociation is an association between the record of used or consumed resources (via ResourceAsRealized) and the corresponding item (specified by ResourceAsRealizedRelationshipSelect).</rdfs:comment>
        <owl:versionInfo>2</owl:versionInfo>
        <skos:changeNote>[2021-07-30] Initial definition.</skos:changeNote>
        <skos:changeNote>[2022-09-01] Phil Spiby, Eurostep: updated name updated comment updated example.</skos:changeNote>
        <skos:example xml:lang="en">&quot;Alternative&quot; and &quot;Corresponding&quot; are examples of classifications of resource as realized association.</skos:example>
        <skos:note xml:lang="en">A resource used or consumed can be recorded without having a corresponding resource requirement statement.</skos:note>
        <skos:prefLabel xml:lang="en">resource as realized association</skos:prefLabel>
    </owl:Class>
    


    <!-- http://standards.iso.org/iso/10303/tech/refdata/core#e0edffd2-a7ee-4c21-9830-563b91caaeae -->

    <owl:Class rdf:about="http://standards.iso.org/iso/10303/tech/refdata/core#e0edffd2-a7ee-4c21-9830-563b91caaeae">
        <rdfs:subClassOf rdf:resource="http://standards.iso.org/iso/10303/tech/refdata/core#916c16a5-5b2e-4665-bb9e-08f100ed1ee1"/>
        <dc:contributor>STEP Harmonization Team</dc:contributor>
        <dc:creator>Jean Brangé, AFNeT Services</dc:creator>
        <dc:date>2023-10-04</dc:date>
        <dc:source>ISO/TS 10303-4000</dc:source>
        <dc:type>InWork</dc:type>
        <rdfs:comment xml:lang="en">A PartTerminal is a type of PartContactFeature that can be used within an assembly as the definition of an OccurrenceTerminal that can be joined with another OccurrenceTerminal to transport information, energy or matter.</rdfs:comment>
        <owl:versionInfo>3</owl:versionInfo>
        <skos:changeNote>[2023-10-04] Jean Brangé, AFNeT Services: Initial definition.</skos:changeNote>
        <skos:prefLabel xml:lang="en">part terminal</skos:prefLabel>
    </owl:Class>
    


    <!-- http://standards.iso.org/iso/10303/tech/refdata/core#e0f93a30-a40b-4f5d-ba62-3cce94727bd0 -->

    <owl:Class rdf:about="http://standards.iso.org/iso/10303/tech/refdata/core#e0f93a30-a40b-4f5d-ba62-3cce94727bd0">
        <rdfs:subClassOf rdf:resource="http://standards.iso.org/iso/10303/tech/refdata/core#8bade30f-ae91-4520-a1bf-cfa1cca24bb7"/>
        <dc:contributor>STEP Harmonization Team</dc:contributor>
        <dc:creator>Jean Brangé, AFNeT Services</dc:creator>
        <dc:date>2023-10-04</dc:date>
        <dc:source>ISO/TS 10303-4000</dc:source>
        <dc:type>InWork</dc:type>
        <rdfs:comment xml:lang="en">A Nominal3dDerivedFeature is a type of Nominal3dFeature that represents a three-dimensional nominal derived feature.</rdfs:comment>
        <owl:versionInfo>3</owl:versionInfo>
        <skos:changeNote>[2023-10-04] Jean Brangé, AFNeT Services: Initial definition.</skos:changeNote>
        <skos:prefLabel xml:lang="en">nominal3d derived feature</skos:prefLabel>
    </owl:Class>
    


    <!-- http://standards.iso.org/iso/10303/tech/refdata/core#e1eaadb2-5cda-4f54-a4f3-61b158771dc0 -->

    <owl:Class rdf:about="http://standards.iso.org/iso/10303/tech/refdata/core#e1eaadb2-5cda-4f54-a4f3-61b158771dc0">
        <rdfs:subClassOf rdf:resource="http://standards.iso.org/iso/10303/tech/refdata/core#55105ef0-713f-409a-8306-fd8708d4ee3f"/>
        <dc:contributor>STEP Harmonization Team</dc:contributor>
        <dc:creator>Jean Brangé, AFNeT Services</dc:creator>
        <dc:date>2023-10-04</dc:date>
        <dc:source>ISO/TS 10303-4000</dc:source>
        <dc:type>InWork</dc:type>
        <rdfs:comment xml:lang="en">A ConcentricityTolerance is a type of GeometricTolerance that controls the median points of a surface of revolution relative to a datum axis. Unless otherwise specified, the rules governing concentricity tolerance defined in ISO 1101 shall apply.</rdfs:comment>
        <owl:versionInfo>3</owl:versionInfo>
        <skos:changeNote>[2023-10-04] Jean Brangé, AFNeT Services: Initial definition.</skos:changeNote>
        <skos:prefLabel xml:lang="en">concentricity tolerance</skos:prefLabel>
    </owl:Class>
    


    <!-- http://standards.iso.org/iso/10303/tech/refdata/core#e1f21c44-a15a-40d1-ac2d-e6849a953d9d -->

    <owl:Class rdf:about="http://standards.iso.org/iso/10303/tech/refdata/core#e1f21c44-a15a-40d1-ac2d-e6849a953d9d">
        <rdfs:subClassOf rdf:resource="http://standards.iso.org/iso/10303/tech/refdata/core#b3a9b996-c18c-4464-b398-d16e36d6711a"/>
        <dc:contributor>STEP Harmonization Team</dc:contributor>
        <dc:creator>Jean Brangé, AFNeT Services</dc:creator>
        <dc:date>2023-10-04</dc:date>
        <dc:source>ISO/TS 10303-4000</dc:source>
        <dc:type>InWork</dc:type>
        <rdfs:comment xml:lang="en">A CompositeSheetRepresentation is a type of ConstituentShapeRepresentation that defines a sheet product. A sheet product is a product whose thickness is constant and small in comparison to its length and width. Most sheet products will conform to the surface on which they are placed. The shape of a sheet product can be represented in a 3-dimensional model of the actual shape, as a shape projected onto the layup surface, or as a shape projected into a 2-dimensional plane. A CompositeSheetRepresentation may be one of the following: FaceBasedSheetRepresentation, GeometricSheetRepresentation.</rdfs:comment>
        <owl:versionInfo>3</owl:versionInfo>
        <skos:changeNote>[2023-10-04] Jean Brangé, AFNeT Services: Initial definition.</skos:changeNote>
        <skos:example xml:lang="en">A typical composite sheet is 0.1 to 0.4 millimeters thick while its length and width are much greater than 25 millimeters.</skos:example>
        <skos:prefLabel xml:lang="en">composite sheet representation</skos:prefLabel>
    </owl:Class>
    


    <!-- http://standards.iso.org/iso/10303/tech/refdata/core#e1f8b9c7-1852-4af6-96cf-c0179fd859ac -->

    <owl:Class rdf:about="http://standards.iso.org/iso/10303/tech/refdata/core#e1f8b9c7-1852-4af6-96cf-c0179fd859ac">
        <rdfs:subClassOf rdf:resource="http://standards.iso.org/iso/10303/tech/refdata/core#6d367e10-7640-4a8f-acaa-42963438a3aa"/>
        <dc:contributor>STEP Harmonization Team</dc:contributor>
        <dc:creator>Jean Brangé, AFNeT Services</dc:creator>
        <dc:date>2023-10-04</dc:date>
        <dc:source>ISO/TS 10303-4000</dc:source>
        <dc:type>InWork</dc:type>
        <rdfs:comment xml:lang="en">A LaidOrientationAngle is a type of PlyOrientationAngle that explicitly defines a direction at a point within a ply.</rdfs:comment>
        <owl:versionInfo>3</owl:versionInfo>
        <skos:changeNote>[2023-10-04] Jean Brangé, AFNeT Services: Initial definition.</skos:changeNote>
        <skos:prefLabel xml:lang="en">laid orientation angle</skos:prefLabel>
    </owl:Class>
    


    <!-- http://standards.iso.org/iso/10303/tech/refdata/core#e42749c0-63c3-455d-9a5d-d7624a4a242c -->

    <owl:Class rdf:about="http://standards.iso.org/iso/10303/tech/refdata/core#e42749c0-63c3-455d-9a5d-d7624a4a242c">
        <rdfs:subClassOf rdf:resource="http://standards.iso.org/iso/10303/tech/refdata/core#d36456e7-f236-4965-a037-486dd8ab90b9"/>
        <dc:contributor>STEP Harmonization Team</dc:contributor>
        <dc:creator>Phil Spiby, Eurostep</dc:creator>
        <dc:date>2022-09-01</dc:date>
        <dc:source>ISO/TS 10303-4000</dc:source>
        <dc:type>InWork</dc:type>
        <rdfs:comment xml:lang="en">A ParameterizedDistribution is a specialization of ProbabilityDistribution that is used to link a named probability distribution to the parameters that define it.</rdfs:comment>
        <owl:versionInfo>1</owl:versionInfo>
        <skos:changeNote>[2022-09-01] Initial definition.</skos:changeNote>
        <skos:note xml:lang="en">The ParameterizationName of this entity is used to discriminate between alternative parameterizations of the same distribution.</skos:note>
        <skos:note xml:lang="en">To calculate a value using a ParameterizedDistribution it is necessary to know the general distribution function, the value of the distribution function parameters, and the specific random variable value for which the probability evaluation is required. The ProbabilityDistribution module does not define the formula for the distribution function, and it is assumed that this is defined externally, either through reference information or via a &quot;formula&quot; module. This entity provides the distribution function parameters.</skos:note>
        <skos:prefLabel xml:lang="en">parameterized distribution</skos:prefLabel>
    </owl:Class>
    


    <!-- http://standards.iso.org/iso/10303/tech/refdata/core#e5d2a0ed-ae68-4834-87eb-5068649e7e5d -->

    <owl:Class rdf:about="http://standards.iso.org/iso/10303/tech/refdata/core#e5d2a0ed-ae68-4834-87eb-5068649e7e5d">
        <rdfs:subClassOf rdf:resource="http://standards.iso.org/iso/10303/tech/refdata/core#STEPThing"/>
        <dc:contributor>STEP Harmonization Team</dc:contributor>
        <dc:creator>Phil Spiby, Eurostep</dc:creator>
        <dc:date>2022-09-01</dc:date>
        <dc:source>ISO/TS 10303-4000</dc:source>
        <dc:type>InWork</dc:type>
        <rdfs:comment xml:lang="en">An AnalysisVersion identifies a specific version of an Analysis.</rdfs:comment>
        <owl:versionInfo>1</owl:versionInfo>
        <skos:changeNote>[2021-07-30] Initial definition.</skos:changeNote>
        <skos:prefLabel xml:lang="en">analysis version</skos:prefLabel>
    </owl:Class>
    


    <!-- http://standards.iso.org/iso/10303/tech/refdata/core#e994e337-4b09-41ab-bcfa-cd53c96d9198 -->

    <owl:Class rdf:about="http://standards.iso.org/iso/10303/tech/refdata/core#e994e337-4b09-41ab-bcfa-cd53c96d9198">
        <rdfs:subClassOf rdf:resource="http://standards.iso.org/iso/10303/tech/refdata/core#STEPThing"/>
        <dc:contributor>STEP Harmonization Team</dc:contributor>
        <dc:creator>Phil Spiby, Eurostep</dc:creator>
        <dc:date>2022-09-01</dc:date>
        <dc:source>ISO/TS 10303-4000</dc:source>
        <dc:type>InWork</dc:type>
        <rdfs:comment xml:lang="en">An ExperienceInstance is a particular episode of contact with and/or observation of facts or events which contributes to the accumulation of knowledge or skill. The nature, duration and worth of the ExperienceInstance can be described using assigned properties or by referring to activities or tasks.</rdfs:comment>
        <owl:versionInfo>1</owl:versionInfo>
        <skos:changeNote>[2022-09-01] Initial definition.</skos:changeNote>
        <skos:example xml:lang="en">100 flying hours in a Tornado jet.</skos:example>
        <skos:example xml:lang="en">2 years work on same type of milling machine.</skos:example>
        <skos:example xml:lang="en">5 years as Workshop Manager.</skos:example>
        <skos:example xml:lang="en">Changing the exhaust system on a car.</skos:example>
        <skos:prefLabel xml:lang="en">experience instance</skos:prefLabel>
    </owl:Class>
    


    <!-- http://standards.iso.org/iso/10303/tech/refdata/core#ea4fdce2-e3af-4863-80a6-3e4ee552487b -->

    <owl:Class rdf:about="http://standards.iso.org/iso/10303/tech/refdata/core#ea4fdce2-e3af-4863-80a6-3e4ee552487b">
        <rdfs:subClassOf rdf:resource="http://standards.iso.org/iso/10303/tech/refdata/core#1cfca290-3279-0135-b58f-598f1b1392ae"/>
        <dc:contributor>STEP Harmonization Team</dc:contributor>
        <dc:creator>Phil Spiby, Eurostep</dc:creator>
        <dc:date>2022-09-01</dc:date>
        <dc:source>ISO/TS 10303-4000</dc:source>
        <dc:type>InWork</dc:type>
        <rdfs:comment xml:lang="en">A JustificationSupportAssignment is the assignment of an item (specified by JustificationSupportAssignmentSelect) providing evidential support to a Justification. The meaning of the assignment can be specified using the ClassifiedAs attribute inherited from the AssignmentObject.</rdfs:comment>
        <owl:versionInfo>2</owl:versionInfo>
        <skos:changeNote>[2021-07-30] Initial definition.</skos:changeNote>
        <skos:changeNote>[2022-09-01] Phil Spiby, Eurostep: updated comment updated example updated note.</skos:changeNote>
        <skos:note xml:lang="en">The support item can be the results from an analysis, a report, or professional judgement.</skos:note>
        <skos:prefLabel xml:lang="en">justification support assignment</skos:prefLabel>
    </owl:Class>
    


    <!-- http://standards.iso.org/iso/10303/tech/refdata/core#eb06428d-80d2-4f6c-ae8d-a2a54935418f -->

    <owl:Class rdf:about="http://standards.iso.org/iso/10303/tech/refdata/core#eb06428d-80d2-4f6c-ae8d-a2a54935418f">
        <rdfs:subClassOf rdf:resource="http://standards.iso.org/iso/10303/tech/refdata/core#84099bf0-130a-0135-b552-598f1b1392ae"/>
        <dc:contributor>STEP Harmonization Team</dc:contributor>
        <dc:creator>Phil Spiby, Eurostep</dc:creator>
        <dc:date>2022-09-01</dc:date>
        <dc:source>ISO/TS 10303-4000</dc:source>
        <dc:type>InWork</dc:type>
        <rdfs:comment xml:lang="en">A SchemeRelationship is a specialization of ActivityMethodRelationship that is a relationship between two Scheme objects.</rdfs:comment>
        <owl:versionInfo>1</owl:versionInfo>
        <skos:changeNote>[2022-09-01] Initial definition.</skos:changeNote>
        <skos:example xml:lang="en">Decomposition, based-on, alternative, and version are different kinds of relationships between Schemes.</skos:example>
        <skos:note xml:lang="en">The SchemeRelationship provides the facility to relate Plans or Schedules, represented by the Scheme entity, in different ways. Classifications can be applied to different SchemeRelationships to indicate their use for different purposes.</skos:note>
        <skos:prefLabel xml:lang="en">scheme relationship</skos:prefLabel>
    </owl:Class>
    


    <!-- http://standards.iso.org/iso/10303/tech/refdata/core#eb0f45bb-2991-485b-bfe5-44f8c83f3ab4 -->

    <owl:Class rdf:about="http://standards.iso.org/iso/10303/tech/refdata/core#eb0f45bb-2991-485b-bfe5-44f8c83f3ab4">
        <rdfs:subClassOf rdf:resource="http://standards.iso.org/iso/10303/tech/refdata/core#STEPThing"/>
        <dc:contributor>STEP Harmonization Team</dc:contributor>
        <dc:creator>Phil Spiby, Eurostep</dc:creator>
        <dc:date>2022-09-01</dc:date>
        <dc:source>ISO/TS 10303-4000</dc:source>
        <dc:type>InWork</dc:type>
        <rdfs:comment xml:lang="en">An Evidence is a collector of items used together to provide a single piece of evidence within a validation or verification.</rdfs:comment>
        <owl:versionInfo>2</owl:versionInfo>
        <skos:changeNote>[2021-07-30] Initial definition.</skos:changeNote>
        <skos:changeNote>[2022-09-01] Phil Spiby, Eurostep: updated example.</skos:changeNote>
        <skos:example xml:lang="en">A document and its approval by a customer can be used together to provide evidence of customer acceptance.</skos:example>
        <skos:prefLabel xml:lang="en">evidence</skos:prefLabel>
    </owl:Class>
    


    <!-- http://standards.iso.org/iso/10303/tech/refdata/core#eb56a499-cc28-42ce-9587-922e784def59 -->

    <owl:Class rdf:about="http://standards.iso.org/iso/10303/tech/refdata/core#eb56a499-cc28-42ce-9587-922e784def59">
        <rdfs:subClassOf rdf:resource="http://standards.iso.org/iso/10303/tech/refdata/core#1d59c650-3279-0135-b58f-598f1b1392ae"/>
        <dc:contributor>STEP Harmonization Team</dc:contributor>
        <dc:creator>Phil Spiby, Eurostep</dc:creator>
        <dc:date>2022-09-01</dc:date>
        <dc:source>ISO/TS 10303-4000</dc:source>
        <dc:type>InWork</dc:type>
        <rdfs:comment xml:lang="en">A CollectionMembership is an association of a CollectionView with an item (specified in CollectionMemberSelect) that represents a member of the collection.</rdfs:comment>
        <owl:versionInfo>1</owl:versionInfo>
        <skos:changeNote>[2021-07-30] Initial definition.</skos:changeNote>
        <skos:prefLabel xml:lang="en">collection membership</skos:prefLabel>
    </owl:Class>
    


    <!-- http://standards.iso.org/iso/10303/tech/refdata/core#ebae0a39-680a-4dcd-a4aa-20966bec83b1 -->

    <owl:Class rdf:about="http://standards.iso.org/iso/10303/tech/refdata/core#ebae0a39-680a-4dcd-a4aa-20966bec83b1">
        <rdfs:subClassOf rdf:resource="http://standards.iso.org/iso/10303/tech/refdata/core#9f656069-ff2c-4f09-9091-f91388a14764"/>
        <dc:contributor>STEP Harmonization Team</dc:contributor>
        <dc:creator>Phil Spiby, Eurostep</dc:creator>
        <dc:date>2022-09-01</dc:date>
        <dc:source>ISO/TS 10303-4000</dc:source>
        <dc:type>InWork</dc:type>
        <rdfs:comment xml:lang="en">A StatePredictedToObserved is a type of StateRelationship that specifies the relationship between two individual states, one of which is a StatePredicted object and the second being a StateObserved object.</rdfs:comment>
        <owl:versionInfo>2</owl:versionInfo>
        <skos:changeNote>[2021-07-30] Initial definition.</skos:changeNote>
        <skos:changeNote>[2022-09-01] Phil Spiby, Eurostep: updated comment.</skos:changeNote>
        <skos:prefLabel xml:lang="en">state predicted to observed</skos:prefLabel>
    </owl:Class>
    


    <!-- http://standards.iso.org/iso/10303/tech/refdata/core#ebfe951f-2c73-4af3-8c62-d32172b6146c -->

    <owl:Class rdf:about="http://standards.iso.org/iso/10303/tech/refdata/core#ebfe951f-2c73-4af3-8c62-d32172b6146c">
        <rdfs:subClassOf rdf:resource="http://standards.iso.org/iso/10303/tech/refdata/core#70fd2ab8-bdcb-481c-8096-ca0246ed15c5"/>
        <dc:contributor>STEP Harmonization Team</dc:contributor>
        <dc:creator>Phil Spiby, Eurostep</dc:creator>
        <dc:date>2022-09-01</dc:date>
        <dc:source>ISO/TS 10303-4000</dc:source>
        <dc:type>InWork</dc:type>
        <rdfs:comment xml:lang="en">A SlotAsPlanned is a specialization of SlotVersion that identifies an individual that is the subject of a plan to realize a Slot.</rdfs:comment>
        <owl:versionInfo>1</owl:versionInfo>
        <skos:changeNote>[2022-09-01] Initial definition.</skos:changeNote>
        <skos:example xml:lang="en">FlyFasterWithUs Group will buy an aircraft with serial number 1234 next year. The company wishes to plan the schedule for removal of engines from the aircraft for maintenance purposes. Instances of the SlotAsPlanned entity data type allow the company to associate individual engines with the aircraft at different times over the planned period.</skos:example>
        <skos:prefLabel xml:lang="en">slot as planned</skos:prefLabel>
    </owl:Class>
    


    <!-- http://standards.iso.org/iso/10303/tech/refdata/core#ec56a938-cbd8-4fac-ba97-4d9b7ecc6442 -->

    <owl:Class rdf:about="http://standards.iso.org/iso/10303/tech/refdata/core#ec56a938-cbd8-4fac-ba97-4d9b7ecc6442">
        <rdfs:subClassOf rdf:resource="http://standards.iso.org/iso/10303/tech/refdata/core#9fee6ad0-130a-0135-b552-598f1b1392ae"/>
        <dc:contributor>STEP Harmonization Team</dc:contributor>
        <dc:creator>Jean Brangé, AFNeT Services</dc:creator>
        <dc:date>2023-10-04</dc:date>
        <dc:source>ISO/TS 10303-4000</dc:source>
        <dc:type>InWork</dc:type>
        <rdfs:comment xml:lang="en">A KinematicLink is a type of GeometricRepresentation of a rigid part of a Mechanism.</rdfs:comment>
        <owl:versionInfo>3</owl:versionInfo>
        <skos:changeNote>[2023-10-04] Jean Brangé, AFNeT Services: Initial definition.</skos:changeNote>
        <skos:prefLabel xml:lang="en">kinematic link</skos:prefLabel>
    </owl:Class>
    


    <!-- http://standards.iso.org/iso/10303/tech/refdata/core#ecd160a3-77c1-4c06-8d69-0589708c3a49 -->

    <owl:Class rdf:about="http://standards.iso.org/iso/10303/tech/refdata/core#ecd160a3-77c1-4c06-8d69-0589708c3a49">
        <rdfs:subClassOf rdf:resource="http://standards.iso.org/iso/10303/tech/refdata/core#9c98fe40-130a-0135-b552-598f1b1392ae"/>
        <dc:contributor>STEP Harmonization Team</dc:contributor>
        <dc:creator>Jean Brangé, AFNeT Services</dc:creator>
        <dc:date>2023-10-04</dc:date>
        <dc:source>ISO/TS 10303-4000</dc:source>
        <dc:type>InWork</dc:type>
        <rdfs:comment xml:lang="en">An ExternalTessellatedShapeRepresentation is a type of ExternalGeometricModel that references an instance of type ../../../resources/geometry_schema/geometry_schema.htm#geometry_schema.surface_curve surface_curve (ISO 10303-42).</rdfs:comment>
        <owl:versionInfo>3</owl:versionInfo>
        <skos:changeNote>[2023-10-04] Jean Brangé, AFNeT Services: Initial definition.</skos:changeNote>
        <skos:prefLabel xml:lang="en">external tessellated shape representation</skos:prefLabel>
    </owl:Class>
    


    <!-- http://standards.iso.org/iso/10303/tech/refdata/core#eea929c3-0513-412f-bbc4-e8c25a64efe9 -->

    <owl:Class rdf:about="http://standards.iso.org/iso/10303/tech/refdata/core#eea929c3-0513-412f-bbc4-e8c25a64efe9">
        <rdfs:subClassOf rdf:resource="http://standards.iso.org/iso/10303/tech/refdata/core#1cfca290-3279-0135-b58f-598f1b1392ae"/>
        <dc:contributor>STEP Harmonization Team</dc:contributor>
        <dc:creator>Phil Spiby, Eurostep</dc:creator>
        <dc:date>2022-09-01</dc:date>
        <dc:source>ISO/TS 10303-4000</dc:source>
        <dc:type>InWork</dc:type>
        <rdfs:comment xml:lang="en">An AssumptionAssignment is an assignment of an Assumption to an item (specified by AssumptionAssignmentSelect). The meaning of the assignment can be specified using the ClassifiedAs attribute inherited from the AssignmentObject.</rdfs:comment>
        <owl:versionInfo>2</owl:versionInfo>
        <skos:changeNote>[2021-07-30] Initial definition.</skos:changeNote>
        <skos:changeNote>[2022-09-01] Phil Spiby, Eurostep: updated comment.</skos:changeNote>
        <skos:example xml:lang="en">The following set of assumptions are relevant to the project.</skos:example>
        <skos:prefLabel xml:lang="en">assumption assignment</skos:prefLabel>
    </owl:Class>
    


    <!-- http://standards.iso.org/iso/10303/tech/refdata/core#ef32e7b5-d45e-46cf-a64a-8e60bb3c36f0 -->

    <owl:Class rdf:about="http://standards.iso.org/iso/10303/tech/refdata/core#ef32e7b5-d45e-46cf-a64a-8e60bb3c36f0">
        <rdfs:subClassOf rdf:resource="http://standards.iso.org/iso/10303/tech/refdata/core#59b11220-3279-0135-b58f-598f1b1392ae"/>
        <dc:contributor>STEP Harmonization Team</dc:contributor>
        <dc:creator>Phil Spiby, Eurostep</dc:creator>
        <dc:date>2022-09-01</dc:date>
        <dc:source>ISO/TS 10303-4000</dc:source>
        <dc:type>InWork</dc:type>
        <rdfs:comment xml:lang="en">An InterfaceSpecificationViewRelationship is a relationship between two InterfaceSpecificationView objects.</rdfs:comment>
        <owl:versionInfo>2</owl:versionInfo>
        <skos:changeNote>[2021-07-30] Initial definition.</skos:changeNote>
        <skos:changeNote>[2022-09-01] Phil Spiby, Eurostep: updated comment.</skos:changeNote>
        <skos:prefLabel xml:lang="en">interface specification view relationship</skos:prefLabel>
    </owl:Class>
    


    <!-- http://standards.iso.org/iso/10303/tech/refdata/core#ef463eb2-567e-4f5f-8437-2dbe3d82745c -->

    <owl:Class rdf:about="http://standards.iso.org/iso/10303/tech/refdata/core#ef463eb2-567e-4f5f-8437-2dbe3d82745c">
        <rdfs:subClassOf rdf:resource="http://standards.iso.org/iso/10303/tech/refdata/core#STEPThing"/>
        <dc:contributor>STEP Harmonization Team</dc:contributor>
        <dc:creator>Phil Spiby, Eurostep</dc:creator>
        <dc:date>2022-09-01</dc:date>
        <dc:source>ISO/TS 10303-4000</dc:source>
        <dc:type>InWork</dc:type>
        <rdfs:comment xml:lang="en">An EnvironmentView is a view of an Environment with respect to specific criteria. This is an abstract object which specializations are EnvironmentDefinitionView and ObservedEnvironmentView.</rdfs:comment>
        <owl:versionInfo>1</owl:versionInfo>
        <skos:changeNote>[2021-07-30] Initial definition.</skos:changeNote>
        <skos:prefLabel xml:lang="en">environment view</skos:prefLabel>
    </owl:Class>
    


    <!-- http://standards.iso.org/iso/10303/tech/refdata/core#f0e37d16-4d8a-480c-96dd-992edd12ea38 -->

    <owl:Class rdf:about="http://standards.iso.org/iso/10303/tech/refdata/core#f0e37d16-4d8a-480c-96dd-992edd12ea38">
        <rdfs:subClassOf rdf:resource="http://standards.iso.org/iso/10303/tech/refdata/core#68242b94-82e8-4841-8005-89981113e22f"/>
        <dc:contributor>STEP Harmonization Team</dc:contributor>
        <dc:creator>Phil Spiby, Eurostep</dc:creator>
        <dc:date>2022-09-01</dc:date>
        <dc:source>ISO/TS 10303-4000</dc:source>
        <dc:type>InWork</dc:type>
        <rdfs:comment xml:lang="en">A RegionalGrid is a type of Locator specified through a reference grid system.</rdfs:comment>
        <owl:versionInfo>1</owl:versionInfo>
        <skos:changeNote>[2021-07-30] Initial definition.</skos:changeNote>
        <skos:prefLabel xml:lang="en">regional grid</skos:prefLabel>
    </owl:Class>
    


    <!-- http://standards.iso.org/iso/10303/tech/refdata/core#f1034041-1281-47e5-9a35-fcb72c591545 -->

    <owl:Class rdf:about="http://standards.iso.org/iso/10303/tech/refdata/core#f1034041-1281-47e5-9a35-fcb72c591545">
        <rdfs:subClassOf rdf:resource="http://standards.iso.org/iso/10303/tech/refdata/core#b44098a0-130a-0135-b552-598f1b1392ae"/>
        <dc:contributor>STEP Harmonization Team</dc:contributor>
        <dc:creator>Jean Brangé, AFNeT Services</dc:creator>
        <dc:date>2023-10-04</dc:date>
        <dc:source>ISO/TS 10303-4000</dc:source>
        <dc:type>InWork</dc:type>
        <rdfs:comment xml:lang="en">A MakeFromRelationship is a type of PartViewRelationship that is a relationship between a PartView which provides the definition of a raw material, or of a semi-finished part and a PartView which provides the definition of an object manufactured out of that material, or semi-finished part. The inherited attribute Related specifies the raw material or the semi-finished part, and the inherited attribute Relating specifies the manufactured part.</rdfs:comment>
        <owl:versionInfo>3</owl:versionInfo>
        <skos:changeNote>[2023-10-04] Jean Brangé, AFNeT Services: Initial definition.</skos:changeNote>
        <skos:prefLabel xml:lang="en">make from relationship</skos:prefLabel>
    </owl:Class>
    


    <!-- http://standards.iso.org/iso/10303/tech/refdata/core#f1c8c663-e95e-4f73-bfbe-a25d33889fde -->

    <owl:Class rdf:about="http://standards.iso.org/iso/10303/tech/refdata/core#f1c8c663-e95e-4f73-bfbe-a25d33889fde">
        <rdfs:subClassOf rdf:resource="http://standards.iso.org/iso/10303/tech/refdata/core#1cfca290-3279-0135-b58f-598f1b1392ae"/>
        <dc:contributor>STEP Harmonization Team</dc:contributor>
        <dc:creator>Phil Spiby, Eurostep</dc:creator>
        <dc:date>2022-09-01</dc:date>
        <dc:source>ISO/TS 10303-4000</dc:source>
        <dc:type>InWork</dc:type>
        <rdfs:comment xml:lang="en">A ConditionEvaluationAssignment is an assignment of a ConditionEvaluation to an item (specified by ConditionEvaluationAssignmentSelect).</rdfs:comment>
        <owl:versionInfo>1</owl:versionInfo>
        <skos:changeNote>[2021-07-30] Initial definition.</skos:changeNote>
        <skos:prefLabel xml:lang="en">condition evaluation assignment</skos:prefLabel>
    </owl:Class>
    


    <!-- http://standards.iso.org/iso/10303/tech/refdata/core#f2636078-e46f-4dbe-b95e-f10e9c9b8a3b -->

    <owl:Class rdf:about="http://standards.iso.org/iso/10303/tech/refdata/core#f2636078-e46f-4dbe-b95e-f10e9c9b8a3b">
        <rdfs:subClassOf rdf:resource="http://standards.iso.org/iso/10303/tech/refdata/core#1d59c650-3279-0135-b58f-598f1b1392ae"/>
        <dc:contributor>STEP Harmonization Team</dc:contributor>
        <dc:creator>Phil Spiby, Eurostep</dc:creator>
        <dc:date>2022-09-01</dc:date>
        <dc:source>ISO/TS 10303-4000</dc:source>
        <dc:type>InWork</dc:type>
        <rdfs:comment xml:lang="en">An ObservedEnvironmentToDefinitionVersion is an association between a version of the record of a set of observations about an environment, represented by an ObservedEnvironmentVersion, and a version of the typical environment, represented by EnvironmentDefinitionVersion. The typical environment is the expected environment about which observations have been made.</rdfs:comment>
        <owl:versionInfo>2</owl:versionInfo>
        <skos:changeNote>[2021-07-30] Initial definition.</skos:changeNote>
        <skos:changeNote>[2022-09-01] Phil Spiby, Eurostep: updated comment.</skos:changeNote>
        <skos:prefLabel xml:lang="en">observed environment to definition version</skos:prefLabel>
    </owl:Class>
    


    <!-- http://standards.iso.org/iso/10303/tech/refdata/core#f296399e-0f80-473d-8f8d-41de9232ec54 -->

    <owl:Class rdf:about="http://standards.iso.org/iso/10303/tech/refdata/core#f296399e-0f80-473d-8f8d-41de9232ec54">
        <rdfs:subClassOf rdf:resource="http://standards.iso.org/iso/10303/tech/refdata/core#cca6c810-130a-0135-b552-598f1b1392ae"/>
        <dc:contributor>STEP Harmonization Team</dc:contributor>
        <dc:creator>Jean Brangé, AFNeT Services</dc:creator>
        <dc:date>2023-10-04</dc:date>
        <dc:source>ISO/TS 10303-4000</dc:source>
        <dc:type>InWork</dc:type>
        <rdfs:comment xml:lang="en">A BoundingBox is a type of ShapeDependentProperty that is the bounding box of the shape, or of a portion of the shape of an object. The bounding box is a mean of providing information about a part extent and location. The bounding box is a characteristic of a part, not its shape. The box is aligned with the 3 axis of the GeometricCoordinateSpace associated to the property. As a consequence, each coordinate (X,Y,Z) of the 8 points of the box can have only two values: X coordinate can be either Xmin or Xmax. Y coordinate can be either Ymin or Ymax. Z coordinate can be either Zmin or Zmax. The bounding box is defined by the two opposite corner points: (Xmin, Ymin, Zmin) and (Xmax, Ymax, Zmax)</rdfs:comment>
        <owl:versionInfo>3</owl:versionInfo>
        <skos:changeNote>[2023-10-04] Jean Brangé, AFNeT Services: Initial definition.</skos:changeNote>
        <skos:note xml:lang="en">If a shape representation is present, the BoundingBox is usually derivable from the shape representation. However, as a characteristic of a part, it may be predefined in order to reflect a requirement.</skos:note>
        <skos:prefLabel xml:lang="en">bounding box</skos:prefLabel>
    </owl:Class>
    


    <!-- http://standards.iso.org/iso/10303/tech/refdata/core#f2b4085a-9185-4774-b4e4-4bf0366190d6 -->

    <owl:Class rdf:about="http://standards.iso.org/iso/10303/tech/refdata/core#f2b4085a-9185-4774-b4e4-4bf0366190d6">
        <rdfs:subClassOf rdf:resource="http://standards.iso.org/iso/10303/tech/refdata/core#1d59c650-3279-0135-b58f-598f1b1392ae"/>
        <dc:contributor>STEP Harmonization Team</dc:contributor>
        <dc:creator>Phil Spiby, Eurostep</dc:creator>
        <dc:date>2022-09-01</dc:date>
        <dc:source>ISO/TS 10303-4000</dc:source>
        <dc:type>InWork</dc:type>
        <rdfs:comment xml:lang="en">An ItemInSlot is an association between a Slot and an item that connects on this Slot. The purpose is to be able to keep record of what can be or is connected in a particular slot.</rdfs:comment>
        <owl:versionInfo>1</owl:versionInfo>
        <skos:changeNote>[2022-09-01] Initial definition.</skos:changeNote>
        <skos:prefLabel xml:lang="en">item in slot</skos:prefLabel>
    </owl:Class>
    


    <!-- http://standards.iso.org/iso/10303/tech/refdata/core#f2cd6fea-7dcf-49f6-9f82-0ff9e4271374 -->

    <owl:Class rdf:about="http://standards.iso.org/iso/10303/tech/refdata/core#f2cd6fea-7dcf-49f6-9f82-0ff9e4271374">
        <rdfs:subClassOf rdf:resource="http://standards.iso.org/iso/10303/tech/refdata/core#44078e31-a1cb-4d89-b8d6-ab60b9140b06"/>
        <dc:contributor>STEP Harmonization Team</dc:contributor>
        <dc:creator>Jean Brangé, AFNeT Services</dc:creator>
        <dc:date>2023-10-04</dc:date>
        <dc:source>ISO/TS 10303-4000</dc:source>
        <dc:type>InWork</dc:type>
        <rdfs:comment xml:lang="en">A TargetCircle is a type of PlacedTarget that specifies a DatumTarget that is defined by an implicit circle. The DatumTarget may be the area inside the circle or the circle, depending on the geometry. The centre of the circle is specified by the placing AxisPlacement. The orientation of the TargetCircle is the x-y-plane of the AxisPlacement.</rdfs:comment>
        <owl:versionInfo>3</owl:versionInfo>
        <skos:changeNote>[2023-10-04] Jean Brangé, AFNeT Services: Initial definition.</skos:changeNote>
        <skos:prefLabel xml:lang="en">target circle</skos:prefLabel>
    </owl:Class>
    


    <!-- http://standards.iso.org/iso/10303/tech/refdata/core#f328b255-6ee9-441c-9d28-b1e998e9599e -->

    <owl:Class rdf:about="http://standards.iso.org/iso/10303/tech/refdata/core#f328b255-6ee9-441c-9d28-b1e998e9599e">
        <rdfs:subClassOf rdf:resource="http://standards.iso.org/iso/10303/tech/refdata/core#STEPThing"/>
        <dc:contributor>STEP Harmonization Team</dc:contributor>
        <dc:creator>Jean Brangé, AFNeT Services</dc:creator>
        <dc:date>2023-10-04</dc:date>
        <dc:source>ISO/TS 10303-4000</dc:source>
        <dc:type>InWork</dc:type>
        <rdfs:comment xml:lang="en">A ProcessOperationDefinition is a specification of an activity that may be included in a ProcessPlan. A ProcessOperationDefinition characterizes a manufacturing or control operation.</rdfs:comment>
        <owl:versionInfo>3</owl:versionInfo>
        <skos:changeNote>[2023-10-04] Jean Brangé, AFNeT Services: Initial definition.</skos:changeNote>
        <skos:note xml:lang="en">In the case where an instance of ProcessOperationDefinition is associated with two application object such as Organization with a location, a context independent one and a context dependent one, the two locations need not be the same, but should be related in a way that the context dependent location should be a specialization of the context independent location such as a specific assembly line in a plant.</skos:note>
        <skos:note xml:lang="en">ProcessOperationDefinition as well as ProcessOperationOccurrence may be associated with organizational data using an assignment such as OrganizationOrPersonInOrganizationAssignment. The reason for having these data available for both types of objects is the requirement to associate ProcessOperationDefinition with organizational data in both a context independent and a context dependent way (the context is a specific ProcessPlan).</skos:note>
        <skos:prefLabel xml:lang="en">process operation definition</skos:prefLabel>
    </owl:Class>
    


    <!-- http://standards.iso.org/iso/10303/tech/refdata/core#f3604d84-2410-43cb-8c78-4807f88dbbfb -->

    <owl:Class rdf:about="http://standards.iso.org/iso/10303/tech/refdata/core#f3604d84-2410-43cb-8c78-4807f88dbbfb">
        <rdfs:subClassOf rdf:resource="http://standards.iso.org/iso/10303/tech/refdata/core#STEPThing"/>
        <dc:contributor>STEP Harmonization Team</dc:contributor>
        <dc:creator>Phil Spiby, Eurostep</dc:creator>
        <dc:date>2022-09-01</dc:date>
        <dc:source>ISO/TS 10303-4000</dc:source>
        <dc:type>InWork</dc:type>
        <rdfs:comment xml:lang="en">A ProductGroup identifies a set of IndividualPart, Part, PartVersion, ProductConcept, ProductGroup, System or SystemVersion that have been grouped together.</rdfs:comment>
        <owl:versionInfo>1</owl:versionInfo>
        <skos:changeNote>[2022-09-01] Initial definition.</skos:changeNote>
        <skos:prefLabel xml:lang="en">product group</skos:prefLabel>
    </owl:Class>
    


    <!-- http://standards.iso.org/iso/10303/tech/refdata/core#f3d14334-d3af-4708-b5af-10232566e2db -->

    <owl:Class rdf:about="http://standards.iso.org/iso/10303/tech/refdata/core#f3d14334-d3af-4708-b5af-10232566e2db">
        <rdfs:subClassOf rdf:resource="http://standards.iso.org/iso/10303/tech/refdata/core#STEPThing"/>
        <dc:contributor>STEP Harmonization Team</dc:contributor>
        <dc:creator>Jean Brangé, AFNeT Services</dc:creator>
        <dc:date>2023-10-04</dc:date>
        <dc:source>ISO/TS 10303-4000</dc:source>
        <dc:type>InWork</dc:type>
        <rdfs:comment xml:lang="en">An EvaluatedCharacteristic is a set of properties resulting from an evaluation or intended evaluation of product data. An EvaluatedCharacteristic object associates evaluation data with one or several PlannedCharacteristic objects for the purposes of traceability.</rdfs:comment>
        <owl:versionInfo>3</owl:versionInfo>
        <skos:changeNote>[2023-10-04] Jean Brangé, AFNeT Services: Initial definition.</skos:changeNote>
        <skos:prefLabel xml:lang="en">evaluated characteristic</skos:prefLabel>
    </owl:Class>
    


    <!-- http://standards.iso.org/iso/10303/tech/refdata/core#f5acf4c6-2654-4ef1-abc2-93e0ea5529d5 -->

    <owl:Class rdf:about="http://standards.iso.org/iso/10303/tech/refdata/core#f5acf4c6-2654-4ef1-abc2-93e0ea5529d5">
        <rdfs:subClassOf rdf:resource="http://standards.iso.org/iso/10303/tech/refdata/core#6d4d4ccd-20d2-4209-9fe6-17da7b3cb1a1"/>
        <dc:contributor>STEP Harmonization Team</dc:contributor>
        <dc:creator>Jean Brangé, AFNeT Services</dc:creator>
        <dc:date>2023-10-04</dc:date>
        <dc:source>ISO/TS 10303-4000</dc:source>
        <dc:type>InWork</dc:type>
        <rdfs:comment xml:lang="en">A ZoneStructuralMakeup is a type of LaminateTable that describes the structural makeup of a specific zone, area, or point within a laminate. A ZoneStructuralMakeup may be either a ThicknessLaminateTable and a SmearedMaterial, or a PercentageLaminateTable and a SmearedMaterial, or a ThicknessLaminateTable or a PercentageLaminateTable or a SmearedMaterial.</rdfs:comment>
        <owl:versionInfo>3</owl:versionInfo>
        <skos:changeNote>[2023-10-04] Jean Brangé, AFNeT Services: Initial definition.</skos:changeNote>
        <skos:note xml:lang="en">A single ZoneStructuralMakeup could apply to the whole part. The would be the case for a homogeneous structural part or a simple laminate of constant thickness and material constituents.</skos:note>
        <skos:note xml:lang="en">Structural makeup information consists of: 1) the smear material properties based on one or more constituents that reside in that zone or point; 2) the percentage of the total thickness within a zone or point that each constituent type makes up; and 3) the ordered list of physical constituents based on position within a zone or point. These three pieces of structural makeup information can coexist in any order to describe a zone or point within a laminate.</skos:note>
        <skos:prefLabel xml:lang="en">zone structural makeup</skos:prefLabel>
    </owl:Class>
    


    <!-- http://standards.iso.org/iso/10303/tech/refdata/core#f619775e-beed-429a-855a-d448fcd644e2 -->

    <owl:Class rdf:about="http://standards.iso.org/iso/10303/tech/refdata/core#f619775e-beed-429a-855a-d448fcd644e2">
        <rdfs:subClassOf rdf:resource="http://standards.iso.org/iso/10303/tech/refdata/core#STEPThing"/>
        <dc:contributor>STEP Harmonization Team</dc:contributor>
        <dc:creator>Phil Spiby, Eurostep</dc:creator>
        <dc:date>2022-09-01</dc:date>
        <dc:source>ISO/TS 10303-4000</dc:source>
        <dc:type>InWork</dc:type>
        <rdfs:comment xml:lang="en">A System is used to identify a conceptual solution to a collection of requirements.</rdfs:comment>
        <owl:versionInfo>1</owl:versionInfo>
        <skos:changeNote>[2022-09-01] Initial definition.</skos:changeNote>
        <skos:note xml:lang="en">The concept system is any thing - matter, energy, organisation or information or a combination of these - for which reproducible measurements exist. The concept system excludes any asserted thing based on personal experience for which no reproducible measurements exist.</skos:note>
        <skos:prefLabel xml:lang="en">system</skos:prefLabel>
    </owl:Class>
    


    <!-- http://standards.iso.org/iso/10303/tech/refdata/core#f654698f-36fa-4a96-8680-290fd5112296 -->

    <owl:Class rdf:about="http://standards.iso.org/iso/10303/tech/refdata/core#f654698f-36fa-4a96-8680-290fd5112296">
        <rdfs:subClassOf rdf:resource="http://standards.iso.org/iso/10303/tech/refdata/core#59b11220-3279-0135-b58f-598f1b1392ae"/>
        <dc:contributor>STEP Harmonization Team</dc:contributor>
        <dc:creator>Phil Spiby, Eurostep</dc:creator>
        <dc:date>2022-09-01</dc:date>
        <dc:source>ISO/TS 10303-4000</dc:source>
        <dc:type>InWork</dc:type>
        <rdfs:comment xml:lang="en">A LocationRelationship is a relationship between two Location objects.</rdfs:comment>
        <owl:versionInfo>2</owl:versionInfo>
        <skos:changeNote>[2021-07-30] Initial definition.</skos:changeNote>
        <skos:changeNote>[2022-09-01] Phil Spiby, Eurostep: updated comment.</skos:changeNote>
        <skos:prefLabel xml:lang="en">location relationship</skos:prefLabel>
    </owl:Class>
    


    <!-- http://standards.iso.org/iso/10303/tech/refdata/core#f8114b4d-b02d-43fe-9a7a-8d8e4b9ebb35 -->

    <owl:Class rdf:about="http://standards.iso.org/iso/10303/tech/refdata/core#f8114b4d-b02d-43fe-9a7a-8d8e4b9ebb35">
        <rdfs:subClassOf rdf:resource="http://standards.iso.org/iso/10303/tech/refdata/core#55105ef0-713f-409a-8306-fd8708d4ee3f"/>
        <dc:contributor>STEP Harmonization Team</dc:contributor>
        <dc:creator>Jean Brangé, AFNeT Services</dc:creator>
        <dc:date>2023-10-04</dc:date>
        <dc:source>ISO/TS 10303-4000</dc:source>
        <dc:type>InWork</dc:type>
        <rdfs:comment xml:lang="en">A FlatnessTolerance is a type of GeometricTolerance that constraints the form of a planar feature. Unless otherwise specified, the rules governing flatness tolerance defined in ISO 1101 shall apply.</rdfs:comment>
        <owl:versionInfo>3</owl:versionInfo>
        <skos:changeNote>[2023-10-04] Jean Brangé, AFNeT Services: Initial definition.</skos:changeNote>
        <skos:note xml:lang="en">Alternatively flatness tolerance can be used according to the specifications given in ASME Y14.5</skos:note>
        <skos:prefLabel xml:lang="en">flatness tolerance</skos:prefLabel>
    </owl:Class>
    


    <!-- http://standards.iso.org/iso/10303/tech/refdata/core#f8816baf-d66a-42f9-bdcc-38e946c9a2fa -->

    <owl:Class rdf:about="http://standards.iso.org/iso/10303/tech/refdata/core#f8816baf-d66a-42f9-bdcc-38e946c9a2fa">
        <rdfs:subClassOf rdf:resource="http://standards.iso.org/iso/10303/tech/refdata/core#66348150-092a-4eb7-9561-0b83adfa15ff"/>
        <dc:contributor>STEP Harmonization Team</dc:contributor>
        <dc:creator>Jean Brangé, AFNeT Services</dc:creator>
        <dc:date>2023-10-04</dc:date>
        <dc:source>ISO/TS 10303-4000</dc:source>
        <dc:type>InWork</dc:type>
        <rdfs:comment xml:lang="en">A DerivedShapeElement is a type of ShapeElement. It represents a shape element derived from one or more other ShapeElements.</rdfs:comment>
        <owl:versionInfo>3</owl:versionInfo>
        <skos:changeNote>[2023-10-04] Jean Brangé, AFNeT Services: Initial definition.</skos:changeNote>
        <skos:example xml:lang="en">The centre plane of an ideal slot is a DerivedShapeElement, that is derived from a symmetrical feature of the shape of a part. Its shape is uniquely specified without further geometric description.</skos:example>
        <skos:prefLabel xml:lang="en">derived shape element</skos:prefLabel>
    </owl:Class>
    


    <!-- http://standards.iso.org/iso/10303/tech/refdata/core#fa0025d0-a9de-435f-881c-c8cc3bdbd601 -->

    <owl:Class rdf:about="http://standards.iso.org/iso/10303/tech/refdata/core#fa0025d0-a9de-435f-881c-c8cc3bdbd601">
        <rdfs:subClassOf rdf:resource="http://standards.iso.org/iso/10303/tech/refdata/core#59b11220-3279-0135-b58f-598f1b1392ae"/>
        <dc:contributor>STEP Harmonization Team</dc:contributor>
        <dc:creator>Phil Spiby, Eurostep</dc:creator>
        <dc:date>2022-09-01</dc:date>
        <dc:source>ISO/TS 10303-4000</dc:source>
        <dc:type>InWork</dc:type>
        <rdfs:comment xml:lang="en">A CollectionMembershipRelationship is a relationship between two CollectionMembership objects.</rdfs:comment>
        <owl:versionInfo>2</owl:versionInfo>
        <skos:changeNote>[2021-07-30] Initial definition.</skos:changeNote>
        <skos:changeNote>[2022-09-01] Phil Spiby, Eurostep: updated comment updated example.</skos:changeNote>
        <skos:example xml:lang="en">Part &quot;smart speaker&quot; replaces part &quot;encyclopaedia Britannia&quot; in the &quot;2019 version&quot; of the consumer price index basket.</skos:example>
        <skos:prefLabel xml:lang="en">collection membership relationship</skos:prefLabel>
    </owl:Class>
    


    <!-- http://standards.iso.org/iso/10303/tech/refdata/core#fadeacc9-ac08-458c-b328-48faa149f74b -->

    <owl:Class rdf:about="http://standards.iso.org/iso/10303/tech/refdata/core#fadeacc9-ac08-458c-b328-48faa149f74b">
        <rdfs:subClassOf rdf:resource="http://standards.iso.org/iso/10303/tech/refdata/core#59b11220-3279-0135-b58f-598f1b1392ae"/>
        <dc:contributor>STEP Harmonization Team</dc:contributor>
        <dc:creator>Phil Spiby, Eurostep</dc:creator>
        <dc:date>2022-09-01</dc:date>
        <dc:source>ISO/TS 10303-4000</dc:source>
        <dc:type>InWork</dc:type>
        <rdfs:comment xml:lang="en">A RiskRelationship is a relationship between two Risk objects.</rdfs:comment>
        <owl:versionInfo>1</owl:versionInfo>
        <skos:changeNote>[2022-09-01] Initial definition.</skos:changeNote>
        <skos:prefLabel xml:lang="en">risk relationship</skos:prefLabel>
    </owl:Class>
    


    <!-- http://standards.iso.org/iso/10303/tech/refdata/core#fb64f36a-51fc-4c43-9f62-341ead3d554e -->

    <owl:Class rdf:about="http://standards.iso.org/iso/10303/tech/refdata/core#fb64f36a-51fc-4c43-9f62-341ead3d554e">
        <rdfs:subClassOf rdf:resource="http://standards.iso.org/iso/10303/tech/refdata/core#1d59c650-3279-0135-b58f-598f1b1392ae"/>
        <dc:contributor>STEP Harmonization Team</dc:contributor>
        <dc:creator>Phil Spiby, Eurostep</dc:creator>
        <dc:date>2022-09-01</dc:date>
        <dc:source>ISO/TS 10303-4000</dc:source>
        <dc:type>InWork</dc:type>
        <rdfs:comment xml:lang="en">A ProductGroupMembership is an association of a ProductGroup with an item (specified in ProductGroupMemberSelect) that represents a member of the product group.</rdfs:comment>
        <owl:versionInfo>1</owl:versionInfo>
        <skos:changeNote>[2022-09-01] Initial definition.</skos:changeNote>
        <skos:prefLabel xml:lang="en">product group membership</skos:prefLabel>
    </owl:Class>
    


    <!-- http://standards.iso.org/iso/10303/tech/refdata/core#fb9cfd9d-166f-4c3f-9a45-ecc9b8420c6b -->

    <owl:Class rdf:about="http://standards.iso.org/iso/10303/tech/refdata/core#fb9cfd9d-166f-4c3f-9a45-ecc9b8420c6b">
        <rdfs:subClassOf rdf:resource="http://standards.iso.org/iso/10303/tech/refdata/core#835280f0-130a-0135-b552-598f1b1392ae"/>
        <dc:contributor>STEP Harmonization Team</dc:contributor>
        <dc:creator>Phil Spiby, Eurostep</dc:creator>
        <dc:date>2022-09-01</dc:date>
        <dc:source>ISO/TS 10303-4000</dc:source>
        <dc:type>InWork</dc:type>
        <rdfs:comment xml:lang="en">A TaskMethodVersion is a specialization of ActivityMethod which allows the explicit reference to versions of a TaskMethod and to track changes against a TaskMethod.</rdfs:comment>
        <owl:versionInfo>1</owl:versionInfo>
        <skos:changeNote>[2021-07-30] Initial definition.</skos:changeNote>
        <skos:prefLabel xml:lang="en">task method version</skos:prefLabel>
    </owl:Class>
    


    <!-- http://standards.iso.org/iso/10303/tech/refdata/core#fc5feb71-9eea-481a-aa2b-91dc0f28112a -->

    <owl:Class rdf:about="http://standards.iso.org/iso/10303/tech/refdata/core#fc5feb71-9eea-481a-aa2b-91dc0f28112a">
        <rdfs:subClassOf rdf:resource="http://standards.iso.org/iso/10303/tech/refdata/core#68242b94-82e8-4841-8005-89981113e22f"/>
        <dc:contributor>STEP Harmonization Team</dc:contributor>
        <dc:creator>Phil Spiby, Eurostep</dc:creator>
        <dc:date>2022-09-01</dc:date>
        <dc:source>ISO/TS 10303-4000</dc:source>
        <dc:type>InWork</dc:type>
        <rdfs:comment xml:lang="en">A CompoundAddress is a type of Locator specified using structured information that allows unambiguous determination of an address for the purpose of communicating, using one or more communication methods. A CompoundAddress consists of a non-empty set of AddressComponents.</rdfs:comment>
        <owl:versionInfo>1</owl:versionInfo>
        <skos:changeNote>[2021-07-30] Initial definition.</skos:changeNote>
        <skos:prefLabel xml:lang="en">compound address</skos:prefLabel>
    </owl:Class>
    


    <!-- http://standards.iso.org/iso/10303/tech/refdata/core#fc80a250-9766-4cec-b524-4504374312f3 -->

    <owl:Class rdf:about="http://standards.iso.org/iso/10303/tech/refdata/core#fc80a250-9766-4cec-b524-4504374312f3">
        <rdfs:subClassOf rdf:resource="http://standards.iso.org/iso/10303/tech/refdata/core#02761765-5f96-4ed2-a51c-38aaa796367d"/>
        <dc:contributor>STEP Harmonization Team</dc:contributor>
        <dc:creator>Jean Brangé, AFNeT Services</dc:creator>
        <dc:date>2023-10-04</dc:date>
        <dc:source>ISO/TS 10303-4000</dc:source>
        <dc:type>InWork</dc:type>
        <rdfs:comment xml:lang="en">A CompositeUnitShapeElement is a type of CompositeShapeElement that is treated as a unit, as opposed to as a group of individual ShapeElement.</rdfs:comment>
        <owl:versionInfo>3</owl:versionInfo>
        <skos:changeNote>[2023-10-04] Jean Brangé, AFNeT Services: Initial definition.</skos:changeNote>
        <skos:example xml:lang="en">A FlatnessTolerance may be applied to a CompositeUnitShapeElement to specify that the coplanar surfaces that make up the CompositeUnitShapeElement are required to fall within a common ToleranceZone.</skos:example>
        <skos:example xml:lang="en">A SurfaceProfileTolerance is applied to a square cut-out that goes through a printed circuit board. The square cut-out is a CompositeUnitShapeElement that consists of the four constituent ShapeElements that correspond to the four surfaces of the cut-out.</skos:example>
        <skos:note xml:lang="en">Combined zone specification are described in ﻿8.2.2.1.2 of ISO 1101.</skos:note>
        <skos:prefLabel xml:lang="en">composite unit shape element</skos:prefLabel>
    </owl:Class>
    


    <!-- http://standards.iso.org/iso/10303/tech/refdata/core#fd79f597-f8d5-464a-b4b8-ab6ef85b8941 -->

    <owl:Class rdf:about="http://standards.iso.org/iso/10303/tech/refdata/core#fd79f597-f8d5-464a-b4b8-ab6ef85b8941">
        <rdfs:subClassOf rdf:resource="http://standards.iso.org/iso/10303/tech/refdata/core#59b11220-3279-0135-b58f-598f1b1392ae"/>
        <dc:contributor>STEP Harmonization Team</dc:contributor>
        <dc:creator>Phil Spiby, Eurostep</dc:creator>
        <dc:date>2022-09-01</dc:date>
        <dc:source>ISO/TS 10303-4000</dc:source>
        <dc:type>InWork</dc:type>
        <rdfs:comment xml:lang="en">A SlotDesignToRealized is a relationship between a design version of a Slot and a realized individual that conforms to the design.</rdfs:comment>
        <owl:versionInfo>1</owl:versionInfo>
        <skos:changeNote>[2022-09-01] Initial definition.</skos:changeNote>
        <skos:example xml:lang="en">WeMakeBigPlanes Limited builds aircraft serial number 1234 with a starboard engine attachment slot that conforms to design version 1.34.</skos:example>
        <skos:prefLabel xml:lang="en">slot design to realized</skos:prefLabel>
    </owl:Class>
    


    <!-- http://standards.iso.org/iso/10303/tech/refdata/core#fe020356-3374-4d28-85ab-2f5d6da3d7d1 -->

    <owl:Class rdf:about="http://standards.iso.org/iso/10303/tech/refdata/core#fe020356-3374-4d28-85ab-2f5d6da3d7d1">
        <rdfs:subClassOf rdf:resource="http://standards.iso.org/iso/10303/tech/refdata/core#STEPThing"/>
        <dc:contributor>STEP Harmonization Team</dc:contributor>
        <dc:creator>Jean Brangé, AFNeT Services</dc:creator>
        <dc:date>2023-10-04</dc:date>
        <dc:source>ISO/TS 10303-4000</dc:source>
        <dc:type>InWork</dc:type>
        <rdfs:comment xml:lang="en">A ProcessPlan is manufacturing planning information, necessary to realize or produce a specific version of a Part. A ProcessPlan might represent a specific version of a ProcessPlan.</rdfs:comment>
        <owl:versionInfo>3</owl:versionInfo>
        <skos:changeNote>[2023-10-04] Jean Brangé, AFNeT Services: Initial definition.</skos:changeNote>
        <skos:prefLabel xml:lang="en">process plan</skos:prefLabel>
    </owl:Class>
    


    <!-- http://standards.iso.org/iso/10303/tech/refdata/core#fe554d1d-3575-4af5-af10-84a3d20a7337 -->

    <owl:Class rdf:about="http://standards.iso.org/iso/10303/tech/refdata/core#fe554d1d-3575-4af5-af10-84a3d20a7337">
        <rdfs:subClassOf rdf:resource="http://standards.iso.org/iso/10303/tech/refdata/core#83b2a250-130a-0135-b552-598f1b1392ae"/>
        <dc:contributor>STEP Harmonization Team</dc:contributor>
        <dc:creator>Phil Spiby, Eurostep</dc:creator>
        <dc:date>2022-09-01</dc:date>
        <dc:source>ISO/TS 10303-4000</dc:source>
        <dc:type>InWork</dc:type>
        <rdfs:comment xml:lang="en">A RiskEvent is a specialization of an ActivityMethodAssignment. It assigns an ActivityMethod, that represents the unwanted (or wanted) event resulting from the risk, to the RiskPerception. The probability of the event occurring is represented by a set of probabilities defined by the attribute Probability. If more than one probability is provided each probability shall be equivalent.</rdfs:comment>
        <owl:versionInfo>1</owl:versionInfo>
        <skos:changeNote>[2022-09-01] Initial definition.</skos:changeNote>
        <skos:prefLabel xml:lang="en">risk event</skos:prefLabel>
    </owl:Class>
    


    <!-- http://standards.iso.org/iso/10303/tech/refdata/core#ff04d2c5-cea4-41a6-be35-821c1495d8ba -->

    <owl:Class rdf:about="http://standards.iso.org/iso/10303/tech/refdata/core#ff04d2c5-cea4-41a6-be35-821c1495d8ba">
        <rdfs:subClassOf rdf:resource="http://standards.iso.org/iso/10303/tech/refdata/core#95f1bde5-b263-4ca1-89df-33e1205800dd"/>
        <dc:contributor>STEP Harmonization Team</dc:contributor>
        <dc:creator>Phil Spiby, Eurostep</dc:creator>
        <dc:date>2022-09-01</dc:date>
        <dc:source>ISO/TS 10303-4000</dc:source>
        <dc:type>InWork</dc:type>
        <rdfs:comment xml:lang="en">A StructuredTaskElement is a type of TaskElement. It is made up of other TaskElements.</rdfs:comment>
        <owl:versionInfo>1</owl:versionInfo>
        <skos:changeNote>[2021-07-30] Initial definition.</skos:changeNote>
        <skos:prefLabel xml:lang="en">structured task element</skos:prefLabel>
    </owl:Class>
    


    <!-- http://standards.iso.org/iso/10303/tech/refdata/core#ff5fba41-da02-4906-b66c-40b83e7bd99e -->

    <owl:Class rdf:about="http://standards.iso.org/iso/10303/tech/refdata/core#ff5fba41-da02-4906-b66c-40b83e7bd99e">
        <rdfs:subClassOf rdf:resource="http://standards.iso.org/iso/10303/tech/refdata/core#STEPThing"/>
        <dc:contributor>STEP Harmonization Team</dc:contributor>
        <dc:creator>Phil Spiby, Eurostep</dc:creator>
        <dc:date>2022-09-01</dc:date>
        <dc:source>ISO/TS 10303-4000</dc:source>
        <dc:type>InWork</dc:type>
        <rdfs:comment xml:lang="en">A TaskObjective is a result or objective that is reached by undertaking a TaskMethod.</rdfs:comment>
        <owl:versionInfo>2</owl:versionInfo>
        <skos:changeNote>[2021-07-30] Initial definition.</skos:changeNote>
        <skos:changeNote>[2022-09-01] Phil Spiby, Eurostep: updated note.</skos:changeNote>
        <skos:note xml:lang="en">More than one TaskMethod can be defined for a given objective if there can be several ways to accomplish the objective.</skos:note>
        <skos:prefLabel xml:lang="en">task objective</skos:prefLabel>
    </owl:Class>
    


    <!-- http://standards.iso.org/iso/10303/tech/refdata/core#ffb1814e-b215-4055-af04-a2808883f04e -->

    <owl:Class rdf:about="http://standards.iso.org/iso/10303/tech/refdata/core#ffb1814e-b215-4055-af04-a2808883f04e">
        <rdfs:subClassOf rdf:resource="http://standards.iso.org/iso/10303/tech/refdata/core#99130bd0-130a-0135-b552-598f1b1392ae"/>
        <dc:contributor>STEP Harmonization Team</dc:contributor>
        <dc:creator>Phil Spiby, Eurostep</dc:creator>
        <dc:date>2022-09-01</dc:date>
        <dc:source>ISO/TS 10303-4000</dc:source>
        <dc:type>InWork</dc:type>
        <rdfs:comment xml:lang="en">An IndividualPartEffectivity is a specialization of Effectivity for which the domain of applicability is defined as a set of instances of IndividualPart.</rdfs:comment>
        <owl:versionInfo>1</owl:versionInfo>
        <skos:changeNote>[2021-07-30] Initial definition.</skos:changeNote>
        <skos:prefLabel xml:lang="en">individual part effectivity</skos:prefLabel>
    </owl:Class>
    


    <!-- http://standards.iso.org/iso/10303/tech/refdata/core#ffbb0f6e-806a-48a4-82cc-04ac8dd2242e -->

    <owl:Class rdf:about="http://standards.iso.org/iso/10303/tech/refdata/core#ffbb0f6e-806a-48a4-82cc-04ac8dd2242e">
        <rdfs:subClassOf rdf:resource="http://standards.iso.org/iso/10303/tech/refdata/core#59b11220-3279-0135-b58f-598f1b1392ae"/>
        <dc:contributor>STEP Harmonization Team</dc:contributor>
        <dc:creator>Phil Spiby, Eurostep</dc:creator>
        <dc:date>2022-09-01</dc:date>
        <dc:source>ISO/TS 10303-4000</dc:source>
        <dc:type>InWork</dc:type>
        <rdfs:comment xml:lang="en">A TypeOfPersonDefinitionRelationship is a relationship between two TypeOfPersonDefinition objects.</rdfs:comment>
        <owl:versionInfo>1</owl:versionInfo>
        <skos:changeNote>[2022-09-01] Initial definition.</skos:changeNote>
        <skos:example xml:lang="en">&quot;alternate&quot; and &quot;superseded by&quot; are examples of TypeOfPersonDefinitionRelationships.</skos:example>
        <skos:prefLabel xml:lang="en">type of person definition relationship</skos:prefLabel>
    </owl:Class>
    


    <!-- http://standards.iso.org/iso/10303/tech/refdata/core#0a15a092-b7c9-4d0c-8623-345db775bc9b -->

    <owl:Class rdf:about="http://standards.iso.org/iso/10303/tech/refdata/core#0a15a092-b7c9-4d0c-8623-345db775bc9b">
        <rdfs:subClassOf rdf:resource="http://standards.iso.org/iso/10303/tech/refdata/core#d2eb1f4f-b98f-4393-a7ed-24dc41900bd2"/>
        <dc:contributor>STEP Harmonization Team</dc:contributor>
        <dc:creator>Jean Brangé, AFNeT Services</dc:creator>
        <dc:date>2023-10-04</dc:date>
        <dc:source>ISO/TS 10303-4000</dc:source>
        <dc:type>InWork</dc:type>
        <rdfs:comment xml:lang="en">A TargetCurve is a type of DatumTarget that is specified by a single curve.</rdfs:comment>
        <owl:versionInfo>3</owl:versionInfo>
        <skos:changeNote>[2023-10-04] Jean Brangé, AFNeT Services: Initial definition.</skos:changeNote>
        <skos:prefLabel xml:lang="en">target curve</skos:prefLabel>
    </owl:Class>
    


    <!-- http://standards.iso.org/iso/10303/tech/refdata/core#0afa5b1a-1fc5-44f6-b186-186ff81228e7 -->

    <owl:Class rdf:about="http://standards.iso.org/iso/10303/tech/refdata/core#0afa5b1a-1fc5-44f6-b186-186ff81228e7">
        <rdfs:subClassOf rdf:resource="http://standards.iso.org/iso/10303/tech/refdata/core#5a6c8b1f-63af-4307-9faf-9fdd6da5572c"/>
        <dc:contributor>STEP Harmonization Team</dc:contributor>
        <dc:creator>Jean Brangé, AFNeT Services</dc:creator>
        <dc:date>2023-10-04</dc:date>
        <dc:source>ISO/TS 10303-4000</dc:source>
        <dc:type>InWork</dc:type>
        <rdfs:comment xml:lang="en">A PlyPiece is a type of ConstituentPart. It is a single portion of a Ply that may be combined with other ply pieces on the same layer to make up the Ply. A PlyPiece has the same material and orientation direction as defined for the Ply of which it is a portion.</rdfs:comment>
        <owl:versionInfo>3</owl:versionInfo>
        <skos:changeNote>[2023-10-04] Jean Brangé, AFNeT Services: Initial definition.</skos:changeNote>
        <skos:example xml:lang="en">Tape strips are a typical example of PlyPieces that are grouped together to fill a PlyShape.</skos:example>
        <skos:note xml:lang="en">StockMaterial may be too small to fully cover the area of a Ply. In this case the application may allow two or more pieces to be used.</skos:note>
        <skos:prefLabel xml:lang="en">ply piece</skos:prefLabel>
    </owl:Class>
    


    <!-- http://standards.iso.org/iso/10303/tech/refdata/core#0b4f613b-79d0-48f6-be21-6b6b87bc4ecb -->

    <owl:Class rdf:about="http://standards.iso.org/iso/10303/tech/refdata/core#0b4f613b-79d0-48f6-be21-6b6b87bc4ecb">
        <rdfs:subClassOf rdf:resource="http://standards.iso.org/iso/10303/tech/refdata/core#f5acf4c6-2654-4ef1-abc2-93e0ea5529d5"/>
        <dc:contributor>STEP Harmonization Team</dc:contributor>
        <dc:creator>Jean Brangé, AFNeT Services</dc:creator>
        <dc:date>2023-10-04</dc:date>
        <dc:source>ISO/TS 10303-4000</dc:source>
        <dc:type>InWork</dc:type>
        <rdfs:comment xml:lang="en">A ThicknessLaminateTable is a type of ZoneStructuralMakeup that is used to capture the ordered list of constituents that make up a zone.</rdfs:comment>
        <owl:versionInfo>3</owl:versionInfo>
        <skos:changeNote>[2023-10-04] Jean Brangé, AFNeT Services: Initial definition.</skos:changeNote>
        <skos:prefLabel xml:lang="en">thickness laminate table</skos:prefLabel>
    </owl:Class>
    


    <!-- http://standards.iso.org/iso/10303/tech/refdata/core#0b5e0ff4-9b59-4840-b1d5-e8a27d403950 -->

    <owl:Class rdf:about="http://standards.iso.org/iso/10303/tech/refdata/core#0b5e0ff4-9b59-4840-b1d5-e8a27d403950">
        <rdfs:subClassOf rdf:resource="http://standards.iso.org/iso/10303/tech/refdata/core#f8816baf-d66a-42f9-bdcc-38e946c9a2fa"/>
        <dc:contributor>STEP Harmonization Team</dc:contributor>
        <dc:creator>Jean Brangé, AFNeT Services</dc:creator>
        <dc:date>2023-10-04</dc:date>
        <dc:source>ISO/TS 10303-4000</dc:source>
        <dc:type>InWork</dc:type>
        <rdfs:comment xml:lang="en">A CentreOfSymmetry is a type of DerivedShapeElement that is derived by determining the geometric centre of one or more ShapeElement.</rdfs:comment>
        <owl:versionInfo>3</owl:versionInfo>
        <skos:changeNote>[2023-10-04] Jean Brangé, AFNeT Services: Initial definition.</skos:changeNote>
        <skos:prefLabel xml:lang="en">centre of symmetry</skos:prefLabel>
    </owl:Class>
    


    <!-- http://standards.iso.org/iso/10303/tech/refdata/core#0c8740e5-ed20-4272-b16e-ae9f9ff1c327 -->

    <owl:Class rdf:about="http://standards.iso.org/iso/10303/tech/refdata/core#0c8740e5-ed20-4272-b16e-ae9f9ff1c327">
        <rdfs:subClassOf rdf:resource="http://standards.iso.org/iso/10303/tech/refdata/core#5a6c8b1f-63af-4307-9faf-9fdd6da5572c"/>
        <dc:contributor>STEP Harmonization Team</dc:contributor>
        <dc:creator>Jean Brangé, AFNeT Services</dc:creator>
        <dc:date>2023-10-04</dc:date>
        <dc:source>ISO/TS 10303-4000</dc:source>
        <dc:type>InWork</dc:type>
        <rdfs:comment xml:lang="en">A CompositeAssembly is a type of ConstituentPart that is made of multiple materials that are bonded together. A CompositeAssembly may be made from any combination of materials. A completed CompositeAssembly need not be a rigid shape. A CompositeAssembly may also be used as a composite part.</rdfs:comment>
        <owl:versionInfo>3</owl:versionInfo>
        <skos:changeNote>[2023-10-04] Jean Brangé, AFNeT Services: Initial definition.</skos:changeNote>
        <skos:prefLabel xml:lang="en">composite assembly</skos:prefLabel>
    </owl:Class>
    


    <!-- http://standards.iso.org/iso/10303/tech/refdata/core#0cc8b831-37f7-4cd5-984f-dbb5588fbc1d -->

    <owl:Class rdf:about="http://standards.iso.org/iso/10303/tech/refdata/core#0cc8b831-37f7-4cd5-984f-dbb5588fbc1d">
        <rdfs:subClassOf rdf:resource="http://standards.iso.org/iso/10303/tech/refdata/core#66348150-092a-4eb7-9561-0b83adfa15ff"/>
        <dc:contributor>STEP Harmonization Team</dc:contributor>
        <dc:creator>Jean Brangé, AFNeT Services</dc:creator>
        <dc:date>2023-10-04</dc:date>
        <dc:source>ISO/TS 10303-4000</dc:source>
        <dc:type>InWork</dc:type>
        <rdfs:comment xml:lang="en">A PartShapeElement is a type of ShapeElement. A PartShapeElement represents an element of the shape of a PartView, a ProductConfiguration or another PartShapeElement.</rdfs:comment>
        <owl:versionInfo>3</owl:versionInfo>
        <skos:changeNote>[2023-10-04] Jean Brangé, AFNeT Services: Initial definition.</skos:changeNote>
        <skos:prefLabel xml:lang="en">part shape element</skos:prefLabel>
    </owl:Class>
    


    <!-- http://standards.iso.org/iso/10303/tech/refdata/core#0ccba30b-b471-4863-8f01-c941e53bcf1a -->

    <owl:Class rdf:about="http://standards.iso.org/iso/10303/tech/refdata/core#0ccba30b-b471-4863-8f01-c941e53bcf1a">
        <rdfs:subClassOf rdf:resource="http://standards.iso.org/iso/10303/tech/refdata/core#59b11220-3279-0135-b58f-598f1b1392ae"/>
        <dc:contributor>STEP Harmonization Team</dc:contributor>
        <dc:creator>Phil Spiby, Eurostep</dc:creator>
        <dc:date>2022-09-01</dc:date>
        <dc:source>ISO/TS 10303-4000</dc:source>
        <dc:type>InWork</dc:type>
        <rdfs:comment xml:lang="en">A ResourceItemRelationship is a relationship between two ResourceItem objects.</rdfs:comment>
        <owl:versionInfo>2</owl:versionInfo>
        <skos:changeNote>[2021-07-30] Initial definition.</skos:changeNote>
        <skos:changeNote>[2022-09-01] Phil Spiby, Eurostep: updated comment updated example.</skos:changeNote>
        <skos:example xml:lang="en">The relationship between a product and a package can be classified as &quot;Preferred&quot;.</skos:example>
        <skos:prefLabel xml:lang="en">resource item relationship</skos:prefLabel>
    </owl:Class>
    


    <!-- http://standards.iso.org/iso/10303/tech/refdata/core#0d02d547-2ff2-44a9-8356-5b6f33bb33d1 -->

    <owl:Class rdf:about="http://standards.iso.org/iso/10303/tech/refdata/core#0d02d547-2ff2-44a9-8356-5b6f33bb33d1">
        <rdfs:subClassOf rdf:resource="http://standards.iso.org/iso/10303/tech/refdata/core#55105ef0-713f-409a-8306-fd8708d4ee3f"/>
        <dc:contributor>STEP Harmonization Team</dc:contributor>
        <dc:creator>Jean Brangé, AFNeT Services</dc:creator>
        <dc:date>2023-10-04</dc:date>
        <dc:source>ISO/TS 10303-4000</dc:source>
        <dc:type>InWork</dc:type>
        <rdfs:comment xml:lang="en">A TotalRunoutTolerance is a type of GeometricTolerance that constrains the deviation features constructed about an axis or at right angles to an axis. It constrains the deviation over a surface with respect to a datum axis about which the part is rotated. The tolerance is applied simultaneously to all measuring positions as the part is rotated 360 degrees. Unless otherwise specified the rules governing total run-out tolerance defined in ISO 1101 shall apply. The set of referenced datums shall contain one revolute surface feature. The tolerance zone is limited either by: two coaxial cylinders with a difference in radii equal to the tolerance value. In this case, the axis of the cylinders shall be the axis of the revolute surface feature, and the ideal feature corresponding to the toleranced surface is a cylinder; two parallel planes separated by the distance specified by the tolerance value. In this case, the planes are perpendicular to the axis of the revolute surface feature, and the ideal feature corresponding to the toleranced surface is a plane.</rdfs:comment>
        <owl:versionInfo>3</owl:versionInfo>
        <skos:changeNote>[2023-10-04] Jean Brangé, AFNeT Services: Initial definition.</skos:changeNote>
        <skos:note xml:lang="en">Alternatively total run-out tolerance can be used according to the specifications given in ASME Y14.5.</skos:note>
        <skos:prefLabel xml:lang="en">total runout tolerance</skos:prefLabel>
    </owl:Class>
    


    <!-- http://standards.iso.org/iso/10303/tech/refdata/core#0f50a78f-3eb8-4045-a0c3-3372805a4ae1 -->

    <owl:Class rdf:about="http://standards.iso.org/iso/10303/tech/refdata/core#0f50a78f-3eb8-4045-a0c3-3372805a4ae1">
        <rdfs:subClassOf rdf:resource="http://standards.iso.org/iso/10303/tech/refdata/core#1cfca290-3279-0135-b58f-598f1b1392ae"/>
        <dc:contributor>STEP Harmonization Team</dc:contributor>
        <dc:creator>Phil Spiby, Eurostep</dc:creator>
        <dc:date>2022-09-01</dc:date>
        <dc:source>ISO/TS 10303-4000</dc:source>
        <dc:type>InWork</dc:type>
        <rdfs:comment xml:lang="en">A PositionGroupAssignment is an assignment of a PositionGroup to an item (specified by PositionGroupAssignmentSelect). The meaning of the assignment can be specified using the ClassifiedAs attribute inherited from the AssignmentObject.</rdfs:comment>
        <owl:versionInfo>1</owl:versionInfo>
        <skos:changeNote>[2022-09-01] Initial definition.</skos:changeNote>
        <skos:prefLabel xml:lang="en">position group assignment</skos:prefLabel>
    </owl:Class>
    


    <!-- http://standards.iso.org/iso/10303/tech/refdata/core#00b6d8ff-c413-4f2f-a15b-0bddcd4f5c6d -->

    <owl:Class rdf:about="http://standards.iso.org/iso/10303/tech/refdata/core#00b6d8ff-c413-4f2f-a15b-0bddcd4f5c6d">
        <rdfs:subClassOf rdf:resource="http://standards.iso.org/iso/10303/tech/refdata/core#1cfca290-3279-0135-b58f-598f1b1392ae"/>
        <dc:contributor>STEP Harmonization Team</dc:contributor>
        <dc:creator>Phil Spiby, Eurostep</dc:creator>
        <dc:date>2022-09-01</dc:date>
        <dc:source>ISO/TS 10303-4000</dc:source>
        <dc:type>InWork</dc:type>
        <rdfs:comment xml:lang="en">A ResourceAsRealizedAssignment is an assignment of a resource record statement (via ResourceAsRealized) to an item (specified by ResourceAsRealizedAssignmentSelect) that used or consumed the resource. The meaning of the assignment can be specified using the ClassifiedAs attribute inherited from the AssignmentObject.</rdfs:comment>
        <owl:versionInfo>2</owl:versionInfo>
        <skos:changeNote>[2021-07-30] Initial definition.</skos:changeNote>
        <skos:changeNote>[2022-09-01] Phil Spiby, Eurostep: updated comment.</skos:changeNote>
        <skos:prefLabel xml:lang="en">resource as realized assignment</skos:prefLabel>
    </owl:Class>
    


    <!-- http://standards.iso.org/iso/10303/tech/refdata/core#00d88892-01a1-4dfb-9174-b5a1e78d6696 -->

    <owl:Class rdf:about="http://standards.iso.org/iso/10303/tech/refdata/core#00d88892-01a1-4dfb-9174-b5a1e78d6696">
        <rdfs:subClassOf rdf:resource="http://standards.iso.org/iso/10303/tech/refdata/core#59b11220-3279-0135-b58f-598f1b1392ae"/>
        <dc:contributor>STEP Harmonization Team</dc:contributor>
        <dc:creator>Phil Spiby, Eurostep</dc:creator>
        <dc:date>2022-09-01</dc:date>
        <dc:source>ISO/TS 10303-4000</dc:source>
        <dc:type>InWork</dc:type>
        <rdfs:comment xml:lang="en">An AssumptionRelationship is a relationship between two Assumption objects.</rdfs:comment>
        <owl:versionInfo>2</owl:versionInfo>
        <skos:changeNote>[2021-07-30] Initial definition.</skos:changeNote>
        <skos:changeNote>[2022-09-01] Phil Spiby, Eurostep: updated comment.</skos:changeNote>
        <skos:prefLabel xml:lang="en">assumption relationship</skos:prefLabel>
    </owl:Class>
    


    <!-- http://standards.iso.org/iso/10303/tech/refdata/core#005283a0-d6bf-4470-9ba6-b1d7fc9eb217 -->

    <owl:Class rdf:about="http://standards.iso.org/iso/10303/tech/refdata/core#005283a0-d6bf-4470-9ba6-b1d7fc9eb217">
        <rdfs:subClassOf rdf:resource="http://standards.iso.org/iso/10303/tech/refdata/core#STEPThing"/>
        <dc:contributor>STEP Harmonization Team</dc:contributor>
        <dc:creator>Phil Spiby, Eurostep</dc:creator>
        <dc:date>2022-09-01</dc:date>
        <dc:source>ISO/TS 10303-4000</dc:source>
        <dc:type>InWork</dc:type>
        <rdfs:comment xml:lang="en">A PersonOrganizationInPosition is a person or an organization (specified by PositionPersonOrganizationSelect) that holds a Position. A person can hold more than one position within an organization or organizations. A position in an organization can be held by more than one person or organization.</rdfs:comment>
        <owl:versionInfo>1</owl:versionInfo>
        <skos:changeNote>[2022-09-01] Initial definition.</skos:changeNote>
        <skos:example xml:lang="en">A person can hold two positions in an organization: Production Manager and Safety Officer.</skos:example>
        <skos:example xml:lang="en">Two people can hold the same position in a job-share scheme.</skos:example>
        <skos:prefLabel xml:lang="en">person organization in position</skos:prefLabel>
    </owl:Class>
    


    <!-- http://standards.iso.org/iso/10303/tech/refdata/core#00567250-a97e-4d46-ae7f-40c329d43c98 -->

    <owl:Class rdf:about="http://standards.iso.org/iso/10303/tech/refdata/core#00567250-a97e-4d46-ae7f-40c329d43c98">
        <rdfs:subClassOf rdf:resource="http://standards.iso.org/iso/10303/tech/refdata/core#d2bb2d90-130a-0135-b552-598f1b1392ae"/>
        <dc:contributor>STEP Harmonization Team</dc:contributor>
        <dc:creator>Jean Brangé, AFNeT Services</dc:creator>
        <dc:date>2023-10-04</dc:date>
        <dc:source>ISO/TS 10303-4000</dc:source>
        <dc:type>InWork</dc:type>
        <rdfs:comment xml:lang="en">An AnnotatedModelPresentation is a type of StyledModel that describes a presentation of model with annotation according to ISO 16792.</rdfs:comment>
        <owl:versionInfo>3</owl:versionInfo>
        <skos:changeNote>[2023-10-04] Jean Brangé, AFNeT Services: Initial definition.</skos:changeNote>
        <skos:prefLabel xml:lang="en">annotated model presentation</skos:prefLabel>
    </owl:Class>
    


    <!-- http://standards.iso.org/iso/10303/tech/refdata/core#0195a37f-c5a5-492f-865c-0aa499047ab7 -->

    <owl:Class rdf:about="http://standards.iso.org/iso/10303/tech/refdata/core#0195a37f-c5a5-492f-865c-0aa499047ab7">
        <rdfs:subClassOf rdf:resource="http://standards.iso.org/iso/10303/tech/refdata/core#55105ef0-713f-409a-8306-fd8708d4ee3f"/>
        <dc:contributor>STEP Harmonization Team</dc:contributor>
        <dc:creator>Jean Brangé, AFNeT Services</dc:creator>
        <dc:date>2023-10-04</dc:date>
        <dc:source>ISO/TS 10303-4000</dc:source>
        <dc:type>InWork</dc:type>
        <rdfs:comment xml:lang="en">A PositionTolerance is a type of GeometricTolerance that controls the position of a ShapeElement that is a feature of size. It can be interpreted as defining a positional boundary within which the entire feature is permitted to lie, or as defining a tolerance zone within which the centre, axis, or centre plane of the considered ShapeElement is permitted to lie. Unless otherwise specified, the tolerance shall be used in accordance with position tolerance in ISO 1101 and ISO 5458. The location of the tolerance zone shall be specified with instances of DimensionalLocation.</rdfs:comment>
        <owl:versionInfo>3</owl:versionInfo>
        <skos:changeNote>[2023-10-04] Jean Brangé, AFNeT Services: Initial definition.</skos:changeNote>
        <skos:note xml:lang="en">Alternatively position tolerance can be used according to the specifications given in ASME Y14.5-2009.</skos:note>
        <skos:note xml:lang="en">Basic theoretically exact dimensions establish the true position from specified datum features and between interrelated features.</skos:note>
        <skos:note xml:lang="en">The type DimensionalLocation is defined in ISO 10303-47.</skos:note>
        <skos:note xml:lang="en">When the toleranced shape element is a CompositeShapeElement, the tolerance zone may but need not be defined by referenced datums (see ISO 1101).</skos:note>
        <skos:prefLabel xml:lang="en">position tolerance</skos:prefLabel>
    </owl:Class>
    


    <!-- http://standards.iso.org/iso/10303/tech/refdata/core#02455f10-cdf5-4478-8388-f7a130fc98c0 -->

    <owl:Class rdf:about="http://standards.iso.org/iso/10303/tech/refdata/core#02455f10-cdf5-4478-8388-f7a130fc98c0">
        <rdfs:subClassOf rdf:resource="http://standards.iso.org/iso/10303/tech/refdata/core#9f656069-ff2c-4f09-9091-f91388a14764"/>
        <dc:contributor>STEP Harmonization Team</dc:contributor>
        <dc:creator>Phil Spiby, Eurostep</dc:creator>
        <dc:date>2022-09-01</dc:date>
        <dc:source>ISO/TS 10303-4000</dc:source>
        <dc:type>InWork</dc:type>
        <rdfs:comment xml:lang="en">A StateComposition is a type of StateRelationship and it relates the nature of states in relation to one another, where two or more Related State parts compose a whole Relating State; and furthermore, whole states can become parts of yet another whole State.</rdfs:comment>
        <owl:versionInfo>2</owl:versionInfo>
        <skos:changeNote>[2021-07-30] Initial definition.</skos:changeNote>
        <skos:changeNote>[2022-09-01] Phil Spiby, Eurostep: updated comment.</skos:changeNote>
        <skos:prefLabel xml:lang="en">state composition</skos:prefLabel>
    </owl:Class>
    


    <!-- http://standards.iso.org/iso/10303/tech/refdata/core#02761765-5f96-4ed2-a51c-38aaa796367d -->

    <owl:Class rdf:about="http://standards.iso.org/iso/10303/tech/refdata/core#02761765-5f96-4ed2-a51c-38aaa796367d">
        <rdfs:subClassOf rdf:resource="http://standards.iso.org/iso/10303/tech/refdata/core#66348150-092a-4eb7-9561-0b83adfa15ff"/>
        <dc:contributor>STEP Harmonization Team</dc:contributor>
        <dc:creator>Jean Brangé, AFNeT Services</dc:creator>
        <dc:date>2023-10-04</dc:date>
        <dc:source>ISO/TS 10303-4000</dc:source>
        <dc:type>InWork</dc:type>
        <rdfs:comment xml:lang="en">A CompositeShapeElement is a type of ShapeElement that is composed of two or more constituent ShapeElements.</rdfs:comment>
        <owl:versionInfo>3</owl:versionInfo>
        <skos:changeNote>[2023-10-04] Jean Brangé, AFNeT Services: Initial definition.</skos:changeNote>
        <skos:prefLabel xml:lang="en">composite shape element</skos:prefLabel>
    </owl:Class>
    


    <!-- http://standards.iso.org/iso/10303/tech/refdata/core#02807aa8-c2ee-40ee-a043-04a73b025a08 -->

    <owl:Class rdf:about="http://standards.iso.org/iso/10303/tech/refdata/core#02807aa8-c2ee-40ee-a043-04a73b025a08">
        <rdfs:subClassOf rdf:resource="http://standards.iso.org/iso/10303/tech/refdata/core#83b2a250-130a-0135-b552-598f1b1392ae"/>
        <dc:contributor>STEP Harmonization Team</dc:contributor>
        <dc:creator>Phil Spiby, Eurostep</dc:creator>
        <dc:date>2022-09-01</dc:date>
        <dc:source>ISO/TS 10303-4000</dc:source>
        <dc:type>InWork</dc:type>
        <rdfs:comment xml:lang="en">A TaskElementAssignment is an assignment of a TaskElement to an item (specified by TaskAssignmentSelect). The meaning of the assignment can be specified using the ClassifiedAs attribute inherited from the AssignmentObject.</rdfs:comment>
        <owl:versionInfo>2</owl:versionInfo>
        <skos:changeNote>[2021-07-30] Initial definition.</skos:changeNote>
        <skos:changeNote>[2022-09-01] Phil Spiby, Eurostep: updated comment updated note.</skos:changeNote>
        <skos:prefLabel xml:lang="en">task element assignment</skos:prefLabel>
    </owl:Class>
    


    <!-- http://standards.iso.org/iso/10303/tech/refdata/core#03421784-0a9f-4bda-b862-8be628c8273c -->

    <owl:Class rdf:about="http://standards.iso.org/iso/10303/tech/refdata/core#03421784-0a9f-4bda-b862-8be628c8273c">
        <rdfs:subClassOf rdf:resource="http://standards.iso.org/iso/10303/tech/refdata/core#6067df0d-3ac2-4fc8-829c-6c59487ead9e"/>
        <dc:contributor>STEP Harmonization Team</dc:contributor>
        <dc:creator>Phil Spiby, Eurostep</dc:creator>
        <dc:date>2022-09-01</dc:date>
        <dc:source>ISO/TS 10303-4000</dc:source>
        <dc:type>InWork</dc:type>
        <rdfs:comment xml:lang="en">A ConditionalConfiguration is a type of ConditionalEffectivity and represents an association of a SpecificationConditionAssignment or a SpecificationAssignment object with a design or with a process in order to define a valid usage of it in the context of a certain ProductClass.</rdfs:comment>
        <owl:versionInfo>1</owl:versionInfo>
        <skos:changeNote>[2021-07-30] Initial definition.</skos:changeNote>
        <skos:note xml:lang="en">The semantics of the kind of association is defined by the attributes ConfigurationType and InheritanceType.</skos:note>
        <skos:prefLabel xml:lang="en">conditional configuration</skos:prefLabel>
    </owl:Class>
    


    <!-- http://standards.iso.org/iso/10303/tech/refdata/core#05ed60d9-67c4-4ae8-9464-66b002f5c387 -->

    <owl:Class rdf:about="http://standards.iso.org/iso/10303/tech/refdata/core#05ed60d9-67c4-4ae8-9464-66b002f5c387">
        <rdfs:subClassOf rdf:resource="http://standards.iso.org/iso/10303/tech/refdata/core#c1247222-6528-4897-a401-5a61bdfd511c"/>
        <dc:contributor>STEP Harmonization Team</dc:contributor>
        <dc:creator>Phil Spiby, Eurostep</dc:creator>
        <dc:date>2022-09-01</dc:date>
        <dc:source>ISO/TS 10303-4000</dc:source>
        <dc:type>InWork</dc:type>
        <rdfs:comment xml:lang="en">A RepeatWhile is a type of LoopingElement. It invokes repetitions of the RepeatedElement inherited from LoopingElement while the specified condition is satisfied. The test condition shall be evaluated prior to invoking the method and can result in the LoopingElement not being executed at all.</rdfs:comment>
        <owl:versionInfo>2</owl:versionInfo>
        <skos:changeNote>[2021-07-30] Initial definition.</skos:changeNote>
        <skos:changeNote>[2022-09-01] Phil Spiby, Eurostep: updated comment.</skos:changeNote>
        <skos:prefLabel xml:lang="en">repeat while</skos:prefLabel>
    </owl:Class>
    


    <!-- http://standards.iso.org/iso/10303/tech/refdata/core#065a439a-f529-4c3a-8880-f27aa45e8451 -->

    <owl:Class rdf:about="http://standards.iso.org/iso/10303/tech/refdata/core#065a439a-f529-4c3a-8880-f27aa45e8451">
        <rdfs:subClassOf rdf:resource="http://standards.iso.org/iso/10303/tech/refdata/core#59b11220-3279-0135-b58f-598f1b1392ae"/>
        <dc:contributor>STEP Harmonization Team</dc:contributor>
        <dc:creator>Phil Spiby, Eurostep</dc:creator>
        <dc:date>2022-09-01</dc:date>
        <dc:source>ISO/TS 10303-4000</dc:source>
        <dc:type>InWork</dc:type>
        <rdfs:comment xml:lang="en">A CollectionRelationship is a relationship between two Collection objects.</rdfs:comment>
        <owl:versionInfo>2</owl:versionInfo>
        <skos:changeNote>[2021-07-30] Initial definition.</skos:changeNote>
        <skos:changeNote>[2022-09-01] Phil Spiby, Eurostep: updated comment.</skos:changeNote>
        <skos:prefLabel xml:lang="en">collection relationship</skos:prefLabel>
    </owl:Class>
    


    <!-- http://standards.iso.org/iso/10303/tech/refdata/core#07b7437f-0898-4d93-a88b-be12e930c991 -->

    <owl:Class rdf:about="http://standards.iso.org/iso/10303/tech/refdata/core#07b7437f-0898-4d93-a88b-be12e930c991">
        <rdfs:subClassOf rdf:resource="http://standards.iso.org/iso/10303/tech/refdata/core#6490f437-5aff-4d04-b436-f4243e3160f8"/>
        <dc:contributor>STEP Harmonization Team</dc:contributor>
        <dc:creator>Phil Spiby, Eurostep</dc:creator>
        <dc:date>2022-09-01</dc:date>
        <dc:source>ISO/TS 10303-4000</dc:source>
        <dc:type>InWork</dc:type>
        <rdfs:comment xml:lang="en">An ObservedEnvironmentVersion is a specialization of EnvironmentVersion that identifies a particular version of an ObservedEnvironment.</rdfs:comment>
        <owl:versionInfo>1</owl:versionInfo>
        <skos:changeNote>[2021-07-30] Initial definition.</skos:changeNote>
        <skos:prefLabel xml:lang="en">observed environment version</skos:prefLabel>
    </owl:Class>
    


    <!-- http://standards.iso.org/iso/10303/tech/refdata/core#07bb893c-aa0b-468d-8204-dfe864c97528 -->

    <owl:Class rdf:about="http://standards.iso.org/iso/10303/tech/refdata/core#07bb893c-aa0b-468d-8204-dfe864c97528">
        <rdfs:subClassOf rdf:resource="http://standards.iso.org/iso/10303/tech/refdata/core#59b11220-3279-0135-b58f-598f1b1392ae"/>
        <dc:contributor>STEP Harmonization Team</dc:contributor>
        <dc:creator>Phil Spiby, Eurostep</dc:creator>
        <dc:date>2022-09-01</dc:date>
        <dc:source>ISO/TS 10303-4000</dc:source>
        <dc:type>InWork</dc:type>
        <rdfs:comment xml:lang="en">An ObservedEnvironmentViewRelationship is a relationship between two ObservedEnvironmentView objects.</rdfs:comment>
        <owl:versionInfo>2</owl:versionInfo>
        <skos:changeNote>[2021-07-30] Initial definition.</skos:changeNote>
        <skos:changeNote>[2022-09-01] Phil Spiby, Eurostep: updated comment.</skos:changeNote>
        <skos:prefLabel xml:lang="en">observed environment view relationship</skos:prefLabel>
    </owl:Class>
    


    <!-- http://standards.iso.org/iso/10303/tech/refdata/core#085b6771-a1f8-4cf7-9771-8de2f3a063a1 -->

    <owl:Class rdf:about="http://standards.iso.org/iso/10303/tech/refdata/core#085b6771-a1f8-4cf7-9771-8de2f3a063a1">
        <rdfs:subClassOf rdf:resource="http://standards.iso.org/iso/10303/tech/refdata/core#1d59c650-3279-0135-b58f-598f1b1392ae"/>
        <dc:contributor>STEP Harmonization Team</dc:contributor>
        <dc:creator>Phil Spiby, Eurostep</dc:creator>
        <dc:date>2022-09-01</dc:date>
        <dc:source>ISO/TS 10303-4000</dc:source>
        <dc:type>InWork</dc:type>
        <rdfs:comment xml:lang="en">A StateDefinitionStateAssociation is used to associate a State to a StateDefinition.</rdfs:comment>
        <owl:versionInfo>2</owl:versionInfo>
        <skos:changeNote>[2021-07-30] Initial definition.</skos:changeNote>
        <skos:changeNote>[2022-09-01] Phil Spiby, Eurostep: updated comment.</skos:changeNote>
        <skos:prefLabel xml:lang="en">state definition state association</skos:prefLabel>
    </owl:Class>
    


    <!-- http://standards.iso.org/iso/10303/tech/refdata/core#09cd1ad9-ed18-4c44-a399-eb27b8148d42 -->

    <owl:Class rdf:about="http://standards.iso.org/iso/10303/tech/refdata/core#09cd1ad9-ed18-4c44-a399-eb27b8148d42">
        <rdfs:subClassOf rdf:resource="http://standards.iso.org/iso/10303/tech/refdata/core#36d7b46c-2554-494b-83d3-26668554cff4"/>
        <dc:contributor>STEP Harmonization Team</dc:contributor>
        <dc:creator>Jean Brangé, AFNeT Services</dc:creator>
        <dc:date>2023-10-04</dc:date>
        <dc:source>ISO/TS 10303-4000</dc:source>
        <dc:type>InWork</dc:type>
        <rdfs:comment xml:lang="en">An OccurrenceTerminal is a type of OccurrenceContactFeature that can be joined with another OccurrenceTerminal for the purpose of transporting information, energy or matter.</rdfs:comment>
        <owl:versionInfo>3</owl:versionInfo>
        <skos:changeNote>[2023-10-04] Jean Brangé, AFNeT Services: Initial definition.</skos:changeNote>
        <skos:prefLabel xml:lang="en">occurrence terminal</skos:prefLabel>
    </owl:Class>
    


    <!-- http://standards.iso.org/iso/10303/tech/refdata/core#09dab389-8ca9-4dc9-b785-b1fe10d5bfa4 -->

    <owl:Class rdf:about="http://standards.iso.org/iso/10303/tech/refdata/core#09dab389-8ca9-4dc9-b785-b1fe10d5bfa4">
        <rdfs:subClassOf rdf:resource="http://standards.iso.org/iso/10303/tech/refdata/core#1d59c650-3279-0135-b58f-598f1b1392ae"/>
        <dc:contributor>STEP Harmonization Team</dc:contributor>
        <dc:creator>Jean Brangé, AFNeT Services</dc:creator>
        <dc:date>2023-10-04</dc:date>
        <dc:source>ISO/TS 10303-4000</dc:source>
        <dc:type>InWork</dc:type>
        <rdfs:comment xml:lang="en">A ProductStructureKinematicPathAssociation is an association of one KinematicsPathDefinedByNodes within the items of a LinkMotionAlongPath and one Occurrence within an AssemblyDefinition.</rdfs:comment>
        <owl:versionInfo>3</owl:versionInfo>
        <skos:changeNote>[2023-10-04] Jean Brangé, AFNeT Services: Initial definition.</skos:changeNote>
        <skos:note xml:lang="en">A ProductStructureKinematicsPathAssociation can be used instead of a combination of LinkMotionTransformation, LinkMotionRelationship and ProductStructureLinkMotionAssociation for the case that the underlying PartView has only one geometric Model associated to it and that LinkMotionTransformation.TransformItem1 is equal to an AxisPlacement with no translation and no rotation.</skos:note>
        <skos:prefLabel xml:lang="en">product structure kinematic path association</skos:prefLabel>
    </owl:Class>
    


    <!-- http://standards.iso.org/iso/10303/tech/refdata/core#09fe3ee7-43ac-4580-a2da-cd21f908be21 -->

    <owl:Class rdf:about="http://standards.iso.org/iso/10303/tech/refdata/core#09fe3ee7-43ac-4580-a2da-cd21f908be21">
        <rdfs:subClassOf rdf:resource="http://standards.iso.org/iso/10303/tech/refdata/core#59b11220-3279-0135-b58f-598f1b1392ae"/>
        <dc:contributor>STEP Harmonization Team</dc:contributor>
        <dc:creator>Phil Spiby, Eurostep</dc:creator>
        <dc:date>2022-09-01</dc:date>
        <dc:source>ISO/TS 10303-4000</dc:source>
        <dc:type>InWork</dc:type>
        <rdfs:comment xml:lang="en">An ObservationRelationship is a relationship between two Observation objects.</rdfs:comment>
        <owl:versionInfo>1</owl:versionInfo>
        <skos:changeNote>[2022-09-01] Initial definition.</skos:changeNote>
        <skos:prefLabel xml:lang="en">observation relationship</skos:prefLabel>
    </owl:Class>
    


    <!-- http://standards.iso.org/iso/10303/tech/refdata/core#090b6b7b-3b3e-4da7-b3f3-1d43aa326c8c -->

    <owl:Class rdf:about="http://standards.iso.org/iso/10303/tech/refdata/core#090b6b7b-3b3e-4da7-b3f3-1d43aa326c8c">
        <rdfs:subClassOf rdf:resource="http://standards.iso.org/iso/10303/tech/refdata/core#9c98fe40-130a-0135-b552-598f1b1392ae"/>
        <dc:contributor>STEP Harmonization Team</dc:contributor>
        <dc:creator>Jean Brangé, AFNeT Services</dc:creator>
        <dc:date>2023-10-04</dc:date>
        <dc:source>ISO/TS 10303-4000</dc:source>
        <dc:type>InWork</dc:type>
        <rdfs:comment xml:lang="en">An ExternalShellBasedWireframeShapeRepresentation is a type of ExternalGeometricModel that references an instance of type ../../../resources/aic_shell_based_wireframe/aic_shell_based_wireframe.htm#aic_shell_based_wireframe.shell_based_wireframe_shape_representation shell_based_wireframe_shape_representation (ISO 10303-502).</rdfs:comment>
        <owl:versionInfo>3</owl:versionInfo>
        <skos:changeNote>[2023-10-04] Jean Brangé, AFNeT Services: Initial definition.</skos:changeNote>
        <skos:prefLabel xml:lang="en">external shell based wireframe shape representation</skos:prefLabel>
    </owl:Class>
    


    <!-- http://standards.iso.org/iso/10303/tech/refdata/core#0931f9ce-62c3-4fa3-857c-2ec7a5076d84 -->

    <owl:Class rdf:about="http://standards.iso.org/iso/10303/tech/refdata/core#0931f9ce-62c3-4fa3-857c-2ec7a5076d84">
        <rdfs:subClassOf rdf:resource="http://standards.iso.org/iso/10303/tech/refdata/core#95f1bde5-b263-4ca1-89df-33e1205800dd"/>
        <dc:contributor>STEP Harmonization Team</dc:contributor>
        <dc:creator>Phil Spiby, Eurostep</dc:creator>
        <dc:date>2022-09-01</dc:date>
        <dc:source>ISO/TS 10303-4000</dc:source>
        <dc:type>InWork</dc:type>
        <rdfs:comment xml:lang="en">An ExitLoop is a type of StructuredTaskElement. It signifies a pointat which to exit from a loop.</rdfs:comment>
        <owl:versionInfo>1</owl:versionInfo>
        <skos:changeNote>[2021-07-30] Initial definition.</skos:changeNote>
        <skos:prefLabel xml:lang="en">exit loop</skos:prefLabel>
    </owl:Class>
    


    <!-- http://standards.iso.org/iso/10303/tech/refdata/core#097ff096-073a-4dc1-b2dc-444297eb94e6 -->

    <owl:Class rdf:about="http://standards.iso.org/iso/10303/tech/refdata/core#097ff096-073a-4dc1-b2dc-444297eb94e6">
        <rdfs:subClassOf rdf:resource="http://standards.iso.org/iso/10303/tech/refdata/core#STEPThing"/>
        <dc:contributor>STEP Harmonization Team</dc:contributor>
        <dc:creator>Phil Spiby, Eurostep</dc:creator>
        <dc:date>2022-09-01</dc:date>
        <dc:source>ISO/TS 10303-4000</dc:source>
        <dc:type>InWork</dc:type>
        <rdfs:comment xml:lang="en">A RiskVersion defines a form of a risk that differ in certain respects from an earlier form of that risk or from other forms of that risk.</rdfs:comment>
        <owl:versionInfo>1</owl:versionInfo>
        <skos:changeNote>[2022-09-01] Initial definition.</skos:changeNote>
        <skos:note xml:lang="en">Use of RiskVersion allows several RiskPerception instances to be assigned to a specific Risk.</skos:note>
        <skos:prefLabel xml:lang="en">risk version</skos:prefLabel>
    </owl:Class>
    


    <!-- http://standards.iso.org/iso/10303/tech/refdata/core#1ab6f279-97db-4102-9cb3-76462f5db8d9 -->

    <owl:Class rdf:about="http://standards.iso.org/iso/10303/tech/refdata/core#1ab6f279-97db-4102-9cb3-76462f5db8d9">
        <rdfs:subClassOf rdf:resource="http://standards.iso.org/iso/10303/tech/refdata/core#STEPThing"/>
        <dc:contributor>STEP Harmonization Team</dc:contributor>
        <dc:creator>Jean Brangé, AFNeT Services</dc:creator>
        <dc:date>2023-10-04</dc:date>
        <dc:source>ISO/TS 10303-4000</dc:source>
        <dc:type>InWork</dc:type>
        <rdfs:comment xml:lang="en">A ShapeFeatureDefinition defines the shape of a feature either by an explicit GeometricModel or by an implicit GeometricModel that is defined by parameters.</rdfs:comment>
        <owl:versionInfo>3</owl:versionInfo>
        <skos:changeNote>[2023-10-04] Jean Brangé, AFNeT Services: Initial definition.</skos:changeNote>
        <skos:prefLabel xml:lang="en">shape feature definition</skos:prefLabel>
    </owl:Class>
    


    <!-- http://standards.iso.org/iso/10303/tech/refdata/core#1acc8c1f-51e7-44ff-8e17-b151b6e5a43e -->

    <owl:Class rdf:about="http://standards.iso.org/iso/10303/tech/refdata/core#1acc8c1f-51e7-44ff-8e17-b151b6e5a43e">
        <rdfs:subClassOf rdf:resource="http://standards.iso.org/iso/10303/tech/refdata/core#1d59c650-3279-0135-b58f-598f1b1392ae"/>
        <dc:contributor>STEP Harmonization Team</dc:contributor>
        <dc:creator>Jean Brangé, AFNeT Services</dc:creator>
        <dc:date>2023-10-04</dc:date>
        <dc:source>ISO/TS 10303-4000</dc:source>
        <dc:type>InWork</dc:type>
        <rdfs:comment xml:lang="en">A KinematicMechanismAssociation is an association of a Mechanism to an AssemblyDefinition.</rdfs:comment>
        <owl:versionInfo>3</owl:versionInfo>
        <skos:changeNote>[2023-10-04] Jean Brangé, AFNeT Services: Initial definition.</skos:changeNote>
        <skos:prefLabel xml:lang="en">kinematic mechanism association</skos:prefLabel>
    </owl:Class>
    


    <!-- http://standards.iso.org/iso/10303/tech/refdata/core#1bc8420c-9fbb-49bd-b87b-925f9889e05e -->

    <owl:Class rdf:about="http://standards.iso.org/iso/10303/tech/refdata/core#1bc8420c-9fbb-49bd-b87b-925f9889e05e">
        <rdfs:subClassOf rdf:resource="http://standards.iso.org/iso/10303/tech/refdata/core#59b11220-3279-0135-b58f-598f1b1392ae"/>
        <dc:contributor>STEP Harmonization Team</dc:contributor>
        <dc:creator>Phil Spiby, Eurostep</dc:creator>
        <dc:date>2022-09-01</dc:date>
        <dc:source>ISO/TS 10303-4000</dc:source>
        <dc:type>InWork</dc:type>
        <rdfs:comment xml:lang="en">A RequiredResourceRelationship is a relationship between two RequiredResource objects.</rdfs:comment>
        <owl:versionInfo>2</owl:versionInfo>
        <skos:changeNote>[2021-07-30] Initial definition.</skos:changeNote>
        <skos:changeNote>[2022-09-01] Phil Spiby, Eurostep: updated comment updated example.</skos:changeNote>
        <skos:example xml:lang="en">&quot;alternative&quot; and &quot;realized by&quot; are examples of required resource relationship.</skos:example>
        <skos:prefLabel xml:lang="en">required resource relationship</skos:prefLabel>
    </owl:Class>
    


    <!-- http://standards.iso.org/iso/10303/tech/refdata/core#1bf34880-abc0-40ab-a68f-547aa4ead243 -->

    <owl:Class rdf:about="http://standards.iso.org/iso/10303/tech/refdata/core#1bf34880-abc0-40ab-a68f-547aa4ead243">
        <rdfs:subClassOf rdf:resource="http://standards.iso.org/iso/10303/tech/refdata/core#44078e31-a1cb-4d89-b8d6-ab60b9140b06"/>
        <dc:contributor>STEP Harmonization Team</dc:contributor>
        <dc:creator>Jean Brangé, AFNeT Services</dc:creator>
        <dc:date>2023-10-04</dc:date>
        <dc:source>ISO/TS 10303-4000</dc:source>
        <dc:type>InWork</dc:type>
        <rdfs:comment xml:lang="en">A TargetStraightLine is a type of PlacedTarget that specifies a DatumTarget that is defined by an implicit straight line. The first end point of the TargetStraightLine is specified by the placing AxisPlacement. The second end point is located on the z-axis of the AxisPlacement at the specified distance.</rdfs:comment>
        <owl:versionInfo>3</owl:versionInfo>
        <skos:changeNote>[2023-10-04] Jean Brangé, AFNeT Services: Initial definition.</skos:changeNote>
        <skos:prefLabel xml:lang="en">target straight line</skos:prefLabel>
    </owl:Class>
    


    <!-- http://standards.iso.org/iso/10303/tech/refdata/core#1bf792d2-2dcc-4f71-9a0c-0245f6a0a7dd -->

    <owl:Class rdf:about="http://standards.iso.org/iso/10303/tech/refdata/core#1bf792d2-2dcc-4f71-9a0c-0245f6a0a7dd">
        <rdfs:subClassOf rdf:resource="http://standards.iso.org/iso/10303/tech/refdata/core#f8816baf-d66a-42f9-bdcc-38e946c9a2fa"/>
        <dc:contributor>STEP Harmonization Team</dc:contributor>
        <dc:creator>Jean Brangé, AFNeT Services</dc:creator>
        <dc:date>2023-10-04</dc:date>
        <dc:source>ISO/TS 10303-4000</dc:source>
        <dc:type>InWork</dc:type>
        <rdfs:comment xml:lang="en">A GeometricIntersection is a type of DerivedShapeElement that is the common intersection of two or more ShapeElements.</rdfs:comment>
        <owl:versionInfo>3</owl:versionInfo>
        <skos:changeNote>[2023-10-04] Jean Brangé, AFNeT Services: Initial definition.</skos:changeNote>
        <skos:example xml:lang="en">A GeometricIntersection is established by the intersection of two planar extensions from the adjacent sides of the block.</skos:example>
        <skos:note xml:lang="en">Since a GeometricIntersection is a derived shape, the use of intersection here is independent of any specific representation.</skos:note>
        <skos:prefLabel xml:lang="en">geometric intersection</skos:prefLabel>
    </owl:Class>
    


    <!-- http://standards.iso.org/iso/10303/tech/refdata/core#1c31126a-cb7c-471f-8be3-ecc1bc82d02f -->

    <owl:Class rdf:about="http://standards.iso.org/iso/10303/tech/refdata/core#1c31126a-cb7c-471f-8be3-ecc1bc82d02f">
        <rdfs:subClassOf rdf:resource="http://standards.iso.org/iso/10303/tech/refdata/core#78133794-f9d2-4e22-aaa0-49690cc93a39"/>
        <dc:contributor>STEP Harmonization Team</dc:contributor>
        <dc:creator>Jean Brangé, AFNeT Services</dc:creator>
        <dc:date>2023-10-04</dc:date>
        <dc:source>ISO/TS 10303-4000</dc:source>
        <dc:type>InWork</dc:type>
        <rdfs:comment xml:lang="en">A CrossSectionalGroupShapeElementWithTubularCover is a type of CrossSectionalGroupShapeElement where the group members are enclosed in a tubular cover.</rdfs:comment>
        <owl:versionInfo>3</owl:versionInfo>
        <skos:changeNote>[2023-10-04] Jean Brangé, AFNeT Services: Initial definition.</skos:changeNote>
        <skos:prefLabel xml:lang="en">cross sectional group shape element with tubular cover</skos:prefLabel>
    </owl:Class>
    


    <!-- http://standards.iso.org/iso/10303/tech/refdata/core#1c70c4cf-4e43-4b6f-9fc4-bfd4e54749d3 -->

    <owl:Class rdf:about="http://standards.iso.org/iso/10303/tech/refdata/core#1c70c4cf-4e43-4b6f-9fc4-bfd4e54749d3">
        <rdfs:subClassOf rdf:resource="http://standards.iso.org/iso/10303/tech/refdata/core#0ccba30b-b471-4863-8f01-c941e53bcf1a"/>
        <dc:contributor>STEP Harmonization Team</dc:contributor>
        <dc:creator>Phil Spiby, Eurostep</dc:creator>
        <dc:date>2022-09-01</dc:date>
        <dc:source>ISO/TS 10303-4000</dc:source>
        <dc:type>InWork</dc:type>
        <rdfs:comment xml:lang="en">A ResourceGroupRelationship is a specialization of ResourceItemRelationship that is a relationship between two ResourceItem objects that are part of a resource group.</rdfs:comment>
        <owl:versionInfo>2</owl:versionInfo>
        <skos:changeNote>[2021-07-30] Initial definition.</skos:changeNote>
        <skos:changeNote>[2022-09-01] Phil Spiby, Eurostep: updated comment updated example.</skos:changeNote>
        <skos:example xml:lang="en">The relationship between a facility and compressed air could be classified as &quot;Provides&quot;.</skos:example>
        <skos:example xml:lang="en">The relationship between a tool set and a mallet could be classified as &quot;Contains&quot;.</skos:example>
        <skos:prefLabel xml:lang="en">resource group relationship</skos:prefLabel>
    </owl:Class>
    


    <!-- http://standards.iso.org/iso/10303/tech/refdata/core#1cfca290-3279-0135-b58f-598f1b1392ae -->

    <owl:Class rdf:about="http://standards.iso.org/iso/10303/tech/refdata/core#1cfca290-3279-0135-b58f-598f1b1392ae">
        <rdfs:subClassOf rdf:resource="http://standards.iso.org/iso/10303/tech/refdata/core#STEPThing"/>
        <dc:contributor>STEP Harmonization Team</dc:contributor>
        <dc:creator>Phil Spiby, Eurostep</dc:creator>
        <dc:date>2022-09-01</dc:date>
        <dc:source>ISO/TS 10303-4000</dc:source>
        <dc:type>InWork</dc:type>
        <rdfs:comment xml:lang="en">An AssignmentObject is a generalization of all assignments in the Core model used to identify common properties of assignments.</rdfs:comment>
        <owl:versionInfo>2</owl:versionInfo>
        <skos:changeNote>[2021-07-30] Initial definition.</skos:changeNote>
        <skos:changeNote>[2022-09-01] Phil Spiby, Eurostep: updated note.</skos:changeNote>
        <skos:note xml:lang="en">An assignment implies a direction from an object to a target object.</skos:note>
        <skos:note xml:lang="en">The object being assigned is normally, but not always, of a different type to the target of the assignment.</skos:note>
        <skos:prefLabel xml:lang="en">assignment object</skos:prefLabel>
    </owl:Class>
    


    <!-- http://standards.iso.org/iso/10303/tech/refdata/core#1d59c650-3279-0135-b58f-598f1b1392ae -->

    <owl:Class rdf:about="http://standards.iso.org/iso/10303/tech/refdata/core#1d59c650-3279-0135-b58f-598f1b1392ae">
        <rdfs:subClassOf rdf:resource="http://standards.iso.org/iso/10303/tech/refdata/core#STEPThing"/>
        <dc:contributor>STEP Harmonization Team</dc:contributor>
        <dc:creator>Phil Spiby, Eurostep</dc:creator>
        <dc:date>2022-09-01</dc:date>
        <dc:source>ISO/TS 10303-4000</dc:source>
        <dc:type>InWork</dc:type>
        <rdfs:comment xml:lang="en">An AssociationObject is a generalization of all associations in the Core model use to identify common properties of associations. An association is defined as a link between two dissimilar objects.</rdfs:comment>
        <owl:versionInfo>1</owl:versionInfo>
        <skos:changeNote>[2021-07-30] Initial definition.</skos:changeNote>
        <skos:note xml:lang="en">An association implies no directionality or precedence between the objects.</skos:note>
        <skos:prefLabel xml:lang="en">association object</skos:prefLabel>
    </owl:Class>
    


    <!-- http://standards.iso.org/iso/10303/tech/refdata/core#1dd0c3c0-c7a2-4304-ba36-545f64255ed3 -->

    <owl:Class rdf:about="http://standards.iso.org/iso/10303/tech/refdata/core#1dd0c3c0-c7a2-4304-ba36-545f64255ed3">
        <rdfs:subClassOf rdf:resource="http://standards.iso.org/iso/10303/tech/refdata/core#66348150-092a-4eb7-9561-0b83adfa15ff"/>
        <dc:contributor>STEP Harmonization Team</dc:contributor>
        <dc:creator>Jean Brangé, AFNeT Services</dc:creator>
        <dc:date>2023-10-04</dc:date>
        <dc:source>ISO/TS 10303-4000</dc:source>
        <dc:type>InWork</dc:type>
        <rdfs:comment xml:lang="en">An AxisPlacementShapeElement is a type of ShapeElement that is associated with an AxisPlacement.</rdfs:comment>
        <owl:versionInfo>3</owl:versionInfo>
        <skos:changeNote>[2023-10-04] Jean Brangé, AFNeT Services: Initial definition.</skos:changeNote>
        <skos:prefLabel xml:lang="en">axis placement shape element</skos:prefLabel>
    </owl:Class>
    


    <!-- http://standards.iso.org/iso/10303/tech/refdata/core#1eb137c7-fe4e-4e82-8a0a-179b465c2dd6 -->

    <owl:Class rdf:about="http://standards.iso.org/iso/10303/tech/refdata/core#1eb137c7-fe4e-4e82-8a0a-179b465c2dd6">
        <rdfs:subClassOf rdf:resource="http://standards.iso.org/iso/10303/tech/refdata/core#55105ef0-713f-409a-8306-fd8708d4ee3f"/>
        <dc:contributor>STEP Harmonization Team</dc:contributor>
        <dc:creator>Jean Brangé, AFNeT Services</dc:creator>
        <dc:date>2023-10-04</dc:date>
        <dc:source>ISO/TS 10303-4000</dc:source>
        <dc:type>InWork</dc:type>
        <rdfs:comment xml:lang="en">A PerpendicularityTolerance is a type of GeometricTolerance that is a constraint that specifies that a surface or a curve shall be perpendicular to a reference datum with an allowed amount of deviation. The reference datum is either a datum plane or a datum axis. A PerpendicularityTolerance specifies one of the following: a tolerance zone limited by two parallel planes perpendicular to a datum plane, or axis, within which the surface or median plane of the considered feature must lie; a tolerance zone limited by two parallel planes perpendicular to a datum axis, within which the axis of the considered feature must lie; a cylindrical tolerance zone (if the attribute DirectedOrOrientedToleranceZone is not specified), perpendicular to a datum plane, within which the axis of the considered feature must lie; a tolerance zone defined by two parallel lines perpendicular to a datum plane, or axis, within which an element of the surface must lie. Unless otherwise specified, the tolerance shall be used in accordance with perpendicularity tolerance in ISO 1101.</rdfs:comment>
        <owl:versionInfo>3</owl:versionInfo>
        <skos:changeNote>[2023-10-04] Jean Brangé, AFNeT Services: Initial definition.</skos:changeNote>
        <skos:note xml:lang="en">Alternatively perpendicularity tolerance can be used according to the specifications given in ASME Y14.5-2009.</skos:note>
        <skos:prefLabel xml:lang="en">perpendicularity tolerance</skos:prefLabel>
    </owl:Class>
    


    <!-- http://standards.iso.org/iso/10303/tech/refdata/core#1f0095b7-4bd7-4819-8f23-5ebcc8c45e62 -->

    <owl:Class rdf:about="http://standards.iso.org/iso/10303/tech/refdata/core#1f0095b7-4bd7-4819-8f23-5ebcc8c45e62">
        <rdfs:subClassOf rdf:resource="http://standards.iso.org/iso/10303/tech/refdata/core#93cfa9b1-4397-4dde-983a-b4ec8677a20f"/>
        <dc:contributor>STEP Harmonization Team</dc:contributor>
        <dc:creator>Jean Brangé, AFNeT Services</dc:creator>
        <dc:date>2023-10-04</dc:date>
        <dc:source>ISO/TS 10303-4000</dc:source>
        <dc:type>InWork</dc:type>
        <rdfs:comment xml:lang="en">A ShapeFeatureDefinitionOccurrenceElement is a type of ShapeFeatureDefinitionElement that is defined by a ShapeFeatureDefinition or a ShapeFeatureDefinitionElement.</rdfs:comment>
        <owl:versionInfo>3</owl:versionInfo>
        <skos:changeNote>[2023-10-04] Jean Brangé, AFNeT Services: Initial definition.</skos:changeNote>
        <skos:prefLabel xml:lang="en">shape feature definition occurrence element</skos:prefLabel>
    </owl:Class>
    


    <!-- http://standards.iso.org/iso/10303/tech/refdata/core#1f09cf40-e045-476a-b811-eb6e56de0ced -->

    <owl:Class rdf:about="http://standards.iso.org/iso/10303/tech/refdata/core#1f09cf40-e045-476a-b811-eb6e56de0ced">
        <rdfs:subClassOf rdf:resource="http://standards.iso.org/iso/10303/tech/refdata/core#c050712f-0dca-495e-aa7d-2b2e21af712b"/>
        <dc:contributor>STEP Harmonization Team</dc:contributor>
        <dc:creator>Jean Brangé, AFNeT Services</dc:creator>
        <dc:date>2023-10-04</dc:date>
        <dc:source>ISO/TS 10303-4000</dc:source>
        <dc:type>InWork</dc:type>
        <rdfs:comment xml:lang="en">A DimensionalLocation is a type of GeometricDimension that represents the specification of the distance or angle that one feature is displaced from another feature. A DimensionalLocation specifies that a spatial constraint exists between two ShapeElements that are represented as a non-directed measure applied along a measurement path. A DimensionalLocation is either an AngularLocation or a CurvedDistance, or a LinearDistance. dimensional_location_and_size.gifDimensional location and dimensional size</rdfs:comment>
        <owl:versionInfo>3</owl:versionInfo>
        <skos:changeNote>[2023-10-04] Jean Brangé, AFNeT Services: Initial definition.</skos:changeNote>
        <skos:example xml:lang="en">The centre of the hole is 10 centimetres from the short edge.</skos:example>
        <skos:example xml:lang="en">The short edge of a plate is located 90 degrees relative to the long edge.</skos:example>
        <skos:note xml:lang="en">Representation of a ShapeElement participating in the DimensionalLocation relationship implies a measuring direction for the DimensionalLocation through the related and relating ShapeElement. The meaning of the direction is specified in an application protocol.</skos:note>
        <skos:note xml:lang="en">The application and use of DimensionalLocation and DimensionalSize are shown in the Figure Dimensional location and dimensional size.</skos:note>
        <skos:prefLabel xml:lang="en">dimensional location</skos:prefLabel>
    </owl:Class>
    


    <!-- http://standards.iso.org/iso/10303/tech/refdata/core#10ceea51-75c7-48f8-a2d5-16bedc0559db -->

    <owl:Class rdf:about="http://standards.iso.org/iso/10303/tech/refdata/core#10ceea51-75c7-48f8-a2d5-16bedc0559db">
        <rdfs:subClassOf rdf:resource="http://standards.iso.org/iso/10303/tech/refdata/core#6d367e10-7640-4a8f-acaa-42963438a3aa"/>
        <dc:contributor>STEP Harmonization Team</dc:contributor>
        <dc:creator>Jean Brangé, AFNeT Services</dc:creator>
        <dc:date>2023-10-04</dc:date>
        <dc:source>ISO/TS 10303-4000</dc:source>
        <dc:type>InWork</dc:type>
        <rdfs:comment xml:lang="en">A DrapedOrientationAngle is a type of PlyOrientationAngle that defines a position and direction at a point within a part.</rdfs:comment>
        <owl:versionInfo>3</owl:versionInfo>
        <skos:changeNote>[2023-10-04] Jean Brangé, AFNeT Services: Initial definition.</skos:changeNote>
        <skos:note xml:lang="en">The warp direction of a fabric shall be placed in the specified direction prior to draping over the part. Once the fabric has been draped, the orientation angle at any given point must be derived from the draped shape of the fabric. The DrapedOrientationAngle will change in the part if the surface of the part has complex curvature.</skos:note>
        <skos:prefLabel xml:lang="en">draped orientation angle</skos:prefLabel>
    </owl:Class>
    


    <!-- http://standards.iso.org/iso/10303/tech/refdata/core#10d2993b-4896-4887-8535-844467faa30d -->

    <owl:Class rdf:about="http://standards.iso.org/iso/10303/tech/refdata/core#10d2993b-4896-4887-8535-844467faa30d">
        <rdfs:subClassOf rdf:resource="http://standards.iso.org/iso/10303/tech/refdata/core#STEPThing"/>
        <dc:contributor>STEP Harmonization Team</dc:contributor>
        <dc:creator>Phil Spiby, Eurostep</dc:creator>
        <dc:date>2022-09-01</dc:date>
        <dc:source>ISO/TS 10303-4000</dc:source>
        <dc:type>InWork</dc:type>
        <rdfs:comment xml:lang="en">A StateDefinition is a mode of being. In formal systems, a StateDefinition is the definition of a situation during which some (usually implicit) invariant condition holds.</rdfs:comment>
        <owl:versionInfo>1</owl:versionInfo>
        <skos:changeNote>[2021-07-30] Initial definition.</skos:changeNote>
        <skos:example xml:lang="en">The definition of the state, ”flying” is that the aircraft is off the ground.</skos:example>
        <skos:prefLabel xml:lang="en">state definition</skos:prefLabel>
    </owl:Class>
    


    <!-- http://standards.iso.org/iso/10303/tech/refdata/core#108e866d-f843-4ef5-b2a7-c5d62479e209 -->

    <owl:Class rdf:about="http://standards.iso.org/iso/10303/tech/refdata/core#108e866d-f843-4ef5-b2a7-c5d62479e209">
        <rdfs:subClassOf rdf:resource="http://standards.iso.org/iso/10303/tech/refdata/core#9fee6ad0-130a-0135-b552-598f1b1392ae"/>
        <dc:contributor>STEP Harmonization Team</dc:contributor>
        <dc:creator>Jean Brangé, AFNeT Services</dc:creator>
        <dc:date>2023-10-04</dc:date>
        <dc:source>ISO/TS 10303-4000</dc:source>
        <dc:type>InWork</dc:type>
        <rdfs:comment xml:lang="en">A LinkMotionAlongPath is a type of GeometricRepresentation for the definition of parameter or time coordinated movements of one or several links along paths in space.</rdfs:comment>
        <owl:versionInfo>3</owl:versionInfo>
        <skos:changeNote>[2023-10-04] Jean Brangé, AFNeT Services: Initial definition.</skos:changeNote>
        <skos:prefLabel xml:lang="en">link motion along path</skos:prefLabel>
    </owl:Class>
    


    <!-- http://standards.iso.org/iso/10303/tech/refdata/core#11e93d03-d8a0-47c0-8163-5114ac2a0c97 -->

    <owl:Class rdf:about="http://standards.iso.org/iso/10303/tech/refdata/core#11e93d03-d8a0-47c0-8163-5114ac2a0c97">
        <rdfs:subClassOf rdf:resource="http://standards.iso.org/iso/10303/tech/refdata/core#STEPThing"/>
        <dc:contributor>STEP Harmonization Team</dc:contributor>
        <dc:creator>Phil Spiby, Eurostep</dc:creator>
        <dc:date>2022-09-01</dc:date>
        <dc:source>ISO/TS 10303-4000</dc:source>
        <dc:type>InWork</dc:type>
        <rdfs:comment xml:lang="en">A ManagedResource is a representation of a resource that is provided with resource management capabilities. The role of a managed resource is specified by the ClassifiedAs attribute.</rdfs:comment>
        <owl:versionInfo>2</owl:versionInfo>
        <skos:changeNote>[2021-07-30] Initial definition.</skos:changeNote>
        <skos:changeNote>[2022-09-01] Phil Spiby, Eurostep: updated comment updated example.</skos:changeNote>
        <skos:example xml:lang="en">A managed resource can be classified as &quot;Stock line&quot;.</skos:example>
        <skos:prefLabel xml:lang="en">managed resource</skos:prefLabel>
    </owl:Class>
    


    <!-- http://standards.iso.org/iso/10303/tech/refdata/core#122f2085-66e8-4d76-9597-e242c965b9f5 -->

    <owl:Class rdf:about="http://standards.iso.org/iso/10303/tech/refdata/core#122f2085-66e8-4d76-9597-e242c965b9f5">
        <rdfs:subClassOf rdf:resource="http://standards.iso.org/iso/10303/tech/refdata/core#59b11220-3279-0135-b58f-598f1b1392ae"/>
        <dc:contributor>STEP Harmonization Team</dc:contributor>
        <dc:creator>Phil Spiby, Eurostep</dc:creator>
        <dc:date>2022-09-01</dc:date>
        <dc:source>ISO/TS 10303-4000</dc:source>
        <dc:type>InWork</dc:type>
        <rdfs:comment xml:lang="en">A ManagedResourceRelationship is a relationship between two ManagedResource objects.</rdfs:comment>
        <owl:versionInfo>2</owl:versionInfo>
        <skos:changeNote>[2021-07-30] Initial definition.</skos:changeNote>
        <skos:changeNote>[2022-09-01] Phil Spiby, Eurostep: updated comment updated example.</skos:changeNote>
        <skos:example xml:lang="en">A managed resource relationship can be classified as &quot;Alternative&quot; or &quot;Preferred&quot;.</skos:example>
        <skos:prefLabel xml:lang="en">managed resource relationship</skos:prefLabel>
    </owl:Class>
    


    <!-- http://standards.iso.org/iso/10303/tech/refdata/core#14ece273-261a-4a3e-8d7b-3f4a91f60b4c -->

    <owl:Class rdf:about="http://standards.iso.org/iso/10303/tech/refdata/core#14ece273-261a-4a3e-8d7b-3f4a91f60b4c">
        <rdfs:subClassOf rdf:resource="http://standards.iso.org/iso/10303/tech/refdata/core#9c98fe40-130a-0135-b552-598f1b1392ae"/>
        <dc:contributor>STEP Harmonization Team</dc:contributor>
        <dc:creator>Jean Brangé, AFNeT Services</dc:creator>
        <dc:date>2023-10-04</dc:date>
        <dc:source>ISO/TS 10303-4000</dc:source>
        <dc:type>InWork</dc:type>
        <rdfs:comment xml:lang="en">An ExternalCurveSweptSolidShapeRepresentation is a type of ExternalGeometricModel that references an instance of type ../../../resources/aic_curve_swept_solid/aic_curve_swept_solid.htm#aic_curve_swept_solid.curve_swept_solid_shape_representationcurve_swept_solid_shape_representation (ISO 10303-523).</rdfs:comment>
        <owl:versionInfo>3</owl:versionInfo>
        <skos:changeNote>[2023-10-04] Jean Brangé, AFNeT Services: Initial definition.</skos:changeNote>
        <skos:prefLabel xml:lang="en">external curve swept solid shape representation</skos:prefLabel>
    </owl:Class>
    


    <!-- http://standards.iso.org/iso/10303/tech/refdata/core#1512eba2-2b3a-4058-a5c8-3189e9af42b8 -->

    <owl:Class rdf:about="http://standards.iso.org/iso/10303/tech/refdata/core#1512eba2-2b3a-4058-a5c8-3189e9af42b8">
        <rdfs:subClassOf rdf:resource="http://standards.iso.org/iso/10303/tech/refdata/core#c565c970-130a-0135-b552-598f1b1392ae"/>
        <dc:contributor>STEP Harmonization Team</dc:contributor>
        <dc:creator>Jean Brangé, AFNeT Services</dc:creator>
        <dc:date>2023-10-04</dc:date>
        <dc:source>ISO/TS 10303-4000</dc:source>
        <dc:type>InWork</dc:type>
        <rdfs:comment xml:lang="en">A PlyAngleRepresentation is a type of Representation. The PlyAngleRepresentation specifies the value of the angle for the PlyOrientationAngle Domain Object.</rdfs:comment>
        <owl:versionInfo>3</owl:versionInfo>
        <skos:changeNote>[2023-10-04] Jean Brangé, AFNeT Services: Initial definition.</skos:changeNote>
        <skos:prefLabel xml:lang="en">ply angle representation</skos:prefLabel>
    </owl:Class>
    


    <!-- http://standards.iso.org/iso/10303/tech/refdata/core#1602d3ca-c730-4445-a567-3a613e730d4d -->

    <owl:Class rdf:about="http://standards.iso.org/iso/10303/tech/refdata/core#1602d3ca-c730-4445-a567-3a613e730d4d">
        <rdfs:subClassOf rdf:resource="http://standards.iso.org/iso/10303/tech/refdata/core#9f656069-ff2c-4f09-9091-f91388a14764"/>
        <dc:contributor>STEP Harmonization Team</dc:contributor>
        <dc:creator>Phil Spiby, Eurostep</dc:creator>
        <dc:date>2022-09-01</dc:date>
        <dc:source>ISO/TS 10303-4000</dc:source>
        <dc:type>InWork</dc:type>
        <rdfs:comment xml:lang="en">A StateCauseEffect is a type of StateRelationship and it relates two or more states as one Relating state causing particular resulting effect Related state(s). In turn, an effect state can become a new causing state yielding in yet more effect states.</rdfs:comment>
        <owl:versionInfo>2</owl:versionInfo>
        <skos:changeNote>[2021-07-30] Initial definition.</skos:changeNote>
        <skos:changeNote>[2022-09-01] Phil Spiby, Eurostep: updated comment.</skos:changeNote>
        <skos:prefLabel xml:lang="en">state cause effect</skos:prefLabel>
    </owl:Class>
    


    <!-- http://standards.iso.org/iso/10303/tech/refdata/core#167d2266-7301-4eef-8f2f-1421f0c5b04d -->

    <owl:Class rdf:about="http://standards.iso.org/iso/10303/tech/refdata/core#167d2266-7301-4eef-8f2f-1421f0c5b04d">
        <rdfs:subClassOf rdf:resource="http://standards.iso.org/iso/10303/tech/refdata/core#55105ef0-713f-409a-8306-fd8708d4ee3f"/>
        <dc:contributor>STEP Harmonization Team</dc:contributor>
        <dc:creator>Jean Brangé, AFNeT Services</dc:creator>
        <dc:date>2023-10-04</dc:date>
        <dc:source>ISO/TS 10303-4000</dc:source>
        <dc:type>InWork</dc:type>
        <rdfs:comment xml:lang="en">A CoaxialityTolerance is a type of GeometricTolerance that constrains a centre point or plane of a surface of revolution, or of circular elements, about a datum feature.</rdfs:comment>
        <owl:versionInfo>3</owl:versionInfo>
        <skos:changeNote>[2023-10-04] Jean Brangé, AFNeT Services: Initial definition.</skos:changeNote>
        <skos:note xml:lang="en">Alternatively coaxiality tolerance can be used according to the specifications given in ASME Y14.5-2009.</skos:note>
        <skos:note xml:lang="en">Some tolerancing standards require the use of position tolerance for control of coaxiality. Unless otherwise specified, the rules governing coaxiality tolerance defined in ISO 1101 shall apply.</skos:note>
        <skos:prefLabel xml:lang="en">coaxiality tolerance</skos:prefLabel>
    </owl:Class>
    


    <!-- http://standards.iso.org/iso/10303/tech/refdata/core#18e3f37e-107d-4d73-92d6-63f3e8444381 -->

    <owl:Class rdf:about="http://standards.iso.org/iso/10303/tech/refdata/core#18e3f37e-107d-4d73-92d6-63f3e8444381">
        <rdfs:subClassOf rdf:resource="http://standards.iso.org/iso/10303/tech/refdata/core#c4a27970-130a-0135-b552-598f1b1392ae"/>
        <dc:contributor>STEP Harmonization Team</dc:contributor>
        <dc:creator>Jean Brangé, AFNeT Services</dc:creator>
        <dc:date>2023-10-04</dc:date>
        <dc:source>ISO/TS 10303-4000</dc:source>
        <dc:type>InWork</dc:type>
        <rdfs:comment xml:lang="en">A CableOccurrence is a type of QuantifiedOccurrence that is an occurrence of a PartView having a specified length. This PartView shall be associated with a Part that is categorized as cable and also as raw_material_by_length (PartTypes).</rdfs:comment>
        <owl:versionInfo>3</owl:versionInfo>
        <skos:changeNote>[2023-10-04] Jean Brangé, AFNeT Services: Initial definition.</skos:changeNote>
        <skos:prefLabel xml:lang="en">cable occurrence</skos:prefLabel>
    </owl:Class>
    


    <!-- http://standards.iso.org/iso/10303/tech/refdata/core#1811507e-f76d-42ad-9656-c399ae1a6309 -->

    <owl:Class rdf:about="http://standards.iso.org/iso/10303/tech/refdata/core#1811507e-f76d-42ad-9656-c399ae1a6309">
        <rdfs:subClassOf rdf:resource="http://standards.iso.org/iso/10303/tech/refdata/core#50f7e4dc-2a92-41e8-a755-0fa506125b9f"/>
        <dc:contributor>STEP Harmonization Team</dc:contributor>
        <dc:creator>Jean Brangé, AFNeT Services</dc:creator>
        <dc:date>2023-10-04</dc:date>
        <dc:source>ISO/TS 10303-4000</dc:source>
        <dc:type>InWork</dc:type>
        <rdfs:comment xml:lang="en">A WireOccurrenceIdentification is a type of OccurrenceTransportFeature that identifies a specific colour code for the occurrence of a wire.</rdfs:comment>
        <owl:versionInfo>3</owl:versionInfo>
        <skos:changeNote>[2023-10-04] Jean Brangé, AFNeT Services: Initial definition.</skos:changeNote>
        <skos:prefLabel xml:lang="en">wire occurrence identification</skos:prefLabel>
    </owl:Class>
    


    <!-- http://standards.iso.org/iso/10303/tech/refdata/core#187e23b5-bc20-4c72-802a-49198ab0c9d7 -->

    <owl:Class rdf:about="http://standards.iso.org/iso/10303/tech/refdata/core#187e23b5-bc20-4c72-802a-49198ab0c9d7">
        <rdfs:subClassOf rdf:resource="http://standards.iso.org/iso/10303/tech/refdata/core#STEPThing"/>
        <dc:contributor>STEP Harmonization Team</dc:contributor>
        <dc:creator>Phil Spiby, Eurostep</dc:creator>
        <dc:date>2022-09-01</dc:date>
        <dc:source>ISO/TS 10303-4000</dc:source>
        <dc:type>InWork</dc:type>
        <rdfs:comment xml:lang="en">An InterfaceConnectorVersion identifies a version of an InterfaceConnector.</rdfs:comment>
        <owl:versionInfo>2</owl:versionInfo>
        <skos:changeNote>[2021-07-30] Initial definition.</skos:changeNote>
        <skos:changeNote>[2022-09-01] Phil Spiby, Eurostep: updated comment.</skos:changeNote>
        <skos:prefLabel xml:lang="en">interface connector version</skos:prefLabel>
    </owl:Class>
    


    <!-- http://standards.iso.org/iso/10303/tech/refdata/core#194f4960-d47b-404e-ba16-b83243da5a40 -->

    <owl:Class rdf:about="http://standards.iso.org/iso/10303/tech/refdata/core#194f4960-d47b-404e-ba16-b83243da5a40">
        <rdfs:subClassOf rdf:resource="http://standards.iso.org/iso/10303/tech/refdata/core#aeba1b40-130a-0135-b552-598f1b1392ae"/>
        <dc:contributor>STEP Harmonization Team</dc:contributor>
        <dc:creator>Jean Brangé, AFNeT Services</dc:creator>
        <dc:date>2023-10-04</dc:date>
        <dc:source>ISO/TS 10303-4000</dc:source>
        <dc:type>InWork</dc:type>
        <rdfs:comment xml:lang="en">A SameTimeMachiningRelationship is a type of OccurrenceRelationship relationship between two Occurrence objects that specifies that those two objects shall be manufactured together within the same ProcessOperationOccurrence. sametimemachiningrelationship.png Illustration of SameTimeMachiningRelationship</rdfs:comment>
        <owl:versionInfo>3</owl:versionInfo>
        <skos:changeNote>[2023-10-04] Jean Brangé, AFNeT Services: Initial definition.</skos:changeNote>
        <skos:example xml:lang="en">The following figure shows an example for this case.</skos:example>
        <skos:prefLabel xml:lang="en">same time machining relationship</skos:prefLabel>
    </owl:Class>
    


    <!-- http://standards.iso.org/iso/10303/tech/refdata/core#19573db2-1baa-4bad-acc6-010eef852d49 -->

    <owl:Class rdf:about="http://standards.iso.org/iso/10303/tech/refdata/core#19573db2-1baa-4bad-acc6-010eef852d49">
        <rdfs:subClassOf rdf:resource="http://standards.iso.org/iso/10303/tech/refdata/core#STEPThing"/>
        <dc:contributor>STEP Harmonization Team</dc:contributor>
        <dc:creator>Phil Spiby, Eurostep</dc:creator>
        <dc:date>2022-09-01</dc:date>
        <dc:source>ISO/TS 10303-4000</dc:source>
        <dc:type>InWork</dc:type>
        <rdfs:comment xml:lang="en">A State is a mode of being in which something does, could, or did exist for a period of time.</rdfs:comment>
        <owl:versionInfo>2</owl:versionInfo>
        <skos:changeNote>[2021-07-30] Initial definition.</skos:changeNote>
        <skos:changeNote>[2022-09-01] Phil Spiby, Eurostep: updated example updated note.</skos:changeNote>
        <skos:example xml:lang="en">Main Engine No. 1 is in &apos;operation&apos;.</skos:example>
        <skos:example xml:lang="en">The portable computer&apos;s power supply was attached after it displayed a &apos;low-battery&apos; warning.</skos:example>
        <skos:example xml:lang="en">When Generator No. 2 surpasses 5,000 service hours, it will enter &apos;maintenance&apos; mode.</skos:example>
        <skos:note xml:lang="en">A state&apos;s existence can be just a state that an object is currently in, a predicted state that an object will eventually be in, or an observed state that an object has been in.</skos:note>
        <skos:note xml:lang="en">The period of existence can be an instant or longer.</skos:note>
        <skos:prefLabel xml:lang="en">state</skos:prefLabel>
    </owl:Class>
    


    <!-- http://standards.iso.org/iso/10303/tech/refdata/core#197fdcb4-0ed5-435c-8677-523c531c796c -->

    <owl:Class rdf:about="http://standards.iso.org/iso/10303/tech/refdata/core#197fdcb4-0ed5-435c-8677-523c531c796c">
        <rdfs:subClassOf rdf:resource="http://standards.iso.org/iso/10303/tech/refdata/core#1d59c650-3279-0135-b58f-598f1b1392ae"/>
        <dc:contributor>STEP Harmonization Team</dc:contributor>
        <dc:creator>Phil Spiby, Eurostep</dc:creator>
        <dc:date>2022-09-01</dc:date>
        <dc:source>ISO/TS 10303-4000</dc:source>
        <dc:type>InWork</dc:type>
        <rdfs:comment xml:lang="en">A PositionGroupAssociation is an association that specifies the participation of a position in a group.</rdfs:comment>
        <owl:versionInfo>1</owl:versionInfo>
        <skos:changeNote>[2022-09-01] Initial definition.</skos:changeNote>
        <skos:prefLabel xml:lang="en">position group association</skos:prefLabel>
    </owl:Class>
    


    <!-- http://standards.iso.org/iso/10303/tech/refdata/core#2a1e05d9-75de-4a93-9628-fdcee577f278 -->

    <owl:Class rdf:about="http://standards.iso.org/iso/10303/tech/refdata/core#2a1e05d9-75de-4a93-9628-fdcee577f278">
        <rdfs:subClassOf rdf:resource="http://standards.iso.org/iso/10303/tech/refdata/core#59b11220-3279-0135-b58f-598f1b1392ae"/>
        <dc:contributor>STEP Harmonization Team</dc:contributor>
        <dc:creator>Phil Spiby, Eurostep</dc:creator>
        <dc:date>2022-09-01</dc:date>
        <dc:source>ISO/TS 10303-4000</dc:source>
        <dc:type>InWork</dc:type>
        <rdfs:comment xml:lang="en">A ConditionEvaluationRelationship is a relationship between two ConditionEvaluation objects.</rdfs:comment>
        <owl:versionInfo>2</owl:versionInfo>
        <skos:changeNote>[2021-07-30] Initial definition.</skos:changeNote>
        <skos:changeNote>[2022-09-01] Phil Spiby, Eurostep: updated comment.</skos:changeNote>
        <skos:prefLabel xml:lang="en">condition evaluation relationship</skos:prefLabel>
    </owl:Class>
    


    <!-- http://standards.iso.org/iso/10303/tech/refdata/core#2aba8839-cb83-4e21-9de8-968c250a9ebc -->

    <owl:Class rdf:about="http://standards.iso.org/iso/10303/tech/refdata/core#2aba8839-cb83-4e21-9de8-968c250a9ebc">
        <rdfs:subClassOf rdf:resource="http://standards.iso.org/iso/10303/tech/refdata/core#5a6c8b1f-63af-4307-9faf-9fdd6da5572c"/>
        <dc:contributor>STEP Harmonization Team</dc:contributor>
        <dc:creator>Jean Brangé, AFNeT Services</dc:creator>
        <dc:date>2023-10-04</dc:date>
        <dc:source>ISO/TS 10303-4000</dc:source>
        <dc:type>InWork</dc:type>
        <rdfs:comment xml:lang="en">A ProcessedCore is a type of ConstituentPart that is the central component of a sandwich construction to which faces, or skins are attached. The primary structural purpose of ProcessedCore is the transfer of shear loads between the faces or skins. ProcessedCore is StockMaterial that has been machined, formed, stabilized and/or bonded together (see following figure ). A core may have a potting compound or adhesive applied to it to make it more rigid and/or provide solid attachment points. ProcessedCore.pngProcessed core</rdfs:comment>
        <owl:versionInfo>3</owl:versionInfo>
        <skos:changeNote>[2023-10-04] Jean Brangé, AFNeT Services: Initial definition.</skos:changeNote>
        <skos:prefLabel xml:lang="en">processed core</skos:prefLabel>
    </owl:Class>
    


    <!-- http://standards.iso.org/iso/10303/tech/refdata/core#2bb924a1-788a-417e-a7c8-d1fa06ce3a2b -->

    <owl:Class rdf:about="http://standards.iso.org/iso/10303/tech/refdata/core#2bb924a1-788a-417e-a7c8-d1fa06ce3a2b">
        <rdfs:subClassOf rdf:resource="http://standards.iso.org/iso/10303/tech/refdata/core#53e20541-4d83-4902-a059-b807ec6e0f42"/>
        <dc:contributor>STEP Harmonization Team</dc:contributor>
        <dc:creator>Phil Spiby, Eurostep</dc:creator>
        <dc:date>2022-09-01</dc:date>
        <dc:source>ISO/TS 10303-4000</dc:source>
        <dc:type>InWork</dc:type>
        <rdfs:comment xml:lang="en">A StateDefinitionTransition represents a transition between two StateDefinition, identified respectively as a start and an end.</rdfs:comment>
        <owl:versionInfo>1</owl:versionInfo>
        <skos:changeNote>[2021-07-30] Initial definition.</skos:changeNote>
        <skos:prefLabel xml:lang="en">state definition transition</skos:prefLabel>
    </owl:Class>
    


    <!-- http://standards.iso.org/iso/10303/tech/refdata/core#2becfaec-aadd-447f-a1d1-d01e5c7bb06f -->

    <owl:Class rdf:about="http://standards.iso.org/iso/10303/tech/refdata/core#2becfaec-aadd-447f-a1d1-d01e5c7bb06f">
        <rdfs:subClassOf rdf:resource="http://standards.iso.org/iso/10303/tech/refdata/core#af0b342e-b77d-4ac9-abdc-26d92ffb92a9"/>
        <dc:contributor>STEP Harmonization Team</dc:contributor>
        <dc:creator>Jean Brangé, AFNeT Services</dc:creator>
        <dc:date>2023-10-04</dc:date>
        <dc:source>ISO/TS 10303-4000</dc:source>
        <dc:type>InWork</dc:type>
        <rdfs:comment xml:lang="en">A RadialSize is a type of DimensionalSize that is a radius of a circular, cylindrical, spherical, or toroidal feature.</rdfs:comment>
        <owl:versionInfo>3</owl:versionInfo>
        <skos:changeNote>[2023-10-04] Jean Brangé, AFNeT Services: Initial definition.</skos:changeNote>
        <skos:prefLabel xml:lang="en">radial size</skos:prefLabel>
    </owl:Class>
    


    <!-- http://standards.iso.org/iso/10303/tech/refdata/core#2c12a8bb-821b-4b97-a208-c88965f41c1c -->

    <owl:Class rdf:about="http://standards.iso.org/iso/10303/tech/refdata/core#2c12a8bb-821b-4b97-a208-c88965f41c1c">
        <rdfs:subClassOf rdf:resource="http://standards.iso.org/iso/10303/tech/refdata/core#9c98fe40-130a-0135-b552-598f1b1392ae"/>
        <dc:contributor>STEP Harmonization Team</dc:contributor>
        <dc:creator>Jean Brangé, AFNeT Services</dc:creator>
        <dc:date>2023-10-04</dc:date>
        <dc:source>ISO/TS 10303-4000</dc:source>
        <dc:type>InWork</dc:type>
        <rdfs:comment xml:lang="en">An ExternalElementaryBrepShapeRepresentation is a type of ExternalGeometricModel that references an instance of type ../../../resources/aic_elementary_brep/aic_elementary_brep.htm#aic_elementary_brep.elementary_brep_shape_representation elementary_brep_shape_representation (ISO 10303-513).</rdfs:comment>
        <owl:versionInfo>3</owl:versionInfo>
        <skos:changeNote>[2023-10-04] Jean Brangé, AFNeT Services: Initial definition.</skos:changeNote>
        <skos:prefLabel xml:lang="en">external elementary brep shape representation</skos:prefLabel>
    </owl:Class>
    


    <!-- http://standards.iso.org/iso/10303/tech/refdata/core#2d7fd94d-3cec-400e-ab14-0983c2efb81f -->

    <owl:Class rdf:about="http://standards.iso.org/iso/10303/tech/refdata/core#2d7fd94d-3cec-400e-ab14-0983c2efb81f">
        <rdfs:subClassOf rdf:resource="http://standards.iso.org/iso/10303/tech/refdata/core#f5acf4c6-2654-4ef1-abc2-93e0ea5529d5"/>
        <dc:contributor>STEP Harmonization Team</dc:contributor>
        <dc:creator>Jean Brangé, AFNeT Services</dc:creator>
        <dc:date>2023-10-04</dc:date>
        <dc:source>ISO/TS 10303-4000</dc:source>
        <dc:type>InWork</dc:type>
        <rdfs:comment xml:lang="en">A PercentageLaminateTable is a type of ZoneStructuralMakeup that defines the percentage of the total thickness within a zone or point that each uniquely oriented constituent stock material makes up. The sum of VolumePercent must equal 100.</rdfs:comment>
        <owl:versionInfo>3</owl:versionInfo>
        <skos:changeNote>[2023-10-04] Jean Brangé, AFNeT Services: Initial definition.</skos:changeNote>
        <skos:example xml:lang="en">An example would be 40% 0 degree fibers, 30% 90 degree fibers, 15% +45 degree fibers, and 15% -45 degree fibers. The sum of the percents (%) have to equal 100.</skos:example>
        <skos:note xml:lang="en">For a simple laminate just made out of plies (PlyLaminate), a PercentageLaminateTable is used to capture the percentages of different fiber orientations within the zone based on the overall thickness of the zone.</skos:note>
        <skos:prefLabel xml:lang="en">percentage laminate table</skos:prefLabel>
    </owl:Class>
    


    <!-- http://standards.iso.org/iso/10303/tech/refdata/core#2dba5a41-b42b-4bef-a417-161358ee493a -->

    <owl:Class rdf:about="http://standards.iso.org/iso/10303/tech/refdata/core#2dba5a41-b42b-4bef-a417-161358ee493a">
        <rdfs:subClassOf rdf:resource="http://standards.iso.org/iso/10303/tech/refdata/core#83b2a250-130a-0135-b552-598f1b1392ae"/>
        <dc:contributor>STEP Harmonization Team</dc:contributor>
        <dc:creator>Phil Spiby, Eurostep</dc:creator>
        <dc:date>2022-09-01</dc:date>
        <dc:source>ISO/TS 10303-4000</dc:source>
        <dc:type>InWork</dc:type>
        <rdfs:comment xml:lang="en">A SchemeEntryAssignment is an assignment of a SchemeEntry to an item (specified by SchemeEntryAssignmentSelect). The meaning of the assignment can be specified using the ClassifiedAs attribute inherited from the AssignmentObject.</rdfs:comment>
        <owl:versionInfo>1</owl:versionInfo>
        <skos:changeNote>[2022-09-01] Initial definition.</skos:changeNote>
        <skos:example xml:lang="en">The SchemeEntryAssignment links the single items included in Plans and Schedules with their associated SchemeEntry. These items can be actions, events, or tasks depending on the nature of the Plan or Schedule.</skos:example>
        <skos:prefLabel xml:lang="en">scheme entry assignment</skos:prefLabel>
    </owl:Class>
    


    <!-- http://standards.iso.org/iso/10303/tech/refdata/core#2e480be6-62f1-46bb-a134-76b214e91463 -->

    <owl:Class rdf:about="http://standards.iso.org/iso/10303/tech/refdata/core#2e480be6-62f1-46bb-a134-76b214e91463">
        <rdfs:subClassOf rdf:resource="http://standards.iso.org/iso/10303/tech/refdata/core#8b5ba2e8-9590-4ef0-be41-93e469bea12d"/>
        <dc:contributor>STEP Harmonization Team</dc:contributor>
        <dc:creator>Jean Brangé, AFNeT Services</dc:creator>
        <dc:date>2023-10-04</dc:date>
        <dc:source>ISO/TS 10303-4000</dc:source>
        <dc:type>InWork</dc:type>
        <rdfs:comment xml:lang="en">An AffectedPlaneToleranceZone is a type of ToleranceZone.</rdfs:comment>
        <owl:versionInfo>3</owl:versionInfo>
        <skos:changeNote>[2023-10-04] Jean Brangé, AFNeT Services: Initial definition.</skos:changeNote>
        <skos:prefLabel xml:lang="en">affected plane tolerance zone</skos:prefLabel>
    </owl:Class>
    


    <!-- http://standards.iso.org/iso/10303/tech/refdata/core#2e7de2fb-3ba2-4bd0-82e6-9d6b6ec62776 -->

    <owl:Class rdf:about="http://standards.iso.org/iso/10303/tech/refdata/core#2e7de2fb-3ba2-4bd0-82e6-9d6b6ec62776">
        <rdfs:subClassOf rdf:resource="http://standards.iso.org/iso/10303/tech/refdata/core#59b11220-3279-0135-b58f-598f1b1392ae"/>
        <dc:contributor>STEP Harmonization Team</dc:contributor>
        <dc:creator>Phil Spiby, Eurostep</dc:creator>
        <dc:date>2022-09-01</dc:date>
        <dc:source>ISO/TS 10303-4000</dc:source>
        <dc:type>InWork</dc:type>
        <rdfs:comment xml:lang="en">A QualificationTypeRelationship is a relationship between two QualificationType objects.</rdfs:comment>
        <owl:versionInfo>1</owl:versionInfo>
        <skos:changeNote>[2022-09-01] Initial definition.</skos:changeNote>
        <skos:example xml:lang="en">Qualification X is a prerequisite for qualification Y.</skos:example>
        <skos:example xml:lang="en">Qualification X is equivalent to qualification Y.</skos:example>
        <skos:prefLabel xml:lang="en">qualification type relationship</skos:prefLabel>
    </owl:Class>
    


    <!-- http://standards.iso.org/iso/10303/tech/refdata/core#2ea624e0-5d2c-4b3b-84fb-d1c32d042635 -->

    <owl:Class rdf:about="http://standards.iso.org/iso/10303/tech/refdata/core#2ea624e0-5d2c-4b3b-84fb-d1c32d042635">
        <rdfs:subClassOf rdf:resource="http://standards.iso.org/iso/10303/tech/refdata/core#c4a27970-130a-0135-b552-598f1b1392ae"/>
        <dc:contributor>STEP Harmonization Team</dc:contributor>
        <dc:creator>Jean Brangé, AFNeT Services</dc:creator>
        <dc:date>2023-10-04</dc:date>
        <dc:source>ISO/TS 10303-4000</dc:source>
        <dc:type>InWork</dc:type>
        <rdfs:comment xml:lang="en">A WireOccurrence is a type of QuantifiedOccurrence. A WireOccurrence is an occurrence of a wire that is defined by a PartView of a particular length and that has wire as one of its PartTypes.</rdfs:comment>
        <owl:versionInfo>3</owl:versionInfo>
        <skos:changeNote>[2023-10-04] Jean Brangé, AFNeT Services: Initial definition.</skos:changeNote>
        <skos:note xml:lang="en">Either Quantity or Criterion or both shall be defined.</skos:note>
        <skos:prefLabel xml:lang="en">wire occurrence</skos:prefLabel>
    </owl:Class>
    


    <!-- http://standards.iso.org/iso/10303/tech/refdata/core#2f30fc41-0f70-43be-8fb7-5b24292818e8 -->

    <owl:Class rdf:about="http://standards.iso.org/iso/10303/tech/refdata/core#2f30fc41-0f70-43be-8fb7-5b24292818e8">
        <rdfs:subClassOf rdf:resource="http://standards.iso.org/iso/10303/tech/refdata/core#9fee6ad0-130a-0135-b552-598f1b1392ae"/>
        <dc:contributor>STEP Harmonization Team</dc:contributor>
        <dc:creator>Jean Brangé, AFNeT Services</dc:creator>
        <dc:date>2023-10-04</dc:date>
        <dc:source>ISO/TS 10303-4000</dc:source>
        <dc:type>InWork</dc:type>
        <rdfs:comment xml:lang="en">A MechanismState is a type of GeometricRepresentation that represents a specific state of a Mechanism where for each KinematicPair of the Mechanism a KinematicPairValue is defined.</rdfs:comment>
        <owl:versionInfo>3</owl:versionInfo>
        <skos:changeNote>[2023-10-04] Jean Brangé, AFNeT Services: Initial definition.</skos:changeNote>
        <skos:prefLabel xml:lang="en">mechanism state</skos:prefLabel>
    </owl:Class>
    


    <!-- http://standards.iso.org/iso/10303/tech/refdata/core#20c3f8e6-b48a-4a0d-89c1-9f8ad4fc8232 -->

    <owl:Class rdf:about="http://standards.iso.org/iso/10303/tech/refdata/core#20c3f8e6-b48a-4a0d-89c1-9f8ad4fc8232">
        <rdfs:subClassOf rdf:resource="http://standards.iso.org/iso/10303/tech/refdata/core#5185cb3e-1c24-4338-991a-0b34babdf714"/>
        <dc:contributor>STEP Harmonization Team</dc:contributor>
        <dc:creator>Jean Brangé, AFNeT Services</dc:creator>
        <dc:date>2023-10-04</dc:date>
        <dc:source>ISO/TS 10303-4000</dc:source>
        <dc:type>InWork</dc:type>
        <rdfs:comment xml:lang="en">A PartContactFeatureFitRelationship is a type of PartFeatureFitRelationship that is a relationship between two instances of the entity data type PartContactFeature stating that usages of these in an assembly can be joined with each other.</rdfs:comment>
        <owl:versionInfo>3</owl:versionInfo>
        <skos:changeNote>[2023-10-04] Jean Brangé, AFNeT Services: Initial definition.</skos:changeNote>
        <skos:note xml:lang="en">The ./4_info_reqs_ElectricalHarness.htm#PartContactFeature.ElementOf ElementOf of the Related and Relating PartContactFeatures may be the same or different PartViews.</skos:note>
        <skos:prefLabel xml:lang="en">part contact feature fit relationship</skos:prefLabel>
    </owl:Class>
    


    <!-- http://standards.iso.org/iso/10303/tech/refdata/core#20fad179-6703-42a4-b16c-51483fd9642e -->

    <owl:Class rdf:about="http://standards.iso.org/iso/10303/tech/refdata/core#20fad179-6703-42a4-b16c-51483fd9642e">
        <rdfs:subClassOf rdf:resource="http://standards.iso.org/iso/10303/tech/refdata/core#9fee6ad0-130a-0135-b552-598f1b1392ae"/>
        <dc:contributor>STEP Harmonization Team</dc:contributor>
        <dc:creator>Jean Brangé, AFNeT Services</dc:creator>
        <dc:date>2023-10-04</dc:date>
        <dc:source>ISO/TS 10303-4000</dc:source>
        <dc:type>InWork</dc:type>
        <rdfs:comment xml:lang="en">An EdgeBasedTopologicalRepresentationWithLengthConstraint is a type of GeometricRepresentation that has as its items one ConnectedEdgeSet and as needed additional Paths and VertexPoints that are within the domain of the ConnectedEdgeSet. An EdgeBasedTopologicalRepresentationWithLengthConstraint might define a sub-domain of another EdgeBasedTopologicalRepresentationWithLengthConstraint by using a ConnectedEdgeSubSet. In this case both EdgeBasedTopologicalRepresentationWithLengthConstraints shall share the same RepresentationContext. The geometry of an EdgeBasedTopologicalRepresentationWithLengthConstraint is defined by unspecific points and curves that are independent of any specific coordinates. Only the lengths of the curves are constrained to specific values.</rdfs:comment>
        <owl:versionInfo>3</owl:versionInfo>
        <skos:changeNote>[2023-10-04] Jean Brangé, AFNeT Services: Initial definition.</skos:changeNote>
        <skos:prefLabel xml:lang="en">edge based topological representation with length constraint</skos:prefLabel>
    </owl:Class>
    


    <!-- http://standards.iso.org/iso/10303/tech/refdata/core#21aaa0ca-0c88-4d9a-91c3-ddf0f4ce61f3 -->

    <owl:Class rdf:about="http://standards.iso.org/iso/10303/tech/refdata/core#21aaa0ca-0c88-4d9a-91c3-ddf0f4ce61f3">
        <rdfs:subClassOf rdf:resource="http://standards.iso.org/iso/10303/tech/refdata/core#d0cd8f0f-07c9-4a4d-9aec-bc0ccc1d901d"/>
        <dc:contributor>STEP Harmonization Team</dc:contributor>
        <dc:creator>Jean Brangé, AFNeT Services</dc:creator>
        <dc:date>2023-10-04</dc:date>
        <dc:source>ISO/TS 10303-4000</dc:source>
        <dc:type>InWork</dc:type>
        <rdfs:comment xml:lang="en">A BetweenShapeElement is a type of ContinuousShapeElement where some of the composing members are marked as forming elements of the borders of the continuous region.</rdfs:comment>
        <owl:versionInfo>3</owl:versionInfo>
        <skos:changeNote>[2023-10-04] Jean Brangé, AFNeT Services: Initial definition.</skos:changeNote>
        <skos:prefLabel xml:lang="en">between shape element</skos:prefLabel>
    </owl:Class>
    


    <!-- http://standards.iso.org/iso/10303/tech/refdata/core#21e3a5c6-4df9-4f13-82a9-478d7a9c744c -->

    <owl:Class rdf:about="http://standards.iso.org/iso/10303/tech/refdata/core#21e3a5c6-4df9-4f13-82a9-478d7a9c744c">
        <rdfs:subClassOf rdf:resource="http://standards.iso.org/iso/10303/tech/refdata/core#d75d6570-130a-0135-b552-598f1b1392ae"/>
        <dc:contributor>STEP Harmonization Team</dc:contributor>
        <dc:creator>Jean Brangé, AFNeT Services</dc:creator>
        <dc:date>2023-10-04</dc:date>
        <dc:source>ISO/TS 10303-4000</dc:source>
        <dc:type>InWork</dc:type>
        <rdfs:comment xml:lang="en">A LimitsAndFits is a tolerance specified by reference to the limits-and-fits system standardized by ISO 286. The application of LimitsAndFits shall conform to the requirements of ISO 286. Limits and fits is a system for assigning tolerances associated with the assembly of mating product features. In limits-and-fits system, a tolerance is assigned to a feature of size by classification rather than by giving an explicit value. A tolerance classification is composed of a fundamental deviation or &quot;position letter&quot; and a tolerance grade. These are used to calculate the size of the tolerance zone and its location relative to the basic or nominal size of the feature according to the tables and formulas found in ISO 286.</rdfs:comment>
        <owl:versionInfo>3</owl:versionInfo>
        <skos:changeNote>[2023-10-04] Jean Brangé, AFNeT Services: Initial definition.</skos:changeNote>
        <skos:example xml:lang="en">A hole and a shaft that are intended to mate in an assembly.</skos:example>
        <skos:prefLabel xml:lang="en">limits and fits</skos:prefLabel>
    </owl:Class>
    


    <!-- http://standards.iso.org/iso/10303/tech/refdata/core#2158251b-c18b-450a-9337-ce796af6c252 -->

    <owl:Class rdf:about="http://standards.iso.org/iso/10303/tech/refdata/core#2158251b-c18b-450a-9337-ce796af6c252">
        <rdfs:subClassOf rdf:resource="http://standards.iso.org/iso/10303/tech/refdata/core#1d59c650-3279-0135-b58f-598f1b1392ae"/>
        <dc:contributor>STEP Harmonization Team</dc:contributor>
        <dc:creator>Phil Spiby, Eurostep</dc:creator>
        <dc:date>2022-09-01</dc:date>
        <dc:source>ISO/TS 10303-4000</dc:source>
        <dc:type>InWork</dc:type>
        <rdfs:comment xml:lang="en">A ResourceItemRealization is a specification of how a resource item can be associated with an item that serves as the resource.</rdfs:comment>
        <owl:versionInfo>2</owl:versionInfo>
        <skos:changeNote>[2021-07-30] Initial definition.</skos:changeNote>
        <skos:changeNote>[2022-09-01] Phil Spiby, Eurostep: updated comment updated example.</skos:changeNote>
        <skos:example xml:lang="en">A product can serve as a resource.</skos:example>
        <skos:prefLabel xml:lang="en">resource item realization</skos:prefLabel>
    </owl:Class>
    


    <!-- http://standards.iso.org/iso/10303/tech/refdata/core#2290b813-9961-40a1-8c4f-3b01cdc5a22a -->

    <owl:Class rdf:about="http://standards.iso.org/iso/10303/tech/refdata/core#2290b813-9961-40a1-8c4f-3b01cdc5a22a">
        <rdfs:subClassOf rdf:resource="http://standards.iso.org/iso/10303/tech/refdata/core#835280f0-130a-0135-b552-598f1b1392ae"/>
        <dc:contributor>STEP Harmonization Team</dc:contributor>
        <dc:creator>Phil Spiby, Eurostep</dc:creator>
        <dc:date>2022-09-01</dc:date>
        <dc:source>ISO/TS 10303-4000</dc:source>
        <dc:type>InWork</dc:type>
        <rdfs:comment xml:lang="en">A SchemeEntry is a specialization of ActivityMethod that provides the identification and description of a single entry in a specific Scheme.</rdfs:comment>
        <owl:versionInfo>1</owl:versionInfo>
        <skos:changeNote>[2022-09-01] Initial definition.</skos:changeNote>
        <skos:note xml:lang="en">A SchemeEntry can be associated with time constraints.</skos:note>
        <skos:note xml:lang="en">A SchemeEntry only exists within the scope of a specific Scheme.</skos:note>
        <skos:prefLabel xml:lang="en">scheme entry</skos:prefLabel>
    </owl:Class>
    


    <!-- http://standards.iso.org/iso/10303/tech/refdata/core#24b43cfd-4090-42e8-8875-7e127a7b934b -->

    <owl:Class rdf:about="http://standards.iso.org/iso/10303/tech/refdata/core#24b43cfd-4090-42e8-8875-7e127a7b934b">
        <rdfs:subClassOf rdf:resource="http://standards.iso.org/iso/10303/tech/refdata/core#1cfca290-3279-0135-b58f-598f1b1392ae"/>
        <dc:contributor>STEP Harmonization Team</dc:contributor>
        <dc:creator>Phil Spiby, Eurostep</dc:creator>
        <dc:date>2022-09-01</dc:date>
        <dc:source>ISO/TS 10303-4000</dc:source>
        <dc:type>InWork</dc:type>
        <rdfs:comment xml:lang="en">A CollectionAssignment is an assignment of a CollectionView to an item (specified by CollectionMemberSelect) to which the CollectionView has relevance.</rdfs:comment>
        <owl:versionInfo>2</owl:versionInfo>
        <skos:changeNote>[2021-07-30] Initial definition.</skos:changeNote>
        <skos:changeNote>[2022-09-01] Phil Spiby, Eurostep: updated comment.</skos:changeNote>
        <skos:prefLabel xml:lang="en">collection assignment</skos:prefLabel>
    </owl:Class>
    


    <!-- http://standards.iso.org/iso/10303/tech/refdata/core#241b8313-cf80-44ca-8b6d-e3ae164ea25a -->

    <owl:Class rdf:about="http://standards.iso.org/iso/10303/tech/refdata/core#241b8313-cf80-44ca-8b6d-e3ae164ea25a">
        <rdfs:subClassOf rdf:resource="http://standards.iso.org/iso/10303/tech/refdata/core#6d4d4ccd-20d2-4209-9fe6-17da7b3cb1a1"/>
        <dc:contributor>STEP Harmonization Team</dc:contributor>
        <dc:creator>Jean Brangé, AFNeT Services</dc:creator>
        <dc:date>2023-10-04</dc:date>
        <dc:source>ISO/TS 10303-4000</dc:source>
        <dc:type>InWork</dc:type>
        <rdfs:comment xml:lang="en">A CompositeAssemblyTable is a type of LaminateTable that provides an ordered list of constituent parts. The ordered list provides basic placement position within the laminate (see following figure). CompositeAssemblyTable.pngComposite assembly table</rdfs:comment>
        <owl:versionInfo>3</owl:versionInfo>
        <skos:changeNote>[2023-10-04] Jean Brangé, AFNeT Services: Initial definition.</skos:changeNote>
        <skos:prefLabel xml:lang="en">composite assembly table</skos:prefLabel>
    </owl:Class>
    


    <!-- http://standards.iso.org/iso/10303/tech/refdata/core#25f8dadd-977c-4274-8096-4dce31fae4e5 -->

    <owl:Class rdf:about="http://standards.iso.org/iso/10303/tech/refdata/core#25f8dadd-977c-4274-8096-4dce31fae4e5">
        <rdfs:subClassOf rdf:resource="http://standards.iso.org/iso/10303/tech/refdata/core#66348150-092a-4eb7-9561-0b83adfa15ff"/>
        <dc:contributor>STEP Harmonization Team</dc:contributor>
        <dc:creator>Jean Brangé, AFNeT Services</dc:creator>
        <dc:date>2023-10-04</dc:date>
        <dc:source>ISO/TS 10303-4000</dc:source>
        <dc:type>InWork</dc:type>
        <rdfs:comment xml:lang="en">A ContactingFeature is a type of ShapeElement that is non-definitional and for which the rules governing contacting feature defined in ISO 5459 shall apply.</rdfs:comment>
        <owl:versionInfo>3</owl:versionInfo>
        <skos:changeNote>[2023-10-04] Jean Brangé, AFNeT Services: Initial definition.</skos:changeNote>
        <skos:prefLabel xml:lang="en">contacting feature</skos:prefLabel>
    </owl:Class>
    


    <!-- http://standards.iso.org/iso/10303/tech/refdata/core#29dbb825-9e6a-420a-a3d7-aca08e15003a -->

    <owl:Class rdf:about="http://standards.iso.org/iso/10303/tech/refdata/core#29dbb825-9e6a-420a-a3d7-aca08e15003a">
        <rdfs:subClassOf rdf:resource="http://standards.iso.org/iso/10303/tech/refdata/core#0cc8b831-37f7-4cd5-984f-dbb5588fbc1d"/>
        <dc:contributor>STEP Harmonization Team</dc:contributor>
        <dc:creator>Jean Brangé, AFNeT Services</dc:creator>
        <dc:date>2023-10-04</dc:date>
        <dc:source>ISO/TS 10303-4000</dc:source>
        <dc:type>InWork</dc:type>
        <rdfs:comment xml:lang="en">An AssemblyShapeConstraint is a type of PartShapeElement that defines a constraint between two or more OccurrenceShapeFeatures within an AssemblyDefinition. An AssemblyShapeConstraint may be composed of other AssemblyShapeConstraints.</rdfs:comment>
        <owl:versionInfo>3</owl:versionInfo>
        <skos:changeNote>[2023-10-04] Jean Brangé, AFNeT Services: Initial definition.</skos:changeNote>
        <skos:prefLabel xml:lang="en">assembly shape constraint</skos:prefLabel>
    </owl:Class>
    


    <!-- http://standards.iso.org/iso/10303/tech/refdata/core#29dc8412-b2ec-410c-acf1-3fcdd53338ed -->

    <owl:Class rdf:about="http://standards.iso.org/iso/10303/tech/refdata/core#29dc8412-b2ec-410c-acf1-3fcdd53338ed">
        <rdfs:subClassOf rdf:resource="http://standards.iso.org/iso/10303/tech/refdata/core#59b11220-3279-0135-b58f-598f1b1392ae"/>
        <dc:contributor>STEP Harmonization Team</dc:contributor>
        <dc:creator>Phil Spiby, Eurostep</dc:creator>
        <dc:date>2022-09-01</dc:date>
        <dc:source>ISO/TS 10303-4000</dc:source>
        <dc:type>InWork</dc:type>
        <rdfs:comment xml:lang="en">A CollectionVersionRelationship is a relationship between two CollectionVersion objects.</rdfs:comment>
        <owl:versionInfo>2</owl:versionInfo>
        <skos:changeNote>[2021-07-30] Initial definition.</skos:changeNote>
        <skos:changeNote>[2022-09-01] Phil Spiby, Eurostep: updated comment.</skos:changeNote>
        <skos:prefLabel xml:lang="en">collection version relationship</skos:prefLabel>
    </owl:Class>
    


    <!-- http://standards.iso.org/iso/10303/tech/refdata/core#2981b8bd-4796-45b6-a012-03d3665378c7 -->

    <owl:Class rdf:about="http://standards.iso.org/iso/10303/tech/refdata/core#2981b8bd-4796-45b6-a012-03d3665378c7">
        <rdfs:subClassOf rdf:resource="http://standards.iso.org/iso/10303/tech/refdata/core#adfff300-130a-0135-b552-598f1b1392ae"/>
        <dc:contributor>STEP Harmonization Team</dc:contributor>
        <dc:creator>Phil Spiby, Eurostep</dc:creator>
        <dc:date>2022-09-01</dc:date>
        <dc:source>ISO/TS 10303-4000</dc:source>
        <dc:type>InWork</dc:type>
        <rdfs:comment xml:lang="en">A ProbabilityDerived is a specialization of NumericalValue that represents a probability value and associates it with the ProbabilityDistribution from which the value is derived together with any parameters used in that derivation.</rdfs:comment>
        <owl:versionInfo>1</owl:versionInfo>
        <skos:changeNote>[2022-09-01] Initial definition.</skos:changeNote>
        <skos:example xml:lang="en">In the case of coin tossing, the distribution is a Binomial distribution, with parameters of &apos;probability for a single toss&apos;, and &apos;number of tosses&apos;, whereas the parameter for the ProbabilityDerived will be the &apos;number of heads obtained&apos;.</skos:example>
        <skos:note xml:lang="en">Where the probability derived from a probability distribution, the parameters of ProbabilityDerived are those needed to get a single value from the distribution, and not those which characterize the distribution.</skos:note>
        <skos:prefLabel xml:lang="en">probability derived</skos:prefLabel>
    </owl:Class>
    


    <!-- http://standards.iso.org/iso/10303/tech/refdata/core#3a0c34b7-f2df-4e90-9b4b-54d23080b748 -->

    <owl:Class rdf:about="http://standards.iso.org/iso/10303/tech/refdata/core#3a0c34b7-f2df-4e90-9b4b-54d23080b748">
        <rdfs:subClassOf rdf:resource="http://standards.iso.org/iso/10303/tech/refdata/core#1d59c650-3279-0135-b58f-598f1b1392ae"/>
        <dc:contributor>STEP Harmonization Team</dc:contributor>
        <dc:creator>Phil Spiby, Eurostep</dc:creator>
        <dc:date>2022-09-01</dc:date>
        <dc:source>ISO/TS 10303-4000</dc:source>
        <dc:type>InWork</dc:type>
        <rdfs:comment xml:lang="en">An OrganizationOrganizationTypeAssociation is an association between an Organization and an OrganizationType.</rdfs:comment>
        <owl:versionInfo>2</owl:versionInfo>
        <skos:changeNote>[2021-07-30] Initial definition.</skos:changeNote>
        <skos:changeNote>[2022-09-01] Phil Spiby, Eurostep: updated name updated comment.</skos:changeNote>
        <skos:prefLabel xml:lang="en">organization organization type association</skos:prefLabel>
    </owl:Class>
    


    <!-- http://standards.iso.org/iso/10303/tech/refdata/core#3a7c473d-13f3-443b-b683-d2ae546c7fbc -->

    <owl:Class rdf:about="http://standards.iso.org/iso/10303/tech/refdata/core#3a7c473d-13f3-443b-b683-d2ae546c7fbc">
        <rdfs:subClassOf rdf:resource="http://standards.iso.org/iso/10303/tech/refdata/core#1cfca290-3279-0135-b58f-598f1b1392ae"/>
        <dc:contributor>STEP Harmonization Team</dc:contributor>
        <dc:creator>Phil Spiby, Eurostep</dc:creator>
        <dc:date>2022-09-01</dc:date>
        <dc:source>ISO/TS 10303-4000</dc:source>
        <dc:type>InWork</dc:type>
        <rdfs:comment xml:lang="en">A ResourceItemAssignment is an assignment of a resource item to an item (specified by ResourceItemAssignmentSelect). The meaning of the assignment can be specified using the ClassifiedAs attribute inherited from the AssignmentObject.</rdfs:comment>
        <owl:versionInfo>2</owl:versionInfo>
        <skos:changeNote>[2021-07-30] Initial definition.</skos:changeNote>
        <skos:changeNote>[2022-09-01] Phil Spiby, Eurostep: updated comment updated example.</skos:changeNote>
        <skos:example xml:lang="en">The assignment can be classified as &quot;applicable to&quot; or &quot;acquired for&quot;.</skos:example>
        <skos:prefLabel xml:lang="en">resource item assignment</skos:prefLabel>
    </owl:Class>
    


    <!-- http://standards.iso.org/iso/10303/tech/refdata/core#3aa67c37-6d1f-42b0-b6b1-e548ddc22b83 -->

    <owl:Class rdf:about="http://standards.iso.org/iso/10303/tech/refdata/core#3aa67c37-6d1f-42b0-b6b1-e548ddc22b83">
        <rdfs:subClassOf rdf:resource="http://standards.iso.org/iso/10303/tech/refdata/core#STEPThing"/>
        <dc:contributor>STEP Harmonization Team</dc:contributor>
        <dc:creator>Phil Spiby, Eurostep</dc:creator>
        <dc:date>2022-09-01</dc:date>
        <dc:source>ISO/TS 10303-4000</dc:source>
        <dc:type>InWork</dc:type>
        <rdfs:comment xml:lang="en">A QualificationType is the identification of a definitive recognition as a practitioner.</rdfs:comment>
        <owl:versionInfo>1</owl:versionInfo>
        <skos:changeNote>[2022-09-01] Initial definition.</skos:changeNote>
        <skos:example xml:lang="en">A Military rank such as Colonel, or Captain.</skos:example>
        <skos:example xml:lang="en">A driving licence.</skos:example>
        <skos:example xml:lang="en">A qualification for executing the Ground Running task for RB211 engines.</skos:example>
        <skos:example xml:lang="en">Educational qualification such as GCSE, A level, Degree, Ordinary National Certificate, Higher National Certificate, City and Guilds, or GNVQ.</skos:example>
        <skos:prefLabel xml:lang="en">qualification type</skos:prefLabel>
    </owl:Class>
    


    <!-- http://standards.iso.org/iso/10303/tech/refdata/core#3b3e1d82-b5b5-4547-8e97-2f50f8d66dd0 -->

    <owl:Class rdf:about="http://standards.iso.org/iso/10303/tech/refdata/core#3b3e1d82-b5b5-4547-8e97-2f50f8d66dd0">
        <rdfs:subClassOf rdf:resource="http://standards.iso.org/iso/10303/tech/refdata/core#59b11220-3279-0135-b58f-598f1b1392ae"/>
        <dc:contributor>STEP Harmonization Team</dc:contributor>
        <dc:creator>Phil Spiby, Eurostep</dc:creator>
        <dc:date>2022-09-01</dc:date>
        <dc:source>ISO/TS 10303-4000</dc:source>
        <dc:type>InWork</dc:type>
        <rdfs:comment xml:lang="en">A MessageRelationship is a relationship between two Message objects.</rdfs:comment>
        <owl:versionInfo>2</owl:versionInfo>
        <skos:changeNote>[2021-07-30] Initial definition.</skos:changeNote>
        <skos:changeNote>[2022-09-01] Phil Spiby, Eurostep: updated comment updated example.</skos:changeNote>
        <skos:example xml:lang="en">If messageB replaces messageA, then MessageRelationship.Related points to messageB and MessageRelationship.Relating points to messageA with MessageRelationship.RelationType set to &apos;replaces&apos; either as a string or standard reference data.</skos:example>
        <skos:prefLabel xml:lang="en">message relationship</skos:prefLabel>
    </owl:Class>
    


    <!-- http://standards.iso.org/iso/10303/tech/refdata/core#3cacd2cf-c4b8-4eb4-b756-6886cb44f3ea -->

    <owl:Class rdf:about="http://standards.iso.org/iso/10303/tech/refdata/core#3cacd2cf-c4b8-4eb4-b756-6886cb44f3ea">
        <rdfs:subClassOf rdf:resource="http://standards.iso.org/iso/10303/tech/refdata/core#1d59c650-3279-0135-b58f-598f1b1392ae"/>
        <dc:contributor>STEP Harmonization Team</dc:contributor>
        <dc:creator>Phil Spiby, Eurostep</dc:creator>
        <dc:date>2022-09-01</dc:date>
        <dc:source>ISO/TS 10303-4000</dc:source>
        <dc:type>InWork</dc:type>
        <rdfs:comment xml:lang="en">An ObservedEnvironmentToDefinitionView is an association between a view of the record of a set of observations about an environment, represented by an ObservedEnvironmentView, and a view of the typical environment, represented by EnvironmentDefinitionView. The typical environment is the expected environment about which observations have been made.</rdfs:comment>
        <owl:versionInfo>2</owl:versionInfo>
        <skos:changeNote>[2021-07-30] Initial definition.</skos:changeNote>
        <skos:changeNote>[2022-09-01] Phil Spiby, Eurostep: updated comment.</skos:changeNote>
        <skos:prefLabel xml:lang="en">observed environment to definition view</skos:prefLabel>
    </owl:Class>
    


    <!-- http://standards.iso.org/iso/10303/tech/refdata/core#3cd595d4-744c-43e0-a10c-d98fa0c30fc5 -->

    <owl:Class rdf:about="http://standards.iso.org/iso/10303/tech/refdata/core#3cd595d4-744c-43e0-a10c-d98fa0c30fc5">
        <rdfs:subClassOf rdf:resource="http://standards.iso.org/iso/10303/tech/refdata/core#0cc8b831-37f7-4cd5-984f-dbb5588fbc1d"/>
        <dc:contributor>STEP Harmonization Team</dc:contributor>
        <dc:creator>Jean Brangé, AFNeT Services</dc:creator>
        <dc:date>2023-10-04</dc:date>
        <dc:source>ISO/TS 10303-4000</dc:source>
        <dc:type>InWork</dc:type>
        <rdfs:comment xml:lang="en">A ComponentPathShapeElement is a type of PartShapeElement of an assembly that identifies a PartShapeElement of an occurrence of a part within this assembly. The referenced part and its PartShapeElement might be defined locally or externally.</rdfs:comment>
        <owl:versionInfo>3</owl:versionInfo>
        <skos:changeNote>[2023-10-04] Jean Brangé, AFNeT Services: Initial definition.</skos:changeNote>
        <skos:prefLabel xml:lang="en">component path shape element</skos:prefLabel>
    </owl:Class>
    


    <!-- http://standards.iso.org/iso/10303/tech/refdata/core#3d6b6422-7842-4b40-9c83-df8e3b7b1c4a -->

    <owl:Class rdf:about="http://standards.iso.org/iso/10303/tech/refdata/core#3d6b6422-7842-4b40-9c83-df8e3b7b1c4a">
        <rdfs:subClassOf rdf:resource="http://standards.iso.org/iso/10303/tech/refdata/core#STEPThing"/>
        <dc:contributor>STEP Harmonization Team</dc:contributor>
        <dc:creator>Phil Spiby, Eurostep</dc:creator>
        <dc:date>2022-09-01</dc:date>
        <dc:source>ISO/TS 10303-4000</dc:source>
        <dc:type>InWork</dc:type>
        <rdfs:comment xml:lang="en">A RequiredResource is an identified need for resource. The role of a RequiredResource is specified by the ClassifiedAs attribute.</rdfs:comment>
        <owl:versionInfo>2</owl:versionInfo>
        <skos:changeNote>[2021-07-30] Initial definition.</skos:changeNote>
        <skos:changeNote>[2022-09-01] Phil Spiby, Eurostep: updated comment updated example.</skos:changeNote>
        <skos:example xml:lang="en">&quot;facility&quot;, &quot;test equipment&quot;, &quot;supervisor&quot; are examples of classifications of a required resource.</skos:example>
        <skos:prefLabel xml:lang="en">required resource</skos:prefLabel>
    </owl:Class>
    


    <!-- http://standards.iso.org/iso/10303/tech/refdata/core#3e054bb3-7936-4694-9975-791156d04a22 -->

    <owl:Class rdf:about="http://standards.iso.org/iso/10303/tech/refdata/core#3e054bb3-7936-4694-9975-791156d04a22">
        <rdfs:subClassOf rdf:resource="http://standards.iso.org/iso/10303/tech/refdata/core#59b11220-3279-0135-b58f-598f1b1392ae"/>
        <dc:contributor>STEP Harmonization Team</dc:contributor>
        <dc:creator>Phil Spiby, Eurostep</dc:creator>
        <dc:date>2022-09-01</dc:date>
        <dc:source>ISO/TS 10303-4000</dc:source>
        <dc:type>InWork</dc:type>
        <rdfs:comment xml:lang="en">An InterfaceConnectorViewRelationship is a relationship between two InterfaceConnectorView objects.</rdfs:comment>
        <owl:versionInfo>2</owl:versionInfo>
        <skos:changeNote>[2021-07-30] Initial definition.</skos:changeNote>
        <skos:changeNote>[2022-09-01] Phil Spiby, Eurostep: updated comment.</skos:changeNote>
        <skos:prefLabel xml:lang="en">interface connector view relationship</skos:prefLabel>
    </owl:Class>
    


    <!-- http://standards.iso.org/iso/10303/tech/refdata/core#3ecb7025-f166-4a82-8c83-aec9e8f61efb -->

    <owl:Class rdf:about="http://standards.iso.org/iso/10303/tech/refdata/core#3ecb7025-f166-4a82-8c83-aec9e8f61efb">
        <rdfs:subClassOf rdf:resource="http://standards.iso.org/iso/10303/tech/refdata/core#59b11220-3279-0135-b58f-598f1b1392ae"/>
        <dc:contributor>STEP Harmonization Team</dc:contributor>
        <dc:creator>Phil Spiby, Eurostep</dc:creator>
        <dc:date>2022-09-01</dc:date>
        <dc:source>ISO/TS 10303-4000</dc:source>
        <dc:type>InWork</dc:type>
        <rdfs:comment xml:lang="en">A CausalConsequence is a relationship that identifies secondary effects related to or resulting from a particular RiskConsequence.</rdfs:comment>
        <owl:versionInfo>1</owl:versionInfo>
        <skos:changeNote>[2022-09-01] Initial definition.</skos:changeNote>
        <skos:note xml:lang="en">The related is considered an after effect of the relating.</skos:note>
        <skos:prefLabel xml:lang="en">causal consequence</skos:prefLabel>
    </owl:Class>
    


    <!-- http://standards.iso.org/iso/10303/tech/refdata/core#3ef97697-54b0-4208-9211-99906a761896 -->

    <owl:Class rdf:about="http://standards.iso.org/iso/10303/tech/refdata/core#3ef97697-54b0-4208-9211-99906a761896">
        <rdfs:subClassOf rdf:resource="http://standards.iso.org/iso/10303/tech/refdata/core#ef463eb2-567e-4f5f-8437-2dbe3d82745c"/>
        <dc:contributor>STEP Harmonization Team</dc:contributor>
        <dc:creator>Phil Spiby, Eurostep</dc:creator>
        <dc:date>2022-09-01</dc:date>
        <dc:source>ISO/TS 10303-4000</dc:source>
        <dc:type>InWork</dc:type>
        <rdfs:comment xml:lang="en">An EnvironmentDefinitionView is a specialization of EnvironmentView that provides a view of a version of an environment definition relevant for one or more application domains. This view collects the characteristics that define an Environment.</rdfs:comment>
        <owl:versionInfo>1</owl:versionInfo>
        <skos:changeNote>[2021-07-30] Initial definition.</skos:changeNote>
        <skos:note xml:lang="en"> The characteristics include the resources available, the locations in which the product is to operate as well as climatic conditions such temperature ranges.</skos:note>
        <skos:prefLabel xml:lang="en">environment definition view</skos:prefLabel>
    </owl:Class>
    


    <!-- http://standards.iso.org/iso/10303/tech/refdata/core#3faa23ef-66a0-4b1b-b6d0-851b648476eb -->

    <owl:Class rdf:about="http://standards.iso.org/iso/10303/tech/refdata/core#3faa23ef-66a0-4b1b-b6d0-851b648476eb">
        <rdfs:subClassOf rdf:resource="http://standards.iso.org/iso/10303/tech/refdata/core#9c98fe40-130a-0135-b552-598f1b1392ae"/>
        <dc:contributor>STEP Harmonization Team</dc:contributor>
        <dc:creator>Jean Brangé, AFNeT Services</dc:creator>
        <dc:date>2023-10-04</dc:date>
        <dc:source>ISO/TS 10303-4000</dc:source>
        <dc:type>InWork</dc:type>
        <rdfs:comment xml:lang="en">An ExternalAdvancedBrepShapeRepresentation is a type of ExternalGeometricModel that references an instance of type ../../../resources/aic_advanced_brep/aic_advanced_brep.htm#aic_advanced_brep.advanced_brep_shape_representationadvanced_brep_shape_representation (ISO 10303-514).</rdfs:comment>
        <owl:versionInfo>3</owl:versionInfo>
        <skos:changeNote>[2023-10-04] Jean Brangé, AFNeT Services: Initial definition.</skos:changeNote>
        <skos:prefLabel xml:lang="en">external advanced brep shape representation</skos:prefLabel>
    </owl:Class>
    


    <!-- http://standards.iso.org/iso/10303/tech/refdata/core#3facfed7-173e-46ee-b552-f72395931191 -->

    <owl:Class rdf:about="http://standards.iso.org/iso/10303/tech/refdata/core#3facfed7-173e-46ee-b552-f72395931191">
        <rdfs:subClassOf rdf:resource="http://standards.iso.org/iso/10303/tech/refdata/core#6490f437-5aff-4d04-b436-f4243e3160f8"/>
        <dc:contributor>STEP Harmonization Team</dc:contributor>
        <dc:creator>Phil Spiby, Eurostep</dc:creator>
        <dc:date>2022-09-01</dc:date>
        <dc:source>ISO/TS 10303-4000</dc:source>
        <dc:type>InWork</dc:type>
        <rdfs:comment xml:lang="en">An EnvironmentDefinitionVersion is a specialization of EnvironmentVersion that identifies a particular version of an EnvironmentDefinition.</rdfs:comment>
        <owl:versionInfo>1</owl:versionInfo>
        <skos:changeNote>[2021-07-30] Initial definition.</skos:changeNote>
        <skos:prefLabel xml:lang="en">environment definition version</skos:prefLabel>
    </owl:Class>
    


    <!-- http://standards.iso.org/iso/10303/tech/refdata/core#30cbe06e-c587-4805-b3b5-8ab899ba8ff2 -->

    <owl:Class rdf:about="http://standards.iso.org/iso/10303/tech/refdata/core#30cbe06e-c587-4805-b3b5-8ab899ba8ff2">
        <rdfs:subClassOf rdf:resource="http://standards.iso.org/iso/10303/tech/refdata/core#STEPThing"/>
        <dc:contributor>STEP Harmonization Team</dc:contributor>
        <dc:creator>Phil Spiby, Eurostep</dc:creator>
        <dc:date>2022-09-01</dc:date>
        <dc:source>ISO/TS 10303-4000</dc:source>
        <dc:type>InWork</dc:type>
        <rdfs:comment xml:lang="en">A TypeOfPerson is a type of person.</rdfs:comment>
        <owl:versionInfo>1</owl:versionInfo>
        <skos:changeNote>[2022-09-01] Initial definition.</skos:changeNote>
        <skos:example xml:lang="en">Class 3 welder, Truck driver, Electronics engineer, Mechanical technician, Helicopter pilot.</skos:example>
        <skos:prefLabel xml:lang="en">type of person</skos:prefLabel>
    </owl:Class>
    


    <!-- http://standards.iso.org/iso/10303/tech/refdata/core#307bf5d3-daa7-40ea-a9b6-388dad0df224 -->

    <owl:Class rdf:about="http://standards.iso.org/iso/10303/tech/refdata/core#307bf5d3-daa7-40ea-a9b6-388dad0df224">
        <rdfs:subClassOf rdf:resource="http://standards.iso.org/iso/10303/tech/refdata/core#66348150-092a-4eb7-9561-0b83adfa15ff"/>
        <dc:contributor>STEP Harmonization Team</dc:contributor>
        <dc:creator>Jean Brangé, AFNeT Services</dc:creator>
        <dc:date>2023-10-04</dc:date>
        <dc:source>ISO/TS 10303-4000</dc:source>
        <dc:type>InWork</dc:type>
        <rdfs:comment xml:lang="en">A CoatingLayer is a type of ShapeElement defining one layer of covering applied to a surface.</rdfs:comment>
        <owl:versionInfo>3</owl:versionInfo>
        <skos:changeNote>[2023-10-04] Jean Brangé, AFNeT Services: Initial definition.</skos:changeNote>
        <skos:example xml:lang="en">A layer of paint, applied to a part, is an example of CoatingLayer.</skos:example>
        <skos:note xml:lang="en">Each CoatingLayer is one specific aspect of a part&apos;s shape.</skos:note>
        <skos:note xml:lang="en">Sequences of CoatingLayer objects can be defined using ShapeElementRelationship with relationType &apos;coating layer sequence&apos;.</skos:note>
        <skos:prefLabel xml:lang="en">coating layer</skos:prefLabel>
    </owl:Class>
    


    <!-- http://standards.iso.org/iso/10303/tech/refdata/core#31d0a87f-d5c4-4a90-b963-f5b26fd45acf -->

    <owl:Class rdf:about="http://standards.iso.org/iso/10303/tech/refdata/core#31d0a87f-d5c4-4a90-b963-f5b26fd45acf">
        <rdfs:subClassOf rdf:resource="http://standards.iso.org/iso/10303/tech/refdata/core#835280f0-130a-0135-b552-598f1b1392ae"/>
        <dc:contributor>STEP Harmonization Team</dc:contributor>
        <dc:creator>Phil Spiby, Eurostep</dc:creator>
        <dc:date>2022-09-01</dc:date>
        <dc:source>ISO/TS 10303-4000</dc:source>
        <dc:type>InWork</dc:type>
        <rdfs:comment xml:lang="en">A TaskMethod is a specialization of ActivityMethod. It is a specification of work.</rdfs:comment>
        <owl:versionInfo>2</owl:versionInfo>
        <skos:changeNote>[2021-07-30] Initial definition.</skos:changeNote>
        <skos:changeNote>[2022-09-01] Phil Spiby, Eurostep: updated note.</skos:changeNote>
        <skos:note xml:lang="en">The task method can be implemented using people, machines or a combination.</skos:note>
        <skos:prefLabel xml:lang="en">task method</skos:prefLabel>
    </owl:Class>
    


    <!-- http://standards.iso.org/iso/10303/tech/refdata/core#32ba94ed-a4c9-4da4-b5e8-231b52733daf -->

    <owl:Class rdf:about="http://standards.iso.org/iso/10303/tech/refdata/core#32ba94ed-a4c9-4da4-b5e8-231b52733daf">
        <rdfs:subClassOf rdf:resource="http://standards.iso.org/iso/10303/tech/refdata/core#66348150-092a-4eb7-9561-0b83adfa15ff"/>
        <dc:contributor>STEP Harmonization Team</dc:contributor>
        <dc:creator>Jean Brangé, AFNeT Services</dc:creator>
        <dc:date>2023-10-04</dc:date>
        <dc:source>ISO/TS 10303-4000</dc:source>
        <dc:type>InWork</dc:type>
        <rdfs:comment xml:lang="en">A DatumSystem is a type of ShapeElement that is non-definitional and that represents the ordered collection of one to three datum reference compartments within a geometric tolerance frame. Unless otherwise specified a DatumSystem shall be used in accordance to the ISO 5459 definition for single datum and datum system.</rdfs:comment>
        <owl:versionInfo>3</owl:versionInfo>
        <skos:changeNote>[2023-10-04] Jean Brangé, AFNeT Services: Initial definition.</skos:changeNote>
        <skos:note xml:lang="en">A DatumSystem can be associated with a model coordinate system and can be shared by several GeometricTolerances.</skos:note>
        <skos:note xml:lang="en">Alternatively DatumSystem might be used for the corresponding concept in ASME Y14.5-2009 or any later edition of this standard.</skos:note>
        <skos:prefLabel xml:lang="en">datum system</skos:prefLabel>
    </owl:Class>
    


    <!-- http://standards.iso.org/iso/10303/tech/refdata/core#33e31a19-691b-43df-9fe3-0a098fcc0c86 -->

    <owl:Class rdf:about="http://standards.iso.org/iso/10303/tech/refdata/core#33e31a19-691b-43df-9fe3-0a098fcc0c86">
        <rdfs:subClassOf rdf:resource="http://standards.iso.org/iso/10303/tech/refdata/core#1cfca290-3279-0135-b58f-598f1b1392ae"/>
        <dc:contributor>STEP Harmonization Team</dc:contributor>
        <dc:creator>Phil Spiby, Eurostep</dc:creator>
        <dc:date>2022-09-01</dc:date>
        <dc:source>ISO/TS 10303-4000</dc:source>
        <dc:type>InWork</dc:type>
        <rdfs:comment xml:lang="en">An ObservationAssignment is an assignment of an Observation to an item (specified by ObservationAssignmentSelect) being observed, or to any item that can be used as part of the observation. The meaning of the assignment can be specified using the ClassifiedAs attribute inherited from the AssignmentObject.</rdfs:comment>
        <owl:versionInfo>1</owl:versionInfo>
        <skos:changeNote>[2022-09-01] Initial definition.</skos:changeNote>
        <skos:prefLabel xml:lang="en">observation assignment</skos:prefLabel>
    </owl:Class>
    


    <!-- http://standards.iso.org/iso/10303/tech/refdata/core#3316072f-8cd7-415c-9c5f-6c5d7eb4b5d3 -->

    <owl:Class rdf:about="http://standards.iso.org/iso/10303/tech/refdata/core#3316072f-8cd7-415c-9c5f-6c5d7eb4b5d3">
        <rdfs:subClassOf rdf:resource="http://standards.iso.org/iso/10303/tech/refdata/core#9a99abd0-130a-0135-b552-598f1b1392ae"/>
        <dc:contributor>STEP Harmonization Team</dc:contributor>
        <dc:creator>Phil Spiby, Eurostep</dc:creator>
        <dc:date>2022-09-01</dc:date>
        <dc:source>ISO/TS 10303-4000</dc:source>
        <dc:type>InWork</dc:type>
        <rdfs:comment xml:lang="en">A RelativeEvent is a type of Event the start of which will occur, respectively has occurred, with a time offset from the start of another Event.</rdfs:comment>
        <owl:versionInfo>1</owl:versionInfo>
        <skos:changeNote>[2021-07-30] Initial definition.</skos:changeNote>
        <skos:prefLabel xml:lang="en">relative event</skos:prefLabel>
    </owl:Class>
    


    <!-- http://standards.iso.org/iso/10303/tech/refdata/core#341273c1-e5b8-4afb-9c8e-a6aa84239ce0 -->

    <owl:Class rdf:about="http://standards.iso.org/iso/10303/tech/refdata/core#341273c1-e5b8-4afb-9c8e-a6aa84239ce0">
        <rdfs:subClassOf rdf:resource="http://standards.iso.org/iso/10303/tech/refdata/core#87556b90-130a-0135-b552-598f1b1392ae"/>
        <dc:contributor>STEP Harmonization Team</dc:contributor>
        <dc:creator>Jean Brangé, AFNeT Services</dc:creator>
        <dc:date>2023-10-04</dc:date>
        <dc:source>ISO/TS 10303-4000</dc:source>
        <dc:type>InWork</dc:type>
        <rdfs:comment xml:lang="en">A MatingDefinition is a type of AssemblyDefinition. It is a view of a PartVersion, defining the physical connection of two or more Occurrence objects. It includes technical information about the kind of connection. This information is independent from the hierarchical assembly structure.</rdfs:comment>
        <owl:versionInfo>3</owl:versionInfo>
        <skos:changeNote>[2023-10-04] Jean Brangé, AFNeT Services: Initial definition.</skos:changeNote>
        <skos:prefLabel xml:lang="en">mating definition</skos:prefLabel>
    </owl:Class>
    


    <!-- http://standards.iso.org/iso/10303/tech/refdata/core#345188b0-a42a-4c17-a38b-f2e90d42d76b -->

    <owl:Class rdf:about="http://standards.iso.org/iso/10303/tech/refdata/core#345188b0-a42a-4c17-a38b-f2e90d42d76b">
        <rdfs:subClassOf rdf:resource="http://standards.iso.org/iso/10303/tech/refdata/core#f5acf4c6-2654-4ef1-abc2-93e0ea5529d5"/>
        <dc:contributor>STEP Harmonization Team</dc:contributor>
        <dc:creator>Jean Brangé, AFNeT Services</dc:creator>
        <dc:date>2023-10-04</dc:date>
        <dc:source>ISO/TS 10303-4000</dc:source>
        <dc:type>InWork</dc:type>
        <rdfs:comment xml:lang="en">A SmearedMaterial is a type of ZoneStructuralMakeup that provides the material properties for an idealized zone or area of a part.</rdfs:comment>
        <owl:versionInfo>3</owl:versionInfo>
        <skos:changeNote>[2023-10-04] Jean Brangé, AFNeT Services: Initial definition.</skos:changeNote>
        <skos:note xml:lang="en">A SmearedMaterial can represent the material properties of a single StockMaterial by having the PercentageLaminateTable reference one StockMaterial and set its percent value of that materials constituent to 100%.</skos:note>
        <skos:prefLabel xml:lang="en">smeared material</skos:prefLabel>
    </owl:Class>
    


    <!-- http://standards.iso.org/iso/10303/tech/refdata/core#36a3188d-b596-4fe2-8eda-51e075853728 -->

    <owl:Class rdf:about="http://standards.iso.org/iso/10303/tech/refdata/core#36a3188d-b596-4fe2-8eda-51e075853728">
        <rdfs:subClassOf rdf:resource="http://standards.iso.org/iso/10303/tech/refdata/core#1cfca290-3279-0135-b58f-598f1b1392ae"/>
        <dc:contributor>STEP Harmonization Team</dc:contributor>
        <dc:creator>Phil Spiby, Eurostep</dc:creator>
        <dc:date>2022-09-01</dc:date>
        <dc:source>ISO/TS 10303-4000</dc:source>
        <dc:type>InWork</dc:type>
        <rdfs:comment xml:lang="en">An EnvironmentAssignment is an assignment of an environment (via EnvironmentDefinitionView) to an item (specified by EnvironmentAssignmentSelect). The meaning of the assignment can be specified using the ClassifiedAs attribute inherited from the AssignmentObject.</rdfs:comment>
        <owl:versionInfo>2</owl:versionInfo>
        <skos:changeNote>[2021-07-30] Initial definition.</skos:changeNote>
        <skos:changeNote>[2022-09-01] Phil Spiby, Eurostep: updated comment.</skos:changeNote>
        <skos:prefLabel xml:lang="en">environment assignment</skos:prefLabel>
    </owl:Class>
    


    <!-- http://standards.iso.org/iso/10303/tech/refdata/core#36d7b46c-2554-494b-83d3-26668554cff4 -->

    <owl:Class rdf:about="http://standards.iso.org/iso/10303/tech/refdata/core#36d7b46c-2554-494b-83d3-26668554cff4">
        <rdfs:subClassOf rdf:resource="http://standards.iso.org/iso/10303/tech/refdata/core#b608a929-7fa0-4643-8237-59c6cf4d0dbc"/>
        <dc:contributor>STEP Harmonization Team</dc:contributor>
        <dc:creator>Jean Brangé, AFNeT Services</dc:creator>
        <dc:date>2023-10-04</dc:date>
        <dc:source>ISO/TS 10303-4000</dc:source>
        <dc:type>InWork</dc:type>
        <rdfs:comment xml:lang="en">An OccurrenceContactFeature is a type of OccurrenceShapeFeature that is intended to be joined with another OccurrenceContactFeature.</rdfs:comment>
        <owl:versionInfo>3</owl:versionInfo>
        <skos:changeNote>[2023-10-04] Jean Brangé, AFNeT Services: Initial definition.</skos:changeNote>
        <skos:prefLabel xml:lang="en">occurrence contact feature</skos:prefLabel>
    </owl:Class>
    


    <!-- http://standards.iso.org/iso/10303/tech/refdata/core#36f870b4-71c7-4606-b3f8-ef6ad24bf23f -->

    <owl:Class rdf:about="http://standards.iso.org/iso/10303/tech/refdata/core#36f870b4-71c7-4606-b3f8-ef6ad24bf23f">
        <rdfs:subClassOf rdf:resource="http://standards.iso.org/iso/10303/tech/refdata/core#9c98fe40-130a-0135-b552-598f1b1392ae"/>
        <dc:contributor>STEP Harmonization Team</dc:contributor>
        <dc:creator>Jean Brangé, AFNeT Services</dc:creator>
        <dc:date>2023-10-04</dc:date>
        <dc:source>ISO/TS 10303-4000</dc:source>
        <dc:type>InWork</dc:type>
        <rdfs:comment xml:lang="en">An ExternalGeometricallyBoundedWireframeShapeRepresentation is a type of ExternalGeometricModel that references an instance of type ../../../resources/aic_geometrically_bounded_wireframe/aic_geometrically_bounded_wireframe.htm#aic_geometrically_bounded_wireframe.geometrically_bounded_wireframe_shape_representation geometrically_bounded_wireframe_shape_representation (ISO 10303-510).</rdfs:comment>
        <owl:versionInfo>3</owl:versionInfo>
        <skos:changeNote>[2023-10-04] Jean Brangé, AFNeT Services: Initial definition.</skos:changeNote>
        <skos:prefLabel xml:lang="en">external geometrically bounded wireframe shape representation</skos:prefLabel>
    </owl:Class>
    


    <!-- http://standards.iso.org/iso/10303/tech/refdata/core#38bc05e3-1d21-4054-8559-5c054fa73826 -->

    <owl:Class rdf:about="http://standards.iso.org/iso/10303/tech/refdata/core#38bc05e3-1d21-4054-8559-5c054fa73826">
        <rdfs:subClassOf rdf:resource="http://standards.iso.org/iso/10303/tech/refdata/core#59b11220-3279-0135-b58f-598f1b1392ae"/>
        <dc:contributor>STEP Harmonization Team</dc:contributor>
        <dc:creator>Phil Spiby, Eurostep</dc:creator>
        <dc:date>2022-09-01</dc:date>
        <dc:source>ISO/TS 10303-4000</dc:source>
        <dc:type>InWork</dc:type>
        <rdfs:comment xml:lang="en">A VerificationRelationship is a relationship between two Verification objects.</rdfs:comment>
        <owl:versionInfo>2</owl:versionInfo>
        <skos:changeNote>[2021-07-30] Initial definition.</skos:changeNote>
        <skos:changeNote>[2022-09-01] Phil Spiby, Eurostep: updated comment updated note.</skos:changeNote>
        <skos:prefLabel xml:lang="en">verification relationship</skos:prefLabel>
    </owl:Class>
    


    <!-- http://standards.iso.org/iso/10303/tech/refdata/core#38088809-8c17-440a-9d8b-0aee422ecc2a -->

    <owl:Class rdf:about="http://standards.iso.org/iso/10303/tech/refdata/core#38088809-8c17-440a-9d8b-0aee422ecc2a">
        <rdfs:subClassOf rdf:resource="http://standards.iso.org/iso/10303/tech/refdata/core#9c98fe40-130a-0135-b552-598f1b1392ae"/>
        <dc:contributor>STEP Harmonization Team</dc:contributor>
        <dc:creator>Jean Brangé, AFNeT Services</dc:creator>
        <dc:date>2023-10-04</dc:date>
        <dc:source>ISO/TS 10303-4000</dc:source>
        <dc:type>InWork</dc:type>
        <rdfs:comment xml:lang="en">An ExternalFacetedBrepShapeRepresentation is a type of ExternalGeometricModel that references an instance of type ../../../resources/aic_faceted_brep/aic_faceted_brep.htm#aic_faceted_brep.faceted_brep_shape_representation faceted_brep_shape_representation (ISO 10303-512).</rdfs:comment>
        <owl:versionInfo>3</owl:versionInfo>
        <skos:changeNote>[2023-10-04] Jean Brangé, AFNeT Services: Initial definition.</skos:changeNote>
        <skos:prefLabel xml:lang="en">external faceted brep shape representation</skos:prefLabel>
    </owl:Class>
    


    <!-- http://standards.iso.org/iso/10303/tech/refdata/core#38946a3f-8296-4297-aff4-1350bafc45c1 -->

    <owl:Class rdf:about="http://standards.iso.org/iso/10303/tech/refdata/core#38946a3f-8296-4297-aff4-1350bafc45c1">
        <rdfs:subClassOf rdf:resource="http://standards.iso.org/iso/10303/tech/refdata/core#STEPThing"/>
        <dc:contributor>STEP Harmonization Team</dc:contributor>
        <dc:creator>Phil Spiby, Eurostep</dc:creator>
        <dc:date>2022-09-01</dc:date>
        <dc:source>ISO/TS 10303-4000</dc:source>
        <dc:type>InWork</dc:type>
        <rdfs:comment xml:lang="en">A ResourceItem is an item that can occur in the role of a resource within the application context.</rdfs:comment>
        <owl:versionInfo>2</owl:versionInfo>
        <skos:changeNote>[2021-07-30] Initial definition.</skos:changeNote>
        <skos:changeNote>[2022-09-01] Phil Spiby, Eurostep: updated example.</skos:changeNote>
        <skos:example xml:lang="en">A ResourceItem can be classified as &quot;Facility&quot;, &quot;Replaceable unit&quot;, or &quot;Package&quot;.</skos:example>
        <skos:prefLabel xml:lang="en">resource item</skos:prefLabel>
    </owl:Class>
    


    <!-- http://standards.iso.org/iso/10303/tech/refdata/core#4af1be44-78a1-4f55-ab58-39d6373f93ef -->

    <owl:Class rdf:about="http://standards.iso.org/iso/10303/tech/refdata/core#4af1be44-78a1-4f55-ab58-39d6373f93ef">
        <rdfs:subClassOf rdf:resource="http://standards.iso.org/iso/10303/tech/refdata/core#70fd2ab8-bdcb-481c-8096-ca0246ed15c5"/>
        <dc:contributor>STEP Harmonization Team</dc:contributor>
        <dc:creator>Phil Spiby, Eurostep</dc:creator>
        <dc:date>2022-09-01</dc:date>
        <dc:source>ISO/TS 10303-4000</dc:source>
        <dc:type>InWork</dc:type>
        <rdfs:comment xml:lang="en">A SlotDesign is a specialization of SlotVersion that identifies the design version of a slot.</rdfs:comment>
        <owl:versionInfo>1</owl:versionInfo>
        <skos:changeNote>[2022-09-01] Initial definition.</skos:changeNote>
        <skos:example xml:lang="en">WeMakeBigPlanes Limited creates design version 1.34 of the attachment slot for the starboard engine of an aircraft.</skos:example>
        <skos:prefLabel xml:lang="en">slot design</skos:prefLabel>
    </owl:Class>
    


    <!-- http://standards.iso.org/iso/10303/tech/refdata/core#4b436ab0-a3fb-40bf-a7e8-676e91b52c9b -->

    <owl:Class rdf:about="http://standards.iso.org/iso/10303/tech/refdata/core#4b436ab0-a3fb-40bf-a7e8-676e91b52c9b">
        <rdfs:subClassOf rdf:resource="http://standards.iso.org/iso/10303/tech/refdata/core#59b11220-3279-0135-b58f-598f1b1392ae"/>
        <dc:contributor>STEP Harmonization Team</dc:contributor>
        <dc:creator>Jean Brangé, AFNeT Services</dc:creator>
        <dc:date>2023-10-04</dc:date>
        <dc:source>ISO/TS 10303-4000</dc:source>
        <dc:type>InWork</dc:type>
        <rdfs:comment xml:lang="en">A MatedPartRelationship is a relationship between two MatedPartAssociation objects. This relationship specifies additional information about the mating of two specific items that go into a MatingDefinition. The two MatedPartAssociation objects that are referenced by the MatedPartRelationship shall refer to the same MatingDefinition.</rdfs:comment>
        <owl:versionInfo>3</owl:versionInfo>
        <skos:changeNote>[2023-10-04] Jean Brangé, AFNeT Services: Initial definition.</skos:changeNote>
        <skos:prefLabel xml:lang="en">mated part relationship</skos:prefLabel>
    </owl:Class>
    


    <!-- http://standards.iso.org/iso/10303/tech/refdata/core#4b61e195-8c82-4e94-adec-a0bc457a30c2 -->

    <owl:Class rdf:about="http://standards.iso.org/iso/10303/tech/refdata/core#4b61e195-8c82-4e94-adec-a0bc457a30c2">
        <rdfs:subClassOf rdf:resource="http://standards.iso.org/iso/10303/tech/refdata/core#a2719b60-dbf3-48e7-be31-ebb8c09491de"/>
        <dc:contributor>STEP Harmonization Team</dc:contributor>
        <dc:creator>Phil Spiby, Eurostep</dc:creator>
        <dc:date>2022-09-01</dc:date>
        <dc:source>ISO/TS 10303-4000</dc:source>
        <dc:type>InWork</dc:type>
        <rdfs:comment xml:lang="en">An IncreasingResourceEvent is a type of ResourceEvent that increases the balance of a managed resource.</rdfs:comment>
        <owl:versionInfo>1</owl:versionInfo>
        <skos:changeNote>[2021-07-30] Initial definition.</skos:changeNote>
        <skos:example xml:lang="en">Purchasing new stock increases an inventory.</skos:example>
        <skos:prefLabel xml:lang="en">increasing resource event</skos:prefLabel>
    </owl:Class>
    


    <!-- http://standards.iso.org/iso/10303/tech/refdata/core#4b7fa44d-ebf6-4376-955f-898315ced722 -->

    <owl:Class rdf:about="http://standards.iso.org/iso/10303/tech/refdata/core#4b7fa44d-ebf6-4376-955f-898315ced722">
        <rdfs:subClassOf rdf:resource="http://standards.iso.org/iso/10303/tech/refdata/core#53e20541-4d83-4902-a059-b807ec6e0f42"/>
        <dc:contributor>STEP Harmonization Team</dc:contributor>
        <dc:creator>Phil Spiby, Eurostep</dc:creator>
        <dc:date>2022-09-01</dc:date>
        <dc:source>ISO/TS 10303-4000</dc:source>
        <dc:type>InWork</dc:type>
        <rdfs:comment xml:lang="en">A StateDefinitionCauseEffect is a type of StateDefinitionRelationship that is used to define a causal relationship between two sets of StateDefinition entities. The Relating StateDefinition acts as a cause and the Related StateDefinition acts as an effect.</rdfs:comment>
        <owl:versionInfo>2</owl:versionInfo>
        <skos:changeNote>[2021-07-30] Initial definition.</skos:changeNote>
        <skos:changeNote>[2022-09-01] Phil Spiby, Eurostep: updated comment.</skos:changeNote>
        <skos:prefLabel xml:lang="en">state definition cause effect</skos:prefLabel>
    </owl:Class>
    


    <!-- http://standards.iso.org/iso/10303/tech/refdata/core#4b984fe8-62f9-43b2-aeda-055f3ffe9c6a -->

    <owl:Class rdf:about="http://standards.iso.org/iso/10303/tech/refdata/core#4b984fe8-62f9-43b2-aeda-055f3ffe9c6a">
        <rdfs:subClassOf rdf:resource="http://standards.iso.org/iso/10303/tech/refdata/core#af0b342e-b77d-4ac9-abdc-26d92ffb92a9"/>
        <dc:contributor>STEP Harmonization Team</dc:contributor>
        <dc:creator>Jean Brangé, AFNeT Services</dc:creator>
        <dc:date>2023-10-04</dc:date>
        <dc:source>ISO/TS 10303-4000</dc:source>
        <dc:type>InWork</dc:type>
        <rdfs:comment xml:lang="en">A CurvedSize is a type of DimensionalSize that is the tolerance on a dimension for a curve measured along the entire path of a curve.</rdfs:comment>
        <owl:versionInfo>3</owl:versionInfo>
        <skos:changeNote>[2023-10-04] Jean Brangé, AFNeT Services: Initial definition.</skos:changeNote>
        <skos:prefLabel xml:lang="en">curved size</skos:prefLabel>
    </owl:Class>
    


    <!-- http://standards.iso.org/iso/10303/tech/refdata/core#4c1fc067-ccb3-4cb7-ab51-953fccd77d70 -->

    <owl:Class rdf:about="http://standards.iso.org/iso/10303/tech/refdata/core#4c1fc067-ccb3-4cb7-ab51-953fccd77d70">
        <rdfs:subClassOf rdf:resource="http://standards.iso.org/iso/10303/tech/refdata/core#b3a9b996-c18c-4464-b398-d16e36d6711a"/>
        <dc:contributor>STEP Harmonization Team</dc:contributor>
        <dc:creator>Jean Brangé, AFNeT Services</dc:creator>
        <dc:date>2023-10-04</dc:date>
        <dc:source>ISO/TS 10303-4000</dc:source>
        <dc:type>InWork</dc:type>
        <rdfs:comment xml:lang="en">A BeveledSheetRepresentation is a type of ConstituentShapeRepresentation that has a significant thickness, and whose edge is beveled at a constant angle around its entire perimeter. It is an extension of the concept of a thin sheet to products, such as honeycomb core, that have significant thickness but can be formed to mate with a curved surface.</rdfs:comment>
        <owl:versionInfo>3</owl:versionInfo>
        <skos:changeNote>[2023-10-04] Jean Brangé, AFNeT Services: Initial definition.</skos:changeNote>
        <skos:prefLabel xml:lang="en">beveled sheet representation</skos:prefLabel>
    </owl:Class>
    


    <!-- http://standards.iso.org/iso/10303/tech/refdata/core#4e6f80cd-9e65-4a7b-9bab-21419f058100 -->

    <owl:Class rdf:about="http://standards.iso.org/iso/10303/tech/refdata/core#4e6f80cd-9e65-4a7b-9bab-21419f058100">
        <rdfs:subClassOf rdf:resource="http://standards.iso.org/iso/10303/tech/refdata/core#84099bf0-130a-0135-b552-598f1b1392ae"/>
        <dc:contributor>STEP Harmonization Team</dc:contributor>
        <dc:creator>Phil Spiby, Eurostep</dc:creator>
        <dc:date>2022-09-01</dc:date>
        <dc:source>ISO/TS 10303-4000</dc:source>
        <dc:type>InWork</dc:type>
        <rdfs:comment xml:lang="en">A SchemeVersionRelationship is a specialization of ActivityMethodRelationship that is a relationship between two SchemeVersion objects.</rdfs:comment>
        <owl:versionInfo>1</owl:versionInfo>
        <skos:changeNote>[2022-09-01] Initial definition.</skos:changeNote>
        <skos:note xml:lang="en">The SchemeVersionRelationship provides the facility to relate versions of Plans or Schedules, represented by the SchemeVersion entity, in different ways. Classifications can be applied to different SchemeVersionRelationships to indicate their use for different purposes.</skos:note>
        <skos:prefLabel xml:lang="en">scheme version relationship</skos:prefLabel>
    </owl:Class>
    


    <!-- http://standards.iso.org/iso/10303/tech/refdata/core#4f470fb7-14c2-40ac-9521-b8885b0d3046 -->

    <owl:Class rdf:about="http://standards.iso.org/iso/10303/tech/refdata/core#4f470fb7-14c2-40ac-9521-b8885b0d3046">
        <rdfs:subClassOf rdf:resource="http://standards.iso.org/iso/10303/tech/refdata/core#af0b342e-b77d-4ac9-abdc-26d92ffb92a9"/>
        <dc:contributor>STEP Harmonization Team</dc:contributor>
        <dc:creator>Jean Brangé, AFNeT Services</dc:creator>
        <dc:date>2023-10-04</dc:date>
        <dc:source>ISO/TS 10303-4000</dc:source>
        <dc:type>InWork</dc:type>
        <rdfs:comment xml:lang="en">A ThicknessSize is a type of DimensionalSize that represents a thickness. Use of ThicknessSize is user defined.</rdfs:comment>
        <owl:versionInfo>3</owl:versionInfo>
        <skos:changeNote>[2023-10-04] Jean Brangé, AFNeT Services: Initial definition.</skos:changeNote>
        <skos:example xml:lang="en">The remaining thickness below a blind hole might be specified as a ThicknessSize.</skos:example>
        <skos:example xml:lang="en">The thickness of a coating layer is a ThicknessSize.</skos:example>
        <skos:prefLabel xml:lang="en">thickness size</skos:prefLabel>
    </owl:Class>
    


    <!-- http://standards.iso.org/iso/10303/tech/refdata/core#4f8985a9-5970-415e-8a13-bdfa544ac176 -->

    <owl:Class rdf:about="http://standards.iso.org/iso/10303/tech/refdata/core#4f8985a9-5970-415e-8a13-bdfa544ac176">
        <rdfs:subClassOf rdf:resource="http://standards.iso.org/iso/10303/tech/refdata/core#ef463eb2-567e-4f5f-8437-2dbe3d82745c"/>
        <dc:contributor>STEP Harmonization Team</dc:contributor>
        <dc:creator>Phil Spiby, Eurostep</dc:creator>
        <dc:date>2022-09-01</dc:date>
        <dc:source>ISO/TS 10303-4000</dc:source>
        <dc:type>InWork</dc:type>
        <rdfs:comment xml:lang="en">An ObservedEnvironmentView is a specialization of EnvironmentView that provides a view of a version of an observed environment relevant for one or more application domains. This view collects the characteristics of the observations on the environment.</rdfs:comment>
        <owl:versionInfo>1</owl:versionInfo>
        <skos:changeNote>[2021-07-30] Initial definition.</skos:changeNote>
        <skos:prefLabel xml:lang="en">observed environment view</skos:prefLabel>
    </owl:Class>
    


    <!-- http://standards.iso.org/iso/10303/tech/refdata/core#4fed74bc-5a1e-447d-b033-07896c8f0593 -->

    <owl:Class rdf:about="http://standards.iso.org/iso/10303/tech/refdata/core#4fed74bc-5a1e-447d-b033-07896c8f0593">
        <rdfs:subClassOf rdf:resource="http://standards.iso.org/iso/10303/tech/refdata/core#59b11220-3279-0135-b58f-598f1b1392ae"/>
        <dc:contributor>STEP Harmonization Team</dc:contributor>
        <dc:creator>Phil Spiby, Eurostep</dc:creator>
        <dc:date>2022-09-01</dc:date>
        <dc:source>ISO/TS 10303-4000</dc:source>
        <dc:type>InWork</dc:type>
        <rdfs:comment xml:lang="en">A LocatorRelationship is a relationship between two Locator objects.</rdfs:comment>
        <owl:versionInfo>2</owl:versionInfo>
        <skos:changeNote>[2021-07-30] Initial definition.</skos:changeNote>
        <skos:changeNote>[2022-09-01] Phil Spiby, Eurostep: updated comment.</skos:changeNote>
        <skos:prefLabel xml:lang="en">locator relationship</skos:prefLabel>
    </owl:Class>
    


    <!-- http://standards.iso.org/iso/10303/tech/refdata/core#40b6f827-7a2a-4787-b2a3-6022842eedf7 -->

    <owl:Class rdf:about="http://standards.iso.org/iso/10303/tech/refdata/core#40b6f827-7a2a-4787-b2a3-6022842eedf7">
        <rdfs:subClassOf rdf:resource="http://standards.iso.org/iso/10303/tech/refdata/core#44078e31-a1cb-4d89-b8d6-ab60b9140b06"/>
        <dc:contributor>STEP Harmonization Team</dc:contributor>
        <dc:creator>Jean Brangé, AFNeT Services</dc:creator>
        <dc:date>2023-10-04</dc:date>
        <dc:source>ISO/TS 10303-4000</dc:source>
        <dc:type>InWork</dc:type>
        <rdfs:comment xml:lang="en">A TargetPoint is a type of PlacedTarget that specifies a DatumTarget that is defined by a single implicit point. The position of the TargetPoint is defined by the placing AxisPlacement.</rdfs:comment>
        <owl:versionInfo>3</owl:versionInfo>
        <skos:changeNote>[2023-10-04] Jean Brangé, AFNeT Services: Initial definition.</skos:changeNote>
        <skos:prefLabel xml:lang="en">target point</skos:prefLabel>
    </owl:Class>
    


    <!-- http://standards.iso.org/iso/10303/tech/refdata/core#4138f20d-32c3-418d-9f69-787977b013b2 -->

    <owl:Class rdf:about="http://standards.iso.org/iso/10303/tech/refdata/core#4138f20d-32c3-418d-9f69-787977b013b2">
        <rdfs:subClassOf rdf:resource="http://standards.iso.org/iso/10303/tech/refdata/core#STEPThing"/>
        <dc:contributor>STEP Harmonization Team</dc:contributor>
        <dc:creator>Phil Spiby, Eurostep</dc:creator>
        <dc:date>2022-09-01</dc:date>
        <dc:source>ISO/TS 10303-4000</dc:source>
        <dc:type>InWork</dc:type>
        <rdfs:comment xml:lang="en">A PositionType is a recognized kind of position.</rdfs:comment>
        <owl:versionInfo>1</owl:versionInfo>
        <skos:changeNote>[2022-09-01] Initial definition.</skos:changeNote>
        <skos:example xml:lang="en">Chief Executive Officer, Manager, Service engineer, Programmer, Aircraft propulsion technician</skos:example>
        <skos:prefLabel xml:lang="en">position type</skos:prefLabel>
    </owl:Class>
    


    <!-- http://standards.iso.org/iso/10303/tech/refdata/core#41752ee7-c1fe-4f5b-8ee8-b3dcf1d67b16 -->

    <owl:Class rdf:about="http://standards.iso.org/iso/10303/tech/refdata/core#41752ee7-c1fe-4f5b-8ee8-b3dcf1d67b16">
        <rdfs:subClassOf rdf:resource="http://standards.iso.org/iso/10303/tech/refdata/core#1cfca290-3279-0135-b58f-598f1b1392ae"/>
        <dc:contributor>STEP Harmonization Team</dc:contributor>
        <dc:creator>Phil Spiby, Eurostep</dc:creator>
        <dc:date>2022-09-01</dc:date>
        <dc:source>ISO/TS 10303-4000</dc:source>
        <dc:type>InWork</dc:type>
        <rdfs:comment xml:lang="en">A QualificationAssignment is the assignment of a qualification to a person or organization (specified by QualificationAssignmentSelect). The meaning of the assignment can be specified using the ClassifiedAs attribute inherited from the AssignmentObject.</rdfs:comment>
        <owl:versionInfo>1</owl:versionInfo>
        <skos:changeNote>[2022-09-01] Initial definition.</skos:changeNote>
        <skos:prefLabel xml:lang="en">qualification assignment</skos:prefLabel>
    </owl:Class>
    


    <!-- http://standards.iso.org/iso/10303/tech/refdata/core#423cc1ad-039d-430d-b59e-1a399fd7bcd7 -->

    <owl:Class rdf:about="http://standards.iso.org/iso/10303/tech/refdata/core#423cc1ad-039d-430d-b59e-1a399fd7bcd7">
        <rdfs:subClassOf rdf:resource="http://standards.iso.org/iso/10303/tech/refdata/core#cf96c7f3-c3f6-4f8f-a640-eb05f182e1d6"/>
        <dc:contributor>STEP Harmonization Team</dc:contributor>
        <dc:creator>Phil Spiby, Eurostep</dc:creator>
        <dc:date>2022-09-01</dc:date>
        <dc:source>ISO/TS 10303-4000</dc:source>
        <dc:type>InWork</dc:type>
        <rdfs:comment xml:lang="en">An AdvisoryTaskStep is a type of TaskStep. It conveys information.</rdfs:comment>
        <owl:versionInfo>2</owl:versionInfo>
        <skos:changeNote>[2021-07-30] Initial definition.</skos:changeNote>
        <skos:changeNote>[2022-09-01] Phil Spiby, Eurostep: updated example updated note.</skos:changeNote>
        <skos:example xml:lang="en">&quot;Beware of hot exhausts&quot;, &quot;do not use tool X this way&quot; and similar messages.</skos:example>
        <skos:note xml:lang="en">Some TaskMethods cannot require any action to be undertaken.</skos:note>
        <skos:prefLabel xml:lang="en">advisory task step</skos:prefLabel>
    </owl:Class>
    


    <!-- http://standards.iso.org/iso/10303/tech/refdata/core#424807d3-8425-49a4-be82-ce9ff2a5eb6b -->

    <owl:Class rdf:about="http://standards.iso.org/iso/10303/tech/refdata/core#424807d3-8425-49a4-be82-ce9ff2a5eb6b">
        <rdfs:subClassOf rdf:resource="http://standards.iso.org/iso/10303/tech/refdata/core#95f1bde5-b263-4ca1-89df-33e1205800dd"/>
        <dc:contributor>STEP Harmonization Team</dc:contributor>
        <dc:creator>Phil Spiby, Eurostep</dc:creator>
        <dc:date>2022-09-01</dc:date>
        <dc:source>ISO/TS 10303-4000</dc:source>
        <dc:type>InWork</dc:type>
        <rdfs:comment xml:lang="en">An EndTask is a type of TaskElement. It signifies a point at which to end the task.</rdfs:comment>
        <owl:versionInfo>1</owl:versionInfo>
        <skos:changeNote>[2021-07-30] Initial definition.</skos:changeNote>
        <skos:prefLabel xml:lang="en">end task</skos:prefLabel>
    </owl:Class>
    


    <!-- http://standards.iso.org/iso/10303/tech/refdata/core#43a66bf1-f44d-42f5-a634-5fbc215426ec -->

    <owl:Class rdf:about="http://standards.iso.org/iso/10303/tech/refdata/core#43a66bf1-f44d-42f5-a634-5fbc215426ec">
        <rdfs:subClassOf rdf:resource="http://standards.iso.org/iso/10303/tech/refdata/core#5952bf98-2ea0-46c9-8915-249fe039b206"/>
        <dc:contributor>STEP Harmonization Team</dc:contributor>
        <dc:creator>Phil Spiby, Eurostep</dc:creator>
        <dc:date>2022-09-01</dc:date>
        <dc:source>ISO/TS 10303-4000</dc:source>
        <dc:type>InWork</dc:type>
        <rdfs:comment xml:lang="en">A RiskConsequence is a specialization of RiskView and specifies the outcome of the risk occurring.</rdfs:comment>
        <owl:versionInfo>1</owl:versionInfo>
        <skos:changeNote>[2022-09-01] Initial definition.</skos:changeNote>
        <skos:note xml:lang="en">Consequences can be expressed qualitatively or quantitatively.</skos:note>
        <skos:note xml:lang="en">Consequences can range from positive to negative. However, consequences are always negative for safety aspects.</skos:note>
        <skos:note xml:lang="en">There can be one or more consequences of a risk occurring.</skos:note>
        <skos:prefLabel xml:lang="en">risk consequence</skos:prefLabel>
    </owl:Class>
    


    <!-- http://standards.iso.org/iso/10303/tech/refdata/core#43cb580d-8cb9-4fa4-b37c-38d3868f21bd -->

    <owl:Class rdf:about="http://standards.iso.org/iso/10303/tech/refdata/core#43cb580d-8cb9-4fa4-b37c-38d3868f21bd">
        <rdfs:subClassOf rdf:resource="http://standards.iso.org/iso/10303/tech/refdata/core#STEPThing"/>
        <dc:contributor>STEP Harmonization Team</dc:contributor>
        <dc:creator>Phil Spiby, Eurostep</dc:creator>
        <dc:date>2022-09-01</dc:date>
        <dc:source>ISO/TS 10303-4000</dc:source>
        <dc:type>InWork</dc:type>
        <rdfs:comment xml:lang="en">An InterfaceSpecificationVersion identifies a version of an InterfaceSpecification.</rdfs:comment>
        <owl:versionInfo>1</owl:versionInfo>
        <skos:changeNote>[2021-07-30] Initial definition.</skos:changeNote>
        <skos:example xml:lang="en">In 1999, BSI issues a new version of a standard for connecting domestic electrical equipment to the electricity supply.</skos:example>
        <skos:prefLabel xml:lang="en">interface specification version</skos:prefLabel>
    </owl:Class>
    


    <!-- http://standards.iso.org/iso/10303/tech/refdata/core#44f308d7-e1ce-4953-813a-37290f4b890b -->

    <owl:Class rdf:about="http://standards.iso.org/iso/10303/tech/refdata/core#44f308d7-e1ce-4953-813a-37290f4b890b">
        <rdfs:subClassOf rdf:resource="http://standards.iso.org/iso/10303/tech/refdata/core#085b6771-a1f8-4cf7-9771-8de2f3a063a1"/>
        <dc:contributor>STEP Harmonization Team</dc:contributor>
        <dc:creator>Phil Spiby, Eurostep</dc:creator>
        <dc:date>2022-09-01</dc:date>
        <dc:source>ISO/TS 10303-4000</dc:source>
        <dc:type>InWork</dc:type>
        <rdfs:comment xml:lang="en">A StateDefinitionPredictedAssociation is a statement that a StatePredicted is expected to conform to a particular StateDefinition.</rdfs:comment>
        <owl:versionInfo>1</owl:versionInfo>
        <skos:changeNote>[2021-07-30] Initial definition.</skos:changeNote>
        <skos:prefLabel xml:lang="en">state definition predicted association</skos:prefLabel>
    </owl:Class>
    


    <!-- http://standards.iso.org/iso/10303/tech/refdata/core#44078e31-a1cb-4d89-b8d6-ab60b9140b06 -->

    <owl:Class rdf:about="http://standards.iso.org/iso/10303/tech/refdata/core#44078e31-a1cb-4d89-b8d6-ab60b9140b06">
        <rdfs:subClassOf rdf:resource="http://standards.iso.org/iso/10303/tech/refdata/core#d2eb1f4f-b98f-4393-a7ed-24dc41900bd2"/>
        <dc:contributor>STEP Harmonization Team</dc:contributor>
        <dc:creator>Jean Brangé, AFNeT Services</dc:creator>
        <dc:date>2023-10-04</dc:date>
        <dc:source>ISO/TS 10303-4000</dc:source>
        <dc:type>InWork</dc:type>
        <rdfs:comment xml:lang="en">A PlacedTarget is a type of DatumTarget that specifies a DatumTarget that is represented implicitly by parameters. Each PlacedTarget is a TargetCircle, a TargetCircularCurve, a TargetPoint, a TargetRectangle, or a TargetStraightLine.</rdfs:comment>
        <owl:versionInfo>3</owl:versionInfo>
        <skos:changeNote>[2023-10-04] Jean Brangé, AFNeT Services: Initial definition.</skos:changeNote>
        <skos:prefLabel xml:lang="en">placed target</skos:prefLabel>
    </owl:Class>
    


    <!-- http://standards.iso.org/iso/10303/tech/refdata/core#44872c80-067e-4656-9c87-bd3e899faa62 -->

    <owl:Class rdf:about="http://standards.iso.org/iso/10303/tech/refdata/core#44872c80-067e-4656-9c87-bd3e899faa62">
        <rdfs:subClassOf rdf:resource="http://standards.iso.org/iso/10303/tech/refdata/core#STEPThing"/>
        <dc:contributor>STEP Harmonization Team</dc:contributor>
        <dc:creator>Jean Brangé, AFNeT Services</dc:creator>
        <dc:date>2023-10-04</dc:date>
        <dc:source>ISO/TS 10303-4000</dc:source>
        <dc:type>InWork</dc:type>
        <rdfs:comment xml:lang="en">A ChangeElementSequence is the specification of the sequence between two DeltaChangeActivity objects.</rdfs:comment>
        <owl:versionInfo>3</owl:versionInfo>
        <skos:changeNote>[2023-10-04] Jean Brangé, AFNeT Services: Initial definition.</skos:changeNote>
        <skos:prefLabel xml:lang="en">change element sequence</skos:prefLabel>
    </owl:Class>
    


    <!-- http://standards.iso.org/iso/10303/tech/refdata/core#45bc2fdc-71c1-4b75-ba27-8326d0c33255 -->

    <owl:Class rdf:about="http://standards.iso.org/iso/10303/tech/refdata/core#45bc2fdc-71c1-4b75-ba27-8326d0c33255">
        <rdfs:subClassOf rdf:resource="http://standards.iso.org/iso/10303/tech/refdata/core#1d59c650-3279-0135-b58f-598f1b1392ae"/>
        <dc:contributor>STEP Harmonization Team</dc:contributor>
        <dc:creator>Phil Spiby, Eurostep</dc:creator>
        <dc:date>2022-09-01</dc:date>
        <dc:source>ISO/TS 10303-4000</dc:source>
        <dc:type>InWork</dc:type>
        <rdfs:comment xml:lang="en">A SlotOn is an association between an item and a Slot that is a location on the item at which to install removable parts.</rdfs:comment>
        <owl:versionInfo>1</owl:versionInfo>
        <skos:changeNote>[2022-09-01] Initial definition.</skos:changeNote>
        <skos:example xml:lang="en">An aircraft has a pylon mounting on a wing as a location at which to install various equipment. An instance of the SlotOn entity data type identifies which attachment slot corresponds to the pylon.</skos:example>
        <skos:prefLabel xml:lang="en">slot on</skos:prefLabel>
    </owl:Class>
    


    <!-- http://standards.iso.org/iso/10303/tech/refdata/core#46bac3e9-3f47-453a-ace2-6f33cb782046 -->

    <owl:Class rdf:about="http://standards.iso.org/iso/10303/tech/refdata/core#46bac3e9-3f47-453a-ace2-6f33cb782046">
        <rdfs:subClassOf rdf:resource="http://standards.iso.org/iso/10303/tech/refdata/core#55105ef0-713f-409a-8306-fd8708d4ee3f"/>
        <dc:contributor>STEP Harmonization Team</dc:contributor>
        <dc:creator>Jean Brangé, AFNeT Services</dc:creator>
        <dc:date>2023-10-04</dc:date>
        <dc:source>ISO/TS 10303-4000</dc:source>
        <dc:type>InWork</dc:type>
        <rdfs:comment xml:lang="en">A SurfaceProfileTolerance is a type of GeometricTolerance that is the definition of a uniform boundary along an ideal profile within which the elements of a surface must lie. The tolerance zone established by a SurfaceProfileTolerance is three dimensional, extending along the length and the width of the considered feature respectively along each segment of a defined size if the FirstUnitSize attribute is specified. If the tolerance is to be unequally disposed about the theoretically exact feature, a ToleranceZone having only one boundary element is associated to the instance of SurfaceProfileTolerance. Unless otherwise specified, the rules governing profile any surface tolerance defined in ISO 1101 shall apply.</rdfs:comment>
        <owl:versionInfo>3</owl:versionInfo>
        <skos:changeNote>[2023-10-04] Jean Brangé, AFNeT Services: Initial definition.</skos:changeNote>
        <skos:note xml:lang="en">Alternatively profile tolerance of a surface can be used according to the specifications given in ASME Y14.5-2009.</skos:note>
        <skos:prefLabel xml:lang="en">surface profile tolerance</skos:prefLabel>
    </owl:Class>
    


    <!-- http://standards.iso.org/iso/10303/tech/refdata/core#46774e46-22a8-48e1-8a0c-d6af49cfd59e -->

    <owl:Class rdf:about="http://standards.iso.org/iso/10303/tech/refdata/core#46774e46-22a8-48e1-8a0c-d6af49cfd59e">
        <rdfs:subClassOf rdf:resource="http://standards.iso.org/iso/10303/tech/refdata/core#84099bf0-130a-0135-b552-598f1b1392ae"/>
        <dc:contributor>STEP Harmonization Team</dc:contributor>
        <dc:creator>Phil Spiby, Eurostep</dc:creator>
        <dc:date>2022-09-01</dc:date>
        <dc:source>ISO/TS 10303-4000</dc:source>
        <dc:type>InWork</dc:type>
        <rdfs:comment xml:lang="en">A TaskMethodRelationship is a specialization of ActivityMethodRelationship that is a relationship between two TaskMethod objects.</rdfs:comment>
        <owl:versionInfo>2</owl:versionInfo>
        <skos:changeNote>[2021-07-30] Initial definition.</skos:changeNote>
        <skos:changeNote>[2022-09-01] Phil Spiby, Eurostep: updated comment updated note.</skos:changeNote>
        <skos:prefLabel xml:lang="en">task method relationship</skos:prefLabel>
    </owl:Class>
    


    <!-- http://standards.iso.org/iso/10303/tech/refdata/core#48196645-acdb-4b2f-8eca-0d596b4cd693 -->

    <owl:Class rdf:about="http://standards.iso.org/iso/10303/tech/refdata/core#48196645-acdb-4b2f-8eca-0d596b4cd693">
        <rdfs:subClassOf rdf:resource="http://standards.iso.org/iso/10303/tech/refdata/core#STEPThing"/>
        <dc:contributor>STEP Harmonization Team</dc:contributor>
        <dc:creator>Phil Spiby, Eurostep</dc:creator>
        <dc:date>2022-09-01</dc:date>
        <dc:source>ISO/TS 10303-4000</dc:source>
        <dc:type>InWork</dc:type>
        <rdfs:comment xml:lang="en">An OrganizationType is a recognized kind of Organization.</rdfs:comment>
        <owl:versionInfo>2</owl:versionInfo>
        <skos:changeNote>[2021-07-30] Initial definition.</skos:changeNote>
        <skos:changeNote>[2022-09-01] Phil Spiby, Eurostep: updated example.</skos:changeNote>
        <skos:example xml:lang="en">Change control board.</skos:example>
        <skos:example xml:lang="en">Department.</skos:example>
        <skos:example xml:lang="en">Legal entity.</skos:example>
        <skos:example xml:lang="en">Manufacturing organization.</skos:example>
        <skos:example xml:lang="en">Sales organization.</skos:example>
        <skos:prefLabel xml:lang="en">organization type</skos:prefLabel>
    </owl:Class>
    


    <!-- http://standards.iso.org/iso/10303/tech/refdata/core#49063745-edcf-40bf-9fce-99ff6d720590 -->

    <owl:Class rdf:about="http://standards.iso.org/iso/10303/tech/refdata/core#49063745-edcf-40bf-9fce-99ff6d720590">
        <rdfs:subClassOf rdf:resource="http://standards.iso.org/iso/10303/tech/refdata/core#STEPThing"/>
        <dc:contributor>STEP Harmonization Team</dc:contributor>
        <dc:creator>Phil Spiby, Eurostep</dc:creator>
        <dc:date>2022-09-01</dc:date>
        <dc:source>ISO/TS 10303-4000</dc:source>
        <dc:type>InWork</dc:type>
        <rdfs:comment xml:lang="en">An Assumption is the identification of something assumed to be true without proof. The reason or justification for an assumption being made shall be represented by a JustificationAssignment being assigned to the Assumption. The item that is assumed shall be related to the Assumption by an ItemAssumed.</rdfs:comment>
        <owl:versionInfo>1</owl:versionInfo>
        <skos:changeNote>[2021-07-30] Initial definition.</skos:changeNote>
        <skos:example xml:lang="en">An activity is planned based on the assumption that the resource required to perform the activity is available at a location.</skos:example>
        <skos:prefLabel xml:lang="en">assumption</skos:prefLabel>
    </owl:Class>
    


    <!-- http://standards.iso.org/iso/10303/tech/refdata/core#5a2218ca-be8d-462a-b45a-1e46a19b3d7b -->

    <owl:Class rdf:about="http://standards.iso.org/iso/10303/tech/refdata/core#5a2218ca-be8d-462a-b45a-1e46a19b3d7b">
        <rdfs:subClassOf rdf:resource="http://standards.iso.org/iso/10303/tech/refdata/core#78133794-f9d2-4e22-aaa0-49690cc93a39"/>
        <dc:contributor>STEP Harmonization Team</dc:contributor>
        <dc:creator>Jean Brangé, AFNeT Services</dc:creator>
        <dc:date>2023-10-04</dc:date>
        <dc:source>ISO/TS 10303-4000</dc:source>
        <dc:type>InWork</dc:type>
        <rdfs:comment xml:lang="en">A TwistedCrossSectionalGroupShapeElement is a type of CrossSectionalGroupShapeElement where all the members are twisted together.</rdfs:comment>
        <owl:versionInfo>3</owl:versionInfo>
        <skos:changeNote>[2023-10-04] Jean Brangé, AFNeT Services: Initial definition.</skos:changeNote>
        <skos:prefLabel xml:lang="en">twisted cross sectional group shape element</skos:prefLabel>
    </owl:Class>
    


    <!-- http://standards.iso.org/iso/10303/tech/refdata/core#5a261d60-7f8f-4fae-a0ae-4fba3cb4b4fb -->

    <owl:Class rdf:about="http://standards.iso.org/iso/10303/tech/refdata/core#5a261d60-7f8f-4fae-a0ae-4fba3cb4b4fb">
        <rdfs:subClassOf rdf:resource="http://standards.iso.org/iso/10303/tech/refdata/core#5e922e0a-8f1d-4650-a0d8-5aaeadccbb0e"/>
        <dc:contributor>STEP Harmonization Team</dc:contributor>
        <dc:creator>Phil Spiby, Eurostep</dc:creator>
        <dc:date>2022-09-01</dc:date>
        <dc:source>ISO/TS 10303-4000</dc:source>
        <dc:type>InWork</dc:type>
        <rdfs:comment xml:lang="en">A HierarchicalInterfaceConnection is a specialization of InterfaceConnection that provides an interconnection between components at different levels in an assembly. Each connection point in the assembly is represented by an InterfaceConnectorOccurrence.</rdfs:comment>
        <owl:versionInfo>1</owl:versionInfo>
        <skos:changeNote>[2021-07-30] Initial definition.</skos:changeNote>
        <skos:example xml:lang="en">An appliance such as a television has a power lead and attached plug. The plug and power lead could be represented as an assembly of parts such as the plug pins and wires. Each connection point of the pins and wires in the assembly is represented by an InterfaceConnectorOccurrence, and an instance of the HierarchicalInterfaceConnection entity data type identifies the connection of the pins (the parts) to the plug (the assembly) in the assembly.</skos:example>
        <skos:prefLabel xml:lang="en">hierarchical interface connection</skos:prefLabel>
    </owl:Class>
    


    <!-- http://standards.iso.org/iso/10303/tech/refdata/core#5a6c8b1f-63af-4307-9faf-9fdd6da5572c -->

    <owl:Class rdf:about="http://standards.iso.org/iso/10303/tech/refdata/core#5a6c8b1f-63af-4307-9faf-9fdd6da5572c">
        <rdfs:subClassOf rdf:resource="http://standards.iso.org/iso/10303/tech/refdata/core#b3911ec0-130a-0135-b552-598f1b1392ae"/>
        <dc:contributor>STEP Harmonization Team</dc:contributor>
        <dc:creator>Jean Brangé, AFNeT Services</dc:creator>
        <dc:date>2023-10-04</dc:date>
        <dc:source>ISO/TS 10303-4000</dc:source>
        <dc:type>InWork</dc:type>
        <rdfs:comment xml:lang="en">A ConstituentPart is a type of PartView. It is a composite item that makes up a composite part. A ConstituentPart may, but need not be, defined in a component-assembly relationship. A ConstituentPart may be either a Ply or a PlyPiece, or a PlyLaminate, or a FilamentLaminate, or a ProcessedCore, or a CompositeAssembly. Several ConstituentParts are illustrated in the figure below. ConstituentPart.pngIllustration of several ConstituentParts</rdfs:comment>
        <owl:versionInfo>3</owl:versionInfo>
        <skos:changeNote>[2023-10-04] Jean Brangé, AFNeT Services: Initial definition.</skos:changeNote>
        <skos:prefLabel xml:lang="en">constituent part</skos:prefLabel>
    </owl:Class>
    


    <!-- http://standards.iso.org/iso/10303/tech/refdata/core#5aafd14f-6efd-4991-9d74-40c779aa2a13 -->

    <owl:Class rdf:about="http://standards.iso.org/iso/10303/tech/refdata/core#5aafd14f-6efd-4991-9d74-40c779aa2a13">
        <rdfs:subClassOf rdf:resource="http://standards.iso.org/iso/10303/tech/refdata/core#c27698c0-130a-0135-b552-598f1b1392ae"/>
        <dc:contributor>STEP Harmonization Team</dc:contributor>
        <dc:creator>Phil Spiby, Eurostep</dc:creator>
        <dc:date>2022-09-01</dc:date>
        <dc:source>ISO/TS 10303-4000</dc:source>
        <dc:type>InWork</dc:type>
        <rdfs:comment xml:lang="en">An ExternalValue is a PropertyValue held in an external system.</rdfs:comment>
        <owl:versionInfo>2</owl:versionInfo>
        <skos:changeNote>[2021-07-30] Initial definition.</skos:changeNote>
        <skos:changeNote>[2022-09-01] Phil Spiby, Eurostep: updated comment updated example.</skos:changeNote>
        <skos:example xml:lang="en">This could include standard values such as &quot;A4&quot; as a paper size. This would be defined as reference data that refers to A4 as defined in ISO 216.</skos:example>
        <skos:prefLabel xml:lang="en">external value</skos:prefLabel>
    </owl:Class>
    


    <!-- http://standards.iso.org/iso/10303/tech/refdata/core#5ade596e-2b7f-4811-b983-a594d88dbfc8 -->

    <owl:Class rdf:about="http://standards.iso.org/iso/10303/tech/refdata/core#5ade596e-2b7f-4811-b983-a594d88dbfc8">
        <rdfs:subClassOf rdf:resource="http://standards.iso.org/iso/10303/tech/refdata/core#1cfca290-3279-0135-b58f-598f1b1392ae"/>
        <dc:contributor>STEP Harmonization Team</dc:contributor>
        <dc:creator>Phil Spiby, Eurostep</dc:creator>
        <dc:date>2022-09-01</dc:date>
        <dc:source>ISO/TS 10303-4000</dc:source>
        <dc:type>InWork</dc:type>
        <rdfs:comment xml:lang="en">A LocatorAssignment is an assignment of a Locator to an item (specified by LocatorAssignmentSelect). The meaning of the assignment can be specified using the ClassifiedAs attribute inherited from the AssignmentObject.</rdfs:comment>
        <owl:versionInfo>2</owl:versionInfo>
        <skos:changeNote>[2021-07-30] Initial definition.</skos:changeNote>
        <skos:changeNote>[2022-09-01] Phil Spiby, Eurostep: updated comment updated note.</skos:changeNote>
        <skos:note xml:lang="en">There can be distinct assignment for each qualification (planned, scheduled or actual). Each assignment can have a start and end date or time. A locator can have multiple assignments.</skos:note>
        <skos:prefLabel xml:lang="en">locator assignment</skos:prefLabel>
    </owl:Class>
    


    <!-- http://standards.iso.org/iso/10303/tech/refdata/core#5b2f693a-2444-4c40-a392-fa1eae4186a2 -->

    <owl:Class rdf:about="http://standards.iso.org/iso/10303/tech/refdata/core#5b2f693a-2444-4c40-a392-fa1eae4186a2">
        <rdfs:subClassOf rdf:resource="http://standards.iso.org/iso/10303/tech/refdata/core#STEPThing"/>
        <dc:contributor>STEP Harmonization Team</dc:contributor>
        <dc:creator>Phil Spiby, Eurostep</dc:creator>
        <dc:date>2022-09-01</dc:date>
        <dc:source>ISO/TS 10303-4000</dc:source>
        <dc:type>InWork</dc:type>
        <rdfs:comment xml:lang="en">An AnalysisRepresentationContext defines the context of an AnalysisModelObject.</rdfs:comment>
        <owl:versionInfo>2</owl:versionInfo>
        <skos:changeNote>[2021-07-30] Initial definition.</skos:changeNote>
        <skos:changeNote>[2022-09-01] Phil Spiby, Eurostep: updated comment.</skos:changeNote>
        <skos:prefLabel xml:lang="en">analysis representation context</skos:prefLabel>
    </owl:Class>
    


    <!-- http://standards.iso.org/iso/10303/tech/refdata/core#5d3983ed-2278-403a-ada3-02526cdcb87a -->

    <owl:Class rdf:about="http://standards.iso.org/iso/10303/tech/refdata/core#5d3983ed-2278-403a-ada3-02526cdcb87a">
        <rdfs:subClassOf rdf:resource="http://standards.iso.org/iso/10303/tech/refdata/core#59b11220-3279-0135-b58f-598f1b1392ae"/>
        <dc:contributor>STEP Harmonization Team</dc:contributor>
        <dc:creator>Phil Spiby, Eurostep</dc:creator>
        <dc:date>2022-09-01</dc:date>
        <dc:source>ISO/TS 10303-4000</dc:source>
        <dc:type>InWork</dc:type>
        <rdfs:comment xml:lang="en">A PersonOrganizationInPositionRelationship is a relationship between two PersonOrganizationInPosition objects.</rdfs:comment>
        <owl:versionInfo>1</owl:versionInfo>
        <skos:changeNote>[2022-09-01] Initial definition.</skos:changeNote>
        <skos:prefLabel xml:lang="en">person organization in position relationship</skos:prefLabel>
    </owl:Class>
    


    <!-- http://standards.iso.org/iso/10303/tech/refdata/core#5d7caeae-c7e0-43a5-b22f-6648fd9752d9 -->

    <owl:Class rdf:about="http://standards.iso.org/iso/10303/tech/refdata/core#5d7caeae-c7e0-43a5-b22f-6648fd9752d9">
        <rdfs:subClassOf rdf:resource="http://standards.iso.org/iso/10303/tech/refdata/core#1cfca290-3279-0135-b58f-598f1b1392ae"/>
        <dc:contributor>STEP Harmonization Team</dc:contributor>
        <dc:creator>Phil Spiby, Eurostep</dc:creator>
        <dc:date>2022-09-01</dc:date>
        <dc:source>ISO/TS 10303-4000</dc:source>
        <dc:type>InWork</dc:type>
        <rdfs:comment xml:lang="en">A RiskPerceptionSourceAssignment is an assignment of an item (specified by RiskPerceptionSourceAssignmentSelect) as a source to a RiskPerception. The meaning of the assignment can be specified using the ClassifiedAs attribute inherited from the AssignmentObject.</rdfs:comment>
        <owl:versionInfo>1</owl:versionInfo>
        <skos:changeNote>[2022-09-01] Initial definition.</skos:changeNote>
        <skos:prefLabel xml:lang="en">risk perception source assignment</skos:prefLabel>
    </owl:Class>
    


    <!-- http://standards.iso.org/iso/10303/tech/refdata/core#5da6df5c-1edc-4a18-b6a1-c371005d6aa1 -->

    <owl:Class rdf:about="http://standards.iso.org/iso/10303/tech/refdata/core#5da6df5c-1edc-4a18-b6a1-c371005d6aa1">
        <rdfs:subClassOf rdf:resource="http://standards.iso.org/iso/10303/tech/refdata/core#bc514af6-504d-408c-aa54-be5472451718"/>
        <dc:contributor>STEP Harmonization Team</dc:contributor>
        <dc:creator>Jean Brangé, AFNeT Services</dc:creator>
        <dc:date>2023-10-04</dc:date>
        <dc:source>ISO/TS 10303-4000</dc:source>
        <dc:type>InWork</dc:type>
        <rdfs:comment xml:lang="en">A DirectionFeatureToleranceZone is a type of ToleranceZoneWithDatum that represents a &quot;direction feature&quot; for a geometric tolerance as defined in ISO 1101.</rdfs:comment>
        <owl:versionInfo>3</owl:versionInfo>
        <skos:changeNote>[2023-10-04] Jean Brangé, AFNeT Services: Initial definition.</skos:changeNote>
        <skos:prefLabel xml:lang="en">direction feature tolerance zone</skos:prefLabel>
    </owl:Class>
    


    <!-- http://standards.iso.org/iso/10303/tech/refdata/core#5de267f0-5f95-4318-ab51-e6552200a8d7 -->

    <owl:Class rdf:about="http://standards.iso.org/iso/10303/tech/refdata/core#5de267f0-5f95-4318-ab51-e6552200a8d7">
        <rdfs:subClassOf rdf:resource="http://standards.iso.org/iso/10303/tech/refdata/core#66348150-092a-4eb7-9561-0b83adfa15ff"/>
        <dc:contributor>STEP Harmonization Team</dc:contributor>
        <dc:creator>Jean Brangé, AFNeT Services</dc:creator>
        <dc:date>2023-10-04</dc:date>
        <dc:source>ISO/TS 10303-4000</dc:source>
        <dc:type>InWork</dc:type>
        <rdfs:comment xml:lang="en">An OccurrenceShapeElement is a type of ShapeElement. An OccurrenceShapeElement represents an element of the shape of an Occurrence. It might be defined by a PartShapeElement, a ShapeFeatureDefinition or another OccurrenceShapeElement from which it inherits all its characteristics.</rdfs:comment>
        <owl:versionInfo>3</owl:versionInfo>
        <skos:changeNote>[2023-10-04] Jean Brangé, AFNeT Services: Initial definition.</skos:changeNote>
        <skos:prefLabel xml:lang="en">occurrence shape element</skos:prefLabel>
    </owl:Class>
    


    <!-- http://standards.iso.org/iso/10303/tech/refdata/core#5e1e2b4e-4284-48f1-9bad-a9c12cb18d07 -->

    <owl:Class rdf:about="http://standards.iso.org/iso/10303/tech/refdata/core#5e1e2b4e-4284-48f1-9bad-a9c12cb18d07">
        <rdfs:subClassOf rdf:resource="http://standards.iso.org/iso/10303/tech/refdata/core#STEPThing"/>
        <dc:contributor>STEP Harmonization Team</dc:contributor>
        <dc:creator>Phil Spiby, Eurostep</dc:creator>
        <dc:date>2022-09-01</dc:date>
        <dc:source>ISO/TS 10303-4000</dc:source>
        <dc:type>InWork</dc:type>
        <rdfs:comment xml:lang="en">An Analysis is the process of studying or examining something in an organized way to learn more about it, or a specific study or examination of something.</rdfs:comment>
        <owl:versionInfo>1</owl:versionInfo>
        <skos:changeNote>[2021-07-30] Initial definition.</skos:changeNote>
        <skos:note xml:lang="en">The full range of the Analysis process includes mathematical, physical testing, cognitive, chemical, etc.</skos:note>
        <skos:prefLabel xml:lang="en">analysis</skos:prefLabel>
    </owl:Class>
    


    <!-- http://standards.iso.org/iso/10303/tech/refdata/core#5e33cc1f-7f90-44f1-9bbf-14e0b01f08a5 -->

    <owl:Class rdf:about="http://standards.iso.org/iso/10303/tech/refdata/core#5e33cc1f-7f90-44f1-9bbf-14e0b01f08a5">
        <rdfs:subClassOf rdf:resource="http://standards.iso.org/iso/10303/tech/refdata/core#9665ed30-130a-0135-b552-598f1b1392ae"/>
        <dc:contributor>STEP Harmonization Team</dc:contributor>
        <dc:creator>Phil Spiby, Eurostep</dc:creator>
        <dc:date>2022-09-01</dc:date>
        <dc:source>ISO/TS 10303-4000</dc:source>
        <dc:type>InWork</dc:type>
        <rdfs:comment xml:lang="en">A PartialDocumentAssignment is an assignment of an identified portion of a document to an item (specified by DocumentAssignmentSelect).</rdfs:comment>
        <owl:versionInfo>2</owl:versionInfo>
        <skos:changeNote>[2021-07-30] Initial definition.</skos:changeNote>
        <skos:changeNote>[2022-09-01] Phil Spiby, Eurostep: updated example.</skos:changeNote>
        <skos:example xml:lang="en">Clause 5 of a Contract document, dealing with project administration, can be assigned to a Project.</skos:example>
        <skos:prefLabel xml:lang="en">partial document assignment</skos:prefLabel>
    </owl:Class>
    


    <!-- http://standards.iso.org/iso/10303/tech/refdata/core#5e343263-3ece-41cc-bd96-d36228e64e62 -->

    <owl:Class rdf:about="http://standards.iso.org/iso/10303/tech/refdata/core#5e343263-3ece-41cc-bd96-d36228e64e62">
        <rdfs:subClassOf rdf:resource="http://standards.iso.org/iso/10303/tech/refdata/core#1cfca290-3279-0135-b58f-598f1b1392ae"/>
        <dc:contributor>STEP Harmonization Team</dc:contributor>
        <dc:creator>Phil Spiby, Eurostep</dc:creator>
        <dc:date>2022-09-01</dc:date>
        <dc:source>ISO/TS 10303-4000</dc:source>
        <dc:type>InWork</dc:type>
        <rdfs:comment xml:lang="en">A PositionTypeAssignment is an assignment of a PositionType to an item (specified by PositionTypeAssignmentSelect). The meaning of the assignment can be specified using the ClassifiedAs attribute inherited from the AssignmentObject.</rdfs:comment>
        <owl:versionInfo>1</owl:versionInfo>
        <skos:changeNote>[2022-09-01] Initial definition.</skos:changeNote>
        <skos:prefLabel xml:lang="en">position type assignment</skos:prefLabel>
    </owl:Class>
    


    <!-- http://standards.iso.org/iso/10303/tech/refdata/core#5e922e0a-8f1d-4650-a0d8-5aaeadccbb0e -->

    <owl:Class rdf:about="http://standards.iso.org/iso/10303/tech/refdata/core#5e922e0a-8f1d-4650-a0d8-5aaeadccbb0e">
        <rdfs:subClassOf rdf:resource="http://standards.iso.org/iso/10303/tech/refdata/core#STEPThing"/>
        <dc:contributor>STEP Harmonization Team</dc:contributor>
        <dc:creator>Phil Spiby, Eurostep</dc:creator>
        <dc:date>2022-09-01</dc:date>
        <dc:source>ISO/TS 10303-4000</dc:source>
        <dc:type>InWork</dc:type>
        <rdfs:comment xml:lang="en">An InterfaceConnection is an interconnection between a pair of items (specified by ConnectionSelect).</rdfs:comment>
        <owl:versionInfo>2</owl:versionInfo>
        <skos:changeNote>[2021-07-30] Initial definition.</skos:changeNote>
        <skos:changeNote>[2022-09-01] Phil Spiby, Eurostep: updated comment.</skos:changeNote>
        <skos:example xml:lang="en">An appliance such as a television has a power lead and attached plug. The plug and power lead could be represented as an assembly of parts such as the plug pins and wires. Each connection point of the pins and wires in the assembly is represented by an InterfaceConnectorOccurrence, and an instance of the InterfaceConnection entity data type identifies the connection of the pins to the wires in the assembly.</skos:example>
        <skos:prefLabel xml:lang="en">interface connection</skos:prefLabel>
    </owl:Class>
    


    <!-- http://standards.iso.org/iso/10303/tech/refdata/core#5ee4842f-9943-4ef1-b118-bfc6ba0e3ac8 -->

    <owl:Class rdf:about="http://standards.iso.org/iso/10303/tech/refdata/core#5ee4842f-9943-4ef1-b118-bfc6ba0e3ac8">
        <rdfs:subClassOf rdf:resource="http://standards.iso.org/iso/10303/tech/refdata/core#d2eb1f4f-b98f-4393-a7ed-24dc41900bd2"/>
        <dc:contributor>STEP Harmonization Team</dc:contributor>
        <dc:creator>Jean Brangé, AFNeT Services</dc:creator>
        <dc:date>2023-10-04</dc:date>
        <dc:source>ISO/TS 10303-4000</dc:source>
        <dc:type>InWork</dc:type>
        <rdfs:comment xml:lang="en">A TargetArea is a type of DatumTarget that specifies an area bounded by a closed ShapeElement. The shape of the TargetArea is described explicitly by a set of curves with reference to the part coordinate system.</rdfs:comment>
        <owl:versionInfo>3</owl:versionInfo>
        <skos:changeNote>[2023-10-04] Jean Brangé, AFNeT Services: Initial definition.</skos:changeNote>
        <skos:prefLabel xml:lang="en">target area</skos:prefLabel>
    </owl:Class>
    


    <!-- http://standards.iso.org/iso/10303/tech/refdata/core#5f758d1e-21e1-4374-90d1-7edcedd1ba90 -->

    <owl:Class rdf:about="http://standards.iso.org/iso/10303/tech/refdata/core#5f758d1e-21e1-4374-90d1-7edcedd1ba90">
        <rdfs:subClassOf rdf:resource="http://standards.iso.org/iso/10303/tech/refdata/core#085b6771-a1f8-4cf7-9771-8de2f3a063a1"/>
        <dc:contributor>STEP Harmonization Team</dc:contributor>
        <dc:creator>Phil Spiby, Eurostep</dc:creator>
        <dc:date>2022-09-01</dc:date>
        <dc:source>ISO/TS 10303-4000</dc:source>
        <dc:type>InWork</dc:type>
        <rdfs:comment xml:lang="en">A StateDefinitionHypothesisAssociation is a subjective statement without supporting evidence that a StateObserved is comparable with a particular StateDefinition.</rdfs:comment>
        <owl:versionInfo>1</owl:versionInfo>
        <skos:changeNote>[2021-07-30] Initial definition.</skos:changeNote>
        <skos:prefLabel xml:lang="en">state definition hypothesis association</skos:prefLabel>
    </owl:Class>
    


    <!-- http://standards.iso.org/iso/10303/tech/refdata/core#5f8212a0-fa71-4a9c-be7c-74eac72bba3e -->

    <owl:Class rdf:about="http://standards.iso.org/iso/10303/tech/refdata/core#5f8212a0-fa71-4a9c-be7c-74eac72bba3e">
        <rdfs:subClassOf rdf:resource="http://standards.iso.org/iso/10303/tech/refdata/core#1cfca290-3279-0135-b58f-598f1b1392ae"/>
        <dc:contributor>STEP Harmonization Team</dc:contributor>
        <dc:creator>Phil Spiby, Eurostep</dc:creator>
        <dc:date>2022-09-01</dc:date>
        <dc:source>ISO/TS 10303-4000</dc:source>
        <dc:type>InWork</dc:type>
        <rdfs:comment xml:lang="en">A PositionAssignment is an assignment of a Position to an item (specified by PositionAssignmentSelect). The meaning of the assignment can be specified using the ClassifiedAs attribute inherited from the AssignmentObject.</rdfs:comment>
        <owl:versionInfo>1</owl:versionInfo>
        <skos:changeNote>[2022-09-01] Initial definition.</skos:changeNote>
        <skos:prefLabel xml:lang="en">position assignment</skos:prefLabel>
    </owl:Class>
    


    <!-- http://standards.iso.org/iso/10303/tech/refdata/core#50e00d4c-edaa-4fba-93a6-feeb2eccc46a -->

    <owl:Class rdf:about="http://standards.iso.org/iso/10303/tech/refdata/core#50e00d4c-edaa-4fba-93a6-feeb2eccc46a">
        <rdfs:subClassOf rdf:resource="http://standards.iso.org/iso/10303/tech/refdata/core#d1796b3a-5ade-4d7a-b9e0-4af28a9cfddb"/>
        <dc:contributor>STEP Harmonization Team</dc:contributor>
        <dc:creator>Jean Brangé, AFNeT Services</dc:creator>
        <dc:date>2023-10-04</dc:date>
        <dc:source>ISO/TS 10303-4000</dc:source>
        <dc:type>InWork</dc:type>
        <rdfs:comment xml:lang="en">A PartShapeElementRelationship is a type of ShapeElementRelationship that represents a relationship between two instances of PartShapeElement.</rdfs:comment>
        <owl:versionInfo>3</owl:versionInfo>
        <skos:changeNote>[2023-10-04] Jean Brangé, AFNeT Services: Initial definition.</skos:changeNote>
        <skos:prefLabel xml:lang="en">part shape element relationship</skos:prefLabel>
    </owl:Class>
    


    <!-- http://standards.iso.org/iso/10303/tech/refdata/core#50f7e4dc-2a92-41e8-a755-0fa506125b9f -->

    <owl:Class rdf:about="http://standards.iso.org/iso/10303/tech/refdata/core#50f7e4dc-2a92-41e8-a755-0fa506125b9f">
        <rdfs:subClassOf rdf:resource="http://standards.iso.org/iso/10303/tech/refdata/core#b608a929-7fa0-4643-8237-59c6cf4d0dbc"/>
        <dc:contributor>STEP Harmonization Team</dc:contributor>
        <dc:creator>Jean Brangé, AFNeT Services</dc:creator>
        <dc:date>2023-10-04</dc:date>
        <dc:source>ISO/TS 10303-4000</dc:source>
        <dc:type>InWork</dc:type>
        <rdfs:comment xml:lang="en">An OccurrenceTransportFeature is a type of OccurrenceShapeFeature that enables the transport of information, energy or matter between several OccurrenceTerminals of the same Occurrence.</rdfs:comment>
        <owl:versionInfo>3</owl:versionInfo>
        <skos:changeNote>[2023-10-04] Jean Brangé, AFNeT Services: Initial definition.</skos:changeNote>
        <skos:prefLabel xml:lang="en">occurrence transport feature</skos:prefLabel>
    </owl:Class>
    


    <!-- http://standards.iso.org/iso/10303/tech/refdata/core#5185cb3e-1c24-4338-991a-0b34babdf714 -->

    <owl:Class rdf:about="http://standards.iso.org/iso/10303/tech/refdata/core#5185cb3e-1c24-4338-991a-0b34babdf714">
        <rdfs:subClassOf rdf:resource="http://standards.iso.org/iso/10303/tech/refdata/core#50e00d4c-edaa-4fba-93a6-feeb2eccc46a"/>
        <dc:contributor>STEP Harmonization Team</dc:contributor>
        <dc:creator>Jean Brangé, AFNeT Services</dc:creator>
        <dc:date>2023-10-04</dc:date>
        <dc:source>ISO/TS 10303-4000</dc:source>
        <dc:type>InWork</dc:type>
        <rdfs:comment xml:lang="en">A PartFeatureFitRelationship is a type of PartShapeElementRelationship that states that the two related PartFeatures fit with each other.</rdfs:comment>
        <owl:versionInfo>3</owl:versionInfo>
        <skos:changeNote>[2023-10-04] Jean Brangé, AFNeT Services: Initial definition.</skos:changeNote>
        <skos:prefLabel xml:lang="en">part feature fit relationship</skos:prefLabel>
    </owl:Class>
    


    <!-- http://standards.iso.org/iso/10303/tech/refdata/core#528ada01-3556-4da5-ab84-ee62c9d68215 -->

    <owl:Class rdf:about="http://standards.iso.org/iso/10303/tech/refdata/core#528ada01-3556-4da5-ab84-ee62c9d68215">
        <rdfs:subClassOf rdf:resource="http://standards.iso.org/iso/10303/tech/refdata/core#d0cd8f0f-07c9-4a4d-9aec-bc0ccc1d901d"/>
        <dc:contributor>STEP Harmonization Team</dc:contributor>
        <dc:creator>Jean Brangé, AFNeT Services</dc:creator>
        <dc:date>2023-10-04</dc:date>
        <dc:source>ISO/TS 10303-4000</dc:source>
        <dc:type>InWork</dc:type>
        <rdfs:comment xml:lang="en">An AllAroundShapeElement is a type of CompositeShapeElement that represents the concept of &quot;all around&quot; as defined in ISO 1101.</rdfs:comment>
        <owl:versionInfo>3</owl:versionInfo>
        <skos:changeNote>[2023-10-04] Jean Brangé, AFNeT Services: Initial definition.</skos:changeNote>
        <skos:note xml:lang="en">Alternatively all around can be used according to the specifications given in ASME Y14.5-2009</skos:note>
        <skos:prefLabel xml:lang="en">all around shape element</skos:prefLabel>
    </owl:Class>
    


    <!-- http://standards.iso.org/iso/10303/tech/refdata/core#53e20541-4d83-4902-a059-b807ec6e0f42 -->

    <owl:Class rdf:about="http://standards.iso.org/iso/10303/tech/refdata/core#53e20541-4d83-4902-a059-b807ec6e0f42">
        <rdfs:subClassOf rdf:resource="http://standards.iso.org/iso/10303/tech/refdata/core#59b11220-3279-0135-b58f-598f1b1392ae"/>
        <dc:contributor>STEP Harmonization Team</dc:contributor>
        <dc:creator>Phil Spiby, Eurostep</dc:creator>
        <dc:date>2022-09-01</dc:date>
        <dc:source>ISO/TS 10303-4000</dc:source>
        <dc:type>InWork</dc:type>
        <rdfs:comment xml:lang="en">A StateDefinitionRelationship is an association between two StateDefinition objects.</rdfs:comment>
        <owl:versionInfo>2</owl:versionInfo>
        <skos:changeNote>[2021-07-30] Initial definition.</skos:changeNote>
        <skos:changeNote>[2022-09-01] Phil Spiby, Eurostep: updated comment updated note.</skos:changeNote>
        <skos:note xml:lang="en">Relationships between StateDefinition entities can be used to support fault diagnosis.</skos:note>
        <skos:prefLabel xml:lang="en">state definition relationship</skos:prefLabel>
    </owl:Class>
    


    <!-- http://standards.iso.org/iso/10303/tech/refdata/core#537e6225-29d7-4028-8397-096cdae5b9b2 -->

    <owl:Class rdf:about="http://standards.iso.org/iso/10303/tech/refdata/core#537e6225-29d7-4028-8397-096cdae5b9b2">
        <rdfs:subClassOf rdf:resource="http://standards.iso.org/iso/10303/tech/refdata/core#1cfca290-3279-0135-b58f-598f1b1392ae"/>
        <dc:contributor>STEP Harmonization Team</dc:contributor>
        <dc:creator>Phil Spiby, Eurostep</dc:creator>
        <dc:date>2022-09-01</dc:date>
        <dc:source>ISO/TS 10303-4000</dc:source>
        <dc:type>InWork</dc:type>
        <rdfs:comment xml:lang="en">A RequiredResourceAssignment is an assignment of a RequiredResource to an item (specified by RequiredResourceAssignmentSelect) that requires the resource. The meaning of the assignment can be specified using the ClassifiedAs attribute inherited from the AssignmentObject.</rdfs:comment>
        <owl:versionInfo>2</owl:versionInfo>
        <skos:changeNote>[2021-07-30] Initial definition.</skos:changeNote>
        <skos:changeNote>[2022-09-01] Phil Spiby, Eurostep: updated comment updated example.</skos:changeNote>
        <skos:example xml:lang="en">A resource required by the activity &quot;12&quot; needs to be calibrated prior to usage. The calibration activity &quot;21&quot; is associated with the same required resource.</skos:example>
        <skos:example xml:lang="en">A resource required by the task &quot;123&quot; needs to be disposed after its usage. This disposal task &quot;456&quot; is associated with the same required resource.</skos:example>
        <skos:example xml:lang="en">Task, task step, activity, activity method, organization are examples of entities to which the resource requirement statement could be related.</skos:example>
        <skos:example xml:lang="en">The assignment can be classified as &quot;required by&quot;.</skos:example>
        <skos:note xml:lang="en">An association between a required resource and actions that are needed prior to its usage.</skos:note>
        <skos:prefLabel xml:lang="en">required resource assignment</skos:prefLabel>
    </owl:Class>
    


    <!-- http://standards.iso.org/iso/10303/tech/refdata/core#543a3366-6b70-442c-a2a1-47953f0e7986 -->

    <owl:Class rdf:about="http://standards.iso.org/iso/10303/tech/refdata/core#543a3366-6b70-442c-a2a1-47953f0e7986">
        <rdfs:subClassOf rdf:resource="http://standards.iso.org/iso/10303/tech/refdata/core#55105ef0-713f-409a-8306-fd8708d4ee3f"/>
        <dc:contributor>STEP Harmonization Team</dc:contributor>
        <dc:creator>Jean Brangé, AFNeT Services</dc:creator>
        <dc:date>2023-10-04</dc:date>
        <dc:source>ISO/TS 10303-4000</dc:source>
        <dc:type>InWork</dc:type>
        <rdfs:comment xml:lang="en">A CircularRunoutTolerance is a type of GeometricTolerance that constrains the deviation of features constructed about an axis or at right angles to an axis. Each measurement position, either along the axis, or away from the axis, is independently rotated through 360 degrees. Unless otherwise specified, the rules governing circular run-out tolerance defined in ISO 1101 shall apply.</rdfs:comment>
        <owl:versionInfo>3</owl:versionInfo>
        <skos:changeNote>[2023-10-04] Jean Brangé, AFNeT Services: Initial definition.</skos:changeNote>
        <skos:note xml:lang="en">Alternatively circular run-out tolerance can be used according to the specifications given in ASME Y14.5-2009.</skos:note>
        <skos:prefLabel xml:lang="en">circular runout tolerance</skos:prefLabel>
    </owl:Class>
    


    <!-- http://standards.iso.org/iso/10303/tech/refdata/core#54850f2e-b0d2-4476-95a4-146ec1202fca -->

    <owl:Class rdf:about="http://standards.iso.org/iso/10303/tech/refdata/core#54850f2e-b0d2-4476-95a4-146ec1202fca">
        <rdfs:subClassOf rdf:resource="http://standards.iso.org/iso/10303/tech/refdata/core#1f09cf40-e045-476a-b811-eb6e56de0ced"/>
        <dc:contributor>STEP Harmonization Team</dc:contributor>
        <dc:creator>Jean Brangé, AFNeT Services</dc:creator>
        <dc:date>2023-10-04</dc:date>
        <dc:source>ISO/TS 10303-4000</dc:source>
        <dc:type>InWork</dc:type>
        <rdfs:comment xml:lang="en">A LinearDistance is a type of DimensionalLocation that specifies the distance along a straight line between two elements of a shape.</rdfs:comment>
        <owl:versionInfo>3</owl:versionInfo>
        <skos:changeNote>[2023-10-04] Jean Brangé, AFNeT Services: Initial definition.</skos:changeNote>
        <skos:prefLabel xml:lang="en">linear distance</skos:prefLabel>
    </owl:Class>
    


    <!-- http://standards.iso.org/iso/10303/tech/refdata/core#55105ef0-713f-409a-8306-fd8708d4ee3f -->

    <owl:Class rdf:about="http://standards.iso.org/iso/10303/tech/refdata/core#55105ef0-713f-409a-8306-fd8708d4ee3f">
        <rdfs:subClassOf rdf:resource="http://standards.iso.org/iso/10303/tech/refdata/core#STEPThing"/>
        <dc:contributor>STEP Harmonization Team</dc:contributor>
        <dc:creator>Jean Brangé, AFNeT Services</dc:creator>
        <dc:date>2023-10-04</dc:date>
        <dc:source>ISO/TS 10303-4000</dc:source>
        <dc:type>InWork</dc:type>
        <rdfs:comment xml:lang="en">A GeometricTolerance is a specification of the allowed deviation of some element of the shape of a product from its theoretically exact shape.</rdfs:comment>
        <owl:versionInfo>3</owl:versionInfo>
        <skos:changeNote>[2023-10-04] Jean Brangé, AFNeT Services: Initial definition.</skos:changeNote>
        <skos:prefLabel xml:lang="en">geometric tolerance</skos:prefLabel>
    </owl:Class>
    


    <!-- http://standards.iso.org/iso/10303/tech/refdata/core#56ca2ef3-43f6-4837-b143-3850a3741816 -->

    <owl:Class rdf:about="http://standards.iso.org/iso/10303/tech/refdata/core#56ca2ef3-43f6-4837-b143-3850a3741816">
        <rdfs:subClassOf rdf:resource="http://standards.iso.org/iso/10303/tech/refdata/core#0cc8b831-37f7-4cd5-984f-dbb5588fbc1d"/>
        <dc:contributor>STEP Harmonization Team</dc:contributor>
        <dc:creator>Jean Brangé, AFNeT Services</dc:creator>
        <dc:date>2023-10-04</dc:date>
        <dc:source>ISO/TS 10303-4000</dc:source>
        <dc:type>InWork</dc:type>
        <rdfs:comment xml:lang="en">An AssemblyShapeJoint is a type of PartShapeElement that defines a joint between two or more OccurrenceShapeFeatures within an AssemblyDefinition. An AssemblyShapeJoint may be composed of other AssemblyShapeJoints.</rdfs:comment>
        <owl:versionInfo>3</owl:versionInfo>
        <skos:changeNote>[2023-10-04] Jean Brangé, AFNeT Services: Initial definition.</skos:changeNote>
        <skos:prefLabel xml:lang="en">assembly shape joint</skos:prefLabel>
    </owl:Class>
    


    <!-- http://standards.iso.org/iso/10303/tech/refdata/core#56fb7e1d-d3d9-415b-83e7-1d6dec561a2e -->

    <owl:Class rdf:about="http://standards.iso.org/iso/10303/tech/refdata/core#56fb7e1d-d3d9-415b-83e7-1d6dec561a2e">
        <rdfs:subClassOf rdf:resource="http://standards.iso.org/iso/10303/tech/refdata/core#STEPThing"/>
        <dc:contributor>STEP Harmonization Team</dc:contributor>
        <dc:creator>Phil Spiby, Eurostep</dc:creator>
        <dc:date>2022-09-01</dc:date>
        <dc:source>ISO/TS 10303-4000</dc:source>
        <dc:type>InWork</dc:type>
        <rdfs:comment xml:lang="en">An InterfaceDefinitionConnection is an interconnection between a pair of views (specified by InterfaceDefinitionConnectionSelect).</rdfs:comment>
        <owl:versionInfo>2</owl:versionInfo>
        <skos:changeNote>[2021-07-30] Initial definition.</skos:changeNote>
        <skos:changeNote>[2022-09-01] Phil Spiby, Eurostep: updated comment.</skos:changeNote>
        <skos:example xml:lang="en">A socket in the wall provides access to the domestic electricity supply. An appliance such as a television has a power lead and plug that fits into the socket. An instance of the InterfaceDefinitionConnection entity data type identifies this fitting of the plug into the socket.</skos:example>
        <skos:prefLabel xml:lang="en">interface definition connection</skos:prefLabel>
    </owl:Class>
    


    <!-- http://standards.iso.org/iso/10303/tech/refdata/core#5620e9b2-61f4-4606-9a56-741680df36f3 -->

    <owl:Class rdf:about="http://standards.iso.org/iso/10303/tech/refdata/core#5620e9b2-61f4-4606-9a56-741680df36f3">
        <rdfs:subClassOf rdf:resource="http://standards.iso.org/iso/10303/tech/refdata/core#756b7320-fa8b-4bb7-83d2-2d6a4e31675d"/>
        <dc:contributor>STEP Harmonization Team</dc:contributor>
        <dc:creator>Jean Brangé, AFNeT Services</dc:creator>
        <dc:date>2023-10-04</dc:date>
        <dc:source>ISO/TS 10303-4000</dc:source>
        <dc:type>InWork</dc:type>
        <rdfs:comment xml:lang="en">A ShapeFeatureDefinitionOccurrenceElementRelationship is a type of ShapeFeatureDefinitionElementRelationship that is defined by a ShapeFeatureDefinitionRelationship or a ShapeFeatureDefinitionElementRelationship.</rdfs:comment>
        <owl:versionInfo>3</owl:versionInfo>
        <skos:changeNote>[2023-10-04] Jean Brangé, AFNeT Services: Initial definition.</skos:changeNote>
        <skos:prefLabel xml:lang="en">shape feature definition occurrence element relationship</skos:prefLabel>
    </owl:Class>
    


    <!-- http://standards.iso.org/iso/10303/tech/refdata/core#567cffbf-b749-428e-8aa7-63ec22c29ee5 -->

    <owl:Class rdf:about="http://standards.iso.org/iso/10303/tech/refdata/core#567cffbf-b749-428e-8aa7-63ec22c29ee5">
        <rdfs:subClassOf rdf:resource="http://standards.iso.org/iso/10303/tech/refdata/core#1ab6f279-97db-4102-9cb3-76462f5db8d9"/>
        <dc:contributor>STEP Harmonization Team</dc:contributor>
        <dc:creator>Jean Brangé, AFNeT Services</dc:creator>
        <dc:date>2023-10-04</dc:date>
        <dc:source>ISO/TS 10303-4000</dc:source>
        <dc:type>InWork</dc:type>
        <rdfs:comment xml:lang="en">A ContactFeatureDefinition is a type of ShapeFeatureDefinition that can be connected with another ContactFeatureDefinition in the case that a ContactFeatureDefinitionFitRelationship is defined between them.</rdfs:comment>
        <owl:versionInfo>3</owl:versionInfo>
        <skos:changeNote>[2023-10-04] Jean Brangé, AFNeT Services: Initial definition.</skos:changeNote>
        <skos:prefLabel xml:lang="en">contact feature definition</skos:prefLabel>
    </owl:Class>
    


    <!-- http://standards.iso.org/iso/10303/tech/refdata/core#57bfc15f-8822-42c2-9259-0bcf8e28f9dd -->

    <owl:Class rdf:about="http://standards.iso.org/iso/10303/tech/refdata/core#57bfc15f-8822-42c2-9259-0bcf8e28f9dd">
        <rdfs:subClassOf rdf:resource="http://standards.iso.org/iso/10303/tech/refdata/core#59b11220-3279-0135-b58f-598f1b1392ae"/>
        <dc:contributor>STEP Harmonization Team</dc:contributor>
        <dc:creator>Phil Spiby, Eurostep</dc:creator>
        <dc:date>2022-09-01</dc:date>
        <dc:source>ISO/TS 10303-4000</dc:source>
        <dc:type>InWork</dc:type>
        <rdfs:comment xml:lang="en">An InterfaceConnectorOccurrenceRelationship is a relationship between two InterfaceConnectorOccurrence objects.</rdfs:comment>
        <owl:versionInfo>2</owl:versionInfo>
        <skos:changeNote>[2021-07-30] Initial definition.</skos:changeNote>
        <skos:changeNote>[2022-09-01] Phil Spiby, Eurostep: updated comment.</skos:changeNote>
        <skos:prefLabel xml:lang="en">interface connector occurrence relationship</skos:prefLabel>
    </owl:Class>
    


    <!-- http://standards.iso.org/iso/10303/tech/refdata/core#57f5782d-8378-4465-8dc9-aa244dfd667f -->

    <owl:Class rdf:about="http://standards.iso.org/iso/10303/tech/refdata/core#57f5782d-8378-4465-8dc9-aa244dfd667f">
        <rdfs:subClassOf rdf:resource="http://standards.iso.org/iso/10303/tech/refdata/core#STEPThing"/>
        <dc:contributor>STEP Harmonization Team</dc:contributor>
        <dc:creator>Phil Spiby, Eurostep</dc:creator>
        <dc:date>2022-09-01</dc:date>
        <dc:source>ISO/TS 10303-4000</dc:source>
        <dc:type>InWork</dc:type>
        <rdfs:comment xml:lang="en">A Message is a collection of information, brought together by an originator (the message definer) for some specific purpose, generally the fulfilment of a process. A Message is an historical record, intended to be sent using an Envelope and in consequence, is not versioned. Once a Message is sent to a first addressee, it shall not be changed. However it shall not remain unsent, since that is to confuse its functions and therefore its meaning with other entities such as Document.</rdfs:comment>
        <owl:versionInfo>2</owl:versionInfo>
        <skos:changeNote>[2021-07-30] Initial definition.</skos:changeNote>
        <skos:changeNote>[2022-09-01] Phil Spiby, Eurostep: updated comment updated note.</skos:changeNote>
        <skos:note xml:lang="en">The same Message can be sent several times using different Envelope objects.</skos:note>
        <skos:prefLabel xml:lang="en">message</skos:prefLabel>
    </owl:Class>
    


    <!-- http://standards.iso.org/iso/10303/tech/refdata/core#571cd187-bb98-479c-ac89-9e1806639328 -->

    <owl:Class rdf:about="http://standards.iso.org/iso/10303/tech/refdata/core#571cd187-bb98-479c-ac89-9e1806639328">
        <rdfs:subClassOf rdf:resource="http://standards.iso.org/iso/10303/tech/refdata/core#1cfca290-3279-0135-b58f-598f1b1392ae"/>
        <dc:contributor>STEP Harmonization Team</dc:contributor>
        <dc:creator>Phil Spiby, Eurostep</dc:creator>
        <dc:date>2022-09-01</dc:date>
        <dc:source>ISO/TS 10303-4000</dc:source>
        <dc:type>InWork</dc:type>
        <rdfs:comment xml:lang="en">A StateAssignment is an assignment of a State to an item (specified by StateAssignmentSelect). The meaning of the assignment can be specified using the ClassifiedAs attribute inherited from the AssignmentObject.</rdfs:comment>
        <owl:versionInfo>2</owl:versionInfo>
        <skos:changeNote>[2021-07-30] Initial definition.</skos:changeNote>
        <skos:changeNote>[2022-09-01] Phil Spiby, Eurostep: updated comment.</skos:changeNote>
        <skos:prefLabel xml:lang="en">state assignment</skos:prefLabel>
    </owl:Class>
    


    <!-- http://standards.iso.org/iso/10303/tech/refdata/core#5751a7a4-365c-4e9f-be33-0b966af998a8 -->

    <owl:Class rdf:about="http://standards.iso.org/iso/10303/tech/refdata/core#5751a7a4-365c-4e9f-be33-0b966af998a8">
        <rdfs:subClassOf rdf:resource="http://standards.iso.org/iso/10303/tech/refdata/core#59b11220-3279-0135-b58f-598f1b1392ae"/>
        <dc:contributor>STEP Harmonization Team</dc:contributor>
        <dc:creator>Jean Brangé, AFNeT Services</dc:creator>
        <dc:date>2023-10-04</dc:date>
        <dc:source>ISO/TS 10303-4000</dc:source>
        <dc:type>InWork</dc:type>
        <rdfs:comment xml:lang="en">A ProcessPlanRelationship is an association between two ProcessPlan objects.</rdfs:comment>
        <owl:versionInfo>3</owl:versionInfo>
        <skos:changeNote>[2023-10-04] Jean Brangé, AFNeT Services: Initial definition.</skos:changeNote>
        <skos:example xml:lang="en">If a part shall be manufactured in two different manufacturing sites, such as one in Paris and the other in Bordeaux, there will be two different process plans, that may be related by a ProcessPlanRelationship.</skos:example>
        <skos:prefLabel xml:lang="en">process plan relationship</skos:prefLabel>
    </owl:Class>
    


    <!-- http://standards.iso.org/iso/10303/tech/refdata/core#59b11220-3279-0135-b58f-598f1b1392ae -->

    <owl:Class rdf:about="http://standards.iso.org/iso/10303/tech/refdata/core#59b11220-3279-0135-b58f-598f1b1392ae">
        <rdfs:subClassOf rdf:resource="http://standards.iso.org/iso/10303/tech/refdata/core#STEPThing"/>
        <dc:contributor>STEP Harmonization Team</dc:contributor>
        <dc:creator>Phil Spiby, Eurostep</dc:creator>
        <dc:date>2022-09-01</dc:date>
        <dc:source>ISO/TS 10303-4000</dc:source>
        <dc:type>InWork</dc:type>
        <rdfs:comment xml:lang="en">A RelationshipObject is a generalization of all relationships in the Core model used to identify common properties of relationships. A Relationship is defined to be a dependency between two objects.</rdfs:comment>
        <owl:versionInfo>1</owl:versionInfo>
        <skos:changeNote>[2021-07-30] Initial definition.</skos:changeNote>
        <skos:note xml:lang="en">The objects being related are normally, but not always, of the same type or specializations.</skos:note>
        <skos:prefLabel xml:lang="en">relationship object</skos:prefLabel>
    </owl:Class>
    


    <!-- http://standards.iso.org/iso/10303/tech/refdata/core#59cf1733-c833-4af3-9a46-faeec7a3301c -->

    <owl:Class rdf:about="http://standards.iso.org/iso/10303/tech/refdata/core#59cf1733-c833-4af3-9a46-faeec7a3301c">
        <rdfs:subClassOf rdf:resource="http://standards.iso.org/iso/10303/tech/refdata/core#STEPThing"/>
        <dc:contributor>STEP Harmonization Team</dc:contributor>
        <dc:creator>Phil Spiby, Eurostep</dc:creator>
        <dc:date>2022-09-01</dc:date>
        <dc:source>ISO/TS 10303-4000</dc:source>
        <dc:type>InWork</dc:type>
        <rdfs:comment xml:lang="en">An AddressComponent is a constituent part of an address. A non-empty set of AddressComponents makes up an address.</rdfs:comment>
        <owl:versionInfo>2</owl:versionInfo>
        <skos:changeNote>[2021-07-30] Initial definition.</skos:changeNote>
        <skos:changeNote>[2022-09-01] Phil Spiby, Eurostep: updated example.</skos:changeNote>
        <skos:example xml:lang="en">&quot;The Hills&quot; is a constituent part of the address &quot;99 Lombardy Street, The Hills, United Kingdom&quot;</skos:example>
        <skos:prefLabel xml:lang="en">address component</skos:prefLabel>
    </owl:Class>
    


    <!-- http://standards.iso.org/iso/10303/tech/refdata/core#5952bf98-2ea0-46c9-8915-249fe039b206 -->

    <owl:Class rdf:about="http://standards.iso.org/iso/10303/tech/refdata/core#5952bf98-2ea0-46c9-8915-249fe039b206">
        <rdfs:subClassOf rdf:resource="http://standards.iso.org/iso/10303/tech/refdata/core#STEPThing"/>
        <dc:contributor>STEP Harmonization Team</dc:contributor>
        <dc:creator>Phil Spiby, Eurostep</dc:creator>
        <dc:date>2022-09-01</dc:date>
        <dc:source>ISO/TS 10303-4000</dc:source>
        <dc:type>InWork</dc:type>
        <rdfs:comment xml:lang="en">A RiskView is an abstract generalization of instances that represent the perception or consequence of a risk.</rdfs:comment>
        <owl:versionInfo>1</owl:versionInfo>
        <skos:changeNote>[2022-09-01] Initial definition.</skos:changeNote>
        <skos:prefLabel xml:lang="en">risk view</skos:prefLabel>
    </owl:Class>
    


    <!-- http://standards.iso.org/iso/10303/tech/refdata/core#6a1b1df6-a932-4c3c-9d2e-7314ccde1588 -->

    <owl:Class rdf:about="http://standards.iso.org/iso/10303/tech/refdata/core#6a1b1df6-a932-4c3c-9d2e-7314ccde1588">
        <rdfs:subClassOf rdf:resource="http://standards.iso.org/iso/10303/tech/refdata/core#9c98fe40-130a-0135-b552-598f1b1392ae"/>
        <dc:contributor>STEP Harmonization Team</dc:contributor>
        <dc:creator>Jean Brangé, AFNeT Services</dc:creator>
        <dc:date>2023-10-04</dc:date>
        <dc:source>ISO/TS 10303-4000</dc:source>
        <dc:type>InWork</dc:type>
        <rdfs:comment xml:lang="en">An ExternalManifoldSurfaceShapeRepresentation is a type of ExternalGeometricModel that references an instance of type ../../../resources/aic_manifold_surface/aic_manifold_surface.htm#aic_manifold_surface.manifold_surface_shape_representation manifold_surface_shape_representation (ISO 10303-509).</rdfs:comment>
        <owl:versionInfo>3</owl:versionInfo>
        <skos:changeNote>[2023-10-04] Jean Brangé, AFNeT Services: Initial definition.</skos:changeNote>
        <skos:prefLabel xml:lang="en">external manifold surface shape representation</skos:prefLabel>
    </owl:Class>
    


    <!-- http://standards.iso.org/iso/10303/tech/refdata/core#6a3f51c5-c90f-4cc4-bb55-a3dffaa8078f -->

    <owl:Class rdf:about="http://standards.iso.org/iso/10303/tech/refdata/core#6a3f51c5-c90f-4cc4-bb55-a3dffaa8078f">
        <rdfs:subClassOf rdf:resource="http://standards.iso.org/iso/10303/tech/refdata/core#59b11220-3279-0135-b58f-598f1b1392ae"/>
        <dc:contributor>STEP Harmonization Team</dc:contributor>
        <dc:creator>Phil Spiby, Eurostep</dc:creator>
        <dc:date>2022-09-01</dc:date>
        <dc:source>ISO/TS 10303-4000</dc:source>
        <dc:type>InWork</dc:type>
        <rdfs:comment xml:lang="en">A RiskPerceptionRelationship is a relationship between two RiskPerception objects.</rdfs:comment>
        <owl:versionInfo>1</owl:versionInfo>
        <skos:changeNote>[2022-09-01] Initial definition.</skos:changeNote>
        <skos:prefLabel xml:lang="en">risk perception relationship</skos:prefLabel>
    </owl:Class>
    


    <!-- http://standards.iso.org/iso/10303/tech/refdata/core#6b33b7bd-217f-4035-a134-fa0ece66891a -->

    <owl:Class rdf:about="http://standards.iso.org/iso/10303/tech/refdata/core#6b33b7bd-217f-4035-a134-fa0ece66891a">
        <rdfs:subClassOf rdf:resource="http://standards.iso.org/iso/10303/tech/refdata/core#1d59c650-3279-0135-b58f-598f1b1392ae"/>
        <dc:contributor>STEP Harmonization Team</dc:contributor>
        <dc:creator>Jean Brangé, AFNeT Services</dc:creator>
        <dc:date>2023-10-04</dc:date>
        <dc:source>ISO/TS 10303-4000</dc:source>
        <dc:type>InWork</dc:type>
        <rdfs:comment xml:lang="en">A MotionModelAssociation is an association of a MotionModelSelect to an AssemblyDefinition.</rdfs:comment>
        <owl:versionInfo>3</owl:versionInfo>
        <skos:changeNote>[2023-10-04] Jean Brangé, AFNeT Services: Initial definition.</skos:changeNote>
        <skos:prefLabel xml:lang="en">motion model association</skos:prefLabel>
    </owl:Class>
    


    <!-- http://standards.iso.org/iso/10303/tech/refdata/core#6b4a9963-0bbc-46ff-b7c5-ff8cf6d858ba -->

    <owl:Class rdf:about="http://standards.iso.org/iso/10303/tech/refdata/core#6b4a9963-0bbc-46ff-b7c5-ff8cf6d858ba">
        <rdfs:subClassOf rdf:resource="http://standards.iso.org/iso/10303/tech/refdata/core#adbb48e0-130a-0135-b552-598f1b1392ae"/>
        <dc:contributor>STEP Harmonization Team</dc:contributor>
        <dc:creator>Jean Brangé, AFNeT Services</dc:creator>
        <dc:date>2023-10-04</dc:date>
        <dc:source>ISO/TS 10303-4000</dc:source>
        <dc:type>InWork</dc:type>
        <rdfs:comment xml:lang="en">A MatedPartAssociation is a type of NextAssemblyOccurrenceUsage between a MatingDefinition and an Occurrence that is used within the MatingDefinition.</rdfs:comment>
        <owl:versionInfo>3</owl:versionInfo>
        <skos:changeNote>[2023-10-04] Jean Brangé, AFNeT Services: Initial definition.</skos:changeNote>
        <skos:prefLabel xml:lang="en">mated part association</skos:prefLabel>
    </owl:Class>
    


    <!-- http://standards.iso.org/iso/10303/tech/refdata/core#6bbd8cb4-9c52-4272-a70f-3683487359a6 -->

    <owl:Class rdf:about="http://standards.iso.org/iso/10303/tech/refdata/core#6bbd8cb4-9c52-4272-a70f-3683487359a6">
        <rdfs:subClassOf rdf:resource="http://standards.iso.org/iso/10303/tech/refdata/core#7a449fab-fe68-4296-a567-4e02b6c32e19"/>
        <dc:contributor>STEP Harmonization Team</dc:contributor>
        <dc:creator>Jean Brangé, AFNeT Services</dc:creator>
        <dc:date>2023-10-04</dc:date>
        <dc:source>ISO/TS 10303-4000</dc:source>
        <dc:type>InWork</dc:type>
        <rdfs:comment xml:lang="en">A WirePartIdentification is a type of PartTransportFeature that identifies a specific colour code for the wire.</rdfs:comment>
        <owl:versionInfo>3</owl:versionInfo>
        <skos:changeNote>[2023-10-04] Jean Brangé, AFNeT Services: Initial definition.</skos:changeNote>
        <skos:prefLabel xml:lang="en">wire part identification</skos:prefLabel>
    </owl:Class>
    


    <!-- http://standards.iso.org/iso/10303/tech/refdata/core#6c4d3383-83eb-464f-8a9b-184db21a8207 -->

    <owl:Class rdf:about="http://standards.iso.org/iso/10303/tech/refdata/core#6c4d3383-83eb-464f-8a9b-184db21a8207">
        <rdfs:subClassOf rdf:resource="http://standards.iso.org/iso/10303/tech/refdata/core#02761765-5f96-4ed2-a51c-38aaa796367d"/>
        <dc:contributor>STEP Harmonization Team</dc:contributor>
        <dc:creator>Jean Brangé, AFNeT Services</dc:creator>
        <dc:date>2023-10-04</dc:date>
        <dc:source>ISO/TS 10303-4000</dc:source>
        <dc:type>InWork</dc:type>
        <rdfs:comment xml:lang="en">A CompositeGroupShapeElement is a type of CompositeShapeElement in which the composite may be thought of as a group of individual ShapeElement in which any property that is applied to the CompositeGroupShapeElement is applied to each of the constituent ShapeElements on an individual basis.</rdfs:comment>
        <owl:versionInfo>3</owl:versionInfo>
        <skos:changeNote>[2023-10-04] Jean Brangé, AFNeT Services: Initial definition.</skos:changeNote>
        <skos:prefLabel xml:lang="en">composite group shape element</skos:prefLabel>
    </owl:Class>
    


    <!-- http://standards.iso.org/iso/10303/tech/refdata/core#6c882234-0c81-4ce4-8c92-67ec53fec5f9 -->

    <owl:Class rdf:about="http://standards.iso.org/iso/10303/tech/refdata/core#6c882234-0c81-4ce4-8c92-67ec53fec5f9">
        <rdfs:subClassOf rdf:resource="http://standards.iso.org/iso/10303/tech/refdata/core#87556b90-130a-0135-b552-598f1b1392ae"/>
        <dc:contributor>STEP Harmonization Team</dc:contributor>
        <dc:creator>Jean Brangé, AFNeT Services</dc:creator>
        <dc:date>2023-10-04</dc:date>
        <dc:source>ISO/TS 10303-4000</dc:source>
        <dc:type>InWork</dc:type>
        <rdfs:comment xml:lang="en">A WiringHarnessAssemblyDesign is a type of AssemblyDefinition. A WiringHarnessAssemblyDesign is a design view of a wiring harness assembly that is designed to allow for installation and removal as a unit. It contains any number of wire harness components that include connectors, contacts, wires, cables, and protections.</rdfs:comment>
        <owl:versionInfo>3</owl:versionInfo>
        <skos:changeNote>[2023-10-04] Jean Brangé, AFNeT Services: Initial definition.</skos:changeNote>
        <skos:prefLabel xml:lang="en">wiring harness assembly design</skos:prefLabel>
    </owl:Class>
    


    <!-- http://standards.iso.org/iso/10303/tech/refdata/core#6d2f2b49-dd73-432b-8e79-07fbc1cc1f34 -->

    <owl:Class rdf:about="http://standards.iso.org/iso/10303/tech/refdata/core#6d2f2b49-dd73-432b-8e79-07fbc1cc1f34">
        <rdfs:subClassOf rdf:resource="http://standards.iso.org/iso/10303/tech/refdata/core#STEPThing"/>
        <dc:contributor>STEP Harmonization Team</dc:contributor>
        <dc:creator>Phil Spiby, Eurostep</dc:creator>
        <dc:date>2022-09-01</dc:date>
        <dc:source>ISO/TS 10303-4000</dc:source>
        <dc:type>InWork</dc:type>
        <rdfs:comment xml:lang="en">An ExperienceGained is a relationship between an ExperienceInstance and a person or organization (specified by PersonOrganizationSelect).</rdfs:comment>
        <owl:versionInfo>1</owl:versionInfo>
        <skos:changeNote>[2022-09-01] Initial definition.</skos:changeNote>
        <skos:prefLabel xml:lang="en">experience gained</skos:prefLabel>
    </owl:Class>
    


    <!-- http://standards.iso.org/iso/10303/tech/refdata/core#6d367e10-7640-4a8f-acaa-42963438a3aa -->

    <owl:Class rdf:about="http://standards.iso.org/iso/10303/tech/refdata/core#6d367e10-7640-4a8f-acaa-42963438a3aa">
        <rdfs:subClassOf rdf:resource="http://standards.iso.org/iso/10303/tech/refdata/core#c6260c30-130a-0135-b552-598f1b1392ae"/>
        <dc:contributor>STEP Harmonization Team</dc:contributor>
        <dc:creator>Jean Brangé, AFNeT Services</dc:creator>
        <dc:date>2023-10-04</dc:date>
        <dc:source>ISO/TS 10303-4000</dc:source>
        <dc:type>InWork</dc:type>
        <rdfs:comment xml:lang="en">A PlyOrientationAngle is an entity that defines a specific direction within a Ply. The direction is defined in the coordinate axis of a ReinforcementOrientationBasis. The measurement is in degrees between -90 and +90. A PlyOrientationAngle may be one either a DrapedOrientationAngle or a LaidOrientationAngle.</rdfs:comment>
        <owl:versionInfo>3</owl:versionInfo>
        <skos:changeNote>[2023-10-04] Jean Brangé, AFNeT Services: Initial definition.</skos:changeNote>
        <skos:note xml:lang="en">For materials with multiple fiber orientations, the direction shall correspond to the warp direction of the material. Warp fibers are the primary load carrying fibers within a fabric material.</skos:note>
        <skos:note xml:lang="en">In the design of a specific composite part, a finite set of PlyOrientationAngle values are established for use. An example of a set of commonly used PlyOrientationAngle is (0, 90, +45, -45).</skos:note>
        <skos:prefLabel xml:lang="en">ply orientation angle</skos:prefLabel>
    </owl:Class>
    


    <!-- http://standards.iso.org/iso/10303/tech/refdata/core#6d4d4ccd-20d2-4209-9fe6-17da7b3cb1a1 -->

    <owl:Class rdf:about="http://standards.iso.org/iso/10303/tech/refdata/core#6d4d4ccd-20d2-4209-9fe6-17da7b3cb1a1">
        <rdfs:subClassOf rdf:resource="http://standards.iso.org/iso/10303/tech/refdata/core#b3911ec0-130a-0135-b552-598f1b1392ae"/>
        <dc:contributor>STEP Harmonization Team</dc:contributor>
        <dc:creator>Jean Brangé, AFNeT Services</dc:creator>
        <dc:date>2023-10-04</dc:date>
        <dc:source>ISO/TS 10303-4000</dc:source>
        <dc:type>InWork</dc:type>
        <rdfs:comment xml:lang="en">A LaminateTable is a type of PartView. A LaminateTable defines the internal constituents or structural makeup of an overall part or a specific zone, area, or point on the part. A LaminateTable may be either a PlyLaminateTable, a ZoneStructuralMakeup or a CompositeAssemblyTable.</rdfs:comment>
        <owl:versionInfo>3</owl:versionInfo>
        <skos:changeNote>[2023-10-04] Jean Brangé, AFNeT Services: Initial definition.</skos:changeNote>
        <skos:note xml:lang="en">There are two functions provided by a LaminateTable. The first is to describe the order in which the physical constituents of a laminate are assembled. This is called a PlyLaminateTable or CompositeAssemblyTable. The second is to describe the structural makeup of a specific zone, area, or point within a laminate. This is called a ZoneStructuralMakeup.</skos:note>
        <skos:prefLabel xml:lang="en">laminate table</skos:prefLabel>
    </owl:Class>
    


    <!-- http://standards.iso.org/iso/10303/tech/refdata/core#6dd8c93b-ba22-465a-831e-8db08feca526 -->

    <owl:Class rdf:about="http://standards.iso.org/iso/10303/tech/refdata/core#6dd8c93b-ba22-465a-831e-8db08feca526">
        <rdfs:subClassOf rdf:resource="http://standards.iso.org/iso/10303/tech/refdata/core#1cfca290-3279-0135-b58f-598f1b1392ae"/>
        <dc:contributor>STEP Harmonization Team</dc:contributor>
        <dc:creator>Jean Brangé, AFNeT Services</dc:creator>
        <dc:date>2023-10-04</dc:date>
        <dc:source>ISO/TS 10303-4000</dc:source>
        <dc:type>InWork</dc:type>
        <rdfs:comment xml:lang="en">An AppearanceAssignment is the identification of the characteristics of visual appearance of geometric or annotation elements.</rdfs:comment>
        <owl:versionInfo>3</owl:versionInfo>
        <skos:changeNote>[2023-10-04] Jean Brangé, AFNeT Services: Initial definition.</skos:changeNote>
        <skos:note xml:lang="en">Several appearance components can be simultaneously specified with an AppearanceAssignment.</skos:note>
        <skos:note xml:lang="en">The appearance can be defined explicitly for each represented element or for a context in which the elements are represented.</skos:note>
        <skos:note xml:lang="en">The various visual characteristics that can be assigned to points, curves or surfaces are defined in other application modules.</skos:note>
        <skos:prefLabel xml:lang="en">appearance assignment</skos:prefLabel>
    </owl:Class>
    


    <!-- http://standards.iso.org/iso/10303/tech/refdata/core#6dd9cf80-d3e5-4f94-8d78-bc20c058e7ab -->

    <owl:Class rdf:about="http://standards.iso.org/iso/10303/tech/refdata/core#6dd9cf80-d3e5-4f94-8d78-bc20c058e7ab">
        <rdfs:subClassOf rdf:resource="http://standards.iso.org/iso/10303/tech/refdata/core#59b11220-3279-0135-b58f-598f1b1392ae"/>
        <dc:contributor>STEP Harmonization Team</dc:contributor>
        <dc:creator>Jean Brangé, AFNeT Services</dc:creator>
        <dc:date>2023-10-04</dc:date>
        <dc:source>ISO/TS 10303-4000</dc:source>
        <dc:type>InWork</dc:type>
        <rdfs:comment xml:lang="en">A LinkMotionRelationship is an association of the GeometricModel or ExternalGeometricModel of a link and a LinkMotionAlongPath with a parameter or time dependent transformation.</rdfs:comment>
        <owl:versionInfo>3</owl:versionInfo>
        <skos:changeNote>[2023-10-04] Jean Brangé, AFNeT Services: Initial definition.</skos:changeNote>
        <skos:prefLabel xml:lang="en">link motion relationship</skos:prefLabel>
    </owl:Class>
    


    <!-- http://standards.iso.org/iso/10303/tech/refdata/core#6e0727ea-e257-4f41-a639-449ed15cf944 -->

    <owl:Class rdf:about="http://standards.iso.org/iso/10303/tech/refdata/core#6e0727ea-e257-4f41-a639-449ed15cf944">
        <rdfs:subClassOf rdf:resource="http://standards.iso.org/iso/10303/tech/refdata/core#e1f21c44-a15a-40d1-ac2d-e6849a953d9d"/>
        <dc:contributor>STEP Harmonization Team</dc:contributor>
        <dc:creator>Jean Brangé, AFNeT Services</dc:creator>
        <dc:date>2023-10-04</dc:date>
        <dc:source>ISO/TS 10303-4000</dc:source>
        <dc:type>InWork</dc:type>
        <rdfs:comment xml:lang="en">A GeometricSheetRepresentation is a type of CompositeSheetRepresentation that is defined by a surface and a set of curves. These curves are related in the application to that surface. The curves define a closed area but are not necessarily restrained topologically.</rdfs:comment>
        <owl:versionInfo>3</owl:versionInfo>
        <skos:changeNote>[2023-10-04] Jean Brangé, AFNeT Services: Initial definition.</skos:changeNote>
        <skos:prefLabel xml:lang="en">geometric sheet representation</skos:prefLabel>
    </owl:Class>
    


    <!-- http://standards.iso.org/iso/10303/tech/refdata/core#6e1b983d-223a-47cb-b041-5fc6bb1675fb -->

    <owl:Class rdf:about="http://standards.iso.org/iso/10303/tech/refdata/core#6e1b983d-223a-47cb-b041-5fc6bb1675fb">
        <rdfs:subClassOf rdf:resource="http://standards.iso.org/iso/10303/tech/refdata/core#af0b342e-b77d-4ac9-abdc-26d92ffb92a9"/>
        <dc:contributor>STEP Harmonization Team</dc:contributor>
        <dc:creator>Jean Brangé, AFNeT Services</dc:creator>
        <dc:date>2023-10-04</dc:date>
        <dc:source>ISO/TS 10303-4000</dc:source>
        <dc:type>InWork</dc:type>
        <rdfs:comment xml:lang="en">A DiameterSize is a type of DimensionalSize that is a diameter of a circular, cylindrical, spherical, or toroidal feature.</rdfs:comment>
        <owl:versionInfo>3</owl:versionInfo>
        <skos:changeNote>[2023-10-04] Jean Brangé, AFNeT Services: Initial definition.</skos:changeNote>
        <skos:prefLabel xml:lang="en">diameter size</skos:prefLabel>
    </owl:Class>
    


    <!-- http://standards.iso.org/iso/10303/tech/refdata/core#6e861f1c-a656-40ca-8ca7-249165a96549 -->

    <owl:Class rdf:about="http://standards.iso.org/iso/10303/tech/refdata/core#6e861f1c-a656-40ca-8ca7-249165a96549">
        <rdfs:subClassOf rdf:resource="http://standards.iso.org/iso/10303/tech/refdata/core#1d59c650-3279-0135-b58f-598f1b1392ae"/>
        <dc:contributor>STEP Harmonization Team</dc:contributor>
        <dc:creator>Phil Spiby, Eurostep</dc:creator>
        <dc:date>2022-09-01</dc:date>
        <dc:source>ISO/TS 10303-4000</dc:source>
        <dc:type>InWork</dc:type>
        <rdfs:comment xml:lang="en">An ObservationConsequence is an association of an observation to the consequences that follow from it, where those consequences are in the form of an activity to be performed (specified by ObservationConsequenceSelect).</rdfs:comment>
        <owl:versionInfo>1</owl:versionInfo>
        <skos:changeNote>[2022-09-01] Initial definition.</skos:changeNote>
        <skos:note xml:lang="en">One of the uses of ObservationConsequence is to close one of the feedback loops from the use of a product to requests for its enhancements.</skos:note>
        <skos:prefLabel xml:lang="en">observation consequence</skos:prefLabel>
    </owl:Class>
    


    <!-- http://standards.iso.org/iso/10303/tech/refdata/core#6e9d6828-a81d-4472-9caf-9d47f240d6d6 -->

    <owl:Class rdf:about="http://standards.iso.org/iso/10303/tech/refdata/core#6e9d6828-a81d-4472-9caf-9d47f240d6d6">
        <rdfs:subClassOf rdf:resource="http://standards.iso.org/iso/10303/tech/refdata/core#STEPThing"/>
        <dc:contributor>STEP Harmonization Team</dc:contributor>
        <dc:creator>Phil Spiby, Eurostep</dc:creator>
        <dc:date>2022-09-01</dc:date>
        <dc:source>ISO/TS 10303-4000</dc:source>
        <dc:type>InWork</dc:type>
        <rdfs:comment xml:lang="en">A ResourceAsRealized is a record of a resource that has been used or consumed.</rdfs:comment>
        <owl:versionInfo>2</owl:versionInfo>
        <skos:changeNote>[2021-07-30] Initial definition.</skos:changeNote>
        <skos:changeNote>[2022-09-01] Phil Spiby, Eurostep: updated example.</skos:changeNote>
        <skos:example xml:lang="en">A resource as realized can be classified as &quot;Used&quot; or &quot;Consumed&quot;.</skos:example>
        <skos:prefLabel xml:lang="en">resource as realized</skos:prefLabel>
    </owl:Class>
    


    <!-- http://standards.iso.org/iso/10303/tech/refdata/core#6ec284f0-30c6-4149-a677-8c6a5af5e6fc -->

    <owl:Class rdf:about="http://standards.iso.org/iso/10303/tech/refdata/core#6ec284f0-30c6-4149-a677-8c6a5af5e6fc">
        <rdfs:subClassOf rdf:resource="http://standards.iso.org/iso/10303/tech/refdata/core#STEPThing"/>
        <dc:contributor>STEP Harmonization Team</dc:contributor>
        <dc:creator>Phil Spiby, Eurostep</dc:creator>
        <dc:date>2022-09-01</dc:date>
        <dc:source>ISO/TS 10303-4000</dc:source>
        <dc:type>InWork</dc:type>
        <rdfs:comment xml:lang="en">A Position is a function or job performed by a person. It defines responsibilities and activities. A position that is not fulfilled by a person is a vacancy.</rdfs:comment>
        <owl:versionInfo>1</owl:versionInfo>
        <skos:changeNote>[2022-09-01] Initial definition.</skos:changeNote>
        <skos:example xml:lang="en">Company Director</skos:example>
        <skos:example xml:lang="en">Service Engineer</skos:example>
        <skos:prefLabel xml:lang="en">position</skos:prefLabel>
    </owl:Class>
    


    <!-- http://standards.iso.org/iso/10303/tech/refdata/core#6067df0d-3ac2-4fc8-829c-6c59487ead9e -->

    <owl:Class rdf:about="http://standards.iso.org/iso/10303/tech/refdata/core#6067df0d-3ac2-4fc8-829c-6c59487ead9e">
        <rdfs:subClassOf rdf:resource="http://standards.iso.org/iso/10303/tech/refdata/core#99130bd0-130a-0135-b552-598f1b1392ae"/>
        <dc:contributor>STEP Harmonization Team</dc:contributor>
        <dc:creator>Phil Spiby, Eurostep</dc:creator>
        <dc:date>2022-09-01</dc:date>
        <dc:source>ISO/TS 10303-4000</dc:source>
        <dc:type>InWork</dc:type>
        <rdfs:comment xml:lang="en">A ConditionalEffectivity is a type of Effectivity for which the domain of applicability is defined by an explicit condition.</rdfs:comment>
        <owl:versionInfo>1</owl:versionInfo>
        <skos:changeNote>[2021-07-30] Initial definition.</skos:changeNote>
        <skos:prefLabel xml:lang="en">conditional effectivity</skos:prefLabel>
    </owl:Class>
    


    <!-- http://standards.iso.org/iso/10303/tech/refdata/core#618e4ba7-0616-48c2-a221-ae93e4c57ba6 -->

    <owl:Class rdf:about="http://standards.iso.org/iso/10303/tech/refdata/core#618e4ba7-0616-48c2-a221-ae93e4c57ba6">
        <rdfs:subClassOf rdf:resource="http://standards.iso.org/iso/10303/tech/refdata/core#STEPThing"/>
        <dc:contributor>STEP Harmonization Team</dc:contributor>
        <dc:creator>Phil Spiby, Eurostep</dc:creator>
        <dc:date>2022-09-01</dc:date>
        <dc:source>ISO/TS 10303-4000</dc:source>
        <dc:type>InWork</dc:type>
        <rdfs:comment xml:lang="en">An InterfaceSpecification provides a definition of necessary attributes for one or more items that participate in an interface.</rdfs:comment>
        <owl:versionInfo>1</owl:versionInfo>
        <skos:changeNote>[2021-07-30] Initial definition.</skos:changeNote>
        <skos:example xml:lang="en">BSI develops a standard for connecting domestic electrical equipment to the electricity supply.</skos:example>
        <skos:prefLabel xml:lang="en">interface specification</skos:prefLabel>
    </owl:Class>
    


    <!-- http://standards.iso.org/iso/10303/tech/refdata/core#63992755-813d-44d5-bc4a-7714c631db1c -->

    <owl:Class rdf:about="http://standards.iso.org/iso/10303/tech/refdata/core#63992755-813d-44d5-bc4a-7714c631db1c">
        <rdfs:subClassOf rdf:resource="http://standards.iso.org/iso/10303/tech/refdata/core#af0b342e-b77d-4ac9-abdc-26d92ffb92a9"/>
        <dc:contributor>STEP Harmonization Team</dc:contributor>
        <dc:creator>Jean Brangé, AFNeT Services</dc:creator>
        <dc:date>2023-10-04</dc:date>
        <dc:source>ISO/TS 10303-4000</dc:source>
        <dc:type>InWork</dc:type>
        <rdfs:comment xml:lang="en">An AngularSize is a type of DimensionalSize. An AngularSize size is the measure of the angle formed by two boundaries of the ShapeElement and their common or projected intersection. An AngularSize defines an angular spatial characteristic of a ShapeElement. An AngularSize is represented by a single magnitude and is independent of the location of the ShapeElement on or within the product. AngularSize.gifAngularSize</rdfs:comment>
        <owl:versionInfo>3</owl:versionInfo>
        <skos:changeNote>[2023-10-04] Jean Brangé, AFNeT Services: Initial definition.</skos:changeNote>
        <skos:note xml:lang="en">The Figure AngularSize illustrates the AngularSize.</skos:note>
        <skos:prefLabel xml:lang="en">angular size</skos:prefLabel>
    </owl:Class>
    


    <!-- http://standards.iso.org/iso/10303/tech/refdata/core#64b61099-86a0-4a34-a439-025c989b9760 -->

    <owl:Class rdf:about="http://standards.iso.org/iso/10303/tech/refdata/core#64b61099-86a0-4a34-a439-025c989b9760">
        <rdfs:subClassOf rdf:resource="http://standards.iso.org/iso/10303/tech/refdata/core#STEPThing"/>
        <dc:contributor>STEP Harmonization Team</dc:contributor>
        <dc:creator>Phil Spiby, Eurostep</dc:creator>
        <dc:date>2022-09-01</dc:date>
        <dc:source>ISO/TS 10303-4000</dc:source>
        <dc:type>InWork</dc:type>
        <rdfs:comment xml:lang="en">A SlotDefinition identifies a definition of a Slot.</rdfs:comment>
        <owl:versionInfo>1</owl:versionInfo>
        <skos:changeNote>[2022-09-01] Initial definition.</skos:changeNote>
        <skos:example xml:lang="en">An airworthiness authority requires an airline company to report which individual engines power the aircraft at different times during the lifetime of the aircraft.</skos:example>
        <skos:prefLabel xml:lang="en">slot definition</skos:prefLabel>
    </owl:Class>
    


    <!-- http://standards.iso.org/iso/10303/tech/refdata/core#6490f437-5aff-4d04-b436-f4243e3160f8 -->

    <owl:Class rdf:about="http://standards.iso.org/iso/10303/tech/refdata/core#6490f437-5aff-4d04-b436-f4243e3160f8">
        <rdfs:subClassOf rdf:resource="http://standards.iso.org/iso/10303/tech/refdata/core#STEPThing"/>
        <dc:contributor>STEP Harmonization Team</dc:contributor>
        <dc:creator>Phil Spiby, Eurostep</dc:creator>
        <dc:date>2022-09-01</dc:date>
        <dc:source>ISO/TS 10303-4000</dc:source>
        <dc:type>InWork</dc:type>
        <rdfs:comment xml:lang="en">An EnvironmentVersion is an identification of a version of an Environment. This is an abstract object which specializations are EnvironmentDefinitionVersion and ObservedEnvironmentVersion.</rdfs:comment>
        <owl:versionInfo>1</owl:versionInfo>
        <skos:changeNote>[2021-07-30] Initial definition.</skos:changeNote>
        <skos:prefLabel xml:lang="en">environment version</skos:prefLabel>
    </owl:Class>
    


    <!-- http://standards.iso.org/iso/10303/tech/refdata/core#65fd71da-4f9c-4fd0-892d-d85274c29fd0 -->

    <owl:Class rdf:about="http://standards.iso.org/iso/10303/tech/refdata/core#65fd71da-4f9c-4fd0-892d-d85274c29fd0">
        <rdfs:subClassOf rdf:resource="http://standards.iso.org/iso/10303/tech/refdata/core#STEPThing"/>
        <dc:contributor>STEP Harmonization Team</dc:contributor>
        <dc:creator>Phil Spiby, Eurostep</dc:creator>
        <dc:date>2022-09-01</dc:date>
        <dc:source>ISO/TS 10303-4000</dc:source>
        <dc:type>InWork</dc:type>
        <rdfs:comment xml:lang="en">A PersonNameComponent is a constituent part of a PersonName. A non-empty set of PersonNameComponent objects makes up a person name.</rdfs:comment>
        <owl:versionInfo>2</owl:versionInfo>
        <skos:changeNote>[2021-07-30] Initial definition.</skos:changeNote>
        <skos:changeNote>[2022-09-01] Phil Spiby, Eurostep: updated comment updated example.</skos:changeNote>
        <skos:example xml:lang="en">&quot;Peter&quot; is a constituent part of the person name &quot;Peter, Pan&quot;.</skos:example>
        <skos:prefLabel xml:lang="en">person name component</skos:prefLabel>
    </owl:Class>
    


    <!-- http://standards.iso.org/iso/10303/tech/refdata/core#66b08bd9-1013-4ef5-adf8-39d30478825f -->

    <owl:Class rdf:about="http://standards.iso.org/iso/10303/tech/refdata/core#66b08bd9-1013-4ef5-adf8-39d30478825f">
        <rdfs:subClassOf rdf:resource="http://standards.iso.org/iso/10303/tech/refdata/core#55105ef0-713f-409a-8306-fd8708d4ee3f"/>
        <dc:contributor>STEP Harmonization Team</dc:contributor>
        <dc:creator>Jean Brangé, AFNeT Services</dc:creator>
        <dc:date>2023-10-04</dc:date>
        <dc:source>ISO/TS 10303-4000</dc:source>
        <dc:type>InWork</dc:type>
        <rdfs:comment xml:lang="en">A ParallelismTolerance is a type of GeometricTolerance that specifies that a surface or a curve shall be parallel to a reference datum, with an allowed amount of deviation. A ParallelismTolerance specifies one of the following: a tolerance zone limited by two planes or two lines (if the attribute DirectedOrOrientedToleranceZone is specified) parallel to a datum plane, or axis, within which the line elements of the surface or the axis of the considered feature must lie; a cylindrical tolerance zone whose axis is parallel to a datum axis within which the axis of the considered feature must lie. Unless otherwise specified, the rules governing parallelism tolerance defined in ISO 1101 shall apply.</rdfs:comment>
        <owl:versionInfo>3</owl:versionInfo>
        <skos:changeNote>[2023-10-04] Jean Brangé, AFNeT Services: Initial definition.</skos:changeNote>
        <skos:note xml:lang="en">Alternatively parallelism tolerance can be used according to the specifications given in ASME Y14.5-2009.</skos:note>
        <skos:prefLabel xml:lang="en">parallelism tolerance</skos:prefLabel>
    </owl:Class>
    


    <!-- http://standards.iso.org/iso/10303/tech/refdata/core#66348150-092a-4eb7-9561-0b83adfa15ff -->

    <owl:Class rdf:about="http://standards.iso.org/iso/10303/tech/refdata/core#66348150-092a-4eb7-9561-0b83adfa15ff">
        <rdfs:subClassOf rdf:resource="http://standards.iso.org/iso/10303/tech/refdata/core#STEPThing"/>
        <dc:contributor>STEP Harmonization Team</dc:contributor>
        <dc:creator>Jean Brangé, AFNeT Services</dc:creator>
        <dc:date>2023-10-04</dc:date>
        <dc:source>ISO/TS 10303-4000</dc:source>
        <dc:type>InWork</dc:type>
        <rdfs:comment xml:lang="en">A ShapeElement is a portion of shape that has to be identified explicitly to be associated with other information.</rdfs:comment>
        <owl:versionInfo>3</owl:versionInfo>
        <skos:changeNote>[2023-10-04] Jean Brangé, AFNeT Services: Initial definition.</skos:changeNote>
        <skos:example xml:lang="en">An example for classifying ShapeElement objects is to identify all parts of an air plane that constitute the outer surface of the plane and are therefore relevant for aerodynamic analyses.</skos:example>
        <skos:example xml:lang="en">In order to identify a portion of one face of a shaft that shall have a surface coating applied to it, ShapeElement is used.</skos:example>
        <skos:example xml:lang="en">The threaded portion of the shape of a bolt may be represented as a ShapeElement, so that other properties, such as surface finish, may be associated with it.</skos:example>
        <skos:note xml:lang="en">A ShapeElement may be a CoatingLayer.</skos:note>
        <skos:note xml:lang="en">ShapeElement objects can be classified using Class.</skos:note>
        <skos:prefLabel xml:lang="en">shape element</skos:prefLabel>
    </owl:Class>
    


    <!-- http://standards.iso.org/iso/10303/tech/refdata/core#67676460-111d-40b5-bf37-b3bb54dff1f5 -->

    <owl:Class rdf:about="http://standards.iso.org/iso/10303/tech/refdata/core#67676460-111d-40b5-bf37-b3bb54dff1f5">
        <rdfs:subClassOf rdf:resource="http://standards.iso.org/iso/10303/tech/refdata/core#95f1bde5-b263-4ca1-89df-33e1205800dd"/>
        <dc:contributor>STEP Harmonization Team</dc:contributor>
        <dc:creator>Phil Spiby, Eurostep</dc:creator>
        <dc:date>2022-09-01</dc:date>
        <dc:source>ISO/TS 10303-4000</dc:source>
        <dc:type>InWork</dc:type>
        <rdfs:comment xml:lang="en">A TaskElementLevels is a type of TaskElement that provides two or more different descriptions in place of a single method. The actual work will be the same whichever alternative TaskElement is followed.</rdfs:comment>
        <owl:versionInfo>1</owl:versionInfo>
        <skos:changeNote>[2021-07-30] Initial definition.</skos:changeNote>
        <skos:note xml:lang="en">This can be used to provide different levels of description of a task for people with varying levels of experience or expertise.</skos:note>
        <skos:prefLabel xml:lang="en">task element levels</skos:prefLabel>
    </owl:Class>
    


    <!-- http://standards.iso.org/iso/10303/tech/refdata/core#68242b94-82e8-4841-8005-89981113e22f -->

    <owl:Class rdf:about="http://standards.iso.org/iso/10303/tech/refdata/core#68242b94-82e8-4841-8005-89981113e22f">
        <rdfs:subClassOf rdf:resource="http://standards.iso.org/iso/10303/tech/refdata/core#STEPThing"/>
        <dc:contributor>STEP Harmonization Team</dc:contributor>
        <dc:creator>Phil Spiby, Eurostep</dc:creator>
        <dc:date>2022-09-01</dc:date>
        <dc:source>ISO/TS 10303-4000</dc:source>
        <dc:type>InWork</dc:type>
        <rdfs:comment xml:lang="en">A Locator is a means of representing a Location.</rdfs:comment>
        <owl:versionInfo>1</owl:versionInfo>
        <skos:changeNote>[2021-07-30] Initial definition.</skos:changeNote>
        <skos:prefLabel xml:lang="en">locator</skos:prefLabel>
    </owl:Class>
    


    <!-- http://standards.iso.org/iso/10303/tech/refdata/core#699b4d8a-1050-44b3-95bb-c2818434d526 -->

    <owl:Class rdf:about="http://standards.iso.org/iso/10303/tech/refdata/core#699b4d8a-1050-44b3-95bb-c2818434d526">
        <rdfs:subClassOf rdf:resource="http://standards.iso.org/iso/10303/tech/refdata/core#1cfca290-3279-0135-b58f-598f1b1392ae"/>
        <dc:contributor>STEP Harmonization Team</dc:contributor>
        <dc:creator>Jean Brangé, AFNeT Services</dc:creator>
        <dc:date>2023-10-04</dc:date>
        <dc:source>ISO/TS 10303-4000</dc:source>
        <dc:type>InWork</dc:type>
        <rdfs:comment xml:lang="en">A ProcessOperationResourceAssignment is a mechanism to associate a resource with a ProcessOperationOccurrence.</rdfs:comment>
        <owl:versionInfo>3</owl:versionInfo>
        <skos:changeNote>[2023-10-04] Jean Brangé, AFNeT Services: Initial definition.</skos:changeNote>
        <skos:prefLabel xml:lang="en">process operation resource assignment</skos:prefLabel>
    </owl:Class>
    


    <!-- http://standards.iso.org/iso/10303/tech/refdata/core#69990b0c-8944-4601-8a54-d3b344628d08 -->

    <owl:Class rdf:about="http://standards.iso.org/iso/10303/tech/refdata/core#69990b0c-8944-4601-8a54-d3b344628d08">
        <rdfs:subClassOf rdf:resource="http://standards.iso.org/iso/10303/tech/refdata/core#a2719b60-dbf3-48e7-be31-ebb8c09491de"/>
        <dc:contributor>STEP Harmonization Team</dc:contributor>
        <dc:creator>Phil Spiby, Eurostep</dc:creator>
        <dc:date>2022-09-01</dc:date>
        <dc:source>ISO/TS 10303-4000</dc:source>
        <dc:type>InWork</dc:type>
        <rdfs:comment xml:lang="en">A DecreasingResourceEvent is a specialization of ResourceEvent that decreases the balance of a managed resource.</rdfs:comment>
        <owl:versionInfo>1</owl:versionInfo>
        <skos:changeNote>[2021-07-30] Initial definition.</skos:changeNote>
        <skos:example xml:lang="en">Filling a requisition reduces an inventory.</skos:example>
        <skos:prefLabel xml:lang="en">decreasing resource event</skos:prefLabel>
    </owl:Class>
    


    <!-- http://standards.iso.org/iso/10303/tech/refdata/core#7a449fab-fe68-4296-a567-4e02b6c32e19 -->

    <owl:Class rdf:about="http://standards.iso.org/iso/10303/tech/refdata/core#7a449fab-fe68-4296-a567-4e02b6c32e19">
        <rdfs:subClassOf rdf:resource="http://standards.iso.org/iso/10303/tech/refdata/core#d8381cb4-ef44-45bb-ba54-3476e2f5f45e"/>
        <dc:contributor>STEP Harmonization Team</dc:contributor>
        <dc:creator>Jean Brangé, AFNeT Services</dc:creator>
        <dc:date>2023-10-04</dc:date>
        <dc:source>ISO/TS 10303-4000</dc:source>
        <dc:type>InWork</dc:type>
        <rdfs:comment xml:lang="en">A PartTransportFeature is a type of PartFeature that is able to transport information, energy or matter within the PartView or ProductConfiguration.</rdfs:comment>
        <owl:versionInfo>3</owl:versionInfo>
        <skos:changeNote>[2023-10-04] Jean Brangé, AFNeT Services: Initial definition.</skos:changeNote>
        <skos:prefLabel xml:lang="en">part transport feature</skos:prefLabel>
    </owl:Class>
    


    <!-- http://standards.iso.org/iso/10303/tech/refdata/core#7c082e33-57b4-465b-aaad-04c8977d2353 -->

    <owl:Class rdf:about="http://standards.iso.org/iso/10303/tech/refdata/core#7c082e33-57b4-465b-aaad-04c8977d2353">
        <rdfs:subClassOf rdf:resource="http://standards.iso.org/iso/10303/tech/refdata/core#ff04d2c5-cea4-41a6-be35-821c1495d8ba"/>
        <dc:contributor>STEP Harmonization Team</dc:contributor>
        <dc:creator>Phil Spiby, Eurostep</dc:creator>
        <dc:date>2022-09-01</dc:date>
        <dc:source>ISO/TS 10303-4000</dc:source>
        <dc:type>InWork</dc:type>
        <rdfs:comment xml:lang="en">A ConcurrentElements is a specialization of StructuredTaskElement that comprises a set of actions to be performed during the time required for the longest task. No specific order is required.</rdfs:comment>
        <owl:versionInfo>2</owl:versionInfo>
        <skos:changeNote>[2021-07-30] Initial definition.</skos:changeNote>
        <skos:changeNote>[2022-09-01] Phil Spiby, Eurostep: updated comment.</skos:changeNote>
        <skos:prefLabel xml:lang="en">concurrent elements</skos:prefLabel>
    </owl:Class>
    


    <!-- http://standards.iso.org/iso/10303/tech/refdata/core#7c6a9a4b-dfd4-4412-9d67-ee16e3510837 -->

    <owl:Class rdf:about="http://standards.iso.org/iso/10303/tech/refdata/core#7c6a9a4b-dfd4-4412-9d67-ee16e3510837">
        <rdfs:subClassOf rdf:resource="http://standards.iso.org/iso/10303/tech/refdata/core#8bade30f-ae91-4520-a1bf-cfa1cca24bb7"/>
        <dc:contributor>STEP Harmonization Team</dc:contributor>
        <dc:creator>Jean Brangé, AFNeT Services</dc:creator>
        <dc:date>2023-10-04</dc:date>
        <dc:source>ISO/TS 10303-4000</dc:source>
        <dc:type>InWork</dc:type>
        <rdfs:comment xml:lang="en">A Nominal3dIntegralFeature is a type of Nominal3dFeature that represents a three-dimensional nominal integral feature.</rdfs:comment>
        <owl:versionInfo>3</owl:versionInfo>
        <skos:changeNote>[2023-10-04] Jean Brangé, AFNeT Services: Initial definition.</skos:changeNote>
        <skos:prefLabel xml:lang="en">nominal3d integral feature</skos:prefLabel>
    </owl:Class>
    


    <!-- http://standards.iso.org/iso/10303/tech/refdata/core#7d431f86-e10e-4802-b1cb-ad4eb05dcb21 -->

    <owl:Class rdf:about="http://standards.iso.org/iso/10303/tech/refdata/core#7d431f86-e10e-4802-b1cb-ad4eb05dcb21">
        <rdfs:subClassOf rdf:resource="http://standards.iso.org/iso/10303/tech/refdata/core#bc514af6-504d-408c-aa54-be5472451718"/>
        <dc:contributor>STEP Harmonization Team</dc:contributor>
        <dc:creator>Jean Brangé, AFNeT Services</dc:creator>
        <dc:date>2023-10-04</dc:date>
        <dc:source>ISO/TS 10303-4000</dc:source>
        <dc:type>InWork</dc:type>
        <rdfs:comment xml:lang="en">An OrientedToleranceZone is a type of ToleranceZoneWithDatum that represents an &quot;orientation plane&quot; for a geometric tolerance as defined in ISO 1101.</rdfs:comment>
        <owl:versionInfo>3</owl:versionInfo>
        <skos:changeNote>[2023-10-04] Jean Brangé, AFNeT Services: Initial definition.</skos:changeNote>
        <skos:prefLabel xml:lang="en">oriented tolerance zone</skos:prefLabel>
    </owl:Class>
    


    <!-- http://standards.iso.org/iso/10303/tech/refdata/core#7d6ab135-c2f0-4ca6-9ddf-636f74fad4a9 -->

    <owl:Class rdf:about="http://standards.iso.org/iso/10303/tech/refdata/core#7d6ab135-c2f0-4ca6-9ddf-636f74fad4a9">
        <rdfs:subClassOf rdf:resource="http://standards.iso.org/iso/10303/tech/refdata/core#c0c6c5e0-130a-0135-b552-598f1b1392ae"/>
        <dc:contributor>STEP Harmonization Team</dc:contributor>
        <dc:creator>Jean Brangé, AFNeT Services</dc:creator>
        <dc:date>2023-10-04</dc:date>
        <dc:source>ISO/TS 10303-4000</dc:source>
        <dc:type>InWork</dc:type>
        <rdfs:comment xml:lang="en">A WireColourBasedIdentificationCode is a type of PropertyDefinition that identifies a particular colour code that is used to identify WireOccurrences.</rdfs:comment>
        <owl:versionInfo>3</owl:versionInfo>
        <skos:changeNote>[2023-10-04] Jean Brangé, AFNeT Services: Initial definition.</skos:changeNote>
        <skos:prefLabel xml:lang="en">wire colour based identification code</skos:prefLabel>
    </owl:Class>
    


    <!-- http://standards.iso.org/iso/10303/tech/refdata/core#7d6c9961-1d1d-4e30-b80c-350b47942932 -->

    <owl:Class rdf:about="http://standards.iso.org/iso/10303/tech/refdata/core#7d6c9961-1d1d-4e30-b80c-350b47942932">
        <rdfs:subClassOf rdf:resource="http://standards.iso.org/iso/10303/tech/refdata/core#9fee6ad0-130a-0135-b552-598f1b1392ae"/>
        <dc:contributor>STEP Harmonization Team</dc:contributor>
        <dc:creator>Jean Brangé, AFNeT Services</dc:creator>
        <dc:date>2023-10-04</dc:date>
        <dc:source>ISO/TS 10303-4000</dc:source>
        <dc:type>InWork</dc:type>
        <rdfs:comment xml:lang="en">A Mechanism is a type of GeometricRepresentation that is a collection of KinematicLinks that are constraint by KinematicPairs.</rdfs:comment>
        <owl:versionInfo>3</owl:versionInfo>
        <skos:changeNote>[2023-10-04] Jean Brangé, AFNeT Services: Initial definition.</skos:changeNote>
        <skos:prefLabel xml:lang="en">mechanism</skos:prefLabel>
    </owl:Class>
    


    <!-- http://standards.iso.org/iso/10303/tech/refdata/core#7f164fdc-56d7-4adf-b7cd-1f93a9fa5a21 -->

    <owl:Class rdf:about="http://standards.iso.org/iso/10303/tech/refdata/core#7f164fdc-56d7-4adf-b7cd-1f93a9fa5a21">
        <rdfs:subClassOf rdf:resource="http://standards.iso.org/iso/10303/tech/refdata/core#32ba94ed-a4c9-4da4-b5e8-231b52733daf"/>
        <dc:contributor>STEP Harmonization Team</dc:contributor>
        <dc:creator>Jean Brangé, AFNeT Services</dc:creator>
        <dc:date>2023-10-04</dc:date>
        <dc:source>ISO/TS 10303-4000</dc:source>
        <dc:type>InWork</dc:type>
        <rdfs:comment xml:lang="en">A DatumSystemWithAssociatedModelCoordinateSystem is a type of Datum_system to represent the relation between a datum system and a model coordinate system as defined in ISO 16792. The model coordinate system is represented by an AxisPlacement that is referenced by the inherited attribute RepresentedGeometry.</rdfs:comment>
        <owl:versionInfo>3</owl:versionInfo>
        <skos:changeNote>[2023-10-04] Jean Brangé, AFNeT Services: Initial definition.</skos:changeNote>
        <skos:prefLabel xml:lang="en">datum system with associated model coordinate system</skos:prefLabel>
    </owl:Class>
    


    <!-- http://standards.iso.org/iso/10303/tech/refdata/core#7f1f1eca-9f6e-4642-9d9f-9f08858601f7 -->

    <owl:Class rdf:about="http://standards.iso.org/iso/10303/tech/refdata/core#7f1f1eca-9f6e-4642-9d9f-9f08858601f7">
        <rdfs:subClassOf rdf:resource="http://standards.iso.org/iso/10303/tech/refdata/core#5a6c8b1f-63af-4307-9faf-9fdd6da5572c"/>
        <dc:contributor>STEP Harmonization Team</dc:contributor>
        <dc:creator>Jean Brangé, AFNeT Services</dc:creator>
        <dc:date>2023-10-04</dc:date>
        <dc:source>ISO/TS 10303-4000</dc:source>
        <dc:type>InWork</dc:type>
        <rdfs:comment xml:lang="en">A Ply is a type of ConstituentPart that defines one of the layers of constant thickness material that make up a composite part. A Ply is a contiguous structure with a defined boundary that is made of one or more PlyPiece objects (see following figure). Ply.pngPly</rdfs:comment>
        <owl:versionInfo>3</owl:versionInfo>
        <skos:changeNote>[2023-10-04] Jean Brangé, AFNeT Services: Initial definition.</skos:changeNote>
        <skos:note xml:lang="en">A Ply may be a sheet pre-impregnated with resin material or a single-pass in a filament winding. Ply pieces that comprise a Ply must be of the same constant thickness material and fiber orientation (if fiber orientation is required). A Ply can also be the application of an isotropic material of constant thickness to an area. A Ply may not necessarily be a physical piece of material but an idealization of material in a zone that shares common fiber orientation and boundary.</skos:note>
        <skos:note xml:lang="en">The boundary of a Ply defines the edge of the material used to make the Ply, and includes an outer boundary and, if required, inner boundaries.</skos:note>
        <skos:prefLabel xml:lang="en">ply</skos:prefLabel>
    </owl:Class>
    


    <!-- http://standards.iso.org/iso/10303/tech/refdata/core#7f866c1a-ce53-4052-96f8-c74746255d9b -->

    <owl:Class rdf:about="http://standards.iso.org/iso/10303/tech/refdata/core#7f866c1a-ce53-4052-96f8-c74746255d9b">
        <rdfs:subClassOf rdf:resource="http://standards.iso.org/iso/10303/tech/refdata/core#19573db2-1baa-4bad-acc6-010eef852d49"/>
        <dc:contributor>STEP Harmonization Team</dc:contributor>
        <dc:creator>Phil Spiby, Eurostep</dc:creator>
        <dc:date>2022-09-01</dc:date>
        <dc:source>ISO/TS 10303-4000</dc:source>
        <dc:type>InWork</dc:type>
        <rdfs:comment xml:lang="en">A StatePredicted is a type of State. It represents an occurrence of the State of something in the future. Where a predicted state needs to be related to a StateObserved, the StatePredictedToObserved entity shall be used.</rdfs:comment>
        <owl:versionInfo>1</owl:versionInfo>
        <skos:changeNote>[2021-07-30] Initial definition.</skos:changeNote>
        <skos:example xml:lang="en">It is anticipated that the aircraft will land in an un-serviceable state. Hence a set of maintenance activities are started.</skos:example>
        <skos:prefLabel xml:lang="en">state predicted</skos:prefLabel>
    </owl:Class>
    


    <!-- http://standards.iso.org/iso/10303/tech/refdata/core#7feba0d9-6519-41e5-b855-95c35d7b641f -->

    <owl:Class rdf:about="http://standards.iso.org/iso/10303/tech/refdata/core#7feba0d9-6519-41e5-b855-95c35d7b641f">
        <rdfs:subClassOf rdf:resource="http://standards.iso.org/iso/10303/tech/refdata/core#59b11220-3279-0135-b58f-598f1b1392ae"/>
        <dc:contributor>STEP Harmonization Team</dc:contributor>
        <dc:creator>Jean Brangé, AFNeT Services</dc:creator>
        <dc:date>2023-10-04</dc:date>
        <dc:source>ISO/TS 10303-4000</dc:source>
        <dc:type>InWork</dc:type>
        <rdfs:comment xml:lang="en">A ProcessOperationOccurrenceRelationship is a relationship between two ProcessOperationOccurrence objects.</rdfs:comment>
        <owl:versionInfo>3</owl:versionInfo>
        <skos:changeNote>[2023-10-04] Jean Brangé, AFNeT Services: Initial definition.</skos:changeNote>
        <skos:prefLabel xml:lang="en">process operation occurrence relationship</skos:prefLabel>
    </owl:Class>
    


    <!-- http://standards.iso.org/iso/10303/tech/refdata/core#70fd2ab8-bdcb-481c-8096-ca0246ed15c5 -->

    <owl:Class rdf:about="http://standards.iso.org/iso/10303/tech/refdata/core#70fd2ab8-bdcb-481c-8096-ca0246ed15c5">
        <rdfs:subClassOf rdf:resource="http://standards.iso.org/iso/10303/tech/refdata/core#STEPThing"/>
        <dc:contributor>STEP Harmonization Team</dc:contributor>
        <dc:creator>Phil Spiby, Eurostep</dc:creator>
        <dc:date>2022-09-01</dc:date>
        <dc:source>ISO/TS 10303-4000</dc:source>
        <dc:type>InWork</dc:type>
        <rdfs:comment xml:lang="en">A SlotVersion is an identification of a version of a Slot.</rdfs:comment>
        <owl:versionInfo>1</owl:versionInfo>
        <skos:changeNote>[2022-09-01] Initial definition.</skos:changeNote>
        <skos:note xml:lang="en">This is a generic concept of version, in most situations it is possible and more specific to represent a version of a Slot as SlotDesign, SlotAsPlanned or SlotAsRealized.</skos:note>
        <skos:prefLabel xml:lang="en">slot version</skos:prefLabel>
    </owl:Class>
    


    <!-- http://standards.iso.org/iso/10303/tech/refdata/core#7011cec9-3484-4090-ad88-70a493229692 -->

    <owl:Class rdf:about="http://standards.iso.org/iso/10303/tech/refdata/core#7011cec9-3484-4090-ad88-70a493229692">
        <rdfs:subClassOf rdf:resource="http://standards.iso.org/iso/10303/tech/refdata/core#0cc8b831-37f7-4cd5-984f-dbb5588fbc1d"/>
        <dc:contributor>STEP Harmonization Team</dc:contributor>
        <dc:creator>Jean Brangé, AFNeT Services</dc:creator>
        <dc:date>2023-10-04</dc:date>
        <dc:source>ISO/TS 10303-4000</dc:source>
        <dc:type>InWork</dc:type>
        <rdfs:comment xml:lang="en">A PartConnectivityDefinition is a type of PartShapeElement that defines a connection between two or more PartTerminals or OccurrenceTerminals within an AssemblyDefinition but without stating the details how these terminals are connected with each other.</rdfs:comment>
        <owl:versionInfo>3</owl:versionInfo>
        <skos:changeNote>[2023-10-04] Jean Brangé, AFNeT Services: Initial definition.</skos:changeNote>
        <skos:prefLabel xml:lang="en">part connectivity definition</skos:prefLabel>
    </owl:Class>
    


    <!-- http://standards.iso.org/iso/10303/tech/refdata/core#72d69087-6dd9-401d-be56-cd178c03027e -->

    <owl:Class rdf:about="http://standards.iso.org/iso/10303/tech/refdata/core#72d69087-6dd9-401d-be56-cd178c03027e">
        <rdfs:subClassOf rdf:resource="http://standards.iso.org/iso/10303/tech/refdata/core#1f09cf40-e045-476a-b811-eb6e56de0ced"/>
        <dc:contributor>STEP Harmonization Team</dc:contributor>
        <dc:creator>Jean Brangé, AFNeT Services</dc:creator>
        <dc:date>2023-10-04</dc:date>
        <dc:source>ISO/TS 10303-4000</dc:source>
        <dc:type>InWork</dc:type>
        <rdfs:comment xml:lang="en">An AngularLocation is a type of DimensionalLocation. An AngularLocation specifies that a spatial constraint exists between two ShapeElements that intersect or would intersect if projected. An AngularLocation is a measure of the angle defined by the two ShapeElements and their common intersection or projected intersection. AngularLocation.gifAngularLocation</rdfs:comment>
        <owl:versionInfo>3</owl:versionInfo>
        <skos:changeNote>[2023-10-04] Jean Brangé, AFNeT Services: Initial definition.</skos:changeNote>
        <skos:note xml:lang="en">The application and use of an AngularLocation is illustrated in the Figure AngularLocation. The Figure AngularLocation also illustrates types of intersection (a and b) and virtual intersection (c and d).</skos:note>
        <skos:prefLabel xml:lang="en">angular location</skos:prefLabel>
    </owl:Class>
    


    <!-- http://standards.iso.org/iso/10303/tech/refdata/core#73ca1764-db10-4d1f-a975-80514004effa -->

    <owl:Class rdf:about="http://standards.iso.org/iso/10303/tech/refdata/core#73ca1764-db10-4d1f-a975-80514004effa">
        <rdfs:subClassOf rdf:resource="http://standards.iso.org/iso/10303/tech/refdata/core#89f36b81-3d5e-48dd-90fc-80eaf4d96f3e"/>
        <dc:contributor>STEP Harmonization Team</dc:contributor>
        <dc:creator>Phil Spiby, Eurostep</dc:creator>
        <dc:date>2022-09-01</dc:date>
        <dc:source>ISO/TS 10303-4000</dc:source>
        <dc:type>InWork</dc:type>
        <rdfs:comment xml:lang="en">An ExternalAnalysisModel is a specialization of AnalysisModel whose content is provided in an external file.</rdfs:comment>
        <owl:versionInfo>1</owl:versionInfo>
        <skos:changeNote>[2021-07-30] Initial definition.</skos:changeNote>
        <skos:prefLabel xml:lang="en">external analysis model</skos:prefLabel>
    </owl:Class>
    


    <!-- http://standards.iso.org/iso/10303/tech/refdata/core#7411c7df-b5ef-4fbe-83a9-00d124cbf35d -->

    <owl:Class rdf:about="http://standards.iso.org/iso/10303/tech/refdata/core#7411c7df-b5ef-4fbe-83a9-00d124cbf35d">
        <rdfs:subClassOf rdf:resource="http://standards.iso.org/iso/10303/tech/refdata/core#9c98fe40-130a-0135-b552-598f1b1392ae"/>
        <dc:contributor>STEP Harmonization Team</dc:contributor>
        <dc:creator>Jean Brangé, AFNeT Services</dc:creator>
        <dc:date>2023-10-04</dc:date>
        <dc:source>ISO/TS 10303-4000</dc:source>
        <dc:type>InWork</dc:type>
        <rdfs:comment xml:lang="en">An ExternalEdgeBasedWireframeShapeRepresentation is a type of ExternalGeometricModel that references an instance of type ../../../resources/aic_edge_based_wireframe/aic_edge_based_wireframe.htm#aic_edge_based_wireframe.edge_based_wireframe_shape_representation edge_based_wireframe_shape_representation (ISO 10303-501).</rdfs:comment>
        <owl:versionInfo>3</owl:versionInfo>
        <skos:changeNote>[2023-10-04] Jean Brangé, AFNeT Services: Initial definition.</skos:changeNote>
        <skos:prefLabel xml:lang="en">external edge based wireframe shape representation</skos:prefLabel>
    </owl:Class>
    


    <!-- http://standards.iso.org/iso/10303/tech/refdata/core#752c1b0f-9844-45da-8a47-dbe39ed4c193 -->

    <owl:Class rdf:about="http://standards.iso.org/iso/10303/tech/refdata/core#752c1b0f-9844-45da-8a47-dbe39ed4c193">
        <rdfs:subClassOf rdf:resource="http://standards.iso.org/iso/10303/tech/refdata/core#d1796b3a-5ade-4d7a-b9e0-4af28a9cfddb"/>
        <dc:contributor>STEP Harmonization Team</dc:contributor>
        <dc:creator>Jean Brangé, AFNeT Services</dc:creator>
        <dc:date>2023-10-04</dc:date>
        <dc:source>ISO/TS 10303-4000</dc:source>
        <dc:type>InWork</dc:type>
        <rdfs:comment xml:lang="en">An AssemblyShapeConstraintItemRelationship is a type of ShapeElementRelationship that relates an OccurrenceShapeFeature into an AssemblyShapeConstraint.</rdfs:comment>
        <owl:versionInfo>3</owl:versionInfo>
        <skos:changeNote>[2023-10-04] Jean Brangé, AFNeT Services: Initial definition.</skos:changeNote>
        <skos:prefLabel xml:lang="en">assembly shape constraint item relationship</skos:prefLabel>
    </owl:Class>
    


    <!-- http://standards.iso.org/iso/10303/tech/refdata/core#756b7320-fa8b-4bb7-83d2-2d6a4e31675d -->

    <owl:Class rdf:about="http://standards.iso.org/iso/10303/tech/refdata/core#756b7320-fa8b-4bb7-83d2-2d6a4e31675d">
        <rdfs:subClassOf rdf:resource="http://standards.iso.org/iso/10303/tech/refdata/core#d1796b3a-5ade-4d7a-b9e0-4af28a9cfddb"/>
        <dc:contributor>STEP Harmonization Team</dc:contributor>
        <dc:creator>Jean Brangé, AFNeT Services</dc:creator>
        <dc:date>2023-10-04</dc:date>
        <dc:source>ISO/TS 10303-4000</dc:source>
        <dc:type>InWork</dc:type>
        <rdfs:comment xml:lang="en">A ShapeFeatureDefinitionElementRelationship is a type of ShapeElementRelationship that relates two ShapeFeatureDefinitionElements.</rdfs:comment>
        <owl:versionInfo>3</owl:versionInfo>
        <skos:changeNote>[2023-10-04] Jean Brangé, AFNeT Services: Initial definition.</skos:changeNote>
        <skos:prefLabel xml:lang="en">shape feature definition element relationship</skos:prefLabel>
    </owl:Class>
    


    <!-- http://standards.iso.org/iso/10303/tech/refdata/core#76641a10-826c-4e2b-a8ff-241402c358ab -->

    <owl:Class rdf:about="http://standards.iso.org/iso/10303/tech/refdata/core#76641a10-826c-4e2b-a8ff-241402c358ab">
        <rdfs:subClassOf rdf:resource="http://standards.iso.org/iso/10303/tech/refdata/core#STEPThing"/>
        <dc:contributor>STEP Harmonization Team</dc:contributor>
        <dc:creator>Phil Spiby, Eurostep</dc:creator>
        <dc:date>2022-09-01</dc:date>
        <dc:source>ISO/TS 10303-4000</dc:source>
        <dc:type>InWork</dc:type>
        <rdfs:comment xml:lang="en">An AnalysisDisciplineDefinition is a definition or view of an AnalysisVersion taken from the perspective of the analysing organization. The AnalysisDisciplineDefinition is controlled by the analysing organization. The entity can be used to capture the definition of a specific version of an Analysis at any intermediate stage of its development where the definition is not formally released by an organization at the Analysis version level. It can be used to capture the various stages in the definition cycle of a product. If the Analysis is explicitly represented by a model, then the model is referenced using the DefinitionalRepresentations attribute.</rdfs:comment>
        <owl:versionInfo>2</owl:versionInfo>
        <skos:changeNote>[2021-07-30] Initial definition.</skos:changeNote>
        <skos:changeNote>[2022-09-01] Phil Spiby, Eurostep: updated comment.</skos:changeNote>
        <skos:prefLabel xml:lang="en">analysis discipline definition</skos:prefLabel>
    </owl:Class>
    


    <!-- http://standards.iso.org/iso/10303/tech/refdata/core#7694a1ca-c9c5-4609-901b-0d8ff06ba698 -->

    <owl:Class rdf:about="http://standards.iso.org/iso/10303/tech/refdata/core#7694a1ca-c9c5-4609-901b-0d8ff06ba698">
        <rdfs:subClassOf rdf:resource="http://standards.iso.org/iso/10303/tech/refdata/core#5a6c8b1f-63af-4307-9faf-9fdd6da5572c"/>
        <dc:contributor>STEP Harmonization Team</dc:contributor>
        <dc:creator>Jean Brangé, AFNeT Services</dc:creator>
        <dc:date>2023-10-04</dc:date>
        <dc:source>ISO/TS 10303-4000</dc:source>
        <dc:type>InWork</dc:type>
        <rdfs:comment xml:lang="en">A PlyLaminateSequenceDefinition is a type of ConstituentPart that is an illustration of a single unique sequence or layer within a PlyLaminate. The sequence or layer contains one or more plies.</rdfs:comment>
        <owl:versionInfo>3</owl:versionInfo>
        <skos:changeNote>[2023-10-04] Jean Brangé, AFNeT Services: Initial definition.</skos:changeNote>
        <skos:note xml:lang="en">When more than one ply resides in the same sequence or layer, the plies must not overlap. If plies do overlap, they must be put on separate sequence or layers.</skos:note>
        <skos:prefLabel xml:lang="en">ply laminate sequence definition</skos:prefLabel>
    </owl:Class>
    


    <!-- http://standards.iso.org/iso/10303/tech/refdata/core#774c2a30-5bf8-4163-9050-b50a2556985b -->

    <owl:Class rdf:about="http://standards.iso.org/iso/10303/tech/refdata/core#774c2a30-5bf8-4163-9050-b50a2556985b">
        <rdfs:subClassOf rdf:resource="http://standards.iso.org/iso/10303/tech/refdata/core#d1796b3a-5ade-4d7a-b9e0-4af28a9cfddb"/>
        <dc:contributor>STEP Harmonization Team</dc:contributor>
        <dc:creator>Jean Brangé, AFNeT Services</dc:creator>
        <dc:date>2023-10-04</dc:date>
        <dc:source>ISO/TS 10303-4000</dc:source>
        <dc:type>InWork</dc:type>
        <rdfs:comment xml:lang="en">An AssemblyShapeJointItemRelationship is a type of ShapeElementRelationship that relates an OccurrenceShapeFeature into an AssemblyShapeJoint.</rdfs:comment>
        <owl:versionInfo>3</owl:versionInfo>
        <skos:changeNote>[2023-10-04] Jean Brangé, AFNeT Services: Initial definition.</skos:changeNote>
        <skos:prefLabel xml:lang="en">assembly shape joint item relationship</skos:prefLabel>
    </owl:Class>
    


    <!-- http://standards.iso.org/iso/10303/tech/refdata/core#78133794-f9d2-4e22-aaa0-49690cc93a39 -->

    <owl:Class rdf:about="http://standards.iso.org/iso/10303/tech/refdata/core#78133794-f9d2-4e22-aaa0-49690cc93a39">
        <rdfs:subClassOf rdf:resource="http://standards.iso.org/iso/10303/tech/refdata/core#c54bc6fa-f6d8-4943-85de-6439071c5325"/>
        <dc:contributor>STEP Harmonization Team</dc:contributor>
        <dc:creator>Jean Brangé, AFNeT Services</dc:creator>
        <dc:date>2023-10-04</dc:date>
        <dc:source>ISO/TS 10303-4000</dc:source>
        <dc:type>InWork</dc:type>
        <rdfs:comment xml:lang="en">A CrossSectionalGroupShapeElement is a type of CrossSectionalPartShapeElement that defines a hierarchical grouping of other CrossSectionalPartShapeElement or CrossSectionalOccurrenceShapeElement.</rdfs:comment>
        <owl:versionInfo>3</owl:versionInfo>
        <skos:changeNote>[2023-10-04] Jean Brangé, AFNeT Services: Initial definition.</skos:changeNote>
        <skos:prefLabel xml:lang="en">cross sectional group shape element</skos:prefLabel>
    </owl:Class>
    


    <!-- http://standards.iso.org/iso/10303/tech/refdata/core#785d10cc-a385-42d8-b649-4fe2bf56b73c -->

    <owl:Class rdf:about="http://standards.iso.org/iso/10303/tech/refdata/core#785d10cc-a385-42d8-b649-4fe2bf56b73c">
        <rdfs:subClassOf rdf:resource="http://standards.iso.org/iso/10303/tech/refdata/core#f8816baf-d66a-42f9-bdcc-38e946c9a2fa"/>
        <dc:contributor>STEP Harmonization Team</dc:contributor>
        <dc:creator>Jean Brangé, AFNeT Services</dc:creator>
        <dc:date>2023-10-04</dc:date>
        <dc:source>ISO/TS 10303-4000</dc:source>
        <dc:type>InWork</dc:type>
        <rdfs:comment xml:lang="en">An Apex is a type of DerivedShapeElement that defines the point corresponding to the common apex (the location where a plane and conical element intersect at a single point) of one or more conical ShapeElements. The common intersection of three or more planes or two curves shall be treated as a GeometricIntersection rather than as an Apex.</rdfs:comment>
        <owl:versionInfo>3</owl:versionInfo>
        <skos:changeNote>[2023-10-04] Jean Brangé, AFNeT Services: Initial definition.</skos:changeNote>
        <skos:prefLabel xml:lang="en">apex</skos:prefLabel>
    </owl:Class>
    


    <!-- http://standards.iso.org/iso/10303/tech/refdata/core#7861dd43-6cc5-4491-9d04-b14d256c3e90 -->

    <owl:Class rdf:about="http://standards.iso.org/iso/10303/tech/refdata/core#7861dd43-6cc5-4491-9d04-b14d256c3e90">
        <rdfs:subClassOf rdf:resource="http://standards.iso.org/iso/10303/tech/refdata/core#95f1bde5-b263-4ca1-89df-33e1205800dd"/>
        <dc:contributor>STEP Harmonization Team</dc:contributor>
        <dc:creator>Phil Spiby, Eurostep</dc:creator>
        <dc:date>2022-09-01</dc:date>
        <dc:source>ISO/TS 10303-4000</dc:source>
        <dc:type>InWork</dc:type>
        <rdfs:comment xml:lang="en">A StartTask is a type of TaskElement. It signifies the start point of the task.</rdfs:comment>
        <owl:versionInfo>1</owl:versionInfo>
        <skos:changeNote>[2021-07-30] Initial definition.</skos:changeNote>
        <skos:note xml:lang="en">Not all formal task description require start and end elements, their inclusion is in a sequence is optional.</skos:note>
        <skos:prefLabel xml:lang="en">start task</skos:prefLabel>
    </owl:Class>
    


    <!-- http://standards.iso.org/iso/10303/tech/refdata/core#794abe2f-e0ab-4952-b5db-ba38b54f9035 -->

    <owl:Class rdf:about="http://standards.iso.org/iso/10303/tech/refdata/core#794abe2f-e0ab-4952-b5db-ba38b54f9035">
        <rdfs:subClassOf rdf:resource="http://standards.iso.org/iso/10303/tech/refdata/core#1d59c650-3279-0135-b58f-598f1b1392ae"/>
        <dc:contributor>STEP Harmonization Team</dc:contributor>
        <dc:creator>Jean Brangé, AFNeT Services</dc:creator>
        <dc:date>2023-10-04</dc:date>
        <dc:source>ISO/TS 10303-4000</dc:source>
        <dc:type>InWork</dc:type>
        <rdfs:comment xml:lang="en">An AnnotatedModelItemAssociation is an identification of a Callout within an AnnotatedModelPresentation as being the element that describes a GeometricDimension, GeometricTolerance, ShapeFeatureDefinition, ShapeElement or a ShapeElementRelationship.</rdfs:comment>
        <owl:versionInfo>3</owl:versionInfo>
        <skos:changeNote>[2023-10-04] Jean Brangé, AFNeT Services: Initial definition.</skos:changeNote>
        <skos:example xml:lang="en">In an application protocol, an instance of GeometricModel describes a characteristic of a product. One element of the GeometricModel - a Curve - represents the boundary of a hole that is a ShapeElement in the product. This entity data type may be used to state that the curve describes the hole, in the context of the entire GeometricModel describing the shape of the product.</skos:example>
        <skos:prefLabel xml:lang="en">annotated model item association</skos:prefLabel>
    </owl:Class>
    


    <!-- http://standards.iso.org/iso/10303/tech/refdata/core#794abe5a-7e64-4202-98df-17ee5c792702 -->

    <owl:Class rdf:about="http://standards.iso.org/iso/10303/tech/refdata/core#794abe5a-7e64-4202-98df-17ee5c792702">
        <rdfs:subClassOf rdf:resource="http://standards.iso.org/iso/10303/tech/refdata/core#68242b94-82e8-4841-8005-89981113e22f"/>
        <dc:contributor>STEP Harmonization Team</dc:contributor>
        <dc:creator>Phil Spiby, Eurostep</dc:creator>
        <dc:date>2022-09-01</dc:date>
        <dc:source>ISO/TS 10303-4000</dc:source>
        <dc:type>InWork</dc:type>
        <rdfs:comment xml:lang="en">A ProductBasedLocator is a type of Locator specified through a product-related referential.</rdfs:comment>
        <owl:versionInfo>1</owl:versionInfo>
        <skos:changeNote>[2021-07-30] Initial definition.</skos:changeNote>
        <skos:example xml:lang="en">The frame numbering inside an aircraft.</skos:example>
        <skos:prefLabel xml:lang="en">product based locator</skos:prefLabel>
    </owl:Class>
    


    <!-- http://standards.iso.org/iso/10303/tech/refdata/core#8a16e65d-935f-4bc6-b068-60ba220fdcc7 -->

    <owl:Class rdf:about="http://standards.iso.org/iso/10303/tech/refdata/core#8a16e65d-935f-4bc6-b068-60ba220fdcc7">
        <rdfs:subClassOf rdf:resource="http://standards.iso.org/iso/10303/tech/refdata/core#09cd1ad9-ed18-4c44-a399-eb27b8148d42"/>
        <dc:contributor>STEP Harmonization Team</dc:contributor>
        <dc:creator>Jean Brangé, AFNeT Services</dc:creator>
        <dc:date>2023-10-04</dc:date>
        <dc:source>ISO/TS 10303-4000</dc:source>
        <dc:type>InWork</dc:type>
        <rdfs:comment xml:lang="en">A WireOccurrenceTerminal is a type of OccurrenceTerminal for the identification of a terminal on a WireOccurrence. The terminal may be located at one of the ends or somewhere in the middle of the wire. The WireOccurrenceTerminals at the ends of the wire shall be named &quot;end a&quot; and &quot;end b&quot; respectively. WireOccurrenceTerminals in the middle of the wire shall start with the letters &quot;intermediate&quot; followed by arbitrary text.</rdfs:comment>
        <owl:versionInfo>3</owl:versionInfo>
        <skos:changeNote>[2023-10-04] Jean Brangé, AFNeT Services: Initial definition.</skos:changeNote>
        <skos:prefLabel xml:lang="en">wire occurrence terminal</skos:prefLabel>
    </owl:Class>
    


    <!-- http://standards.iso.org/iso/10303/tech/refdata/core#8a3cd410-130a-0135-b552-598f1b1392ae -->

    <owl:Class rdf:about="http://standards.iso.org/iso/10303/tech/refdata/core#8a3cd410-130a-0135-b552-598f1b1392ae">
        <rdfs:subClassOf rdf:resource="http://standards.iso.org/iso/10303/tech/refdata/core#59b11220-3279-0135-b58f-598f1b1392ae"/>
        <dc:contributor>STEP Harmonization Team</dc:contributor>
        <dc:creator>Phil Spiby, Eurostep</dc:creator>
        <dc:date>2022-09-01</dc:date>
        <dc:source>ISO/TS 10303-4000</dc:source>
        <dc:type>InWork</dc:type>
        <rdfs:comment xml:lang="en">A BreakdownElementRelationship is a relationship between two BreakdownElement objects.</rdfs:comment>
        <owl:versionInfo>2</owl:versionInfo>
        <skos:changeNote>[2021-07-30] Initial definition.</skos:changeNote>
        <skos:changeNote>[2022-09-01] Phil Spiby, Eurostep: updated comment.</skos:changeNote>
        <skos:prefLabel xml:lang="en">breakdown element relationship</skos:prefLabel>
    </owl:Class>
    


    <!-- http://standards.iso.org/iso/10303/tech/refdata/core#8a785670-130a-0135-b552-598f1b1392ae -->

    <owl:Class rdf:about="http://standards.iso.org/iso/10303/tech/refdata/core#8a785670-130a-0135-b552-598f1b1392ae">
        <rdfs:subClassOf rdf:resource="http://standards.iso.org/iso/10303/tech/refdata/core#STEPThing"/>
        <dc:contributor>STEP Harmonization Team</dc:contributor>
        <dc:creator>Phil Spiby, Eurostep</dc:creator>
        <dc:date>2022-09-01</dc:date>
        <dc:source>ISO/TS 10303-4000</dc:source>
        <dc:type>InWork</dc:type>
        <rdfs:comment xml:lang="en">A BreakdownElementVersion is a revision of a BreakdownElement. It is a collector of the views of this revision of the BreakdownElement.</rdfs:comment>
        <owl:versionInfo>1</owl:versionInfo>
        <skos:changeNote>[2021-07-30] Initial definition.</skos:changeNote>
        <skos:note xml:lang="en">The set of all instances of BreakdownElementVersion of the same BreakdownElement represents the history of the BreakdownElement.</skos:note>
        <skos:prefLabel xml:lang="en">breakdown element version</skos:prefLabel>
    </owl:Class>
    


    <!-- http://standards.iso.org/iso/10303/tech/refdata/core#8ad25d50-130a-0135-b552-598f1b1392ae -->

    <owl:Class rdf:about="http://standards.iso.org/iso/10303/tech/refdata/core#8ad25d50-130a-0135-b552-598f1b1392ae">
        <rdfs:subClassOf rdf:resource="http://standards.iso.org/iso/10303/tech/refdata/core#59b11220-3279-0135-b58f-598f1b1392ae"/>
        <dc:contributor>STEP Harmonization Team</dc:contributor>
        <dc:creator>Phil Spiby, Eurostep</dc:creator>
        <dc:date>2022-09-01</dc:date>
        <dc:source>ISO/TS 10303-4000</dc:source>
        <dc:type>InWork</dc:type>
        <rdfs:comment xml:lang="en">A BreakdownElementVersionRelationship is a relationship between two BreakdownElementVersion objects.</rdfs:comment>
        <owl:versionInfo>2</owl:versionInfo>
        <skos:changeNote>[2021-07-30] Initial definition.</skos:changeNote>
        <skos:changeNote>[2022-09-01] Phil Spiby, Eurostep: updated comment updated note.</skos:changeNote>
        <skos:note xml:lang="en">Such a relationship can exist between two BreakdownElementVersion instances of the same BreakdownElement instance or of different BreakdownElement instances.</skos:note>
        <skos:prefLabel xml:lang="en">breakdown element version relationship</skos:prefLabel>
    </owl:Class>
    


    <!-- http://standards.iso.org/iso/10303/tech/refdata/core#8aec96ba-d0b5-42d6-8717-ed07b11ba244 -->

    <owl:Class rdf:about="http://standards.iso.org/iso/10303/tech/refdata/core#8aec96ba-d0b5-42d6-8717-ed07b11ba244">
        <rdfs:subClassOf rdf:resource="http://standards.iso.org/iso/10303/tech/refdata/core#c0c6c5e0-130a-0135-b552-598f1b1392ae"/>
        <dc:contributor>STEP Harmonization Team</dc:contributor>
        <dc:creator>Jean Brangé, AFNeT Services</dc:creator>
        <dc:date>2023-10-04</dc:date>
        <dc:source>ISO/TS 10303-4000</dc:source>
        <dc:type>InWork</dc:type>
        <rdfs:comment xml:lang="en">A MaterialPropertyDefinition is a type of PropertyDefinition that is a characteristic that depends on material aspects. It is the definition of a MaterialPropertyValue.</rdfs:comment>
        <owl:versionInfo>3</owl:versionInfo>
        <skos:changeNote>[2023-10-04] Jean Brangé, AFNeT Services: Initial definition.</skos:changeNote>
        <skos:prefLabel xml:lang="en">material property definition</skos:prefLabel>
    </owl:Class>
    


    <!-- http://standards.iso.org/iso/10303/tech/refdata/core#8b21b5d0-130a-0135-b552-598f1b1392ae -->

    <owl:Class rdf:about="http://standards.iso.org/iso/10303/tech/refdata/core#8b21b5d0-130a-0135-b552-598f1b1392ae">
        <rdfs:subClassOf rdf:resource="http://standards.iso.org/iso/10303/tech/refdata/core#STEPThing"/>
        <dc:contributor>STEP Harmonization Team</dc:contributor>
        <dc:creator>Phil Spiby, Eurostep</dc:creator>
        <dc:date>2022-09-01</dc:date>
        <dc:source>ISO/TS 10303-4000</dc:source>
        <dc:type>InWork</dc:type>
        <rdfs:comment xml:lang="en">A BreakdownElementView is a characterization of a BreakdownElementVersion in one or more application domains and for one or more life-cycle stages. A BreakdownElementView is a collector of the properties that characterize the BreakdownElementVersion in the InitialContext and the AdditionalContexts.</rdfs:comment>
        <owl:versionInfo>2</owl:versionInfo>
        <skos:changeNote>[2021-07-30] Initial definition.</skos:changeNote>
        <skos:changeNote>[2022-09-01] Phil Spiby, Eurostep: updated comment.</skos:changeNote>
        <skos:example xml:lang="en">The design function of a pump and its as-built function can be represented by two objects of BreakdownElementView.</skos:example>
        <skos:prefLabel xml:lang="en">breakdown element view</skos:prefLabel>
    </owl:Class>
    


    <!-- http://standards.iso.org/iso/10303/tech/refdata/core#8b2a7f00-5e0e-4e83-af9d-53c8cfc2aaaa -->

    <owl:Class rdf:about="http://standards.iso.org/iso/10303/tech/refdata/core#8b2a7f00-5e0e-4e83-af9d-53c8cfc2aaaa">
        <rdfs:subClassOf rdf:resource="http://standards.iso.org/iso/10303/tech/refdata/core#STEPThing"/>
        <dc:contributor>STEP Harmonization Team</dc:contributor>
        <dc:creator>Phil Spiby, Eurostep</dc:creator>
        <dc:date>2022-09-01</dc:date>
        <dc:source>ISO/TS 10303-4000</dc:source>
        <dc:type>InWork</dc:type>
        <rdfs:comment xml:lang="en">A SystemVersion represents a particular version of a system.</rdfs:comment>
        <owl:versionInfo>1</owl:versionInfo>
        <skos:changeNote>[2022-09-01] Initial definition.</skos:changeNote>
        <skos:example xml:lang="en">A fuel injection system can have a system design version v1 and a system design version v1.1.</skos:example>
        <skos:note xml:lang="en">In this case, this means &quot;revision&quot;. A given system can have several versions of system design.</skos:note>
        <skos:prefLabel xml:lang="en">system version</skos:prefLabel>
    </owl:Class>
    


    <!-- http://standards.iso.org/iso/10303/tech/refdata/core#8b5ba2e8-9590-4ef0-be41-93e469bea12d -->

    <owl:Class rdf:about="http://standards.iso.org/iso/10303/tech/refdata/core#8b5ba2e8-9590-4ef0-be41-93e469bea12d">
        <rdfs:subClassOf rdf:resource="http://standards.iso.org/iso/10303/tech/refdata/core#90864677-a5ac-4f4c-b261-a0347fc3a4cb"/>
        <dc:contributor>STEP Harmonization Team</dc:contributor>
        <dc:creator>Jean Brangé, AFNeT Services</dc:creator>
        <dc:date>2023-10-04</dc:date>
        <dc:source>ISO/TS 10303-4000</dc:source>
        <dc:type>InWork</dc:type>
        <rdfs:comment xml:lang="en">A DirectedOrOrientedToleranceZone is a type of ToleranceZone that includes additional direction or orientation information for the tolerance zone. A DirectedOrOrientedToleranceZone shall be either a ToleranceZoneWithDatum or an AffectedPlaneToleranceZone.</rdfs:comment>
        <owl:versionInfo>3</owl:versionInfo>
        <skos:changeNote>[2023-10-04] Jean Brangé, AFNeT Services: Initial definition.</skos:changeNote>
        <skos:prefLabel xml:lang="en">directed or oriented tolerance zone</skos:prefLabel>
    </owl:Class>
    


    <!-- http://standards.iso.org/iso/10303/tech/refdata/core#8b77b756-73b0-48d2-a17f-0927512f489c -->

    <owl:Class rdf:about="http://standards.iso.org/iso/10303/tech/refdata/core#8b77b756-73b0-48d2-a17f-0927512f489c">
        <rdfs:subClassOf rdf:resource="http://standards.iso.org/iso/10303/tech/refdata/core#59b11220-3279-0135-b58f-598f1b1392ae"/>
        <dc:contributor>STEP Harmonization Team</dc:contributor>
        <dc:creator>Phil Spiby, Eurostep</dc:creator>
        <dc:date>2022-09-01</dc:date>
        <dc:source>ISO/TS 10303-4000</dc:source>
        <dc:type>InWork</dc:type>
        <rdfs:comment xml:lang="en">A SystemVersionRelationship is a relationship between two SystemVersion objects. Unless specified in a specialization of this object, this relationship does not involve inheritance of data between the two related objects.</rdfs:comment>
        <owl:versionInfo>1</owl:versionInfo>
        <skos:changeNote>[2022-09-01] Initial definition.</skos:changeNote>
        <skos:prefLabel xml:lang="en">system version relationship</skos:prefLabel>
    </owl:Class>
    


    <!-- http://standards.iso.org/iso/10303/tech/refdata/core#8b8e0c30-130a-0135-b552-598f1b1392ae -->

    <owl:Class rdf:about="http://standards.iso.org/iso/10303/tech/refdata/core#8b8e0c30-130a-0135-b552-598f1b1392ae">
        <rdfs:subClassOf rdf:resource="http://standards.iso.org/iso/10303/tech/refdata/core#59b11220-3279-0135-b58f-598f1b1392ae"/>
        <dc:contributor>STEP Harmonization Team</dc:contributor>
        <dc:creator>Phil Spiby, Eurostep</dc:creator>
        <dc:date>2022-09-01</dc:date>
        <dc:source>ISO/TS 10303-4000</dc:source>
        <dc:type>InWork</dc:type>
        <rdfs:comment xml:lang="en">A BreakdownElementViewRelationship is a relationship between two BreakdownElementView objects.</rdfs:comment>
        <owl:versionInfo>2</owl:versionInfo>
        <skos:changeNote>[2021-07-30] Initial definition.</skos:changeNote>
        <skos:changeNote>[2022-09-01] Phil Spiby, Eurostep: updated comment updated note.</skos:changeNote>
        <skos:note xml:lang="en">Such a relationship can exist between two BreakdownElementView instances of the same BreakdownElementVersion instance or of different BreakdownElementVersion instances.</skos:note>
        <skos:prefLabel xml:lang="en">breakdown element view relationship</skos:prefLabel>
    </owl:Class>
    


    <!-- http://standards.iso.org/iso/10303/tech/refdata/core#8bade30f-ae91-4520-a1bf-cfa1cca24bb7 -->

    <owl:Class rdf:about="http://standards.iso.org/iso/10303/tech/refdata/core#8bade30f-ae91-4520-a1bf-cfa1cca24bb7">
        <rdfs:subClassOf rdf:resource="http://standards.iso.org/iso/10303/tech/refdata/core#0cc8b831-37f7-4cd5-984f-dbb5588fbc1d"/>
        <dc:contributor>STEP Harmonization Team</dc:contributor>
        <dc:creator>Jean Brangé, AFNeT Services</dc:creator>
        <dc:date>2023-10-04</dc:date>
        <dc:source>ISO/TS 10303-4000</dc:source>
        <dc:type>InWork</dc:type>
        <rdfs:comment xml:lang="en">A Nominal3dFeature is a type of PartShapeElement that represents a three-dimensional nominal feature. Each Nominal3dFeature is either a Nominal3dIntegralFeature or a Nominal3dDerivedFeature.</rdfs:comment>
        <owl:versionInfo>3</owl:versionInfo>
        <skos:changeNote>[2023-10-04] Jean Brangé, AFNeT Services: Initial definition.</skos:changeNote>
        <skos:prefLabel xml:lang="en">nominal3d feature</skos:prefLabel>
    </owl:Class>
    


    <!-- http://standards.iso.org/iso/10303/tech/refdata/core#8be071f0-130a-0135-b552-598f1b1392ae -->

    <owl:Class rdf:about="http://standards.iso.org/iso/10303/tech/refdata/core#8be071f0-130a-0135-b552-598f1b1392ae">
        <rdfs:subClassOf rdf:resource="http://standards.iso.org/iso/10303/tech/refdata/core#59b11220-3279-0135-b58f-598f1b1392ae"/>
        <dc:contributor>STEP Harmonization Team</dc:contributor>
        <dc:creator>Phil Spiby, Eurostep</dc:creator>
        <dc:date>2022-09-01</dc:date>
        <dc:source>ISO/TS 10303-4000</dc:source>
        <dc:type>InWork</dc:type>
        <rdfs:comment xml:lang="en">A BreakdownRelationship is a relationship between two Breakdown objects.</rdfs:comment>
        <owl:versionInfo>2</owl:versionInfo>
        <skos:changeNote>[2021-07-30] Initial definition.</skos:changeNote>
        <skos:changeNote>[2022-09-01] Phil Spiby, Eurostep: updated comment.</skos:changeNote>
        <skos:prefLabel xml:lang="en">breakdown relationship</skos:prefLabel>
    </owl:Class>
    


    <!-- http://standards.iso.org/iso/10303/tech/refdata/core#8c15d9d0-130a-0135-b552-598f1b1392ae -->

    <owl:Class rdf:about="http://standards.iso.org/iso/10303/tech/refdata/core#8c15d9d0-130a-0135-b552-598f1b1392ae">
        <rdfs:subClassOf rdf:resource="http://standards.iso.org/iso/10303/tech/refdata/core#STEPThing"/>
        <dc:contributor>STEP Harmonization Team</dc:contributor>
        <dc:creator>Phil Spiby, Eurostep</dc:creator>
        <dc:date>2022-09-01</dc:date>
        <dc:source>ISO/TS 10303-4000</dc:source>
        <dc:type>InWork</dc:type>
        <rdfs:comment xml:lang="en">A BreakdownVersion is a revision of a Breakdown.</rdfs:comment>
        <owl:versionInfo>1</owl:versionInfo>
        <skos:changeNote>[2021-07-30] Initial definition.</skos:changeNote>
        <skos:note xml:lang="en">The set of all instances of BreakdownVersion of the same Breakdown represents the history of the Breakdown.</skos:note>
        <skos:prefLabel xml:lang="en">breakdown version</skos:prefLabel>
    </owl:Class>
    


    <!-- http://standards.iso.org/iso/10303/tech/refdata/core#8c284ede-a307-4818-8ef9-3c85376c3ee8 -->

    <owl:Class rdf:about="http://standards.iso.org/iso/10303/tech/refdata/core#8c284ede-a307-4818-8ef9-3c85376c3ee8">
        <rdfs:subClassOf rdf:resource="http://standards.iso.org/iso/10303/tech/refdata/core#29dc8412-b2ec-410c-acf1-3fcdd53338ed"/>
        <dc:contributor>STEP Harmonization Team</dc:contributor>
        <dc:creator>Phil Spiby, Eurostep</dc:creator>
        <dc:date>2022-09-01</dc:date>
        <dc:source>ISO/TS 10303-4000</dc:source>
        <dc:type>InWork</dc:type>
        <rdfs:comment xml:lang="en">A CollectionVersionSequenceRelationship is a specialization of CollectionVersionRelationship that represents a sequential relationship between two CollectionVersion objects, where the Related succeeds to the Relating.</rdfs:comment>
        <owl:versionInfo>2</owl:versionInfo>
        <skos:changeNote>[2021-07-30] Initial definition.</skos:changeNote>
        <skos:changeNote>[2022-09-01] Phil Spiby, Eurostep: updated comment.</skos:changeNote>
        <skos:prefLabel xml:lang="en">collection version sequence relationship</skos:prefLabel>
    </owl:Class>
    


    <!-- http://standards.iso.org/iso/10303/tech/refdata/core#8c63e8fb-2e14-4124-b2a7-71084b236615 -->

    <owl:Class rdf:about="http://standards.iso.org/iso/10303/tech/refdata/core#8c63e8fb-2e14-4124-b2a7-71084b236615">
        <rdfs:subClassOf rdf:resource="http://standards.iso.org/iso/10303/tech/refdata/core#66348150-092a-4eb7-9561-0b83adfa15ff"/>
        <dc:contributor>STEP Harmonization Team</dc:contributor>
        <dc:creator>Jean Brangé, AFNeT Services</dc:creator>
        <dc:date>2023-10-04</dc:date>
        <dc:source>ISO/TS 10303-4000</dc:source>
        <dc:type>InWork</dc:type>
        <rdfs:comment xml:lang="en">A PointShapeElement is a type of ShapeElement that is associated with a Point.</rdfs:comment>
        <owl:versionInfo>3</owl:versionInfo>
        <skos:changeNote>[2023-10-04] Jean Brangé, AFNeT Services: Initial definition.</skos:changeNote>
        <skos:prefLabel xml:lang="en">point shape element</skos:prefLabel>
    </owl:Class>
    


    <!-- http://standards.iso.org/iso/10303/tech/refdata/core#8c6b4cd0-130a-0135-b552-598f1b1392ae -->

    <owl:Class rdf:about="http://standards.iso.org/iso/10303/tech/refdata/core#8c6b4cd0-130a-0135-b552-598f1b1392ae">
        <rdfs:subClassOf rdf:resource="http://standards.iso.org/iso/10303/tech/refdata/core#1d59c650-3279-0135-b58f-598f1b1392ae"/>
        <dc:contributor>STEP Harmonization Team</dc:contributor>
        <dc:creator>Phil Spiby, Eurostep</dc:creator>
        <dc:date>2022-09-01</dc:date>
        <dc:source>ISO/TS 10303-4000</dc:source>
        <dc:type>InWork</dc:type>
        <rdfs:comment xml:lang="en">A BreakdownOf is an association between a BreakdownVersion and an item (specified by BreakdownOfSelect) of which the BreakdownVersion is a view.</rdfs:comment>
        <owl:versionInfo>2</owl:versionInfo>
        <skos:changeNote>[2021-07-30] Initial definition.</skos:changeNote>
        <skos:changeNote>[2022-09-01] Phil Spiby, Eurostep: updated comment.</skos:changeNote>
        <skos:prefLabel xml:lang="en">breakdown of</skos:prefLabel>
    </owl:Class>
    


    <!-- http://standards.iso.org/iso/10303/tech/refdata/core#8c6d60ca-b819-4480-a184-b1fb33e0c6f5 -->

    <owl:Class rdf:about="http://standards.iso.org/iso/10303/tech/refdata/core#8c6d60ca-b819-4480-a184-b1fb33e0c6f5">
        <rdfs:subClassOf rdf:resource="http://standards.iso.org/iso/10303/tech/refdata/core#STEPThing"/>
        <dc:contributor>STEP Harmonization Team</dc:contributor>
        <dc:creator>Jean Brangé, AFNeT Services</dc:creator>
        <dc:date>2023-10-04</dc:date>
        <dc:source>ISO/TS 10303-4000</dc:source>
        <dc:type>InWork</dc:type>
        <rdfs:comment xml:lang="en">A ProcessOperationOccurrence is a usage of a ProcessOperationDefinition in a ProcessPlan. This association states that the ProcessOperationDefinition is part of the ProcessPlan.</rdfs:comment>
        <owl:versionInfo>3</owl:versionInfo>
        <skos:changeNote>[2023-10-04] Jean Brangé, AFNeT Services: Initial definition.</skos:changeNote>
        <skos:note xml:lang="en">This mechanism enables the reuse of a ProcessOperationDefinition in the context of more than one ProcessPlan.</skos:note>
        <skos:prefLabel xml:lang="en">process operation occurrence</skos:prefLabel>
    </owl:Class>
    


    <!-- http://standards.iso.org/iso/10303/tech/refdata/core#8ca97b6c-c669-45d8-9851-867e50427242 -->

    <owl:Class rdf:about="http://standards.iso.org/iso/10303/tech/refdata/core#8ca97b6c-c669-45d8-9851-867e50427242">
        <rdfs:subClassOf rdf:resource="http://standards.iso.org/iso/10303/tech/refdata/core#59b11220-3279-0135-b58f-598f1b1392ae"/>
        <dc:contributor>STEP Harmonization Team</dc:contributor>
        <dc:creator>Phil Spiby, Eurostep</dc:creator>
        <dc:date>2022-09-01</dc:date>
        <dc:source>ISO/TS 10303-4000</dc:source>
        <dc:type>InWork</dc:type>
        <rdfs:comment xml:lang="en">An InterfaceConnectorVersionRelationship is a relationship between two InterfaceConnectorVersion objects.</rdfs:comment>
        <owl:versionInfo>2</owl:versionInfo>
        <skos:changeNote>[2021-07-30] Initial definition.</skos:changeNote>
        <skos:changeNote>[2022-09-01] Phil Spiby, Eurostep: updated comment.</skos:changeNote>
        <skos:prefLabel xml:lang="en">interface connector version relationship</skos:prefLabel>
    </owl:Class>
    


    <!-- http://standards.iso.org/iso/10303/tech/refdata/core#8cb91eb0-130a-0135-b552-598f1b1392ae -->

    <owl:Class rdf:about="http://standards.iso.org/iso/10303/tech/refdata/core#8cb91eb0-130a-0135-b552-598f1b1392ae">
        <rdfs:subClassOf rdf:resource="http://standards.iso.org/iso/10303/tech/refdata/core#59b11220-3279-0135-b58f-598f1b1392ae"/>
        <dc:contributor>STEP Harmonization Team</dc:contributor>
        <dc:creator>Phil Spiby, Eurostep</dc:creator>
        <dc:date>2022-09-01</dc:date>
        <dc:source>ISO/TS 10303-4000</dc:source>
        <dc:type>InWork</dc:type>
        <rdfs:comment xml:lang="en">A BreakdownVersionRelationship is a relationship between two BreakdownVersion objects.</rdfs:comment>
        <owl:versionInfo>2</owl:versionInfo>
        <skos:changeNote>[2021-07-30] Initial definition.</skos:changeNote>
        <skos:changeNote>[2022-09-01] Phil Spiby, Eurostep: updated comment updated note.</skos:changeNote>
        <skos:note xml:lang="en">Such relationship can exist between two BreakdownVersion instances of the same Breakdown or of different Breakdown instances.</skos:note>
        <skos:prefLabel xml:lang="en">breakdown version relationship</skos:prefLabel>
    </owl:Class>
    


    <!-- http://standards.iso.org/iso/10303/tech/refdata/core#8d31f24a-08bb-4632-8261-89e8dbabe6ee -->

    <owl:Class rdf:about="http://standards.iso.org/iso/10303/tech/refdata/core#8d31f24a-08bb-4632-8261-89e8dbabe6ee">
        <rdfs:subClassOf rdf:resource="http://standards.iso.org/iso/10303/tech/refdata/core#085b6771-a1f8-4cf7-9771-8de2f3a063a1"/>
        <dc:contributor>STEP Harmonization Team</dc:contributor>
        <dc:creator>Phil Spiby, Eurostep</dc:creator>
        <dc:date>2022-09-01</dc:date>
        <dc:source>ISO/TS 10303-4000</dc:source>
        <dc:type>InWork</dc:type>
        <rdfs:comment xml:lang="en">A StateDefinitionConfirmedAssociation is a statement confirmed by evidence such as a measurement assertion that a StateObserved is in conformance with a particular StateDefinition.</rdfs:comment>
        <owl:versionInfo>1</owl:versionInfo>
        <skos:changeNote>[2021-07-30] Initial definition.</skos:changeNote>
        <skos:prefLabel xml:lang="en">state definition confirmed association</skos:prefLabel>
    </owl:Class>
    


    <!-- http://standards.iso.org/iso/10303/tech/refdata/core#8d60f770-130a-0135-b552-598f1b1392ae -->

    <owl:Class rdf:about="http://standards.iso.org/iso/10303/tech/refdata/core#8d60f770-130a-0135-b552-598f1b1392ae">
        <rdfs:subClassOf rdf:resource="http://standards.iso.org/iso/10303/tech/refdata/core#cca6c810-130a-0135-b552-598f1b1392ae"/>
        <dc:contributor>STEP Harmonization Team</dc:contributor>
        <dc:creator>Jean Brangé, AFNeT Services</dc:creator>
        <dc:date>2023-10-04</dc:date>
        <dc:source>ISO/TS 10303-4000</dc:source>
        <dc:type>InWork</dc:type>
        <rdfs:comment xml:lang="en">A CentreOfMass is a type of ShapeDependentProperty that is the centre of the mass of a body. The relative position of the CentreOfMass within the body is an invariant datum relative to rotation and translation. The CentreOfMass is a characteristic of a part, not its shape.</rdfs:comment>
        <owl:versionInfo>3</owl:versionInfo>
        <skos:changeNote>[2023-10-04] Jean Brangé, AFNeT Services: Initial definition.</skos:changeNote>
        <skos:note xml:lang="en">If a shape representation is present, the CentreOfMass is usually derivable from the shape representation. However, as a characteristic of a part, it may be predefined in order to reflect a requirement.</skos:note>
        <skos:note xml:lang="en">In order to convey the information about the actual centre of mass of a geometric model, the use of GeneralShapeDependentProperty with value &apos;centroid&apos; for its attribute PropertyType is appropriate.</skos:note>
        <skos:prefLabel xml:lang="en">centre of mass</skos:prefLabel>
    </owl:Class>
    


    <!-- http://standards.iso.org/iso/10303/tech/refdata/core#8d765430-130a-0135-b552-598f1b1392ae -->

    <owl:Class rdf:about="http://standards.iso.org/iso/10303/tech/refdata/core#8d765430-130a-0135-b552-598f1b1392ae">
        <rdfs:subClassOf rdf:resource="http://standards.iso.org/iso/10303/tech/refdata/core#STEPThing"/>
        <dc:contributor>STEP Harmonization Team</dc:contributor>
        <dc:creator>Phil Spiby, Eurostep</dc:creator>
        <dc:date>2022-09-01</dc:date>
        <dc:source>ISO/TS 10303-4000</dc:source>
        <dc:type>InWork</dc:type>
        <rdfs:comment xml:lang="en">A Certification is a written assurance by a third party that a product, process or service conforms to specified requirements. A Certification can be associated with a document that asserts the satisfaction of specific quality criteria.</rdfs:comment>
        <owl:versionInfo>2</owl:versionInfo>
        <skos:changeNote>[2021-07-30] Initial definition.</skos:changeNote>
        <skos:changeNote>[2022-09-01] Phil Spiby, Eurostep: updated comment updated note.</skos:changeNote>
        <skos:note xml:lang="en">Certification information can be attached to a product, tool, process, activity, service or the skill of a person for a certain task.</skos:note>
        <skos:prefLabel xml:lang="en">certification</skos:prefLabel>
    </owl:Class>
    


    <!-- http://standards.iso.org/iso/10303/tech/refdata/core#8d823b22-d4d9-46f6-aebb-d082e6b8d45d -->

    <owl:Class rdf:about="http://standards.iso.org/iso/10303/tech/refdata/core#8d823b22-d4d9-46f6-aebb-d082e6b8d45d">
        <rdfs:subClassOf rdf:resource="http://standards.iso.org/iso/10303/tech/refdata/core#59b11220-3279-0135-b58f-598f1b1392ae"/>
        <dc:contributor>STEP Harmonization Team</dc:contributor>
        <dc:creator>Phil Spiby, Eurostep</dc:creator>
        <dc:date>2022-09-01</dc:date>
        <dc:source>ISO/TS 10303-4000</dc:source>
        <dc:type>InWork</dc:type>
        <rdfs:comment xml:lang="en">An EnvironmentDefinitionViewRelationship is a relationship between two EnvironmentDefinitionView objects.</rdfs:comment>
        <owl:versionInfo>2</owl:versionInfo>
        <skos:changeNote>[2021-07-30] Initial definition.</skos:changeNote>
        <skos:changeNote>[2022-09-01] Phil Spiby, Eurostep: updated comment.</skos:changeNote>
        <skos:prefLabel xml:lang="en">environment definition view relationship</skos:prefLabel>
    </owl:Class>
    


    <!-- http://standards.iso.org/iso/10303/tech/refdata/core#8d941a6d-b602-42c0-846c-1c8058074312 -->

    <owl:Class rdf:about="http://standards.iso.org/iso/10303/tech/refdata/core#8d941a6d-b602-42c0-846c-1c8058074312">
        <rdfs:subClassOf rdf:resource="http://standards.iso.org/iso/10303/tech/refdata/core#STEPThing"/>
        <dc:contributor>STEP Harmonization Team</dc:contributor>
        <dc:creator>Phil Spiby, Eurostep</dc:creator>
        <dc:date>2022-09-01</dc:date>
        <dc:source>ISO/TS 10303-4000</dc:source>
        <dc:type>InWork</dc:type>
        <rdfs:comment xml:lang="en">An Envelope is an historical record of the transmission of a Message. It is used to record the audit data for sending and acknowledging a Message. Each Envelope is only used once because it is a historical record and is not versioned.</rdfs:comment>
        <owl:versionInfo>1</owl:versionInfo>
        <skos:changeNote>[2021-07-30] Initial definition.</skos:changeNote>
        <skos:prefLabel xml:lang="en">envelope</skos:prefLabel>
    </owl:Class>
    


    <!-- http://standards.iso.org/iso/10303/tech/refdata/core#8dad895b-cef6-41b8-8a11-cb6c54ef8b9c -->

    <owl:Class rdf:about="http://standards.iso.org/iso/10303/tech/refdata/core#8dad895b-cef6-41b8-8a11-cb6c54ef8b9c">
        <rdfs:subClassOf rdf:resource="http://standards.iso.org/iso/10303/tech/refdata/core#0cc8b831-37f7-4cd5-984f-dbb5588fbc1d"/>
        <dc:contributor>STEP Harmonization Team</dc:contributor>
        <dc:creator>Jean Brangé, AFNeT Services</dc:creator>
        <dc:date>2023-10-04</dc:date>
        <dc:source>ISO/TS 10303-4000</dc:source>
        <dc:type>InWork</dc:type>
        <rdfs:comment xml:lang="en">A HarnessSegment is a type of PartShapeElement that represents an Edge from a ConnectedEdgeWithLengthSetRepresentation for a WiringHarnessAssemblyDesign.</rdfs:comment>
        <owl:versionInfo>3</owl:versionInfo>
        <skos:changeNote>[2023-10-04] Jean Brangé, AFNeT Services: Initial definition.</skos:changeNote>
        <skos:prefLabel xml:lang="en">harness segment</skos:prefLabel>
    </owl:Class>
    


    <!-- http://standards.iso.org/iso/10303/tech/refdata/core#8db495b0-130a-0135-b552-598f1b1392ae -->

    <owl:Class rdf:about="http://standards.iso.org/iso/10303/tech/refdata/core#8db495b0-130a-0135-b552-598f1b1392ae">
        <rdfs:subClassOf rdf:resource="http://standards.iso.org/iso/10303/tech/refdata/core#1cfca290-3279-0135-b58f-598f1b1392ae"/>
        <dc:contributor>STEP Harmonization Team</dc:contributor>
        <dc:creator>Phil Spiby, Eurostep</dc:creator>
        <dc:date>2022-09-01</dc:date>
        <dc:source>ISO/TS 10303-4000</dc:source>
        <dc:type>InWork</dc:type>
        <rdfs:comment xml:lang="en">A CertificationAssignment is an assignment of a Certification to an item (specified by CertificationAssignmentSelect). The meaning of the assignment can be specified using the ClassifiedAs attribute inherited from the AssignmentObject.</rdfs:comment>
        <owl:versionInfo>2</owl:versionInfo>
        <skos:changeNote>[2021-07-30] Initial definition.</skos:changeNote>
        <skos:changeNote>[2022-09-01] Phil Spiby, Eurostep: updated comment.</skos:changeNote>
        <skos:prefLabel xml:lang="en">certification assignment</skos:prefLabel>
    </owl:Class>
    


    <!-- http://standards.iso.org/iso/10303/tech/refdata/core#8de95357-342b-408f-9e56-5a4c658803a2 -->

    <owl:Class rdf:about="http://standards.iso.org/iso/10303/tech/refdata/core#8de95357-342b-408f-9e56-5a4c658803a2">
        <rdfs:subClassOf rdf:resource="http://standards.iso.org/iso/10303/tech/refdata/core#STEPThing"/>
        <dc:contributor>STEP Harmonization Team</dc:contributor>
        <dc:creator>Phil Spiby, Eurostep</dc:creator>
        <dc:date>2022-09-01</dc:date>
        <dc:source>ISO/TS 10303-4000</dc:source>
        <dc:type>InWork</dc:type>
        <rdfs:comment xml:lang="en">A TypeOfPersonDefinition is the definition of a TypeOfPerson in terms of required properties or attributes.</rdfs:comment>
        <owl:versionInfo>1</owl:versionInfo>
        <skos:changeNote>[2022-09-01] Initial definition.</skos:changeNote>
        <skos:example xml:lang="en">A junior mechanical design engineer could be specified to be either someone who has 3 years experience of working in a mechanical design department, or a degree in mechanical engineering.</skos:example>
        <skos:prefLabel xml:lang="en">type of person definition</skos:prefLabel>
    </owl:Class>
    


    <!-- http://standards.iso.org/iso/10303/tech/refdata/core#8e51b43d-49ca-4a6f-880d-4cb737a79dff -->

    <owl:Class rdf:about="http://standards.iso.org/iso/10303/tech/refdata/core#8e51b43d-49ca-4a6f-880d-4cb737a79dff">
        <rdfs:subClassOf rdf:resource="http://standards.iso.org/iso/10303/tech/refdata/core#9b55c2b7-5397-4cfa-9aa1-a3a6785467b4"/>
        <dc:contributor>STEP Harmonization Team</dc:contributor>
        <dc:creator>Jean Brangé, AFNeT Services</dc:creator>
        <dc:date>2023-10-04</dc:date>
        <dc:source>ISO/TS 10303-4000</dc:source>
        <dc:type>InWork</dc:type>
        <rdfs:comment xml:lang="en">A ShapeFeatureDefinitionFitRelationship is a type of ShapeFeatureDefinitionRelationship that states that the two related ShapeFeatureDefinition fit with each other.</rdfs:comment>
        <owl:versionInfo>3</owl:versionInfo>
        <skos:changeNote>[2023-10-04] Jean Brangé, AFNeT Services: Initial definition.</skos:changeNote>
        <skos:prefLabel xml:lang="en">shape feature definition fit relationship</skos:prefLabel>
    </owl:Class>
    


    <!-- http://standards.iso.org/iso/10303/tech/refdata/core#8eb0f710-130a-0135-b552-598f1b1392ae -->

    <owl:Class rdf:about="http://standards.iso.org/iso/10303/tech/refdata/core#8eb0f710-130a-0135-b552-598f1b1392ae">
        <rdfs:subClassOf rdf:resource="http://standards.iso.org/iso/10303/tech/refdata/core#STEPThing"/>
        <dc:contributor>STEP Harmonization Team</dc:contributor>
        <dc:creator>Phil Spiby, Eurostep</dc:creator>
        <dc:date>2022-09-01</dc:date>
        <dc:source>ISO/TS 10303-4000</dc:source>
        <dc:type>InWork</dc:type>
        <rdfs:comment xml:lang="en">A Classification is an object that associates a Class with one or more objects.</rdfs:comment>
        <owl:versionInfo>1</owl:versionInfo>
        <skos:changeNote>[2021-07-30] Initial definition.</skos:changeNote>
        <skos:prefLabel xml:lang="en">classification</skos:prefLabel>
    </owl:Class>
    


    <!-- http://standards.iso.org/iso/10303/tech/refdata/core#8ed59610-130a-0135-b552-598f1b1392ae -->

    <owl:Class rdf:about="http://standards.iso.org/iso/10303/tech/refdata/core#8ed59610-130a-0135-b552-598f1b1392ae">
        <rdfs:subClassOf rdf:resource="http://standards.iso.org/iso/10303/tech/refdata/core#59b11220-3279-0135-b58f-598f1b1392ae"/>
        <dc:contributor>STEP Harmonization Team</dc:contributor>
        <dc:creator>Phil Spiby, Eurostep</dc:creator>
        <dc:date>2022-09-01</dc:date>
        <dc:source>ISO/TS 10303-4000</dc:source>
        <dc:type>InWork</dc:type>
        <rdfs:comment xml:lang="en">A ClassificationRelationship is a relationship between two Classification objects.</rdfs:comment>
        <owl:versionInfo>1</owl:versionInfo>
        <skos:changeNote>[2021-07-30] Initial definition.</skos:changeNote>
        <skos:prefLabel xml:lang="en">classification relationship</skos:prefLabel>
    </owl:Class>
    


    <!-- http://standards.iso.org/iso/10303/tech/refdata/core#8f1732f0-130a-0135-b552-598f1b1392ae -->

    <owl:Class rdf:about="http://standards.iso.org/iso/10303/tech/refdata/core#8f1732f0-130a-0135-b552-598f1b1392ae">
        <rdfs:subClassOf rdf:resource="http://standards.iso.org/iso/10303/tech/refdata/core#d80a2030-130a-0135-b552-598f1b1392ae"/>
        <dc:contributor>STEP Harmonization Team</dc:contributor>
        <dc:creator>Phil Spiby, Eurostep</dc:creator>
        <dc:date>2022-09-01</dc:date>
        <dc:source>ISO/TS 10303-4000</dc:source>
        <dc:type>InWork</dc:type>
        <rdfs:comment xml:lang="en">A CollectedPartRelationship is a type of ViewOccurrenceRelationship that is a mechanism to associate Occurrence objects with a CollectionDefinition.</rdfs:comment>
        <owl:versionInfo>1</owl:versionInfo>
        <skos:changeNote>[2021-07-30] Initial definition.</skos:changeNote>
        <skos:prefLabel xml:lang="en">collected part relationship</skos:prefLabel>
    </owl:Class>
    


    <!-- http://standards.iso.org/iso/10303/tech/refdata/core#8f24ee90-130a-0135-b552-598f1b1392ae -->

    <owl:Class rdf:about="http://standards.iso.org/iso/10303/tech/refdata/core#8f24ee90-130a-0135-b552-598f1b1392ae">
        <rdfs:subClassOf rdf:resource="http://standards.iso.org/iso/10303/tech/refdata/core#b3911ec0-130a-0135-b552-598f1b1392ae"/>
        <dc:contributor>STEP Harmonization Team</dc:contributor>
        <dc:creator>Phil Spiby, Eurostep</dc:creator>
        <dc:date>2022-09-01</dc:date>
        <dc:source>ISO/TS 10303-4000</dc:source>
        <dc:type>InWork</dc:type>
        <rdfs:comment xml:lang="en">A CollectionDefinition is a type of PartView that is the definition of a PartVersion that serves as a collector for Occurrence objects.</rdfs:comment>
        <owl:versionInfo>2</owl:versionInfo>
        <skos:changeNote>[2021-07-30] Initial definition.</skos:changeNote>
        <skos:changeNote>[2022-09-01] Phil Spiby, Eurostep: updated example.</skos:changeNote>
        <skos:example xml:lang="en">Brake pads on the left and right front brake from same supplier, locks and keys of the car all from one supplier, wooden panels in the interior from the same supplier (to ensure common structure of the wood) are examples for collections.</skos:example>
        <skos:example xml:lang="en">Objects that are mounted in the same vehicle but cannot be assembled together.</skos:example>
        <skos:prefLabel xml:lang="en">collection definition</skos:prefLabel>
    </owl:Class>
    


    <!-- http://standards.iso.org/iso/10303/tech/refdata/core#8f543bf0-130a-0135-b552-598f1b1392ae -->

    <owl:Class rdf:about="http://standards.iso.org/iso/10303/tech/refdata/core#8f543bf0-130a-0135-b552-598f1b1392ae">
        <rdfs:subClassOf rdf:resource="http://standards.iso.org/iso/10303/tech/refdata/core#9fddc900-130a-0135-b552-598f1b1392ae"/>
        <dc:contributor>STEP Harmonization Team</dc:contributor>
        <dc:creator>Phil Spiby, Eurostep</dc:creator>
        <dc:date>2022-09-01</dc:date>
        <dc:source>ISO/TS 10303-4000</dc:source>
        <dc:type>InWork</dc:type>
        <rdfs:comment xml:lang="en">A ComposedGeometricModel is a type of GeometricModel that is the result of composing other GeometricModels (via GeometricRepresentationRelationship) into a single one.</rdfs:comment>
        <owl:versionInfo>2</owl:versionInfo>
        <skos:changeNote>[2021-07-30] Initial definition.</skos:changeNote>
        <skos:changeNote>[2022-09-01] Phil Spiby, Eurostep: updated comment.</skos:changeNote>
        <skos:prefLabel xml:lang="en">composed geometric model</skos:prefLabel>
    </owl:Class>
    


    <!-- http://standards.iso.org/iso/10303/tech/refdata/core#8fb45d50-130a-0135-b552-598f1b1392ae -->

    <owl:Class rdf:about="http://standards.iso.org/iso/10303/tech/refdata/core#8fb45d50-130a-0135-b552-598f1b1392ae">
        <rdfs:subClassOf rdf:resource="http://standards.iso.org/iso/10303/tech/refdata/core#STEPThing"/>
        <dc:contributor>STEP Harmonization Team</dc:contributor>
        <dc:creator>Phil Spiby, Eurostep</dc:creator>
        <dc:date>2022-09-01</dc:date>
        <dc:source>ISO/TS 10303-4000</dc:source>
        <dc:type>InWork</dc:type>
        <rdfs:comment xml:lang="en">A Condition is a definition of the precedent that has to be fulfilled before a statement or relationship becomes valid.</rdfs:comment>
        <owl:versionInfo>2</owl:versionInfo>
        <skos:changeNote>[2021-07-30] Initial definition.</skos:changeNote>
        <skos:changeNote>[2022-09-01] Phil Spiby, Eurostep: updated comment updated example.</skos:changeNote>
        <skos:example xml:lang="en">&apos;If the engine has been running for 10000 hours then it requires a service&apos; is an example of a conditional statement. The conditional part of the statement is &apos;If the engine has been running for 10000 hours&apos; which is stored in definition attribute on Condition. The parameter or subject of the condition is &apos;the engine&apos; which is represented by a ConditionParameter identifying the IndividualPart which represents the engine. The consequence of the condition is &apos;then it requires a service&apos;. This is represented by ConditionAssignment identifying the activity to perform the service.</skos:example>
        <skos:note xml:lang="en">The condition is defined as a text-based expression that is represented by the description attribute. The parameters against which the condition is to be evaluated are identified by ConditionParameter. The target or consequence of a condition is represented by ConditionAssignment.</skos:note>
        <skos:prefLabel xml:lang="en">condition</skos:prefLabel>
    </owl:Class>
    


    <!-- http://standards.iso.org/iso/10303/tech/refdata/core#8009fd1b-d1dc-4bdd-be6c-a359398bb79b -->

    <owl:Class rdf:about="http://standards.iso.org/iso/10303/tech/refdata/core#8009fd1b-d1dc-4bdd-be6c-a359398bb79b">
        <rdfs:subClassOf rdf:resource="http://standards.iso.org/iso/10303/tech/refdata/core#c54bc6fa-f6d8-4943-85de-6439071c5325"/>
        <dc:contributor>STEP Harmonization Team</dc:contributor>
        <dc:creator>Jean Brangé, AFNeT Services</dc:creator>
        <dc:date>2023-10-04</dc:date>
        <dc:source>ISO/TS 10303-4000</dc:source>
        <dc:type>InWork</dc:type>
        <rdfs:comment xml:lang="en">A CrossSectionalAlternativePartShapeElement is a type of CrossSectionalPartShapeElement that is an alternative between one or more CrossSectionalOccurrenceShapeElement or CrossSectionalPartShapeElement for the same purpose. At one position on a specific HarnessSegment, there is exactly one CrossSectionalOccurrenceShapeElement or CrossSectionalPartShapeElement.</rdfs:comment>
        <owl:versionInfo>3</owl:versionInfo>
        <skos:changeNote>[2023-10-04] Jean Brangé, AFNeT Services: Initial definition.</skos:changeNote>
        <skos:example xml:lang="en">A splice connecting two wires at a HarnessNode where each WireOccurrence has the same purpose and does not change the cross section of the HarnessSegment.</skos:example>
        <skos:prefLabel xml:lang="en">cross sectional alternative part shape element</skos:prefLabel>
    </owl:Class>
    


    <!-- http://standards.iso.org/iso/10303/tech/refdata/core#807ca790-e51d-42fd-ab6b-fd30ecbf7949 -->

    <owl:Class rdf:about="http://standards.iso.org/iso/10303/tech/refdata/core#807ca790-e51d-42fd-ab6b-fd30ecbf7949">
        <rdfs:subClassOf rdf:resource="http://standards.iso.org/iso/10303/tech/refdata/core#09cd1ad9-ed18-4c44-a399-eb27b8148d42"/>
        <dc:contributor>STEP Harmonization Team</dc:contributor>
        <dc:creator>Jean Brangé, AFNeT Services</dc:creator>
        <dc:date>2023-10-04</dc:date>
        <dc:source>ISO/TS 10303-4000</dc:source>
        <dc:type>InWork</dc:type>
        <rdfs:comment xml:lang="en">A CableOccurrenceTerminalLocationGroup is a type of OccurrenceTerminal that represents the grouping of CableOccurrenceTerminals on one of the ends, or at intermediate positions between the ends, of a CableOccurrence. The CableOccurrenceTerminalLocationGroups at the ends of the cable are named &quot;end a&quot; and &quot;end b&quot; respectively. CableOccurrenceTerminalLocationGroups in the middle of the cable shall start with the letters &quot;intermediate&quot; followed by arbitrary text.</rdfs:comment>
        <owl:versionInfo>3</owl:versionInfo>
        <skos:changeNote>[2023-10-04] Jean Brangé, AFNeT Services: Initial definition.</skos:changeNote>
        <skos:prefLabel xml:lang="en">cable occurrence terminal location group</skos:prefLabel>
    </owl:Class>
    


    <!-- http://standards.iso.org/iso/10303/tech/refdata/core#815e62dc-6223-42f9-af5c-166dbec77d8f -->

    <owl:Class rdf:about="http://standards.iso.org/iso/10303/tech/refdata/core#815e62dc-6223-42f9-af5c-166dbec77d8f">
        <rdfs:subClassOf rdf:resource="http://standards.iso.org/iso/10303/tech/refdata/core#1d59c650-3279-0135-b58f-598f1b1392ae"/>
        <dc:contributor>STEP Harmonization Team</dc:contributor>
        <dc:creator>Phil Spiby, Eurostep</dc:creator>
        <dc:date>2022-09-01</dc:date>
        <dc:source>ISO/TS 10303-4000</dc:source>
        <dc:type>InWork</dc:type>
        <rdfs:comment xml:lang="en">An ItemAssumed is an association between an Assumption and the item (specified by AssumedItemSelect) that is being assumed. The facility shall be represented by a ResourceItemAssignment, the location by a Location, and the existence of the facility at the location, by a LocationAssignment assigning a location to the resource.</rdfs:comment>
        <owl:versionInfo>1</owl:versionInfo>
        <skos:changeNote>[2021-07-30] Initial definition.</skos:changeNote>
        <skos:example xml:lang="en">A facility is assumed to exist at a given location.</skos:example>
        <skos:prefLabel xml:lang="en">item assumed</skos:prefLabel>
    </owl:Class>
    


    <!-- http://standards.iso.org/iso/10303/tech/refdata/core#8192782a-76cc-4acd-9f1e-3b4d52188105 -->

    <owl:Class rdf:about="http://standards.iso.org/iso/10303/tech/refdata/core#8192782a-76cc-4acd-9f1e-3b4d52188105">
        <rdfs:subClassOf rdf:resource="http://standards.iso.org/iso/10303/tech/refdata/core#84099bf0-130a-0135-b552-598f1b1392ae"/>
        <dc:contributor>STEP Harmonization Team</dc:contributor>
        <dc:creator>Phil Spiby, Eurostep</dc:creator>
        <dc:date>2022-09-01</dc:date>
        <dc:source>ISO/TS 10303-4000</dc:source>
        <dc:type>InWork</dc:type>
        <rdfs:comment xml:lang="en">A TaskElementRelationship is a relationship between two TaskElement objects.</rdfs:comment>
        <owl:versionInfo>2</owl:versionInfo>
        <skos:changeNote>[2021-07-30] Initial definition.</skos:changeNote>
        <skos:changeNote>[2022-09-01] Phil Spiby, Eurostep: updated comment updated example.</skos:changeNote>
        <skos:example xml:lang="en">A TaskElementRelationship can be used to capture a time dependency that cuts across the structure of the method.</skos:example>
        <skos:prefLabel xml:lang="en">task element relationship</skos:prefLabel>
    </owl:Class>
    


    <!-- http://standards.iso.org/iso/10303/tech/refdata/core#82f3e630-130a-0135-b552-598f1b1392ae -->

    <owl:Class rdf:about="http://standards.iso.org/iso/10303/tech/refdata/core#82f3e630-130a-0135-b552-598f1b1392ae">
        <rdfs:subClassOf rdf:resource="http://standards.iso.org/iso/10303/tech/refdata/core#1cfca290-3279-0135-b58f-598f1b1392ae"/>
        <dc:contributor>STEP Harmonization Team</dc:contributor>
        <dc:creator>Phil Spiby, Eurostep</dc:creator>
        <dc:date>2022-09-01</dc:date>
        <dc:source>ISO/TS 10303-4000</dc:source>
        <dc:type>InWork</dc:type>
        <rdfs:comment xml:lang="en">An ActivityAssignment is an assignment of an Activity to an item (specified by ActivityAssignmentSelect). It characterizes the role of the related data with respect to the activity. ActivityAssignment should not be used to represent the association of an activity with the people or organizations that are responsible for its execution or its management. That kind of information should be represented by instances of PersonOrganizationAssignment.</rdfs:comment>
        <owl:versionInfo>2</owl:versionInfo>
        <skos:changeNote>[2021-07-30] Initial definition.</skos:changeNote>
        <skos:changeNote>[2022-09-01] Phil Spiby, Eurostep: updated comment updated note.</skos:changeNote>
        <skos:prefLabel xml:lang="en">activity assignment</skos:prefLabel>
    </owl:Class>
    


    <!-- http://standards.iso.org/iso/10303/tech/refdata/core#8276c6f0-130a-0135-b552-598f1b1392ae -->

    <owl:Class rdf:about="http://standards.iso.org/iso/10303/tech/refdata/core#8276c6f0-130a-0135-b552-598f1b1392ae">
        <rdfs:subClassOf rdf:resource="http://standards.iso.org/iso/10303/tech/refdata/core#STEPThing"/>
        <dc:contributor>STEP Harmonization Team</dc:contributor>
        <dc:creator>Phil Spiby, Eurostep</dc:creator>
        <dc:date>2022-09-01</dc:date>
        <dc:source>ISO/TS 10303-4000</dc:source>
        <dc:type>InWork</dc:type>
        <rdfs:comment xml:lang="en">An Activity represents an occurrence of an action that has taken place, is taking place, or is expected to take place in the future. The mechanism by which the Activity is performed is identified by an ActivityMethod that is referred to by the ChosenMethod property.</rdfs:comment>
        <owl:versionInfo>1</owl:versionInfo>
        <skos:changeNote>[2021-07-30] Initial definition.</skos:changeNote>
        <skos:example xml:lang="en">Change, distilling, design, a process to drill a hole, and a task such as training someone, are examples of activities.</skos:example>
        <skos:note xml:lang="en">The items that are affected by an Activity are identified by instances of ActivityAssignment.</skos:note>
        <skos:prefLabel xml:lang="en">activity</skos:prefLabel>
    </owl:Class>
    


    <!-- http://standards.iso.org/iso/10303/tech/refdata/core#83b2a250-130a-0135-b552-598f1b1392ae -->

    <owl:Class rdf:about="http://standards.iso.org/iso/10303/tech/refdata/core#83b2a250-130a-0135-b552-598f1b1392ae">
        <rdfs:subClassOf rdf:resource="http://standards.iso.org/iso/10303/tech/refdata/core#1cfca290-3279-0135-b58f-598f1b1392ae"/>
        <dc:contributor>STEP Harmonization Team</dc:contributor>
        <dc:creator>Phil Spiby, Eurostep</dc:creator>
        <dc:date>2022-09-01</dc:date>
        <dc:source>ISO/TS 10303-4000</dc:source>
        <dc:type>InWork</dc:type>
        <rdfs:comment xml:lang="en">An ActivityMethodAssignment is an assignment of an ActivityMethod to an item (specified by ActivityMethodAssignmentSelect).</rdfs:comment>
        <owl:versionInfo>2</owl:versionInfo>
        <skos:changeNote>[2021-07-30] Initial definition.</skos:changeNote>
        <skos:changeNote>[2022-09-01] Phil Spiby, Eurostep: updated comment.</skos:changeNote>
        <skos:prefLabel xml:lang="en">activity method assignment</skos:prefLabel>
    </owl:Class>
    


    <!-- http://standards.iso.org/iso/10303/tech/refdata/core#833e0c52-0fcc-43dc-bcbe-b6094f2fba49 -->

    <owl:Class rdf:about="http://standards.iso.org/iso/10303/tech/refdata/core#833e0c52-0fcc-43dc-bcbe-b6094f2fba49">
        <rdfs:subClassOf rdf:resource="http://standards.iso.org/iso/10303/tech/refdata/core#f8816baf-d66a-42f9-bdcc-38e946c9a2fa"/>
        <dc:contributor>STEP Harmonization Team</dc:contributor>
        <dc:creator>Jean Brangé, AFNeT Services</dc:creator>
        <dc:date>2023-10-04</dc:date>
        <dc:source>ISO/TS 10303-4000</dc:source>
        <dc:type>InWork</dc:type>
        <rdfs:comment xml:lang="en">A Tangent is a type of DerivedShapeElement that contacts a curve or surface ShapeElement at a single point or line. A Tangent may be a TangentPlane.</rdfs:comment>
        <owl:versionInfo>3</owl:versionInfo>
        <skos:changeNote>[2023-10-04] Jean Brangé, AFNeT Services: Initial definition.</skos:changeNote>
        <skos:prefLabel xml:lang="en">tangent</skos:prefLabel>
    </owl:Class>
    


    <!-- http://standards.iso.org/iso/10303/tech/refdata/core#833eaad0-130a-0135-b552-598f1b1392ae -->

    <owl:Class rdf:about="http://standards.iso.org/iso/10303/tech/refdata/core#833eaad0-130a-0135-b552-598f1b1392ae">
        <rdfs:subClassOf rdf:resource="http://standards.iso.org/iso/10303/tech/refdata/core#844b38d0-130a-0135-b552-598f1b1392ae"/>
        <dc:contributor>STEP Harmonization Team</dc:contributor>
        <dc:creator>Phil Spiby, Eurostep</dc:creator>
        <dc:date>2022-09-01</dc:date>
        <dc:source>ISO/TS 10303-4000</dc:source>
        <dc:type>InWork</dc:type>
        <rdfs:comment xml:lang="en">An ActivityHappeningRelationship is a type of ActivityRelationship that relates a PlannedActivity and its ActualActivity.</rdfs:comment>
        <owl:versionInfo>2</owl:versionInfo>
        <skos:changeNote>[2021-07-30] Initial definition.</skos:changeNote>
        <skos:changeNote>[2022-09-01] Phil Spiby, Eurostep: updated example updated note.</skos:changeNote>
        <skos:example xml:lang="en">A single defined activity is recorded historically by several sub-activities.</skos:example>
        <skos:example xml:lang="en">A single servicing activity takes the opportunity to make additional checks and repairs.</skos:example>
        <skos:note xml:lang="en">A single ActualActivity can fulfil several PlannedActivity objects.</skos:note>
        <skos:note xml:lang="en">Many ActualActivity objects can be the actual for a single PlannedActivity.</skos:note>
        <skos:prefLabel xml:lang="en">activity happening relationship</skos:prefLabel>
    </owl:Class>
    


    <!-- http://standards.iso.org/iso/10303/tech/refdata/core#835280f0-130a-0135-b552-598f1b1392ae -->

    <owl:Class rdf:about="http://standards.iso.org/iso/10303/tech/refdata/core#835280f0-130a-0135-b552-598f1b1392ae">
        <rdfs:subClassOf rdf:resource="http://standards.iso.org/iso/10303/tech/refdata/core#STEPThing"/>
        <dc:contributor>STEP Harmonization Team</dc:contributor>
        <dc:creator>Phil Spiby, Eurostep</dc:creator>
        <dc:date>2022-09-01</dc:date>
        <dc:source>ISO/TS 10303-4000</dc:source>
        <dc:type>InWork</dc:type>
        <rdfs:comment xml:lang="en">An ActivityMethod is a way to carry out an Activity.</rdfs:comment>
        <owl:versionInfo>2</owl:versionInfo>
        <skos:changeNote>[2021-07-30] Initial definition.</skos:changeNote>
        <skos:changeNote>[2022-09-01] Phil Spiby, Eurostep: updated note.</skos:changeNote>
        <skos:note xml:lang="en">There can be more than one method for producing a required result.</skos:note>
        <skos:note xml:lang="en">This definition can be used to characterize a way to resolve a request for action.</skos:note>
        <skos:prefLabel xml:lang="en">activity method</skos:prefLabel>
    </owl:Class>
    


    <!-- http://standards.iso.org/iso/10303/tech/refdata/core#8369b682-376e-45eb-8451-87f9feb1a56a -->

    <owl:Class rdf:about="http://standards.iso.org/iso/10303/tech/refdata/core#8369b682-376e-45eb-8451-87f9feb1a56a">
        <rdfs:subClassOf rdf:resource="http://standards.iso.org/iso/10303/tech/refdata/core#44078e31-a1cb-4d89-b8d6-ab60b9140b06"/>
        <dc:contributor>STEP Harmonization Team</dc:contributor>
        <dc:creator>Jean Brangé, AFNeT Services</dc:creator>
        <dc:date>2023-10-04</dc:date>
        <dc:source>ISO/TS 10303-4000</dc:source>
        <dc:type>InWork</dc:type>
        <rdfs:comment xml:lang="en">A TargetRectangle is a type of PlacedTarget that specifies a DatumTarget that is defined by an implicit rectangle. The centre of the rectangle is specified by the placing AxisPlacement. The orientation of the TargetRectangle is the x-y-plane with half the length of the rectangle in positive and half the length in negative direction along the x-axis and with half the width of the rectangle in positive and half the width in negative direction along the y-axis of the AxisPlacement.</rdfs:comment>
        <owl:versionInfo>3</owl:versionInfo>
        <skos:changeNote>[2023-10-04] Jean Brangé, AFNeT Services: Initial definition.</skos:changeNote>
        <skos:prefLabel xml:lang="en">target rectangle</skos:prefLabel>
    </owl:Class>
    


    <!-- http://standards.iso.org/iso/10303/tech/refdata/core#837acc56-e28d-4eb0-8b03-98c1a6215f61 -->

    <owl:Class rdf:about="http://standards.iso.org/iso/10303/tech/refdata/core#837acc56-e28d-4eb0-8b03-98c1a6215f61">
        <rdfs:subClassOf rdf:resource="http://standards.iso.org/iso/10303/tech/refdata/core#1d59c650-3279-0135-b58f-598f1b1392ae"/>
        <dc:contributor>STEP Harmonization Team</dc:contributor>
        <dc:creator>Phil Spiby, Eurostep</dc:creator>
        <dc:date>2022-09-01</dc:date>
        <dc:source>ISO/TS 10303-4000</dc:source>
        <dc:type>InWork</dc:type>
        <rdfs:comment xml:lang="en">A RelatedConditionParameter is an association between a ConditionParameter and a parameter (specified by EvaluationParameterSelect). This association is used to record the association between the parameters used to define a condition and the parameters used to evaluate it.</rdfs:comment>
        <owl:versionInfo>2</owl:versionInfo>
        <skos:changeNote>[2021-07-30] Initial definition.</skos:changeNote>
        <skos:changeNote>[2022-09-01] Phil Spiby, Eurostep: updated comment.</skos:changeNote>
        <skos:prefLabel xml:lang="en">related condition parameter</skos:prefLabel>
    </owl:Class>
    


    <!-- http://standards.iso.org/iso/10303/tech/refdata/core#83730b79-1452-431f-b7b3-9055c2e8ca3c -->

    <owl:Class rdf:about="http://standards.iso.org/iso/10303/tech/refdata/core#83730b79-1452-431f-b7b3-9055c2e8ca3c">
        <rdfs:subClassOf rdf:resource="http://standards.iso.org/iso/10303/tech/refdata/core#59b11220-3279-0135-b58f-598f1b1392ae"/>
        <dc:contributor>STEP Harmonization Team</dc:contributor>
        <dc:creator>Phil Spiby, Eurostep</dc:creator>
        <dc:date>2022-09-01</dc:date>
        <dc:source>ISO/TS 10303-4000</dc:source>
        <dc:type>InWork</dc:type>
        <rdfs:comment xml:lang="en">An InterfaceConnectorRelationship is a relationship between two InterfaceConnector objects.</rdfs:comment>
        <owl:versionInfo>2</owl:versionInfo>
        <skos:changeNote>[2021-07-30] Initial definition.</skos:changeNote>
        <skos:changeNote>[2022-09-01] Phil Spiby, Eurostep: updated comment.</skos:changeNote>
        <skos:prefLabel xml:lang="en">interface connector relationship</skos:prefLabel>
    </owl:Class>
    


    <!-- http://standards.iso.org/iso/10303/tech/refdata/core#84cff930-130a-0135-b552-598f1b1392ae -->

    <owl:Class rdf:about="http://standards.iso.org/iso/10303/tech/refdata/core#84cff930-130a-0135-b552-598f1b1392ae">
        <rdfs:subClassOf rdf:resource="http://standards.iso.org/iso/10303/tech/refdata/core#68242b94-82e8-4841-8005-89981113e22f"/>
        <dc:contributor>STEP Harmonization Team</dc:contributor>
        <dc:creator>Phil Spiby, Eurostep</dc:creator>
        <dc:date>2022-09-01</dc:date>
        <dc:source>ISO/TS 10303-4000</dc:source>
        <dc:type>InWork</dc:type>
        <rdfs:comment xml:lang="en">An Address is a type of Locator specified using the information necessary for communicating, using one or more communication methods.</rdfs:comment>
        <owl:versionInfo>1</owl:versionInfo>
        <skos:changeNote>[2021-07-30] Initial definition.</skos:changeNote>
        <skos:prefLabel xml:lang="en">address</skos:prefLabel>
    </owl:Class>
    


    <!-- http://standards.iso.org/iso/10303/tech/refdata/core#84099bf0-130a-0135-b552-598f1b1392ae -->

    <owl:Class rdf:about="http://standards.iso.org/iso/10303/tech/refdata/core#84099bf0-130a-0135-b552-598f1b1392ae">
        <rdfs:subClassOf rdf:resource="http://standards.iso.org/iso/10303/tech/refdata/core#59b11220-3279-0135-b58f-598f1b1392ae"/>
        <dc:contributor>STEP Harmonization Team</dc:contributor>
        <dc:creator>Phil Spiby, Eurostep</dc:creator>
        <dc:date>2022-09-01</dc:date>
        <dc:source>ISO/TS 10303-4000</dc:source>
        <dc:type>InWork</dc:type>
        <rdfs:comment xml:lang="en">An ActivityMethodRelationship is a relationship between two ActivityMethod objects.</rdfs:comment>
        <owl:versionInfo>2</owl:versionInfo>
        <skos:changeNote>[2021-07-30] Initial definition.</skos:changeNote>
        <skos:changeNote>[2022-09-01] Phil Spiby, Eurostep: updated comment.</skos:changeNote>
        <skos:prefLabel xml:lang="en">activity method relationship</skos:prefLabel>
    </owl:Class>
    


    <!-- http://standards.iso.org/iso/10303/tech/refdata/core#842a94a5-1644-46d1-af3f-98c39137b3ae -->

    <owl:Class rdf:about="http://standards.iso.org/iso/10303/tech/refdata/core#842a94a5-1644-46d1-af3f-98c39137b3ae">
        <rdfs:subClassOf rdf:resource="http://standards.iso.org/iso/10303/tech/refdata/core#7c6a9a4b-dfd4-4412-9d67-ee16e3510837"/>
        <dc:contributor>STEP Harmonization Team</dc:contributor>
        <dc:creator>Jean Brangé, AFNeT Services</dc:creator>
        <dc:date>2023-10-04</dc:date>
        <dc:source>ISO/TS 10303-4000</dc:source>
        <dc:type>InWork</dc:type>
        <rdfs:comment xml:lang="en">A Nominal3dEdge is a type of Nominal3dIntegralFeature that represents a three-dimensional nominal integral feature that is an edge.</rdfs:comment>
        <owl:versionInfo>3</owl:versionInfo>
        <skos:changeNote>[2023-10-04] Jean Brangé, AFNeT Services: Initial definition.</skos:changeNote>
        <skos:prefLabel xml:lang="en">nominal3d edge</skos:prefLabel>
    </owl:Class>
    


    <!-- http://standards.iso.org/iso/10303/tech/refdata/core#844b38d0-130a-0135-b552-598f1b1392ae -->

    <owl:Class rdf:about="http://standards.iso.org/iso/10303/tech/refdata/core#844b38d0-130a-0135-b552-598f1b1392ae">
        <rdfs:subClassOf rdf:resource="http://standards.iso.org/iso/10303/tech/refdata/core#59b11220-3279-0135-b58f-598f1b1392ae"/>
        <dc:contributor>STEP Harmonization Team</dc:contributor>
        <dc:creator>Phil Spiby, Eurostep</dc:creator>
        <dc:date>2022-09-01</dc:date>
        <dc:source>ISO/TS 10303-4000</dc:source>
        <dc:type>InWork</dc:type>
        <rdfs:comment xml:lang="en">An ActivityRelationship is a relationship between two Activity objects.</rdfs:comment>
        <owl:versionInfo>2</owl:versionInfo>
        <skos:changeNote>[2021-07-30] Initial definition.</skos:changeNote>
        <skos:changeNote>[2022-09-01] Phil Spiby, Eurostep: updated example.</skos:changeNote>
        <skos:example xml:lang="en">The activity required to complete a work order, can be decomposed into a series of activities. Their corresponding instances would be related using instances of the ActivityRelationship entity.</skos:example>
        <skos:prefLabel xml:lang="en">activity relationship</skos:prefLabel>
    </owl:Class>
    


    <!-- http://standards.iso.org/iso/10303/tech/refdata/core#84853490-130a-0135-b552-598f1b1392ae -->

    <owl:Class rdf:about="http://standards.iso.org/iso/10303/tech/refdata/core#84853490-130a-0135-b552-598f1b1392ae">
        <rdfs:subClassOf rdf:resource="http://standards.iso.org/iso/10303/tech/refdata/core#8276c6f0-130a-0135-b552-598f1b1392ae"/>
        <dc:contributor>STEP Harmonization Team</dc:contributor>
        <dc:creator>Phil Spiby, Eurostep</dc:creator>
        <dc:date>2022-09-01</dc:date>
        <dc:source>ISO/TS 10303-4000</dc:source>
        <dc:type>InWork</dc:type>
        <rdfs:comment xml:lang="en">An ActualActivity is a type of Activity that is a record of the occurrence of an Activity taking place. The ActualActivity can be related through an ActivityHappeningRelationship to the PlannedActivity of which it is an occurrence. The existence of an ActualActivity instance means that the ActualActivity has commenced.</rdfs:comment>
        <owl:versionInfo>2</owl:versionInfo>
        <skos:changeNote>[2021-07-30] Initial definition.</skos:changeNote>
        <skos:changeNote>[2022-09-01] Phil Spiby, Eurostep: updated comment.</skos:changeNote>
        <skos:example xml:lang="en">The replacement of the tyres of my bicycle, frame number ZH002342, on October 25, 2011.</skos:example>
        <skos:prefLabel xml:lang="en">actual activity</skos:prefLabel>
    </owl:Class>
    


    <!-- http://standards.iso.org/iso/10303/tech/refdata/core#85c10ff0-130a-0135-b552-598f1b1392ae -->

    <owl:Class rdf:about="http://standards.iso.org/iso/10303/tech/refdata/core#85c10ff0-130a-0135-b552-598f1b1392ae">
        <rdfs:subClassOf rdf:resource="http://standards.iso.org/iso/10303/tech/refdata/core#8a785670-130a-0135-b552-598f1b1392ae"/>
        <dc:contributor>STEP Harmonization Team</dc:contributor>
        <dc:creator>Phil Spiby, Eurostep</dc:creator>
        <dc:date>2022-09-01</dc:date>
        <dc:source>ISO/TS 10303-4000</dc:source>
        <dc:type>InWork</dc:type>
        <rdfs:comment xml:lang="en">An AlternativeSolution is an object that identifies one of potentially many mutually exclusive implementations of a BreakdownElement.</rdfs:comment>
        <owl:versionInfo>1</owl:versionInfo>
        <skos:changeNote>[2021-07-30] Initial definition.</skos:changeNote>
        <skos:prefLabel xml:lang="en">alternative solution</skos:prefLabel>
    </owl:Class>
    


    <!-- http://standards.iso.org/iso/10303/tech/refdata/core#85d64572-a48f-44d2-89a9-3ed1809fe8e0 -->

    <owl:Class rdf:about="http://standards.iso.org/iso/10303/tech/refdata/core#85d64572-a48f-44d2-89a9-3ed1809fe8e0">
        <rdfs:subClassOf rdf:resource="http://standards.iso.org/iso/10303/tech/refdata/core#1cfca290-3279-0135-b58f-598f1b1392ae"/>
        <dc:contributor>STEP Harmonization Team</dc:contributor>
        <dc:creator>Phil Spiby, Eurostep</dc:creator>
        <dc:date>2022-09-01</dc:date>
        <dc:source>ISO/TS 10303-4000</dc:source>
        <dc:type>InWork</dc:type>
        <rdfs:comment xml:lang="en">A RiskImpactAssignment is an assignment of an item that might be impacted by the risk occurring to the associated RiskConsequence. The meaning of the assignment can be specified using the ClassifiedAs attribute inherited from the AssignmentObject.</rdfs:comment>
        <owl:versionInfo>1</owl:versionInfo>
        <skos:changeNote>[2022-09-01] Initial definition.</skos:changeNote>
        <skos:prefLabel xml:lang="en">risk impact assignment</skos:prefLabel>
    </owl:Class>
    


    <!-- http://standards.iso.org/iso/10303/tech/refdata/core#854f6570-2cd0-4c4e-8d29-d87bc1a0fbf0 -->

    <owl:Class rdf:about="http://standards.iso.org/iso/10303/tech/refdata/core#854f6570-2cd0-4c4e-8d29-d87bc1a0fbf0">
        <rdfs:subClassOf rdf:resource="http://standards.iso.org/iso/10303/tech/refdata/core#ceb138fc-fefc-4b1c-adcc-a7b54167744c"/>
        <dc:contributor>STEP Harmonization Team</dc:contributor>
        <dc:creator>Phil Spiby, Eurostep</dc:creator>
        <dc:date>2022-09-01</dc:date>
        <dc:source>ISO/TS 10303-4000</dc:source>
        <dc:type>InWork</dc:type>
        <rdfs:comment xml:lang="en">An ObservedEnvironment is a specialization of Environment that represents a record of observations about the environment in which a product is or has been operating.</rdfs:comment>
        <owl:versionInfo>1</owl:versionInfo>
        <skos:changeNote>[2021-07-30] Initial definition.</skos:changeNote>
        <skos:prefLabel xml:lang="en">observed environment</skos:prefLabel>
    </owl:Class>
    


    <!-- http://standards.iso.org/iso/10303/tech/refdata/core#85564030-130a-0135-b552-598f1b1392ae -->

    <owl:Class rdf:about="http://standards.iso.org/iso/10303/tech/refdata/core#85564030-130a-0135-b552-598f1b1392ae">
        <rdfs:subClassOf rdf:resource="http://standards.iso.org/iso/10303/tech/refdata/core#1cfca290-3279-0135-b58f-598f1b1392ae"/>
        <dc:contributor>STEP Harmonization Team</dc:contributor>
        <dc:creator>Phil Spiby, Eurostep</dc:creator>
        <dc:date>2022-09-01</dc:date>
        <dc:source>ISO/TS 10303-4000</dc:source>
        <dc:type>InWork</dc:type>
        <rdfs:comment xml:lang="en">An AddressAssignment is an assignment of an Address to an item (specified by PersonOrganizationSelect).</rdfs:comment>
        <owl:versionInfo>1</owl:versionInfo>
        <skos:changeNote>[2021-07-30] Initial definition.</skos:changeNote>
        <skos:prefLabel xml:lang="en">address assignment</skos:prefLabel>
    </owl:Class>
    


    <!-- http://standards.iso.org/iso/10303/tech/refdata/core#8580c636-b115-4fdc-af16-fa090a9ed0fb -->

    <owl:Class rdf:about="http://standards.iso.org/iso/10303/tech/refdata/core#8580c636-b115-4fdc-af16-fa090a9ed0fb">
        <rdfs:subClassOf rdf:resource="http://standards.iso.org/iso/10303/tech/refdata/core#55105ef0-713f-409a-8306-fd8708d4ee3f"/>
        <dc:contributor>STEP Harmonization Team</dc:contributor>
        <dc:creator>Jean Brangé, AFNeT Services</dc:creator>
        <dc:date>2023-10-04</dc:date>
        <dc:source>ISO/TS 10303-4000</dc:source>
        <dc:type>InWork</dc:type>
        <rdfs:comment xml:lang="en">A LineProfileTolerance is a type of GeometricTolerance that specifies the definition of a uniform boundary along the true profile within which the elements of the toleranced surface shall lie. The tolerance zone established by a LineProfileTolerance is two-dimensional. Unless otherwise specified, the rules governing profile tolerance defined in ISO 1101 shall apply.</rdfs:comment>
        <owl:versionInfo>3</owl:versionInfo>
        <skos:changeNote>[2023-10-04] Jean Brangé, AFNeT Services: Initial definition.</skos:changeNote>
        <skos:note xml:lang="en">Alternatively profile tolerance of a line can be used according to the specifications given in ASME Y14.5-2009.</skos:note>
        <skos:prefLabel xml:lang="en">line profile tolerance</skos:prefLabel>
    </owl:Class>
    


    <!-- http://standards.iso.org/iso/10303/tech/refdata/core#859c70f0-130a-0135-b552-598f1b1392ae -->

    <owl:Class rdf:about="http://standards.iso.org/iso/10303/tech/refdata/core#859c70f0-130a-0135-b552-598f1b1392ae">
        <rdfs:subClassOf rdf:resource="http://standards.iso.org/iso/10303/tech/refdata/core#b1611f60-130a-0135-b552-598f1b1392ae"/>
        <dc:contributor>STEP Harmonization Team</dc:contributor>
        <dc:creator>Phil Spiby, Eurostep</dc:creator>
        <dc:date>2022-09-01</dc:date>
        <dc:source>ISO/TS 10303-4000</dc:source>
        <dc:type>InWork</dc:type>
        <rdfs:comment xml:lang="en">An AlternatePartRelationship is a type of PartRelationship where the relating part represents the base part and the related part represents the alternate part. It specifies that any version of the alternate part, can be used in place of any version of the base part, regardless of its usages and of its versions. The relationship established by the AlternatePartRelationship is not symmetric: if part B is an alternate part for part A, part A is not implied to be an alternate part for part B.</rdfs:comment>
        <owl:versionInfo>2</owl:versionInfo>
        <skos:changeNote>[2021-07-30] Initial definition.</skos:changeNote>
        <skos:changeNote>[2022-09-01] Phil Spiby, Eurostep: updated comment updated note.</skos:changeNote>
        <skos:example xml:lang="en">Two bolts of the same size are parts. One bolt has a square head and the other has a hexagonal head. The two bolts are considered equivalent with respect to form, fit, and function: they both have sufficiently close physical shape, they take up the same space when used, and they both serve to fasten two things together. Thus, one of these two bolts could be considered to be an alternate part for the other bolt.</skos:example>
        <skos:note xml:lang="en">An AlternatePartRelationship can relate parts of any kind, provided both related Part objects identify parts of the same part category.</skos:note>
        <skos:note xml:lang="en">An AlternatePartRelationship for which the base part is an assembly involves that the entire part structure of the alternate part can be used in place of the base part and its part structure.</skos:note>
        <skos:note xml:lang="en">An organization can track design changes for a base part and establish effectivity conditions for the use of that base part in various assemblies to be manufactured. The use of an alternate part implies that an organization does not specify any specific version of the alternate part nor establish effectivities relating to it.</skos:note>
        <skos:note xml:lang="en">If a part is an alternate for another part, it is understood that there is no interest in keeping track of which part, the base or any alternates specified, is used as a specific instance of the base part within a part structure.</skos:note>
        <skos:note xml:lang="en">This concept usually refers to form, fit, function, and quality. Additional properties such as performance, noise, endurance, or reliability can also be considered as a prerequisite for the replacement.</skos:note>
        <skos:prefLabel xml:lang="en">alternate part relationship</skos:prefLabel>
    </owl:Class>
    


    <!-- http://standards.iso.org/iso/10303/tech/refdata/core#86b3ad50-130a-0135-b552-598f1b1392ae -->

    <owl:Class rdf:about="http://standards.iso.org/iso/10303/tech/refdata/core#86b3ad50-130a-0135-b552-598f1b1392ae">
        <rdfs:subClassOf rdf:resource="http://standards.iso.org/iso/10303/tech/refdata/core#1cfca290-3279-0135-b58f-598f1b1392ae"/>
        <dc:contributor>STEP Harmonization Team</dc:contributor>
        <dc:creator>Phil Spiby, Eurostep</dc:creator>
        <dc:date>2022-09-01</dc:date>
        <dc:source>ISO/TS 10303-4000</dc:source>
        <dc:type>InWork</dc:type>
        <rdfs:comment xml:lang="en">An ApprovalAssignment is an assignment of an Approval to an item (specified by ApprovalAssignmentSelect). The meaning of the assignment can be specified using the ClassifiedAs attribute inherited from the AssignmentObject.</rdfs:comment>
        <owl:versionInfo>2</owl:versionInfo>
        <skos:changeNote>[2021-07-30] Initial definition.</skos:changeNote>
        <skos:changeNote>[2022-09-01] Phil Spiby, Eurostep: updated comment.</skos:changeNote>
        <skos:prefLabel xml:lang="en">approval assignment</skos:prefLabel>
    </owl:Class>
    


    <!-- http://standards.iso.org/iso/10303/tech/refdata/core#86f3c390-130a-0135-b552-598f1b1392ae -->

    <owl:Class rdf:about="http://standards.iso.org/iso/10303/tech/refdata/core#86f3c390-130a-0135-b552-598f1b1392ae">
        <rdfs:subClassOf rdf:resource="http://standards.iso.org/iso/10303/tech/refdata/core#59b11220-3279-0135-b58f-598f1b1392ae"/>
        <dc:contributor>STEP Harmonization Team</dc:contributor>
        <dc:creator>Phil Spiby, Eurostep</dc:creator>
        <dc:date>2022-09-01</dc:date>
        <dc:source>ISO/TS 10303-4000</dc:source>
        <dc:type>InWork</dc:type>
        <rdfs:comment xml:lang="en">An ApprovalRelationship is a relationship between two Approval objects.</rdfs:comment>
        <owl:versionInfo>2</owl:versionInfo>
        <skos:changeNote>[2021-07-30] Initial definition.</skos:changeNote>
        <skos:changeNote>[2022-09-01] Phil Spiby, Eurostep: updated comment.</skos:changeNote>
        <skos:prefLabel xml:lang="en">approval relationship</skos:prefLabel>
    </owl:Class>
    


    <!-- http://standards.iso.org/iso/10303/tech/refdata/core#8659a670-130a-0135-b552-598f1b1392ae -->

    <owl:Class rdf:about="http://standards.iso.org/iso/10303/tech/refdata/core#8659a670-130a-0135-b552-598f1b1392ae">
        <rdfs:subClassOf rdf:resource="http://standards.iso.org/iso/10303/tech/refdata/core#STEPThing"/>
        <dc:contributor>STEP Harmonization Team</dc:contributor>
        <dc:creator>Phil Spiby, Eurostep</dc:creator>
        <dc:date>2022-09-01</dc:date>
        <dc:source>ISO/TS 10303-4000</dc:source>
        <dc:type>InWork</dc:type>
        <rdfs:comment xml:lang="en">An ApplicationDomain is an identification of the applications for which an object can be relevant.</rdfs:comment>
        <owl:versionInfo>2</owl:versionInfo>
        <skos:changeNote>[2021-07-30] Initial definition.</skos:changeNote>
        <skos:changeNote>[2022-09-01] Phil Spiby, Eurostep: updated comment.</skos:changeNote>
        <skos:prefLabel xml:lang="en">application domain</skos:prefLabel>
    </owl:Class>
    


    <!-- http://standards.iso.org/iso/10303/tech/refdata/core#866a6f50-130a-0135-b552-598f1b1392ae -->

    <owl:Class rdf:about="http://standards.iso.org/iso/10303/tech/refdata/core#866a6f50-130a-0135-b552-598f1b1392ae">
        <rdfs:subClassOf rdf:resource="http://standards.iso.org/iso/10303/tech/refdata/core#STEPThing"/>
        <dc:contributor>STEP Harmonization Team</dc:contributor>
        <dc:creator>Phil Spiby, Eurostep</dc:creator>
        <dc:date>2022-09-01</dc:date>
        <dc:source>ISO/TS 10303-4000</dc:source>
        <dc:type>InWork</dc:type>
        <rdfs:comment xml:lang="en">An Approval is a judgement and formal confirmation of the quality of those product or activity data that are subject of the Approval. An Approval represents a statement made by technical personnel or management personnel whether certain requirements are met. The absence of approval information does not imply any approval status by default.</rdfs:comment>
        <owl:versionInfo>2</owl:versionInfo>
        <skos:changeNote>[2021-07-30] Initial definition.</skos:changeNote>
        <skos:changeNote>[2022-09-01] Phil Spiby, Eurostep: updated note.</skos:changeNote>
        <skos:note xml:lang="en">Approval purposes are defined within a given life-cycle stage view and are typically dependent upon the approval cycles within an individual business process. For each defined purpose, generally there is a defined sequence of values for the status, usually leading towards the status value &apos;approved&apos; indicating achievement of the specific purpose.</skos:note>
        <skos:prefLabel xml:lang="en">approval</skos:prefLabel>
    </owl:Class>
    


    <!-- http://standards.iso.org/iso/10303/tech/refdata/core#869768b5-cb81-4f50-94b0-31e7ef028016 -->

    <owl:Class rdf:about="http://standards.iso.org/iso/10303/tech/refdata/core#869768b5-cb81-4f50-94b0-31e7ef028016">
        <rdfs:subClassOf rdf:resource="http://standards.iso.org/iso/10303/tech/refdata/core#b44098a0-130a-0135-b552-598f1b1392ae"/>
        <dc:contributor>STEP Harmonization Team</dc:contributor>
        <dc:creator>Jean Brangé, AFNeT Services</dc:creator>
        <dc:date>2023-10-04</dc:date>
        <dc:source>ISO/TS 10303-4000</dc:source>
        <dc:type>InWork</dc:type>
        <rdfs:comment xml:lang="en">A ProcessStateRelationship is a type of PartViewRelationship that is a relationship between two PartView objects where the Relating PartView is an in-process-item definition of a specific version of a Part. It characterizes a state of the PartVersion that occurs before the state identified by the Related PartView.</rdfs:comment>
        <owl:versionInfo>3</owl:versionInfo>
        <skos:changeNote>[2023-10-04] Jean Brangé, AFNeT Services: Initial definition.</skos:changeNote>
        <skos:note xml:lang="en">A ProcessStateRelationship may be used to characterize intermediate states of the PartVersion, if this PartVersion is one of the produced outputs of a ProcessPlan.</skos:note>
        <skos:prefLabel xml:lang="en">process state relationship</skos:prefLabel>
    </owl:Class>
    


    <!-- http://standards.iso.org/iso/10303/tech/refdata/core#87a4c410-130a-0135-b552-598f1b1392ae -->

    <owl:Class rdf:about="http://standards.iso.org/iso/10303/tech/refdata/core#87a4c410-130a-0135-b552-598f1b1392ae">
        <rdfs:subClassOf rdf:resource="http://standards.iso.org/iso/10303/tech/refdata/core#59b11220-3279-0135-b58f-598f1b1392ae"/>
        <dc:contributor>STEP Harmonization Team</dc:contributor>
        <dc:creator>Phil Spiby, Eurostep</dc:creator>
        <dc:date>2022-09-01</dc:date>
        <dc:source>ISO/TS 10303-4000</dc:source>
        <dc:type>InWork</dc:type>
        <rdfs:comment xml:lang="en">An AssemblyOccurrenceRelationshipSubstitution is a relationship that indicates that one AssemblyOccurrenceRelationship can be substituted for another AssemblyOccurrenceRelationship. The subjects of the substitution are the related Occurrence objects of both AssemblyOccurrenceRelationship objects. The Relating AssemblyDefinition shall be the same in both AssemblyOccurrenceRelationship objects.</rdfs:comment>
        <owl:versionInfo>2</owl:versionInfo>
        <skos:changeNote>[2021-07-30] Initial definition.</skos:changeNote>
        <skos:changeNote>[2022-09-01] Phil Spiby, Eurostep: updated comment.</skos:changeNote>
        <skos:prefLabel xml:lang="en">assembly occurrence relationship substitution</skos:prefLabel>
    </owl:Class>
    


    <!-- http://standards.iso.org/iso/10303/tech/refdata/core#87e353b0-130a-0135-b552-598f1b1392ae -->

    <owl:Class rdf:about="http://standards.iso.org/iso/10303/tech/refdata/core#87e353b0-130a-0135-b552-598f1b1392ae">
        <rdfs:subClassOf rdf:resource="http://standards.iso.org/iso/10303/tech/refdata/core#STEPThing"/>
        <dc:contributor>STEP Harmonization Team</dc:contributor>
        <dc:creator>Phil Spiby, Eurostep</dc:creator>
        <dc:date>2022-09-01</dc:date>
        <dc:source>ISO/TS 10303-4000</dc:source>
        <dc:type>InWork</dc:type>
        <rdfs:comment xml:lang="en">An AssemblyRealizationContext is an association between an individual assembly and its design (specified by AssemblyDesignSelect).</rdfs:comment>
        <owl:versionInfo>2</owl:versionInfo>
        <skos:changeNote>[2021-07-30] Initial definition.</skos:changeNote>
        <skos:changeNote>[2022-09-01] Phil Spiby, Eurostep: updated comment.</skos:changeNote>
        <skos:prefLabel xml:lang="en">assembly realization context</skos:prefLabel>
    </owl:Class>
    


    <!-- http://standards.iso.org/iso/10303/tech/refdata/core#875b871a-25c1-4e6d-bdcc-b413e99f5998 -->

    <owl:Class rdf:about="http://standards.iso.org/iso/10303/tech/refdata/core#875b871a-25c1-4e6d-bdcc-b413e99f5998">
        <rdfs:subClassOf rdf:resource="http://standards.iso.org/iso/10303/tech/refdata/core#1d59c650-3279-0135-b58f-598f1b1392ae"/>
        <dc:contributor>STEP Harmonization Team</dc:contributor>
        <dc:creator>Phil Spiby, Eurostep</dc:creator>
        <dc:date>2022-09-01</dc:date>
        <dc:source>ISO/TS 10303-4000</dc:source>
        <dc:type>InWork</dc:type>
        <rdfs:comment xml:lang="en">An InterfaceConnectionToDefinitionAssociation is an association between an InterfaceConnection and an InterfaceDefinitionConnection that represents the definition.</rdfs:comment>
        <owl:versionInfo>2</owl:versionInfo>
        <skos:changeNote>[2021-07-30] Initial definition.</skos:changeNote>
        <skos:changeNote>[2022-09-01] Phil Spiby, Eurostep: updated comment.</skos:changeNote>
        <skos:prefLabel xml:lang="en">interface connection to definition association</skos:prefLabel>
    </owl:Class>
    


    <!-- http://standards.iso.org/iso/10303/tech/refdata/core#87556b90-130a-0135-b552-598f1b1392ae -->

    <owl:Class rdf:about="http://standards.iso.org/iso/10303/tech/refdata/core#87556b90-130a-0135-b552-598f1b1392ae">
        <rdfs:subClassOf rdf:resource="http://standards.iso.org/iso/10303/tech/refdata/core#b3911ec0-130a-0135-b552-598f1b1392ae"/>
        <dc:contributor>STEP Harmonization Team</dc:contributor>
        <dc:creator>Phil Spiby, Eurostep</dc:creator>
        <dc:date>2022-09-01</dc:date>
        <dc:source>ISO/TS 10303-4000</dc:source>
        <dc:type>InWork</dc:type>
        <rdfs:comment xml:lang="en">An AssemblyDefinition is a type of PartView that is a definition of a PartVersion that contains other subordinate components.</rdfs:comment>
        <owl:versionInfo>1</owl:versionInfo>
        <skos:changeNote>[2021-07-30] Initial definition.</skos:changeNote>
        <skos:prefLabel xml:lang="en">assembly definition</skos:prefLabel>
    </owl:Class>
    


    <!-- http://standards.iso.org/iso/10303/tech/refdata/core#8768f395-4d2c-4d62-85b3-4de1f1240458 -->

    <owl:Class rdf:about="http://standards.iso.org/iso/10303/tech/refdata/core#8768f395-4d2c-4d62-85b3-4de1f1240458">
        <rdfs:subClassOf rdf:resource="http://standards.iso.org/iso/10303/tech/refdata/core#1cfca290-3279-0135-b58f-598f1b1392ae"/>
        <dc:contributor>STEP Harmonization Team</dc:contributor>
        <dc:creator>Phil Spiby, Eurostep</dc:creator>
        <dc:date>2022-09-01</dc:date>
        <dc:source>ISO/TS 10303-4000</dc:source>
        <dc:type>InWork</dc:type>
        <rdfs:comment xml:lang="en">A JustificationAssignment is an assignment of a Justification to an item (specified by JustificationAssignmentSelect). The meaning of the assignment can be specified using the ClassifiedAs attribute inherited from the AssignmentObject.</rdfs:comment>
        <owl:versionInfo>2</owl:versionInfo>
        <skos:changeNote>[2021-07-30] Initial definition.</skos:changeNote>
        <skos:changeNote>[2022-09-01] Phil Spiby, Eurostep: updated comment updated example updated note.</skos:changeNote>
        <skos:note xml:lang="en">The item can be an activity or a product design.</skos:note>
        <skos:prefLabel xml:lang="en">justification assignment</skos:prefLabel>
    </owl:Class>
    


    <!-- http://standards.iso.org/iso/10303/tech/refdata/core#87863f90-130a-0135-b552-598f1b1392ae -->

    <owl:Class rdf:about="http://standards.iso.org/iso/10303/tech/refdata/core#87863f90-130a-0135-b552-598f1b1392ae">
        <rdfs:subClassOf rdf:resource="http://standards.iso.org/iso/10303/tech/refdata/core#d80a2030-130a-0135-b552-598f1b1392ae"/>
        <dc:contributor>STEP Harmonization Team</dc:contributor>
        <dc:creator>Phil Spiby, Eurostep</dc:creator>
        <dc:date>2022-09-01</dc:date>
        <dc:source>ISO/TS 10303-4000</dc:source>
        <dc:type>InWork</dc:type>
        <rdfs:comment xml:lang="en">An AssemblyOccurrenceRelationship is a relationship between an AssemblyDefinition and a DefinitionBasedOccurrence representing a constituent of the assembly. The AssemblyDefinition and the PartView that serves as &apos;definition&apos; of the DefinitionBasedOccurrence shall share at least one ViewContext. An AssemblyOccurrenceRelationship is a type of ViewOccurrenceRelationship. Each AssemblyOccurrenceRelationship is a NextAssemblyOccurrenceUsage or a PromissoryAssemblyOccurrenceUsage.</rdfs:comment>
        <owl:versionInfo>2</owl:versionInfo>
        <skos:changeNote>[2021-07-30] Initial definition.</skos:changeNote>
        <skos:changeNote>[2022-09-01] Phil Spiby, Eurostep: updated comment updated note.</skos:changeNote>
        <skos:note xml:lang="en">The constituent can also be an assembly.</skos:note>
        <skos:prefLabel xml:lang="en">assembly occurrence relationship</skos:prefLabel>
    </owl:Class>
    


    <!-- http://standards.iso.org/iso/10303/tech/refdata/core#8792b992-6e58-4cf2-8d3e-2e9dee39fc52 -->

    <owl:Class rdf:about="http://standards.iso.org/iso/10303/tech/refdata/core#8792b992-6e58-4cf2-8d3e-2e9dee39fc52">
        <rdfs:subClassOf rdf:resource="http://standards.iso.org/iso/10303/tech/refdata/core#59b11220-3279-0135-b58f-598f1b1392ae"/>
        <dc:contributor>STEP Harmonization Team</dc:contributor>
        <dc:creator>Phil Spiby, Eurostep</dc:creator>
        <dc:date>2022-09-01</dc:date>
        <dc:source>ISO/TS 10303-4000</dc:source>
        <dc:type>InWork</dc:type>
        <rdfs:comment xml:lang="en">A StateDefinitionStateAssociationRelationship is a relationship between two StateDefinitionStateAssociation objects.</rdfs:comment>
        <owl:versionInfo>2</owl:versionInfo>
        <skos:changeNote>[2021-07-30] Initial definition.</skos:changeNote>
        <skos:changeNote>[2022-09-01] Phil Spiby, Eurostep: updated comment.</skos:changeNote>
        <skos:prefLabel xml:lang="en">state definition state association relationship</skos:prefLabel>
    </owl:Class>
    


    <!-- http://standards.iso.org/iso/10303/tech/refdata/core#88035ed0-130a-0135-b552-598f1b1392ae -->

    <owl:Class rdf:about="http://standards.iso.org/iso/10303/tech/refdata/core#88035ed0-130a-0135-b552-598f1b1392ae">
        <rdfs:subClassOf rdf:resource="http://standards.iso.org/iso/10303/tech/refdata/core#b44098a0-130a-0135-b552-598f1b1392ae"/>
        <dc:contributor>STEP Harmonization Team</dc:contributor>
        <dc:creator>Phil Spiby, Eurostep</dc:creator>
        <dc:date>2022-09-01</dc:date>
        <dc:source>ISO/TS 10303-4000</dc:source>
        <dc:type>InWork</dc:type>
        <rdfs:comment xml:lang="en">An AssemblyViewRelationship is the relationship between an AssemblyDefinition and a PartView representing a view of the assembly. An AssemblyViewRelationship is a type of PartViewRelationship. The AssemblyDefinition and the PartView shall share at least one ViewContext.</rdfs:comment>
        <owl:versionInfo>2</owl:versionInfo>
        <skos:changeNote>[2021-07-30] Initial definition.</skos:changeNote>
        <skos:changeNote>[2022-09-01] Phil Spiby, Eurostep: updated comment.</skos:changeNote>
        <skos:prefLabel xml:lang="en">assembly view relationship</skos:prefLabel>
    </owl:Class>
    


    <!-- http://standards.iso.org/iso/10303/tech/refdata/core#8835b970-130a-0135-b552-598f1b1392ae -->

    <owl:Class rdf:about="http://standards.iso.org/iso/10303/tech/refdata/core#8835b970-130a-0135-b552-598f1b1392ae">
        <rdfs:subClassOf rdf:resource="http://standards.iso.org/iso/10303/tech/refdata/core#59b11220-3279-0135-b58f-598f1b1392ae"/>
        <dc:contributor>STEP Harmonization Team</dc:contributor>
        <dc:creator>Phil Spiby, Eurostep</dc:creator>
        <dc:date>2022-09-01</dc:date>
        <dc:source>ISO/TS 10303-4000</dc:source>
        <dc:type>InWork</dc:type>
        <rdfs:comment xml:lang="en">An AssemblyViewRelationshipSubstitution is a relationship that indicates that one AssemblyViewRelationship can be substituted for another AssemblyViewRelationship. The subjects of the substitution are the related Occurrence objects of both AssemblyViewRelationship objects. The Relating AssemblyDefinition shall be the same in both AssemblyViewRelationship objects.</rdfs:comment>
        <owl:versionInfo>2</owl:versionInfo>
        <skos:changeNote>[2021-07-30] Initial definition.</skos:changeNote>
        <skos:changeNote>[2022-09-01] Phil Spiby, Eurostep: updated comment.</skos:changeNote>
        <skos:prefLabel xml:lang="en">assembly view relationship substitution</skos:prefLabel>
    </owl:Class>
    


    <!-- http://standards.iso.org/iso/10303/tech/refdata/core#88744910-130a-0135-b552-598f1b1392ae -->

    <owl:Class rdf:about="http://standards.iso.org/iso/10303/tech/refdata/core#88744910-130a-0135-b552-598f1b1392ae">
        <rdfs:subClassOf rdf:resource="http://standards.iso.org/iso/10303/tech/refdata/core#59b11220-3279-0135-b58f-598f1b1392ae"/>
        <dc:contributor>STEP Harmonization Team</dc:contributor>
        <dc:creator>Phil Spiby, Eurostep</dc:creator>
        <dc:date>2022-09-01</dc:date>
        <dc:source>ISO/TS 10303-4000</dc:source>
        <dc:type>InWork</dc:type>
        <rdfs:comment xml:lang="en">An AssignmentObjectRelationship is a relationship between two Assignment objects.</rdfs:comment>
        <owl:versionInfo>2</owl:versionInfo>
        <skos:changeNote>[2021-07-30] Initial definition.</skos:changeNote>
        <skos:changeNote>[2022-09-01] Phil Spiby, Eurostep: updated comment.</skos:changeNote>
        <skos:prefLabel xml:lang="en">assignment object relationship</skos:prefLabel>
    </owl:Class>
    


    <!-- http://standards.iso.org/iso/10303/tech/refdata/core#89f36b81-3d5e-48dd-90fc-80eaf4d96f3e -->

    <owl:Class rdf:about="http://standards.iso.org/iso/10303/tech/refdata/core#89f36b81-3d5e-48dd-90fc-80eaf4d96f3e">
        <rdfs:subClassOf rdf:resource="http://standards.iso.org/iso/10303/tech/refdata/core#STEPThing"/>
        <dc:contributor>STEP Harmonization Team</dc:contributor>
        <dc:creator>Phil Spiby, Eurostep</dc:creator>
        <dc:date>2022-09-01</dc:date>
        <dc:source>ISO/TS 10303-4000</dc:source>
        <dc:type>InWork</dc:type>
        <rdfs:comment xml:lang="en">An AnalysisModelObject represents the results of an Analysis.</rdfs:comment>
        <owl:versionInfo>2</owl:versionInfo>
        <skos:changeNote>[2021-07-30] Initial definition.</skos:changeNote>
        <skos:changeNote>[2022-09-01] Phil Spiby, Eurostep: updated note.</skos:changeNote>
        <skos:note xml:lang="en">This entity allows the identification of analysis results. ISO 10303-209 provides capabilities to represent such analysis results.</skos:note>
        <skos:prefLabel xml:lang="en">analysis model object</skos:prefLabel>
    </owl:Class>
    


    <!-- http://standards.iso.org/iso/10303/tech/refdata/core#89f39610-130a-0135-b552-598f1b1392ae -->

    <owl:Class rdf:about="http://standards.iso.org/iso/10303/tech/refdata/core#89f39610-130a-0135-b552-598f1b1392ae">
        <rdfs:subClassOf rdf:resource="http://standards.iso.org/iso/10303/tech/refdata/core#1d59c650-3279-0135-b58f-598f1b1392ae"/>
        <dc:contributor>STEP Harmonization Team</dc:contributor>
        <dc:creator>Phil Spiby, Eurostep</dc:creator>
        <dc:date>2022-09-01</dc:date>
        <dc:source>ISO/TS 10303-4000</dc:source>
        <dc:type>InWork</dc:type>
        <rdfs:comment xml:lang="en">A BreakdownElementRealization is an association between a breakdown element (specified by BreakdownElementWithRealizationSelect) and the item (specified by BreakdownElementRealizationSelect) that realizes that element.</rdfs:comment>
        <owl:versionInfo>2</owl:versionInfo>
        <skos:changeNote>[2021-07-30] Initial definition.</skos:changeNote>
        <skos:changeNote>[2022-09-01] Phil Spiby, Eurostep: updated comment updated example.</skos:changeNote>
        <skos:example xml:lang="en">A pump realizes the &apos;provide fuel to engine&apos; element in a functional breakdown for a ship.</skos:example>
        <skos:prefLabel xml:lang="en">breakdown element realization</skos:prefLabel>
    </owl:Class>
    


    <!-- http://standards.iso.org/iso/10303/tech/refdata/core#89084bb0-130a-0135-b552-598f1b1392ae -->

    <owl:Class rdf:about="http://standards.iso.org/iso/10303/tech/refdata/core#89084bb0-130a-0135-b552-598f1b1392ae">
        <rdfs:subClassOf rdf:resource="http://standards.iso.org/iso/10303/tech/refdata/core#STEPThing"/>
        <dc:contributor>STEP Harmonization Team</dc:contributor>
        <dc:creator>Phil Spiby, Eurostep</dc:creator>
        <dc:date>2022-09-01</dc:date>
        <dc:source>ISO/TS 10303-4000</dc:source>
        <dc:type>InWork</dc:type>
        <rdfs:comment xml:lang="en">A Breakdown is a set of breakdown elements chosen in order to partition a product in a desired way, together with the hierarchical relationships between these breakdown elements. The hierarchical relationships, a parent-child view, is represented by BreakdownElementHierarchy instances relating the elements in the breakdown that are represented by BreakdownElement instances.</rdfs:comment>
        <owl:versionInfo>1</owl:versionInfo>
        <skos:changeNote>[2021-07-30] Initial definition.</skos:changeNote>
        <skos:prefLabel xml:lang="en">breakdown</skos:prefLabel>
    </owl:Class>
    


    <!-- http://standards.iso.org/iso/10303/tech/refdata/core#8958e8e3-abc5-404e-bccc-ab0847100d71 -->

    <owl:Class rdf:about="http://standards.iso.org/iso/10303/tech/refdata/core#8958e8e3-abc5-404e-bccc-ab0847100d71">
        <rdfs:subClassOf rdf:resource="http://standards.iso.org/iso/10303/tech/refdata/core#1cfca290-3279-0135-b58f-598f1b1392ae"/>
        <dc:contributor>STEP Harmonization Team</dc:contributor>
        <dc:creator>Phil Spiby, Eurostep</dc:creator>
        <dc:date>2022-09-01</dc:date>
        <dc:source>ISO/TS 10303-4000</dc:source>
        <dc:type>InWork</dc:type>
        <rdfs:comment xml:lang="en">A LocationAssignment is an assignment of a location to an item (specified by LocationAssignmentSelect). The meaning of the assignment can be specified using the ClassifiedAs attribute inherited from the AssignmentObject.</rdfs:comment>
        <owl:versionInfo>2</owl:versionInfo>
        <skos:changeNote>[2021-07-30] Initial definition.</skos:changeNote>
        <skos:changeNote>[2022-09-01] Phil Spiby, Eurostep: updated comment updated note.</skos:changeNote>
        <skos:note xml:lang="en">There can be distinct assignment for each qualification (planned, scheduled or actual). Each assignment can have a start and end date or time. A location can have multiple assignments.</skos:note>
        <skos:prefLabel xml:lang="en">location assignment</skos:prefLabel>
    </owl:Class>
    


    <!-- http://standards.iso.org/iso/10303/tech/refdata/core#89626e2d-7cb7-439c-aef7-7cec58014c80 -->

    <owl:Class rdf:about="http://standards.iso.org/iso/10303/tech/refdata/core#89626e2d-7cb7-439c-aef7-7cec58014c80">
        <rdfs:subClassOf rdf:resource="http://standards.iso.org/iso/10303/tech/refdata/core#STEPThing"/>
        <dc:contributor>STEP Harmonization Team</dc:contributor>
        <dc:creator>Phil Spiby, Eurostep</dc:creator>
        <dc:date>2022-09-01</dc:date>
        <dc:source>ISO/TS 10303-4000</dc:source>
        <dc:type>InWork</dc:type>
        <rdfs:comment xml:lang="en">An InterfaceSpecificationView provides a view of an InterfaceSpecification.</rdfs:comment>
        <owl:versionInfo>1</owl:versionInfo>
        <skos:changeNote>[2021-07-30] Initial definition.</skos:changeNote>
        <skos:example xml:lang="en">When developing a BSI standard for connecting domestic electrical equipment to the electricity supply, collected comments from experts form a new view on a version of the standard.</skos:example>
        <skos:prefLabel xml:lang="en">interface specification view</skos:prefLabel>
    </owl:Class>
    


    <!-- http://standards.iso.org/iso/10303/tech/refdata/core#8966e670-130a-0135-b552-598f1b1392ae -->

    <owl:Class rdf:about="http://standards.iso.org/iso/10303/tech/refdata/core#8966e670-130a-0135-b552-598f1b1392ae">
        <rdfs:subClassOf rdf:resource="http://standards.iso.org/iso/10303/tech/refdata/core#1d59c650-3279-0135-b58f-598f1b1392ae"/>
        <dc:contributor>STEP Harmonization Team</dc:contributor>
        <dc:creator>Phil Spiby, Eurostep</dc:creator>
        <dc:date>2022-09-01</dc:date>
        <dc:source>ISO/TS 10303-4000</dc:source>
        <dc:type>InWork</dc:type>
        <rdfs:comment xml:lang="en">A BreakdownMember is a membership association between a BreakdownVersion and a member BreakdownElementView.</rdfs:comment>
        <owl:versionInfo>2</owl:versionInfo>
        <skos:changeNote>[2021-07-30] Initial definition.</skos:changeNote>
        <skos:changeNote>[2022-09-01] Phil Spiby, Eurostep: updated comment.</skos:changeNote>
        <skos:prefLabel xml:lang="en">breakdown member</skos:prefLabel>
    </owl:Class>
    


    <!-- http://standards.iso.org/iso/10303/tech/refdata/core#89919ff0-130a-0135-b552-598f1b1392ae -->

    <owl:Class rdf:about="http://standards.iso.org/iso/10303/tech/refdata/core#89919ff0-130a-0135-b552-598f1b1392ae">
        <rdfs:subClassOf rdf:resource="http://standards.iso.org/iso/10303/tech/refdata/core#STEPThing"/>
        <dc:contributor>STEP Harmonization Team</dc:contributor>
        <dc:creator>Phil Spiby, Eurostep</dc:creator>
        <dc:date>2022-09-01</dc:date>
        <dc:source>ISO/TS 10303-4000</dc:source>
        <dc:type>InWork</dc:type>
        <rdfs:comment xml:lang="en">A BreakdownElement is a constituent in one or more Breakdown instances. In such structure a BreakdownElement can play the role of a parent or a child or both.</rdfs:comment>
        <owl:versionInfo>2</owl:versionInfo>
        <skos:changeNote>[2021-07-30] Initial definition.</skos:changeNote>
        <skos:changeNote>[2022-09-01] Phil Spiby, Eurostep: updated comment updated note.</skos:changeNote>
        <skos:note xml:lang="en">A BreakdownElement can be referenced from several Breakdown instances.</skos:note>
        <skos:prefLabel xml:lang="en">breakdown element</skos:prefLabel>
    </owl:Class>
    


    <!-- http://standards.iso.org/iso/10303/tech/refdata/core#9a26ed01-5416-4604-ba20-79712280b5bb -->

    <owl:Class rdf:about="http://standards.iso.org/iso/10303/tech/refdata/core#9a26ed01-5416-4604-ba20-79712280b5bb">
        <rdfs:subClassOf rdf:resource="http://standards.iso.org/iso/10303/tech/refdata/core#8792b992-6e58-4cf2-8d3e-2e9dee39fc52"/>
        <dc:contributor>STEP Harmonization Team</dc:contributor>
        <dc:creator>Phil Spiby, Eurostep</dc:creator>
        <dc:date>2022-09-01</dc:date>
        <dc:source>ISO/TS 10303-4000</dc:source>
        <dc:type>InWork</dc:type>
        <rdfs:comment xml:lang="en">A StateHypothesisToConfirmationRelationship is a relationship representing the fact that a StateObserved (via StateDefinitionHypothesisAssignment) has moved from being hypothesized as conforming to a StateDefinition to being confirmed (via StateDefinitionConfirmedAssignment) as conforming to a StateDefinition.</rdfs:comment>
        <owl:versionInfo>1</owl:versionInfo>
        <skos:changeNote>[2021-07-30] Initial definition.</skos:changeNote>
        <skos:prefLabel xml:lang="en">state hypothesis to confirmation relationship</skos:prefLabel>
    </owl:Class>
    


    <!-- http://standards.iso.org/iso/10303/tech/refdata/core#9a81b562-26a3-474e-bcef-f6e8478d054d -->

    <owl:Class rdf:about="http://standards.iso.org/iso/10303/tech/refdata/core#9a81b562-26a3-474e-bcef-f6e8478d054d">
        <rdfs:subClassOf rdf:resource="http://standards.iso.org/iso/10303/tech/refdata/core#STEPThing"/>
        <dc:contributor>STEP Harmonization Team</dc:contributor>
        <dc:creator>Jean Brangé, AFNeT Services</dc:creator>
        <dc:date>2023-10-04</dc:date>
        <dc:source>ISO/TS 10303-4000</dc:source>
        <dc:type>InWork</dc:type>
        <rdfs:comment xml:lang="en">A DeltaChange is a mechanism to describe changes in product data. It collects the change activities that describe the differences between the two objects referenced by the specified relationship object.</rdfs:comment>
        <owl:versionInfo>3</owl:versionInfo>
        <skos:changeNote>[2023-10-04] Jean Brangé, AFNeT Services: Initial definition.</skos:changeNote>
        <skos:example xml:lang="en">Consider two PartVersion objects A and B which are related by a PartVersionRelationship with ./4_info_reqs_ProductDataManagement.htm#PartVersionRelationship.RelationType RelationType &apos;sequence&apos;. The attribute DescribedChange of DeltaChange references this PartVersionRelationship. The activities leading to the changes between version A and version B are collected by the attribute ChangeActivities.</skos:example>
        <skos:prefLabel xml:lang="en">delta change</skos:prefLabel>
    </owl:Class>
    


    <!-- http://standards.iso.org/iso/10303/tech/refdata/core#9a99abd0-130a-0135-b552-598f1b1392ae -->

    <owl:Class rdf:about="http://standards.iso.org/iso/10303/tech/refdata/core#9a99abd0-130a-0135-b552-598f1b1392ae">
        <rdfs:subClassOf rdf:resource="http://standards.iso.org/iso/10303/tech/refdata/core#STEPThing"/>
        <dc:contributor>STEP Harmonization Team</dc:contributor>
        <dc:creator>Phil Spiby, Eurostep</dc:creator>
        <dc:date>2022-09-01</dc:date>
        <dc:source>ISO/TS 10303-4000</dc:source>
        <dc:type>InWork</dc:type>
        <rdfs:comment xml:lang="en">An Event is the fact of the existence of a state at some point in time.</rdfs:comment>
        <owl:versionInfo>1</owl:versionInfo>
        <skos:changeNote>[2021-07-30] Initial definition.</skos:changeNote>
        <skos:prefLabel xml:lang="en">event</skos:prefLabel>
    </owl:Class>
    


    <!-- http://standards.iso.org/iso/10303/tech/refdata/core#9aa74d8d-d41a-4ff2-9b3f-3800cb0580e2 -->

    <owl:Class rdf:about="http://standards.iso.org/iso/10303/tech/refdata/core#9aa74d8d-d41a-4ff2-9b3f-3800cb0580e2">
        <rdfs:subClassOf rdf:resource="http://standards.iso.org/iso/10303/tech/refdata/core#53e20541-4d83-4902-a059-b807ec6e0f42"/>
        <dc:contributor>STEP Harmonization Team</dc:contributor>
        <dc:creator>Phil Spiby, Eurostep</dc:creator>
        <dc:date>2022-09-01</dc:date>
        <dc:source>ISO/TS 10303-4000</dc:source>
        <dc:type>InWork</dc:type>
        <rdfs:comment xml:lang="en">A StateDefinitionComposition is a type of StateDefinitionRelationship. It relates StateDefinition entities to one another, when two or more Related StateDefinition entities act as parts to compose a whole Relating StateDefinition; and furthermore, whole StateDefinition entities can become parts of yet another whole StateDefinition.</rdfs:comment>
        <owl:versionInfo>2</owl:versionInfo>
        <skos:changeNote>[2021-07-30] Initial definition.</skos:changeNote>
        <skos:changeNote>[2022-09-01] Phil Spiby, Eurostep: updated comment.</skos:changeNote>
        <skos:prefLabel xml:lang="en">state definition composition</skos:prefLabel>
    </owl:Class>
    


    <!-- http://standards.iso.org/iso/10303/tech/refdata/core#9ae0adae-6359-4fc0-9160-35e429d7a380 -->

    <owl:Class rdf:about="http://standards.iso.org/iso/10303/tech/refdata/core#9ae0adae-6359-4fc0-9160-35e429d7a380">
        <rdfs:subClassOf rdf:resource="http://standards.iso.org/iso/10303/tech/refdata/core#STEPThing"/>
        <dc:contributor>STEP Harmonization Team</dc:contributor>
        <dc:creator>Phil Spiby, Eurostep</dc:creator>
        <dc:date>2022-09-01</dc:date>
        <dc:source>ISO/TS 10303-4000</dc:source>
        <dc:type>InWork</dc:type>
        <rdfs:comment xml:lang="en">A ValueFormatTypeQualifier is the specification of the allowed formats for presentation of the string and numeric values that can be associated with a property.</rdfs:comment>
        <owl:versionInfo>2</owl:versionInfo>
        <skos:changeNote>[2021-07-30] Initial definition.</skos:changeNote>
        <skos:changeNote>[2022-09-01] Phil Spiby, Eurostep: updated comment.</skos:changeNote>
        <skos:prefLabel xml:lang="en">value format type qualifier</skos:prefLabel>
    </owl:Class>
    


    <!-- http://standards.iso.org/iso/10303/tech/refdata/core#9aed9830-130a-0135-b552-598f1b1392ae -->

    <owl:Class rdf:about="http://standards.iso.org/iso/10303/tech/refdata/core#9aed9830-130a-0135-b552-598f1b1392ae">
        <rdfs:subClassOf rdf:resource="http://standards.iso.org/iso/10303/tech/refdata/core#1cfca290-3279-0135-b58f-598f1b1392ae"/>
        <dc:contributor>STEP Harmonization Team</dc:contributor>
        <dc:creator>Phil Spiby, Eurostep</dc:creator>
        <dc:date>2022-09-01</dc:date>
        <dc:source>ISO/TS 10303-4000</dc:source>
        <dc:type>InWork</dc:type>
        <rdfs:comment xml:lang="en">An EventAssignment is the assignment of an Event to an item (specified by EventAssignmentSelect).</rdfs:comment>
        <owl:versionInfo>1</owl:versionInfo>
        <skos:changeNote>[2021-07-30] Initial definition.</skos:changeNote>
        <skos:prefLabel xml:lang="en">event assignment</skos:prefLabel>
    </owl:Class>
    


    <!-- http://standards.iso.org/iso/10303/tech/refdata/core#9b461870-130a-0135-b552-598f1b1392ae -->

    <owl:Class rdf:about="http://standards.iso.org/iso/10303/tech/refdata/core#9b461870-130a-0135-b552-598f1b1392ae">
        <rdfs:subClassOf rdf:resource="http://standards.iso.org/iso/10303/tech/refdata/core#59b11220-3279-0135-b58f-598f1b1392ae"/>
        <dc:contributor>STEP Harmonization Team</dc:contributor>
        <dc:creator>Phil Spiby, Eurostep</dc:creator>
        <dc:date>2022-09-01</dc:date>
        <dc:source>ISO/TS 10303-4000</dc:source>
        <dc:type>InWork</dc:type>
        <rdfs:comment xml:lang="en">An EventRelationship is a relationship between two Event objects.</rdfs:comment>
        <owl:versionInfo>2</owl:versionInfo>
        <skos:changeNote>[2021-07-30] Initial definition.</skos:changeNote>
        <skos:changeNote>[2022-09-01] Phil Spiby, Eurostep: updated comment updated example.</skos:changeNote>
        <skos:example xml:lang="en">An instance of this entity data type with RelationType &apos;sequence&apos; can be used to specify that an event shall end before another event starts.</skos:example>
        <skos:prefLabel xml:lang="en">event relationship</skos:prefLabel>
    </owl:Class>
    


    <!-- http://standards.iso.org/iso/10303/tech/refdata/core#9b55c2b7-5397-4cfa-9aa1-a3a6785467b4 -->

    <owl:Class rdf:about="http://standards.iso.org/iso/10303/tech/refdata/core#9b55c2b7-5397-4cfa-9aa1-a3a6785467b4">
        <rdfs:subClassOf rdf:resource="http://standards.iso.org/iso/10303/tech/refdata/core#59b11220-3279-0135-b58f-598f1b1392ae"/>
        <dc:contributor>STEP Harmonization Team</dc:contributor>
        <dc:creator>Jean Brangé, AFNeT Services</dc:creator>
        <dc:date>2023-10-04</dc:date>
        <dc:source>ISO/TS 10303-4000</dc:source>
        <dc:type>InWork</dc:type>
        <rdfs:comment xml:lang="en">A ShapeFeatureDefinitionRelationship is a relationship between two instances of the entity data type ShapeFeatureDefinition and provides an identification and description of this relationship.</rdfs:comment>
        <owl:versionInfo>3</owl:versionInfo>
        <skos:changeNote>[2023-10-04] Jean Brangé, AFNeT Services: Initial definition.</skos:changeNote>
        <skos:prefLabel xml:lang="en">shape feature definition relationship</skos:prefLabel>
    </owl:Class>
    


    <!-- http://standards.iso.org/iso/10303/tech/refdata/core#9bb92a27-6557-48a4-a762-e23918ff4f6c -->

    <owl:Class rdf:about="http://standards.iso.org/iso/10303/tech/refdata/core#9bb92a27-6557-48a4-a762-e23918ff4f6c">
        <rdfs:subClassOf rdf:resource="http://standards.iso.org/iso/10303/tech/refdata/core#STEPThing"/>
        <dc:contributor>STEP Harmonization Team</dc:contributor>
        <dc:creator>Phil Spiby, Eurostep</dc:creator>
        <dc:date>2022-09-01</dc:date>
        <dc:source>ISO/TS 10303-4000</dc:source>
        <dc:type>InWork</dc:type>
        <rdfs:comment xml:lang="en">A Verification is an objective assertion of a claim, that a requirement is satisfied by a specific item represented in a RequirementSatisfactionAssertion, has been verified. Verification is commonly understood to mean the answer to, &apos;Have we built the system right?&apos;. Verification ensures that the specified requirements have been met. Verification uses the methods of Test, Analysis, Inspection, Demonstration, and Similarity.</rdfs:comment>
        <owl:versionInfo>2</owl:versionInfo>
        <skos:changeNote>[2021-07-30] Initial definition.</skos:changeNote>
        <skos:changeNote>[2022-09-01] Phil Spiby, Eurostep: updated comment updated example updated note.</skos:changeNote>
        <skos:example xml:lang="en">A data type used to represent a vehicle&apos;s engine with a power output of 160BHP could be asserted to satisfy a requirement &apos;the vehicle shall have a maximum power output of at least 150BHP&apos;. This assertion can be verified by analysis results on simulations of the engine. In this case the analysis results would be identified in the items collection of an evidence instance, possibly including the approval of the analysis. The Evidence instance would identify that it is used to support the required Verification.</skos:example>
        <skos:note xml:lang="en">It is assumed that meta data supporting the verification will be applied using assignment entities, such as identification assignment, person and organization assignment etc..</skos:note>
        <skos:note xml:lang="en">Just because an item is verified does not ensure that it meets all stakeholder needs or expectations, many of these are never specified, or are of an untestable nature, such as &apos;the car should look sporty&apos;.</skos:note>
        <skos:prefLabel xml:lang="en">verification</skos:prefLabel>
    </owl:Class>
    


    <!-- http://standards.iso.org/iso/10303/tech/refdata/core#9bbd1d30-130a-0135-b552-598f1b1392ae -->

    <owl:Class rdf:about="http://standards.iso.org/iso/10303/tech/refdata/core#9bbd1d30-130a-0135-b552-598f1b1392ae">
        <rdfs:subClassOf rdf:resource="http://standards.iso.org/iso/10303/tech/refdata/core#d237f3d0-130a-0135-b552-598f1b1392ae"/>
        <dc:contributor>STEP Harmonization Team</dc:contributor>
        <dc:creator>Phil Spiby, Eurostep</dc:creator>
        <dc:date>2022-09-01</dc:date>
        <dc:source>ISO/TS 10303-4000</dc:source>
        <dc:type>InWork</dc:type>
        <rdfs:comment xml:lang="en">An ExpandedUncertainty is a type of StandardUncertainty that specifies the factor of an uncertainty.</rdfs:comment>
        <owl:versionInfo>1</owl:versionInfo>
        <skos:changeNote>[2021-07-30] Initial definition.</skos:changeNote>
        <skos:prefLabel xml:lang="en">expanded uncertainty</skos:prefLabel>
    </owl:Class>
    


    <!-- http://standards.iso.org/iso/10303/tech/refdata/core#9c95b5de-202b-48c4-9b58-ba727240fef3 -->

    <owl:Class rdf:about="http://standards.iso.org/iso/10303/tech/refdata/core#9c95b5de-202b-48c4-9b58-ba727240fef3">
        <rdfs:subClassOf rdf:resource="http://standards.iso.org/iso/10303/tech/refdata/core#59b11220-3279-0135-b58f-598f1b1392ae"/>
        <dc:contributor>STEP Harmonization Team</dc:contributor>
        <dc:creator>Phil Spiby, Eurostep</dc:creator>
        <dc:date>2022-09-01</dc:date>
        <dc:source>ISO/TS 10303-4000</dc:source>
        <dc:type>InWork</dc:type>
        <rdfs:comment xml:lang="en">A SlotDesignToPlanned is a relationship between a design version of a Slot and a planned individual that conforms to the design.</rdfs:comment>
        <owl:versionInfo>1</owl:versionInfo>
        <skos:changeNote>[2022-09-01] Initial definition.</skos:changeNote>
        <skos:example xml:lang="en">WeMakeBigPlanes Limited plans production of aircraft serial number 1234 with a starboard engine attachment slot that is to conform to design version 1.34.</skos:example>
        <skos:prefLabel xml:lang="en">slot design to planned</skos:prefLabel>
    </owl:Class>
    


    <!-- http://standards.iso.org/iso/10303/tech/refdata/core#9c98fe40-130a-0135-b552-598f1b1392ae -->

    <owl:Class rdf:about="http://standards.iso.org/iso/10303/tech/refdata/core#9c98fe40-130a-0135-b552-598f1b1392ae">
        <rdfs:subClassOf rdf:resource="http://standards.iso.org/iso/10303/tech/refdata/core#9fddc900-130a-0135-b552-598f1b1392ae"/>
        <dc:contributor>STEP Harmonization Team</dc:contributor>
        <dc:creator>Phil Spiby, Eurostep</dc:creator>
        <dc:date>2022-09-01</dc:date>
        <dc:source>ISO/TS 10303-4000</dc:source>
        <dc:type>InWork</dc:type>
        <rdfs:comment xml:lang="en">An ExternalGeometricModel is a type of GeometricModel that contains geometry in a three-dimensional context only.</rdfs:comment>
        <owl:versionInfo>1</owl:versionInfo>
        <skos:changeNote>[2021-07-30] Initial definition.</skos:changeNote>
        <skos:prefLabel xml:lang="en">external geometric model</skos:prefLabel>
    </owl:Class>
    


    <!-- http://standards.iso.org/iso/10303/tech/refdata/core#9d7f5922-5a61-4d2b-a73f-e4a27e70b2ce -->

    <owl:Class rdf:about="http://standards.iso.org/iso/10303/tech/refdata/core#9d7f5922-5a61-4d2b-a73f-e4a27e70b2ce">
        <rdfs:subClassOf rdf:resource="http://standards.iso.org/iso/10303/tech/refdata/core#84099bf0-130a-0135-b552-598f1b1392ae"/>
        <dc:contributor>STEP Harmonization Team</dc:contributor>
        <dc:creator>Phil Spiby, Eurostep</dc:creator>
        <dc:date>2022-09-01</dc:date>
        <dc:source>ISO/TS 10303-4000</dc:source>
        <dc:type>InWork</dc:type>
        <rdfs:comment xml:lang="en">A SchemeEntryRelationship is a specialization of ActivityMethodRelationship that is a relationship between two SchemeEntry objects. A SchemeEntryRelationship can exist between SchemeEntry objects that relate to different Schemes or between different SchemeEntry objects of the same Scheme.</rdfs:comment>
        <owl:versionInfo>1</owl:versionInfo>
        <skos:changeNote>[2022-09-01] Initial definition.</skos:changeNote>
        <skos:example xml:lang="en">Decomposition, Dependency, and sequencing are examples of kinds of relationships possible between schema entries.</skos:example>
        <skos:note xml:lang="en">The SchemeEntryRelationship provides the facility to relate entries included in Plans or Schedules in different ways. By applying classifications on the SchemeEntryRelationship it can be used for different purposes.</skos:note>
        <skos:prefLabel xml:lang="en">scheme entry relationship</skos:prefLabel>
    </owl:Class>
    


    <!-- http://standards.iso.org/iso/10303/tech/refdata/core#9daedb10-130a-0135-b552-598f1b1392ae -->

    <owl:Class rdf:about="http://standards.iso.org/iso/10303/tech/refdata/core#9daedb10-130a-0135-b552-598f1b1392ae">
        <rdfs:subClassOf rdf:resource="http://standards.iso.org/iso/10303/tech/refdata/core#STEPThing"/>
        <dc:contributor>STEP Harmonization Team</dc:contributor>
        <dc:creator>Phil Spiby, Eurostep</dc:creator>
        <dc:date>2022-09-01</dc:date>
        <dc:source>ISO/TS 10303-4000</dc:source>
        <dc:type>InWork</dc:type>
        <rdfs:comment xml:lang="en">An ExternalUnit is an external specification of a quantity.</rdfs:comment>
        <owl:versionInfo>1</owl:versionInfo>
        <skos:changeNote>[2021-07-30] Initial definition.</skos:changeNote>
        <skos:prefLabel xml:lang="en">external unit</skos:prefLabel>
    </owl:Class>
    


    <!-- http://standards.iso.org/iso/10303/tech/refdata/core#9dba1851-6682-4143-9fb1-c4dd0bf75be7 -->

    <owl:Class rdf:about="http://standards.iso.org/iso/10303/tech/refdata/core#9dba1851-6682-4143-9fb1-c4dd0bf75be7">
        <rdfs:subClassOf rdf:resource="http://standards.iso.org/iso/10303/tech/refdata/core#59b11220-3279-0135-b58f-598f1b1392ae"/>
        <dc:contributor>STEP Harmonization Team</dc:contributor>
        <dc:creator>Phil Spiby, Eurostep</dc:creator>
        <dc:date>2022-09-01</dc:date>
        <dc:source>ISO/TS 10303-4000</dc:source>
        <dc:type>InWork</dc:type>
        <rdfs:comment xml:lang="en">An EnvelopeRelationship is a relationship between two Envelope objects.</rdfs:comment>
        <owl:versionInfo>2</owl:versionInfo>
        <skos:changeNote>[2021-07-30] Initial definition.</skos:changeNote>
        <skos:changeNote>[2022-09-01] Phil Spiby, Eurostep: updated comment.</skos:changeNote>
        <skos:note xml:lang="en">The most obvious use of the association is to link an Envelope to its acknowledgements.</skos:note>
        <skos:prefLabel xml:lang="en">envelope relationship</skos:prefLabel>
    </owl:Class>
    


    <!-- http://standards.iso.org/iso/10303/tech/refdata/core#9dc2b049-3c4d-414e-b125-883e393d9b14 -->

    <owl:Class rdf:about="http://standards.iso.org/iso/10303/tech/refdata/core#9dc2b049-3c4d-414e-b125-883e393d9b14">
        <rdfs:subClassOf rdf:resource="http://standards.iso.org/iso/10303/tech/refdata/core#c1247222-6528-4897-a401-5a61bdfd511c"/>
        <dc:contributor>STEP Harmonization Team</dc:contributor>
        <dc:creator>Phil Spiby, Eurostep</dc:creator>
        <dc:date>2022-09-01</dc:date>
        <dc:source>ISO/TS 10303-4000</dc:source>
        <dc:type>InWork</dc:type>
        <rdfs:comment xml:lang="en">A RepeatUntil is a type of LoopingElement. It invokes repetitions of the RepeatedElement inherited from LoopingElement until the specified condition is satisfied. The element being repeated shall be executed at least once and the condition tested after the first execution.</rdfs:comment>
        <owl:versionInfo>2</owl:versionInfo>
        <skos:changeNote>[2021-07-30] Initial definition.</skos:changeNote>
        <skos:changeNote>[2022-09-01] Phil Spiby, Eurostep: updated comment.</skos:changeNote>
        <skos:prefLabel xml:lang="en">repeat until</skos:prefLabel>
    </owl:Class>
    


    <!-- http://standards.iso.org/iso/10303/tech/refdata/core#9e16c4a0-130a-0135-b552-598f1b1392ae -->

    <owl:Class rdf:about="http://standards.iso.org/iso/10303/tech/refdata/core#9e16c4a0-130a-0135-b552-598f1b1392ae">
        <rdfs:subClassOf rdf:resource="http://standards.iso.org/iso/10303/tech/refdata/core#STEPThing"/>
        <dc:contributor>STEP Harmonization Team</dc:contributor>
        <dc:creator>Phil Spiby, Eurostep</dc:creator>
        <dc:date>2022-09-01</dc:date>
        <dc:source>ISO/TS 10303-4000</dc:source>
        <dc:type>InWork</dc:type>
        <rdfs:comment xml:lang="en">A File is one of potentially more files on a computer system or in actual stacks of paper that can make up a DocumentDefinition.</rdfs:comment>
        <owl:versionInfo>2</owl:versionInfo>
        <skos:changeNote>[2021-07-30] Initial definition.</skos:changeNote>
        <skos:changeNote>[2022-09-01] Phil Spiby, Eurostep: updated comment.</skos:changeNote>
        <skos:prefLabel xml:lang="en">file</skos:prefLabel>
    </owl:Class>
    


    <!-- http://standards.iso.org/iso/10303/tech/refdata/core#9e971830-130a-0135-b552-598f1b1392ae -->

    <owl:Class rdf:about="http://standards.iso.org/iso/10303/tech/refdata/core#9e971830-130a-0135-b552-598f1b1392ae">
        <rdfs:subClassOf rdf:resource="http://standards.iso.org/iso/10303/tech/refdata/core#59b11220-3279-0135-b58f-598f1b1392ae"/>
        <dc:contributor>STEP Harmonization Team</dc:contributor>
        <dc:creator>Phil Spiby, Eurostep</dc:creator>
        <dc:date>2022-09-01</dc:date>
        <dc:source>ISO/TS 10303-4000</dc:source>
        <dc:type>InWork</dc:type>
        <rdfs:comment xml:lang="en">A FileRelationship is a relationship between two File objects.</rdfs:comment>
        <owl:versionInfo>1</owl:versionInfo>
        <skos:changeNote>[2021-07-30] Initial definition.</skos:changeNote>
        <skos:prefLabel xml:lang="en">file relationship</skos:prefLabel>
    </owl:Class>
    


    <!-- http://standards.iso.org/iso/10303/tech/refdata/core#9f656069-ff2c-4f09-9091-f91388a14764 -->

    <owl:Class rdf:about="http://standards.iso.org/iso/10303/tech/refdata/core#9f656069-ff2c-4f09-9091-f91388a14764">
        <rdfs:subClassOf rdf:resource="http://standards.iso.org/iso/10303/tech/refdata/core#59b11220-3279-0135-b58f-598f1b1392ae"/>
        <dc:contributor>STEP Harmonization Team</dc:contributor>
        <dc:creator>Phil Spiby, Eurostep</dc:creator>
        <dc:date>2022-09-01</dc:date>
        <dc:source>ISO/TS 10303-4000</dc:source>
        <dc:type>InWork</dc:type>
        <rdfs:comment xml:lang="en">A StateRelationship is a relationship between two State objects.</rdfs:comment>
        <owl:versionInfo>2</owl:versionInfo>
        <skos:changeNote>[2021-07-30] Initial definition.</skos:changeNote>
        <skos:changeNote>[2022-09-01] Phil Spiby, Eurostep: updated comment.</skos:changeNote>
        <skos:prefLabel xml:lang="en">state relationship</skos:prefLabel>
    </owl:Class>
    


    <!-- http://standards.iso.org/iso/10303/tech/refdata/core#9f8cc2d0-130a-0135-b552-598f1b1392ae -->

    <owl:Class rdf:about="http://standards.iso.org/iso/10303/tech/refdata/core#9f8cc2d0-130a-0135-b552-598f1b1392ae">
        <rdfs:subClassOf rdf:resource="http://standards.iso.org/iso/10303/tech/refdata/core#a014de90-130a-0135-b552-598f1b1392ae"/>
        <dc:contributor>STEP Harmonization Team</dc:contributor>
        <dc:creator>Phil Spiby, Eurostep</dc:creator>
        <dc:date>2022-09-01</dc:date>
        <dc:source>ISO/TS 10303-4000</dc:source>
        <dc:type>InWork</dc:type>
        <rdfs:comment xml:lang="en">A GeneralGeometricRepresentationRelationship is a type of GeometricRepresentationRelationship that defines a user-defined relationship between two GeometricModel objects whose meaning is defined by the attribute RelationType.</rdfs:comment>
        <owl:versionInfo>2</owl:versionInfo>
        <skos:changeNote>[2021-07-30] Initial definition.</skos:changeNote>
        <skos:changeNote>[2022-09-01] Phil Spiby, Eurostep: updated comment.</skos:changeNote>
        <skos:prefLabel xml:lang="en">general geometric representation relationship</skos:prefLabel>
    </owl:Class>
    


    <!-- http://standards.iso.org/iso/10303/tech/refdata/core#9f9d8bb0-130a-0135-b552-598f1b1392ae -->

    <owl:Class rdf:about="http://standards.iso.org/iso/10303/tech/refdata/core#9f9d8bb0-130a-0135-b552-598f1b1392ae">
        <rdfs:subClassOf rdf:resource="http://standards.iso.org/iso/10303/tech/refdata/core#cca6c810-130a-0135-b552-598f1b1392ae"/>
        <dc:contributor>STEP Harmonization Team</dc:contributor>
        <dc:creator>Jean Brangé, AFNeT Services</dc:creator>
        <dc:date>2023-10-04</dc:date>
        <dc:source>ISO/TS 10303-4000</dc:source>
        <dc:type>InWork</dc:type>
        <rdfs:comment xml:lang="en">A GeneralShapeDependentProperty is a type of ShapeDependentProperty that defines a user-defined characteristic of an object. The PropertyValue specified by a GeneralShapeDependentProperty is derived from geometry.</rdfs:comment>
        <owl:versionInfo>3</owl:versionInfo>
        <skos:changeNote>[2023-10-04] Jean Brangé, AFNeT Services: Initial definition.</skos:changeNote>
        <skos:example xml:lang="en">If a geometry model is exchanged between two partners, the calculation of various properties of the bodies, such as centre of mass, overall surface, or overall volume, is performed by originator and recipient. When comparing these set of values, the existence of deficiencies in the received model can be easily detected.</skos:example>
        <skos:note xml:lang="en">The GeneralShapeDependentProperty may be used for the purpose of validation of geometric models.</skos:note>
        <skos:prefLabel xml:lang="en">general shape dependent property</skos:prefLabel>
    </owl:Class>
    


    <!-- http://standards.iso.org/iso/10303/tech/refdata/core#9fbf4480-130a-0135-b552-598f1b1392ae -->

    <owl:Class rdf:about="http://standards.iso.org/iso/10303/tech/refdata/core#9fbf4480-130a-0135-b552-598f1b1392ae">
        <rdfs:subClassOf rdf:resource="http://standards.iso.org/iso/10303/tech/refdata/core#b44098a0-130a-0135-b552-598f1b1392ae"/>
        <dc:contributor>STEP Harmonization Team</dc:contributor>
        <dc:creator>Phil Spiby, Eurostep</dc:creator>
        <dc:date>2022-09-01</dc:date>
        <dc:source>ISO/TS 10303-4000</dc:source>
        <dc:type>InWork</dc:type>
        <rdfs:comment xml:lang="en">A GeometricalRelationship is the relationship between two PartViewRelationship objects specifying two parts that are geometrically related. Therefore, the shape of the related parts can be represented only once and can be reused for the geometrically related situation. In this case the shape of the relating PartView is derived from the shape of the related PartView. The two PartViewRelationship objects that are related by this relationship shall belong to different PartVersion objects. Other properties except shape are not subject to this relationship and therefore are not &apos;inherited&apos; from the related PartView to the relating PartView. geometricalrelationship.png Mudguard illustration of GeometricalRelationship</rdfs:comment>
        <owl:versionInfo>2</owl:versionInfo>
        <skos:changeNote>[2021-07-30] Initial definition.</skos:changeNote>
        <skos:changeNote>[2022-09-01] Phil Spiby, Eurostep: updated comment.</skos:changeNote>
        <skos:example xml:lang="en">The following figure shows an example for a GeometricalRelationship: in this case the left mudguard of a car is symmetrical to the right mudguard. A given plane mirroring transformation specifies the location of the left mudguard regarding the location of the right mudguard.</skos:example>
        <skos:prefLabel xml:lang="en">geometrical relationship</skos:prefLabel>
    </owl:Class>
    


    <!-- http://standards.iso.org/iso/10303/tech/refdata/core#9fddc900-130a-0135-b552-598f1b1392ae -->

    <owl:Class rdf:about="http://standards.iso.org/iso/10303/tech/refdata/core#9fddc900-130a-0135-b552-598f1b1392ae">
        <rdfs:subClassOf rdf:resource="http://standards.iso.org/iso/10303/tech/refdata/core#9fee6ad0-130a-0135-b552-598f1b1392ae"/>
        <dc:contributor>STEP Harmonization Team</dc:contributor>
        <dc:creator>Phil Spiby, Eurostep</dc:creator>
        <dc:date>2022-09-01</dc:date>
        <dc:source>ISO/TS 10303-4000</dc:source>
        <dc:type>InWork</dc:type>
        <rdfs:comment xml:lang="en">A GeometricModel is a type of GeometricRepresentation that represents the geometric shape of a product.</rdfs:comment>
        <owl:versionInfo>1</owl:versionInfo>
        <skos:changeNote>[2021-07-30] Initial definition.</skos:changeNote>
        <skos:prefLabel xml:lang="en">geometric model</skos:prefLabel>
    </owl:Class>
    


    <!-- http://standards.iso.org/iso/10303/tech/refdata/core#9fee6ad0-130a-0135-b552-598f1b1392ae -->

    <owl:Class rdf:about="http://standards.iso.org/iso/10303/tech/refdata/core#9fee6ad0-130a-0135-b552-598f1b1392ae">
        <rdfs:subClassOf rdf:resource="http://standards.iso.org/iso/10303/tech/refdata/core#c565c970-130a-0135-b552-598f1b1392ae"/>
        <dc:contributor>STEP Harmonization Team</dc:contributor>
        <dc:creator>Phil Spiby, Eurostep</dc:creator>
        <dc:date>2022-09-01</dc:date>
        <dc:source>ISO/TS 10303-4000</dc:source>
        <dc:type>InWork</dc:type>
        <rdfs:comment xml:lang="en">A GeometricRepresentation is a type of Representation which is defined in a GeometricCoordinateSpace.</rdfs:comment>
        <owl:versionInfo>1</owl:versionInfo>
        <skos:changeNote>[2021-07-30] Initial definition.</skos:changeNote>
        <skos:prefLabel xml:lang="en">geometric representation</skos:prefLabel>
    </owl:Class>
    


    <!-- http://standards.iso.org/iso/10303/tech/refdata/core#90dc6290-130a-0135-b552-598f1b1392ae -->

    <owl:Class rdf:about="http://standards.iso.org/iso/10303/tech/refdata/core#90dc6290-130a-0135-b552-598f1b1392ae">
        <rdfs:subClassOf rdf:resource="http://standards.iso.org/iso/10303/tech/refdata/core#STEPThing"/>
        <dc:contributor>STEP Harmonization Team</dc:contributor>
        <dc:creator>Phil Spiby, Eurostep</dc:creator>
        <dc:date>2022-09-01</dc:date>
        <dc:source>ISO/TS 10303-4000</dc:source>
        <dc:type>InWork</dc:type>
        <rdfs:comment xml:lang="en">A ConfiguredAssemblyEffectivity is an effectivity controlled association of a ProductDesignAssociation with an item (specified by AssemblyDesignSelect).</rdfs:comment>
        <owl:versionInfo>1</owl:versionInfo>
        <skos:changeNote>[2021-07-30] Initial definition.</skos:changeNote>
        <skos:prefLabel xml:lang="en">configured assembly effectivity</skos:prefLabel>
    </owl:Class>
    


    <!-- http://standards.iso.org/iso/10303/tech/refdata/core#9029db70-130a-0135-b552-598f1b1392ae -->

    <owl:Class rdf:about="http://standards.iso.org/iso/10303/tech/refdata/core#9029db70-130a-0135-b552-598f1b1392ae">
        <rdfs:subClassOf rdf:resource="http://standards.iso.org/iso/10303/tech/refdata/core#1cfca290-3279-0135-b58f-598f1b1392ae"/>
        <dc:contributor>STEP Harmonization Team</dc:contributor>
        <dc:creator>Phil Spiby, Eurostep</dc:creator>
        <dc:date>2022-09-01</dc:date>
        <dc:source>ISO/TS 10303-4000</dc:source>
        <dc:type>InWork</dc:type>
        <rdfs:comment xml:lang="en">A ConditionAssignment is an assignment of a Condition to an item (specified by ConditionAssignmentSelect). The meaning of the assignment can be specified using the ClassifiedAs attribute inherited from the AssignmentObject.</rdfs:comment>
        <owl:versionInfo>2</owl:versionInfo>
        <skos:changeNote>[2021-07-30] Initial definition.</skos:changeNote>
        <skos:changeNote>[2022-09-01] Phil Spiby, Eurostep: updated comment.</skos:changeNote>
        <skos:prefLabel xml:lang="en">condition assignment</skos:prefLabel>
    </owl:Class>
    


    <!-- http://standards.iso.org/iso/10303/tech/refdata/core#907933f0-130a-0135-b552-598f1b1392ae -->

    <owl:Class rdf:about="http://standards.iso.org/iso/10303/tech/refdata/core#907933f0-130a-0135-b552-598f1b1392ae">
        <rdfs:subClassOf rdf:resource="http://standards.iso.org/iso/10303/tech/refdata/core#STEPThing"/>
        <dc:contributor>STEP Harmonization Team</dc:contributor>
        <dc:creator>Phil Spiby, Eurostep</dc:creator>
        <dc:date>2022-09-01</dc:date>
        <dc:source>ISO/TS 10303-4000</dc:source>
        <dc:type>InWork</dc:type>
        <rdfs:comment xml:lang="en">A ConditionParameter is a representation of an item (specified by ConditionParameterSelect) that is used to specify a Condition.</rdfs:comment>
        <owl:versionInfo>1</owl:versionInfo>
        <skos:changeNote>[2021-07-30] Initial definition.</skos:changeNote>
        <skos:prefLabel xml:lang="en">condition parameter</skos:prefLabel>
    </owl:Class>
    


    <!-- http://standards.iso.org/iso/10303/tech/refdata/core#90864677-a5ac-4f4c-b261-a0347fc3a4cb -->

    <owl:Class rdf:about="http://standards.iso.org/iso/10303/tech/refdata/core#90864677-a5ac-4f4c-b261-a0347fc3a4cb">
        <rdfs:subClassOf rdf:resource="http://standards.iso.org/iso/10303/tech/refdata/core#66348150-092a-4eb7-9561-0b83adfa15ff"/>
        <dc:contributor>STEP Harmonization Team</dc:contributor>
        <dc:creator>Jean Brangé, AFNeT Services</dc:creator>
        <dc:date>2023-10-04</dc:date>
        <dc:source>ISO/TS 10303-4000</dc:source>
        <dc:type>InWork</dc:type>
        <rdfs:comment xml:lang="en">A ToleranceZone is a type of ShapeElement that represents a tolerance zone as defined in ISO 1101. A ToleranceZone is the region within which the toleranced feature shall be defined. The characteristics of the region are specified by the way the toleranced feature is dimensioned.</rdfs:comment>
        <owl:versionInfo>3</owl:versionInfo>
        <skos:changeNote>[2023-10-04] Jean Brangé, AFNeT Services: Initial definition.</skos:changeNote>
        <skos:note xml:lang="en">A geometric location tolerance applied to a hole defines a ToleranceZoneType referenced by FormType.</skos:note>
        <skos:prefLabel xml:lang="en">tolerance zone</skos:prefLabel>
    </owl:Class>
    


    <!-- http://standards.iso.org/iso/10303/tech/refdata/core#909dd2f0-130a-0135-b552-598f1b1392ae -->

    <owl:Class rdf:about="http://standards.iso.org/iso/10303/tech/refdata/core#909dd2f0-130a-0135-b552-598f1b1392ae">
        <rdfs:subClassOf rdf:resource="http://standards.iso.org/iso/10303/tech/refdata/core#59b11220-3279-0135-b58f-598f1b1392ae"/>
        <dc:contributor>STEP Harmonization Team</dc:contributor>
        <dc:creator>Phil Spiby, Eurostep</dc:creator>
        <dc:date>2022-09-01</dc:date>
        <dc:source>ISO/TS 10303-4000</dc:source>
        <dc:type>InWork</dc:type>
        <rdfs:comment xml:lang="en">A ConditionRelationship is a relationship between two Condition objects.</rdfs:comment>
        <owl:versionInfo>2</owl:versionInfo>
        <skos:changeNote>[2021-07-30] Initial definition.</skos:changeNote>
        <skos:changeNote>[2022-09-01] Phil Spiby, Eurostep: updated comment.</skos:changeNote>
        <skos:prefLabel xml:lang="en">condition relationship</skos:prefLabel>
    </owl:Class>
    


    <!-- http://standards.iso.org/iso/10303/tech/refdata/core#91af796a-c733-4d0a-8de2-ada45ba26d63 -->

    <owl:Class rdf:about="http://standards.iso.org/iso/10303/tech/refdata/core#91af796a-c733-4d0a-8de2-ada45ba26d63">
        <rdfs:subClassOf rdf:resource="http://standards.iso.org/iso/10303/tech/refdata/core#59b11220-3279-0135-b58f-598f1b1392ae"/>
        <dc:contributor>STEP Harmonization Team</dc:contributor>
        <dc:creator>Phil Spiby, Eurostep</dc:creator>
        <dc:date>2022-09-01</dc:date>
        <dc:source>ISO/TS 10303-4000</dc:source>
        <dc:type>InWork</dc:type>
        <rdfs:comment xml:lang="en">A CollectionViewRelationship is a relationship between two CollectionView objects.</rdfs:comment>
        <owl:versionInfo>2</owl:versionInfo>
        <skos:changeNote>[2021-07-30] Initial definition.</skos:changeNote>
        <skos:changeNote>[2022-09-01] Phil Spiby, Eurostep: updated comment.</skos:changeNote>
        <skos:prefLabel xml:lang="en">collection view relationship</skos:prefLabel>
    </owl:Class>
    


    <!-- http://standards.iso.org/iso/10303/tech/refdata/core#91d08690-130a-0135-b552-598f1b1392ae -->

    <owl:Class rdf:about="http://standards.iso.org/iso/10303/tech/refdata/core#91d08690-130a-0135-b552-598f1b1392ae">
        <rdfs:subClassOf rdf:resource="http://standards.iso.org/iso/10303/tech/refdata/core#STEPThing"/>
        <dc:contributor>STEP Harmonization Team</dc:contributor>
        <dc:creator>Phil Spiby, Eurostep</dc:creator>
        <dc:date>2022-09-01</dc:date>
        <dc:source>ISO/TS 10303-4000</dc:source>
        <dc:type>InWork</dc:type>
        <rdfs:comment xml:lang="en">A Contract is a binding agreement between two or more parties.</rdfs:comment>
        <owl:versionInfo>2</owl:versionInfo>
        <skos:changeNote>[2021-07-30] Initial definition.</skos:changeNote>
        <skos:changeNote>[2022-09-01] Phil Spiby, Eurostep: updated example.</skos:changeNote>
        <skos:example xml:lang="en">Contracts can concern the design of part version objects, the delivery of drawing objects, or the execution of activity objects.</skos:example>
        <skos:prefLabel xml:lang="en">contract</skos:prefLabel>
    </owl:Class>
    


    <!-- http://standards.iso.org/iso/10303/tech/refdata/core#91d2508f-9f91-46e3-9434-2f8c0d0cc311 -->

    <owl:Class rdf:about="http://standards.iso.org/iso/10303/tech/refdata/core#91d2508f-9f91-46e3-9434-2f8c0d0cc311">
        <rdfs:subClassOf rdf:resource="http://standards.iso.org/iso/10303/tech/refdata/core#e1f21c44-a15a-40d1-ac2d-e6849a953d9d"/>
        <dc:contributor>STEP Harmonization Team</dc:contributor>
        <dc:creator>Jean Brangé, AFNeT Services</dc:creator>
        <dc:date>2023-10-04</dc:date>
        <dc:source>ISO/TS 10303-4000</dc:source>
        <dc:type>InWork</dc:type>
        <rdfs:comment xml:lang="en">A FaceBasedSheetRepresentation is a type of CompositeSheetRepresentation that is defined topologically.</rdfs:comment>
        <owl:versionInfo>3</owl:versionInfo>
        <skos:changeNote>[2023-10-04] Jean Brangé, AFNeT Services: Initial definition.</skos:changeNote>
        <skos:prefLabel xml:lang="en">face based sheet representation</skos:prefLabel>
    </owl:Class>
    


    <!-- http://standards.iso.org/iso/10303/tech/refdata/core#913c1856-862f-4f77-ba95-3a2f1c9c573a -->

    <owl:Class rdf:about="http://standards.iso.org/iso/10303/tech/refdata/core#913c1856-862f-4f77-ba95-3a2f1c9c573a">
        <rdfs:subClassOf rdf:resource="http://standards.iso.org/iso/10303/tech/refdata/core#STEPThing"/>
        <dc:contributor>STEP Harmonization Team</dc:contributor>
        <dc:creator>Phil Spiby, Eurostep</dc:creator>
        <dc:date>2022-09-01</dc:date>
        <dc:source>ISO/TS 10303-4000</dc:source>
        <dc:type>InWork</dc:type>
        <rdfs:comment xml:lang="en">A Validation is a subjective assertion that an item is &apos;fit for purpose&apos;. Validation is commonly understood to mean &apos;Have we built the right system?&apos;. Validation is concerned with ensuring that the system will meet the customer’s objectives and expectations. Validation usually includes testing under normal usage conditions.</rdfs:comment>
        <owl:versionInfo>2</owl:versionInfo>
        <skos:changeNote>[2021-07-30] Initial definition.</skos:changeNote>
        <skos:changeNote>[2022-09-01] Phil Spiby, Eurostep: updated comment updated example updated note.</skos:changeNote>
        <skos:example xml:lang="en">Every flight of every Space Shuttle has been a &apos;Validation&apos; flight to test the new design under actual conditions. No two shuttles have flown in the same configuration and many systems cannot be validated except under actual conditions.</skos:example>
        <skos:note xml:lang="en">An item can pass validation even though some requirements fail verification.</skos:note>
        <skos:note xml:lang="en">It is assumed that meta data supporting the validation will be applied using assignment entities, such as identification assignment, person and organization assignment etc..</skos:note>
        <skos:prefLabel xml:lang="en">validation</skos:prefLabel>
    </owl:Class>
    


    <!-- http://standards.iso.org/iso/10303/tech/refdata/core#914be3fd-65ac-4a15-a63e-3775dd255b6c -->

    <owl:Class rdf:about="http://standards.iso.org/iso/10303/tech/refdata/core#914be3fd-65ac-4a15-a63e-3775dd255b6c">
        <rdfs:subClassOf rdf:resource="http://standards.iso.org/iso/10303/tech/refdata/core#8e51b43d-49ca-4a6f-880d-4cb737a79dff"/>
        <dc:contributor>STEP Harmonization Team</dc:contributor>
        <dc:creator>Jean Brangé, AFNeT Services</dc:creator>
        <dc:date>2023-10-04</dc:date>
        <dc:source>ISO/TS 10303-4000</dc:source>
        <dc:type>InWork</dc:type>
        <rdfs:comment xml:lang="en">A ContactFeatureDefinitionFitRelationship is a type of ShapeFeatureDefinitionFitRelationship that is a relationship between two instances of the entity data type ContactFeatureDefinition that fit together.</rdfs:comment>
        <owl:versionInfo>3</owl:versionInfo>
        <skos:changeNote>[2023-10-04] Jean Brangé, AFNeT Services: Initial definition.</skos:changeNote>
        <skos:prefLabel xml:lang="en">contact feature definition fit relationship</skos:prefLabel>
    </owl:Class>
    


    <!-- http://standards.iso.org/iso/10303/tech/refdata/core#916c16a5-5b2e-4665-bb9e-08f100ed1ee1 -->

    <owl:Class rdf:about="http://standards.iso.org/iso/10303/tech/refdata/core#916c16a5-5b2e-4665-bb9e-08f100ed1ee1">
        <rdfs:subClassOf rdf:resource="http://standards.iso.org/iso/10303/tech/refdata/core#d8381cb4-ef44-45bb-ba54-3476e2f5f45e"/>
        <dc:contributor>STEP Harmonization Team</dc:contributor>
        <dc:creator>Jean Brangé, AFNeT Services</dc:creator>
        <dc:date>2023-10-04</dc:date>
        <dc:source>ISO/TS 10303-4000</dc:source>
        <dc:type>InWork</dc:type>
        <rdfs:comment xml:lang="en">A PartContactFeature is a type of PartFeature that is intended to be joined with another PartFeature when used in an assembly.</rdfs:comment>
        <owl:versionInfo>3</owl:versionInfo>
        <skos:changeNote>[2023-10-04] Jean Brangé, AFNeT Services: Initial definition.</skos:changeNote>
        <skos:prefLabel xml:lang="en">part contact feature</skos:prefLabel>
    </owl:Class>
    


    <!-- http://standards.iso.org/iso/10303/tech/refdata/core#9225f990-130a-0135-b552-598f1b1392ae -->

    <owl:Class rdf:about="http://standards.iso.org/iso/10303/tech/refdata/core#9225f990-130a-0135-b552-598f1b1392ae">
        <rdfs:subClassOf rdf:resource="http://standards.iso.org/iso/10303/tech/refdata/core#1cfca290-3279-0135-b58f-598f1b1392ae"/>
        <dc:contributor>STEP Harmonization Team</dc:contributor>
        <dc:creator>Phil Spiby, Eurostep</dc:creator>
        <dc:date>2022-09-01</dc:date>
        <dc:source>ISO/TS 10303-4000</dc:source>
        <dc:type>InWork</dc:type>
        <rdfs:comment xml:lang="en">A ContractAssignment is an assignment of a Contract to an item (specified by ContractAssignmentSelect). The meaning of the assignment can be specified using the ClassifiedAs attribute inherited from the AssignmentObject.</rdfs:comment>
        <owl:versionInfo>2</owl:versionInfo>
        <skos:changeNote>[2021-07-30] Initial definition.</skos:changeNote>
        <skos:changeNote>[2022-09-01] Phil Spiby, Eurostep: updated comment.</skos:changeNote>
        <skos:prefLabel xml:lang="en">contract assignment</skos:prefLabel>
    </owl:Class>
    


    <!-- http://standards.iso.org/iso/10303/tech/refdata/core#924a44f4-5dba-4e6b-875c-0ec76bb8f342 -->

    <owl:Class rdf:about="http://standards.iso.org/iso/10303/tech/refdata/core#924a44f4-5dba-4e6b-875c-0ec76bb8f342">
        <rdfs:subClassOf rdf:resource="http://standards.iso.org/iso/10303/tech/refdata/core#STEPThing"/>
        <dc:contributor>STEP Harmonization Team</dc:contributor>
        <dc:creator>Jean Brangé, AFNeT Services</dc:creator>
        <dc:date>2023-10-04</dc:date>
        <dc:source>ISO/TS 10303-4000</dc:source>
        <dc:type>InWork</dc:type>
        <rdfs:comment xml:lang="en">A ProcessOperationInputOrOutput is an input or expected result of a ProcessOperationDefinition.</rdfs:comment>
        <owl:versionInfo>3</owl:versionInfo>
        <skos:changeNote>[2023-10-04] Jean Brangé, AFNeT Services: Initial definition.</skos:changeNote>
        <skos:prefLabel xml:lang="en">process operation input or output</skos:prefLabel>
    </owl:Class>
    


    <!-- http://standards.iso.org/iso/10303/tech/refdata/core#925c9f2b-76ff-4dce-9ce8-4dc1e4dc8234 -->

    <owl:Class rdf:about="http://standards.iso.org/iso/10303/tech/refdata/core#925c9f2b-76ff-4dce-9ce8-4dc1e4dc8234">
        <rdfs:subClassOf rdf:resource="http://standards.iso.org/iso/10303/tech/refdata/core#59b11220-3279-0135-b58f-598f1b1392ae"/>
        <dc:contributor>STEP Harmonization Team</dc:contributor>
        <dc:creator>Phil Spiby, Eurostep</dc:creator>
        <dc:date>2022-09-01</dc:date>
        <dc:source>ISO/TS 10303-4000</dc:source>
        <dc:type>InWork</dc:type>
        <rdfs:comment xml:lang="en">An InterfaceSpecificationRelationship is a relationship between two InterfaceSpecification objects.</rdfs:comment>
        <owl:versionInfo>2</owl:versionInfo>
        <skos:changeNote>[2021-07-30] Initial definition.</skos:changeNote>
        <skos:changeNote>[2022-09-01] Phil Spiby, Eurostep: updated comment.</skos:changeNote>
        <skos:prefLabel xml:lang="en">interface specification relationship</skos:prefLabel>
    </owl:Class>
    


    <!-- http://standards.iso.org/iso/10303/tech/refdata/core#9279e5f0-130a-0135-b552-598f1b1392ae -->

    <owl:Class rdf:about="http://standards.iso.org/iso/10303/tech/refdata/core#9279e5f0-130a-0135-b552-598f1b1392ae">
        <rdfs:subClassOf rdf:resource="http://standards.iso.org/iso/10303/tech/refdata/core#59b11220-3279-0135-b58f-598f1b1392ae"/>
        <dc:contributor>STEP Harmonization Team</dc:contributor>
        <dc:creator>Phil Spiby, Eurostep</dc:creator>
        <dc:date>2022-09-01</dc:date>
        <dc:source>ISO/TS 10303-4000</dc:source>
        <dc:type>InWork</dc:type>
        <rdfs:comment xml:lang="en">A ContractRelationship is a relationship between two different Contract objects.</rdfs:comment>
        <owl:versionInfo>2</owl:versionInfo>
        <skos:changeNote>[2021-07-30] Initial definition.</skos:changeNote>
        <skos:changeNote>[2022-09-01] Phil Spiby, Eurostep: updated comment updated example.</skos:changeNote>
        <skos:example xml:lang="en">A sub-contract can be related to the main contract with the customer.</skos:example>
        <skos:prefLabel xml:lang="en">contract relationship</skos:prefLabel>
    </owl:Class>
    


    <!-- http://standards.iso.org/iso/10303/tech/refdata/core#93cfa9b1-4397-4dde-983a-b4ec8677a20f -->

    <owl:Class rdf:about="http://standards.iso.org/iso/10303/tech/refdata/core#93cfa9b1-4397-4dde-983a-b4ec8677a20f">
        <rdfs:subClassOf rdf:resource="http://standards.iso.org/iso/10303/tech/refdata/core#66348150-092a-4eb7-9561-0b83adfa15ff"/>
        <dc:contributor>STEP Harmonization Team</dc:contributor>
        <dc:creator>Jean Brangé, AFNeT Services</dc:creator>
        <dc:date>2023-10-04</dc:date>
        <dc:source>ISO/TS 10303-4000</dc:source>
        <dc:type>InWork</dc:type>
        <rdfs:comment xml:lang="en">A ShapeFeatureDefinitionElement is a type of ShapeElement that represents a part of the shape of a ShapeFeatureDefinition.</rdfs:comment>
        <owl:versionInfo>3</owl:versionInfo>
        <skos:changeNote>[2023-10-04] Jean Brangé, AFNeT Services: Initial definition.</skos:changeNote>
        <skos:prefLabel xml:lang="en">shape feature definition element</skos:prefLabel>
    </owl:Class>
    


    <!-- http://standards.iso.org/iso/10303/tech/refdata/core#93e56e3d-c125-4419-b785-90a469ba2d26 -->

    <owl:Class rdf:about="http://standards.iso.org/iso/10303/tech/refdata/core#93e56e3d-c125-4419-b785-90a469ba2d26">
        <rdfs:subClassOf rdf:resource="http://standards.iso.org/iso/10303/tech/refdata/core#c6260c30-130a-0135-b552-598f1b1392ae"/>
        <dc:contributor>STEP Harmonization Team</dc:contributor>
        <dc:creator>Jean Brangé, AFNeT Services</dc:creator>
        <dc:date>2023-10-04</dc:date>
        <dc:source>ISO/TS 10303-4000</dc:source>
        <dc:type>InWork</dc:type>
        <rdfs:comment xml:lang="en">A GeometryToTopologyModelAssociation is a type of RepresentationRelationship that defines a set of allocation associations between a geometric origin item and a topological target item. This association is not definitional and therefore will not bring the definition of the source into the target model. This set of allocation associations is realized by a list of origin items and a list of target items that are coordinated so that the first origin item corresponds to the first target item, the second to the second and so on. The number of items on the origin and target sides shall be the same. In the case that the Target object is an Edge, the placement for the Origin is intended to represent a position and direction in the cross section of the origin shape.</rdfs:comment>
        <owl:versionInfo>3</owl:versionInfo>
        <skos:changeNote>[2023-10-04] Jean Brangé, AFNeT Services: Initial definition.</skos:changeNote>
        <skos:note xml:lang="en">For users and implementers, note that the structure is not intended for Geometric Modeling. It is intended for traceability and verification purposes of the structure of the electrical wiring harness. To support wiring harness design requirements, the entities GeometryToTopologyModelAssociation and TopologyToGeometryModelAssociation, which are subtypes of RepresentationRelationship, are based on WiringHarnessAssemblyDesign, which is a subtype of AssemblyDefinition. GeometryToTopologyModelAssociation and TopologyToGeometryModelAssociation are referenced by an AssemblyOccurrenceRelationship. The design intent of the information model is to create one or more pairwise allocation associations between geometric elements and topological elements specific to electrical wire harness design. This specific usage of AssemblyOccurrenceRelationship is restricted to WiringHarnessAssemblyDesign.</skos:note>
        <skos:prefLabel xml:lang="en">geometry to topology model association</skos:prefLabel>
    </owl:Class>
    


    <!-- http://standards.iso.org/iso/10303/tech/refdata/core#93f143b0-130a-0135-b552-598f1b1392ae -->

    <owl:Class rdf:about="http://standards.iso.org/iso/10303/tech/refdata/core#93f143b0-130a-0135-b552-598f1b1392ae">
        <rdfs:subClassOf rdf:resource="http://standards.iso.org/iso/10303/tech/refdata/core#1cfca290-3279-0135-b58f-598f1b1392ae"/>
        <dc:contributor>STEP Harmonization Team</dc:contributor>
        <dc:creator>Phil Spiby, Eurostep</dc:creator>
        <dc:date>2022-09-01</dc:date>
        <dc:source>ISO/TS 10303-4000</dc:source>
        <dc:type>InWork</dc:type>
        <rdfs:comment xml:lang="en">A DateTimeAssignment is an assignment of point in time specified as a DateTimeString to an item (specified by DateTimeAssignmentSelect). The meaning of the assignment can be specified using the ClassifiedAs attribute inherited from the AssignmentObject.</rdfs:comment>
        <owl:versionInfo>2</owl:versionInfo>
        <skos:changeNote>[2021-07-30] Initial definition.</skos:changeNote>
        <skos:changeNote>[2022-09-01] Phil Spiby, Eurostep: updated comment updated example updated note.</skos:changeNote>
        <skos:example xml:lang="en">If applied to an instance of Part with classification &apos;creation date&apos;, the DateTimeAssignment specifies the creation date of the part, tool, or raw material as a new object in the activity domain, and not the creation date of the instance of Part in a product management system.</skos:example>
        <skos:prefLabel xml:lang="en">date time assignment</skos:prefLabel>
    </owl:Class>
    


    <!-- http://standards.iso.org/iso/10303/tech/refdata/core#9384ed50-130a-0135-b552-598f1b1392ae -->

    <owl:Class rdf:about="http://standards.iso.org/iso/10303/tech/refdata/core#9384ed50-130a-0135-b552-598f1b1392ae">
        <rdfs:subClassOf rdf:resource="http://standards.iso.org/iso/10303/tech/refdata/core#99130bd0-130a-0135-b552-598f1b1392ae"/>
        <dc:contributor>STEP Harmonization Team</dc:contributor>
        <dc:creator>Phil Spiby, Eurostep</dc:creator>
        <dc:date>2022-09-01</dc:date>
        <dc:source>ISO/TS 10303-4000</dc:source>
        <dc:type>InWork</dc:type>
        <rdfs:comment xml:lang="en">A DatedEffectivity is a specialization of Effectivity for which the domain of applicability is defined as an interval of time bounded by dates or events. The time bounds are defined by its inherited attributes StartDefinition or EndDefinition. The interval can be open-ended. Depending on which of the StartDefinition and EndDefinition attributes are specified, the actual domain of time defined by a DatedEffectivity is: the time interval between the start and end date or event; the open time interval that starts at the start date or event; the open time interval that ends at the end date or event (in this case the start is unknown). If the EndDefinition is an event that actually identifies a point in time that comes before the StartDefinition, then the actual domain of effectivity is empty.</rdfs:comment>
        <owl:versionInfo>2</owl:versionInfo>
        <skos:changeNote>[2021-07-30] Initial definition.</skos:changeNote>
        <skos:changeNote>[2022-09-01] Phil Spiby, Eurostep: updated comment updated example.</skos:changeNote>
        <skos:example xml:lang="en">Events can be used to bound a DatedEffectivity period, at planning phase.</skos:example>
        <skos:prefLabel xml:lang="en">dated effectivity</skos:prefLabel>
    </owl:Class>
    


    <!-- http://standards.iso.org/iso/10303/tech/refdata/core#939f1236-c822-429c-bfa5-de45d7781044 -->

    <owl:Class rdf:about="http://standards.iso.org/iso/10303/tech/refdata/core#939f1236-c822-429c-bfa5-de45d7781044">
        <rdfs:subClassOf rdf:resource="http://standards.iso.org/iso/10303/tech/refdata/core#5a6c8b1f-63af-4307-9faf-9fdd6da5572c"/>
        <dc:contributor>STEP Harmonization Team</dc:contributor>
        <dc:creator>Jean Brangé, AFNeT Services</dc:creator>
        <dc:date>2023-10-04</dc:date>
        <dc:source>ISO/TS 10303-4000</dc:source>
        <dc:type>InWork</dc:type>
        <rdfs:comment xml:lang="en">A FilamentLaminate is a type of ConstituentPart that is a bonded material of two or more bundles of filament construction. The FilamentLaminate defines a volume to fill with filament assemblies. FilamentLaminate.pngFilament laminate</rdfs:comment>
        <owl:versionInfo>3</owl:versionInfo>
        <skos:changeNote>[2023-10-04] Jean Brangé, AFNeT Services: Initial definition.</skos:changeNote>
        <skos:example xml:lang="en">Pultruded shapes, radius fillers, and filament wound structure are types of FilamentLaminate (see following figure).</skos:example>
        <skos:note xml:lang="en">The difference between a ply and a FilamentLaminate, when referencing a StockMaterial, is that a ply describes a constant thickness area to be filled by a StockMaterial and a FilamentLaminate describes a general volume to be filled by a StockMaterial.</skos:note>
        <skos:note xml:lang="en">The shape of a FilamentLaminate may be defined by a cross section and a length.</skos:note>
        <skos:note xml:lang="en">When a FilamentLaminate is made from a StockMaterial, it usually refers to individual tows, yarns, and rovings. These volumes can be as simple as the cross section and length of a radius filler to as complex as a filament wound vessel. FilamentLaminates that are made by pulling and forming processes, called pultrusions, may use a tape form of FilamentAssembly.</skos:note>
        <skos:prefLabel xml:lang="en">filament laminate</skos:prefLabel>
    </owl:Class>
    


    <!-- http://standards.iso.org/iso/10303/tech/refdata/core#94e25a70-130a-0135-b552-598f1b1392ae -->

    <owl:Class rdf:about="http://standards.iso.org/iso/10303/tech/refdata/core#94e25a70-130a-0135-b552-598f1b1392ae">
        <rdfs:subClassOf rdf:resource="http://standards.iso.org/iso/10303/tech/refdata/core#STEPThing"/>
        <dc:contributor>STEP Harmonization Team</dc:contributor>
        <dc:creator>Phil Spiby, Eurostep</dc:creator>
        <dc:date>2022-09-01</dc:date>
        <dc:source>ISO/TS 10303-4000</dc:source>
        <dc:type>InWork</dc:type>
        <rdfs:comment xml:lang="en">A Descriptor is a set of words that describe something.</rdfs:comment>
        <owl:versionInfo>2</owl:versionInfo>
        <skos:changeNote>[2021-07-30] Initial definition.</skos:changeNote>
        <skos:changeNote>[2022-09-01] Phil Spiby, Eurostep: updated example.</skos:changeNote>
        <skos:example xml:lang="en">The same item can have multiple descriptions associated with it. Assigning both a short description and a long description to an activity or an organization are examples of multiple descriptions applied to the same item.</skos:example>
        <skos:prefLabel xml:lang="en">descriptor</skos:prefLabel>
    </owl:Class>
    


    <!-- http://standards.iso.org/iso/10303/tech/refdata/core#94453010-130a-0135-b552-598f1b1392ae -->

    <owl:Class rdf:about="http://standards.iso.org/iso/10303/tech/refdata/core#94453010-130a-0135-b552-598f1b1392ae">
        <rdfs:subClassOf rdf:resource="http://standards.iso.org/iso/10303/tech/refdata/core#ae1e7780-130a-0135-b552-598f1b1392ae"/>
        <dc:contributor>STEP Harmonization Team</dc:contributor>
        <dc:creator>Phil Spiby, Eurostep</dc:creator>
        <dc:date>2022-09-01</dc:date>
        <dc:source>ISO/TS 10303-4000</dc:source>
        <dc:type>InWork</dc:type>
        <rdfs:comment xml:lang="en">A DefinitionBasedOccurrence is a type of Occurrence that uses an item (specified by OccurrenceDefinitionSelect) as its definition. It is either a SingleOccurrence or a QuantifiedOccurrence.</rdfs:comment>
        <owl:versionInfo>2</owl:versionInfo>
        <skos:changeNote>[2021-07-30] Initial definition.</skos:changeNote>
        <skos:changeNote>[2022-09-01] Phil Spiby, Eurostep: updated comment.</skos:changeNote>
        <skos:prefLabel xml:lang="en">definition based occurrence</skos:prefLabel>
    </owl:Class>
    


    <!-- http://standards.iso.org/iso/10303/tech/refdata/core#9452ebb0-130a-0135-b552-598f1b1392ae -->

    <owl:Class rdf:about="http://standards.iso.org/iso/10303/tech/refdata/core#9452ebb0-130a-0135-b552-598f1b1392ae">
        <rdfs:subClassOf rdf:resource="http://standards.iso.org/iso/10303/tech/refdata/core#b44098a0-130a-0135-b552-598f1b1392ae"/>
        <dc:contributor>STEP Harmonization Team</dc:contributor>
        <dc:creator>Phil Spiby, Eurostep</dc:creator>
        <dc:date>2022-09-01</dc:date>
        <dc:source>ISO/TS 10303-4000</dc:source>
        <dc:type>InWork</dc:type>
        <rdfs:comment xml:lang="en">A DefinitionalPartViewUsage is a type of PartViewRelationship where all the elements of the Related PartView are then available to the Relating PartView. These elements are specifically all PartShapeElements, properties and NextAssemblyOccurrenceUsages on the Related PartView. These elements are either direct or indirect. A direct element references explicitly a PartView. An indirect element is available to a PartView via a DefinitionalPartViewUsage of another PartView. All DefinitionalPartViewUsages shall describe an acyclic graph.</rdfs:comment>
        <owl:versionInfo>2</owl:versionInfo>
        <skos:changeNote>[2021-07-30] Initial definition.</skos:changeNote>
        <skos:changeNote>[2022-09-01] Phil Spiby, Eurostep: updated comment.</skos:changeNote>
        <skos:note xml:lang="en">A related PartView can be a definitional constituent of the relating PartView only once.</skos:note>
        <skos:prefLabel xml:lang="en">definitional part view usage</skos:prefLabel>
    </owl:Class>
    


    <!-- http://standards.iso.org/iso/10303/tech/refdata/core#95f1bde5-b263-4ca1-89df-33e1205800dd -->

    <owl:Class rdf:about="http://standards.iso.org/iso/10303/tech/refdata/core#95f1bde5-b263-4ca1-89df-33e1205800dd">
        <rdfs:subClassOf rdf:resource="http://standards.iso.org/iso/10303/tech/refdata/core#835280f0-130a-0135-b552-598f1b1392ae"/>
        <dc:contributor>STEP Harmonization Team</dc:contributor>
        <dc:creator>Phil Spiby, Eurostep</dc:creator>
        <dc:date>2022-09-01</dc:date>
        <dc:source>ISO/TS 10303-4000</dc:source>
        <dc:type>InWork</dc:type>
        <rdfs:comment xml:lang="en">A TaskElement is a specialization of ActivityMethod. It is a representation of all or part of how to undertake a task.</rdfs:comment>
        <owl:versionInfo>1</owl:versionInfo>
        <skos:changeNote>[2021-07-30] Initial definition.</skos:changeNote>
        <skos:prefLabel xml:lang="en">task element</skos:prefLabel>
    </owl:Class>
    


    <!-- http://standards.iso.org/iso/10303/tech/refdata/core#95f502f0-130a-0135-b552-598f1b1392ae -->

    <owl:Class rdf:about="http://standards.iso.org/iso/10303/tech/refdata/core#95f502f0-130a-0135-b552-598f1b1392ae">
        <rdfs:subClassOf rdf:resource="http://standards.iso.org/iso/10303/tech/refdata/core#STEPThing"/>
        <dc:contributor>STEP Harmonization Team</dc:contributor>
        <dc:creator>Phil Spiby, Eurostep</dc:creator>
        <dc:date>2022-09-01</dc:date>
        <dc:source>ISO/TS 10303-4000</dc:source>
        <dc:type>InWork</dc:type>
        <rdfs:comment xml:lang="en">A Document is a logical container for documentation data under configuration control.</rdfs:comment>
        <owl:versionInfo>1</owl:versionInfo>
        <skos:changeNote>[2021-07-30] Initial definition.</skos:changeNote>
        <skos:prefLabel xml:lang="en">document</skos:prefLabel>
    </owl:Class>
    


    <!-- http://standards.iso.org/iso/10303/tech/refdata/core#9520cf55-f02b-47f8-9c2b-257553036333 -->

    <owl:Class rdf:about="http://standards.iso.org/iso/10303/tech/refdata/core#9520cf55-f02b-47f8-9c2b-257553036333">
        <rdfs:subClassOf rdf:resource="http://standards.iso.org/iso/10303/tech/refdata/core#59b11220-3279-0135-b58f-598f1b1392ae"/>
        <dc:contributor>STEP Harmonization Team</dc:contributor>
        <dc:creator>Phil Spiby, Eurostep</dc:creator>
        <dc:date>2022-09-01</dc:date>
        <dc:source>ISO/TS 10303-4000</dc:source>
        <dc:type>InWork</dc:type>
        <rdfs:comment xml:lang="en">A ResourceEventRelationship is a relationship between two ResourceEvent objects.</rdfs:comment>
        <owl:versionInfo>2</owl:versionInfo>
        <skos:changeNote>[2021-07-30] Initial definition.</skos:changeNote>
        <skos:changeNote>[2022-09-01] Phil Spiby, Eurostep: updated comment updated example.</skos:changeNote>
        <skos:example xml:lang="en">A managed resource relationship can be classified as &quot;realized by&quot; or &quot;replaces&quot;.</skos:example>
        <skos:prefLabel xml:lang="en">resource event relationship</skos:prefLabel>
    </owl:Class>
    


    <!-- http://standards.iso.org/iso/10303/tech/refdata/core#9520ea10-130a-0135-b552-598f1b1392ae -->

    <owl:Class rdf:about="http://standards.iso.org/iso/10303/tech/refdata/core#9520ea10-130a-0135-b552-598f1b1392ae">
        <rdfs:subClassOf rdf:resource="http://standards.iso.org/iso/10303/tech/refdata/core#59b11220-3279-0135-b58f-598f1b1392ae"/>
        <dc:contributor>STEP Harmonization Team</dc:contributor>
        <dc:creator>Phil Spiby, Eurostep</dc:creator>
        <dc:date>2022-09-01</dc:date>
        <dc:source>ISO/TS 10303-4000</dc:source>
        <dc:type>InWork</dc:type>
        <rdfs:comment xml:lang="en">A DescriptorRelationship is a relationship between two Descriptor objects.</rdfs:comment>
        <owl:versionInfo>1</owl:versionInfo>
        <skos:changeNote>[2021-07-30] Initial definition.</skos:changeNote>
        <skos:prefLabel xml:lang="en">descriptor relationship</skos:prefLabel>
    </owl:Class>
    


    <!-- http://standards.iso.org/iso/10303/tech/refdata/core#956ebbf0-130a-0135-b552-598f1b1392ae -->

    <owl:Class rdf:about="http://standards.iso.org/iso/10303/tech/refdata/core#956ebbf0-130a-0135-b552-598f1b1392ae">
        <rdfs:subClassOf rdf:resource="http://standards.iso.org/iso/10303/tech/refdata/core#96c60e90-130a-0135-b552-598f1b1392ae"/>
        <dc:contributor>STEP Harmonization Team</dc:contributor>
        <dc:creator>Phil Spiby, Eurostep</dc:creator>
        <dc:date>2022-09-01</dc:date>
        <dc:source>ISO/TS 10303-4000</dc:source>
        <dc:type>InWork</dc:type>
        <rdfs:comment xml:lang="en">A DigitalDocumentDefinition is a type of DocumentDefinition that collects files that are archived on an optical computer disc, magnetic, electronic storage, or a combination thereof. A DigitalDocumentDefinition can consist of one or many component DigitalFile.</rdfs:comment>
        <owl:versionInfo>2</owl:versionInfo>
        <skos:changeNote>[2021-07-30] Initial definition.</skos:changeNote>
        <skos:changeNote>[2022-09-01] Phil Spiby, Eurostep: updated comment.</skos:changeNote>
        <skos:prefLabel xml:lang="en">digital document definition</skos:prefLabel>
    </owl:Class>
    


    <!-- http://standards.iso.org/iso/10303/tech/refdata/core#957c7790-130a-0135-b552-598f1b1392ae -->

    <owl:Class rdf:about="http://standards.iso.org/iso/10303/tech/refdata/core#957c7790-130a-0135-b552-598f1b1392ae">
        <rdfs:subClassOf rdf:resource="http://standards.iso.org/iso/10303/tech/refdata/core#9e16c4a0-130a-0135-b552-598f1b1392ae"/>
        <dc:contributor>STEP Harmonization Team</dc:contributor>
        <dc:creator>Phil Spiby, Eurostep</dc:creator>
        <dc:date>2022-09-01</dc:date>
        <dc:source>ISO/TS 10303-4000</dc:source>
        <dc:type>InWork</dc:type>
        <rdfs:comment xml:lang="en">A DigitalFile is a type of File that contains computer interpretable data and is stored on an electronic device.</rdfs:comment>
        <owl:versionInfo>1</owl:versionInfo>
        <skos:changeNote>[2021-07-30] Initial definition.</skos:changeNote>
        <skos:prefLabel xml:lang="en">digital file</skos:prefLabel>
    </owl:Class>
    


    <!-- http://standards.iso.org/iso/10303/tech/refdata/core#959c82b0-130a-0135-b552-598f1b1392ae -->

    <owl:Class rdf:about="http://standards.iso.org/iso/10303/tech/refdata/core#959c82b0-130a-0135-b552-598f1b1392ae">
        <rdfs:subClassOf rdf:resource="http://standards.iso.org/iso/10303/tech/refdata/core#b72f5420-130a-0135-b552-598f1b1392ae"/>
        <dc:contributor>STEP Harmonization Team</dc:contributor>
        <dc:creator>Phil Spiby, Eurostep</dc:creator>
        <dc:date>2022-09-01</dc:date>
        <dc:source>ISO/TS 10303-4000</dc:source>
        <dc:type>InWork</dc:type>
        <rdfs:comment xml:lang="en">A DirectedPlannedActivity is a type of PlannedActivity that identifies a PlannedActivity governed by a WorkOrder.</rdfs:comment>
        <owl:versionInfo>1</owl:versionInfo>
        <skos:changeNote>[2021-07-30] Initial definition.</skos:changeNote>
        <skos:prefLabel xml:lang="en">directed planned activity</skos:prefLabel>
    </owl:Class>
    


    <!-- http://standards.iso.org/iso/10303/tech/refdata/core#95976136-28f1-459a-9c46-814d3078e27f -->

    <owl:Class rdf:about="http://standards.iso.org/iso/10303/tech/refdata/core#95976136-28f1-459a-9c46-814d3078e27f">
        <rdfs:subClassOf rdf:resource="http://standards.iso.org/iso/10303/tech/refdata/core#59b11220-3279-0135-b58f-598f1b1392ae"/>
        <dc:contributor>STEP Harmonization Team</dc:contributor>
        <dc:creator>Phil Spiby, Eurostep</dc:creator>
        <dc:date>2022-09-01</dc:date>
        <dc:source>ISO/TS 10303-4000</dc:source>
        <dc:type>InWork</dc:type>
        <rdfs:comment xml:lang="en">A SlotDefinitionRelationship is a relationship between two SlotDefinition objects.</rdfs:comment>
        <owl:versionInfo>1</owl:versionInfo>
        <skos:changeNote>[2022-09-01] Initial definition.</skos:changeNote>
        <skos:prefLabel xml:lang="en">slot definition relationship</skos:prefLabel>
    </owl:Class>
    


    <!-- http://standards.iso.org/iso/10303/tech/refdata/core#96c60e90-130a-0135-b552-598f1b1392ae -->

    <owl:Class rdf:about="http://standards.iso.org/iso/10303/tech/refdata/core#96c60e90-130a-0135-b552-598f1b1392ae">
        <rdfs:subClassOf rdf:resource="http://standards.iso.org/iso/10303/tech/refdata/core#STEPThing"/>
        <dc:contributor>STEP Harmonization Team</dc:contributor>
        <dc:creator>Phil Spiby, Eurostep</dc:creator>
        <dc:date>2022-09-01</dc:date>
        <dc:source>ISO/TS 10303-4000</dc:source>
        <dc:type>InWork</dc:type>
        <rdfs:comment xml:lang="en">A DocumentDefinition is one of potentially more alternative views of a DocumentVersion.</rdfs:comment>
        <owl:versionInfo>2</owl:versionInfo>
        <skos:changeNote>[2021-07-30] Initial definition.</skos:changeNote>
        <skos:changeNote>[2022-09-01] Phil Spiby, Eurostep: updated example updated note.</skos:changeNote>
        <skos:example xml:lang="en">A version of a logical document, which contains a shape model, can be represented in the different native formats of two three-dimensional CAD systems.</skos:example>
        <skos:note xml:lang="en">A DocumentVersion can have more than one view.</skos:note>
        <skos:prefLabel xml:lang="en">document definition</skos:prefLabel>
    </owl:Class>
    


    <!-- http://standards.iso.org/iso/10303/tech/refdata/core#96d3588c-c6cf-461c-ae07-9d343a97238e -->

    <owl:Class rdf:about="http://standards.iso.org/iso/10303/tech/refdata/core#96d3588c-c6cf-461c-ae07-9d343a97238e">
        <rdfs:subClassOf rdf:resource="http://standards.iso.org/iso/10303/tech/refdata/core#1cfca290-3279-0135-b58f-598f1b1392ae"/>
        <dc:contributor>STEP Harmonization Team</dc:contributor>
        <dc:creator>Phil Spiby, Eurostep</dc:creator>
        <dc:date>2022-09-01</dc:date>
        <dc:source>ISO/TS 10303-4000</dc:source>
        <dc:type>InWork</dc:type>
        <rdfs:comment xml:lang="en">An ObservedEnvironmentAssignment is an assignment of an environment (via ObservedEnvironmentView) to an item (specified in ObservedEnvironmentAssignmentSelect). The meaning of the assignment can be specified using the ClassifiedAs attribute inherited from the AssignmentObject.</rdfs:comment>
        <owl:versionInfo>2</owl:versionInfo>
        <skos:changeNote>[2021-07-30] Initial definition.</skos:changeNote>
        <skos:changeNote>[2022-09-01] Phil Spiby, Eurostep: updated comment.</skos:changeNote>
        <skos:prefLabel xml:lang="en">observed environment assignment</skos:prefLabel>
    </owl:Class>
    


    <!-- http://standards.iso.org/iso/10303/tech/refdata/core#9600ac69-b918-4620-8503-72dc06699f83 -->

    <owl:Class rdf:about="http://standards.iso.org/iso/10303/tech/refdata/core#9600ac69-b918-4620-8503-72dc06699f83">
        <rdfs:subClassOf rdf:resource="http://standards.iso.org/iso/10303/tech/refdata/core#1d59c650-3279-0135-b58f-598f1b1392ae"/>
        <dc:contributor>STEP Harmonization Team</dc:contributor>
        <dc:creator>Phil Spiby, Eurostep</dc:creator>
        <dc:date>2022-09-01</dc:date>
        <dc:source>ISO/TS 10303-4000</dc:source>
        <dc:type>InWork</dc:type>
        <rdfs:comment xml:lang="en">A PositionPositionTypeAssociation is an association between a PositionType and a Position. It allows many positions to be described by many position types.</rdfs:comment>
        <owl:versionInfo>1</owl:versionInfo>
        <skos:changeNote>[2022-09-01] Initial definition.</skos:changeNote>
        <skos:prefLabel xml:lang="en">position position type association</skos:prefLabel>
    </owl:Class>
    


    <!-- http://standards.iso.org/iso/10303/tech/refdata/core#96562395-fe55-4cc6-a59d-1c71f880097a -->

    <owl:Class rdf:about="http://standards.iso.org/iso/10303/tech/refdata/core#96562395-fe55-4cc6-a59d-1c71f880097a">
        <rdfs:subClassOf rdf:resource="http://standards.iso.org/iso/10303/tech/refdata/core#ff04d2c5-cea4-41a6-be35-821c1495d8ba"/>
        <dc:contributor>STEP Harmonization Team</dc:contributor>
        <dc:creator>Phil Spiby, Eurostep</dc:creator>
        <dc:date>2022-09-01</dc:date>
        <dc:source>ISO/TS 10303-4000</dc:source>
        <dc:type>InWork</dc:type>
        <rdfs:comment xml:lang="en">A TaskElementSequence is a specialization of TaskElement that comprises a sequence of steps to be followed in a specified order.</rdfs:comment>
        <owl:versionInfo>1</owl:versionInfo>
        <skos:changeNote>[2021-07-30] Initial definition.</skos:changeNote>
        <skos:prefLabel xml:lang="en">task element sequence</skos:prefLabel>
    </owl:Class>
    


    <!-- http://standards.iso.org/iso/10303/tech/refdata/core#9665ed30-130a-0135-b552-598f1b1392ae -->

    <owl:Class rdf:about="http://standards.iso.org/iso/10303/tech/refdata/core#9665ed30-130a-0135-b552-598f1b1392ae">
        <rdfs:subClassOf rdf:resource="http://standards.iso.org/iso/10303/tech/refdata/core#1cfca290-3279-0135-b58f-598f1b1392ae"/>
        <dc:contributor>STEP Harmonization Team</dc:contributor>
        <dc:creator>Phil Spiby, Eurostep</dc:creator>
        <dc:date>2022-09-01</dc:date>
        <dc:source>ISO/TS 10303-4000</dc:source>
        <dc:type>InWork</dc:type>
        <rdfs:comment xml:lang="en">A DocumentAssignment is an assignment of a Document to an item (specified by DocumentAssignmentSelect), where the assigned document provides information about the object to which it is assigned.</rdfs:comment>
        <owl:versionInfo>2</owl:versionInfo>
        <skos:changeNote>[2021-07-30] Initial definition.</skos:changeNote>
        <skos:changeNote>[2022-09-01] Phil Spiby, Eurostep: updated comment.</skos:changeNote>
        <skos:prefLabel xml:lang="en">document assignment</skos:prefLabel>
    </owl:Class>
    


    <!-- http://standards.iso.org/iso/10303/tech/refdata/core#97b41810-130a-0135-b552-598f1b1392ae -->

    <owl:Class rdf:about="http://standards.iso.org/iso/10303/tech/refdata/core#97b41810-130a-0135-b552-598f1b1392ae">
        <rdfs:subClassOf rdf:resource="http://standards.iso.org/iso/10303/tech/refdata/core#59b11220-3279-0135-b58f-598f1b1392ae"/>
        <dc:contributor>STEP Harmonization Team</dc:contributor>
        <dc:creator>Phil Spiby, Eurostep</dc:creator>
        <dc:date>2022-09-01</dc:date>
        <dc:source>ISO/TS 10303-4000</dc:source>
        <dc:type>InWork</dc:type>
        <rdfs:comment xml:lang="en">A DocumentRelationship is a relationship between two Document objects.</rdfs:comment>
        <owl:versionInfo>1</owl:versionInfo>
        <skos:changeNote>[2021-07-30] Initial definition.</skos:changeNote>
        <skos:prefLabel xml:lang="en">document relationship</skos:prefLabel>
    </owl:Class>
    


    <!-- http://standards.iso.org/iso/10303/tech/refdata/core#97ef9a70-130a-0135-b552-598f1b1392ae -->

    <owl:Class rdf:about="http://standards.iso.org/iso/10303/tech/refdata/core#97ef9a70-130a-0135-b552-598f1b1392ae">
        <rdfs:subClassOf rdf:resource="http://standards.iso.org/iso/10303/tech/refdata/core#STEPThing"/>
        <dc:contributor>STEP Harmonization Team</dc:contributor>
        <dc:creator>Phil Spiby, Eurostep</dc:creator>
        <dc:date>2022-09-01</dc:date>
        <dc:source>ISO/TS 10303-4000</dc:source>
        <dc:type>InWork</dc:type>
        <rdfs:comment xml:lang="en">A DocumentVersion identifies a particular version of a Document.</rdfs:comment>
        <owl:versionInfo>1</owl:versionInfo>
        <skos:changeNote>[2021-07-30] Initial definition.</skos:changeNote>
        <skos:prefLabel xml:lang="en">document version</skos:prefLabel>
    </owl:Class>
    


    <!-- http://standards.iso.org/iso/10303/tech/refdata/core#97323f9a-90c1-4f72-96e2-0f88ea0ee060 -->

    <owl:Class rdf:about="http://standards.iso.org/iso/10303/tech/refdata/core#97323f9a-90c1-4f72-96e2-0f88ea0ee060">
        <rdfs:subClassOf rdf:resource="http://standards.iso.org/iso/10303/tech/refdata/core#55105ef0-713f-409a-8306-fd8708d4ee3f"/>
        <dc:contributor>STEP Harmonization Team</dc:contributor>
        <dc:creator>Jean Brangé, AFNeT Services</dc:creator>
        <dc:date>2023-10-04</dc:date>
        <dc:source>ISO/TS 10303-4000</dc:source>
        <dc:type>InWork</dc:type>
        <rdfs:comment xml:lang="en">A SymmetryTolerance is a type of GeometricTolerance that is a constraint on the amount of deviation a toleranced element may have from being symmetrical to a datum. Any edge or (median) plane of the part must lie in a tolerance zone limited by two parallel lines or planes, symmetrically located with respect to a datum. Unless otherwise specified, the rules governing symmetry tolerance defined in ISO 1101 shall apply.</rdfs:comment>
        <owl:versionInfo>3</owl:versionInfo>
        <skos:changeNote>[2023-10-04] Jean Brangé, AFNeT Services: Initial definition.</skos:changeNote>
        <skos:note xml:lang="en">Alternatively symmetry tolerance can be used according to the specifications given in ASME Y14.5-2009.</skos:note>
        <skos:prefLabel xml:lang="en">symmetry tolerance</skos:prefLabel>
    </owl:Class>
    


    <!-- http://standards.iso.org/iso/10303/tech/refdata/core#97557d50-130a-0135-b552-598f1b1392ae -->

    <owl:Class rdf:about="http://standards.iso.org/iso/10303/tech/refdata/core#97557d50-130a-0135-b552-598f1b1392ae">
        <rdfs:subClassOf rdf:resource="http://standards.iso.org/iso/10303/tech/refdata/core#59b11220-3279-0135-b58f-598f1b1392ae"/>
        <dc:contributor>STEP Harmonization Team</dc:contributor>
        <dc:creator>Phil Spiby, Eurostep</dc:creator>
        <dc:date>2022-09-01</dc:date>
        <dc:source>ISO/TS 10303-4000</dc:source>
        <dc:type>InWork</dc:type>
        <rdfs:comment xml:lang="en">A DocumentDefinitionRelationship is a relationship between two DocumentDefinition objects.</rdfs:comment>
        <owl:versionInfo>1</owl:versionInfo>
        <skos:changeNote>[2021-07-30] Initial definition.</skos:changeNote>
        <skos:prefLabel xml:lang="en">document definition relationship</skos:prefLabel>
    </owl:Class>
    


    <!-- http://standards.iso.org/iso/10303/tech/refdata/core#98b47110-130a-0135-b552-598f1b1392ae -->

    <owl:Class rdf:about="http://standards.iso.org/iso/10303/tech/refdata/core#98b47110-130a-0135-b552-598f1b1392ae">
        <rdfs:subClassOf rdf:resource="http://standards.iso.org/iso/10303/tech/refdata/core#adfff300-130a-0135-b552-598f1b1392ae"/>
        <dc:contributor>STEP Harmonization Team</dc:contributor>
        <dc:creator>Phil Spiby, Eurostep</dc:creator>
        <dc:date>2022-09-01</dc:date>
        <dc:source>ISO/TS 10303-4000</dc:source>
        <dc:type>InWork</dc:type>
        <rdfs:comment xml:lang="en">A Duration is the definition of a period of time.</rdfs:comment>
        <owl:versionInfo>1</owl:versionInfo>
        <skos:changeNote>[2021-07-30] Initial definition.</skos:changeNote>
        <skos:prefLabel xml:lang="en">duration</skos:prefLabel>
    </owl:Class>
    


    <!-- http://standards.iso.org/iso/10303/tech/refdata/core#98575cf0-130a-0135-b552-598f1b1392ae -->

    <owl:Class rdf:about="http://standards.iso.org/iso/10303/tech/refdata/core#98575cf0-130a-0135-b552-598f1b1392ae">
        <rdfs:subClassOf rdf:resource="http://standards.iso.org/iso/10303/tech/refdata/core#59b11220-3279-0135-b58f-598f1b1392ae"/>
        <dc:contributor>STEP Harmonization Team</dc:contributor>
        <dc:creator>Phil Spiby, Eurostep</dc:creator>
        <dc:date>2022-09-01</dc:date>
        <dc:source>ISO/TS 10303-4000</dc:source>
        <dc:type>InWork</dc:type>
        <rdfs:comment xml:lang="en">A DocumentVersionRelationship is a relationship between two DocumentVersion objects.</rdfs:comment>
        <owl:versionInfo>1</owl:versionInfo>
        <skos:changeNote>[2021-07-30] Initial definition.</skos:changeNote>
        <skos:prefLabel xml:lang="en">document version relationship</skos:prefLabel>
    </owl:Class>
    


    <!-- http://standards.iso.org/iso/10303/tech/refdata/core#99d96910-130a-0135-b552-598f1b1392ae -->

    <owl:Class rdf:about="http://standards.iso.org/iso/10303/tech/refdata/core#99d96910-130a-0135-b552-598f1b1392ae">
        <rdfs:subClassOf rdf:resource="http://standards.iso.org/iso/10303/tech/refdata/core#59b11220-3279-0135-b58f-598f1b1392ae"/>
        <dc:contributor>STEP Harmonization Team</dc:contributor>
        <dc:creator>Phil Spiby, Eurostep</dc:creator>
        <dc:date>2022-09-01</dc:date>
        <dc:source>ISO/TS 10303-4000</dc:source>
        <dc:type>InWork</dc:type>
        <rdfs:comment xml:lang="en">An EffectivityRelationship is a relationship between two Effectivity objects. The meaning of the relationship is represented by the RelationType attribute.</rdfs:comment>
        <owl:versionInfo>1</owl:versionInfo>
        <skos:changeNote>[2021-07-30] Initial definition.</skos:changeNote>
        <skos:note xml:lang="en">Sometimes effectivity is not dependent on specific dates or serial numbers, but on the effectivity of other items. In this case end values are not instantiated but are derived via an EffectivityRelationship to the reference Effectivity.</skos:note>
        <skos:prefLabel xml:lang="en">effectivity relationship</skos:prefLabel>
    </owl:Class>
    


    <!-- http://standards.iso.org/iso/10303/tech/refdata/core#99130bd0-130a-0135-b552-598f1b1392ae -->

    <owl:Class rdf:about="http://standards.iso.org/iso/10303/tech/refdata/core#99130bd0-130a-0135-b552-598f1b1392ae">
        <rdfs:subClassOf rdf:resource="http://standards.iso.org/iso/10303/tech/refdata/core#STEPThing"/>
        <dc:contributor>STEP Harmonization Team</dc:contributor>
        <dc:creator>Phil Spiby, Eurostep</dc:creator>
        <dc:date>2022-09-01</dc:date>
        <dc:source>ISO/TS 10303-4000</dc:source>
        <dc:type>InWork</dc:type>
        <rdfs:comment xml:lang="en">An Effectivity is an identification of the valid use of an aspect of product data tracked by date, event, serial number or lot size. An Effectivity can &apos;inherit&apos; its interval from another Effectivity through an EffectivityRelationship with ./4_info_reqs_CommonResources.htm#EffectivityRelationship.RelationType RelationType &apos;inheritance effectivity relationship&apos;. If a &apos;start&apos; and no &apos;end&apos; is specified, the period is then added to &apos;start&apos; in order to get the actual &apos;end&apos; of the effectivity or ineffectivity.</rdfs:comment>
        <owl:versionInfo>2</owl:versionInfo>
        <skos:changeNote>[2021-07-30] Initial definition.</skos:changeNote>
        <skos:changeNote>[2022-09-01] Phil Spiby, Eurostep: updated comment updated note.</skos:changeNote>
        <skos:note xml:lang="en">An instance of Effectivity can define a period of ineffectivity or invalid use, if it is referred to by an instance of EffectivityAssignment with EffectivityIndication set to &apos;false&apos;.</skos:note>
        <skos:prefLabel xml:lang="en">effectivity</skos:prefLabel>
    </owl:Class>
    


    <!-- http://standards.iso.org/iso/10303/tech/refdata/core#9960085e-ce9b-4f94-8165-81289dc0c69c -->

    <owl:Class rdf:about="http://standards.iso.org/iso/10303/tech/refdata/core#9960085e-ce9b-4f94-8165-81289dc0c69c">
        <rdfs:subClassOf rdf:resource="http://standards.iso.org/iso/10303/tech/refdata/core#9fee6ad0-130a-0135-b552-598f1b1392ae"/>
        <dc:contributor>STEP Harmonization Team</dc:contributor>
        <dc:creator>Jean Brangé, AFNeT Services</dc:creator>
        <dc:date>2023-10-04</dc:date>
        <dc:source>ISO/TS 10303-4000</dc:source>
        <dc:type>InWork</dc:type>
        <rdfs:comment xml:lang="en">An InterpolatedConfigurationModel is a type of GeometricRepresentation that specifies a motion (forward analysis) of a Mechanism where the motion is defined by different states of the KinematicPairs at different parameter values or times.</rdfs:comment>
        <owl:versionInfo>3</owl:versionInfo>
        <skos:changeNote>[2023-10-04] Jean Brangé, AFNeT Services: Initial definition.</skos:changeNote>
        <skos:prefLabel xml:lang="en">interpolated configuration model</skos:prefLabel>
    </owl:Class>
    


    <!-- http://standards.iso.org/iso/10303/tech/refdata/core#9977c110-130a-0135-b552-598f1b1392ae -->

    <owl:Class rdf:about="http://standards.iso.org/iso/10303/tech/refdata/core#9977c110-130a-0135-b552-598f1b1392ae">
        <rdfs:subClassOf rdf:resource="http://standards.iso.org/iso/10303/tech/refdata/core#1cfca290-3279-0135-b58f-598f1b1392ae"/>
        <dc:contributor>STEP Harmonization Team</dc:contributor>
        <dc:creator>Phil Spiby, Eurostep</dc:creator>
        <dc:date>2022-09-01</dc:date>
        <dc:source>ISO/TS 10303-4000</dc:source>
        <dc:type>InWork</dc:type>
        <rdfs:comment xml:lang="en">An EffectivityAssignment is an assignment of an Effectivity to an item (specified by EffectivityAssignmentSelect) whose effectivity is controlled by the assigned Effectivity. The association of an Effectivity to product or activity data does not imply any statement concerning effectivity outside of the specified interval. The same applies in the absence of any AssignedEffectivity, that is, no statement concerning effectivity is implied.</rdfs:comment>
        <owl:versionInfo>1</owl:versionInfo>
        <skos:changeNote>[2021-07-30] Initial definition.</skos:changeNote>
        <skos:prefLabel xml:lang="en">effectivity assignment</skos:prefLabel>
    </owl:Class>
</rdf:RDF>



<!-- Generated by the OWL API (version 4.5.9.2019-02-01T07:24:44Z) https://github.com/owlcs/owlapi -->

